@prefix : <http://aida.kmi.open.ac.uk/ontology#> .
@prefix csos: <http://cso.kmi.open.ac.uk/schema/cso#> .
@prefix foaf: <http://xmlns.com/foaf/0.1/> .
@prefix orgz: <http://www.w3.org/ns/org#> .
@prefix owl: <http://www.w3.org/2002/07/owl#> .
@prefix rdf: <http://www.w3.org/1999/02/22-rdf-syntax-ns#> .
@prefix rdfs: <http://www.w3.org/2000/01/rdf-schema#> .


#################################################################
#    Object Properties
#################################################################

### http://aida.kmi.open.ac.uk/ontology#isInDimensionsWithId
:isInDimensionsWithId rdf:type owl:ObjectProperty ;
			   rdfs:domain :patent ;
			   rdfs:range  rdfs:Literal ;
			   rdfs:comment "We use this relation to indicate the id used in Dimensions database." ;
			   rdfs:label "is in dimensions with id"@en .
			   
###  http://aida.kmi.open.ac.uk/ontology#hasSyntacticTopic
:hasSyntacticTopic rdf:type owl:ObjectProperty ;
               rdfs:domain [ rdf:type owl:Class ; owl:unionOf( :paper :patent)] ;
               rdfs:range csos:Topic ;
               rdfs:comment "We use this relation to indicate the syntactic topics identified in a paper." ;
               rdfs:label "has syntactic topic"@en .

###  http://aida.kmi.open.ac.uk/ontology#hasSemanticTopic
:hasSemanticTopic rdf:type owl:ObjectProperty ;
               rdfs:domain [ rdf:type owl:Class ; owl:unionOf( :paper :patent)] ;
               rdfs:range csos:Topic ;
               rdfs:comment "We use this relation to indicate the semantic topics identified in a paper." ;
               rdfs:label "has semantic topic"@en .

###  http://aida.kmi.open.ac.uk/ontology#hasTopic
:hasTopic rdf:type owl:ObjectProperty ;
               rdfs:domain [ rdf:type owl:Class ; owl:unionOf( :paper :patent)] ;
               rdfs:range csos:Topic ;
               rdfs:comment "We use this relation to indicate the topics identified in a paper (including syntactic and semantic)." ;
               rdfs:label "has topic"@en .

###  http://aida.kmi.open.ac.uk/ontology#hasAffiliationType
:hasAffiliationType rdf:type owl:ObjectProperty ;
               rdfs:domain :paper ;
               rdfs:range rdfs:Literal  ;
               rdfs:comment "We use this relation to indicate the type of the paper: academia, industry, collaborative." ;
               rdfs:label "has affiliation type"@en .

###  http://aida.kmi.open.ac.uk/ontology#hasOriginalAssigneeType
:hasOriginalAssigneeType rdf:type owl:ObjectProperty ;
               rdfs:domain :patent ;
               rdfs:range rdfs:Literal  ;
               rdfs:comment "We use this relation to indicate the type of the original assignee: academia, industry, collaborative." ;
               rdfs:label "has affiliation type"@en .

###  http://aida.kmi.open.ac.uk/ontology#hasCurrentAssigneeType
:hasCurrentAssigneeType rdf:type owl:ObjectProperty ;
               rdfs:domain :patent ;
               rdfs:range rdfs:Literal  ;
               rdfs:comment "We use this relation to indicate the type of the current assignee: academia, industry, collaborative." ;
               rdfs:label "has affiliation type"@en .

###  http://aida.kmi.open.ac.uk/ontology#hasAssigneeGridType
:hasAssigneeGridType rdf:type owl:ObjectProperty ;
               rdfs:domain :patent ;
               rdfs:range rdfs:Literal  ;
               rdfs:comment "We use this relation to indicate the type of the assignee according to the GRID classification: Education, Company, Government, Non-profit and others." ;
               rdfs:label "has affiliation type"@en .

###  http://aida.kmi.open.ac.uk/ontology#hasGridType
:hasGridType rdf:type owl:ObjectProperty ;
               rdfs:domain :affiliation ;
               rdfs:range rdfs:Literal ;
               rdfs:comment "We use this relation to indicate the type of the affiliation according to the GRID classification: Education, Company, Government, Non-profit and others." ;
               rdfs:label "has grid type"@en .

###  http://aida.kmi.open.ac.uk/ontology#hasPercentageOfAcademy
:hasPercentageOfAcademy rdf:type owl:ObjectProperty ;
               rdfs:domain :paper ;
               rdfs:range rdfs:Literal ;
               rdfs:comment "We use this relation to indicate the percentage of authors who authored this paper, and belong to academia." ;
               rdfs:label "has percentage of academy"@en .


###  http://aida.kmi.open.ac.uk/ontology#hasPercentageOfAcademy
:hasPercentageOfIndustry rdf:type owl:ObjectProperty ;
               rdfs:domain :paper ;
               rdfs:range rdfs:Literal ;
               rdfs:comment "We use this relation to indicate the percentage of authors who authored this paper, and belong to industry." ;
               rdfs:label "has percentage of industry"@en .
               
###  http://aida.kmi.open.ac.uk/ontology#hasIndustrialSector
:hasIndustrialSector rdf:type owl:ObjectProperty ;
               rdfs:domain [ rdf:type owl:Class ; owl:unionOf( :paper :patent :affiliation)] ;
               rdfs:range  :industrialSector ;
               rdfs:comment "We use this relation to indicate the industrial sector of affiliation." ;
               rdfs:label "has industrial category"@en .

###  http://aida.kmi.open.ac.uk/ontology#hasDBpediaCategory
:hasDBpediaCategory rdf:type owl:Objectproperty ;
			   rdfs:domain [ rdf:type owl:Class ; owl:unionOf( :paper :patent :affiliation)] ;
               rdfs:range  :DBpediaCategory ;
               rdfs:comment "We use this relation to indicate the industrial sector given by DBpedia in About:Property and About:Industry ." ;
               rdfs:label "classified by DBpedia as"@en .

#################################################################
#    Classes
#################################################################

###  http://aida.kmi.open.ac.uk/ontology#paper
:paper rdf:type owl:Class ;
       rdfs:subClassOf owl:Thing .

###  http://aida.kmi.open.ac.uk/ontology#patent
:patent rdf:type owl:Class ;
       rdfs:subClassOf owl:Thing .

###  http://aida.kmi.open.ac.uk/ontology#author
:author rdf:type owl:Class ;
       rdfs:subClassOf foaf:Agent .

###  http://aida.kmi.open.ac.uk/ontology#affiliation
:affiliation rdf:type owl:Class ;
       rdfs:subClassOf orgz:Organization .

### http://aida.kmi.open.ac.uk/ontology#industrialSector
:industrialSector rdf:type owl:Class ;
	   rdfs:subClassOf owl:Thing .

### http://aida.kmi.open.ac.uk/ontology#DBpediaCategory
:DBpediaCategory rdf:type owl:Class ;
	   rdfs:comment "This class is populated by all the categories that we inferred from DBpedia. As some of them are literals we created a class.";
	   rdfs:subClassOf owl:Thing .


