<?xml version="1.0"?>
<rdf:RDF xmlns="http://xworks.gr/ontologies/ccso#"
     xml:base="http://xworks.gr/ontologies/ccso"
     xmlns:schema="http://schema.org/"
     xmlns:CCSO="http://www.semanticweb.org/vkreations/ontologies/2017/CCSO#"
     xmlns:ns="http://www.w3.org/2003/06/sw-vocab-status/ns#"
     xmlns:owl="http://www.w3.org/2002/07/owl#"
     xmlns:swrlb="http://www.w3.org/2003/11/swrlb#"
     xmlns:swrl="http://www.w3.org/2003/11/swrl#"
     xmlns:xsd="http://www.w3.org/2001/XMLSchema#"
     xmlns:skos="http://www.w3.org/2004/02/skos/core#"
     xmlns:rdfs="http://www.w3.org/2000/01/rdf-schema#"
     xmlns:ccso="http://xworks.gr/ontologies/ccso#"
     xmlns:rdf="http://www.w3.org/1999/02/22-rdf-syntax-ns#"
     xmlns:xml="http://www.w3.org/XML/1998/namespace"
     xmlns:foaf="http://xmlns.com/foaf/0.1/"
     xmlns:dc="http://purl.org/dc/elements/1.1/">
    <owl:Ontology rdf:about="http://xworks.gr/ontologies/ccso">
        <owl:versionInfo rdf:datatype="http://www.w3.org/2001/XMLSchema#decimal">0.6</owl:versionInfo>
        <rdfs:comment xml:lang="en">This Ontology aims to provide data model for describing the subjects of Curriculum, Course and Syllabus in Higher education.</rdfs:comment>
        <CCSO:provider xml:lang="en">mailto:evskg@sch.gr</CCSO:provider>
        <rdfs:label xml:lang="en">Curriculum Course Syllabus Ontology (CCSO)</rdfs:label>
        <owl:versionInfo rdf:datatype="http://www.w3.org/2001/XMLSchema#string">Changes in 0.31 from priorVersion 0.30:
1. Addition of some Disjoints between various types of ProgramofStudy, Events and Persons
2. Addition of numerous Data properties in classes ProgramofStudy, EducationalOrganization, Syllabus.
3. Addition of some Restrictions.
4. Addition of class Employee.
5. Addition of class Publication.
6. Fixes in the hierarchy of EducationalOrganization subtree  (using belongsTo relationship).
7. Fixes in the hierarchy of FieldofStudy subtree (using partOf relationship).
8. Addition of Instances
9. Addition of Rules
10. Addition of DC-Elements properties in classes Publications &amp; LearningMaterial.

Changes in 0.4 from 0.3:
1. Change the ontology URI to a permanentURI:
http://purl.org/net/CCSO
2. Change the ontology URI to a permanentURI:
http://xworks.gr/ontologies/ccso
3. Correct some pitfalls detected by OOPS

Changes to 0.5 from 0.4:
1. Merge classes Publication &amp; LearningMaterial into Resource
2. Tests with SPAQL Queries based on Competency Questions

Changes to 0.6 from 0.5:
1. Replace Students names with Greek names.</owl:versionInfo>
        <rdfs:comment xml:lang="gr">Αυτή η Οντολογία στοχεύει αποσκοπεί στη δημιουργία ενός μοντέλου δεδομένων για την περιγραφή των πλαισίων του Προγράμματος Σπουδών, του Μαθήματος και του Περιγράμματος Μαθήματος στην Τριτοβάθμια εκπαίδευση.</rdfs:comment>
    </owl:Ontology>
    


    <!-- 
    ///////////////////////////////////////////////////////////////////////////////////////
    //
    // Annotation properties
    //
    ///////////////////////////////////////////////////////////////////////////////////////
     -->

    


    <!-- http://www.w3.org/2003/06/sw-vocab-status/ns#term_status -->

    <owl:AnnotationProperty rdf:about="http://www.w3.org/2003/06/sw-vocab-status/ns#term_status"/>
    


    <!-- http://www.w3.org/2004/02/skos/core#altLabel -->

    <owl:AnnotationProperty rdf:about="http://www.w3.org/2004/02/skos/core#altLabel"/>
    


    <!-- 
    ///////////////////////////////////////////////////////////////////////////////////////
    //
    // Datatypes
    //
    ///////////////////////////////////////////////////////////////////////////////////////
     -->

    


    <!-- http://www.w3.org/2001/XMLSchema#date -->

    <rdfs:Datatype rdf:about="http://www.w3.org/2001/XMLSchema#date"/>
    


    <!-- http://www.w3.org/2001/XMLSchema#duration -->

    <rdfs:Datatype rdf:about="http://www.w3.org/2001/XMLSchema#duration"/>
    


    <!-- internal:anonymous-constants -->

    <rdfs:Datatype rdf:about="internal:anonymous-constants"/>
    


    <!-- 
    ///////////////////////////////////////////////////////////////////////////////////////
    //
    // Object Properties
    //
    ///////////////////////////////////////////////////////////////////////////////////////
     -->

    


    <!-- http://purl.org/dc/elements/1.1/contributor -->

    <owl:ObjectProperty rdf:about="http://purl.org/dc/elements/1.1/contributor">
        <rdfs:domain rdf:resource="http://xworks.gr/ontologies/ccso#Resource"/>
        <rdfs:range rdf:resource="http://xmlns.com/foaf/0.1/Person"/>
        <rdfs:comment xml:lang="en">An entity responsible for making contributions to the resource.
Examples of a Contributor include a person, an organization, or a service. Typically, the name of a Contributor should be used to indicate the entity.</rdfs:comment>
        <rdfs:comment xml:lang="gr">Μία οντότητα που είναι υπεύθυνη στο να συνεισφέρει στην πηγή. 
Παραδείγματα συνεισφοράς μπορεί να περιλαμβάνουν ένα άτομο, έναν οργανισμό, ή μία υπηρεσία. Τυπικά, το όνομα αυτού που συνεισφέρει θα πρέπει να χρησιμοποιείται για να υποδείξει την οντότητα.</rdfs:comment>
    </owl:ObjectProperty>
    


    <!-- http://purl.org/dc/elements/1.1/creator -->

    <owl:ObjectProperty rdf:about="http://purl.org/dc/elements/1.1/creator">
        <owl:inverseOf rdf:resource="http://xworks.gr/ontologies/ccso#hasPublication"/>
        <rdf:type rdf:resource="http://www.w3.org/2002/07/owl#AsymmetricProperty"/>
        <rdf:type rdf:resource="http://www.w3.org/2002/07/owl#IrreflexiveProperty"/>
        <rdfs:domain rdf:resource="http://xworks.gr/ontologies/ccso#Resource"/>
        <rdfs:range rdf:resource="http://xmlns.com/foaf/0.1/Person"/>
        <rdfs:comment xml:lang="en">An entity primarily responsible for making the resource.
Examples of a Creator include a person, an organization, or a service. Typically, the name of a Creator should be used to indicate the entity.
Here is used to indicate the Author of a work.</rdfs:comment>
        <rdfs:comment xml:lang="gr">Μία οντότητα που πρωταρχικά είναι υπεύθυνη για το σχεδιασμό/δημιουργία της πηγής. 
Παραδείγματα Δημιουργού περιλαμβάνουν ένα άτομο, έναν οργανισμό, ή μία υπηρεσία. Τυπικά, το όνομα αυτού που δημιουργεί πρέπει να χρησιμοποιείται προκειμένου να υποδείξει την οντότητα. Στην προκειμένη περίπτωση χρησιμοποιείται για να υποδείξει τον Συντάκτη ενός έργου.</rdfs:comment>
    </owl:ObjectProperty>
    


    <!-- http://xworks.gr/ontologies/ccso#acquiredInCourse -->

    <owl:ObjectProperty rdf:about="http://xworks.gr/ontologies/ccso#acquiredInCourse">
        <owl:inverseOf rdf:resource="http://xworks.gr/ontologies/ccso#aimsToLO"/>
        <rdf:type rdf:resource="http://www.w3.org/2002/07/owl#AsymmetricProperty"/>
        <rdf:type rdf:resource="http://www.w3.org/2002/07/owl#IrreflexiveProperty"/>
        <rdfs:domain rdf:resource="http://xworks.gr/ontologies/ccso#LearningOutcome"/>
        <rdfs:range rdf:resource="http://xworks.gr/ontologies/ccso#Syllabus"/>
        <rdfs:comment xml:lang="en">A Learning Outcome may expected to be acquired in various Courses.</rdfs:comment>
        <rdfs:comment xml:lang="gr">Ένα Μαθησιακό Αποτέλεσμα αναμένεται να αποκτηθεί σε διάφορα Μαθήματα (Courses).</rdfs:comment>
    </owl:ObjectProperty>
    


    <!-- http://xworks.gr/ontologies/ccso#affiliatedWith -->

    <owl:ObjectProperty rdf:about="http://xworks.gr/ontologies/ccso#affiliatedWith">
        <rdfs:comment xml:lang="en">Super-property of some object properties that represents any kind of affiliation relation between the following classes: EducationalOrganization, Person, ProgramofStudy, Course, Event</rdfs:comment>
        <rdfs:comment xml:lang="gr">Υπερ-ιδιότητα ιδιοτήτων κάποιων αντικειμένων που αναπαριστά κάθε είδους σχέση ένταξης μεταξύ των εξής κλάσεων: EducationalOrganization, Person, ProgramofStudy, Course, Event</rdfs:comment>
    </owl:ObjectProperty>
    


    <!-- http://xworks.gr/ontologies/ccso#aimsToLO -->

    <owl:ObjectProperty rdf:about="http://xworks.gr/ontologies/ccso#aimsToLO">
        <rdf:type rdf:resource="http://www.w3.org/2002/07/owl#AsymmetricProperty"/>
        <rdf:type rdf:resource="http://www.w3.org/2002/07/owl#IrreflexiveProperty"/>
        <rdfs:domain rdf:resource="http://xworks.gr/ontologies/ccso#Syllabus"/>
        <rdfs:range rdf:resource="http://xworks.gr/ontologies/ccso#LearningOutcome"/>
        <rdfs:comment xml:lang="en">A Course may aim to several Learning Outcomes in connection with the covered Topics.</rdfs:comment>
        <rdfs:comment xml:lang="gr">Ένα Μάθημα μπορεί να στοχεύει σε διάφορα Μαθησιακά Αποτελέσματα σε σχέση με τα Αντικείμενα που καλύπτει.</rdfs:comment>
    </owl:ObjectProperty>
    


    <!-- http://xworks.gr/ontologies/ccso#alumnusOf -->

    <owl:ObjectProperty rdf:about="http://xworks.gr/ontologies/ccso#alumnusOf">
        <rdfs:subPropertyOf rdf:resource="http://xworks.gr/ontologies/ccso#affiliatedWith"/>
        <rdfs:subPropertyOf>
            <rdf:Description>
                <owl:inverseOf rdf:resource="http://xworks.gr/ontologies/ccso#affiliatedWith"/>
            </rdf:Description>
        </rdfs:subPropertyOf>
        <owl:inverseOf rdf:resource="http://xworks.gr/ontologies/ccso#hasAlumnus"/>
        <rdf:type rdf:resource="http://www.w3.org/2002/07/owl#AsymmetricProperty"/>
        <rdf:type rdf:resource="http://www.w3.org/2002/07/owl#IrreflexiveProperty"/>
        <rdfs:domain rdf:resource="http://xmlns.com/foaf/0.1/Person"/>
        <rdfs:range rdf:resource="http://xworks.gr/ontologies/ccso#Department"/>
        <rdfs:comment xml:lang="en">A Person is Alumnus of a Department</rdfs:comment>
        <rdfs:comment xml:lang="gr">Ένα πρόσωπο  είναι Απόφοιτος ενός Τμήματος.</rdfs:comment>
    </owl:ObjectProperty>
    


    <!-- http://xworks.gr/ontologies/ccso#areaOfCourse -->

    <owl:ObjectProperty rdf:about="http://xworks.gr/ontologies/ccso#areaOfCourse">
        <owl:inverseOf rdf:resource="http://xworks.gr/ontologies/ccso#coversKA"/>
        <rdfs:domain rdf:resource="http://xworks.gr/ontologies/ccso#KnowledgeArea"/>
        <rdfs:range rdf:resource="http://xworks.gr/ontologies/ccso#Course"/>
        <rdfs:comment xml:lang="en">Knowledge Area is area of a Course</rdfs:comment>
        <rdfs:comment xml:lang="gr">Πεδίο Γνώσης είναι το πεδίο ενός Μαθήματος.</rdfs:comment>
    </owl:ObjectProperty>
    


    <!-- http://xworks.gr/ontologies/ccso#assistsInCourse -->

    <owl:ObjectProperty rdf:about="http://xworks.gr/ontologies/ccso#assistsInCourse">
        <rdfs:subPropertyOf rdf:resource="http://xworks.gr/ontologies/ccso#affiliatedWith"/>
        <rdfs:subPropertyOf>
            <rdf:Description>
                <owl:inverseOf rdf:resource="http://xworks.gr/ontologies/ccso#affiliatedWith"/>
            </rdf:Description>
        </rdfs:subPropertyOf>
        <owl:inverseOf rdf:resource="http://xworks.gr/ontologies/ccso#hasCourseAssistant"/>
        <rdfs:domain rdf:resource="http://xworks.gr/ontologies/ccso#Assistant"/>
        <rdfs:range rdf:resource="http://xworks.gr/ontologies/ccso#Syllabus"/>
        <owl:propertyDisjointWith rdf:resource="http://xworks.gr/ontologies/ccso#attendsCourse"/>
        <owl:propertyDisjointWith rdf:resource="http://xworks.gr/ontologies/ccso#instructorOf"/>
        <owl:propertyDisjointWith rdf:resource="http://xworks.gr/ontologies/ccso#supervisorOf"/>
        <rdfs:comment xml:lang="en">An Assistant is (Teaching) Assistant in a Course.</rdfs:comment>
        <rdfs:comment xml:lang="gr">Ένας Βοηθός είναι Βοηθός (Διδάσκων) σε ένα Μάθημα.</rdfs:comment>
    </owl:ObjectProperty>
    


    <!-- http://xworks.gr/ontologies/ccso#assistsInEvent -->

    <owl:ObjectProperty rdf:about="http://xworks.gr/ontologies/ccso#assistsInEvent">
        <rdfs:subPropertyOf rdf:resource="http://xworks.gr/ontologies/ccso#affiliatedWith"/>
        <rdfs:subPropertyOf>
            <rdf:Description>
                <owl:inverseOf rdf:resource="http://xworks.gr/ontologies/ccso#affiliatedWith"/>
            </rdf:Description>
        </rdfs:subPropertyOf>
        <owl:inverseOf rdf:resource="http://xworks.gr/ontologies/ccso#hasEventAssistant"/>
        <rdfs:domain rdf:resource="http://xworks.gr/ontologies/ccso#Assistant"/>
        <rdfs:range rdf:resource="http://xworks.gr/ontologies/ccso#Event"/>
        <rdfs:comment xml:lang="en">An Assistant may assists in a teaching event, an evaluation event or some other stuff and events.</rdfs:comment>
        <rdfs:comment xml:lang="gr">Ένας Βοηθός μπορεί να βοηθάει στη διδαασκαλία, στην αξιολόγηση ή σε άλλα πεδία και γεγονότα.</rdfs:comment>
    </owl:ObjectProperty>
    


    <!-- http://xworks.gr/ontologies/ccso#attendsCourse -->

    <owl:ObjectProperty rdf:about="http://xworks.gr/ontologies/ccso#attendsCourse">
        <rdfs:subPropertyOf rdf:resource="http://xworks.gr/ontologies/ccso#affiliatedWith"/>
        <rdfs:subPropertyOf>
            <rdf:Description>
                <owl:inverseOf rdf:resource="http://xworks.gr/ontologies/ccso#affiliatedWith"/>
            </rdf:Description>
        </rdfs:subPropertyOf>
        <owl:inverseOf rdf:resource="http://xworks.gr/ontologies/ccso#hasAttender"/>
        <rdf:type rdf:resource="http://www.w3.org/2002/07/owl#AsymmetricProperty"/>
        <rdf:type rdf:resource="http://www.w3.org/2002/07/owl#IrreflexiveProperty"/>
        <rdfs:domain rdf:resource="http://xworks.gr/ontologies/ccso#Student"/>
        <rdfs:range rdf:resource="http://xworks.gr/ontologies/ccso#Course"/>
        <owl:propertyDisjointWith rdf:resource="http://xworks.gr/ontologies/ccso#hasCompleted"/>
        <owl:propertyDisjointWith rdf:resource="http://xworks.gr/ontologies/ccso#instructorOf"/>
        <rdfs:comment xml:lang="en">A Student attends some Courses of a study program.</rdfs:comment>
        <rdfs:comment xml:lang="gr">Ένας Φοιτητής παρακολουθεί κάποια Μαθήματα σε ένα πρόγραμμα σπουδών.</rdfs:comment>
    </owl:ObjectProperty>
    


    <!-- http://xworks.gr/ontologies/ccso#belongsTo -->

    <owl:ObjectProperty rdf:about="http://xworks.gr/ontologies/ccso#belongsTo">
        <rdf:type rdf:resource="http://www.w3.org/2002/07/owl#TransitiveProperty"/>
        <rdfs:domain rdf:resource="http://schema.org/EducationalOrganization"/>
        <rdfs:range rdf:resource="http://schema.org/EducationalOrganization"/>
        <rdfs:comment xml:lang="en">School belongsTo University.
Department belongsTo School.</rdfs:comment>
        <rdfs:comment xml:lang="gr">Η Σχολή ανήκει στο Τμήμα.
Το Τμήμα ανήκει στη Σχολή.</rdfs:comment>
    </owl:ObjectProperty>
    


    <!-- http://xworks.gr/ontologies/ccso#coveredInCourse -->

    <owl:ObjectProperty rdf:about="http://xworks.gr/ontologies/ccso#coveredInCourse">
        <owl:inverseOf rdf:resource="http://xworks.gr/ontologies/ccso#coversTopic"/>
        <rdf:type rdf:resource="http://www.w3.org/2002/07/owl#AsymmetricProperty"/>
        <rdf:type rdf:resource="http://www.w3.org/2002/07/owl#IrreflexiveProperty"/>
        <rdfs:domain rdf:resource="http://xworks.gr/ontologies/ccso#Topic"/>
        <rdfs:range rdf:resource="http://xworks.gr/ontologies/ccso#Syllabus"/>
        <rdfs:comment xml:lang="en">A Topic may be covered in several Courses included in different ProgramofStudies.</rdfs:comment>
        <rdfs:comment xml:lang="gr">Ένα Θέμα μπορεί να καλύπτεται σε διάφορα Μαθήματα, ακόμα και σε διαφορετικά Προγράμματα Σπουδών.</rdfs:comment>
    </owl:ObjectProperty>
    


    <!-- http://xworks.gr/ontologies/ccso#coversKA -->

    <owl:ObjectProperty rdf:about="http://xworks.gr/ontologies/ccso#coversKA">
        <rdfs:domain rdf:resource="http://xworks.gr/ontologies/ccso#Course"/>
        <rdfs:range rdf:resource="http://xworks.gr/ontologies/ccso#KnowledgeArea"/>
        <rdfs:comment xml:lang="en">Course covers part of a Knowledge Area</rdfs:comment>
        <rdfs:comment xml:lang="gr">Ένα Μάθημα καλύπτει ένα Πεδίο Γνώσης.</rdfs:comment>
    </owl:ObjectProperty>
    


    <!-- http://xworks.gr/ontologies/ccso#coversTopic -->

    <owl:ObjectProperty rdf:about="http://xworks.gr/ontologies/ccso#coversTopic">
        <rdf:type rdf:resource="http://www.w3.org/2002/07/owl#AsymmetricProperty"/>
        <rdf:type rdf:resource="http://www.w3.org/2002/07/owl#IrreflexiveProperty"/>
        <rdfs:domain rdf:resource="http://xworks.gr/ontologies/ccso#Syllabus"/>
        <rdfs:range rdf:resource="http://xworks.gr/ontologies/ccso#Topic"/>
        <rdfs:comment xml:lang="en">A Course may Cover several Topics. 
The coverage of a Topic is depending from how many hours are being taught; A national or international curriculum guide of the Body of Knowledge can provide information about the coverage, the learning outcomes and the minimum hours.</rdfs:comment>
        <rdfs:comment xml:lang="gr">Ένα Μάθημα μπορεί να καλύπτει διάφορα Θέματα. 
Αυτή η κάλυψη εξαρτάται από το πόσες ώρες διδάσκονται. Ένας εθνικός ή διεθνής οδηγός πρόγραμματος σπουδών για το Βασικό Κορμό της Γνώσης μπορεί να δώσει πληροφορίες σχετικά με το πεδίο που καλύπτει, τα μαθησιακά αποτελέσματα και τις ελάχιστες ώρες διδασκαλίας.</rdfs:comment>
    </owl:ObjectProperty>
    


    <!-- http://xworks.gr/ontologies/ccso#enrolledIn -->

    <owl:ObjectProperty rdf:about="http://xworks.gr/ontologies/ccso#enrolledIn">
        <rdfs:subPropertyOf rdf:resource="http://xworks.gr/ontologies/ccso#affiliatedWith"/>
        <rdfs:subPropertyOf>
            <rdf:Description>
                <owl:inverseOf rdf:resource="http://xworks.gr/ontologies/ccso#affiliatedWith"/>
            </rdf:Description>
        </rdfs:subPropertyOf>
        <owl:inverseOf rdf:resource="http://xworks.gr/ontologies/ccso#hasRegistered"/>
        <rdf:type rdf:resource="http://www.w3.org/2002/07/owl#AsymmetricProperty"/>
        <rdf:type rdf:resource="http://www.w3.org/2002/07/owl#IrreflexiveProperty"/>
        <rdfs:domain rdf:resource="http://xworks.gr/ontologies/ccso#Student"/>
        <rdfs:range rdf:resource="http://xworks.gr/ontologies/ccso#ProgramofStudy"/>
        <owl:propertyDisjointWith rdf:resource="http://xworks.gr/ontologies/ccso#hasDegree"/>
        <rdfs:comment xml:lang="en">A Student is enrolled (registered) in a Study Program.</rdfs:comment>
        <rdfs:comment xml:lang="gr">Ένας Φοιτητής είναι εγγεγραμμένος σε ένα Πρόγραμμα Σπουδών.</rdfs:comment>
    </owl:ObjectProperty>
    


    <!-- http://xworks.gr/ontologies/ccso#expectsLO -->

    <owl:ObjectProperty rdf:about="http://xworks.gr/ontologies/ccso#expectsLO">
        <rdf:type rdf:resource="http://www.w3.org/2002/07/owl#AsymmetricProperty"/>
        <rdf:type rdf:resource="http://www.w3.org/2002/07/owl#IrreflexiveProperty"/>
        <rdfs:domain rdf:resource="http://xworks.gr/ontologies/ccso#TeachingEvent"/>
        <rdfs:range rdf:resource="http://xworks.gr/ontologies/ccso#LearningOutcome"/>
        <rdfs:comment xml:lang="en">A Teaching Event expects (aims to) one or more Learning Outcomes for the students.</rdfs:comment>
        <rdfs:comment xml:lang="gr">Μία Διδασκαλία αναμένεται να φέρει ένα ή περισσότερα Μαθησιακά Αποτελέσματα στοyς Φοιτητές.</rdfs:comment>
    </owl:ObjectProperty>
    


    <!-- http://xworks.gr/ontologies/ccso#focusIn -->

    <owl:ObjectProperty rdf:about="http://xworks.gr/ontologies/ccso#focusIn">
        <rdf:type rdf:resource="http://www.w3.org/2002/07/owl#AsymmetricProperty"/>
        <rdf:type rdf:resource="http://www.w3.org/2002/07/owl#IrreflexiveProperty"/>
        <rdfs:domain rdf:resource="http://xworks.gr/ontologies/ccso#ProgramofStudy"/>
        <rdfs:range rdf:resource="http://xworks.gr/ontologies/ccso#KnowledgeBody"/>
        <rdfs:comment xml:lang="en">A Study Program is focused in a Body of Knowledge, at least.</rdfs:comment>
        <rdfs:comment xml:lang="gr">Ένα Πρόγραμμα Σπουδών στοχεύει τουλάχιστον σε έναν Βασικό Κορμό Γνώσης.</rdfs:comment>
    </owl:ObjectProperty>
    


    <!-- http://xworks.gr/ontologies/ccso#followsTEMethod -->

    <owl:ObjectProperty rdf:about="http://xworks.gr/ontologies/ccso#followsTEMethod">
        <rdf:type rdf:resource="http://www.w3.org/2002/07/owl#AsymmetricProperty"/>
        <rdf:type rdf:resource="http://www.w3.org/2002/07/owl#IrreflexiveProperty"/>
        <rdfs:domain>
            <owl:Class>
                <owl:unionOf rdf:parseType="Collection">
                    <rdf:Description rdf:about="http://xworks.gr/ontologies/ccso#EvaluationEvent"/>
                    <rdf:Description rdf:about="http://xworks.gr/ontologies/ccso#Syllabus"/>
                    <rdf:Description rdf:about="http://xworks.gr/ontologies/ccso#TeachingEvent"/>
                </owl:unionOf>
            </owl:Class>
        </rdfs:domain>
        <rdfs:range rdf:resource="http://xworks.gr/ontologies/ccso#TeachingEvaluationMethod"/>
        <rdfs:comment xml:lang="en">An Event in the classroom follows one or more Teaching Methods or either Evaluation Methods.</rdfs:comment>
        <rdfs:comment xml:lang="gr">Ένα Γεγονός στην τάξη ακολουθεί μία ή περισσότερες Διδακτικές Μεθόδους ή διάφορες Μεθόδους Αξιολόγησης.</rdfs:comment>
    </owl:ObjectProperty>
    


    <!-- http://xworks.gr/ontologies/ccso#hasAcademicStaff -->

    <owl:ObjectProperty rdf:about="http://xworks.gr/ontologies/ccso#hasAcademicStaff">
        <rdfs:subPropertyOf rdf:resource="http://xworks.gr/ontologies/ccso#affiliatedWith"/>
        <rdfs:subPropertyOf>
            <rdf:Description>
                <owl:inverseOf rdf:resource="http://xworks.gr/ontologies/ccso#affiliatedWith"/>
            </rdf:Description>
        </rdfs:subPropertyOf>
        <owl:inverseOf rdf:resource="http://xworks.gr/ontologies/ccso#memberOf"/>
        <rdfs:domain rdf:resource="http://xworks.gr/ontologies/ccso#Department"/>
        <rdfs:range rdf:resource="http://xworks.gr/ontologies/ccso#AcademicStaff"/>
        <rdfs:comment xml:lang="en">A Department has staff that is member of the Academic staff (known as Faculty also) like Professors, Researchers and Lecturers.</rdfs:comment>
        <rdfs:comment xml:lang="gr">Ένα Τμήμα έχει προσωπικό που αποτελεί μέρος του Ακαδημαϊκού Προσωπικού όπως Καθηγητές, Ερευνητές και Εισηγητές.</rdfs:comment>
    </owl:ObjectProperty>
    


    <!-- http://xworks.gr/ontologies/ccso#hasAlumnus -->

    <owl:ObjectProperty rdf:about="http://xworks.gr/ontologies/ccso#hasAlumnus">
        <rdfs:subPropertyOf rdf:resource="http://xworks.gr/ontologies/ccso#affiliatedWith"/>
        <rdfs:subPropertyOf>
            <rdf:Description>
                <owl:inverseOf rdf:resource="http://xworks.gr/ontologies/ccso#affiliatedWith"/>
            </rdf:Description>
        </rdfs:subPropertyOf>
        <rdf:type rdf:resource="http://www.w3.org/2002/07/owl#AsymmetricProperty"/>
        <rdf:type rdf:resource="http://www.w3.org/2002/07/owl#IrreflexiveProperty"/>
        <rdfs:domain rdf:resource="http://xworks.gr/ontologies/ccso#Department"/>
        <rdfs:range rdf:resource="http://xmlns.com/foaf/0.1/Person"/>
        <rdfs:comment xml:lang="en">A Department has alumnus, a person who completed successfully a Program of Study.</rdfs:comment>
        <rdfs:comment xml:lang="gr">Ένα Τμήμα έχει Απόφοιτο, ένα άτομο που έχει ολοκληρώσει επιτυχώς το Πρόγραμμα Σπουδών.</rdfs:comment>
    </owl:ObjectProperty>
    


    <!-- http://xworks.gr/ontologies/ccso#hasAttender -->

    <owl:ObjectProperty rdf:about="http://xworks.gr/ontologies/ccso#hasAttender">
        <rdfs:subPropertyOf rdf:resource="http://xworks.gr/ontologies/ccso#affiliatedWith"/>
        <rdfs:subPropertyOf>
            <rdf:Description>
                <owl:inverseOf rdf:resource="http://xworks.gr/ontologies/ccso#affiliatedWith"/>
            </rdf:Description>
        </rdfs:subPropertyOf>
        <rdf:type rdf:resource="http://www.w3.org/2002/07/owl#AsymmetricProperty"/>
        <rdf:type rdf:resource="http://www.w3.org/2002/07/owl#IrreflexiveProperty"/>
        <rdfs:domain rdf:resource="http://xworks.gr/ontologies/ccso#Course"/>
        <rdfs:range rdf:resource="http://xworks.gr/ontologies/ccso#Student"/>
        <owl:propertyDisjointWith rdf:resource="http://xworks.gr/ontologies/ccso#hasCourseAssistant"/>
        <owl:propertyDisjointWith rdf:resource="http://xworks.gr/ontologies/ccso#hasInstructor"/>
        <owl:propertyDisjointWith rdf:resource="http://xworks.gr/ontologies/ccso#hasSupervisor"/>
        <rdfs:comment xml:lang="en">A Course has Student as Attender.</rdfs:comment>
        <rdfs:comment xml:lang="gr">Ένα Μάθημα έχει Φοιτητή ως Συμμετέχοντα.</rdfs:comment>
    </owl:ObjectProperty>
    


    <!-- http://xworks.gr/ontologies/ccso#hasCompleted -->

    <owl:ObjectProperty rdf:about="http://xworks.gr/ontologies/ccso#hasCompleted">
        <rdfs:subPropertyOf rdf:resource="http://xworks.gr/ontologies/ccso#affiliatedWith"/>
        <rdfs:domain rdf:resource="http://xworks.gr/ontologies/ccso#Student"/>
        <rdfs:range rdf:resource="http://xworks.gr/ontologies/ccso#Course"/>
        <rdfs:comment xml:lang="en">A Student who has successfully completed a Study Program or either a Course.</rdfs:comment>
        <rdfs:comment xml:lang="gr">Ένας Φοιτητής που έχει επιτυχώς ολοκληρώσει ένα Πρόγραμμα Σπουδών ή ένα Μάθημα.</rdfs:comment>
    </owl:ObjectProperty>
    


    <!-- http://xworks.gr/ontologies/ccso#hasCourseAssistant -->

    <owl:ObjectProperty rdf:about="http://xworks.gr/ontologies/ccso#hasCourseAssistant">
        <rdfs:subPropertyOf rdf:resource="http://xworks.gr/ontologies/ccso#affiliatedWith"/>
        <rdfs:subPropertyOf>
            <rdf:Description>
                <owl:inverseOf rdf:resource="http://xworks.gr/ontologies/ccso#affiliatedWith"/>
            </rdf:Description>
        </rdfs:subPropertyOf>
        <rdfs:domain rdf:resource="http://xworks.gr/ontologies/ccso#Syllabus"/>
        <rdfs:range rdf:resource="http://xworks.gr/ontologies/ccso#Assistant"/>
        <owl:propertyDisjointWith rdf:resource="http://xworks.gr/ontologies/ccso#hasInstructor"/>
        <owl:propertyDisjointWith rdf:resource="http://xworks.gr/ontologies/ccso#hasSupervisor"/>
        <rdfs:comment xml:lang="en">A Course has Assistant.</rdfs:comment>
        <rdfs:comment xml:lang="gr">Το Μάθημα έχει έναν Βοηθό.</rdfs:comment>
    </owl:ObjectProperty>
    


    <!-- http://xworks.gr/ontologies/ccso#hasDegree -->

    <owl:ObjectProperty rdf:about="http://xworks.gr/ontologies/ccso#hasDegree">
        <rdfs:subPropertyOf rdf:resource="http://xworks.gr/ontologies/ccso#affiliatedWith"/>
        <rdfs:domain rdf:resource="http://xmlns.com/foaf/0.1/Person"/>
        <rdfs:range rdf:resource="http://xworks.gr/ontologies/ccso#ProgramofStudy"/>
        <rdfs:comment xml:lang="en">Person has some Degrees from some Departments (e.g. Bachelor Degree, Master Degree, etc)</rdfs:comment>
        <rdfs:comment xml:lang="gr">Ένα πρόσωπο που έχει ολοκληρώσει επιτυχώς ένα πρόγραμμα Σπουδών και έχει λάβει τον Τίτλο Σπουδών.</rdfs:comment>
    </owl:ObjectProperty>
    


    <!-- http://xworks.gr/ontologies/ccso#hasDuration -->

    <owl:ObjectProperty rdf:about="http://xworks.gr/ontologies/ccso#hasDuration">
        <rdf:type rdf:resource="http://www.w3.org/2002/07/owl#AsymmetricProperty"/>
        <rdf:type rdf:resource="http://www.w3.org/2002/07/owl#IrreflexiveProperty"/>
        <rdfs:domain>
            <owl:Class>
                <owl:unionOf rdf:parseType="Collection">
                    <rdf:Description rdf:about="http://xworks.gr/ontologies/ccso#Course"/>
                    <rdf:Description rdf:about="http://xworks.gr/ontologies/ccso#ProgramofStudy"/>
                </owl:unionOf>
            </owl:Class>
        </rdfs:domain>
        <rdfs:range rdf:resource="http://xworks.gr/ontologies/ccso#DateTimeDuration"/>
        <rdfs:comment xml:lang="en">A Study Program or either a Course has some Duration in weeks, months or years.</rdfs:comment>
        <rdfs:comment xml:lang="gr">Ένα Πρόγραμμα Σπουδών ή ένα Μάθημα έχει Διάρκεια που ορίζεται σε εβδομάδες, μήνες ή χρόνια.</rdfs:comment>
    </owl:ObjectProperty>
    


    <!-- http://xworks.gr/ontologies/ccso#hasEmployee -->

    <owl:ObjectProperty rdf:about="http://xworks.gr/ontologies/ccso#hasEmployee">
        <rdfs:subPropertyOf rdf:resource="http://xworks.gr/ontologies/ccso#affiliatedWith"/>
        <owl:inverseOf rdf:resource="http://xworks.gr/ontologies/ccso#worksFor"/>
        <rdfs:domain rdf:resource="http://schema.org/EducationalOrganization"/>
        <rdfs:range rdf:resource="http://xworks.gr/ontologies/ccso#Employee"/>
        <rdfs:comment xml:lang="en">EducationalOrganization hasEmployee Employee</rdfs:comment>
        <rdfs:comment xml:lang="gr">Ένας Εκπαιδευτικός Οργανισμός έχει Απασχολούμενους.</rdfs:comment>
    </owl:ObjectProperty>
    


    <!-- http://xworks.gr/ontologies/ccso#hasEvent -->

    <owl:ObjectProperty rdf:about="http://xworks.gr/ontologies/ccso#hasEvent">
        <rdf:type rdf:resource="http://www.w3.org/2002/07/owl#AsymmetricProperty"/>
        <rdf:type rdf:resource="http://www.w3.org/2002/07/owl#IrreflexiveProperty"/>
        <rdfs:domain rdf:resource="http://xworks.gr/ontologies/ccso#Syllabus"/>
        <rdfs:range>
            <owl:Class>
                <owl:unionOf rdf:parseType="Collection">
                    <rdf:Description rdf:about="http://xworks.gr/ontologies/ccso#EvaluationEvent"/>
                    <rdf:Description rdf:about="http://xworks.gr/ontologies/ccso#TeachingEvent"/>
                </owl:unionOf>
            </owl:Class>
        </rdfs:range>
        <rdfs:comment xml:lang="en">A Course is composed of several Events; most of them are Teaching Events and some are Evaluation Events.</rdfs:comment>
        <rdfs:comment xml:lang="gr">Ένα Μάθημα αποτελείται από διάφορα Γεγονότα. Τα περισσότερα από αυτά είναι Διδακτικά Γεγονότα και κάποια από αυτά είναι Γεγονότα Αξιολόγησης.</rdfs:comment>
    </owl:ObjectProperty>
    


    <!-- http://xworks.gr/ontologies/ccso#hasEventAssistant -->

    <owl:ObjectProperty rdf:about="http://xworks.gr/ontologies/ccso#hasEventAssistant">
        <rdfs:subPropertyOf rdf:resource="http://xworks.gr/ontologies/ccso#affiliatedWith"/>
        <rdfs:subPropertyOf>
            <rdf:Description>
                <owl:inverseOf rdf:resource="http://xworks.gr/ontologies/ccso#affiliatedWith"/>
            </rdf:Description>
        </rdfs:subPropertyOf>
        <rdfs:domain rdf:resource="http://xworks.gr/ontologies/ccso#Event"/>
        <rdfs:range rdf:resource="http://xworks.gr/ontologies/ccso#Assistant"/>
        <rdfs:comment xml:lang="en">An Event may have one or more Assistants.</rdfs:comment>
        <rdfs:comment xml:lang="gr">Ένα Γεγονός μπορεί να έχει έναν ή παραπάνω Βοηθούς.</rdfs:comment>
    </owl:ObjectProperty>
    


    <!-- http://xworks.gr/ontologies/ccso#hasGrader -->

    <owl:ObjectProperty rdf:about="http://xworks.gr/ontologies/ccso#hasGrader">
        <rdfs:subPropertyOf rdf:resource="http://xworks.gr/ontologies/ccso#affiliatedWith"/>
        <rdf:type rdf:resource="http://www.w3.org/2002/07/owl#AsymmetricProperty"/>
        <rdf:type rdf:resource="http://www.w3.org/2002/07/owl#IrreflexiveProperty"/>
        <rdfs:domain rdf:resource="http://xworks.gr/ontologies/ccso#EvaluationEvent"/>
        <rdfs:range rdf:resource="http://xworks.gr/ontologies/ccso#Professor"/>
        <rdfs:comment xml:lang="en">An Evaluation Event can have at least one Professor as Grader.</rdfs:comment>
        <rdfs:comment xml:lang="gr">Ένα Γεγονός Αξιολόγησης μπορεί να έχει τουλάχιστον έναν Καθηγητή ως Βοθμολογητή.</rdfs:comment>
    </owl:ObjectProperty>
    


    <!-- http://xworks.gr/ontologies/ccso#hasInstructor -->

    <owl:ObjectProperty rdf:about="http://xworks.gr/ontologies/ccso#hasInstructor">
        <rdfs:subPropertyOf rdf:resource="http://xworks.gr/ontologies/ccso#affiliatedWith"/>
        <rdfs:subPropertyOf>
            <rdf:Description>
                <owl:inverseOf rdf:resource="http://xworks.gr/ontologies/ccso#affiliatedWith"/>
            </rdf:Description>
        </rdfs:subPropertyOf>
        <owl:inverseOf rdf:resource="http://xworks.gr/ontologies/ccso#instructorOf"/>
        <rdf:type rdf:resource="http://www.w3.org/2002/07/owl#AsymmetricProperty"/>
        <rdf:type rdf:resource="http://www.w3.org/2002/07/owl#IrreflexiveProperty"/>
        <rdfs:domain rdf:resource="http://xworks.gr/ontologies/ccso#Syllabus"/>
        <rdfs:range rdf:resource="http://xworks.gr/ontologies/ccso#Professor"/>
        <rdfs:comment xml:lang="en">A Course has one or more Professors as Instructors.</rdfs:comment>
        <rdfs:comment xml:lang="gr">Ένα Μάθημα έχει ένα ή παραπάνω Καθηγητές ως Εισηγητές.</rdfs:comment>
    </owl:ObjectProperty>
    


    <!-- http://xworks.gr/ontologies/ccso#hasLM -->

    <owl:ObjectProperty rdf:about="http://xworks.gr/ontologies/ccso#hasLM">
        <rdf:type rdf:resource="http://www.w3.org/2002/07/owl#AsymmetricProperty"/>
        <rdf:type rdf:resource="http://www.w3.org/2002/07/owl#IrreflexiveProperty"/>
        <rdfs:domain>
            <owl:Class>
                <owl:unionOf rdf:parseType="Collection">
                    <rdf:Description rdf:about="http://xworks.gr/ontologies/ccso#Event"/>
                    <rdf:Description rdf:about="http://xworks.gr/ontologies/ccso#Syllabus"/>
                </owl:unionOf>
            </owl:Class>
        </rdfs:domain>
        <rdfs:range rdf:resource="http://xworks.gr/ontologies/ccso#Resource"/>
        <rdfs:comment xml:lang="en">A Course may use several Resources as Learning Material.
An Event may use several Resources as Learning Material.</rdfs:comment>
        <rdfs:comment xml:lang="gr">Ένα Μάθημα χρησιμοποιεί έναν αριθμό Πηγών ως Μαθησιακό Υλικό.
Ένα Συμβάν Διδασκαλίας χρησιμοποιεί έναν αριθμό Πηγών ως Μαθησιακό Υλικό.</rdfs:comment>
    </owl:ObjectProperty>
    


    <!-- http://xworks.gr/ontologies/ccso#hasPrerequisite -->

    <owl:ObjectProperty rdf:about="http://xworks.gr/ontologies/ccso#hasPrerequisite">
        <rdf:type rdf:resource="http://www.w3.org/2002/07/owl#AsymmetricProperty"/>
        <rdf:type rdf:resource="http://www.w3.org/2002/07/owl#IrreflexiveProperty"/>
        <rdfs:domain rdf:resource="http://xworks.gr/ontologies/ccso#Course"/>
        <rdfs:range rdf:resource="http://xworks.gr/ontologies/ccso#Course"/>
        <rdfs:comment xml:lang="en">A Course may require previous knowledge from other Courses.</rdfs:comment>
        <rdfs:comment xml:lang="gr">Ένα Μάθημα μπορεί να απαιτεί γνώσεις από άλλα Μαθήματα.</rdfs:comment>
    </owl:ObjectProperty>
    


    <!-- http://xworks.gr/ontologies/ccso#hasPublication -->

    <owl:ObjectProperty rdf:about="http://xworks.gr/ontologies/ccso#hasPublication">
        <rdf:type rdf:resource="http://www.w3.org/2002/07/owl#AsymmetricProperty"/>
        <rdf:type rdf:resource="http://www.w3.org/2002/07/owl#IrreflexiveProperty"/>
        <rdfs:domain rdf:resource="http://www.w3.org/2000/10/swap/pim/contact#Person"/>
        <rdfs:range rdf:resource="http://xworks.gr/ontologies/ccso#Resource"/>
        <rdfs:comment xml:lang="en">A person creates and publishes a work.</rdfs:comment>
        <rdfs:comment xml:lang="gr">Ένα άτομο δημιουργεί και εκδίδει μία εργασία.</rdfs:comment>
    </owl:ObjectProperty>
    


    <!-- http://xworks.gr/ontologies/ccso#hasRegistered -->

    <owl:ObjectProperty rdf:about="http://xworks.gr/ontologies/ccso#hasRegistered">
        <rdfs:subPropertyOf rdf:resource="http://xworks.gr/ontologies/ccso#affiliatedWith"/>
        <rdfs:subPropertyOf>
            <rdf:Description>
                <owl:inverseOf rdf:resource="http://xworks.gr/ontologies/ccso#affiliatedWith"/>
            </rdf:Description>
        </rdfs:subPropertyOf>
        <rdf:type rdf:resource="http://www.w3.org/2002/07/owl#AsymmetricProperty"/>
        <rdf:type rdf:resource="http://www.w3.org/2002/07/owl#IrreflexiveProperty"/>
        <rdfs:domain rdf:resource="http://xworks.gr/ontologies/ccso#ProgramofStudy"/>
        <rdfs:range rdf:resource="http://xworks.gr/ontologies/ccso#Student"/>
        <rdfs:comment>A Study Program can have a lot of Students registered.</rdfs:comment>
        <rdfs:comment xml:lang="gr">Ένα Πρόγραμμα Σπουδών μπορεί έχει πολλούς εγγρεγραμμένους Φοιτητές.</rdfs:comment>
    </owl:ObjectProperty>
    


    <!-- http://xworks.gr/ontologies/ccso#hasSupervisor -->

    <owl:ObjectProperty rdf:about="http://xworks.gr/ontologies/ccso#hasSupervisor">
        <rdfs:subPropertyOf rdf:resource="http://xworks.gr/ontologies/ccso#affiliatedWith"/>
        <rdfs:subPropertyOf>
            <rdf:Description>
                <owl:inverseOf rdf:resource="http://xworks.gr/ontologies/ccso#affiliatedWith"/>
            </rdf:Description>
        </rdfs:subPropertyOf>
        <owl:inverseOf rdf:resource="http://xworks.gr/ontologies/ccso#supervisorOf"/>
        <rdf:type rdf:resource="http://www.w3.org/2002/07/owl#AsymmetricProperty"/>
        <rdf:type rdf:resource="http://www.w3.org/2002/07/owl#IrreflexiveProperty"/>
        <rdfs:domain rdf:resource="http://xworks.gr/ontologies/ccso#Syllabus"/>
        <rdfs:range rdf:resource="http://xworks.gr/ontologies/ccso#Professor"/>
        <rdfs:comment xml:lang="en">A Course can have a Professor as Supervisor who manages all the activities within a Course such as the design, the implementation, the lessons, the outcomes, etc.</rdfs:comment>
        <rdfs:comment xml:lang="gr">Ένα Μάθημα μπορεί να έχει έναν Καθηγητή ως Επιβλέπων ο οποίος διαχειρίζεται όλες τις δραστηριότητες στο Μάθημα όπως το σχεδιασμό, την εφαρμογή, τη διδασκαλία, τα αποτελέσματα κτλ.</rdfs:comment>
    </owl:ObjectProperty>
    


    <!-- http://xworks.gr/ontologies/ccso#hasSyllabus -->

    <owl:ObjectProperty rdf:about="http://xworks.gr/ontologies/ccso#hasSyllabus">
        <owl:inverseOf rdf:resource="http://xworks.gr/ontologies/ccso#syllabusOf"/>
        <rdfs:domain rdf:resource="http://xworks.gr/ontologies/ccso#Course"/>
        <rdfs:range rdf:resource="http://xworks.gr/ontologies/ccso#Syllabus"/>
        <rdfs:comment xml:lang="en">A  Course has Syllabus (maybe more).</rdfs:comment>
        <rdfs:comment xml:lang="gr">Ένα Μάθημα έχει ένα Περίγραμμα Σπουδών (μπορεί και περισσότερα).</rdfs:comment>
    </owl:ObjectProperty>
    


    <!-- http://xworks.gr/ontologies/ccso#hasTeacher -->

    <owl:ObjectProperty rdf:about="http://xworks.gr/ontologies/ccso#hasTeacher">
        <rdfs:subPropertyOf rdf:resource="http://xworks.gr/ontologies/ccso#affiliatedWith"/>
        <rdfs:subPropertyOf>
            <rdf:Description>
                <owl:inverseOf rdf:resource="http://xworks.gr/ontologies/ccso#affiliatedWith"/>
            </rdf:Description>
        </rdfs:subPropertyOf>
        <owl:inverseOf rdf:resource="http://xworks.gr/ontologies/ccso#teachesIn"/>
        <rdf:type rdf:resource="http://www.w3.org/2002/07/owl#AsymmetricProperty"/>
        <rdf:type rdf:resource="http://www.w3.org/2002/07/owl#IrreflexiveProperty"/>
        <rdfs:domain rdf:resource="http://xworks.gr/ontologies/ccso#TeachingEvent"/>
        <rdfs:range rdf:resource="http://xworks.gr/ontologies/ccso#Professor"/>
        <rdfs:comment xml:lang="en">A Teaching Event has one or more Professors as teachers.</rdfs:comment>
        <rdfs:comment xml:lang="gr">Μία Διδασκαλία έχει έναν ή παραπάνω Καθηγητές ως δάσκαλο.</rdfs:comment>
    </owl:ObjectProperty>
    


    <!-- http://xworks.gr/ontologies/ccso#hasTopic -->

    <owl:ObjectProperty rdf:about="http://xworks.gr/ontologies/ccso#hasTopic">
        <rdf:type rdf:resource="http://www.w3.org/2002/07/owl#AsymmetricProperty"/>
        <rdf:type rdf:resource="http://www.w3.org/2002/07/owl#IrreflexiveProperty"/>
        <rdfs:domain rdf:resource="http://xworks.gr/ontologies/ccso#TeachingEvent"/>
        <rdfs:range rdf:resource="http://xworks.gr/ontologies/ccso#Topic"/>
        <rdfs:comment xml:lang="en">A Teaching Event has one or more Topics.</rdfs:comment>
        <rdfs:comment xml:lang="gr">Μία Διδασκαλία έχει ένα ή περισσότερα Θέματα.</rdfs:comment>
    </owl:ObjectProperty>
    


    <!-- http://xworks.gr/ontologies/ccso#includedIn -->

    <owl:ObjectProperty rdf:about="http://xworks.gr/ontologies/ccso#includedIn">
        <owl:inverseOf rdf:resource="http://xworks.gr/ontologies/ccso#includesCourse"/>
        <rdf:type rdf:resource="http://www.w3.org/2002/07/owl#AsymmetricProperty"/>
        <rdf:type rdf:resource="http://www.w3.org/2002/07/owl#IrreflexiveProperty"/>
        <rdfs:domain rdf:resource="http://xworks.gr/ontologies/ccso#Course"/>
        <rdfs:range rdf:resource="http://xworks.gr/ontologies/ccso#ProgramofStudy"/>
        <rdfs:comment xml:lang="en">A Course can be included in various Study Programs.</rdfs:comment>
        <rdfs:comment xml:lang="gr">Ένα Μάθημα μπορεί να περιλαμβάνεται σε διάφορα Προγράμματα Σπουδών.</rdfs:comment>
    </owl:ObjectProperty>
    


    <!-- http://xworks.gr/ontologies/ccso#includesCourse -->

    <owl:ObjectProperty rdf:about="http://xworks.gr/ontologies/ccso#includesCourse">
        <rdf:type rdf:resource="http://www.w3.org/2002/07/owl#AsymmetricProperty"/>
        <rdf:type rdf:resource="http://www.w3.org/2002/07/owl#IrreflexiveProperty"/>
        <rdfs:domain rdf:resource="http://xworks.gr/ontologies/ccso#ProgramofStudy"/>
        <rdfs:range rdf:resource="http://xworks.gr/ontologies/ccso#Course"/>
        <rdfs:comment>A Study Program can includes many Courses.</rdfs:comment>
        <rdfs:comment xml:lang="gr">Ένα Πρόγραμμα Σπουδών μπορεί να περιλαμβάνει πολλά Μαθήματα.</rdfs:comment>
    </owl:ObjectProperty>
    


    <!-- http://xworks.gr/ontologies/ccso#instructorOf -->

    <owl:ObjectProperty rdf:about="http://xworks.gr/ontologies/ccso#instructorOf">
        <rdfs:subPropertyOf rdf:resource="http://xworks.gr/ontologies/ccso#affiliatedWith"/>
        <rdfs:subPropertyOf>
            <rdf:Description>
                <owl:inverseOf rdf:resource="http://xworks.gr/ontologies/ccso#affiliatedWith"/>
            </rdf:Description>
        </rdfs:subPropertyOf>
        <rdf:type rdf:resource="http://www.w3.org/2002/07/owl#AsymmetricProperty"/>
        <rdf:type rdf:resource="http://www.w3.org/2002/07/owl#IrreflexiveProperty"/>
        <rdfs:domain rdf:resource="http://xworks.gr/ontologies/ccso#Professor"/>
        <rdfs:range rdf:resource="http://xworks.gr/ontologies/ccso#Syllabus"/>
        <rdfs:comment xml:lang="en">Professor is Instructor in some Courses</rdfs:comment>
        <rdfs:comment xml:lang="gr">Ο Καθηγητής είναι διδάσκων σε κάποια μαθήματα.</rdfs:comment>
    </owl:ObjectProperty>
    


    <!-- http://xworks.gr/ontologies/ccso#listedInKU -->

    <owl:ObjectProperty rdf:about="http://xworks.gr/ontologies/ccso#listedInKU">
        <owl:inverseOf rdf:resource="http://xworks.gr/ontologies/ccso#lists"/>
        <rdfs:domain>
            <owl:Class>
                <owl:unionOf rdf:parseType="Collection">
                    <rdf:Description rdf:about="http://xworks.gr/ontologies/ccso#LearningOutcome"/>
                    <rdf:Description rdf:about="http://xworks.gr/ontologies/ccso#Topic"/>
                </owl:unionOf>
            </owl:Class>
        </rdfs:domain>
        <rdfs:range rdf:resource="http://xworks.gr/ontologies/ccso#KnowledgeUnit"/>
        <rdfs:comment xml:lang="en">Each Topic and Learning Outcome that students are expected to achieve, is listed in a Knowledge Unit (KU)</rdfs:comment>
        <rdfs:comment xml:lang="gr">Κάθε Θέμα και Μαθησιακό Αποτέλεσμα περιλαμβάνεται σε μια Μονάδα Γνώσης (KU)</rdfs:comment>
    </owl:ObjectProperty>
    


    <!-- http://xworks.gr/ontologies/ccso#lists -->

    <owl:ObjectProperty rdf:about="http://xworks.gr/ontologies/ccso#lists">
        <rdfs:domain rdf:resource="http://xworks.gr/ontologies/ccso#KnowledgeUnit"/>
        <rdfs:range>
            <owl:Class>
                <owl:unionOf rdf:parseType="Collection">
                    <rdf:Description rdf:about="http://xworks.gr/ontologies/ccso#LearningOutcome"/>
                    <rdf:Description rdf:about="http://xworks.gr/ontologies/ccso#Topic"/>
                </owl:unionOf>
            </owl:Class>
        </rdfs:range>
        <rdfs:comment xml:lang="en">Each KU lists a set of Topics and the Learning Outcomes students are expected to achieve.</rdfs:comment>
        <rdfs:comment xml:lang="gr">Κάθε KU περιλαμβάνει μία ομάδα από Θέματα και Μαθησιακά Αποτελέσματα που αναμένεται να επιτύχουν οι Φοιτητές.</rdfs:comment>
    </owl:ObjectProperty>
    


    <!-- http://xworks.gr/ontologies/ccso#memberOf -->

    <owl:ObjectProperty rdf:about="http://xworks.gr/ontologies/ccso#memberOf">
        <rdfs:subPropertyOf rdf:resource="http://xworks.gr/ontologies/ccso#affiliatedWith"/>
        <rdfs:subPropertyOf>
            <rdf:Description>
                <owl:inverseOf rdf:resource="http://xworks.gr/ontologies/ccso#affiliatedWith"/>
            </rdf:Description>
        </rdfs:subPropertyOf>
        <rdfs:domain rdf:resource="http://xworks.gr/ontologies/ccso#AcademicStaff"/>
        <rdfs:range rdf:resource="http://xworks.gr/ontologies/ccso#Department"/>
        <rdfs:comment xml:lang="en">The academic staff of an institution, a school or a university such as professors of various ranks, lecturers and/or researchers. In North America the term Faculty is used instead.</rdfs:comment>
        <rdfs:comment xml:lang="gr">Το Ακαδημαϊκό Προσωπικό ενός ινστιτούτου, ενός σχολείου ή ενός Πανεπιστημίου όπως καθηγητές διαφόρων βαθμίδων, εισηγητές, ερευνητές. Στη Βόρεια Αμερική χρησμοποιείται ο όρος Faculty.</rdfs:comment>
    </owl:ObjectProperty>
    


    <!-- http://xworks.gr/ontologies/ccso#offeredBy -->

    <owl:ObjectProperty rdf:about="http://xworks.gr/ontologies/ccso#offeredBy">
        <owl:inverseOf rdf:resource="http://xworks.gr/ontologies/ccso#offersCourse"/>
        <rdfs:domain rdf:resource="http://xworks.gr/ontologies/ccso#Course"/>
        <rdfs:range rdf:resource="http://xworks.gr/ontologies/ccso#Department"/>
        <rdfs:comment xml:lang="en">Course is offered by Department</rdfs:comment>
        <rdfs:comment xml:lang="gr">Το μάθημα παρέχεται από ένα Τμήμα.</rdfs:comment>
    </owl:ObjectProperty>
    


    <!-- http://xworks.gr/ontologies/ccso#offersCourse -->

    <owl:ObjectProperty rdf:about="http://xworks.gr/ontologies/ccso#offersCourse">
        <rdfs:domain rdf:resource="http://xworks.gr/ontologies/ccso#Department"/>
        <rdfs:range rdf:resource="http://xworks.gr/ontologies/ccso#Course"/>
        <rdfs:comment xml:lang="en">A Department offers some Courses available to Students.</rdfs:comment>
        <rdfs:comment xml:lang="gr">Ένα Τμήμα προσφέρει κάποια Μαθήματα που είναι διαθέσιμα στους Φοιτητές.</rdfs:comment>
    </owl:ObjectProperty>
    


    <!-- http://xworks.gr/ontologies/ccso#partOfFS -->

    <owl:ObjectProperty rdf:about="http://xworks.gr/ontologies/ccso#partOfFS">
        <rdf:type rdf:resource="http://www.w3.org/2002/07/owl#TransitiveProperty"/>
        <rdfs:domain rdf:resource="http://xworks.gr/ontologies/ccso#FieldofStudy"/>
        <rdfs:range rdf:resource="http://xworks.gr/ontologies/ccso#FieldofStudy"/>
        <rdfs:comment xml:lang="en">A field of study may be part of a broader field of study.</rdfs:comment>
        <rdfs:comment xml:lang="gr">Ένα πεδίο μελέτης που μπορεί να είναι μέρος ενός ευρύτερου πεδιού μελέτης.</rdfs:comment>
    </owl:ObjectProperty>
    


    <!-- http://xworks.gr/ontologies/ccso#providedBy -->

    <owl:ObjectProperty rdf:about="http://xworks.gr/ontologies/ccso#providedBy">
        <owl:inverseOf rdf:resource="http://xworks.gr/ontologies/ccso#providesProgram"/>
        <rdf:type rdf:resource="http://www.w3.org/2002/07/owl#AsymmetricProperty"/>
        <rdf:type rdf:resource="http://www.w3.org/2002/07/owl#IrreflexiveProperty"/>
        <rdfs:domain rdf:resource="http://xworks.gr/ontologies/ccso#ProgramofStudy"/>
        <rdfs:range rdf:resource="http://xworks.gr/ontologies/ccso#Department"/>
        <rdfs:comment>A Study Program is provided by an Educational Organization.</rdfs:comment>
        <rdfs:comment xml:lang="gr">Ένα Πρόγραμμα Σπουδών παρέχεται από έναν Εκπαιδευτικό Οργανισμό.</rdfs:comment>
    </owl:ObjectProperty>
    


    <!-- http://xworks.gr/ontologies/ccso#providesProgram -->

    <owl:ObjectProperty rdf:about="http://xworks.gr/ontologies/ccso#providesProgram">
        <rdf:type rdf:resource="http://www.w3.org/2002/07/owl#AsymmetricProperty"/>
        <rdf:type rdf:resource="http://www.w3.org/2002/07/owl#IrreflexiveProperty"/>
        <rdfs:domain rdf:resource="http://xworks.gr/ontologies/ccso#Department"/>
        <rdfs:range rdf:resource="http://xworks.gr/ontologies/ccso#ProgramofStudy"/>
        <rdfs:comment>An Educational Organization provides a variety of Study Programs in many Disciplines and Knowledge Bodies.</rdfs:comment>
        <rdfs:comment xml:lang="gr">Ένας Εκπαιδευτικός Οργανισμός παρέχει μία ποικιλία από Προγράμματα Σπουδών σε πολλούς Τομείς Γνώσης.</rdfs:comment>
    </owl:ObjectProperty>
    


    <!-- http://xworks.gr/ontologies/ccso#requiresProgram -->

    <owl:ObjectProperty rdf:about="http://xworks.gr/ontologies/ccso#requiresProgram">
        <rdf:type rdf:resource="http://www.w3.org/2002/07/owl#AsymmetricProperty"/>
        <rdf:type rdf:resource="http://www.w3.org/2002/07/owl#IrreflexiveProperty"/>
        <rdfs:domain rdf:resource="http://xworks.gr/ontologies/ccso#ProgramofStudy"/>
        <rdfs:range rdf:resource="http://xworks.gr/ontologies/ccso#ProgramofStudy"/>
        <rdfs:comment xml:lang="en">Study Program requires a Study Program.</rdfs:comment>
        <rdfs:comment xml:lang="gr">Ένα Πρόγραμμα Σπουδών απαιτεί ένα Πρόγραμμα Σπουδών.</rdfs:comment>
    </owl:ObjectProperty>
    


    <!-- http://xworks.gr/ontologies/ccso#supervisorOf -->

    <owl:ObjectProperty rdf:about="http://xworks.gr/ontologies/ccso#supervisorOf">
        <rdfs:subPropertyOf rdf:resource="http://xworks.gr/ontologies/ccso#affiliatedWith"/>
        <rdfs:subPropertyOf>
            <rdf:Description>
                <owl:inverseOf rdf:resource="http://xworks.gr/ontologies/ccso#affiliatedWith"/>
            </rdf:Description>
        </rdfs:subPropertyOf>
        <rdf:type rdf:resource="http://www.w3.org/2002/07/owl#AsymmetricProperty"/>
        <rdf:type rdf:resource="http://www.w3.org/2002/07/owl#IrreflexiveProperty"/>
        <rdfs:domain rdf:resource="http://xworks.gr/ontologies/ccso#Professor"/>
        <rdfs:range rdf:resource="http://xworks.gr/ontologies/ccso#Syllabus"/>
        <rdfs:comment xml:lang="en">A Professor can supervises and manages all the activities within a Course such as the design, the implementation, the lessons, the outcomes, etc.</rdfs:comment>
        <rdfs:comment xml:lang="gr">Ένας Καθηγητής μπορεί να επιβλέπει και να διαχειρίζεται όλες τις δραστηριότητες σε ένα Μάθημα όπως το σχεδιασμό, την εφαρμογή, τη διδασκαλία, τα αποτελέσματα κτλ.</rdfs:comment>
    </owl:ObjectProperty>
    


    <!-- http://xworks.gr/ontologies/ccso#syllabusOf -->

    <owl:ObjectProperty rdf:about="http://xworks.gr/ontologies/ccso#syllabusOf">
        <rdfs:domain rdf:resource="http://xworks.gr/ontologies/ccso#Syllabus"/>
        <rdfs:range rdf:resource="http://xworks.gr/ontologies/ccso#Course"/>
        <rdfs:comment xml:lang="en">It is Syllabus of a Course.</rdfs:comment>
        <rdfs:comment xml:lang="gr">Είναι το Περίγραμμα Σπουδών ενός Μαθήματος.</rdfs:comment>
    </owl:ObjectProperty>
    


    <!-- http://xworks.gr/ontologies/ccso#teachesIn -->

    <owl:ObjectProperty rdf:about="http://xworks.gr/ontologies/ccso#teachesIn">
        <rdfs:subPropertyOf rdf:resource="http://xworks.gr/ontologies/ccso#affiliatedWith"/>
        <rdfs:subPropertyOf>
            <rdf:Description>
                <owl:inverseOf rdf:resource="http://xworks.gr/ontologies/ccso#affiliatedWith"/>
            </rdf:Description>
        </rdfs:subPropertyOf>
        <rdf:type rdf:resource="http://www.w3.org/2002/07/owl#AsymmetricProperty"/>
        <rdf:type rdf:resource="http://www.w3.org/2002/07/owl#IrreflexiveProperty"/>
        <rdfs:domain rdf:resource="http://xworks.gr/ontologies/ccso#Professor"/>
        <rdfs:range rdf:resource="http://xworks.gr/ontologies/ccso#TeachingEvent"/>
        <rdfs:comment xml:lang="en">A Professor teaches in some Teaching Events within a course.</rdfs:comment>
        <rdfs:comment xml:lang="gr">Ένας Καθηγητής κάνει κάποιες Διδασκαλίες μέσα σε ένα Μάθημα.</rdfs:comment>
    </owl:ObjectProperty>
    


    <!-- http://xworks.gr/ontologies/ccso#worksFor -->

    <owl:ObjectProperty rdf:about="http://xworks.gr/ontologies/ccso#worksFor">
        <rdfs:subPropertyOf>
            <rdf:Description>
                <owl:inverseOf rdf:resource="http://xworks.gr/ontologies/ccso#affiliatedWith"/>
            </rdf:Description>
        </rdfs:subPropertyOf>
        <rdfs:domain rdf:resource="http://xworks.gr/ontologies/ccso#Employee"/>
        <rdfs:range rdf:resource="http://schema.org/EducationalOrganization"/>
        <rdfs:comment xml:lang="en">An employee works for an organization.</rdfs:comment>
        <rdfs:comment xml:lang="gr">Ένας υπάλληλος εργάζεται σε έναν Οργανισμό.</rdfs:comment>
    </owl:ObjectProperty>
    


    <!-- 
    ///////////////////////////////////////////////////////////////////////////////////////
    //
    // Data properties
    //
    ///////////////////////////////////////////////////////////////////////////////////////
     -->

    


    <!-- http://purl.org/dc/elements/1.1/date -->

    <owl:DatatypeProperty rdf:about="http://purl.org/dc/elements/1.1/date">
        <rdfs:subPropertyOf rdf:resource="http://xworks.gr/ontologies/ccso#dates"/>
        <rdfs:domain rdf:resource="http://xworks.gr/ontologies/ccso#Resource"/>
        <rdfs:range rdf:resource="http://www.w3.org/2001/XMLSchema#date"/>
        <rdfs:comment xml:lang="en">A point or period of time associated with an event in the lifecycle of the resource.
Date may be used to express temporal information at any level of granularity. Recommended best practice is to use an encoding scheme, such as the W3CDTF profile of ISO 8601 [W3CDTF] (e.g. 2017-03-15).</rdfs:comment>
        <rdfs:comment xml:lang="gr">Ένα σημείο ή περιόδος του χρόνου που σχετίζεται με ένα γεγονός στον κύκλο ζωής μίας πηγής. 
Η ημερομηνία μπορεί να χρησιμοποιηθεί για να εκφράσει μία προσωρινή πληροφορία σε οποιδήποτε επίπεδο του επιπέδου ανάλυσης. Προτείνεται να γίνεται χρήση ενός σχήματος κωδικοποίησης, όπως το  W3CDTF profile του ISO 8601 [W3CDTF] (π.χ. 2017-03-15).</rdfs:comment>
    </owl:DatatypeProperty>
    


    <!-- http://purl.org/dc/elements/1.1/description -->

    <owl:DatatypeProperty rdf:about="http://purl.org/dc/elements/1.1/description">
        <rdfs:domain rdf:resource="http://xworks.gr/ontologies/ccso#Resource"/>
        <rdfs:range rdf:resource="http://www.w3.org/2001/XMLSchema#string"/>
        <rdfs:comment xml:lang="gr"></rdfs:comment>
        <rdfs:comment xml:lang="en">An account of the resource.
Description may includes: an abstract, a table of contents, a graphical representation, or a free-text account of the resource.</rdfs:comment>
        <rdfs:comment xml:lang="gr">Ο Λογαριασμός μία πηγής.
Η περιγραφή μπορεί περιλαμβάνει: μια περίληψη, πίνακα περιεχομένων, γραγική απεικόνιση, ελεύθερο κείμενο.</rdfs:comment>
    </owl:DatatypeProperty>
    


    <!-- http://purl.org/dc/elements/1.1/format -->

    <owl:DatatypeProperty rdf:about="http://purl.org/dc/elements/1.1/format">
        <rdfs:domain rdf:resource="http://xworks.gr/ontologies/ccso#Resource"/>
        <rdfs:range rdf:resource="http://www.w3.org/2001/XMLSchema#string"/>
        <rdfs:comment xml:lang="en">The file format, physical medium, or dimensions of the resource.
Examples of dimensions include size and duration. Recommended best practice is to use a controlled vocabulary such as the list of Internet Media Types.</rdfs:comment>
        <rdfs:comment xml:lang="gr">Η μορφή του αρχείου, η φυσική του υπόσταση ή οι διαστάσεις της πηγής.
Παραδείγματα από διαστάσεις περιλαμβάνουν το μέγεθος και τη διάρκεια. Προτεινόμενες πρακτικές είναι η χρήση ενός ελεγχόμενου λεξιλογίου όπως η λίστα των Internet Media Types.</rdfs:comment>
        <rdfs:seeAlso xml:lang="en">[MIME] http://www.iana.org/assignments/media-types/</rdfs:seeAlso>
    </owl:DatatypeProperty>
    


    <!-- http://purl.org/dc/elements/1.1/language -->

    <owl:DatatypeProperty rdf:about="http://purl.org/dc/elements/1.1/language">
        <rdfs:domain rdf:resource="http://xworks.gr/ontologies/ccso#Resource"/>
        <rdfs:range rdf:resource="http://www.w3.org/2001/XMLSchema#language"/>
        <rdfs:comment xml:lang="en">A language of the resource.
Recommended best practice is to use a controlled vocabulary such as RFC 4646 [RFC4646].</rdfs:comment>
        <rdfs:comment xml:lang="gr">Η γλώσσα της πηγής.
Προτεινόμενη καλή πρακτική είναι η χρήση ενός ελεγχόμενου λεξιλογίου όπως το RFC 4646 [RFC4646].</rdfs:comment>
        <rdfs:seeAlso xml:lang="en">[RFC4646] http://www.ietf.org/rfc/rfc4646.txt</rdfs:seeAlso>
    </owl:DatatypeProperty>
    


    <!-- http://purl.org/dc/elements/1.1/publisher -->

    <owl:DatatypeProperty rdf:about="http://purl.org/dc/elements/1.1/publisher">
        <rdfs:domain rdf:resource="http://xworks.gr/ontologies/ccso#Resource"/>
        <rdfs:range rdf:resource="http://www.w3.org/2001/XMLSchema#string"/>
        <rdfs:comment xml:lang="en">An entity responsible for making the resource available.
Examples of a Publisher include a person, an organization, or a service. Typically, the name of a Publisher should be used to indicate the entity.</rdfs:comment>
        <rdfs:comment xml:lang="gr">Μία οντότητα που είναι υπεύθυνη να κάνει μία πηγή διαθέσιμη/δημοσιευμένη. 
Εκδότης μπορεί να είναι ένα πρόσωπο, ένας οργανισμός, ή μία υπηρεσία. Τυπικά, το όνομα του Εκδότη θα πρέπει να χρησιμοποιείται προκειμένου να υποδεικνύεται η οντότητα.</rdfs:comment>
    </owl:DatatypeProperty>
    


    <!-- http://purl.org/dc/elements/1.1/source -->

    <owl:DatatypeProperty rdf:about="http://purl.org/dc/elements/1.1/source">
        <rdfs:domain rdf:resource="http://xworks.gr/ontologies/ccso#Resource"/>
        <rdfs:range rdf:resource="http://www.w3.org/2001/XMLSchema#string"/>
        <rdfs:comment xml:lang="en">A related resource from which the described resource is derived.
The described resource may be derived from the related resource in whole or in part. Recommended best practice is to identify the related resource by means of a string conforming to a formal identification system.

Here: The various types of media where the work is published.
The most common types are: 
• Book,
• Journal, 
• Workshop, 
• Conference, 
• Proceedings, 
• Thesis, 
• Magazine, 
• Newspaper, 
• Webpage,  
• UnofficialPublication, 
• etc.</rdfs:comment>
        <rdfs:comment xml:lang="gr">Μία συναφής πηγή από την οποία προέρχεται η περιγραφόμενη πηγή. 
Η περιγραφόμενη πηγή μπορεί να προέρχεται από μία συναφή πηγή συνολικά ή μερικώς. Προτεινόμενη καλή πρακτική είναι να αναγνωριστεί η συναφής πηγή μέσω ενός νήματος που ενσωματώνεται σε ένα επίσημο σύστημα αναγνώρισης.

Εδώ: τα διάφορα είδη μέσων όπου μπορεί να δημοσιευτεί μία δουλειά. 
Τα πιο συνηθισμένα είδη είναι:
• Βιβλία,
• Επιστημονικά Περιοδικά,
• Εργαστήρια,
• Συνέδρια,
• Διαδικασίες,
• Διατριβές, 
• Περιοδικά, 
• Εφημερίδες, 
• Ιστοσελίδες,
• Μη επίσημες Εκδόσεις
• κτλ</rdfs:comment>
    </owl:DatatypeProperty>
    


    <!-- http://purl.org/dc/elements/1.1/subject -->

    <owl:DatatypeProperty rdf:about="http://purl.org/dc/elements/1.1/subject">
        <rdfs:domain rdf:resource="http://xworks.gr/ontologies/ccso#Resource"/>
        <rdfs:range rdf:resource="http://www.w3.org/2001/XMLSchema#string"/>
        <rdfs:comment xml:lang="en">The topic of the resource.
Typically, the subject will be represented using keywords, key phrases, or classification codes. Recommended best practice is to use a controlled vocabulary.</rdfs:comment>
        <rdfs:comment xml:lang="gr">Το θέμα μίας Πηγής. 
Τυπικά, το αντικείμενο μπορεί να αναπαραστεί χρησιμοποιώντας λέξεις κλειδιά, φράσεις κλειδιά, ή κωδικοί ταξινόμησης. 
Προτείνεται να γίνεται χρήση ελεγχόμενου λεξιλογίου.</rdfs:comment>
    </owl:DatatypeProperty>
    


    <!-- http://purl.org/dc/elements/1.1/title -->

    <owl:DatatypeProperty rdf:about="http://purl.org/dc/elements/1.1/title">
        <rdfs:domain rdf:resource="http://xworks.gr/ontologies/ccso#Resource"/>
        <rdfs:range rdf:resource="http://www.w3.org/2001/XMLSchema#string"/>
        <rdfs:comment xml:lang="en">A name given to the resource.
Typically, a Title will be a name by which the resource is formally known.</rdfs:comment>
        <rdfs:comment xml:lang="gr">Το όνομα που δίνεται σε μία πηγή. 
Τυπικά, ένας Τίτλος μπορεί να είναι ένα όνομα με βάση το οποίο η Πηγή είναι επισήμως γνωστή.</rdfs:comment>
    </owl:DatatypeProperty>
    


    <!-- http://purl.org/dc/elements/1.1/type -->

    <owl:DatatypeProperty rdf:about="http://purl.org/dc/elements/1.1/type">
        <rdfs:domain rdf:resource="http://xworks.gr/ontologies/ccso#Resource"/>
        <rdfs:range rdf:resource="http://www.w3.org/2001/XMLSchema#string"/>
        <rdfs:comment xml:lang="en">The nature or genre of the resource.
The various types of the work. The most common types of works are: 
• Article, 
• Chapter, 
• Paper, 
• Booklet, 
• Poster, 
• Thesis, 
• Software, 
• Specification, 
• Report, 
• UnofficialPublication, etc.
A Thesis could be BachelorThesis, MasterThesis or DoctoralThesis.</rdfs:comment>
        <rdfs:comment xml:lang="gr">Η φύση ή το είδος της Πηγής. 
Οι διάφοροι τύποι του έργου. Οι πιο συνηθισμένοι τύποι έργου είναι:
• Άρθρο,
• Κεφάλαιο, 
• Επιστημονικό Άρθρο, 
• Φυλλάδιο, 
• Αφίσα, 
• Διπλωματική Εργασία,
• Λογισμικό, 
• Εξειδίκευση, 
• Αναφορά, 
• Ανεπίσημη Έκδοση, κτλ.
Η Διπλωματική Εργασία μπορεί να είναι Πτυχιακή Εργασία, Μεταπτυχιακή Εργασία ή Διδακτορική Διατριβή.</rdfs:comment>
    </owl:DatatypeProperty>
    


    <!-- http://schema.org/address -->

    <owl:DatatypeProperty rdf:about="http://schema.org/address">
        <rdfs:domain rdf:resource="http://schema.org/EducationalOrganization"/>
        <rdfs:range rdf:resource="http://www.w3.org/2001/XMLSchema#string"/>
        <rdfs:comment xml:lang="en">The physical address of an Organization.</rdfs:comment>
        <rdfs:comment xml:lang="gr">Η διεύθυνση ενός Οργανισμού.</rdfs:comment>
        <rdfs:isDefinedBy rdf:resource="http://schema.org/address"/>
    </owl:DatatypeProperty>
    


    <!-- http://schema.org/email -->

    <owl:DatatypeProperty rdf:about="http://schema.org/email">
        <rdfs:subPropertyOf rdf:resource="http://xworks.gr/ontologies/ccso#eContactInfo"/>
        <rdfs:domain>
            <owl:Class>
                <owl:unionOf rdf:parseType="Collection">
                    <rdf:Description rdf:about="http://schema.org/EducationalOrganization"/>
                    <rdf:Description rdf:about="http://www.w3.org/2000/10/swap/pim/contact#Person"/>
                </owl:unionOf>
            </owl:Class>
        </rdfs:domain>
        <rdfs:range rdf:resource="http://www.w3.org/2001/XMLSchema#anyURI"/>
        <rdfs:comment xml:lang="gr">H ηλεκτρινική διεύθυνση ενός Οργανισμού ή ενός Προσώπου (το προσωπικό eMail).</rdfs:comment>
        <rdfs:comment xml:lang="en">The eMail address of an Organization or a Person (personal eMail).</rdfs:comment>
        <rdfs:isDefinedBy rdf:resource="http://schema.org/email"/>
    </owl:DatatypeProperty>
    


    <!-- http://schema.org/faxNumber -->

    <owl:DatatypeProperty rdf:about="http://schema.org/faxNumber">
        <rdfs:subPropertyOf rdf:resource="http://xworks.gr/ontologies/ccso#phone"/>
        <rdfs:domain>
            <owl:Class>
                <owl:unionOf rdf:parseType="Collection">
                    <rdf:Description rdf:about="http://schema.org/EducationalOrganization"/>
                    <rdf:Description rdf:about="http://xmlns.com/foaf/0.1/Person"/>
                </owl:unionOf>
            </owl:Class>
        </rdfs:domain>
        <rdfs:range rdf:resource="http://www.w3.org/2001/XMLSchema#string"/>
        <rdfs:comment xml:lang="en">The fax number of an Organization or a Person.</rdfs:comment>
        <rdfs:isDefinedBy rdf:resource="http://schema.org/faxNumber"/>
        <ns:term_status xml:lang="gr">Ο αριθμός φαξ ενός Οργανισμού ή ενός Προσώπου.</ns:term_status>
    </owl:DatatypeProperty>
    


    <!-- http://schema.org/identifier -->

    <owl:DatatypeProperty rdf:about="http://schema.org/identifier">
        <rdfs:domain rdf:resource="http://schema.org/EducationalOrganization"/>
        <rdfs:range rdf:resource="http://www.w3.org/2001/XMLSchema#string"/>
        <rdfs:comment xml:lang="en">The organization identifier that uniquely identifies the legal entity of the organization.</rdfs:comment>
        <rdfs:isDefinedBy>http://schema.org/identifier</rdfs:isDefinedBy>
        <ns:term_status xml:lang="gr">Το αναγνωριστικό ενός Οργανισμού που χαρακτηρίζει αποκλειστικά τη νομική οντότητα του οργανισμού.</ns:term_status>
    </owl:DatatypeProperty>
    


    <!-- http://schema.org/legalName -->

    <owl:DatatypeProperty rdf:about="http://schema.org/legalName">
        <rdfs:domain rdf:resource="http://schema.org/EducationalOrganization"/>
        <rdfs:range rdf:resource="http://www.w3.org/2001/XMLSchema#string"/>
        <rdfs:comment xml:lang="en">The official name of the organization.</rdfs:comment>
        <rdfs:isDefinedBy rdf:resource="http://schema.org/legalName"/>
        <ns:term_status xml:lang="gr">Το επίσημο όνομα ενός οργανισμού.</ns:term_status>
    </owl:DatatypeProperty>
    


    <!-- http://schema.org/location -->

    <owl:DatatypeProperty rdf:about="http://schema.org/location">
        <rdfs:domain rdf:resource="http://schema.org/EducationalOrganization"/>
        <rdfs:range rdf:resource="http://www.w3.org/2001/XMLSchema#string"/>
        <rdfs:comment xml:lang="en">The location an organization is located.</rdfs:comment>
        <rdfs:comment xml:lang="gr">Η τοποθεσία ενός οργανισμού.</rdfs:comment>
        <rdfs:isDefinedBy>http://schema.org/location</rdfs:isDefinedBy>
    </owl:DatatypeProperty>
    


    <!-- http://schema.org/logo -->

    <owl:DatatypeProperty rdf:about="http://schema.org/logo">
        <rdfs:domain rdf:resource="http://schema.org/EducationalOrganization"/>
        <rdfs:range rdf:resource="http://www.w3.org/2001/XMLSchema#anyURI"/>
        <rdfs:comment xml:lang="en">An associated image as the logo of an Organization.</rdfs:comment>
        <rdfs:comment xml:lang="gr">Μία σχετική εικόνα ως λογότυπο ενός Οργανισμού.</rdfs:comment>
        <rdfs:isDefinedBy rdf:resource="http://schema.org/logo"/>
    </owl:DatatypeProperty>
    


    <!-- http://schema.org/url -->

    <owl:DatatypeProperty rdf:about="http://schema.org/url">
        <rdfs:subPropertyOf rdf:resource="http://xworks.gr/ontologies/ccso#eContactInfo"/>
        <rdfs:domain>
            <owl:Class>
                <owl:unionOf rdf:parseType="Collection">
                    <rdf:Description rdf:about="http://schema.org/EducationalOrganization"/>
                    <rdf:Description rdf:about="http://xmlns.com/foaf/0.1/Person"/>
                    <rdf:Description rdf:about="http://xworks.gr/ontologies/ccso#Resource"/>
                </owl:unionOf>
            </owl:Class>
        </rdfs:domain>
        <rdfs:range rdf:resource="http://www.w3.org/2001/XMLSchema#anyURI"/>
        <rdfs:comment xml:lang="en">The address of the webpage of an Organization, a Person or a Publication</rdfs:comment>
        <rdfs:comment xml:lang="gr">Η διεύθυνση μίας ιστοσελίδας ενός Οργανισμού ή ενός Προσώπου.</rdfs:comment>
        <rdfs:isDefinedBy rdf:resource="http://schema.org/url"/>
        <skos:altLabel xml:lang="en">homepage</skos:altLabel>
    </owl:DatatypeProperty>
    


    <!-- http://xmlns.com/foaf/0.1/age -->

    <owl:DatatypeProperty rdf:about="http://xmlns.com/foaf/0.1/age">
        <rdf:type rdf:resource="http://www.w3.org/2002/07/owl#FunctionalProperty"/>
        <rdfs:domain rdf:resource="http://xmlns.com/foaf/0.1/Agent"/>
        <rdfs:range rdf:resource="http://www.w3.org/2000/01/rdf-schema#Literal"/>
        <rdfs:comment>The age in years of some agent.</rdfs:comment>
        <rdfs:comment xml:lang="gr">Η ηλικία σε έτη ενός εκπροσώπου.</rdfs:comment>
        <rdfs:isDefinedBy rdf:resource="http://xmlns.com/foaf/0.1/"/>
        <rdfs:label>age</rdfs:label>
        <ns:term_status>unstable</ns:term_status>
    </owl:DatatypeProperty>
    


    <!-- http://xmlns.com/foaf/0.1/familyName -->

    <owl:DatatypeProperty rdf:about="http://xmlns.com/foaf/0.1/familyName">
        <rdfs:domain rdf:resource="http://xmlns.com/foaf/0.1/Person"/>
        <rdfs:range rdf:resource="http://www.w3.org/2000/01/rdf-schema#Literal"/>
        <rdfs:comment>The family name of a person.</rdfs:comment>
        <rdfs:comment xml:lang="gr">Το Επώνυμο ενός Προσώπου.</rdfs:comment>
        <rdfs:isDefinedBy rdf:resource="http://xmlns.com/foaf/0.1/"/>
        <rdfs:label>familyName</rdfs:label>
        <ns:term_status>testing</ns:term_status>
    </owl:DatatypeProperty>
    


    <!-- http://xmlns.com/foaf/0.1/firstName -->

    <owl:DatatypeProperty rdf:about="http://xmlns.com/foaf/0.1/firstName">
        <rdfs:domain rdf:resource="http://xmlns.com/foaf/0.1/Person"/>
        <rdfs:range rdf:resource="http://www.w3.org/2000/01/rdf-schema#Literal"/>
        <rdfs:comment>The first name of a person.</rdfs:comment>
        <rdfs:comment xml:lang="gr">Το κυρίως όνομα ενός Προσώπου.</rdfs:comment>
        <rdfs:isDefinedBy rdf:resource="http://xmlns.com/foaf/0.1/"/>
        <rdfs:label>firstName</rdfs:label>
        <ns:term_status>testing</ns:term_status>
    </owl:DatatypeProperty>
    


    <!-- http://xmlns.com/foaf/0.1/gender -->

    <owl:DatatypeProperty rdf:about="http://xmlns.com/foaf/0.1/gender">
        <rdf:type rdf:resource="http://www.w3.org/2002/07/owl#FunctionalProperty"/>
        <rdfs:domain rdf:resource="http://xmlns.com/foaf/0.1/Agent"/>
        <rdfs:range rdf:resource="http://www.w3.org/2000/01/rdf-schema#Literal"/>
        <rdfs:comment>The gender of this Agent (typically but not necessarily &apos;male&apos; or &apos;female&apos;).</rdfs:comment>
        <rdfs:comment xml:lang="gr">Το γένος (φύλο) ενός εκπροσώπου (τυπικά αλλά όχι απαραίτητα &quot;άνδρας&quot; ή &quot;γυναίκα&quot;).</rdfs:comment>
        <rdfs:isDefinedBy rdf:resource="http://xmlns.com/foaf/0.1/"/>
        <rdfs:label>gender</rdfs:label>
        <ns:term_status>testing</ns:term_status>
    </owl:DatatypeProperty>
    


    <!-- http://xmlns.com/foaf/0.1/lastName -->

    <owl:DatatypeProperty rdf:about="http://xmlns.com/foaf/0.1/lastName">
        <rdfs:domain rdf:resource="http://xmlns.com/foaf/0.1/Person"/>
        <rdfs:range rdf:resource="http://www.w3.org/2000/01/rdf-schema#Literal"/>
        <rdfs:comment>The last name of a person.</rdfs:comment>
        <rdfs:comment xml:lang="gr">Το επώνυμο ενός Προσώπου.</rdfs:comment>
        <rdfs:isDefinedBy rdf:resource="http://xmlns.com/foaf/0.1/"/>
        <rdfs:label>lastName</rdfs:label>
        <ns:term_status>testing</ns:term_status>
    </owl:DatatypeProperty>
    


    <!-- http://xmlns.com/foaf/0.1/title -->

    <owl:DatatypeProperty rdf:about="http://xmlns.com/foaf/0.1/title">
        <rdfs:domain rdf:resource="http://xmlns.com/foaf/0.1/Person"/>
        <rdfs:range rdf:resource="http://www.w3.org/2001/XMLSchema#string"/>
        <rdfs:comment>Title (Mr, Mrs, Ms, Dr. etc)</rdfs:comment>
        <rdfs:isDefinedBy rdf:resource="http://xmlns.com/foaf/0.1/"/>
        <rdfs:label>title</rdfs:label>
        <ns:term_status>testing</ns:term_status>
        <ns:term_status xml:lang="gr">Ο τίτλος (Κος, Κα, Δρ, κτλ).</ns:term_status>
    </owl:DatatypeProperty>
    


    <!-- http://xworks.gr/ontologies/ccso#abbreviation -->

    <owl:DatatypeProperty rdf:about="http://xworks.gr/ontologies/ccso#abbreviation">
        <rdfs:domain rdf:resource="http://xworks.gr/ontologies/ccso#Discipline"/>
        <rdfs:range rdf:resource="http://www.w3.org/2001/XMLSchema#string"/>
        <rdfs:comment xml:lang="en">The shorten form of the Name of a Discipline.
The shorten form of the Name of Body of Knowledge (inherited property).
The shorten form of the Name of Area of Knowledge (inherited property).
The shorten form of the Name of Unit of Knowledge (inherited property).</rdfs:comment>
        <rdfs:comment xml:lang="gr">Η συντομευμένη μορφή του Ονόματους του Τομέα.
Η συντομευμένη μορφή του Ονόματος του Βασικού Κορμού της Γνώσης. 
Η συντομευμένη μορφή του Ονόματος του Πεδίου Γνώσης. 
Η συντομευμένη μορφή του Ονόματος της Μονάδας Γνώσης.</rdfs:comment>
    </owl:DatatypeProperty>
    


    <!-- http://xworks.gr/ontologies/ccso#academicYear -->

    <owl:DatatypeProperty rdf:about="http://xworks.gr/ontologies/ccso#academicYear">
        <rdfs:domain rdf:resource="http://xworks.gr/ontologies/ccso#Syllabus"/>
        <rdfs:range rdf:resource="http://www.w3.org/2001/XMLSchema#string"/>
        <rdfs:comment xml:lang="en">The academic year where the Course is offered and starts (e.g. 2015-16 or 2017-2018).</rdfs:comment>
        <rdfs:comment xml:lang="gr">To Ακαδημαϊκό Έτος στο οποίο διδάσκεται το μάθημα (π.χ. 2015-16 ή 2017-2018).</rdfs:comment>
    </owl:DatatypeProperty>
    


    <!-- http://xworks.gr/ontologies/ccso#code -->

    <owl:DatatypeProperty rdf:about="http://xworks.gr/ontologies/ccso#code">
        <rdf:type rdf:resource="http://www.w3.org/2002/07/owl#FunctionalProperty"/>
        <rdfs:range rdf:resource="http://www.w3.org/2000/01/rdf-schema#Literal"/>
        <rdfs:comment xml:lang="en">The identifier that uniquely identifies a Study Programme in the national curriculum or either a Course or Syllabus in an Institute.</rdfs:comment>
        <rdfs:comment xml:lang="gr">Το αναγνωριστικό που χαρακτηρίζει ενιαία ένα Πρόγραμμα Σπουδών στο εθνικό πρόγραμμα μαθημάτων ή ένα Μάθημα ή ένα Περίγραμμα Σπουδών σε ένα Φορέα.</rdfs:comment>
    </owl:DatatypeProperty>
    


    <!-- http://xworks.gr/ontologies/ccso#courseType -->

    <owl:DatatypeProperty rdf:about="http://xworks.gr/ontologies/ccso#courseType">
        <rdf:type rdf:resource="http://www.w3.org/2002/07/owl#FunctionalProperty"/>
        <rdfs:domain>
            <owl:Class>
                <owl:unionOf rdf:parseType="Collection">
                    <rdf:Description rdf:about="http://xworks.gr/ontologies/ccso#Course"/>
                    <rdf:Description rdf:about="http://xworks.gr/ontologies/ccso#Syllabus"/>
                </owl:unionOf>
            </owl:Class>
        </rdfs:domain>
        <rdfs:range>
            <rdfs:Datatype>
                <owl:oneOf>
                    <rdf:Description>
                        <rdf:type rdf:resource="http://www.w3.org/1999/02/22-rdf-syntax-ns#List"/>
                        <rdf:first>Compulsory</rdf:first>
                        <rdf:rest>
                            <rdf:Description>
                                <rdf:type rdf:resource="http://www.w3.org/1999/02/22-rdf-syntax-ns#List"/>
                                <rdf:first>Core</rdf:first>
                                <rdf:rest>
                                    <rdf:Description>
                                        <rdf:type rdf:resource="http://www.w3.org/1999/02/22-rdf-syntax-ns#List"/>
                                        <rdf:first>Elective</rdf:first>
                                        <rdf:rest rdf:resource="http://www.w3.org/1999/02/22-rdf-syntax-ns#nil"/>
                                    </rdf:Description>
                                </rdf:rest>
                            </rdf:Description>
                        </rdf:rest>
                    </rdf:Description>
                </owl:oneOf>
            </rdfs:Datatype>
        </rdfs:range>
        <rdfs:comment xml:lang="en">The type of the Course. There are two types of course available:
•  Core: Courses that cover core topics and are deemed essential for an academic degree. 
•  Compulsory: A term with the same meaning as “Core” which is used in syllabuses. It’s also expresses the Courses that cover core topics and are deemed essential for an academic degree. 
•  Elective: a Course that the student can select from other alternative courses.</rdfs:comment>
        <rdfs:comment xml:lang="gr">Ο τύπος ενός Μαθήματος. Υπάρχουν δύο διαθέσιμοι τύποι μαθημάτων. 
- Κορμού: Τα μαθήματα που καλύπτουν βασικά θέματα και κρίνονται απαραίτητα για την απόκτηση ακαδημαϊκού πτυχίου. 
- Υποχρεωτικά: Ένας όρος με το ίδιο νόημα όπως τα μαθήματα Κορμού που χρησιμοποιείται στα Περιγράμματα Σπουδών. Χαρακτηρίζει επίσης τα Μαθήματα που καλύπτουν βασικά θεμάτα και κρίνοντια απαραίτητα για την απόκτηση ακαδημαϊκού πτυχίου. 
- Επιλογής: ένα Μάθημα που ο φοιτητής μπορεί να επιλέξει από μία λίστα άλλων μαθημάτων.</rdfs:comment>
    </owl:DatatypeProperty>
    


    <!-- http://xworks.gr/ontologies/ccso#courseURL -->

    <owl:DatatypeProperty rdf:about="http://xworks.gr/ontologies/ccso#courseURL">
        <rdfs:subPropertyOf rdf:resource="http://xworks.gr/ontologies/ccso#webaddressURL"/>
        <rdfs:domain rdf:resource="http://xworks.gr/ontologies/ccso#Syllabus"/>
        <rdfs:range rdf:resource="http://www.w3.org/2001/XMLSchema#anyURI"/>
        <rdfs:comment xml:lang="en">The webpage of a Course where someone can find useful information about the Course, the Syllabus, the Assignments, etc.</rdfs:comment>
        <ns:term_status xml:lang="gr">Η ιστοσελίδα ενός Μαθήματος όπου μπορεί να βρει κανείς χρήσιμες πληροφορίες σχετικά με το Μάθημα, το Περίγραμμο Σπουδών, τις Εργασίες κτλ.</ns:term_status>
    </owl:DatatypeProperty>
    


    <!-- http://xworks.gr/ontologies/ccso#creditsECTS -->

    <owl:DatatypeProperty rdf:about="http://xworks.gr/ontologies/ccso#creditsECTS">
        <rdf:type rdf:resource="http://www.w3.org/2002/07/owl#FunctionalProperty"/>
        <rdfs:domain>
            <owl:Class>
                <owl:unionOf rdf:parseType="Collection">
                    <rdf:Description rdf:about="http://xworks.gr/ontologies/ccso#ProgramofStudy"/>
                    <rdf:Description rdf:about="http://xworks.gr/ontologies/ccso#Syllabus"/>
                </owl:unionOf>
            </owl:Class>
        </rdfs:domain>
        <rdfs:range rdf:resource="http://www.w3.org/2001/XMLSchema#decimal"/>
        <rdfs:comment xml:lang="en">The credits that corresponds to a Study Program or a Course, according to European Credit Transfer and Accumulation System (ECTS).</rdfs:comment>
        <rdfs:comment xml:lang="gr">Οι μονάδες που ανταποκρίνονται στο Πρόγραμμα Σπουδών ή σε ένα Μάθημα, σύμφωνα με το Ευρωπαϊκό σύστημα μεταφοράς και συσσώρευσης ακαδημαϊκών μονάδων (ECTS).</rdfs:comment>
    </owl:DatatypeProperty>
    


    <!-- http://xworks.gr/ontologies/ccso#csName -->

    <owl:DatatypeProperty rdf:about="http://xworks.gr/ontologies/ccso#csName">
        <rdfs:domain>
            <owl:Class>
                <owl:unionOf rdf:parseType="Collection">
                    <rdf:Description rdf:about="http://xworks.gr/ontologies/ccso#Course"/>
                    <rdf:Description rdf:about="http://xworks.gr/ontologies/ccso#Syllabus"/>
                </owl:unionOf>
            </owl:Class>
        </rdfs:domain>
        <rdfs:range rdf:resource="http://www.w3.org/2001/XMLSchema#string"/>
        <rdfs:comment xml:lang="en">The official Name of a Course or a Syllabus.</rdfs:comment>
        <rdfs:comment xml:lang="gr">Το επίσημο Όνομα ενός Μαθήματος ή ενός Προγράμματος Σπουδών.</rdfs:comment>
    </owl:DatatypeProperty>
    


    <!-- http://xworks.gr/ontologies/ccso#dates -->

    <owl:DatatypeProperty rdf:about="http://xworks.gr/ontologies/ccso#dates">
        <rdfs:comment xml:lang="en">Super-property for properties related to date:
•  startDate 
•  endDate 
•  EnrollmentDate
•  graduationDate 
•  pubDate</rdfs:comment>
        <rdfs:comment xml:lang="gr">Υπερ-ιδιότητα για ιδιότητες σχετικές με ημερομηνίες:
•  Ημερομηνία Έναρξης
•  Ημερομηνία Λήξης
•  Ημερομηνία Εγγραφής
•  Ημερομηνία Αποφοίτησης
•  Ημερομηνία pub</rdfs:comment>
    </owl:DatatypeProperty>
    


    <!-- http://xworks.gr/ontologies/ccso#degreeTitle -->

    <owl:DatatypeProperty rdf:about="http://xworks.gr/ontologies/ccso#degreeTitle">
        <rdfs:domain rdf:resource="http://xworks.gr/ontologies/ccso#ProgramofStudy"/>
        <rdfs:range rdf:resource="http://www.w3.org/2001/XMLSchema#string"/>
        <rdfs:comment xml:lang="en">The official title of the Degree that awarded to the students upon a successful completion of Study Program in an educational institution.</rdfs:comment>
        <rdfs:comment xml:lang="gr">Ο επίσημος τίτλος του Πτυχίου που έχει απονεμηθεί στους φοιτητές με την επιτυχή ολοκήρωση του Προγράμματος Σπουδών σε ένα εκπαιδευτικό ίδρυμα.</rdfs:comment>
    </owl:DatatypeProperty>
    


    <!-- http://xworks.gr/ontologies/ccso#degreeType -->

    <owl:DatatypeProperty rdf:about="http://xworks.gr/ontologies/ccso#degreeType">
        <rdfs:domain rdf:resource="http://xworks.gr/ontologies/ccso#ProgramofStudy"/>
        <rdfs:range rdf:resource="http://www.w3.org/2001/XMLSchema#string"/>
        <rdfs:comment xml:lang="en">The various types of studies and degrees.
A specific list of allowed values  in this property can also be used:
•  Bachelor of Science
•  Bachelor of Arts
•  Bachelor of Business Administration
•  Master of Science
•  Master of Arts
•  Master of Business Administration
•  Doctor of Philosophy</rdfs:comment>
        <rdfs:comment xml:lang="gr">Οι διάφοροι τύποι σπουδών και πτυχίων. 
Μπορεί επίσης να χρησιμοποιηθεί μία συγκεκριμένη λίστα με στοιχεία για αυτή την ιδιότητα:
•  Bachelor (Πτυχίο) στις Επιστήμες
•  Bachelor (Πτυχίο) στις Τέχνες
•  Bachelor (Πτυχίο) στη Διοίκηση Επιχειρήσεων
•  Μεταπτυχιακό στις Επιστήμες
•  Μεταπτυχιακό στις Τέχνες
•  Μεταπτυχιακό στη Διοίκηση Επιχειρήσεων
•  Διδακτορικός Τίτλος</rdfs:comment>
    </owl:DatatypeProperty>
    


    <!-- http://xworks.gr/ontologies/ccso#degreeURL -->

    <owl:DatatypeProperty rdf:about="http://xworks.gr/ontologies/ccso#degreeURL">
        <rdfs:subPropertyOf rdf:resource="http://xworks.gr/ontologies/ccso#webaddressURL"/>
        <rdfs:domain rdf:resource="http://xworks.gr/ontologies/ccso#ProgramofStudy"/>
        <rdfs:range rdf:resource="http://www.w3.org/2001/XMLSchema#anyURI"/>
        <rdfs:comment xml:lang="en">The URL of the official webpage with information about the Degree.</rdfs:comment>
        <ns:term_status xml:lang="gr">Το URL της επίσημης ιστοσελίδας με πληροφορίες σχετικά με το Πτυχίο.</ns:term_status>
    </owl:DatatypeProperty>
    


    <!-- http://xworks.gr/ontologies/ccso#description -->

    <owl:DatatypeProperty rdf:about="http://xworks.gr/ontologies/ccso#description">
        <rdfs:range rdf:resource="http://www.w3.org/2001/XMLSchema#string"/>
        <rdfs:comment xml:lang="en">Description of a concept such as:
•  Course
•  Syllabus
•  Event
•  Publication
•  TeachingEvaluationMethod</rdfs:comment>
        <rdfs:comment xml:lang="gr">Περιγραφή μίας έννοιας όπως:
•  Μάθημα
•  Περίγραμμα Σπουδών
•  Γεγονός
•  Έκδοση
•  Μέθοδος Εκπαιδευτικής Αξιολόγησης</rdfs:comment>
    </owl:DatatypeProperty>
    


    <!-- http://xworks.gr/ontologies/ccso#duration -->

    <owl:DatatypeProperty rdf:about="http://xworks.gr/ontologies/ccso#duration">
        <rdfs:domain>
            <owl:Class>
                <owl:unionOf rdf:parseType="Collection">
                    <rdf:Description rdf:about="http://xworks.gr/ontologies/ccso#Event"/>
                    <rdf:Description rdf:about="http://xworks.gr/ontologies/ccso#ProgramofStudy"/>
                    <rdf:Description rdf:about="http://xworks.gr/ontologies/ccso#Syllabus"/>
                    <rdf:Description rdf:about="http://xworks.gr/ontologies/ccso#Topic"/>
                </owl:unionOf>
            </owl:Class>
        </rdfs:domain>
        <rdfs:range rdf:resource="http://www.w3.org/2001/XMLSchema#duration"/>
        <rdfs:comment xml:lang="en">The type represents the duration of time of the following concepts:
•  ProgramofStudy
•  Syllabus
•  Event: represents the minimum amount of time that is required in order to reach the sufficient depth of coverage.
•  Topic.
It is expressed as a number of years, months, days, hours, minutes, and seconds. Valid examples: P4Y=4 years, P6M=6 months, PT2H45M=2 hours and 45 minutes, PT50M=50 minutes.</rdfs:comment>
        <rdfs:comment xml:lang="gr">Αυτός ο τύπος αναπαριστά τη διάρκεια των παρακάτω εννοιών:
•  Πρόγραμμα Σπουδών 
•  Περίγραμμα Σπουδών 
•  Γεγονός: αναπαριστά τον ελάχιστο χρόνο που απαιτείται προκειμένου να καλυφθεί επαρκώς
Αποτυπώνεται ως ένας αριθμός σε χρόνια, μήνες, μέρες, ώρες, λεπτά και δευτερόλεπτα. Παραδείγμα που ισχύουν: P4Y=4 χρόνια, P6M=6 μήνες, PT2H45M=2 ώρες και 45 λεπτά, PT50M=50 λεπτά.</rdfs:comment>
        <rdfs:seeAlso rdf:resource="http://www.datypic.com/sc/xsd11/t-xsd_duration.html"/>
    </owl:DatatypeProperty>
    


    <!-- http://xworks.gr/ontologies/ccso#eClassURL -->

    <owl:DatatypeProperty rdf:about="http://xworks.gr/ontologies/ccso#eClassURL">
        <rdfs:subPropertyOf rdf:resource="http://xworks.gr/ontologies/ccso#webaddressURL"/>
        <rdfs:domain rdf:resource="http://xworks.gr/ontologies/ccso#Syllabus"/>
        <rdfs:range rdf:resource="http://www.w3.org/2001/XMLSchema#anyURI"/>
        <rdfs:comment xml:lang="en">The URL of the Course’s eClass platform.</rdfs:comment>
        <ns:term_status xml:lang="gr">To URL της πλατφόρμας eClass του Μαθήματος.</ns:term_status>
    </owl:DatatypeProperty>
    


    <!-- http://xworks.gr/ontologies/ccso#eContactInfo -->

    <owl:DatatypeProperty rdf:about="http://xworks.gr/ontologies/ccso#eContactInfo">
        <rdfs:comment xml:lang="en">Contact Information of a Person or an Organization for Electonic communication.</rdfs:comment>
        <rdfs:comment xml:lang="gr">Στοιχεία επαφής ενός Προσώπου ή ενός Οργανισμού για Ηλεκτρονική Επικοινωνία.</rdfs:comment>
    </owl:DatatypeProperty>
    


    <!-- http://xworks.gr/ontologies/ccso#endDate -->

    <owl:DatatypeProperty rdf:about="http://xworks.gr/ontologies/ccso#endDate">
        <rdfs:subPropertyOf rdf:resource="http://xworks.gr/ontologies/ccso#dates"/>
        <rdfs:domain rdf:resource="http://xworks.gr/ontologies/ccso#Syllabus"/>
        <rdfs:range rdf:resource="http://www.w3.org/2001/XMLSchema#date"/>
        <rdfs:comment xml:lang="en">The date that the course lessons end (e.g. 2018-01-29).</rdfs:comment>
        <rdfs:comment xml:lang="gr">Η ημερομηνία που λήγουν τα μαθήματα.</rdfs:comment>
        <rdfs:seeAlso rdf:resource="http://www.datypic.com/sc/xsd11/t-xsd_date.html"/>
    </owl:DatatypeProperty>
    


    <!-- http://xworks.gr/ontologies/ccso#enrollmentDate -->

    <owl:DatatypeProperty rdf:about="http://xworks.gr/ontologies/ccso#enrollmentDate">
        <rdfs:subPropertyOf rdf:resource="http://xworks.gr/ontologies/ccso#dates"/>
        <rdfs:domain rdf:resource="http://xworks.gr/ontologies/ccso#Student"/>
        <rdfs:range rdf:resource="http://www.w3.org/2001/XMLSchema#date"/>
        <rdfs:comment xml:lang="en">The exact date that student has enrolled in a Study Program (e.g. 2016-09-01).</rdfs:comment>
        <rdfs:comment xml:lang="gr">Η ακριβής ημερομηνία όπου ο Φοιτητής εγγράφεται στο Πρόγραμμα Σπουδών.</rdfs:comment>
    </owl:DatatypeProperty>
    


    <!-- http://xworks.gr/ontologies/ccso#evaluationInfo -->

    <owl:DatatypeProperty rdf:about="http://xworks.gr/ontologies/ccso#evaluationInfo">
        <rdfs:domain rdf:resource="http://xworks.gr/ontologies/ccso#Syllabus"/>
        <rdfs:range rdf:resource="http://www.w3.org/2001/XMLSchema#string"/>
        <rdfs:comment xml:lang="en">Information about Evaluation and Performance of the Course.</rdfs:comment>
        <rdfs:comment xml:lang="gr">Πληροφορίες σχετικά με την Αξιολόγηση και Επίδοση σε ένα Μάθημα.</rdfs:comment>
    </owl:DatatypeProperty>
    


    <!-- http://xworks.gr/ontologies/ccso#eventClassroom -->

    <owl:DatatypeProperty rdf:about="http://xworks.gr/ontologies/ccso#eventClassroom">
        <rdfs:domain rdf:resource="http://xworks.gr/ontologies/ccso#Event"/>
        <rdfs:range rdf:resource="http://www.w3.org/2001/XMLSchema#string"/>
        <rdfs:comment xml:lang="en">The classroom, laboratory or any other location that the Event takes place.</rdfs:comment>
        <rdfs:comment xml:lang="gr">Η αίθουσα, το εργαστήριο ή οποιοσδήποτε άλλος χώρος που ένα Γεγονός λαμβάνει χώρα.</rdfs:comment>
    </owl:DatatypeProperty>
    


    <!-- http://xworks.gr/ontologies/ccso#eventDateTime -->

    <owl:DatatypeProperty rdf:about="http://xworks.gr/ontologies/ccso#eventDateTime">
        <rdfs:subPropertyOf rdf:resource="http://xworks.gr/ontologies/ccso#dates"/>
        <rdfs:domain rdf:resource="http://xworks.gr/ontologies/ccso#Event"/>
        <rdfs:range rdf:resource="http://www.w3.org/2001/XMLSchema#dateTime"/>
        <rdfs:comment xml:lang="gr">H ημερομηνία και η ώρα που το γεγονός λαμβάνει χώρα. Αν το γεγονός διαρκεί περισσότερες από μια φορές, τότε η τιμή αφορά την ημερομηνία έναρξης του γεγονότος  (π.χ. 2018-03-14T12:30:00 σημαίνει 12:30 μμ στις 14 Μαρτίου, 2018).</rdfs:comment>
        <rdfs:comment xml:lang="en">The date and time the Event occurs. If the event lasts more one time then the value is the date the event is starting (e.g. 2018-03-14T12:30:00 means 12:30 pm at 14 March, 2018).</rdfs:comment>
        <rdfs:seeAlso rdf:resource="http://www.datypic.com/sc/xsd11/t-xsd_dateTime.html"/>
    </owl:DatatypeProperty>
    


    <!-- http://xworks.gr/ontologies/ccso#eventWeekNo -->

    <owl:DatatypeProperty rdf:about="http://xworks.gr/ontologies/ccso#eventWeekNo">
        <rdfs:domain rdf:resource="http://xworks.gr/ontologies/ccso#Event"/>
        <rdfs:range rdf:resource="http://www.w3.org/2001/XMLSchema#short"/>
        <rdfs:comment xml:lang="en">The number of the week in the semester of the Course that the Event occurs.</rdfs:comment>
        <rdfs:comment xml:lang="gr">Ο αριθμός της εβδομάδας σε ένα εξάμηνο ενός Μαθήματος που το γεγονός λαμβάνει χώρα.</rdfs:comment>
    </owl:DatatypeProperty>
    


    <!-- http://xworks.gr/ontologies/ccso#eventWorkload -->

    <owl:DatatypeProperty rdf:about="http://xworks.gr/ontologies/ccso#eventWorkload">
        <rdfs:domain rdf:resource="http://xworks.gr/ontologies/ccso#Event"/>
        <rdfs:range rdf:resource="http://www.w3.org/2001/XMLSchema#duration"/>
        <rdfs:comment xml:lang="en">The workload in hours that required for the learning activities of an Event; the duration of the Event is not included (e.g. PT4H30M=4 hours and 30 minutes, PT90M=90 minutes).</rdfs:comment>
        <rdfs:comment xml:lang="gr">Η δουλειά σε ώρες που απαιτείται για τις μαθησιακές δραστηριότητες ενός Γεγονότος. Η διάρκεια του γεγονότος δε περιλαμβάνεται (Π.χ. PT4H30M=4 ώρες και 30 λεπτά, PT90M=90 λεπτά).</rdfs:comment>
    </owl:DatatypeProperty>
    


    <!-- http://xworks.gr/ontologies/ccso#fsName -->

    <owl:DatatypeProperty rdf:about="http://xworks.gr/ontologies/ccso#fsName">
        <rdfs:domain rdf:resource="http://xworks.gr/ontologies/ccso#FieldofStudy"/>
        <rdfs:range rdf:resource="http://www.w3.org/2001/XMLSchema#string"/>
        <rdfs:comment xml:lang="en">Name of a Discipline.
Name of Body of Knowledge (inherited property).
Name of Area of Knowledge (inherited property).
Name of Unit of Knowledge  (inherited property).</rdfs:comment>
        <rdfs:comment xml:lang="gr">Το όνομα ενός Τομέα. 
Το όνομα ενός Βασικού Κορμού Γνώσης (inherited property). 
Το όνομα μίας Περιοχής Γνώσης (inherited property). 
Το όνομα μίας Μονάδας Γνώσης (inherited property).</rdfs:comment>
    </owl:DatatypeProperty>
    


    <!-- http://xworks.gr/ontologies/ccso#fsTopic -->

    <owl:DatatypeProperty rdf:about="http://xworks.gr/ontologies/ccso#fsTopic">
        <rdfs:domain>
            <owl:Class>
                <owl:unionOf rdf:parseType="Collection">
                    <rdf:Description rdf:about="http://xworks.gr/ontologies/ccso#KnowledgeArea"/>
                    <rdf:Description rdf:about="http://xworks.gr/ontologies/ccso#KnowledgeBody"/>
                    <rdf:Description rdf:about="http://xworks.gr/ontologies/ccso#KnowledgeUnit"/>
                </owl:unionOf>
            </owl:Class>
        </rdfs:domain>
        <rdfs:range rdf:resource="http://www.w3.org/2001/XMLSchema#string"/>
        <rdfs:comment xml:lang="en">Topic of Body of Knowledge.
Topic of Area of Knowledge.
Topic of Unit of Knowledge.</rdfs:comment>
        <rdfs:comment xml:lang="gr">Το θέμα ενός Βασικού Κορμού Γνώσης.
Το θέμα μίας Περιοχής Γνώσης. 
Το θέμα μίας Μονάδας Γνώσης.</rdfs:comment>
    </owl:DatatypeProperty>
    


    <!-- http://xworks.gr/ontologies/ccso#graduationDate -->

    <owl:DatatypeProperty rdf:about="http://xworks.gr/ontologies/ccso#graduationDate">
        <rdfs:subPropertyOf rdf:resource="http://xworks.gr/ontologies/ccso#dates"/>
        <rdfs:domain rdf:resource="http://xworks.gr/ontologies/ccso#Student"/>
        <rdfs:range rdf:resource="http://www.w3.org/2001/XMLSchema#date"/>
        <rdfs:comment xml:lang="en">The exact date that student has graduated a Study Program (e.g. 2017-03-15).</rdfs:comment>
        <rdfs:comment xml:lang="gr">Η ακριβής ημερομηνία που ο Φοιτητής έχει αποφοιτήσει από ένα Πρόγραμμα Σπουδών  (π.χ. 2017-03-15).</rdfs:comment>
    </owl:DatatypeProperty>
    


    <!-- http://xworks.gr/ontologies/ccso#homePhone -->

    <owl:DatatypeProperty rdf:about="http://xworks.gr/ontologies/ccso#homePhone">
        <rdfs:subPropertyOf rdf:resource="http://xworks.gr/ontologies/ccso#phone"/>
        <rdfs:domain rdf:resource="http://xmlns.com/foaf/0.1/Person"/>
        <rdfs:range rdf:resource="http://www.w3.org/2001/XMLSchema#string"/>
        <rdfs:comment xml:lang="en">The phone number at the home of a person.</rdfs:comment>
        <rdfs:isDefinedBy rdf:resource="http://schema.org/telephone"/>
        <ns:term_status xml:lang="gr">Ο αριθμός τηλεφώνου στο σπίτι ενός Προσώπου.</ns:term_status>
    </owl:DatatypeProperty>
    


    <!-- http://xworks.gr/ontologies/ccso#label -->

    <owl:DatatypeProperty rdf:about="http://xworks.gr/ontologies/ccso#label">
        <rdfs:domain>
            <owl:Class>
                <owl:unionOf rdf:parseType="Collection">
                    <rdf:Description rdf:about="http://xworks.gr/ontologies/ccso#Event"/>
                    <rdf:Description rdf:about="http://xworks.gr/ontologies/ccso#LearningOutcome"/>
                    <rdf:Description rdf:about="http://xworks.gr/ontologies/ccso#Topic"/>
                </owl:unionOf>
            </owl:Class>
        </rdfs:domain>
        <rdfs:range rdf:resource="http://www.w3.org/2001/XMLSchema#string"/>
        <rdfs:comment xml:lang="en">The Name of an Event, a Topic or a LearningOutcome.</rdfs:comment>
        <rdfs:comment xml:lang="gr">Το Όνομα ενός Γεγονότος, ενός Θέματος ή ενός Μαθησιακού Αποτελέσματος.</rdfs:comment>
    </owl:DatatypeProperty>
    


    <!-- http://xworks.gr/ontologies/ccso#language -->

    <owl:DatatypeProperty rdf:about="http://xworks.gr/ontologies/ccso#language">
        <rdfs:domain>
            <owl:Class>
                <owl:unionOf rdf:parseType="Collection">
                    <rdf:Description rdf:about="http://xworks.gr/ontologies/ccso#Event"/>
                    <rdf:Description rdf:about="http://xworks.gr/ontologies/ccso#Syllabus"/>
                </owl:unionOf>
            </owl:Class>
        </rdfs:domain>
        <rdfs:range rdf:resource="http://www.w3.org/2001/XMLSchema#language"/>
        <rdfs:comment xml:lang="en">The Language that used during the lessons, at the assignments and at the evaluation tests of a Course.(e.g. &apos;en&apos; for English, &apos;gr&apos; for Greek).</rdfs:comment>
        <rdfs:comment xml:lang="gr">Η Γλώσσα που χρησιμοποιείται στη διάρκεια των μαθημάτων, στις εργασίες και στα τεστ αξιολόγησης ενός Μαθήματος (π.χ. &apos;en&apos; για Αγγλικά, &apos;gr&apos; για Ελληνικά).</rdfs:comment>
        <rdfs:seeAlso rdf:resource="http://www.datypic.com/sc/xsd11/t-xsd_language.html"/>
    </owl:DatatypeProperty>
    


    <!-- http://xworks.gr/ontologies/ccso#levelofMastery -->

    <owl:DatatypeProperty rdf:about="http://xworks.gr/ontologies/ccso#levelofMastery">
        <rdfs:domain rdf:resource="http://xworks.gr/ontologies/ccso#LearningOutcome"/>
        <rdfs:range>
            <rdfs:Datatype>
                <owl:oneOf>
                    <rdf:Description>
                        <rdf:type rdf:resource="http://www.w3.org/1999/02/22-rdf-syntax-ns#List"/>
                        <rdf:first>Assessment</rdf:first>
                        <rdf:rest>
                            <rdf:Description>
                                <rdf:type rdf:resource="http://www.w3.org/1999/02/22-rdf-syntax-ns#List"/>
                                <rdf:first>Familiarity</rdf:first>
                                <rdf:rest>
                                    <rdf:Description>
                                        <rdf:type rdf:resource="http://www.w3.org/1999/02/22-rdf-syntax-ns#List"/>
                                        <rdf:first>Usage</rdf:first>
                                        <rdf:rest rdf:resource="http://www.w3.org/1999/02/22-rdf-syntax-ns#nil"/>
                                    </rdf:Description>
                                </rdf:rest>
                            </rdf:Description>
                        </rdf:rest>
                    </rdf:Description>
                </owl:oneOf>
            </rdfs:Datatype>
        </rdfs:range>
        <rdfs:comment xml:lang="en">Each Learning Outcome has an associated Level of Mastery students are expected to achieve with respect to the Topics specified.
There are three Level of Mastery:
•  Familiarity:  student understands what a concept is or what it means.
•  Usage:  student is able to use and apply a concept.
•  Assessment:  student is able to consider a concept from multiple viewpoints and select the appropriate approach for a problem.</rdfs:comment>
        <rdfs:comment xml:lang="gr">Κάθε Μαθησιακό Αποτέλεσμα συνδέεται με ένα Επίπεδο Κεκτημένης Γνώσης που αναμένεται να έχουν οι φοιτητές σε τρεις συγκεκριμένους τομείς:
•  Εξοικείωση: όταν ο φοιτητής καταλαβαίνει τι είναι ή τι σημαίνει μία έννοια. 
•  Χρήση/Εφαρμογή: όταν ο φοιτητής μπορεί να χρησιμοποιήσει ή να εφαρμόσει μία έννοια. 
•  Αξιολόγηση: όταν ο φοιτητής μπορεί να εξετάσει μία έννοια από διάφορες οπτικές και να διαλέξει την κατάλληλη προσέγγιση για ένα πρόβλημα.</rdfs:comment>
    </owl:DatatypeProperty>
    


    <!-- http://xworks.gr/ontologies/ccso#mediaUsed -->

    <owl:DatatypeProperty rdf:about="http://xworks.gr/ontologies/ccso#mediaUsed">
        <rdfs:domain rdf:resource="http://xworks.gr/ontologies/ccso#TeachingEvaluationMethod"/>
        <rdfs:range rdf:resource="http://www.w3.org/2001/XMLSchema#string"/>
        <rdfs:comment xml:lang="en">The devices, tools and objects that are used to store and deliver teaching and learning content and data.</rdfs:comment>
        <rdfs:comment xml:lang="gr">Οι συσκευές, τα εργαλεία και τα αντικείμενα που χρησιμοποιούνται για να αποθηκεύεται και να διανέμεται το μαθησιακό περιεχόμενο και τα σχετικά με αυτό δεδομένα.</rdfs:comment>
    </owl:DatatypeProperty>
    


    <!-- http://xworks.gr/ontologies/ccso#methodName -->

    <owl:DatatypeProperty rdf:about="http://xworks.gr/ontologies/ccso#methodName">
        <rdfs:domain rdf:resource="http://xworks.gr/ontologies/ccso#TeachingEvaluationMethod"/>
        <rdfs:range>
            <rdfs:Datatype>
                <owl:oneOf>
                    <rdf:Description>
                        <rdf:type rdf:resource="http://www.w3.org/1999/02/22-rdf-syntax-ns#List"/>
                        <rdf:first>Demonstration</rdf:first>
                        <rdf:rest>
                            <rdf:Description>
                                <rdf:type rdf:resource="http://www.w3.org/1999/02/22-rdf-syntax-ns#List"/>
                                <rdf:first>Discussion</rdf:first>
                                <rdf:rest>
                                    <rdf:Description>
                                        <rdf:type rdf:resource="http://www.w3.org/1999/02/22-rdf-syntax-ns#List"/>
                                        <rdf:first>Homework</rdf:first>
                                        <rdf:rest>
                                            <rdf:Description>
                                                <rdf:type rdf:resource="http://www.w3.org/1999/02/22-rdf-syntax-ns#List"/>
                                                <rdf:first>Laboratory</rdf:first>
                                                <rdf:rest>
                                                    <rdf:Description>
                                                        <rdf:type rdf:resource="http://www.w3.org/1999/02/22-rdf-syntax-ns#List"/>
                                                        <rdf:first>Lecture</rdf:first>
                                                        <rdf:rest>
                                                            <rdf:Description>
                                                                <rdf:type rdf:resource="http://www.w3.org/1999/02/22-rdf-syntax-ns#List"/>
                                                                <rdf:first>OralExamination</rdf:first>
                                                                <rdf:rest>
                                                                    <rdf:Description>
                                                                        <rdf:type rdf:resource="http://www.w3.org/1999/02/22-rdf-syntax-ns#List"/>
                                                                        <rdf:first>Project</rdf:first>
                                                                        <rdf:rest>
                                                                            <rdf:Description>
                                                                                <rdf:type rdf:resource="http://www.w3.org/1999/02/22-rdf-syntax-ns#List"/>
                                                                                <rdf:first>Seminar</rdf:first>
                                                                                <rdf:rest>
                                                                                    <rdf:Description>
                                                                                        <rdf:type rdf:resource="http://www.w3.org/1999/02/22-rdf-syntax-ns#List"/>
                                                                                        <rdf:first>Study</rdf:first>
                                                                                        <rdf:rest>
                                                                                            <rdf:Description>
                                                                                                <rdf:type rdf:resource="http://www.w3.org/1999/02/22-rdf-syntax-ns#List"/>
                                                                                                <rdf:first>WrittenExamination</rdf:first>
                                                                                                <rdf:rest>
                                                                                                    <rdf:Description>
                                                                                                        <rdf:type rdf:resource="http://www.w3.org/1999/02/22-rdf-syntax-ns#List"/>
                                                                                                        <rdf:first>other</rdf:first>
                                                                                                        <rdf:rest rdf:resource="http://www.w3.org/1999/02/22-rdf-syntax-ns#nil"/>
                                                                                                    </rdf:Description>
                                                                                                </rdf:rest>
                                                                                            </rdf:Description>
                                                                                        </rdf:rest>
                                                                                    </rdf:Description>
                                                                                </rdf:rest>
                                                                            </rdf:Description>
                                                                        </rdf:rest>
                                                                    </rdf:Description>
                                                                </rdf:rest>
                                                            </rdf:Description>
                                                        </rdf:rest>
                                                    </rdf:Description>
                                                </rdf:rest>
                                            </rdf:Description>
                                        </rdf:rest>
                                    </rdf:Description>
                                </rdf:rest>
                            </rdf:Description>
                        </rdf:rest>
                    </rdf:Description>
                </owl:oneOf>
            </rdfs:Datatype>
        </rdfs:range>
        <rdfs:comment xml:lang="en">The name of the Method that is followed in a Teaching or Evaluation Event.
There is a specific list of allowed values, for this property: 
•  Lecture: the instructor oral presents the subject or teaches people with little interaction.
•  Demonstration: involves showing by reason or proof, explaining or making clear by use of examples or experiments.
•  Discussion: the subject is being examined and discussed  in the classroom where each student has equal opportunity to interact and put forth his views.
•  Seminar: the students prepare by themselves and present their work for discussion and critique.
•  Study: the instructor assigns readings for each session which are then discussed in a meeting or a conference.
•  Homework: students are writing short or long papers or essays about a topic, solving problem sets, etc.
•  Laboratory: most of the work is taken place in a laboratory.
•  Project: students are organized in one or more groups, work on a topic and meet with the instructor weekly for discussion and guidance.
•  OralExam: the examiner poses questions to the student or group of students who have to answer in order to demonstrate sufficient knowledge about the subject.
•  WrittenExam: the students participate in a written examination which intended to measure student’s knowledge, skills and attitude.</rdfs:comment>
        <rdfs:comment xml:lang="gr">Το όνομα της μεθόδου που ακολουθείται σε μια διδασκαλία ή σε μία αξιολόγηση.
Υπάρχει ένας συγκεκριμένος κατάλογος επιτρεπόμενων τιμών, για αυτήν την ιδιότητα:
•  Διάλεξη: ο εκπαιδευτής παρουσιάζει προφορικά το θέμα ή διδάσκει άτομα με ένα μικρό επίπεδο αλληλεπίδρασης.
•  Επίδειξη: περιλαμβάνει την επίδειξη με βάση τα αιτία ή με αποδείξεις, εξηγώντας ή διευκρινίζοντας με τη χρήση παραδειγμάτων ή πειραμάτων.
•  Συζήτηση: το θέμα εξετάζεται και συζητείται στην τάξη, όπου ο κάθε φοιτητής έχει ίσες ευκαιρίες με τους υπόλοιπους να αλληλεπιδράσει και να εκθέσει τις απόψεις του.
•  Σεμινάριο: οι φοιτητές προετοιμάζονται από μόνοι τους και παρουσιάζουν το έργο τους για συζήτηση και κριτική.
•  Μελέτη: ο εκπαιδευτής αναθέτει κείμενα/εργασίες για κάθε συνάντηση, τα οποία στη συνέχεια συζητούνται σε μια συνάντηση ή σε μια διάσκεψη.
•  Εργασία στο σπίτι: οι φοιτητές γράφουν μικρά ή μεγάλα κείμενα ή δοκίμια για ένα θέμα, επιλύουν προβλήματα κ.λπ.
•  Εργαστήριο: το μεγαλύτερο μέρος των εργασιών πραγματοποιείται σε εργαστήριο.
•  Έργο: οι φοιτητές οργανώνονται σε μία ή περισσότερες ομάδες, εργάζονται πάνω σε ένα θέμα και συναντώνται με τον εκπαιδευτή εβδομαδιαίως για συζήτηση και καθοδήγηση.
•  OralExam: ο εξεταστής θέτει ερωτήσεις στον φοιτητή ή την ομάδα των φοιτητών που πρέπει να απαντήσουν για να δείξουν την επαρκή γνώση σχετικά με το εξεταζόμενο θέμα.
•  WrittenExam: οι φοιτητές συμμετέχουν σε γραπτή εξέταση που αποσκοπεί στη αριθμητική αξιολόγηση των γνώσεων, δεξιοτήτων και ικανοτήτων τους.</rdfs:comment>
    </owl:DatatypeProperty>
    


    <!-- http://xworks.gr/ontologies/ccso#mobilePhone -->

    <owl:DatatypeProperty rdf:about="http://xworks.gr/ontologies/ccso#mobilePhone">
        <rdfs:subPropertyOf rdf:resource="http://xworks.gr/ontologies/ccso#phone"/>
        <rdfs:domain rdf:resource="http://xmlns.com/foaf/0.1/Person"/>
        <rdfs:range rdf:resource="http://www.w3.org/2001/XMLSchema#string"/>
        <rdfs:comment xml:lang="en">The mobile’s phone number of a person.</rdfs:comment>
        <rdfs:isDefinedBy rdf:resource="http://schema.org/telephone"/>
        <ns:term_status xml:lang="gr">Ο αριθμός του κινητού τηλεφώνου ενός Προσώπου.</ns:term_status>
    </owl:DatatypeProperty>
    


    <!-- http://xworks.gr/ontologies/ccso#offeredtoErasmus -->

    <owl:DatatypeProperty rdf:about="http://xworks.gr/ontologies/ccso#offeredtoErasmus">
        <rdf:type rdf:resource="http://www.w3.org/2002/07/owl#FunctionalProperty"/>
        <rdfs:domain rdf:resource="http://xworks.gr/ontologies/ccso#Syllabus"/>
        <rdfs:range rdf:resource="http://www.w3.org/2001/XMLSchema#boolean"/>
        <rdfs:comment xml:lang="en">A Course can be offered to Erasmus students or not.</rdfs:comment>
        <rdfs:comment xml:lang="gr">Το Μάθημα μπορεί να προσφερθεί σε φοιτητές Erasmus ή όχι.</rdfs:comment>
    </owl:DatatypeProperty>
    


    <!-- http://xworks.gr/ontologies/ccso#officeHours -->

    <owl:DatatypeProperty rdf:about="http://xworks.gr/ontologies/ccso#officeHours">
        <rdfs:domain rdf:resource="http://xworks.gr/ontologies/ccso#Employee"/>
        <rdfs:range rdf:resource="http://www.w3.org/2001/XMLSchema#string"/>
        <rdfs:comment xml:lang="en">Dates and time that the Person is available at his office</rdfs:comment>
        <rdfs:comment xml:lang="gr">Οι ημερομηνίες και οι ώρες που ένα Πρόσωπο είναι διαθέσιμο στο γραφείο του.</rdfs:comment>
    </owl:DatatypeProperty>
    


    <!-- http://xworks.gr/ontologies/ccso#officeNo -->

    <owl:DatatypeProperty rdf:about="http://xworks.gr/ontologies/ccso#officeNo">
        <rdfs:domain rdf:resource="http://xworks.gr/ontologies/ccso#Employee"/>
        <rdfs:range rdf:resource="http://www.w3.org/2001/XMLSchema#string"/>
        <rdfs:comment xml:lang="en">The number and building of employee’s office.</rdfs:comment>
        <rdfs:comment xml:lang="gr">Ο αριθμός και το κτήριο όπου βρίσκεται το γραφείο ενός εργαζόμενου.</rdfs:comment>
    </owl:DatatypeProperty>
    


    <!-- http://xworks.gr/ontologies/ccso#personID -->

    <owl:DatatypeProperty rdf:about="http://xworks.gr/ontologies/ccso#personID">
        <rdf:type rdf:resource="http://www.w3.org/2002/07/owl#FunctionalProperty"/>
        <rdfs:domain rdf:resource="http://xmlns.com/foaf/0.1/Person"/>
        <rdfs:range rdf:resource="http://www.w3.org/2000/01/rdf-schema#Literal"/>
        <rdfs:comment xml:lang="en">Person’s identifier that uniquely identifies a person.</rdfs:comment>
        <ns:term_status xml:lang="gr">Το αναγνωριστικό ενός προσώπου που χαρακτηρίζει ένα πρόσωπο.</ns:term_status>
    </owl:DatatypeProperty>
    


    <!-- http://xworks.gr/ontologies/ccso#phone -->

    <owl:DatatypeProperty rdf:about="http://xworks.gr/ontologies/ccso#phone">
        <rdfs:comment xml:lang="en">Contact numbers of a Person or an Organization for phonetic communication.</rdfs:comment>
        <ns:term_status xml:lang="gr">Οι αριθμοί επικοινωνίας ενός Προσώπου ή ενός Οργανισμού για τηλεφωνική επικοινωνία.</ns:term_status>
    </owl:DatatypeProperty>
    


    <!-- http://xworks.gr/ontologies/ccso#profilePic -->

    <owl:DatatypeProperty rdf:about="http://xworks.gr/ontologies/ccso#profilePic">
        <rdfs:domain rdf:resource="http://xmlns.com/foaf/0.1/Person"/>
        <rdfs:range rdf:resource="http://www.w3.org/2001/XMLSchema#anyURI"/>
        <rdfs:comment xml:lang="en">An associated profile picture of a person.</rdfs:comment>
        <ns:term_status xml:lang="gr">Μία σχετική φωτογραφία προφίλ ενός προσώπου.</ns:term_status>
    </owl:DatatypeProperty>
    


    <!-- http://xworks.gr/ontologies/ccso#psName -->

    <owl:DatatypeProperty rdf:about="http://xworks.gr/ontologies/ccso#psName">
        <rdfs:domain rdf:resource="http://xworks.gr/ontologies/ccso#ProgramofStudy"/>
        <rdfs:range rdf:resource="http://www.w3.org/2001/XMLSchema#string"/>
        <rdfs:comment xml:lang="en">The official Name of Program of Study.</rdfs:comment>
        <ns:term_status xml:lang="gr">Το επίσημο όνομα ενός Πρoγράμματος Σπουδών.</ns:term_status>
    </owl:DatatypeProperty>
    


    <!-- http://xworks.gr/ontologies/ccso#pubURL -->

    <owl:DatatypeProperty rdf:about="http://xworks.gr/ontologies/ccso#pubURL">
        <rdfs:subPropertyOf rdf:resource="http://xworks.gr/ontologies/ccso#webaddressURL"/>
        <rdfs:range rdf:resource="http://www.w3.org/2001/XMLSchema#string"/>
        <rdfs:comment xml:lang="en">The URL of the published work.</rdfs:comment>
        <ns:term_status xml:lang="gr">To URL των έργων που έχουν εκδοθεί.</ns:term_status>
    </owl:DatatypeProperty>
    


    <!-- http://xworks.gr/ontologies/ccso#resourceCitation -->

    <owl:DatatypeProperty rdf:about="http://xworks.gr/ontologies/ccso#resourceCitation">
        <rdfs:domain rdf:resource="http://xworks.gr/ontologies/ccso#Resource"/>
        <rdfs:range rdf:resource="http://www.w3.org/2001/XMLSchema#string"/>
        <rdfs:comment xml:lang="en">The official cited reference for the published learning material or  unofficial in case it isn’t published.</rdfs:comment>
        <ns:term_status xml:lang="gr">Η επίσημη αναφορά που έχει παρατεθεί σε ένα μαθησιακό υλικό που έχει εκδοθεί ή η ανεπίσημη σε περίπτωση που δεν έχει εκδοθεί.</ns:term_status>
    </owl:DatatypeProperty>
    


    <!-- http://xworks.gr/ontologies/ccso#semesterinProgram -->

    <owl:DatatypeProperty rdf:about="http://xworks.gr/ontologies/ccso#semesterinProgram">
        <rdfs:domain rdf:resource="http://xworks.gr/ontologies/ccso#Syllabus"/>
        <rdfs:range rdf:resource="http://www.w3.org/2001/XMLSchema#short"/>
        <rdfs:comment xml:lang="en">The number of semester within the ProgramofStudy where the Course is offered and starts (e.g. 3).</rdfs:comment>
        <ns:term_status xml:lang="gr">Ο αριθμός του εξαμήνου στο Πρόγραμμα Σπουδών όπου το Μάθημα προσφέρεται και ξεκινά (π.χ. 3).</ns:term_status>
    </owl:DatatypeProperty>
    


    <!-- http://xworks.gr/ontologies/ccso#staffPosition -->

    <owl:DatatypeProperty rdf:about="http://xworks.gr/ontologies/ccso#staffPosition">
        <rdfs:domain rdf:resource="http://xworks.gr/ontologies/ccso#Employee"/>
        <rdfs:range rdf:resource="http://www.w3.org/2001/XMLSchema#string"/>
        <rdfs:comment xml:lang="en">The position where a person is being employed in the organization.</rdfs:comment>
        <ns:term_status xml:lang="gr">Η θέση στην οποία ένα πρόσωπο απασχολείται μέσα σε έναν οργανισμό.</ns:term_status>
    </owl:DatatypeProperty>
    


    <!-- http://xworks.gr/ontologies/ccso#staffSpecialization -->

    <owl:DatatypeProperty rdf:about="http://xworks.gr/ontologies/ccso#staffSpecialization">
        <rdfs:domain rdf:resource="http://xworks.gr/ontologies/ccso#Employee"/>
        <rdfs:range rdf:resource="http://www.w3.org/2001/XMLSchema#string"/>
        <rdfs:comment xml:lang="en">The subject that a person is specialist and practices in.</rdfs:comment>
        <ns:term_status xml:lang="gr">Το αντικείμενο στο οποίο ένα πρόσωπο είναι εξειδικευμένο και εξασκεί.</ns:term_status>
    </owl:DatatypeProperty>
    


    <!-- http://xworks.gr/ontologies/ccso#startDate -->

    <owl:DatatypeProperty rdf:about="http://xworks.gr/ontologies/ccso#startDate">
        <rdfs:subPropertyOf rdf:resource="http://xworks.gr/ontologies/ccso#dates"/>
        <rdfs:domain rdf:resource="http://xworks.gr/ontologies/ccso#Syllabus"/>
        <rdfs:range rdf:resource="http://www.w3.org/2001/XMLSchema#date"/>
        <rdfs:comment xml:lang="en">The date that the course lessons start (e.g. 2017-10-01).</rdfs:comment>
        <rdfs:comment xml:lang="gr">Η ημερομηνία που ένα μάθημα ξεκινά.</rdfs:comment>
        <rdfs:seeAlso rdf:resource="http://www.datypic.com/sc/xsd11/t-xsd_date.html"/>
    </owl:DatatypeProperty>
    


    <!-- http://xworks.gr/ontologies/ccso#topicType -->

    <owl:DatatypeProperty rdf:about="http://xworks.gr/ontologies/ccso#topicType">
        <rdfs:domain rdf:resource="http://xworks.gr/ontologies/ccso#Topic"/>
        <rdfs:range>
            <rdfs:Datatype>
                <owl:oneOf>
                    <rdf:Description>
                        <rdf:type rdf:resource="http://www.w3.org/1999/02/22-rdf-syntax-ns#List"/>
                        <rdf:first>Core</rdf:first>
                        <rdf:rest>
                            <rdf:Description>
                                <rdf:type rdf:resource="http://www.w3.org/1999/02/22-rdf-syntax-ns#List"/>
                                <rdf:first>Core-Tier-1</rdf:first>
                                <rdf:rest>
                                    <rdf:Description>
                                        <rdf:type rdf:resource="http://www.w3.org/1999/02/22-rdf-syntax-ns#List"/>
                                        <rdf:first>Core-Tier-2</rdf:first>
                                        <rdf:rest>
                                            <rdf:Description>
                                                <rdf:type rdf:resource="http://www.w3.org/1999/02/22-rdf-syntax-ns#List"/>
                                                <rdf:first>Elective</rdf:first>
                                                <rdf:rest rdf:resource="http://www.w3.org/1999/02/22-rdf-syntax-ns#nil"/>
                                            </rdf:Description>
                                        </rdf:rest>
                                    </rdf:Description>
                                </rdf:rest>
                            </rdf:Description>
                        </rdf:rest>
                    </rdf:Description>
                </owl:oneOf>
            </rdfs:Datatype>
        </rdfs:range>
        <rdfs:comment xml:lang="en">The type of the Topic defines the importance of the topic for inclusion in a study programme.
The types of a topic could be the values: 
•  Core
•  Core-Tier-1
•  Core-Tier-2
•  Elective</rdfs:comment>
        <ns:term_status xml:lang="gr">Ο τύπος ενός Θέματος καθορίζει τη σημασία ενός θέματος προκειμένου να συμπεριληφθεί σε ένα πρόγραμμα σπουδών. 
Οι τύπου ενός θέματος μπορεί να έχει τις εξής τιμές:
•  Κορμού
•  Κορμού - Βαθμίδα 1
•  Κορμού - Βαθμίδα 2
•  Επιλογής</ns:term_status>
    </owl:DatatypeProperty>
    


    <!-- http://xworks.gr/ontologies/ccso#versionNo -->

    <owl:DatatypeProperty rdf:about="http://xworks.gr/ontologies/ccso#versionNo">
        <rdfs:domain>
            <owl:Class>
                <owl:unionOf rdf:parseType="Collection">
                    <rdf:Description rdf:about="http://xworks.gr/ontologies/ccso#Resource"/>
                    <rdf:Description rdf:about="http://xworks.gr/ontologies/ccso#Syllabus"/>
                </owl:unionOf>
            </owl:Class>
        </rdfs:domain>
        <rdfs:range rdf:resource="http://www.w3.org/2001/XMLSchema#decimal"/>
        <rdfs:comment xml:lang="en">The version number of a Publication.
The version number of a Syllabus.</rdfs:comment>
        <ns:term_status xml:lang="gr">Ο αριθμός έκδοσης μίας Δημοσίευσης. 
Ο αριθμός έκδοσης ενός Περιγράμματος Σπουδών.</ns:term_status>
    </owl:DatatypeProperty>
    


    <!-- http://xworks.gr/ontologies/ccso#webaddressURL -->

    <owl:DatatypeProperty rdf:about="http://xworks.gr/ontologies/ccso#webaddressURL">
        <rdfs:comment xml:lang="en">Super-property for properties related to URL:
•  degreeURL
•  courseURL
•  eClassURL
•  pubURL</rdfs:comment>
        <ns:term_status xml:lang="gr">Υπερ-ιδιότητα για ιδιότητες που σχετίζονται με ένα URL:
• degreeURL
• courseURL
• eClassURL
• pubURL</ns:term_status>
    </owl:DatatypeProperty>
    


    <!-- http://xworks.gr/ontologies/ccso#weeklyClassSchedule -->

    <owl:DatatypeProperty rdf:about="http://xworks.gr/ontologies/ccso#weeklyClassSchedule">
        <rdfs:domain rdf:resource="http://xworks.gr/ontologies/ccso#Syllabus"/>
        <rdfs:range rdf:resource="http://www.w3.org/2001/XMLSchema#string"/>
        <rdfs:comment xml:lang="en">The weekly class schedule presents the time, day and dates that the events of the Course are scheduled.</rdfs:comment>
        <ns:term_status xml:lang="gr">Το εβδομαδιαίο πρόγραμμα που περιλαμβάνει την ώρα, την ημέρα και τις ημερομηνίες του Μαθήματος όπως έχουν προγραμματιστεί.</ns:term_status>
    </owl:DatatypeProperty>
    


    <!-- http://xworks.gr/ontologies/ccso#weeklyHours -->

    <owl:DatatypeProperty rdf:about="http://xworks.gr/ontologies/ccso#weeklyHours">
        <rdfs:domain rdf:resource="http://xworks.gr/ontologies/ccso#Syllabus"/>
        <rdfs:range rdf:resource="http://www.w3.org/2001/XMLSchema#duration"/>
        <rdfs:comment xml:lang="en">The weekly teaching hours of the course.</rdfs:comment>
        <ns:term_status xml:lang="gr">Οι διδακτικές ώρες ενός μαθήματος μέσα σε μία εβδομάδα.</ns:term_status>
    </owl:DatatypeProperty>
    


    <!-- http://xworks.gr/ontologies/ccso#weeklyWorkload -->

    <owl:DatatypeProperty rdf:about="http://xworks.gr/ontologies/ccso#weeklyWorkload">
        <rdfs:domain rdf:resource="http://xworks.gr/ontologies/ccso#Syllabus"/>
        <rdfs:range rdf:resource="http://www.w3.org/2001/XMLSchema#duration"/>
        <rdfs:comment xml:lang="en">The workload in hours that required for the learning activities and assignments of a Course in weekly basis. The hours of the lessons are not included (e.g. PT3H50M=3 hours and 50 minutes, PT60M=60 minutes).</rdfs:comment>
        <ns:term_status xml:lang="gr">Η δουλειά σε ώρες που απαιτούνται για τις μαθησιακές δραστηριότητες και τις εργασίες σε ένα Μάθημα σε εβδομαδιαία βάση. Οι ώρες των μαθημάτων δεν συμπεριλαμβάνονται (π.χ.  PT3H50M=3 ώρες και 50 λεπτά, PT60M=60 λεπτά).</ns:term_status>
    </owl:DatatypeProperty>
    


    <!-- http://xworks.gr/ontologies/ccso#workEmail -->

    <owl:DatatypeProperty rdf:about="http://xworks.gr/ontologies/ccso#workEmail">
        <rdfs:subPropertyOf rdf:resource="http://xworks.gr/ontologies/ccso#eContactInfo"/>
        <rdfs:domain rdf:resource="http://xmlns.com/foaf/0.1/Person"/>
        <rdfs:range rdf:resource="http://www.w3.org/2001/XMLSchema#anyURI"/>
        <rdfs:comment xml:lang="en">The work eMail address of a person.</rdfs:comment>
        <rdfs:comment xml:lang="gr">Η ηλεκτρονική διεύθυνση εργασίας ενός Προσώπου.</rdfs:comment>
        <rdfs:isDefinedBy rdf:resource="http://schema.org/email"/>
    </owl:DatatypeProperty>
    


    <!-- http://xworks.gr/ontologies/ccso#workPhone -->

    <owl:DatatypeProperty rdf:about="http://xworks.gr/ontologies/ccso#workPhone">
        <rdfs:subPropertyOf rdf:resource="http://xworks.gr/ontologies/ccso#phone"/>
        <rdfs:domain>
            <owl:Class>
                <owl:unionOf rdf:parseType="Collection">
                    <rdf:Description rdf:about="http://schema.org/EducationalOrganization"/>
                    <rdf:Description rdf:about="http://xmlns.com/foaf/0.1/Person"/>
                </owl:unionOf>
            </owl:Class>
        </rdfs:domain>
        <rdfs:range rdf:resource="http://www.w3.org/2001/XMLSchema#string"/>
        <rdfs:comment xml:lang="en">The main phone number of an Organization or at the work of a Person.</rdfs:comment>
        <rdfs:isDefinedBy rdf:resource="http://schema.org/telephone"/>
        <ns:term_status xml:lang="gr">Ο κύριος αριθμός τηλεφώνου ενός οργανισμού ή της εργασίας ενός Προσώπου.</ns:term_status>
    </owl:DatatypeProperty>
    


    <!-- 
    ///////////////////////////////////////////////////////////////////////////////////////
    //
    // Classes
    //
    ///////////////////////////////////////////////////////////////////////////////////////
     -->

    


    <!-- http://schema.org/EducationalOrganization -->

    <owl:Class rdf:about="http://schema.org/EducationalOrganization">
        <rdfs:subClassOf rdf:resource="http://schema.org/Organization"/>
        <owl:disjointWith rdf:resource="http://www.w3.org/2000/10/swap/pim/contact#Person"/>
        <owl:disjointWith rdf:resource="http://xworks.gr/ontologies/ccso#Discipline"/>
        <owl:disjointWith rdf:resource="http://xworks.gr/ontologies/ccso#FieldofStudy"/>
        <owl:disjointWith rdf:resource="http://xworks.gr/ontologies/ccso#KnowledgeArea"/>
        <owl:disjointWith rdf:resource="http://xworks.gr/ontologies/ccso#KnowledgeBody"/>
        <owl:disjointWith rdf:resource="http://xworks.gr/ontologies/ccso#KnowledgeUnit"/>
        <rdfs:comment xml:lang="en">An Organization designed to provide educational services and learning environments.</rdfs:comment>
        <rdfs:comment xml:lang="gr">Ένας Οργανισμός που έχει σχεδιαστεί για την παροχή εκπαιδευτικών υπηρεσιών και μαθησιακών περιβαλλόντων.</rdfs:comment>
        <rdfs:isDefinedBy rdf:resource="http://schema.org/EducationalOrganization"/>
        <rdfs:label xml:lang="gr">Εκπαιδευτικός Οργανισμός</rdfs:label>
    </owl:Class>
    


    <!-- http://schema.org/Organization -->

    <owl:Class rdf:about="http://schema.org/Organization">
        <rdfs:comment xml:lang="en">An organization is an entity comprising multiple people, such as an institution or an association, that has a collective goal and is linked to an external environment.</rdfs:comment>
    </owl:Class>
    


    <!-- http://www.w3.org/2000/10/swap/pim/contact#Person -->

    <owl:Class rdf:about="http://www.w3.org/2000/10/swap/pim/contact#Person">
        <owl:disjointWith rdf:resource="http://xworks.gr/ontologies/ccso#Department"/>
        <owl:disjointWith rdf:resource="http://xworks.gr/ontologies/ccso#Institute"/>
        <owl:disjointWith rdf:resource="http://xworks.gr/ontologies/ccso#School"/>
        <owl:disjointWith rdf:resource="http://xworks.gr/ontologies/ccso#University"/>
        <rdfs:comment xml:lang="en">A person, a human being.</rdfs:comment>
        <rdfs:comment xml:lang="gr">Ένας άνθρωπος.</rdfs:comment>
        <rdfs:label xml:lang="gr">Άνθρωπος</rdfs:label>
        <rdfs:label xml:lang="gr">Πρόσωπο</rdfs:label>
    </owl:Class>
    


    <!-- http://xmlns.com/foaf/0.1/Agent -->

    <owl:Class rdf:about="http://xmlns.com/foaf/0.1/Agent"/>
    


    <!-- http://xmlns.com/foaf/0.1/Person -->

    <owl:Class rdf:about="http://xmlns.com/foaf/0.1/Person">
        <owl:disjointWith rdf:resource="http://xworks.gr/ontologies/ccso#Discipline"/>
        <owl:disjointWith rdf:resource="http://xworks.gr/ontologies/ccso#FieldofStudy"/>
        <owl:disjointWith rdf:resource="http://xworks.gr/ontologies/ccso#KnowledgeArea"/>
        <owl:disjointWith rdf:resource="http://xworks.gr/ontologies/ccso#KnowledgeBody"/>
        <owl:disjointWith rdf:resource="http://xworks.gr/ontologies/ccso#KnowledgeUnit"/>
        <rdfs:comment xml:lang="en">A person, a human being.</rdfs:comment>
        <rdfs:comment xml:lang="gr">Ένας άνθρωπος.</rdfs:comment>
        <rdfs:label xml:lang="gr">Άνθρωπος</rdfs:label>
        <rdfs:label xml:lang="gr">Πρόσωπο</rdfs:label>
    </owl:Class>
    


    <!-- http://xworks.gr/ontologies/ccso#AcademicStaff -->

    <owl:Class rdf:about="http://xworks.gr/ontologies/ccso#AcademicStaff">
        <rdfs:subClassOf rdf:resource="http://xworks.gr/ontologies/ccso#Employee"/>
        <owl:disjointWith rdf:resource="http://xworks.gr/ontologies/ccso#Assistant"/>
        <owl:disjointWith rdf:resource="http://xworks.gr/ontologies/ccso#Discipline"/>
        <owl:disjointWith rdf:resource="http://xworks.gr/ontologies/ccso#FieldofStudy"/>
        <owl:disjointWith rdf:resource="http://xworks.gr/ontologies/ccso#KnowledgeArea"/>
        <owl:disjointWith rdf:resource="http://xworks.gr/ontologies/ccso#KnowledgeBody"/>
        <owl:disjointWith rdf:resource="http://xworks.gr/ontologies/ccso#KnowledgeUnit"/>
        <owl:disjointWith rdf:resource="http://xworks.gr/ontologies/ccso#PostgraduateStudent"/>
        <owl:disjointWith rdf:resource="http://xworks.gr/ontologies/ccso#Student"/>
        <owl:disjointWith rdf:resource="http://xworks.gr/ontologies/ccso#TechnicalStaff"/>
        <owl:disjointWith rdf:resource="http://xworks.gr/ontologies/ccso#UndergraduateStudent"/>
        <rdfs:comment xml:lang="en">The academic staff of an institution, a school or a university such as professors of various ranks, lecturers and/or researchers. In North America the term Faculty is used instead.</rdfs:comment>
        <rdfs:comment xml:lang="gr">Το ακαδημαϊκό/εκπαιδευτικό προσωπικό ενός ιδρύματος, ενός σχολείου ή ενός πανεπιστημίου, όπως καθηγητές διαφόρων τάξεων, λέκτορες ή / και ερευνητές.</rdfs:comment>
        <rdfs:label xml:lang="gr">Aκαδημαϊκό προσωπικό</rdfs:label>
        <rdfs:label xml:lang="gr">Eκπαιδευτικό προσωπικό</rdfs:label>
        <skos:altLabel xml:lang="en">Academic Staff</skos:altLabel>
        <skos:altLabel xml:lang="en">Faculty</skos:altLabel>
    </owl:Class>
    


    <!-- http://xworks.gr/ontologies/ccso#AdministrativeStaff -->

    <owl:Class rdf:about="http://xworks.gr/ontologies/ccso#AdministrativeStaff">
        <rdfs:subClassOf rdf:resource="http://xworks.gr/ontologies/ccso#Employee"/>
        <owl:disjointWith rdf:resource="http://xworks.gr/ontologies/ccso#Assistant"/>
        <owl:disjointWith rdf:resource="http://xworks.gr/ontologies/ccso#Discipline"/>
        <owl:disjointWith rdf:resource="http://xworks.gr/ontologies/ccso#FieldofStudy"/>
        <owl:disjointWith rdf:resource="http://xworks.gr/ontologies/ccso#KnowledgeArea"/>
        <owl:disjointWith rdf:resource="http://xworks.gr/ontologies/ccso#KnowledgeBody"/>
        <owl:disjointWith rdf:resource="http://xworks.gr/ontologies/ccso#KnowledgeUnit"/>
        <owl:disjointWith rdf:resource="http://xworks.gr/ontologies/ccso#PostgraduateStudent"/>
        <owl:disjointWith rdf:resource="http://xworks.gr/ontologies/ccso#Student"/>
        <owl:disjointWith rdf:resource="http://xworks.gr/ontologies/ccso#TechnicalStaff"/>
        <owl:disjointWith rdf:resource="http://xworks.gr/ontologies/ccso#UndergraduateStudent"/>
        <rdfs:comment xml:lang="en">An employee who conducts of the administrating of an educational organization.</rdfs:comment>
        <rdfs:comment xml:lang="gr">Ένας εργαζόμενος που ασκεί τη διοίκηση ενός εκπαιδευτικού οργανισμού.</rdfs:comment>
        <rdfs:label xml:lang="gr">Διοικητικό Προσωπικό</rdfs:label>
        <skos:altLabel xml:lang="en">Administrative Staff</skos:altLabel>
    </owl:Class>
    


    <!-- http://xworks.gr/ontologies/ccso#Assistant -->

    <owl:Class rdf:about="http://xworks.gr/ontologies/ccso#Assistant">
        <owl:equivalentClass>
            <owl:Class>
                <owl:intersectionOf rdf:parseType="Collection">
                    <rdf:Description rdf:about="http://xmlns.com/foaf/0.1/Person"/>
                    <owl:Class>
                        <owl:unionOf rdf:parseType="Collection">
                            <owl:Restriction>
                                <owl:onProperty rdf:resource="http://xworks.gr/ontologies/ccso#assistsInCourse"/>
                                <owl:someValuesFrom rdf:resource="http://xworks.gr/ontologies/ccso#Syllabus"/>
                            </owl:Restriction>
                            <owl:Restriction>
                                <owl:onProperty rdf:resource="http://xworks.gr/ontologies/ccso#assistsInEvent"/>
                                <owl:someValuesFrom rdf:resource="http://xworks.gr/ontologies/ccso#Event"/>
                            </owl:Restriction>
                        </owl:unionOf>
                    </owl:Class>
                </owl:intersectionOf>
            </owl:Class>
        </owl:equivalentClass>
        <rdfs:subClassOf rdf:resource="http://xworks.gr/ontologies/ccso#Employee"/>
        <owl:disjointWith rdf:resource="http://xworks.gr/ontologies/ccso#Discipline"/>
        <owl:disjointWith rdf:resource="http://xworks.gr/ontologies/ccso#FieldofStudy"/>
        <owl:disjointWith rdf:resource="http://xworks.gr/ontologies/ccso#KnowledgeArea"/>
        <owl:disjointWith rdf:resource="http://xworks.gr/ontologies/ccso#KnowledgeBody"/>
        <owl:disjointWith rdf:resource="http://xworks.gr/ontologies/ccso#KnowledgeUnit"/>
        <owl:disjointWith rdf:resource="http://xworks.gr/ontologies/ccso#Lecturer"/>
        <owl:disjointWith rdf:resource="http://xworks.gr/ontologies/ccso#Professor"/>
        <owl:disjointWith rdf:resource="http://xworks.gr/ontologies/ccso#Researcher"/>
        <owl:disjointWith rdf:resource="http://xworks.gr/ontologies/ccso#TechnicalStaff"/>
        <owl:disjointWith rdf:resource="http://xworks.gr/ontologies/ccso#UndergraduateStudent"/>
        <rdfs:comment xml:lang="en">A person, usually an postgraduate student, who helps by assuming duties in lessons (TeachingAssistant), projects (ProjectAssistant), research (ResearchAssistant), etc.</rdfs:comment>
        <rdfs:comment xml:lang="gr">Κάποιο άτομο, συνήθως ένας μεταπτυχιακός φοιτητής, ο οποίος βοηθά με την ανάληψη καθηκόντων σε μαθήματα (βοηθός διδασκαλίας), σε έργα (βοηθός έργου), σε έρευνα (βοηθός έρευνας) κλπ.</rdfs:comment>
        <rdfs:label xml:lang="gr">Βοηθός</rdfs:label>
    </owl:Class>
    


    <!-- http://xworks.gr/ontologies/ccso#Bachelor -->

    <owl:Class rdf:about="http://xworks.gr/ontologies/ccso#Bachelor">
        <rdfs:subClassOf rdf:resource="http://xworks.gr/ontologies/ccso#ProgramofStudy"/>
        <owl:disjointWith rdf:resource="http://xworks.gr/ontologies/ccso#Certificate"/>
        <owl:disjointWith rdf:resource="http://xworks.gr/ontologies/ccso#Doctorate"/>
        <owl:disjointWith rdf:resource="http://xworks.gr/ontologies/ccso#Master"/>
        <owl:disjointWith rdf:resource="http://xworks.gr/ontologies/ccso#SchoolDiploma"/>
        <rdfs:comment xml:lang="en">The undergraduate academic degree awarded by universities and colleges, known as Bachelor’s degree.</rdfs:comment>
        <rdfs:comment xml:lang="gr">Το προπτυχιακό ακαδημαϊκό δίπλωμα που απονέμεται από πανεπιστήμια και κολέγια.</rdfs:comment>
        <rdfs:label xml:lang="gr">Προπτυχιακό Ακαδημαϊκό Δίπλωμα</rdfs:label>
        <rdfs:label xml:lang="gr">Πτυχίο</rdfs:label>
    </owl:Class>
    


    <!-- http://xworks.gr/ontologies/ccso#Certificate -->

    <owl:Class rdf:about="http://xworks.gr/ontologies/ccso#Certificate">
        <rdfs:subClassOf rdf:resource="http://xworks.gr/ontologies/ccso#ProgramofStudy"/>
        <owl:disjointWith rdf:resource="http://xworks.gr/ontologies/ccso#Doctorate"/>
        <owl:disjointWith rdf:resource="http://xworks.gr/ontologies/ccso#Master"/>
        <owl:disjointWith rdf:resource="http://xworks.gr/ontologies/ccso#SchoolDiploma"/>
        <rdfs:comment xml:lang="en">The diplomas that cannot be classified to the other subclasses such as Vocation diploma, Teaching diploma, Languages diploma, etc.</rdfs:comment>
        <rdfs:comment xml:lang="gr">Τα διπλώματα που δεν μπορούν να ταξινομηθούν στις άλλες υποκατηγορίες, όπως το δίπλωμα Επαγγελματικής Κατάρτισης, το δίπλωμα Διδακτικής Επάρκειας, το δίπλωμα Ξένων Γλωσσών, κ.α.</rdfs:comment>
        <rdfs:label xml:lang="gr">Πιστοποιητικό Γνώσεων</rdfs:label>
        <rdfs:label xml:lang="gr">Πιστοποιητικό Ικανοτήτων</rdfs:label>
        <rdfs:label xml:lang="gr">Πιστοποιητικό Σπουδών</rdfs:label>
    </owl:Class>
    


    <!-- http://xworks.gr/ontologies/ccso#Course -->

    <owl:Class rdf:about="http://xworks.gr/ontologies/ccso#Course">
        <rdfs:comment xml:lang="en">An institutional unit of teaching that lasts one academic term with a specific subject, usually is led by one or more instructors and has a fixed group of students.</rdfs:comment>
        <rdfs:comment xml:lang="gr">Μια μονάδα διδασκαλίας εκπαιδευτικού ιδρύματος που διαρκεί έναν ακαδημαϊκό εξάμηνο με ένα συγκεκριμένο θέμα, συνήθως διδάσκεται από έναν ή περισσότερους εκπαιδευτές και απευθύνεται σε μια σταθερή ομάδα μαθητών.</rdfs:comment>
        <rdfs:label xml:lang="gr">Μάθημα</rdfs:label>
        <rdfs:label xml:lang="gr">Σεμινάριο</rdfs:label>
    </owl:Class>
    


    <!-- http://xworks.gr/ontologies/ccso#DateTimeDuration -->

    <owl:Class rdf:about="http://xworks.gr/ontologies/ccso#DateTimeDuration"/>
    


    <!-- http://xworks.gr/ontologies/ccso#Department -->

    <owl:Class rdf:about="http://xworks.gr/ontologies/ccso#Department">
        <rdfs:subClassOf rdf:resource="http://schema.org/EducationalOrganization"/>
        <owl:disjointWith rdf:resource="http://xworks.gr/ontologies/ccso#Discipline"/>
        <owl:disjointWith rdf:resource="http://xworks.gr/ontologies/ccso#FieldofStudy"/>
        <owl:disjointWith rdf:resource="http://xworks.gr/ontologies/ccso#KnowledgeArea"/>
        <owl:disjointWith rdf:resource="http://xworks.gr/ontologies/ccso#KnowledgeBody"/>
        <owl:disjointWith rdf:resource="http://xworks.gr/ontologies/ccso#KnowledgeUnit"/>
        <owl:disjointWith rdf:resource="http://xworks.gr/ontologies/ccso#School"/>
        <owl:disjointWith rdf:resource="http://xworks.gr/ontologies/ccso#University"/>
        <rdfs:comment xml:lang="en">A division of a School (or College) devoted to a particular academic degree.</rdfs:comment>
        <rdfs:comment xml:lang="gr">Ένα τμήμα μίας Σχολής (ή Kολλεγίου) που προσφέρει ένα συγκεκριμένο ακαδημαϊκό πτυχίο.</rdfs:comment>
        <rdfs:label xml:lang="gr">Τμήμα</rdfs:label>
    </owl:Class>
    


    <!-- http://xworks.gr/ontologies/ccso#Discipline -->

    <owl:Class rdf:about="http://xworks.gr/ontologies/ccso#Discipline">
        <rdfs:subClassOf rdf:resource="http://xworks.gr/ontologies/ccso#FieldofStudy"/>
        <owl:disjointWith rdf:resource="http://xworks.gr/ontologies/ccso#Employee"/>
        <owl:disjointWith rdf:resource="http://xworks.gr/ontologies/ccso#Institute"/>
        <owl:disjointWith rdf:resource="http://xworks.gr/ontologies/ccso#Lecturer"/>
        <owl:disjointWith rdf:resource="http://xworks.gr/ontologies/ccso#PostgraduateStudent"/>
        <owl:disjointWith rdf:resource="http://xworks.gr/ontologies/ccso#Professor"/>
        <owl:disjointWith rdf:resource="http://xworks.gr/ontologies/ccso#Researcher"/>
        <owl:disjointWith rdf:resource="http://xworks.gr/ontologies/ccso#School"/>
        <owl:disjointWith rdf:resource="http://xworks.gr/ontologies/ccso#Student"/>
        <owl:disjointWith rdf:resource="http://xworks.gr/ontologies/ccso#TechnicalStaff"/>
        <owl:disjointWith rdf:resource="http://xworks.gr/ontologies/ccso#UndergraduateStudent"/>
        <owl:disjointWith rdf:resource="http://xworks.gr/ontologies/ccso#University"/>
        <rdfs:comment xml:lang="en">An ‘Academic Discipline&apos; (here &apos;Discipline&apos;) is a branch of knowledge or a field of study.</rdfs:comment>
        <rdfs:comment xml:lang="gr">Μία Επιστήμη ή &apos;Aκαδημαϊκή Επιστήμη&apos; αντιπροσωπεύει ένα κλάδο γνώσης ή πεδίο σπουδών.</rdfs:comment>
        <rdfs:label xml:lang="gr">Επιστήμη</rdfs:label>
        <rdfs:seeAlso rdf:resource="https://en.wikipedia.org/wiki/Outline_of_academic_disciplines"/>
        <skos:altLabel xml:lang="en">Academic Discipline</skos:altLabel>
    </owl:Class>
    


    <!-- http://xworks.gr/ontologies/ccso#Doctorate -->

    <owl:Class rdf:about="http://xworks.gr/ontologies/ccso#Doctorate">
        <rdfs:subClassOf rdf:resource="http://xworks.gr/ontologies/ccso#ProgramofStudy"/>
        <rdfs:subClassOf>
            <owl:Restriction>
                <owl:onProperty rdf:resource="http://xworks.gr/ontologies/ccso#requiresProgram"/>
                <owl:minQualifiedCardinality rdf:datatype="http://www.w3.org/2001/XMLSchema#nonNegativeInteger">1</owl:minQualifiedCardinality>
                <owl:onClass rdf:resource="http://xworks.gr/ontologies/ccso#Master"/>
            </owl:Restriction>
        </rdfs:subClassOf>
        <owl:disjointWith rdf:resource="http://xworks.gr/ontologies/ccso#Master"/>
        <owl:disjointWith rdf:resource="http://xworks.gr/ontologies/ccso#SchoolDiploma"/>
        <rdfs:comment xml:lang="en">The academic and research degree, also known as Doctor’s degree, awarded by universities that certifies the person as an expert of art or sciences in a field and qualifies to teach at the university level.</rdfs:comment>
        <rdfs:comment xml:lang="gr">Ο ακαδημαϊκός και ερευνητικός τίτλος, επίσης γνωστός ως Διδακτορικό δίπλωμα, απονέμεται από πανεπιστήμια που πιστοποιούν το άτομο ως ειδικός της τέχνης ή των επιστημών σε έναν τομέα και είναι ικανός να διδάσκει σε πανεπιστημιακό επίπεδο.</rdfs:comment>
        <rdfs:label xml:lang="gr">Διδακτορικό</rdfs:label>
        <rdfs:label xml:lang="gr">Διδακτορικό Aκαδημαϊκό Δίπλωμα</rdfs:label>
    </owl:Class>
    


    <!-- http://xworks.gr/ontologies/ccso#Employee -->

    <owl:Class rdf:about="http://xworks.gr/ontologies/ccso#Employee">
        <owl:equivalentClass>
            <owl:Class>
                <owl:intersectionOf rdf:parseType="Collection">
                    <rdf:Description rdf:about="http://xmlns.com/foaf/0.1/Person"/>
                    <owl:Restriction>
                        <owl:onProperty rdf:resource="http://xworks.gr/ontologies/ccso#worksFor"/>
                        <owl:someValuesFrom rdf:resource="http://schema.org/EducationalOrganization"/>
                    </owl:Restriction>
                </owl:intersectionOf>
            </owl:Class>
        </owl:equivalentClass>
        <rdfs:subClassOf rdf:resource="http://xmlns.com/foaf/0.1/Person"/>
        <owl:disjointWith rdf:resource="http://xworks.gr/ontologies/ccso#FieldofStudy"/>
        <owl:disjointWith rdf:resource="http://xworks.gr/ontologies/ccso#KnowledgeArea"/>
        <owl:disjointWith rdf:resource="http://xworks.gr/ontologies/ccso#KnowledgeBody"/>
        <owl:disjointWith rdf:resource="http://xworks.gr/ontologies/ccso#KnowledgeUnit"/>
        <rdfs:comment xml:lang="en">Employee of an organization.</rdfs:comment>
        <rdfs:comment xml:lang="gr">Εργαζόμενος σε κάποιον οργανισμό.</rdfs:comment>
        <rdfs:label xml:lang="gr">Εργαζόμενος</rdfs:label>
        <skos:altLabel xml:lang="en">Worker</skos:altLabel>
    </owl:Class>
    


    <!-- http://xworks.gr/ontologies/ccso#EvaluationEvent -->

    <owl:Class rdf:about="http://xworks.gr/ontologies/ccso#EvaluationEvent">
        <rdfs:subClassOf rdf:resource="http://xworks.gr/ontologies/ccso#Event"/>
        <owl:disjointWith rdf:resource="http://xworks.gr/ontologies/ccso#TeachingEvent"/>
        <rdfs:comment xml:lang="en">Events included in evaluation procedure.</rdfs:comment>
        <rdfs:comment xml:lang="gr">Γεγονότα που συμπεριλαμβάνονται στη διαδικασία αξιολόγησης.</rdfs:comment>
        <rdfs:label xml:lang="gr">Εξέταση</rdfs:label>
        <rdfs:label xml:lang="gr">Συμβάν Εξετάσεων</rdfs:label>
        <skos:altLabel xml:lang="en">Evaluation</skos:altLabel>
        <skos:altLabel xml:lang="en">Examination</skos:altLabel>
    </owl:Class>
    


    <!-- http://xworks.gr/ontologies/ccso#Event -->

    <owl:Class rdf:about="http://xworks.gr/ontologies/ccso#Event">
        <rdfs:comment xml:lang="en">All events that happen in a class within a course.</rdfs:comment>
        <rdfs:comment xml:lang="gr">Όλα τα γεγονότα που συμβαίνουν σε μια τάξη κατά τη διάρκεια του προγράμματος μαθημάτων.</rdfs:comment>
        <rdfs:label xml:lang="gr">Συμβάν</rdfs:label>
    </owl:Class>
    


    <!-- http://xworks.gr/ontologies/ccso#FieldofStudy -->

    <owl:Class rdf:about="http://xworks.gr/ontologies/ccso#FieldofStudy">
        <owl:disjointWith rdf:resource="http://xworks.gr/ontologies/ccso#Institute"/>
        <owl:disjointWith rdf:resource="http://xworks.gr/ontologies/ccso#Lecturer"/>
        <owl:disjointWith rdf:resource="http://xworks.gr/ontologies/ccso#PostgraduateStudent"/>
        <owl:disjointWith rdf:resource="http://xworks.gr/ontologies/ccso#Professor"/>
        <owl:disjointWith rdf:resource="http://xworks.gr/ontologies/ccso#Researcher"/>
        <owl:disjointWith rdf:resource="http://xworks.gr/ontologies/ccso#School"/>
        <owl:disjointWith rdf:resource="http://xworks.gr/ontologies/ccso#Student"/>
        <owl:disjointWith rdf:resource="http://xworks.gr/ontologies/ccso#TechnicalStaff"/>
        <owl:disjointWith rdf:resource="http://xworks.gr/ontologies/ccso#UndergraduateStudent"/>
        <owl:disjointWith rdf:resource="http://xworks.gr/ontologies/ccso#University"/>
        <rdfs:comment xml:lang="en">The root class of knowledge structure. It refers to the Academic Disciplines.</rdfs:comment>
        <rdfs:comment xml:lang="gr">Η κλάση-ρίζα της οργανωτικής δομής με τις έννοιες που αφορούν τη γνώση και αφορά όλες τις Ακαδημαϊκές επιστήμες.</rdfs:comment>
        <rdfs:label xml:lang="gr">Πεδίο Γνώσης</rdfs:label>
        <skos:altLabel xml:lang="en">Field of Study</skos:altLabel>
    </owl:Class>
    


    <!-- http://xworks.gr/ontologies/ccso#Institute -->

    <owl:Class rdf:about="http://xworks.gr/ontologies/ccso#Institute">
        <rdfs:subClassOf rdf:resource="http://schema.org/EducationalOrganization"/>
        <owl:disjointWith rdf:resource="http://xworks.gr/ontologies/ccso#KnowledgeArea"/>
        <owl:disjointWith rdf:resource="http://xworks.gr/ontologies/ccso#KnowledgeBody"/>
        <owl:disjointWith rdf:resource="http://xworks.gr/ontologies/ccso#KnowledgeUnit"/>
        <rdfs:comment xml:lang="en">An autonomous educational institution which provides learning services in areas of Non-Formal Education.</rdfs:comment>
        <rdfs:comment xml:lang="gr">Ένα αυτόνομο εκπαιδευτικό ίδρυμα που παρέχει υπηρεσίες μάθησης σε περιοχές της Μη-Τυπικής Εκπαίδευσης.</rdfs:comment>
        <rdfs:label xml:lang="gr">Ινστιτούτο</rdfs:label>
    </owl:Class>
    


    <!-- http://xworks.gr/ontologies/ccso#KnowledgeArea -->

    <owl:Class rdf:about="http://xworks.gr/ontologies/ccso#KnowledgeArea">
        <rdfs:subClassOf rdf:resource="http://xworks.gr/ontologies/ccso#FieldofStudy"/>
        <owl:disjointWith rdf:resource="http://xworks.gr/ontologies/ccso#Lecturer"/>
        <owl:disjointWith rdf:resource="http://xworks.gr/ontologies/ccso#PostgraduateStudent"/>
        <owl:disjointWith rdf:resource="http://xworks.gr/ontologies/ccso#Professor"/>
        <owl:disjointWith rdf:resource="http://xworks.gr/ontologies/ccso#Researcher"/>
        <owl:disjointWith rdf:resource="http://xworks.gr/ontologies/ccso#School"/>
        <owl:disjointWith rdf:resource="http://xworks.gr/ontologies/ccso#Student"/>
        <owl:disjointWith rdf:resource="http://xworks.gr/ontologies/ccso#TechnicalStaff"/>
        <owl:disjointWith rdf:resource="http://xworks.gr/ontologies/ccso#UndergraduateStudent"/>
        <owl:disjointWith rdf:resource="http://xworks.gr/ontologies/ccso#University"/>
        <rdfs:comment xml:lang="en">Subjects of a Body of Knowledge.</rdfs:comment>
        <rdfs:comment xml:lang="gr">Θέματα ενός Σώματος Γνώσης (KnowledgeBody).</rdfs:comment>
        <rdfs:label xml:lang="gr">Περιοχή Γνώσης</rdfs:label>
        <skos:altLabel xml:lang="en">Area of Knowledge</skos:altLabel>
    </owl:Class>
    


    <!-- http://xworks.gr/ontologies/ccso#KnowledgeBody -->

    <owl:Class rdf:about="http://xworks.gr/ontologies/ccso#KnowledgeBody">
        <rdfs:subClassOf rdf:resource="http://xworks.gr/ontologies/ccso#FieldofStudy"/>
        <owl:disjointWith rdf:resource="http://xworks.gr/ontologies/ccso#Lecturer"/>
        <owl:disjointWith rdf:resource="http://xworks.gr/ontologies/ccso#PostgraduateStudent"/>
        <owl:disjointWith rdf:resource="http://xworks.gr/ontologies/ccso#Professor"/>
        <owl:disjointWith rdf:resource="http://xworks.gr/ontologies/ccso#Researcher"/>
        <owl:disjointWith rdf:resource="http://xworks.gr/ontologies/ccso#School"/>
        <owl:disjointWith rdf:resource="http://xworks.gr/ontologies/ccso#Student"/>
        <owl:disjointWith rdf:resource="http://xworks.gr/ontologies/ccso#TechnicalStaff"/>
        <owl:disjointWith rdf:resource="http://xworks.gr/ontologies/ccso#UndergraduateStudent"/>
        <owl:disjointWith rdf:resource="http://xworks.gr/ontologies/ccso#University"/>
        <rdfs:comment xml:lang="en">Main knowledge body of a Discipline, a specification of the content to be covered in a curriculum.</rdfs:comment>
        <rdfs:comment xml:lang="gr">Το κύριο σώμα γνώσης μιας Επιστήμης, μια προδιαγραφή του περιεχομένου που πρέπει να καλύπτεται σε ένα πρόγραμμα σπουδών.</rdfs:comment>
        <rdfs:label xml:lang="gr">Κύριο Σώμα Γνώσης</rdfs:label>
        <skos:altLabel xml:lang="en">Body of Knowledge</skos:altLabel>
    </owl:Class>
    


    <!-- http://xworks.gr/ontologies/ccso#KnowledgeUnit -->

    <owl:Class rdf:about="http://xworks.gr/ontologies/ccso#KnowledgeUnit">
        <rdfs:subClassOf rdf:resource="http://xworks.gr/ontologies/ccso#FieldofStudy"/>
        <owl:disjointWith rdf:resource="http://xworks.gr/ontologies/ccso#Lecturer"/>
        <owl:disjointWith rdf:resource="http://xworks.gr/ontologies/ccso#PostgraduateStudent"/>
        <owl:disjointWith rdf:resource="http://xworks.gr/ontologies/ccso#Professor"/>
        <owl:disjointWith rdf:resource="http://xworks.gr/ontologies/ccso#Researcher"/>
        <owl:disjointWith rdf:resource="http://xworks.gr/ontologies/ccso#School"/>
        <owl:disjointWith rdf:resource="http://xworks.gr/ontologies/ccso#Student"/>
        <owl:disjointWith rdf:resource="http://xworks.gr/ontologies/ccso#TechnicalStaff"/>
        <owl:disjointWith rdf:resource="http://xworks.gr/ontologies/ccso#UndergraduateStudent"/>
        <owl:disjointWith rdf:resource="http://xworks.gr/ontologies/ccso#University"/>
        <rdfs:comment xml:lang="en">Part of a Knowledge Area.</rdfs:comment>
        <rdfs:comment xml:lang="gr">Μέρος μιας Περιοχής Γνώσης (KnowledgeArea).</rdfs:comment>
        <rdfs:label xml:lang="gr">Μέρος Γνώσης μιας Περιοχής Γνώσης</rdfs:label>
        <skos:altLabel xml:lang="en">Unit of Knowledge</skos:altLabel>
    </owl:Class>
    


    <!-- http://xworks.gr/ontologies/ccso#LearningOutcome -->

    <owl:Class rdf:about="http://xworks.gr/ontologies/ccso#LearningOutcome">
        <rdfs:comment xml:lang="en">The learning outcomes, specific knowledge, skills and competences, which the students will acquire with the successful completion of the course.</rdfs:comment>
        <rdfs:comment xml:lang="gr">Τα μαθησιακά αποτελέσματα, οι ειδικές γνώσεις, δεξιότητες και ικανότητες, τις οποίες οι σπουδαστές θα αποκτήσουν με την επιτυχή ολοκλήρωση του μαθήματος.</rdfs:comment>
        <rdfs:label xml:lang="gr">Μαθησιακό Αποτέλεσμα</rdfs:label>
        <skos:altLabel xml:lang="en">Learning Objective</skos:altLabel>
    </owl:Class>
    


    <!-- http://xworks.gr/ontologies/ccso#Lecturer -->

    <owl:Class rdf:about="http://xworks.gr/ontologies/ccso#Lecturer">
        <rdfs:subClassOf rdf:resource="http://xworks.gr/ontologies/ccso#AcademicStaff"/>
        <owl:disjointWith rdf:resource="http://xworks.gr/ontologies/ccso#PostgraduateStudent"/>
        <owl:disjointWith rdf:resource="http://xworks.gr/ontologies/ccso#Student"/>
        <owl:disjointWith rdf:resource="http://xworks.gr/ontologies/ccso#TechnicalStaff"/>
        <owl:disjointWith rdf:resource="http://xworks.gr/ontologies/ccso#UndergraduateStudent"/>
        <rdfs:comment xml:lang="en">An academic person at an early career stage with open-ended or tenured position in a university who teaches and conducts research.</rdfs:comment>
        <rdfs:comment xml:lang="gr">Ένα ακαδημαϊκό άτομο το οποίο βρίσκεται στο αρχικό στάδιο της σταδιοδρομίας του με αορίστου ή μόνιμη θέση σε ένα πανεπιστήμιο που διδάσκει και διεξάγει έρευνα.</rdfs:comment>
        <rdfs:label xml:lang="gr">Λέκτορας</rdfs:label>
    </owl:Class>
    


    <!-- http://xworks.gr/ontologies/ccso#Master -->

    <owl:Class rdf:about="http://xworks.gr/ontologies/ccso#Master">
        <rdfs:subClassOf rdf:resource="http://xworks.gr/ontologies/ccso#ProgramofStudy"/>
        <rdfs:subClassOf>
            <owl:Restriction>
                <owl:onProperty rdf:resource="http://xworks.gr/ontologies/ccso#requiresProgram"/>
                <owl:minQualifiedCardinality rdf:datatype="http://www.w3.org/2001/XMLSchema#nonNegativeInteger">1</owl:minQualifiedCardinality>
                <owl:onClass rdf:resource="http://xworks.gr/ontologies/ccso#Bachelor"/>
            </owl:Restriction>
        </rdfs:subClassOf>
        <owl:disjointWith rdf:resource="http://xworks.gr/ontologies/ccso#SchoolDiploma"/>
        <rdfs:comment xml:lang="en">The postgraduate academic degree, known as Master’s degree, awarded by universities or colleges upon completion of a course of study demonstrating mastery of a specific field of study or area of professional practice.</rdfs:comment>
        <rdfs:comment xml:lang="gr">Το μεταπτυχιακό ακαδημαϊκό δίπλωμα που απονέμεται από πανεπιστήμια ή κολέγια μετά την ολοκλήρωση ενός κύκλου σπουδών που αποδεικνύει την απόκτηση ειδικού πεδίου σπουδών ή τομέα επαγγελματικής πρακτικής.</rdfs:comment>
        <rdfs:label xml:lang="gr">Μεταπτυχιακό</rdfs:label>
        <rdfs:label xml:lang="gr">Μεταπτυχιακό Aκαδημαϊκό Δίπλωμα</rdfs:label>
    </owl:Class>
    


    <!-- http://xworks.gr/ontologies/ccso#PostgraduateStudent -->

    <owl:Class rdf:about="http://xworks.gr/ontologies/ccso#PostgraduateStudent">
        <owl:equivalentClass>
            <owl:Class>
                <owl:intersectionOf rdf:parseType="Collection">
                    <rdf:Description rdf:about="http://xworks.gr/ontologies/ccso#Student"/>
                    <owl:Class>
                        <owl:intersectionOf rdf:parseType="Collection">
                            <owl:Restriction>
                                <owl:onProperty rdf:resource="http://xworks.gr/ontologies/ccso#enrolledIn"/>
                                <owl:someValuesFrom rdf:resource="http://xworks.gr/ontologies/ccso#Master"/>
                            </owl:Restriction>
                            <owl:Restriction>
                                <owl:onProperty rdf:resource="http://xworks.gr/ontologies/ccso#hasDegree"/>
                                <owl:someValuesFrom rdf:resource="http://xworks.gr/ontologies/ccso#Bachelor"/>
                            </owl:Restriction>
                        </owl:intersectionOf>
                    </owl:Class>
                </owl:intersectionOf>
            </owl:Class>
        </owl:equivalentClass>
        <rdfs:subClassOf rdf:resource="http://xworks.gr/ontologies/ccso#Student"/>
        <rdfs:subClassOf>
            <owl:Class>
                <owl:intersectionOf rdf:parseType="Collection">
                    <owl:Class>
                        <owl:complementOf>
                            <owl:Restriction>
                                <owl:onProperty rdf:resource="http://xworks.gr/ontologies/ccso#enrolledIn"/>
                                <owl:someValuesFrom rdf:resource="http://xworks.gr/ontologies/ccso#Bachelor"/>
                            </owl:Restriction>
                        </owl:complementOf>
                    </owl:Class>
                    <owl:Restriction>
                        <owl:onProperty rdf:resource="http://xworks.gr/ontologies/ccso#hasDegree"/>
                        <owl:someValuesFrom rdf:resource="http://xworks.gr/ontologies/ccso#Bachelor"/>
                    </owl:Restriction>
                    <owl:Restriction>
                        <owl:onProperty rdf:resource="http://xworks.gr/ontologies/ccso#enrolledIn"/>
                        <owl:qualifiedCardinality rdf:datatype="http://www.w3.org/2001/XMLSchema#nonNegativeInteger">1</owl:qualifiedCardinality>
                        <owl:onClass rdf:resource="http://xworks.gr/ontologies/ccso#Master"/>
                    </owl:Restriction>
                </owl:intersectionOf>
            </owl:Class>
        </rdfs:subClassOf>
        <owl:disjointWith rdf:resource="http://xworks.gr/ontologies/ccso#Professor"/>
        <owl:disjointWith rdf:resource="http://xworks.gr/ontologies/ccso#Researcher"/>
        <owl:disjointWith rdf:resource="http://xworks.gr/ontologies/ccso#UndergraduateStudent"/>
        <rdfs:comment xml:lang="en">A student who own a Bachelor’s degree and studying for an academic or professional certificate.</rdfs:comment>
        <rdfs:comment xml:lang="gr">Ένας φοιτητής που κατέχει πτυχίο Bachelor και σπουδάζει για ακαδημαϊκό ή επαγγελματικό πιστοποιητικό σπουδών.</rdfs:comment>
        <rdfs:label xml:lang="gr">Μεταπτυχιακός Φοιτητής</rdfs:label>
        <skos:altLabel xml:lang="en">Postgraduate Student</skos:altLabel>
    </owl:Class>
    


    <!-- http://xworks.gr/ontologies/ccso#Professor -->

    <owl:Class rdf:about="http://xworks.gr/ontologies/ccso#Professor">
        <rdfs:subClassOf rdf:resource="http://xworks.gr/ontologies/ccso#AcademicStaff"/>
        <owl:disjointWith rdf:resource="http://xworks.gr/ontologies/ccso#Student"/>
        <owl:disjointWith rdf:resource="http://xworks.gr/ontologies/ccso#TechnicalStaff"/>
        <owl:disjointWith rdf:resource="http://xworks.gr/ontologies/ccso#UndergraduateStudent"/>
        <rdfs:comment xml:lang="en">An instructor that is an expert of art or sciences and participates in a program of study of an educational institution.</rdfs:comment>
        <rdfs:comment xml:lang="gr">Ο εκπαιδευτής που είναι ειδικός της τέχνης ή της επιστήμης και συμμετέχει σε πρόγραμμα σπουδών ενός εκπαιδευτικού ιδρύματος.</rdfs:comment>
        <rdfs:label xml:lang="gr">Καθηγητής</rdfs:label>
    </owl:Class>
    


    <!-- http://xworks.gr/ontologies/ccso#ProgramofStudy -->

    <owl:Class rdf:about="http://xworks.gr/ontologies/ccso#ProgramofStudy">
        <rdfs:comment xml:lang="en">The degrees awarded to students upon a successful completion of a course of study in an educational institution.</rdfs:comment>
        <rdfs:comment xml:lang="gr">Τα πτυχία που απονέμονται στους φοιτητές μετά την επιτυχή ολοκλήρωση ενός κύκλου σπουδών σε ένα εκπαιδευτικό ίδρυμα.</rdfs:comment>
        <rdfs:label xml:lang="gr">Τίτλος Προγράμματος Σπουδών</rdfs:label>
        <skos:altLabel xml:lang="en">Institutional Degree</skos:altLabel>
        <skos:altLabel xml:lang="en">Program of Study</skos:altLabel>
        <skos:altLabel xml:lang="en">Programme of Study</skos:altLabel>
    </owl:Class>
    


    <!-- http://xworks.gr/ontologies/ccso#Researcher -->

    <owl:Class rdf:about="http://xworks.gr/ontologies/ccso#Researcher">
        <rdfs:subClassOf rdf:resource="http://xworks.gr/ontologies/ccso#AcademicStaff"/>
        <owl:disjointWith rdf:resource="http://xworks.gr/ontologies/ccso#Student"/>
        <owl:disjointWith rdf:resource="http://xworks.gr/ontologies/ccso#TechnicalStaff"/>
        <owl:disjointWith rdf:resource="http://xworks.gr/ontologies/ccso#UndergraduateStudent"/>
        <rdfs:comment xml:lang="en">An academic person that conducts research, participates in research projects or leads research groups.</rdfs:comment>
        <rdfs:comment xml:lang="gr">Μέλος του ακαδημαϊκού προσωπικού που διεξάγει έρευνα, συμμετέχει σε ερευνητικά έργα ή είναι υπεύθυνος ερευνητικών ομάδων.</rdfs:comment>
        <rdfs:label xml:lang="gr">Ερευνητής</rdfs:label>
    </owl:Class>
    


    <!-- http://xworks.gr/ontologies/ccso#Resource -->

    <owl:Class rdf:about="http://xworks.gr/ontologies/ccso#Resource">
        <rdfs:comment xml:lang="en">The teaching and learning resources that are being used during a course. Books, academic articles, notes as well as webpages, videos, images, audios and other stuff with educational interest for a course can be included to the learning material for a course.

The resource could be an official Publication.
A work of a person which its content is available to the general public. The content may vary; usually it refers to text, images, audio or visual content, software programs, etc. The text includes papers and articles in newspapers, magazines, books, journals, etc.</rdfs:comment>
        <rdfs:comment xml:lang="gr">Οι πηγές διδασκαλίας και εκμάθησης που χρησιμοποιούνται κατά τη διάρκεια ενός μαθήματος. Βιβλία, ακαδημαϊκά άρθρα, σημειώσεις καθώς και ιστοσελίδες, βίντεο, εικόνες, ηχητικά και άλλα στοιχεία με εκπαιδευτικό ενδιαφέρον μπορούν να συμπεριληφθούν στο εκπαιδευτικό υλικό για ένα μάθημα.

Η πηγή ενδέχεται να αποτελεί επίησημη Δημοσίευση.
Ένα έργο ενός προσώπου, το περιεχόμενο του οποίου είναι διαθέσιμο στο ευρύ κοινό. Το περιεχόμενο ποικίλει. συνήθως αναφέρεται σε κείμενο, εικόνες, ηχητικό ή οπτικό περιεχόμενο, προγράμματα λογισμικού, κλπ. Το κείμενο περιλαμβάνει άρθρα και άρθρα σε εφημερίδες, περιοδικά, βιβλία, περιοδικά κλπ.</rdfs:comment>
        <rdfs:label xml:lang="gr">Πηγή</rdfs:label>
        <skos:altLabel xml:lang="en">Learning Material</skos:altLabel>
    </owl:Class>
    


    <!-- http://xworks.gr/ontologies/ccso#School -->

    <owl:Class rdf:about="http://xworks.gr/ontologies/ccso#School">
        <rdfs:subClassOf rdf:resource="http://schema.org/EducationalOrganization"/>
        <owl:disjointWith rdf:resource="http://xworks.gr/ontologies/ccso#University"/>
        <rdfs:comment xml:lang="en">A division within a university comprising one subject area, or a number of related subject areas. 
The American usage is followed where such divisions are referred to as Colleges or Schools rather than using the term Faculty which is used in other countries in order to avoid misunderstandings because the same term (Faculty) refers to the Academic staff of a University in American usage.</rdfs:comment>
        <rdfs:comment xml:lang="en">An institution that belongs to the Formal Education system of a country and is designed to provide learning environment for teaching students.</rdfs:comment>
        <rdfs:comment xml:lang="gr">Ένα ίδρυμα που ανήκει στο σύστημα τυπικής εκπαίδευσης μιας χώρας και έχει σχεδιαστεί για να παρέχει περιβάλλον μάθησης για τη διδασκαλία των μαθητών.</rdfs:comment>
        <rdfs:comment xml:lang="gr">Ένα τμήμα ενός πανεπιστημίου που περιλαμβάνει ένα θεματικό πεδίο ή έναν αριθμό σχετικών θεματικών πεδίων. 
Ακολουθήθηκε η αμερικάνικη προσέγγιση όπου τέτοια τμήματα αναφέρονται ως Κολλέγια ή Σχολεία αντί να χρησιμοποιηθεί ο όρος Faculty που χρησιμοποιείται σε άλλες χώρες για να αποφευχθούν παρεξηγήσεις, επειδή ο ίδιος όρος (Faculty) στην Αμερική αναφέρεται στο Ακαδημαϊκό Προσωπικό ενός Πανεπιστημίου.</rdfs:comment>
        <rdfs:label xml:lang="en">School</rdfs:label>
        <rdfs:label xml:lang="gr">Κολλέγιο</rdfs:label>
        <rdfs:label xml:lang="gr">Σχολή</rdfs:label>
        <skos:altLabel xml:lang="en">College</skos:altLabel>
    </owl:Class>
    


    <!-- http://xworks.gr/ontologies/ccso#SchoolDiploma -->

    <owl:Class rdf:about="http://xworks.gr/ontologies/ccso#SchoolDiploma">
        <rdfs:subClassOf rdf:resource="http://xworks.gr/ontologies/ccso#ProgramofStudy"/>
        <rdfs:comment xml:lang="en">The graduation degrees provided by Primary and Secondary schools (Primary School, Secondary School and High School).</rdfs:comment>
        <rdfs:comment xml:lang="gr">Τα πτυχία αποφοίτησης που δίδονται από σχολεία της Πρωτοβάθμιας και Δευτεροβάθμιας εκπαίδευσης (Δημοτικό, Γυμνάσιο και Λύκειο).</rdfs:comment>
        <rdfs:label xml:lang="gr">Πτυχίο Αποφοίτησης</rdfs:label>
    </owl:Class>
    


    <!-- http://xworks.gr/ontologies/ccso#Student -->

    <owl:Class rdf:about="http://xworks.gr/ontologies/ccso#Student">
        <rdfs:subClassOf rdf:resource="http://xmlns.com/foaf/0.1/Person"/>
        <rdfs:comment xml:lang="en">A learner who attends an educational programme</rdfs:comment>
        <rdfs:comment xml:lang="gr">O εκπαιδευόμενος που παρακολουθεί κάποιο εκπαιδευτικό πρόγραμμα.</rdfs:comment>
        <rdfs:label xml:lang="gr">Εκπαιδευόμενος</rdfs:label>
        <rdfs:label xml:lang="gr">Μαθητής</rdfs:label>
        <rdfs:label xml:lang="gr">Σπουδαστής</rdfs:label>
        <rdfs:label xml:lang="gr">Φοιτητής</rdfs:label>
        <skos:altLabel xml:lang="en">Learner</skos:altLabel>
    </owl:Class>
    


    <!-- http://xworks.gr/ontologies/ccso#Syllabus -->

    <owl:Class rdf:about="http://xworks.gr/ontologies/ccso#Syllabus">
        <rdfs:comment xml:lang="en">A document that addresses course information, expectations and responsibilities to students.</rdfs:comment>
        <rdfs:comment xml:lang="gr">Ένα έγγραφο που επικοινωνεί προς τους φοιτητές τις πληροφορίες του μαθήματος, τις προσδοκίες καθώς και τις υποχρεώσεις τους.</rdfs:comment>
        <rdfs:label xml:lang="gr">Περίγραμμα Μαθήματος</rdfs:label>
        <skos:altLabel xml:lang="en">Course Syllabus</skos:altLabel>
    </owl:Class>
    


    <!-- http://xworks.gr/ontologies/ccso#TeachingEvaluationMethod -->

    <owl:Class rdf:about="http://xworks.gr/ontologies/ccso#TeachingEvaluationMethod">
        <rdfs:comment xml:lang="en">The manner and the different kinds of teaching methods and learning activities within a course.</rdfs:comment>
        <rdfs:comment xml:lang="gr">Ο τρόπος και τα είδη μεθόδων διδασκαλίας και μαθησιακών δραστηριοτήτων που χρησιμοποιούνται κατά τη διάρκεια των μαθημάτων.</rdfs:comment>
        <rdfs:label xml:lang="gr">Μέθοδος Διδασκαλίας</rdfs:label>
        <skos:altLabel xml:lang="en">Teaching Evaluation Method</skos:altLabel>
    </owl:Class>
    


    <!-- http://xworks.gr/ontologies/ccso#TeachingEvent -->

    <owl:Class rdf:about="http://xworks.gr/ontologies/ccso#TeachingEvent">
        <rdfs:subClassOf rdf:resource="http://xworks.gr/ontologies/ccso#Event"/>
        <rdfs:comment xml:lang="en">Events that happen in a class which are related to teaching.</rdfs:comment>
        <rdfs:comment xml:lang="gr">Γεγονότα που συμβαίνουν σε μια τάξη και σχετίζονται με τη διδασκαλία.</rdfs:comment>
        <rdfs:label xml:lang="gr">Διδασκαλία</rdfs:label>
        <rdfs:label xml:lang="gr">Συμβάν Διδασκαλίας</rdfs:label>
        <skos:altLabel xml:lang="en">Teaching Event</skos:altLabel>
        <skos:altLabel xml:lang="en">Teaching Lesson</skos:altLabel>
    </owl:Class>
    


    <!-- http://xworks.gr/ontologies/ccso#TechnicalStaff -->

    <owl:Class rdf:about="http://xworks.gr/ontologies/ccso#TechnicalStaff">
        <rdfs:subClassOf rdf:resource="http://xworks.gr/ontologies/ccso#Employee"/>
        <rdfs:comment xml:lang="en">An employee who is specialized and related to provide practical, mechanical and applied services (e.g. electrician, plumber, etc).</rdfs:comment>
        <rdfs:comment xml:lang="gr">Ο εργαζόμενος ο οποίος είναι ειδικευμένος στην παροχή πρακτικών, μηχανικών και εφαρμοσμένων υπηρεσιών (π.χ. ηλεκτρολόγος, υδραυλικός κ.λπ.).</rdfs:comment>
        <rdfs:label xml:lang="gr">Τεχνικό Προσωπικό</rdfs:label>
        <rdfs:label xml:lang="gr">Τεχνικός</rdfs:label>
        <skos:altLabel xml:lang="en">Technical Staff</skos:altLabel>
    </owl:Class>
    


    <!-- http://xworks.gr/ontologies/ccso#Topic -->

    <owl:Class rdf:about="http://xworks.gr/ontologies/ccso#Topic">
        <rdfs:comment xml:lang="en">A subject of study, small piece from Body of Knowledge that could be organized into course and covered during lessons.</rdfs:comment>
        <rdfs:comment xml:lang="gr">Ένα θέμα μελέτης, ένα μικρό κομμάτι από το Σώμα της Γνώσης που θα μπορούσε να οργανωθεί σε πορεία και να καλυφθεί κατά τη διάρκεια των μαθημάτων.</rdfs:comment>
        <rdfs:label xml:lang="gr">Θέμα</rdfs:label>
        <skos:altLabel xml:lang="en">Subject</skos:altLabel>
    </owl:Class>
    


    <!-- http://xworks.gr/ontologies/ccso#UndergraduateStudent -->

    <owl:Class rdf:about="http://xworks.gr/ontologies/ccso#UndergraduateStudent">
        <owl:equivalentClass>
            <owl:Class>
                <owl:intersectionOf rdf:parseType="Collection">
                    <rdf:Description rdf:about="http://xworks.gr/ontologies/ccso#Student"/>
                    <owl:Restriction>
                        <owl:onProperty rdf:resource="http://xworks.gr/ontologies/ccso#enrolledIn"/>
                        <owl:someValuesFrom rdf:resource="http://xworks.gr/ontologies/ccso#Bachelor"/>
                    </owl:Restriction>
                </owl:intersectionOf>
            </owl:Class>
        </owl:equivalentClass>
        <rdfs:subClassOf rdf:resource="http://xworks.gr/ontologies/ccso#Student"/>
        <rdfs:subClassOf>
            <owl:Class>
                <owl:intersectionOf rdf:parseType="Collection">
                    <owl:Class>
                        <owl:complementOf>
                            <owl:Class>
                                <owl:unionOf rdf:parseType="Collection">
                                    <owl:Restriction>
                                        <owl:onProperty rdf:resource="http://xworks.gr/ontologies/ccso#enrolledIn"/>
                                        <owl:someValuesFrom rdf:resource="http://xworks.gr/ontologies/ccso#Doctorate"/>
                                    </owl:Restriction>
                                    <owl:Restriction>
                                        <owl:onProperty rdf:resource="http://xworks.gr/ontologies/ccso#enrolledIn"/>
                                        <owl:someValuesFrom rdf:resource="http://xworks.gr/ontologies/ccso#Master"/>
                                    </owl:Restriction>
                                </owl:unionOf>
                            </owl:Class>
                        </owl:complementOf>
                    </owl:Class>
                    <owl:Restriction>
                        <owl:onProperty rdf:resource="http://xworks.gr/ontologies/ccso#enrolledIn"/>
                        <owl:qualifiedCardinality rdf:datatype="http://www.w3.org/2001/XMLSchema#nonNegativeInteger">1</owl:qualifiedCardinality>
                        <owl:onClass rdf:resource="http://xworks.gr/ontologies/ccso#Bachelor"/>
                    </owl:Restriction>
                </owl:intersectionOf>
            </owl:Class>
        </rdfs:subClassOf>
        <rdfs:comment xml:lang="en">A student who attends a university program up to the level to the Bachelor’s degree.</rdfs:comment>
        <rdfs:comment xml:lang="gr">Ένας φοιτητής που παρακολουθεί κάποιο προπτυχιακό πανεπιστημιακό πρόγραμμα σπουδών.</rdfs:comment>
        <rdfs:label xml:lang="gr">Προπτυχιακός Φοιτητής</rdfs:label>
        <skos:altLabel xml:lang="en">Undergraduate Student</skos:altLabel>
    </owl:Class>
    


    <!-- http://xworks.gr/ontologies/ccso#University -->

    <owl:Class rdf:about="http://xworks.gr/ontologies/ccso#University">
        <rdfs:subClassOf rdf:resource="http://schema.org/EducationalOrganization"/>
        <rdfs:comment xml:lang="en">An institution of Higher Education and research which awards academic degrees in a set of academic disciplines.</rdfs:comment>
        <rdfs:comment xml:lang="gr">Ένα ίδρυμα Τριτοβάθμιας Εκπαίδευσης και Έρευνας που απονέμει ακαδημαϊκούς τίτλους σε ένα σύνολο ακαδημαϊκών κλάδων.</rdfs:comment>
        <rdfs:label xml:lang="gr">Ανώτατο Εκπαιδευτικό Ίδρυμα  (Α.Ε.Ι.)</rdfs:label>
        <rdfs:label xml:lang="gr">Ανώτατο Τεχνολογικό Εκπαιδευτικό Ίδρυμα (Α.Τ.Ε.Ι.)</rdfs:label>
        <rdfs:label xml:lang="gr">Πανεπιστήμιο</rdfs:label>
    </owl:Class>
    


    <!-- 
    ///////////////////////////////////////////////////////////////////////////////////////
    //
    // Individuals
    //
    ///////////////////////////////////////////////////////////////////////////////////////
     -->

    


    <!-- http://xworks.gr/ontologies/ccso#Agrimakis_Samson -->

    <owl:NamedIndividual rdf:about="http://xworks.gr/ontologies/ccso#Agrimakis_Samson">
        <rdf:type rdf:resource="http://xmlns.com/foaf/0.1/Person"/>
        <rdf:type rdf:resource="http://xworks.gr/ontologies/ccso#PostgraduateStudent"/>
        <rdf:type rdf:resource="http://xworks.gr/ontologies/ccso#Student"/>
        <affiliatedWith rdf:resource="http://xworks.gr/ontologies/ccso#Department_of_Informatics_Engineering_of_TEI_of_Crete"/>
        <affiliatedWith rdf:resource="http://xworks.gr/ontologies/ccso#BSc_Informatics_Engineering/IE_BSc/IED/STEF/TEIC"/>
        <affiliatedWith rdf:resource="http://xworks.gr/ontologies/ccso#IM101/IM_MSc/IED/STEF/TEIC"/>
        <affiliatedWith rdf:resource="http://xworks.gr/ontologies/ccso#IM103/IM_MSc/IED/STEF/TEIC"/>
        <affiliatedWith rdf:resource="http://xworks.gr/ontologies/ccso#IM108/IM_MSc/IED/STEF/TEIC"/>
        <affiliatedWith rdf:resource="http://xworks.gr/ontologies/ccso#IM201/IM_MSc/IED/STEF/TEIC"/>
        <affiliatedWith rdf:resource="http://xworks.gr/ontologies/ccso#IM206/IM_MSc/IED/STEF/TEIC"/>
        <affiliatedWith rdf:resource="http://xworks.gr/ontologies/ccso#IM209/IM_MSc/IED/STEF/TEIC"/>
        <affiliatedWith rdf:resource="http://xworks.gr/ontologies/ccso#MSc_Informatics_&amp;_Multimedia/IM_MSc/IED/STEF/TEIC"/>
        <alumnusOf rdf:resource="http://xworks.gr/ontologies/ccso#Department_of_Informatics_Engineering_of_TEI_of_Crete"/>
        <attendsCourse rdf:resource="http://xworks.gr/ontologies/ccso#IM201/IM_MSc/IED/STEF/TEIC"/>
        <attendsCourse rdf:resource="http://xworks.gr/ontologies/ccso#IM206/IM_MSc/IED/STEF/TEIC"/>
        <attendsCourse rdf:resource="http://xworks.gr/ontologies/ccso#IM209/IM_MSc/IED/STEF/TEIC"/>
        <enrolledIn rdf:resource="http://xworks.gr/ontologies/ccso#MSc_Informatics_&amp;_Multimedia/IM_MSc/IED/STEF/TEIC"/>
        <hasCompleted rdf:resource="http://xworks.gr/ontologies/ccso#IM101/IM_MSc/IED/STEF/TEIC"/>
        <hasCompleted rdf:resource="http://xworks.gr/ontologies/ccso#IM103/IM_MSc/IED/STEF/TEIC"/>
        <hasCompleted rdf:resource="http://xworks.gr/ontologies/ccso#IM108/IM_MSc/IED/STEF/TEIC"/>
        <hasDegree rdf:resource="http://xworks.gr/ontologies/ccso#BSc_Informatics_Engineering/IE_BSc/IED/STEF/TEIC"/>
        <foaf:firstName rdf:datatype="http://www.w3.org/2001/XMLSchema#string">Samson</foaf:firstName>
        <foaf:lastName rdf:datatype="http://www.w3.org/2001/XMLSchema#string">Agrimakis</foaf:lastName>
    </owl:NamedIndividual>
    


    <!-- http://xworks.gr/ontologies/ccso#Aivalis_Costas -->

    <owl:NamedIndividual rdf:about="http://xworks.gr/ontologies/ccso#Aivalis_Costas">
        <rdf:type rdf:resource="http://xmlns.com/foaf/0.1/Person"/>
        <rdf:type rdf:resource="http://xworks.gr/ontologies/ccso#AcademicStaff"/>
        <rdf:type rdf:resource="http://xworks.gr/ontologies/ccso#Employee"/>
        <rdf:type rdf:resource="http://xworks.gr/ontologies/ccso#Professor"/>
        <affiliatedWith rdf:resource="http://xworks.gr/ontologies/ccso#Department_of_Informatics_Engineering_of_TEI_of_Crete"/>
        <affiliatedWith rdf:resource="http://xworks.gr/ontologies/ccso#TP50L4s1/IE_BSc/IED/STEF/TEIC"/>
        <affiliatedWith rdf:resource="http://xworks.gr/ontologies/ccso#TP60L5s1/IE_BSc/IED/STEF/TEIC"/>
        <instructorOf rdf:resource="http://xworks.gr/ontologies/ccso#TP50L4s1/IE_BSc/IED/STEF/TEIC"/>
        <instructorOf rdf:resource="http://xworks.gr/ontologies/ccso#TP60L5s1/IE_BSc/IED/STEF/TEIC"/>
        <memberOf rdf:resource="http://xworks.gr/ontologies/ccso#Department_of_Informatics_Engineering_of_TEI_of_Crete"/>
        <supervisorOf rdf:resource="http://xworks.gr/ontologies/ccso#TP50L4s1/IE_BSc/IED/STEF/TEIC"/>
        <supervisorOf rdf:resource="http://xworks.gr/ontologies/ccso#TP60L5s1/IE_BSc/IED/STEF/TEIC"/>
        <worksFor rdf:resource="http://xworks.gr/ontologies/ccso#Department_of_Informatics_Engineering_of_TEI_of_Crete"/>
        <schema:email rdf:datatype="http://www.w3.org/2001/XMLSchema#anyURI">aivalis@ie.teicrete.gr</schema:email>
        <foaf:firstName rdf:datatype="http://www.w3.org/2001/XMLSchema#string">Costas</foaf:firstName>
        <foaf:lastName rdf:datatype="http://www.w3.org/2001/XMLSchema#string">Aivalis</foaf:lastName>
        <eContactInfo rdf:datatype="http://www.w3.org/2001/XMLSchema#anyURI">aivalis@ie.teicrete.gr</eContactInfo>
    </owl:NamedIndividual>
    


    <!-- http://xworks.gr/ontologies/ccso#Akoumianakis_Demosthenes -->

    <owl:NamedIndividual rdf:about="http://xworks.gr/ontologies/ccso#Akoumianakis_Demosthenes">
        <rdf:type rdf:resource="http://xmlns.com/foaf/0.1/Person"/>
        <rdf:type rdf:resource="http://xworks.gr/ontologies/ccso#AcademicStaff"/>
        <rdf:type rdf:resource="http://xworks.gr/ontologies/ccso#Employee"/>
        <rdf:type rdf:resource="http://xworks.gr/ontologies/ccso#Professor"/>
        <affiliatedWith rdf:resource="http://xworks.gr/ontologies/ccso#Computers_Sciences_Department_of_University_of_Crete"/>
        <affiliatedWith rdf:resource="http://xworks.gr/ontologies/ccso#Department_of_Informatics_Engineering_of_TEI_of_Crete"/>
        <affiliatedWith rdf:resource="http://xworks.gr/ontologies/ccso#BSc_Computer_Science/CS_BSc/CSD/SSE/UoC"/>
        <affiliatedWith rdf:resource="http://xworks.gr/ontologies/ccso#IM208s1/IM_MSc/IED/STEF/TEI"/>
        <affiliatedWith rdf:resource="http://xworks.gr/ontologies/ccso#MSc_Computer_Science_and_Engineering/CSE_MSc/CSD/SSE/UoC"/>
        <affiliatedWith rdf:resource="http://xworks.gr/ontologies/ccso#PhD_Computer_Science_and_Engineering/CSE_PhD/CSD/SSE/UoC"/>
        <affiliatedWith rdf:resource="http://xworks.gr/ontologies/ccso#TP30K2s1/IE_BSc/IED/STEF/TEIC"/>
        <affiliatedWith rdf:resource="http://xworks.gr/ontologies/ccso#TP60L1s1/IE_BSc/IED/STEF/TEIC"/>
        <affiliatedWith rdf:resource="http://xworks.gr/ontologies/ccso#TP70L2s1/IE_BSc/IED/STEF/TEIC"/>
        <affiliatedWith rdf:resource="http://xworks.gr/ontologies/ccso#TP70L4s1/IE_BSc/IED/STEF/TEIC"/>
        <alumnusOf rdf:resource="http://xworks.gr/ontologies/ccso#Computers_Sciences_Department_of_University_of_Crete"/>
        <hasDegree rdf:resource="http://xworks.gr/ontologies/ccso#BSc_Computer_Science/CS_BSc/CSD/SSE/UoC"/>
        <hasDegree rdf:resource="http://xworks.gr/ontologies/ccso#MSc_Computer_Science_and_Engineering/CSE_MSc/CSD/SSE/UoC"/>
        <hasDegree rdf:resource="http://xworks.gr/ontologies/ccso#PhD_Computer_Science_and_Engineering/CSE_PhD/CSD/SSE/UoC"/>
        <instructorOf rdf:resource="http://xworks.gr/ontologies/ccso#IM208s1/IM_MSc/IED/STEF/TEI"/>
        <instructorOf rdf:resource="http://xworks.gr/ontologies/ccso#TP30K2s1/IE_BSc/IED/STEF/TEIC"/>
        <instructorOf rdf:resource="http://xworks.gr/ontologies/ccso#TP60L1s1/IE_BSc/IED/STEF/TEIC"/>
        <instructorOf rdf:resource="http://xworks.gr/ontologies/ccso#TP70L2s1/IE_BSc/IED/STEF/TEIC"/>
        <instructorOf rdf:resource="http://xworks.gr/ontologies/ccso#TP70L4s1/IE_BSc/IED/STEF/TEIC"/>
        <memberOf rdf:resource="http://xworks.gr/ontologies/ccso#Department_of_Informatics_Engineering_of_TEI_of_Crete"/>
        <supervisorOf rdf:resource="http://xworks.gr/ontologies/ccso#IM208s1/IM_MSc/IED/STEF/TEI"/>
        <supervisorOf rdf:resource="http://xworks.gr/ontologies/ccso#TP30K2s1/IE_BSc/IED/STEF/TEIC"/>
        <supervisorOf rdf:resource="http://xworks.gr/ontologies/ccso#TP60L1s1/IE_BSc/IED/STEF/TEIC"/>
        <supervisorOf rdf:resource="http://xworks.gr/ontologies/ccso#TP70L2s1/IE_BSc/IED/STEF/TEIC"/>
        <supervisorOf rdf:resource="http://xworks.gr/ontologies/ccso#TP70L4s1/IE_BSc/IED/STEF/TEIC"/>
        <worksFor rdf:resource="http://xworks.gr/ontologies/ccso#Department_of_Informatics_Engineering_of_TEI_of_Crete"/>
        <schema:email rdf:datatype="http://www.w3.org/2001/XMLSchema#anyURI">akoumianakis@ie.teicrete.gr</schema:email>
        <foaf:firstName rdf:datatype="http://www.w3.org/2001/XMLSchema#string">Demosthenes</foaf:firstName>
        <foaf:lastName rdf:datatype="http://www.w3.org/2001/XMLSchema#string">Akoumianakis</foaf:lastName>
        <eContactInfo rdf:datatype="http://www.w3.org/2001/XMLSchema#anyURI">akoumianakis@ie.teicrete.gr</eContactInfo>
    </owl:NamedIndividual>
    


    <!-- http://xworks.gr/ontologies/ccso#AlgorithmDesign_F-A-IE -->

    <owl:NamedIndividual rdf:about="http://xworks.gr/ontologies/ccso#AlgorithmDesign_F-A-IE">
        <rdf:type rdf:resource="http://xworks.gr/ontologies/ccso#Resource"/>
        <resourceCitation rdf:datatype="http://www.w3.org/2001/XMLSchema#string">Algorithm Design: Foundations, Analysis, and Internet Examples</resourceCitation>
        <rdfs:label xml:lang="en">Algorithm Design: Foundations, Analysis, and Internet Examples</rdfs:label>
    </owl:NamedIndividual>
    


    <!-- http://xworks.gr/ontologies/ccso#American_Psychological_Association_Standards_2010 -->

    <owl:NamedIndividual rdf:about="http://xworks.gr/ontologies/ccso#American_Psychological_Association_Standards_2010">
        <rdf:type rdf:resource="http://xworks.gr/ontologies/ccso#FieldofStudy"/>
        <rdf:type rdf:resource="http://xworks.gr/ontologies/ccso#KnowledgeBody"/>
        <partOfFS rdf:resource="http://xworks.gr/ontologies/ccso#Psychology"/>
        <fsName rdf:datatype="http://www.w3.org/2001/XMLSchema#string">American Psychological Association Standards 2010</fsName>
    </owl:NamedIndividual>
    


    <!-- http://xworks.gr/ontologies/ccso#Anthropology -->

    <owl:NamedIndividual rdf:about="http://xworks.gr/ontologies/ccso#Anthropology">
        <rdf:type rdf:resource="http://xworks.gr/ontologies/ccso#Discipline"/>
        <rdf:type rdf:resource="http://xworks.gr/ontologies/ccso#FieldofStudy"/>
        <fsName rdf:datatype="http://www.w3.org/2001/XMLSchema#string">Anthropology</fsName>
    </owl:NamedIndividual>
    


    <!-- http://xworks.gr/ontologies/ccso#Argyros_Antonis -->

    <owl:NamedIndividual rdf:about="http://xworks.gr/ontologies/ccso#Argyros_Antonis">
        <rdf:type rdf:resource="http://xmlns.com/foaf/0.1/Person"/>
        <rdf:type rdf:resource="http://xworks.gr/ontologies/ccso#AcademicStaff"/>
        <rdf:type rdf:resource="http://xworks.gr/ontologies/ccso#Employee"/>
        <rdf:type rdf:resource="http://xworks.gr/ontologies/ccso#Professor"/>
        <affiliatedWith rdf:resource="http://xworks.gr/ontologies/ccso#Computers_Sciences_Department_of_University_of_Crete"/>
        <affiliatedWith rdf:resource="http://xworks.gr/ontologies/ccso#CS118s1/CS_BSc/CSD/SSE/UoC"/>
        <memberOf rdf:resource="http://xworks.gr/ontologies/ccso#Computers_Sciences_Department_of_University_of_Crete"/>
        <supervisorOf rdf:resource="http://xworks.gr/ontologies/ccso#CS118s1/CS_BSc/CSD/SSE/UoC"/>
        <schema:email rdf:datatype="http://www.w3.org/2001/XMLSchema#anyURI">argyros@csd.uoc.gr</schema:email>
        <foaf:firstName rdf:datatype="http://www.w3.org/2001/XMLSchema#string">Antonis</foaf:firstName>
        <foaf:lastName rdf:datatype="http://www.w3.org/2001/XMLSchema#string">Argyros</foaf:lastName>
        <eContactInfo rdf:datatype="http://www.w3.org/2001/XMLSchema#anyURI">argyros@csd.uoc.gr</eContactInfo>
    </owl:NamedIndividual>
    


    <!-- http://xworks.gr/ontologies/ccso#Assarioti_Mellisandri -->

    <owl:NamedIndividual rdf:about="http://xworks.gr/ontologies/ccso#Assarioti_Mellisandri">
        <rdf:type rdf:resource="http://xmlns.com/foaf/0.1/Agent"/>
        <rdf:type rdf:resource="http://xmlns.com/foaf/0.1/Person"/>
        <rdf:type rdf:resource="http://xworks.gr/ontologies/ccso#PostgraduateStudent"/>
        <rdf:type rdf:resource="http://xworks.gr/ontologies/ccso#Student"/>
        <affiliatedWith rdf:resource="http://xworks.gr/ontologies/ccso#Psychology_Department_of_University_of_Crete"/>
        <affiliatedWith rdf:resource="http://xworks.gr/ontologies/ccso#BSc_Psychology/PSY_BSc/SoC/UoC"/>
        <affiliatedWith rdf:resource="http://xworks.gr/ontologies/ccso#MSc_School_Psychology/SP_MSc/PSY/SoC/UoC"/>
        <alumnusOf rdf:resource="http://xworks.gr/ontologies/ccso#Psychology_Department_of_University_of_Crete"/>
        <enrolledIn rdf:resource="http://xworks.gr/ontologies/ccso#MSc_School_Psychology/SP_MSc/PSY/SoC/UoC"/>
        <hasDegree rdf:resource="http://xworks.gr/ontologies/ccso#BSc_Psychology/PSY_BSc/SoC/UoC"/>
        <schema:email rdf:datatype="http://www.w3.org/2001/XMLSchema#anyURI">Assarioti_Mellisandri@psy.uoc.gr</schema:email>
        <foaf:firstName rdf:datatype="http://www.w3.org/2001/XMLSchema#string">Mellisandri</foaf:firstName>
        <foaf:gender rdf:datatype="http://www.w3.org/2001/XMLSchema#string">Female</foaf:gender>
        <foaf:lastName rdf:datatype="http://www.w3.org/2001/XMLSchema#string">Assarioti</foaf:lastName>
        <eContactInfo rdf:datatype="http://www.w3.org/2001/XMLSchema#anyURI">Assarioti_Mellisandri@psy.uoc.gr</eContactInfo>
    </owl:NamedIndividual>
    


    <!-- http://xworks.gr/ontologies/ccso#Assarioti_Tina -->

    <owl:NamedIndividual rdf:about="http://xworks.gr/ontologies/ccso#Assarioti_Tina">
        <rdf:type rdf:resource="http://xmlns.com/foaf/0.1/Agent"/>
        <rdf:type rdf:resource="http://xmlns.com/foaf/0.1/Person"/>
        <rdf:type rdf:resource="http://xworks.gr/ontologies/ccso#Student"/>
        <affiliatedWith rdf:resource="http://xworks.gr/ontologies/ccso#MSc_School_Psychology/SP_MSc/PSY/SoC/UoC"/>
        <enrolledIn rdf:resource="http://xworks.gr/ontologies/ccso#MSc_School_Psychology/SP_MSc/PSY/SoC/UoC"/>
        <schema:email rdf:datatype="http://www.w3.org/2001/XMLSchema#anyURI">Assarioti_Tina@psy.uoc.gr</schema:email>
        <foaf:familyName rdf:datatype="http://www.w3.org/2001/XMLSchema#string">Stark</foaf:familyName>
        <foaf:firstName rdf:datatype="http://www.w3.org/2001/XMLSchema#string">Tina</foaf:firstName>
        <foaf:gender rdf:datatype="http://www.w3.org/2001/XMLSchema#string">Female</foaf:gender>
        <foaf:lastName rdf:datatype="http://www.w3.org/2001/XMLSchema#string">Assarioti</foaf:lastName>
        <eContactInfo rdf:datatype="http://www.w3.org/2001/XMLSchema#anyURI">Assarioti_Tina@psy.uoc.gr</eContactInfo>
    </owl:NamedIndividual>
    


    <!-- http://xworks.gr/ontologies/ccso#BernersLee1998RoadmapSemanticWeb -->

    <owl:NamedIndividual rdf:about="http://xworks.gr/ontologies/ccso#BernersLee1998RoadmapSemanticWeb">
        <rdf:type rdf:resource="http://xworks.gr/ontologies/ccso#Resource"/>
        <dc:date rdf:datatype="http://www.w3.org/2001/XMLSchema#date">1998</dc:date>
        <dc:date rdf:datatype="internal:anonymous-constants">1998</dc:date>
        <dc:title rdf:datatype="http://www.w3.org/2001/XMLSchema#string">A roadmap to the Semantic Web</dc:title>
        <dates rdf:datatype="internal:anonymous-constants">1998</dates>
        <resourceCitation rdf:datatype="http://www.w3.org/2001/XMLSchema#string">Tim Berners-Lee (1998) A roadmap to the Semantic Web</resourceCitation>
        <rdfs:label xml:lang="en">Tim Berners-Lee (1998) A roadmap to the Semantic Web</rdfs:label>
    </owl:NamedIndividual>
    


    <!-- http://xworks.gr/ontologies/ccso#BernersLee2001SemanticWeb -->

    <owl:NamedIndividual rdf:about="http://xworks.gr/ontologies/ccso#BernersLee2001SemanticWeb">
        <rdf:type rdf:resource="http://xworks.gr/ontologies/ccso#Resource"/>
        <resourceCitation rdf:datatype="http://www.w3.org/2001/XMLSchema#string">Tim Berners-Lee, James Hendler and Ora Lassila (2001) The Semantic Web, Scientific American</resourceCitation>
        <rdfs:label xml:lang="en">Berners-Lee, Hendler, Lassila (2001) The Semantic Web</rdfs:label>
    </owl:NamedIndividual>
    


    <!-- http://xworks.gr/ontologies/ccso#Biology -->

    <owl:NamedIndividual rdf:about="http://xworks.gr/ontologies/ccso#Biology">
        <rdf:type rdf:resource="http://xworks.gr/ontologies/ccso#Discipline"/>
        <rdf:type rdf:resource="http://xworks.gr/ontologies/ccso#FieldofStudy"/>
        <fsName rdf:datatype="http://www.w3.org/2001/XMLSchema#string">Biology</fsName>
    </owl:NamedIndividual>
    


    <!-- http://xworks.gr/ontologies/ccso#Chemistry -->

    <owl:NamedIndividual rdf:about="http://xworks.gr/ontologies/ccso#Chemistry">
        <rdf:type rdf:resource="http://xworks.gr/ontologies/ccso#Discipline"/>
        <rdf:type rdf:resource="http://xworks.gr/ontologies/ccso#FieldofStudy"/>
        <fsName rdf:datatype="http://www.w3.org/2001/XMLSchema#string">Chemistry</fsName>
    </owl:NamedIndividual>
    


    <!-- http://xworks.gr/ontologies/ccso#Christofides_Vassilis -->

    <owl:NamedIndividual rdf:about="http://xworks.gr/ontologies/ccso#Christofides_Vassilis">
        <rdf:type rdf:resource="http://xmlns.com/foaf/0.1/Person"/>
        <rdf:type rdf:resource="http://xworks.gr/ontologies/ccso#AcademicStaff"/>
        <rdf:type rdf:resource="http://xworks.gr/ontologies/ccso#Employee"/>
        <rdf:type rdf:resource="http://xworks.gr/ontologies/ccso#Professor"/>
        <affiliatedWith rdf:resource="http://xworks.gr/ontologies/ccso#Computers_Sciences_Department_of_University_of_Crete"/>
        <affiliatedWith rdf:resource="http://xworks.gr/ontologies/ccso#CS252s1/CS_BSc/CSD/SSE/UoC"/>
        <instructorOf rdf:resource="http://xworks.gr/ontologies/ccso#CS252s1/CS_BSc/CSD/SSE/UoC"/>
        <memberOf rdf:resource="http://xworks.gr/ontologies/ccso#Computers_Sciences_Department_of_University_of_Crete"/>
        <supervisorOf rdf:resource="http://xworks.gr/ontologies/ccso#CS252s1/CS_BSc/CSD/SSE/UoC"/>
        <worksFor rdf:resource="http://xworks.gr/ontologies/ccso#Computers_Sciences_Department_of_University_of_Crete"/>
        <schema:email rdf:datatype="http://www.w3.org/2001/XMLSchema#anyURI">christofides@csd.uoc.gr</schema:email>
        <foaf:firstName rdf:datatype="http://www.w3.org/2001/XMLSchema#string">Vassilis</foaf:firstName>
        <foaf:lastName rdf:datatype="http://www.w3.org/2001/XMLSchema#string">Christofides</foaf:lastName>
        <eContactInfo rdf:datatype="http://www.w3.org/2001/XMLSchema#anyURI">christofides@csd.uoc.gr</eContactInfo>
    </owl:NamedIndividual>
    


    <!-- http://xworks.gr/ontologies/ccso#Computer_Science -->

    <owl:NamedIndividual rdf:about="http://xworks.gr/ontologies/ccso#Computer_Science">
        <rdf:type rdf:resource="http://xworks.gr/ontologies/ccso#Discipline"/>
        <rdf:type rdf:resource="http://xworks.gr/ontologies/ccso#FieldofStudy"/>
        <abbreviation rdf:datatype="http://www.w3.org/2001/XMLSchema#string">CS</abbreviation>
        <fsName rdf:datatype="http://www.w3.org/2001/XMLSchema#string">Computer Science</fsName>
    </owl:NamedIndividual>
    


    <!-- http://xworks.gr/ontologies/ccso#Computer_Science_Curricula_2013 -->

    <owl:NamedIndividual rdf:about="http://xworks.gr/ontologies/ccso#Computer_Science_Curricula_2013">
        <rdf:type rdf:resource="http://xworks.gr/ontologies/ccso#Discipline"/>
        <rdf:type rdf:resource="http://xworks.gr/ontologies/ccso#FieldofStudy"/>
        <rdf:type rdf:resource="http://xworks.gr/ontologies/ccso#KnowledgeBody"/>
        <partOfFS rdf:resource="http://xworks.gr/ontologies/ccso#Computer_Science"/>
        <abbreviation rdf:datatype="http://www.w3.org/2001/XMLSchema#string">CSC2013</abbreviation>
        <fsName rdf:datatype="http://www.w3.org/2001/XMLSchema#string">Computer Science Curricula 2013</fsName>
    </owl:NamedIndividual>
    


    <!-- http://xworks.gr/ontologies/ccso#Computers_Sciences_Department_of_University_of_Crete -->

    <owl:NamedIndividual rdf:about="http://xworks.gr/ontologies/ccso#Computers_Sciences_Department_of_University_of_Crete">
        <rdf:type rdf:resource="http://schema.org/EducationalOrganization"/>
        <rdf:type rdf:resource="http://schema.org/Organization"/>
        <rdf:type rdf:resource="http://xworks.gr/ontologies/ccso#Department"/>
        <affiliatedWith rdf:resource="http://xworks.gr/ontologies/ccso#Akoumianakis_Demosthenes"/>
        <affiliatedWith rdf:resource="http://xworks.gr/ontologies/ccso#Argyros_Antonis"/>
        <affiliatedWith rdf:resource="http://xworks.gr/ontologies/ccso#Christofides_Vassilis"/>
        <affiliatedWith rdf:resource="http://xworks.gr/ontologies/ccso#Dallas_Nektarios"/>
        <affiliatedWith rdf:resource="http://xworks.gr/ontologies/ccso#Faturou_Panagiota"/>
        <affiliatedWith rdf:resource="http://xworks.gr/ontologies/ccso#Georgakopoulos_George"/>
        <affiliatedWith rdf:resource="http://xworks.gr/ontologies/ccso#Gramma_Joanna"/>
        <affiliatedWith rdf:resource="http://xworks.gr/ontologies/ccso#Hionis_John"/>
        <affiliatedWith rdf:resource="http://xworks.gr/ontologies/ccso#Kalogiannakis_Michail"/>
        <affiliatedWith rdf:resource="http://xworks.gr/ontologies/ccso#Katevenis_Manolis"/>
        <affiliatedWith rdf:resource="http://xworks.gr/ontologies/ccso#Kondylakis_Haridimos"/>
        <affiliatedWith rdf:resource="http://xworks.gr/ontologies/ccso#Kornaros_George"/>
        <affiliatedWith rdf:resource="http://xworks.gr/ontologies/ccso#Lionis_Joshua"/>
        <affiliatedWith rdf:resource="http://xworks.gr/ontologies/ccso#Markatos_Evangelos"/>
        <affiliatedWith rdf:resource="http://xworks.gr/ontologies/ccso#Mouxtaris_Athanasios"/>
        <affiliatedWith rdf:resource="http://xworks.gr/ontologies/ccso#Papadakis_Nikos"/>
        <affiliatedWith rdf:resource="http://xworks.gr/ontologies/ccso#Papadopouli_Maria"/>
        <affiliatedWith rdf:resource="http://xworks.gr/ontologies/ccso#Pappa_Pepi"/>
        <affiliatedWith rdf:resource="http://xworks.gr/ontologies/ccso#Pasta_Flora"/>
        <affiliatedWith rdf:resource="http://xworks.gr/ontologies/ccso#Plexousakis_Dimitris"/>
        <affiliatedWith rdf:resource="http://xworks.gr/ontologies/ccso#Pratikakis_Polyvios"/>
        <affiliatedWith rdf:resource="http://xworks.gr/ontologies/ccso#Rizopoulou_Noni"/>
        <affiliatedWith rdf:resource="http://xworks.gr/ontologies/ccso#Savidis_Anthony"/>
        <affiliatedWith rdf:resource="http://xworks.gr/ontologies/ccso#Starkeiou_Michael"/>
        <affiliatedWith rdf:resource="http://xworks.gr/ontologies/ccso#Tollis_Ioannis"/>
        <affiliatedWith rdf:resource="http://xworks.gr/ontologies/ccso#Triantafillou_Irene"/>
        <affiliatedWith rdf:resource="http://xworks.gr/ontologies/ccso#Tsakalidis_Panayiotis"/>
        <affiliatedWith rdf:resource="http://xworks.gr/ontologies/ccso#Tsiknakis_Manolis"/>
        <affiliatedWith rdf:resource="http://xworks.gr/ontologies/ccso#Tziritas_George"/>
        <affiliatedWith rdf:resource="http://xworks.gr/ontologies/ccso#Vassilakis_Kostas"/>
        <affiliatedWith rdf:resource="http://xworks.gr/ontologies/ccso#Vassilakis_Vassilis"/>
        <belongsTo rdf:resource="http://xworks.gr/ontologies/ccso#School_of_Sciences_and_Engineering_of_University_of_Crete"/>
        <belongsTo rdf:resource="http://xworks.gr/ontologies/ccso#University_of_Crete"/>
        <hasAcademicStaff rdf:resource="http://xworks.gr/ontologies/ccso#Argyros_Antonis"/>
        <hasAcademicStaff rdf:resource="http://xworks.gr/ontologies/ccso#Christofides_Vassilis"/>
        <hasAcademicStaff rdf:resource="http://xworks.gr/ontologies/ccso#Faturou_Panagiota"/>
        <hasAcademicStaff rdf:resource="http://xworks.gr/ontologies/ccso#Georgakopoulos_George"/>
        <hasAcademicStaff rdf:resource="http://xworks.gr/ontologies/ccso#Kalogiannakis_Michail"/>
        <hasAcademicStaff rdf:resource="http://xworks.gr/ontologies/ccso#Katevenis_Manolis"/>
        <hasAcademicStaff rdf:resource="http://xworks.gr/ontologies/ccso#Markatos_Evangelos"/>
        <hasAcademicStaff rdf:resource="http://xworks.gr/ontologies/ccso#Mouxtaris_Athanasios"/>
        <hasAcademicStaff rdf:resource="http://xworks.gr/ontologies/ccso#Papadopouli_Maria"/>
        <hasAcademicStaff rdf:resource="http://xworks.gr/ontologies/ccso#Plexousakis_Dimitris"/>
        <hasAcademicStaff rdf:resource="http://xworks.gr/ontologies/ccso#Pratikakis_Polyvios"/>
        <hasAcademicStaff rdf:resource="http://xworks.gr/ontologies/ccso#Rizopoulou_Noni"/>
        <hasAcademicStaff rdf:resource="http://xworks.gr/ontologies/ccso#Savidis_Anthony"/>
        <hasAcademicStaff rdf:resource="http://xworks.gr/ontologies/ccso#Tollis_Ioannis"/>
        <hasAcademicStaff rdf:resource="http://xworks.gr/ontologies/ccso#Tsakalidis_Panayiotis"/>
        <hasAcademicStaff rdf:resource="http://xworks.gr/ontologies/ccso#Tsiknakis_Manolis"/>
        <hasAcademicStaff rdf:resource="http://xworks.gr/ontologies/ccso#Tziritas_George"/>
        <hasAlumnus rdf:resource="http://xworks.gr/ontologies/ccso#Akoumianakis_Demosthenes"/>
        <hasAlumnus rdf:resource="http://xworks.gr/ontologies/ccso#Dallas_Nektarios"/>
        <hasAlumnus rdf:resource="http://xworks.gr/ontologies/ccso#Hionis_John"/>
        <hasAlumnus rdf:resource="http://xworks.gr/ontologies/ccso#Kalogiannakis_Michail"/>
        <hasAlumnus rdf:resource="http://xworks.gr/ontologies/ccso#Kondylakis_Haridimos"/>
        <hasAlumnus rdf:resource="http://xworks.gr/ontologies/ccso#Kornaros_George"/>
        <hasAlumnus rdf:resource="http://xworks.gr/ontologies/ccso#Lionis_Joshua"/>
        <hasAlumnus rdf:resource="http://xworks.gr/ontologies/ccso#Papadakis_Nikos"/>
        <hasAlumnus rdf:resource="http://xworks.gr/ontologies/ccso#Starkeiou_Michael"/>
        <hasAlumnus rdf:resource="http://xworks.gr/ontologies/ccso#Triantafillou_Irene"/>
        <hasAlumnus rdf:resource="http://xworks.gr/ontologies/ccso#Tsiknakis_Manolis"/>
        <hasAlumnus rdf:resource="http://xworks.gr/ontologies/ccso#Vassilakis_Kostas"/>
        <hasAlumnus rdf:resource="http://xworks.gr/ontologies/ccso#Vassilakis_Vassilis"/>
        <hasEmployee rdf:resource="http://xworks.gr/ontologies/ccso#Christofides_Vassilis"/>
        <hasEmployee rdf:resource="http://xworks.gr/ontologies/ccso#Faturou_Panagiota"/>
        <hasEmployee rdf:resource="http://xworks.gr/ontologies/ccso#Georgakopoulos_George"/>
        <hasEmployee rdf:resource="http://xworks.gr/ontologies/ccso#Gramma_Joanna"/>
        <hasEmployee rdf:resource="http://xworks.gr/ontologies/ccso#Kalogiannakis_Michail"/>
        <hasEmployee rdf:resource="http://xworks.gr/ontologies/ccso#Katevenis_Manolis"/>
        <hasEmployee rdf:resource="http://xworks.gr/ontologies/ccso#Kondylakis_Haridimos"/>
        <hasEmployee rdf:resource="http://xworks.gr/ontologies/ccso#Markatos_Evangelos"/>
        <hasEmployee rdf:resource="http://xworks.gr/ontologies/ccso#Mouxtaris_Athanasios"/>
        <hasEmployee rdf:resource="http://xworks.gr/ontologies/ccso#Papadopouli_Maria"/>
        <hasEmployee rdf:resource="http://xworks.gr/ontologies/ccso#Pappa_Pepi"/>
        <hasEmployee rdf:resource="http://xworks.gr/ontologies/ccso#Pasta_Flora"/>
        <hasEmployee rdf:resource="http://xworks.gr/ontologies/ccso#Plexousakis_Dimitris"/>
        <hasEmployee rdf:resource="http://xworks.gr/ontologies/ccso#Rizopoulou_Noni"/>
        <hasEmployee rdf:resource="http://xworks.gr/ontologies/ccso#Savidis_Anthony"/>
        <hasEmployee rdf:resource="http://xworks.gr/ontologies/ccso#Tollis_Ioannis"/>
        <hasEmployee rdf:resource="http://xworks.gr/ontologies/ccso#Tsakalidis_Panayiotis"/>
        <hasEmployee rdf:resource="http://xworks.gr/ontologies/ccso#Tsiknakis_Manolis"/>
        <hasEmployee rdf:resource="http://xworks.gr/ontologies/ccso#Tziritas_George"/>
        <offersCourse rdf:resource="http://xworks.gr/ontologies/ccso#CS100/CS_BSc/CSD/SSE/UoC"/>
        <offersCourse rdf:resource="http://xworks.gr/ontologies/ccso#CS108/CS_BSc/CSD/SSE/UoC"/>
        <offersCourse rdf:resource="http://xworks.gr/ontologies/ccso#CS109/CS_BSc/CSD/SSE/UoC"/>
        <offersCourse rdf:resource="http://xworks.gr/ontologies/ccso#CS110/CS_BSc/CSD/SSE/UoC"/>
        <offersCourse rdf:resource="http://xworks.gr/ontologies/ccso#CS118/CS_BSc/CSD/SSE/UoC"/>
        <offersCourse rdf:resource="http://xworks.gr/ontologies/ccso#CS119/CS_BSc/CSD/SSE/UoC"/>
        <offersCourse rdf:resource="http://xworks.gr/ontologies/ccso#CS120/CS_BSc/CSD/SSE/UoC"/>
        <offersCourse rdf:resource="http://xworks.gr/ontologies/ccso#CS150/CS_BSc/CSD/SSE/UoC"/>
        <offersCourse rdf:resource="http://xworks.gr/ontologies/ccso#CS180/CS_BSc/CSD/SSE/UoC"/>
        <offersCourse rdf:resource="http://xworks.gr/ontologies/ccso#CS208/CS_BSc/CSD/SSE/UoC"/>
        <offersCourse rdf:resource="http://xworks.gr/ontologies/ccso#CS209/CS_BSc/CSD/SSE/UoC"/>
        <offersCourse rdf:resource="http://xworks.gr/ontologies/ccso#CS215/CS_BSc/CSD/SSE/UoC"/>
        <offersCourse rdf:resource="http://xworks.gr/ontologies/ccso#CS217/CS_BSc/CSD/SSE/UoC"/>
        <offersCourse rdf:resource="http://xworks.gr/ontologies/ccso#CS220/CS_BSc/CSD/SSE/UoC"/>
        <offersCourse rdf:resource="http://xworks.gr/ontologies/ccso#CS225/CS_BSc/CSD/SSE/UoC"/>
        <offersCourse rdf:resource="http://xworks.gr/ontologies/ccso#CS240/CS_BSc/CSD/SSE/UoC"/>
        <offersCourse rdf:resource="http://xworks.gr/ontologies/ccso#CS252/CS_BSc/CSD/SSE/UoC"/>
        <offersCourse rdf:resource="http://xworks.gr/ontologies/ccso#CS255/CS_BSc/CSD/SSE/UoC"/>
        <offersCourse rdf:resource="http://xworks.gr/ontologies/ccso#CS280/CS_BSc/CSD/SSE/UoC"/>
        <offersCourse rdf:resource="http://xworks.gr/ontologies/ccso#CS302/CS_BSc/CSD/SSE/UoC"/>
        <offersCourse rdf:resource="http://xworks.gr/ontologies/ccso#CS317/CS_BSc/CSD/SSE/UoC"/>
        <offersCourse rdf:resource="http://xworks.gr/ontologies/ccso#CS330/CS_BSc/CSD/SSE/UoC"/>
        <offersCourse rdf:resource="http://xworks.gr/ontologies/ccso#CS335/CS_BSc/CSD/SSE/UoC"/>
        <offersCourse rdf:resource="http://xworks.gr/ontologies/ccso#CS340/CS_BSc/CSD/SSE/UoC"/>
        <offersCourse rdf:resource="http://xworks.gr/ontologies/ccso#CS342/CS_BSc/CSD/SSE/UoC"/>
        <offersCourse rdf:resource="http://xworks.gr/ontologies/ccso#CS345/CS_BSc/CSD/SSE/UoC"/>
        <offersCourse rdf:resource="http://xworks.gr/ontologies/ccso#CS351/CS_BSc/CSD/SSE/UoC"/>
        <offersCourse rdf:resource="http://xworks.gr/ontologies/ccso#CS352/CS_BSc/CSD/SSE/UoC"/>
        <offersCourse rdf:resource="http://xworks.gr/ontologies/ccso#CS358/CS_BSc/CSD/SSE/UoC"/>
        <offersCourse rdf:resource="http://xworks.gr/ontologies/ccso#CS360/CS_BSc/CSD/SSE/UoC"/>
        <offersCourse rdf:resource="http://xworks.gr/ontologies/ccso#CS364/CS_BSc/CSD/SSE/UoC"/>
        <offersCourse rdf:resource="http://xworks.gr/ontologies/ccso#CS370/CS_BSc/CSD/SSE/UoC"/>
        <offersCourse rdf:resource="http://xworks.gr/ontologies/ccso#CS371/CS_BSc/CSD/SSE/UoC"/>
        <offersCourse rdf:resource="http://xworks.gr/ontologies/ccso#CS380/CS_BSc/CSD/SSE/UoC"/>
        <offersCourse rdf:resource="http://xworks.gr/ontologies/ccso#CS383/CS_BSc/CSD/SSE/UoC"/>
        <offersCourse rdf:resource="http://xworks.gr/ontologies/ccso#CS387/CS_BSc/CSD/SSE/UoC"/>
        <offersCourse rdf:resource="http://xworks.gr/ontologies/ccso#CS404/CS_BSc/CSD/SSE/UoC"/>
        <offersCourse rdf:resource="http://xworks.gr/ontologies/ccso#CS422/CS_BSc/CSD/SSE/UoC"/>
        <offersCourse rdf:resource="http://xworks.gr/ontologies/ccso#CS425/CS_BSc/CSD/SSE/UoC"/>
        <offersCourse rdf:resource="http://xworks.gr/ontologies/ccso#CS428/CS_BSc/CSD/SSE/UoC"/>
        <offersCourse rdf:resource="http://xworks.gr/ontologies/ccso#CS435/CS_BSc/CSD/SSE/UoC"/>
        <offersCourse rdf:resource="http://xworks.gr/ontologies/ccso#CS436/CS_BSc/CSD/SSE/UoC"/>
        <offersCourse rdf:resource="http://xworks.gr/ontologies/ccso#CS439/CS_BSc/CSD/SSE/UoC"/>
        <offersCourse rdf:resource="http://xworks.gr/ontologies/ccso#CS446/CS_BSc/CSD/SSE/UoC"/>
        <offersCourse rdf:resource="http://xworks.gr/ontologies/ccso#CS452/CS_BSc/CSD/SSE/UoC"/>
        <offersCourse rdf:resource="http://xworks.gr/ontologies/ccso#CS455/CS_BSc/CSD/SSE/UoC"/>
        <offersCourse rdf:resource="http://xworks.gr/ontologies/ccso#CS457/CS_BSc/CSD/SSE/UoC"/>
        <offersCourse rdf:resource="http://xworks.gr/ontologies/ccso#CS459/CS_BSc/CSD/SSE/UoC"/>
        <offersCourse rdf:resource="http://xworks.gr/ontologies/ccso#CS460/CS_BSc/CSD/SSE/UoC"/>
        <offersCourse rdf:resource="http://xworks.gr/ontologies/ccso#CS463/CS_BSc/CSD/SSE/UoC"/>
        <offersCourse rdf:resource="http://xworks.gr/ontologies/ccso#CS468/CS_BSc/CSD/SSE/UoC"/>
        <offersCourse rdf:resource="http://xworks.gr/ontologies/ccso#CS469/CS_BSc/CSD/SSE/UoC"/>
        <offersCourse rdf:resource="http://xworks.gr/ontologies/ccso#CS471/CS_BSc/CSD/SSE/UoC"/>
        <offersCourse rdf:resource="http://xworks.gr/ontologies/ccso#CS472/CS_BSc/CSD/SSE/UoC"/>
        <offersCourse rdf:resource="http://xworks.gr/ontologies/ccso#CS473/CS_BSc/CSD/SSE/UoC"/>
        <offersCourse rdf:resource="http://xworks.gr/ontologies/ccso#CS474/CS_BSc/CSD/SSE/UoC"/>
        <offersCourse rdf:resource="http://xworks.gr/ontologies/ccso#CS475/CS_BSc/CSD/SSE/UoC"/>
        <offersCourse rdf:resource="http://xworks.gr/ontologies/ccso#CS482/CS_BSc/CSD/SSE/UoC"/>
        <offersCourse rdf:resource="http://xworks.gr/ontologies/ccso#CS486/CS_BSc/CSD/SSE/UoC"/>
        <offersCourse rdf:resource="http://xworks.gr/ontologies/ccso#CS499/CS_BSc/CSD/SSE/UoC"/>
        <offersCourse rdf:resource="http://xworks.gr/ontologies/ccso#CS539/CSE_MSc/CSD/SSE/UoC"/>
        <offersCourse rdf:resource="http://xworks.gr/ontologies/ccso#CS540/CSE_MSc/CSD/SSE/UoC"/>
        <offersCourse rdf:resource="http://xworks.gr/ontologies/ccso#CS672/CSE_PhD/CSD/SSE/UoC"/>
        <providesProgram rdf:resource="http://xworks.gr/ontologies/ccso#BSc_Computer_Science/CS_BSc/CSD/SSE/UoC"/>
        <providesProgram rdf:resource="http://xworks.gr/ontologies/ccso#MSc_Computer_Science_and_Engineering/CSE_MSc/CSD/SSE/UoC"/>
        <providesProgram rdf:resource="http://xworks.gr/ontologies/ccso#PhD_Computer_Science_and_Engineering/CSE_PhD/CSD/SSE/UoC"/>
        <schema:address rdf:datatype="http://www.w3.org/2001/XMLSchema#string">Computers Sciences Department
Univesity of Crete
Voutes Campus
70013, Heraklion
Crete</schema:address>
        <schema:email rdf:datatype="http://www.w3.org/2001/XMLSchema#anyURI">csd@csd.uoc.gr</schema:email>
        <schema:faxNumber rdf:datatype="http://www.w3.org/2001/XMLSchema#string">+30 2810393501</schema:faxNumber>
        <schema:identifier rdf:datatype="http://www.w3.org/2001/XMLSchema#string">CSD/SSE/UoC</schema:identifier>
        <schema:legalName rdf:datatype="http://www.w3.org/2001/XMLSchema#string">Computers Sciences Department of University of Crete</schema:legalName>
        <schema:legalName rdf:datatype="http://www.w3.org/2001/XMLSchema#string">Τμήμα Επιστήμης Υπολογιστών Πανεπιστημίου Κρήτης</schema:legalName>
        <schema:location rdf:datatype="http://www.w3.org/2001/XMLSchema#string">Voutes Heraklion</schema:location>
        <schema:logo rdf:datatype="http://www.w3.org/2001/XMLSchema#anyURI">http://csd.uoc.gr/CSD/images/csd_logo_2.png</schema:logo>
        <schema:url rdf:datatype="http://www.w3.org/2001/XMLSchema#anyURI">http://csd.uoc.gr</schema:url>
        <eContactInfo rdf:datatype="http://www.w3.org/2001/XMLSchema#anyURI">csd@csd.uoc.gr</eContactInfo>
        <eContactInfo rdf:datatype="http://www.w3.org/2001/XMLSchema#anyURI">http://csd.uoc.gr</eContactInfo>
        <phone rdf:datatype="http://www.w3.org/2001/XMLSchema#string">+30 2810393500</phone>
        <phone rdf:datatype="http://www.w3.org/2001/XMLSchema#string">+30 2810393501</phone>
        <workPhone rdf:datatype="http://www.w3.org/2001/XMLSchema#string">+30 2810393500</workPhone>
        <rdfs:label xml:lang="en">Computers Sciences Department | University of Crete</rdfs:label>
        <rdfs:label xml:lang="gr">Τμήμα Επιστήμης Υπολογιστών | Πανεπιστήμιο Κρήτης</rdfs:label>
    </owl:NamedIndividual>
    


    <!-- http://xworks.gr/ontologies/ccso#DEK_Technician_for_Networks_and_Telecommunications_of_IEK -->

    <owl:NamedIndividual rdf:about="http://xworks.gr/ontologies/ccso#DEK_Technician_for_Networks_and_Telecommunications_of_IEK">
        <rdf:type rdf:resource="http://xworks.gr/ontologies/ccso#Certificate"/>
        <rdf:type rdf:resource="http://xworks.gr/ontologies/ccso#ProgramofStudy"/>
        <degreeTitle rdf:datatype="http://www.w3.org/2001/XMLSchema#string">Vocational Training Diploma IEK
Technician for Networks and Telecommunications</degreeTitle>
        <degreeTitle rdf:datatype="http://www.w3.org/2001/XMLSchema#string">Δίπλωμα Επαγγελματικής Κατάρτισης IEK
Τεχνικός Δικτύων και Τηλεπικοινωνιών</degreeTitle>
        <degreeType rdf:datatype="http://www.w3.org/2001/XMLSchema#string">Vocational Training Diploma - IEK level 4</degreeType>
        <degreeType rdf:datatype="http://www.w3.org/2001/XMLSchema#string">Δίπλωμα Επαγγελματικής Κατάρτισης - ΙΕΚ επιπέδου 4</degreeType>
        <psName rdf:datatype="http://www.w3.org/2001/XMLSchema#string">DEK Technician for Networks and Telecommunications IEK</psName>
        <psName rdf:datatype="http://www.w3.org/2001/XMLSchema#string">ΔEK Τεχνικός Δικτύων και Τηλεπικοινωνιών IEK</psName>
        <rdfs:label xml:lang="en">DEK Technician for Networks and Telecommunications IEK</rdfs:label>
        <rdfs:label xml:lang="gr">ΔEK Τεχνικός Δικτύων και Τηλεπικοινωνιών IEK</rdfs:label>
    </owl:NamedIndividual>
    


    <!-- http://xworks.gr/ontologies/ccso#Dallas_Nektarios -->

    <owl:NamedIndividual rdf:about="http://xworks.gr/ontologies/ccso#Dallas_Nektarios">
        <rdf:type rdf:resource="http://xmlns.com/foaf/0.1/Agent"/>
        <rdf:type rdf:resource="http://xmlns.com/foaf/0.1/Person"/>
        <rdf:type rdf:resource="http://xworks.gr/ontologies/ccso#PostgraduateStudent"/>
        <rdf:type rdf:resource="http://xworks.gr/ontologies/ccso#Student"/>
        <affiliatedWith rdf:resource="http://xworks.gr/ontologies/ccso#Computers_Sciences_Department_of_University_of_Crete"/>
        <affiliatedWith rdf:resource="http://xworks.gr/ontologies/ccso#BSc_Computer_Science/CS_BSc/CSD/SSE/UoC"/>
        <affiliatedWith rdf:resource="http://xworks.gr/ontologies/ccso#IM101/IM_MSc/IED/STEF/TEIC"/>
        <affiliatedWith rdf:resource="http://xworks.gr/ontologies/ccso#IM104/IM_MSc/IED/STEF/TEIC"/>
        <affiliatedWith rdf:resource="http://xworks.gr/ontologies/ccso#IM107/IM_MSc/IED/STEF/TEIC"/>
        <affiliatedWith rdf:resource="http://xworks.gr/ontologies/ccso#IM109/IM_MSc/IED/STEF/TEIC"/>
        <affiliatedWith rdf:resource="http://xworks.gr/ontologies/ccso#IM201/IM_MSc/IED/STEF/TEIC"/>
        <affiliatedWith rdf:resource="http://xworks.gr/ontologies/ccso#IM204/IM_MSc/IED/STEF/TEIC"/>
        <affiliatedWith rdf:resource="http://xworks.gr/ontologies/ccso#IM209/IM_MSc/IED/STEF/TEIC"/>
        <affiliatedWith rdf:resource="http://xworks.gr/ontologies/ccso#MSc_Informatics_&amp;_Multimedia/IM_MSc/IED/STEF/TEIC"/>
        <alumnusOf rdf:resource="http://xworks.gr/ontologies/ccso#Computers_Sciences_Department_of_University_of_Crete"/>
        <attendsCourse rdf:resource="http://xworks.gr/ontologies/ccso#IM201/IM_MSc/IED/STEF/TEIC"/>
        <attendsCourse rdf:resource="http://xworks.gr/ontologies/ccso#IM204/IM_MSc/IED/STEF/TEIC"/>
        <attendsCourse rdf:resource="http://xworks.gr/ontologies/ccso#IM209/IM_MSc/IED/STEF/TEIC"/>
        <enrolledIn rdf:resource="http://xworks.gr/ontologies/ccso#MSc_Informatics_&amp;_Multimedia/IM_MSc/IED/STEF/TEIC"/>
        <hasCompleted rdf:resource="http://xworks.gr/ontologies/ccso#IM101/IM_MSc/IED/STEF/TEIC"/>
        <hasCompleted rdf:resource="http://xworks.gr/ontologies/ccso#IM104/IM_MSc/IED/STEF/TEIC"/>
        <hasCompleted rdf:resource="http://xworks.gr/ontologies/ccso#IM107/IM_MSc/IED/STEF/TEIC"/>
        <hasCompleted rdf:resource="http://xworks.gr/ontologies/ccso#IM109/IM_MSc/IED/STEF/TEIC"/>
        <hasDegree rdf:resource="http://xworks.gr/ontologies/ccso#BSc_Computer_Science/CS_BSc/CSD/SSE/UoC"/>
        <schema:email rdf:datatype="http://www.w3.org/2001/XMLSchema#anyURI">Dallas_Nektarios@csd.uoc.gr</schema:email>
        <foaf:firstName rdf:datatype="http://www.w3.org/2001/XMLSchema#string">Nektarios</foaf:firstName>
        <foaf:gender rdf:datatype="http://www.w3.org/2001/XMLSchema#string">Male</foaf:gender>
        <foaf:lastName rdf:datatype="http://www.w3.org/2001/XMLSchema#string">Dallas</foaf:lastName>
        <eContactInfo rdf:datatype="http://www.w3.org/2001/XMLSchema#anyURI">Dallas_Nektarios@csd.uoc.gr</eContactInfo>
    </owl:NamedIndividual>
    


    <!-- http://xworks.gr/ontologies/ccso#Demonstration -->

    <owl:NamedIndividual rdf:about="http://xworks.gr/ontologies/ccso#Demonstration">
        <rdf:type rdf:resource="http://xworks.gr/ontologies/ccso#TeachingEvaluationMethod"/>
        <mediaUsed rdf:datatype="http://www.w3.org/2001/XMLSchema#string">Computer, Projector</mediaUsed>
        <methodName rdf:datatype="http://www.w3.org/2001/XMLSchema#string">Demonstration</methodName>
    </owl:NamedIndividual>
    


    <!-- http://xworks.gr/ontologies/ccso#Department_of_Informatics_Engineering_of_TEI_of_Crete -->

    <owl:NamedIndividual rdf:about="http://xworks.gr/ontologies/ccso#Department_of_Informatics_Engineering_of_TEI_of_Crete">
        <rdf:type rdf:resource="http://schema.org/EducationalOrganization"/>
        <rdf:type rdf:resource="http://schema.org/Organization"/>
        <rdf:type rdf:resource="http://xworks.gr/ontologies/ccso#Department"/>
        <affiliatedWith rdf:resource="http://xworks.gr/ontologies/ccso#Agrimakis_Samson"/>
        <affiliatedWith rdf:resource="http://xworks.gr/ontologies/ccso#Aivalis_Costas"/>
        <affiliatedWith rdf:resource="http://xworks.gr/ontologies/ccso#Akoumianakis_Demosthenes"/>
        <affiliatedWith rdf:resource="http://xworks.gr/ontologies/ccso#Fragopoulou_Paraskevi"/>
        <affiliatedWith rdf:resource="http://xworks.gr/ontologies/ccso#Grammatikakis_Miltiadis"/>
        <affiliatedWith rdf:resource="http://xworks.gr/ontologies/ccso#Kalogiannakis_Michail"/>
        <affiliatedWith rdf:resource="http://xworks.gr/ontologies/ccso#Karagiannakis_Dimitrios"/>
        <affiliatedWith rdf:resource="http://xworks.gr/ontologies/ccso#Katis_Evangelos"/>
        <affiliatedWith rdf:resource="http://xworks.gr/ontologies/ccso#Kokkinos_Heraklis"/>
        <affiliatedWith rdf:resource="http://xworks.gr/ontologies/ccso#Kondylakis_Haridimos"/>
        <affiliatedWith rdf:resource="http://xworks.gr/ontologies/ccso#Kornaros_George"/>
        <affiliatedWith rdf:resource="http://xworks.gr/ontologies/ccso#Malamos_Athanasios"/>
        <affiliatedWith rdf:resource="http://xworks.gr/ontologies/ccso#Manifavas_Harry"/>
        <affiliatedWith rdf:resource="http://xworks.gr/ontologies/ccso#Marakakis_Manolis"/>
        <affiliatedWith rdf:resource="http://xworks.gr/ontologies/ccso#Marias_Kostas"/>
        <affiliatedWith rdf:resource="http://xworks.gr/ontologies/ccso#Martelis_Stelios"/>
        <affiliatedWith rdf:resource="http://xworks.gr/ontologies/ccso#Mastorakis_George"/>
        <affiliatedWith rdf:resource="http://xworks.gr/ontologies/ccso#Pachoulakis_Ioannis"/>
        <affiliatedWith rdf:resource="http://xworks.gr/ontologies/ccso#Pallis_Evangelos"/>
        <affiliatedWith rdf:resource="http://xworks.gr/ontologies/ccso#Panagiotakis_Spyros"/>
        <affiliatedWith rdf:resource="http://xworks.gr/ontologies/ccso#Papadakis_Nikos"/>
        <affiliatedWith rdf:resource="http://xworks.gr/ontologies/ccso#Papadourakis_George"/>
        <affiliatedWith rdf:resource="http://xworks.gr/ontologies/ccso#Pappa_Pepi"/>
        <affiliatedWith rdf:resource="http://xworks.gr/ontologies/ccso#Raderis_Jim"/>
        <affiliatedWith rdf:resource="http://xworks.gr/ontologies/ccso#Sandi_Elina"/>
        <affiliatedWith rdf:resource="http://xworks.gr/ontologies/ccso#Starkeiou_Alexandros"/>
        <affiliatedWith rdf:resource="http://xworks.gr/ontologies/ccso#Starkeiou_Aria"/>
        <affiliatedWith rdf:resource="http://xworks.gr/ontologies/ccso#Stratakis_Dimitrios"/>
        <affiliatedWith rdf:resource="http://xworks.gr/ontologies/ccso#Triantafyllidis_George"/>
        <affiliatedWith rdf:resource="http://xworks.gr/ontologies/ccso#Tsiknakis_Manolis"/>
        <affiliatedWith rdf:resource="http://xworks.gr/ontologies/ccso#Vassilakis_Kostas"/>
        <affiliatedWith rdf:resource="http://xworks.gr/ontologies/ccso#Vassileiou_Tom"/>
        <affiliatedWith rdf:resource="http://xworks.gr/ontologies/ccso#Vidakis_Nikolaos"/>
        <affiliatedWith rdf:resource="http://xworks.gr/ontologies/ccso#Vourkas_Michail"/>
        <affiliatedWith rdf:resource="http://xworks.gr/ontologies/ccso#Xezonakis_Ioannis"/>
        <belongsTo rdf:resource="http://xworks.gr/ontologies/ccso#School_of_Engineering_of_TEI_of_Crete"/>
        <belongsTo rdf:resource="http://xworks.gr/ontologies/ccso#TEI_of_Crete"/>
        <hasAcademicStaff rdf:resource="http://xworks.gr/ontologies/ccso#Aivalis_Costas"/>
        <hasAcademicStaff rdf:resource="http://xworks.gr/ontologies/ccso#Akoumianakis_Demosthenes"/>
        <hasAcademicStaff rdf:resource="http://xworks.gr/ontologies/ccso#Fragopoulou_Paraskevi"/>
        <hasAcademicStaff rdf:resource="http://xworks.gr/ontologies/ccso#Grammatikakis_Miltiadis"/>
        <hasAcademicStaff rdf:resource="http://xworks.gr/ontologies/ccso#Kalogiannakis_Michail"/>
        <hasAcademicStaff rdf:resource="http://xworks.gr/ontologies/ccso#Karagiannakis_Dimitrios"/>
        <hasAcademicStaff rdf:resource="http://xworks.gr/ontologies/ccso#Kornaros_George"/>
        <hasAcademicStaff rdf:resource="http://xworks.gr/ontologies/ccso#Malamos_Athanasios"/>
        <hasAcademicStaff rdf:resource="http://xworks.gr/ontologies/ccso#Manifavas_Harry"/>
        <hasAcademicStaff rdf:resource="http://xworks.gr/ontologies/ccso#Marakakis_Manolis"/>
        <hasAcademicStaff rdf:resource="http://xworks.gr/ontologies/ccso#Marias_Kostas"/>
        <hasAcademicStaff rdf:resource="http://xworks.gr/ontologies/ccso#Mastorakis_George"/>
        <hasAcademicStaff rdf:resource="http://xworks.gr/ontologies/ccso#Pachoulakis_Ioannis"/>
        <hasAcademicStaff rdf:resource="http://xworks.gr/ontologies/ccso#Pallis_Evangelos"/>
        <hasAcademicStaff rdf:resource="http://xworks.gr/ontologies/ccso#Panagiotakis_Spyros"/>
        <hasAcademicStaff rdf:resource="http://xworks.gr/ontologies/ccso#Papadakis_Nikos"/>
        <hasAcademicStaff rdf:resource="http://xworks.gr/ontologies/ccso#Papadourakis_George"/>
        <hasAcademicStaff rdf:resource="http://xworks.gr/ontologies/ccso#Stratakis_Dimitrios"/>
        <hasAcademicStaff rdf:resource="http://xworks.gr/ontologies/ccso#Triantafyllidis_George"/>
        <hasAcademicStaff rdf:resource="http://xworks.gr/ontologies/ccso#Tsiknakis_Manolis"/>
        <hasAcademicStaff rdf:resource="http://xworks.gr/ontologies/ccso#Vassilakis_Kostas"/>
        <hasAcademicStaff rdf:resource="http://xworks.gr/ontologies/ccso#Vidakis_Nikolaos"/>
        <hasAcademicStaff rdf:resource="http://xworks.gr/ontologies/ccso#Vourkas_Michail"/>
        <hasAcademicStaff rdf:resource="http://xworks.gr/ontologies/ccso#Xezonakis_Ioannis"/>
        <hasAlumnus rdf:resource="http://xworks.gr/ontologies/ccso#Agrimakis_Samson"/>
        <hasAlumnus rdf:resource="http://xworks.gr/ontologies/ccso#Kokkinos_Heraklis"/>
        <hasAlumnus rdf:resource="http://xworks.gr/ontologies/ccso#Kornaros_George"/>
        <hasAlumnus rdf:resource="http://xworks.gr/ontologies/ccso#Martelis_Stelios"/>
        <hasAlumnus rdf:resource="http://xworks.gr/ontologies/ccso#Raderis_Jim"/>
        <hasAlumnus rdf:resource="http://xworks.gr/ontologies/ccso#Sandi_Elina"/>
        <hasAlumnus rdf:resource="http://xworks.gr/ontologies/ccso#Starkeiou_Alexandros"/>
        <hasAlumnus rdf:resource="http://xworks.gr/ontologies/ccso#Starkeiou_Aria"/>
        <hasAlumnus rdf:resource="http://xworks.gr/ontologies/ccso#Vassileiou_Tom"/>
        <hasEmployee rdf:resource="http://xworks.gr/ontologies/ccso#Aivalis_Costas"/>
        <hasEmployee rdf:resource="http://xworks.gr/ontologies/ccso#Akoumianakis_Demosthenes"/>
        <hasEmployee rdf:resource="http://xworks.gr/ontologies/ccso#Fragopoulou_Paraskevi"/>
        <hasEmployee rdf:resource="http://xworks.gr/ontologies/ccso#Grammatikakis_Miltiadis"/>
        <hasEmployee rdf:resource="http://xworks.gr/ontologies/ccso#Kalogiannakis_Michail"/>
        <hasEmployee rdf:resource="http://xworks.gr/ontologies/ccso#Karagiannakis_Dimitrios"/>
        <hasEmployee rdf:resource="http://xworks.gr/ontologies/ccso#Katis_Evangelos"/>
        <hasEmployee rdf:resource="http://xworks.gr/ontologies/ccso#Kondylakis_Haridimos"/>
        <hasEmployee rdf:resource="http://xworks.gr/ontologies/ccso#Kornaros_George"/>
        <hasEmployee rdf:resource="http://xworks.gr/ontologies/ccso#Malamos_Athanasios"/>
        <hasEmployee rdf:resource="http://xworks.gr/ontologies/ccso#Manifavas_Harry"/>
        <hasEmployee rdf:resource="http://xworks.gr/ontologies/ccso#Marakakis_Manolis"/>
        <hasEmployee rdf:resource="http://xworks.gr/ontologies/ccso#Marias_Kostas"/>
        <hasEmployee rdf:resource="http://xworks.gr/ontologies/ccso#Pachoulakis_Ioannis"/>
        <hasEmployee rdf:resource="http://xworks.gr/ontologies/ccso#Pallis_Evangelos"/>
        <hasEmployee rdf:resource="http://xworks.gr/ontologies/ccso#Panagiotakis_Spyros"/>
        <hasEmployee rdf:resource="http://xworks.gr/ontologies/ccso#Papadakis_Nikos"/>
        <hasEmployee rdf:resource="http://xworks.gr/ontologies/ccso#Papadourakis_George"/>
        <hasEmployee rdf:resource="http://xworks.gr/ontologies/ccso#Pappa_Pepi"/>
        <hasEmployee rdf:resource="http://xworks.gr/ontologies/ccso#Stratakis_Dimitrios"/>
        <hasEmployee rdf:resource="http://xworks.gr/ontologies/ccso#Triantafyllidis_George"/>
        <hasEmployee rdf:resource="http://xworks.gr/ontologies/ccso#Tsiknakis_Manolis"/>
        <hasEmployee rdf:resource="http://xworks.gr/ontologies/ccso#Vassilakis_Kostas"/>
        <hasEmployee rdf:resource="http://xworks.gr/ontologies/ccso#Vidakis_Nikolaos"/>
        <hasEmployee rdf:resource="http://xworks.gr/ontologies/ccso#Vourkas_Michail"/>
        <hasEmployee rdf:resource="http://xworks.gr/ontologies/ccso#Xezonakis_Ioannis"/>
        <offersCourse rdf:resource="http://xworks.gr/ontologies/ccso#IM101/IM_MSc/IED/STEF/TEIC"/>
        <offersCourse rdf:resource="http://xworks.gr/ontologies/ccso#IM102/IM_MSc/IED/STEF/TEIC"/>
        <offersCourse rdf:resource="http://xworks.gr/ontologies/ccso#IM103/IM_MSc/IED/STEF/TEIC"/>
        <offersCourse rdf:resource="http://xworks.gr/ontologies/ccso#IM104/IM_MSc/IED/STEF/TEIC"/>
        <offersCourse rdf:resource="http://xworks.gr/ontologies/ccso#IM105/IM_MSc/IED/STEF/TEIC"/>
        <offersCourse rdf:resource="http://xworks.gr/ontologies/ccso#IM106/IM_MSc/IED/STEF/TEIC"/>
        <offersCourse rdf:resource="http://xworks.gr/ontologies/ccso#IM107/IM_MSc/IED/STEF/TEIC"/>
        <offersCourse rdf:resource="http://xworks.gr/ontologies/ccso#IM108/IM_MSc/IED/STEF/TEIC"/>
        <offersCourse rdf:resource="http://xworks.gr/ontologies/ccso#IM109/IM_MSc/IED/STEF/TEIC"/>
        <offersCourse rdf:resource="http://xworks.gr/ontologies/ccso#IM201/IM_MSc/IED/STEF/TEIC"/>
        <offersCourse rdf:resource="http://xworks.gr/ontologies/ccso#IM202/IM_MSc/IED/STEF/TEIC"/>
        <offersCourse rdf:resource="http://xworks.gr/ontologies/ccso#IM203/IM_MSc/IED/STEF/TEIC"/>
        <offersCourse rdf:resource="http://xworks.gr/ontologies/ccso#IM204/IM_MSc/IED/STEF/TEIC"/>
        <offersCourse rdf:resource="http://xworks.gr/ontologies/ccso#IM205/IM_MSc/IED/STEF/TEIC"/>
        <offersCourse rdf:resource="http://xworks.gr/ontologies/ccso#IM206/IM_MSc/IED/STEF/TEIC"/>
        <offersCourse rdf:resource="http://xworks.gr/ontologies/ccso#IM207/IM_MSc/IED/STEF/TEIC"/>
        <offersCourse rdf:resource="http://xworks.gr/ontologies/ccso#IM208/IM_MSc/IED/STEF/TEIC"/>
        <offersCourse rdf:resource="http://xworks.gr/ontologies/ccso#IM209/IM_MSc/IED/STEF/TEIC"/>
        <offersCourse rdf:resource="http://xworks.gr/ontologies/ccso#IM210/IM_MSc/IED/STEF/TEIC"/>
        <offersCourse rdf:resource="http://xworks.gr/ontologies/ccso#IM211/IM_MSc/IED/STEF/TEIC"/>
        <offersCourse rdf:resource="http://xworks.gr/ontologies/ccso#TP10K1/IE_BSc/IED/STEF/TEIC"/>
        <offersCourse rdf:resource="http://xworks.gr/ontologies/ccso#TP10K2/IE_BSc/IED/STEF/TEIC"/>
        <offersCourse rdf:resource="http://xworks.gr/ontologies/ccso#TP10K3/IE_BSc/IED/STEF/TEIC"/>
        <offersCourse rdf:resource="http://xworks.gr/ontologies/ccso#TP10K4/IE_BSc/IED/STEF/TEIC"/>
        <offersCourse rdf:resource="http://xworks.gr/ontologies/ccso#TP10K5/IE_BSc/IED/STEF/TEIC"/>
        <offersCourse rdf:resource="http://xworks.gr/ontologies/ccso#TP10K6/IE_BSc/IED/STEF/TEIC"/>
        <offersCourse rdf:resource="http://xworks.gr/ontologies/ccso#TP20K1/IE_BSc/IED/STEF/TEIC"/>
        <offersCourse rdf:resource="http://xworks.gr/ontologies/ccso#TP20K2/IE_BSc/IED/STEF/TEIC"/>
        <offersCourse rdf:resource="http://xworks.gr/ontologies/ccso#TP20K3/IE_BSc/IED/STEF/TEIC"/>
        <offersCourse rdf:resource="http://xworks.gr/ontologies/ccso#TP20K4/IE_BSc/IED/STEF/TEIC"/>
        <offersCourse rdf:resource="http://xworks.gr/ontologies/ccso#TP20K6/IE_BSc/IED/STEF/TEIC"/>
        <offersCourse rdf:resource="http://xworks.gr/ontologies/ccso#TP20K7/IE_BSc/IED/STEF/TEIC"/>
        <offersCourse rdf:resource="http://xworks.gr/ontologies/ccso#TP30K1/IE_BSc/IED/STEF/TEIC"/>
        <offersCourse rdf:resource="http://xworks.gr/ontologies/ccso#TP30K2/IE_BSc/IED/STEF/TEIC"/>
        <offersCourse rdf:resource="http://xworks.gr/ontologies/ccso#TP30K4/IE_BSc/IED/STEF/TEIC"/>
        <offersCourse rdf:resource="http://xworks.gr/ontologies/ccso#TP30K5/IE_BSc/IED/STEF/TEIC"/>
        <offersCourse rdf:resource="http://xworks.gr/ontologies/ccso#TP30K6/IE_BSc/IED/STEF/TEIC"/>
        <offersCourse rdf:resource="http://xworks.gr/ontologies/ccso#TP30K7/IE_BSc/IED/STEF/TEIC"/>
        <offersCourse rdf:resource="http://xworks.gr/ontologies/ccso#TP40K1/IE_BSc/IED/STEF/TEIC"/>
        <offersCourse rdf:resource="http://xworks.gr/ontologies/ccso#TP40K2/IE_BSc/IED/STEF/TEIC"/>
        <offersCourse rdf:resource="http://xworks.gr/ontologies/ccso#TP40K3/IE_BSc/IED/STEF/TEIC"/>
        <offersCourse rdf:resource="http://xworks.gr/ontologies/ccso#TP40K4/IE_BSc/IED/STEF/TEIC"/>
        <offersCourse rdf:resource="http://xworks.gr/ontologies/ccso#TP40K5/IE_BSc/IED/STEF/TEIC"/>
        <offersCourse rdf:resource="http://xworks.gr/ontologies/ccso#TP40K6/IE_BSc/IED/STEF/TEIC"/>
        <offersCourse rdf:resource="http://xworks.gr/ontologies/ccso#TP50D2/IE_BSc/IED/STEF/TEIC"/>
        <offersCourse rdf:resource="http://xworks.gr/ontologies/ccso#TP50D4/IE_BSc/IED/STEF/TEIC"/>
        <offersCourse rdf:resource="http://xworks.gr/ontologies/ccso#TP50D5/IE_BSc/IED/STEF/TEIC"/>
        <offersCourse rdf:resource="http://xworks.gr/ontologies/ccso#TP50D6/IE_BSc/IED/STEF/TEIC"/>
        <offersCourse rdf:resource="http://xworks.gr/ontologies/ccso#TP50L1/IE_BSc/IED/STEF/TEIC"/>
        <offersCourse rdf:resource="http://xworks.gr/ontologies/ccso#TP50L2/IE_BSc/IED/STEF/TEIC"/>
        <offersCourse rdf:resource="http://xworks.gr/ontologies/ccso#TP50L3/IE_BSc/IED/STEF/TEIC"/>
        <offersCourse rdf:resource="http://xworks.gr/ontologies/ccso#TP50L4/IE_BSc/IED/STEF/TEIC"/>
        <offersCourse rdf:resource="http://xworks.gr/ontologies/ccso#TP50L5/IE_BSc/IED/STEF/TEIC"/>
        <offersCourse rdf:resource="http://xworks.gr/ontologies/ccso#TP50Y1/IE_BSc/IED/STEF/TEIC"/>
        <offersCourse rdf:resource="http://xworks.gr/ontologies/ccso#TP50Y2/IE_BSc/IED/STEF/TEIC"/>
        <offersCourse rdf:resource="http://xworks.gr/ontologies/ccso#TP50Y3/IE_BSc/IED/STEF/TEIC"/>
        <offersCourse rdf:resource="http://xworks.gr/ontologies/ccso#TP50Y4/IE_BSc/IED/STEF/TEIC"/>
        <offersCourse rdf:resource="http://xworks.gr/ontologies/ccso#TP50Y5/IE_BSc/IED/STEF/TEIC"/>
        <offersCourse rdf:resource="http://xworks.gr/ontologies/ccso#TP60D1/IE_BSc/IED/STEF/TEIC"/>
        <offersCourse rdf:resource="http://xworks.gr/ontologies/ccso#TP60D2/IE_BSc/IED/STEF/TEIC"/>
        <offersCourse rdf:resource="http://xworks.gr/ontologies/ccso#TP60D3/IE_BSc/IED/STEF/TEIC"/>
        <offersCourse rdf:resource="http://xworks.gr/ontologies/ccso#TP60D4/IE_BSc/IED/STEF/TEIC"/>
        <offersCourse rdf:resource="http://xworks.gr/ontologies/ccso#TP60D5/IE_BSc/IED/STEF/TEIC"/>
        <offersCourse rdf:resource="http://xworks.gr/ontologies/ccso#TP60L1/IE_BSc/IED/STEF/TEIC"/>
        <offersCourse rdf:resource="http://xworks.gr/ontologies/ccso#TP60L2/IE_BSc/IED/STEF/TEIC"/>
        <offersCourse rdf:resource="http://xworks.gr/ontologies/ccso#TP60L3/IE_BSc/IED/STEF/TEIC"/>
        <offersCourse rdf:resource="http://xworks.gr/ontologies/ccso#TP60L4/IE_BSc/IED/STEF/TEIC"/>
        <offersCourse rdf:resource="http://xworks.gr/ontologies/ccso#TP60L5/IE_BSc/IED/STEF/TEIC"/>
        <offersCourse rdf:resource="http://xworks.gr/ontologies/ccso#TP60Y1/IE_BSc/IED/STEF/TEIC"/>
        <offersCourse rdf:resource="http://xworks.gr/ontologies/ccso#TP60Y2/IE_BSc/IED/STEF/TEIC"/>
        <offersCourse rdf:resource="http://xworks.gr/ontologies/ccso#TP60Y6/IE_BSc/IED/STEF/TEIC"/>
        <offersCourse rdf:resource="http://xworks.gr/ontologies/ccso#TP70D1/IE_BSc/IED/STEF/TEIC"/>
        <offersCourse rdf:resource="http://xworks.gr/ontologies/ccso#TP70D2/IE_BSc/IED/STEF/TEIC"/>
        <offersCourse rdf:resource="http://xworks.gr/ontologies/ccso#TP70D3/IE_BSc/IED/STEF/TEIC"/>
        <offersCourse rdf:resource="http://xworks.gr/ontologies/ccso#TP70D5/IE_BSc/IED/STEF/TEIC"/>
        <offersCourse rdf:resource="http://xworks.gr/ontologies/ccso#TP70L1/IE_BSc/IED/STEF/TEIC"/>
        <offersCourse rdf:resource="http://xworks.gr/ontologies/ccso#TP70L2/IE_BSc/IED/STEF/TEIC"/>
        <offersCourse rdf:resource="http://xworks.gr/ontologies/ccso#TP70L3/IE_BSc/IED/STEF/TEIC"/>
        <offersCourse rdf:resource="http://xworks.gr/ontologies/ccso#TP70L4/IE_BSc/IED/STEF/TEIC"/>
        <offersCourse rdf:resource="http://xworks.gr/ontologies/ccso#TP70L5/IE_BSc/IED/STEF/TEIC"/>
        <offersCourse rdf:resource="http://xworks.gr/ontologies/ccso#TP70Y1/IE_BSc/IED/STEF/TEIC"/>
        <offersCourse rdf:resource="http://xworks.gr/ontologies/ccso#TP70Y2/IE_BSc/IED/STEF/TEIC"/>
        <offersCourse rdf:resource="http://xworks.gr/ontologies/ccso#TP70Y6/IE_BSc/IED/STEF/TEIC"/>
        <offersCourse rdf:resource="http://xworks.gr/ontologies/ccso#TP80/IE_BSc/IED/STEF/TEIC"/>
        <providesProgram rdf:resource="http://xworks.gr/ontologies/ccso#BSc_Informatics_Engineering/IE_BSc/IED/STEF/TEIC"/>
        <providesProgram rdf:resource="http://xworks.gr/ontologies/ccso#MSc_Informatics_&amp;_Multimedia/IM_MSc/IED/STEF/TEIC"/>
        <schema:address rdf:datatype="http://www.w3.org/2001/XMLSchema#string">Department of Informatics Engineering
School of Engineering
TEI of Crete
P.O Box 71500
Heraklion, Crete, Greece</schema:address>
        <schema:email rdf:datatype="http://www.w3.org/2001/XMLSchema#anyURI">secretariat@ie.teicrete.gr</schema:email>
        <schema:faxNumber rdf:datatype="http://www.w3.org/2001/XMLSchema#string">2810-379717</schema:faxNumber>
        <schema:identifier rdf:datatype="http://www.w3.org/2001/XMLSchema#string">IED/STEF/TEIC</schema:identifier>
        <schema:legalName rdf:datatype="http://www.w3.org/2001/XMLSchema#string">Department of Informatics Engineering of School of Engineering (STEF) of Technological Educational Institute (TEI) of Crete</schema:legalName>
        <schema:legalName rdf:datatype="http://www.w3.org/2001/XMLSchema#string">Τμήμα Μηχανικών Πληροφορικής της Σχολής Τεχνολογικών Εφαρμογών (ΣΤΕΦ) του Τεχνολογικού Ιδρύματος (ΤΕΙ) Κρήτης</schema:legalName>
        <schema:location rdf:datatype="http://www.w3.org/2001/XMLSchema#string">Estavromenos Heraklion</schema:location>
        <schema:url rdf:datatype="http://www.w3.org/2001/XMLSchema#anyURI">http://www.ie.teicrete.gr</schema:url>
        <eContactInfo rdf:datatype="http://www.w3.org/2001/XMLSchema#anyURI">http://www.ie.teicrete.gr</eContactInfo>
        <eContactInfo rdf:datatype="http://www.w3.org/2001/XMLSchema#anyURI">secretariat@ie.teicrete.gr</eContactInfo>
        <phone rdf:datatype="http://www.w3.org/2001/XMLSchema#string">2810-379716, 2810-379795, 2810-379853</phone>
        <phone rdf:datatype="http://www.w3.org/2001/XMLSchema#string">2810-379717</phone>
        <workPhone rdf:datatype="http://www.w3.org/2001/XMLSchema#string">2810-379716, 2810-379795, 2810-379853</workPhone>
        <rdfs:label xml:lang="en">Department of Informatics Engineering |TEI of Crete</rdfs:label>
        <rdfs:label xml:lang="gr">Τμήμα Μηχανικών Πληροφορικής | ΤΕΙ Κρήτης</rdfs:label>
    </owl:NamedIndividual>
    


    <!-- http://xworks.gr/ontologies/ccso#Discussion -->

    <owl:NamedIndividual rdf:about="http://xworks.gr/ontologies/ccso#Discussion">
        <rdf:type rdf:resource="http://xworks.gr/ontologies/ccso#TeachingEvaluationMethod"/>
        <methodName rdf:datatype="http://www.w3.org/2001/XMLSchema#string">Discussion</methodName>
    </owl:NamedIndividual>
    


    <!-- http://xworks.gr/ontologies/ccso#Earth_Sciences -->

    <owl:NamedIndividual rdf:about="http://xworks.gr/ontologies/ccso#Earth_Sciences">
        <rdf:type rdf:resource="http://xworks.gr/ontologies/ccso#Discipline"/>
        <rdf:type rdf:resource="http://xworks.gr/ontologies/ccso#FieldofStudy"/>
        <fsName rdf:datatype="http://www.w3.org/2001/XMLSchema#string">Earth Sciences</fsName>
    </owl:NamedIndividual>
    


    <!-- http://xworks.gr/ontologies/ccso#Economics -->

    <owl:NamedIndividual rdf:about="http://xworks.gr/ontologies/ccso#Economics">
        <rdf:type rdf:resource="http://xworks.gr/ontologies/ccso#Discipline"/>
        <rdf:type rdf:resource="http://xworks.gr/ontologies/ccso#FieldofStudy"/>
        <fsName rdf:datatype="http://www.w3.org/2001/XMLSchema#string">Economics</fsName>
    </owl:NamedIndividual>
    


    <!-- http://xworks.gr/ontologies/ccso#Faturou_Panagiota -->

    <owl:NamedIndividual rdf:about="http://xworks.gr/ontologies/ccso#Faturou_Panagiota">
        <rdf:type rdf:resource="http://xmlns.com/foaf/0.1/Person"/>
        <rdf:type rdf:resource="http://xworks.gr/ontologies/ccso#AcademicStaff"/>
        <rdf:type rdf:resource="http://xworks.gr/ontologies/ccso#Employee"/>
        <rdf:type rdf:resource="http://xworks.gr/ontologies/ccso#Professor"/>
        <affiliatedWith rdf:resource="http://xworks.gr/ontologies/ccso#Computers_Sciences_Department_of_University_of_Crete"/>
        <affiliatedWith rdf:resource="http://xworks.gr/ontologies/ccso#CS240s1/CS_BSc/CSD/SSE/UoC"/>
        <instructorOf rdf:resource="http://xworks.gr/ontologies/ccso#CS240s1/CS_BSc/CSD/SSE/UoC"/>
        <memberOf rdf:resource="http://xworks.gr/ontologies/ccso#Computers_Sciences_Department_of_University_of_Crete"/>
        <supervisorOf rdf:resource="http://xworks.gr/ontologies/ccso#CS240s1/CS_BSc/CSD/SSE/UoC"/>
        <worksFor rdf:resource="http://xworks.gr/ontologies/ccso#Computers_Sciences_Department_of_University_of_Crete"/>
        <schema:email rdf:datatype="http://www.w3.org/2001/XMLSchema#anyURI">faturu@@csd.uoc.gr</schema:email>
        <foaf:firstName rdf:datatype="http://www.w3.org/2001/XMLSchema#string">Panagiota</foaf:firstName>
        <foaf:lastName rdf:datatype="http://www.w3.org/2001/XMLSchema#string">Faturou</foaf:lastName>
        <eContactInfo rdf:datatype="http://www.w3.org/2001/XMLSchema#anyURI">faturu@@csd.uoc.gr</eContactInfo>
    </owl:NamedIndividual>
    


    <!-- http://xworks.gr/ontologies/ccso#Flyn_Vasilis -->

    <owl:NamedIndividual rdf:about="http://xworks.gr/ontologies/ccso#Flyn_Vasilis">
        <rdf:type rdf:resource="http://xmlns.com/foaf/0.1/Person"/>
        <rdf:type rdf:resource="http://xworks.gr/ontologies/ccso#Student"/>
        <schema:email rdf:datatype="http://www.w3.org/2001/XMLSchema#anyURI">Flyn_Vasilis@mail.gr</schema:email>
        <foaf:firstName rdf:datatype="http://www.w3.org/2001/XMLSchema#string">Flyn</foaf:firstName>
        <foaf:firstName rdf:datatype="http://www.w3.org/2001/XMLSchema#string">Vasilis</foaf:firstName>
        <eContactInfo rdf:datatype="http://www.w3.org/2001/XMLSchema#anyURI">Flyn_Vasilis@mail.gr</eContactInfo>
    </owl:NamedIndividual>
    


    <!-- http://xworks.gr/ontologies/ccso#Fragopoulou_Paraskevi -->

    <owl:NamedIndividual rdf:about="http://xworks.gr/ontologies/ccso#Fragopoulou_Paraskevi">
        <rdf:type rdf:resource="http://xmlns.com/foaf/0.1/Agent"/>
        <rdf:type rdf:resource="http://xmlns.com/foaf/0.1/Person"/>
        <rdf:type rdf:resource="http://xworks.gr/ontologies/ccso#AcademicStaff"/>
        <rdf:type rdf:resource="http://xworks.gr/ontologies/ccso#Employee"/>
        <rdf:type rdf:resource="http://xworks.gr/ontologies/ccso#Professor"/>
        <affiliatedWith rdf:resource="http://xworks.gr/ontologies/ccso#Department_of_Informatics_Engineering_of_TEI_of_Crete"/>
        <affiliatedWith rdf:resource="http://xworks.gr/ontologies/ccso#IM201s1/IM_MSc/IED/STEF/TEI"/>
        <affiliatedWith rdf:resource="http://xworks.gr/ontologies/ccso#IM204s1/IM_MSc/IED/STEF/TEI"/>
        <affiliatedWith rdf:resource="http://xworks.gr/ontologies/ccso#TP30K4s1/IE_BSc/IED/STEF/TEIC"/>
        <affiliatedWith rdf:resource="http://xworks.gr/ontologies/ccso#TP60D1s1/IE_BSc/IED/STEF/TEIC"/>
        <affiliatedWith rdf:resource="http://xworks.gr/ontologies/ccso#TP60D5s1/IE_BSc/IED/STEF/TEIC"/>
        <affiliatedWith rdf:resource="http://xworks.gr/ontologies/ccso#TP70D3s1/IE_BSc/IED/STEF/TEIC"/>
        <instructorOf rdf:resource="http://xworks.gr/ontologies/ccso#IM201s1/IM_MSc/IED/STEF/TEI"/>
        <instructorOf rdf:resource="http://xworks.gr/ontologies/ccso#IM204s1/IM_MSc/IED/STEF/TEI"/>
        <instructorOf rdf:resource="http://xworks.gr/ontologies/ccso#TP30K4s1/IE_BSc/IED/STEF/TEIC"/>
        <instructorOf rdf:resource="http://xworks.gr/ontologies/ccso#TP60D1s1/IE_BSc/IED/STEF/TEIC"/>
        <instructorOf rdf:resource="http://xworks.gr/ontologies/ccso#TP60D5s1/IE_BSc/IED/STEF/TEIC"/>
        <instructorOf rdf:resource="http://xworks.gr/ontologies/ccso#TP70D3s1/IE_BSc/IED/STEF/TEIC"/>
        <memberOf rdf:resource="http://xworks.gr/ontologies/ccso#Department_of_Informatics_Engineering_of_TEI_of_Crete"/>
        <supervisorOf rdf:resource="http://xworks.gr/ontologies/ccso#IM204s1/IM_MSc/IED/STEF/TEI"/>
        <supervisorOf rdf:resource="http://xworks.gr/ontologies/ccso#TP30K4s1/IE_BSc/IED/STEF/TEIC"/>
        <supervisorOf rdf:resource="http://xworks.gr/ontologies/ccso#TP60D1s1/IE_BSc/IED/STEF/TEIC"/>
        <supervisorOf rdf:resource="http://xworks.gr/ontologies/ccso#TP60D5s1/IE_BSc/IED/STEF/TEIC"/>
        <supervisorOf rdf:resource="http://xworks.gr/ontologies/ccso#TP70D3s1/IE_BSc/IED/STEF/TEIC"/>
        <worksFor rdf:resource="http://xworks.gr/ontologies/ccso#Department_of_Informatics_Engineering_of_TEI_of_Crete"/>
        <schema:email rdf:datatype="http://www.w3.org/2001/XMLSchema#anyURI">fragopoulou@ie.teicrete.gr</schema:email>
        <foaf:firstName rdf:datatype="http://www.w3.org/2001/XMLSchema#string">Paraskevi</foaf:firstName>
        <foaf:gender rdf:datatype="http://www.w3.org/2001/XMLSchema#string">Female</foaf:gender>
        <foaf:lastName rdf:datatype="http://www.w3.org/2001/XMLSchema#string">Fragopoulou</foaf:lastName>
        <eContactInfo rdf:datatype="http://www.w3.org/2001/XMLSchema#anyURI">fragopoulou@ie.teicrete.gr</eContactInfo>
    </owl:NamedIndividual>
    


    <!-- http://xworks.gr/ontologies/ccso#Friedman2011OxfordHandbook -->

    <owl:NamedIndividual rdf:about="http://xworks.gr/ontologies/ccso#Friedman2011OxfordHandbook">
        <rdf:type rdf:resource="http://xworks.gr/ontologies/ccso#Resource"/>
        <dc:publisher rdf:datatype="http://www.w3.org/2001/XMLSchema#string">Oxford University Press</dc:publisher>
        <dc:title rdf:datatype="http://www.w3.org/2001/XMLSchema#string">The Oxford handbook of health psychology</dc:title>
        <resourceCitation rdf:datatype="http://www.w3.org/2001/XMLSchema#string">Friedman, H.F. (2011) The Oxford handbook of health psychology.Oxford: Oxford University Press</resourceCitation>
        <rdfs:label xml:lang="en">Friedman (2011) The Oxford handbook of Health Psychology</rdfs:label>
    </owl:NamedIndividual>
    


    <!-- http://xworks.gr/ontologies/ccso#Gakis_George -->

    <owl:NamedIndividual rdf:about="http://xworks.gr/ontologies/ccso#Gakis_George">
        <rdf:type rdf:resource="http://xmlns.com/foaf/0.1/Person"/>
        <rdf:type rdf:resource="http://xworks.gr/ontologies/ccso#Student"/>
        <foaf:firstName rdf:datatype="http://www.w3.org/2001/XMLSchema#string">George</foaf:firstName>
        <foaf:lastName rdf:datatype="http://www.w3.org/2001/XMLSchema#string">Gakis</foaf:lastName>
    </owl:NamedIndividual>
    


    <!-- http://xworks.gr/ontologies/ccso#Georgakopoulos_George -->

    <owl:NamedIndividual rdf:about="http://xworks.gr/ontologies/ccso#Georgakopoulos_George">
        <rdf:type rdf:resource="http://xmlns.com/foaf/0.1/Person"/>
        <rdf:type rdf:resource="http://xworks.gr/ontologies/ccso#AcademicStaff"/>
        <rdf:type rdf:resource="http://xworks.gr/ontologies/ccso#Employee"/>
        <rdf:type rdf:resource="http://xworks.gr/ontologies/ccso#Professor"/>
        <affiliatedWith rdf:resource="http://xworks.gr/ontologies/ccso#Computers_Sciences_Department_of_University_of_Crete"/>
        <affiliatedWith rdf:resource="http://xworks.gr/ontologies/ccso#CS255s1/CS_BSc/CSD/SSE/UoC"/>
        <instructorOf rdf:resource="http://xworks.gr/ontologies/ccso#CS255s1/CS_BSc/CSD/SSE/UoC"/>
        <memberOf rdf:resource="http://xworks.gr/ontologies/ccso#Computers_Sciences_Department_of_University_of_Crete"/>
        <supervisorOf rdf:resource="http://xworks.gr/ontologies/ccso#CS255s1/CS_BSc/CSD/SSE/UoC"/>
        <worksFor rdf:resource="http://xworks.gr/ontologies/ccso#Computers_Sciences_Department_of_University_of_Crete"/>
        <schema:email rdf:datatype="http://www.w3.org/2001/XMLSchema#anyURI">ggeo@csd.uoc.gr</schema:email>
        <foaf:firstName rdf:datatype="http://www.w3.org/2001/XMLSchema#string">George</foaf:firstName>
        <foaf:lastName rdf:datatype="http://www.w3.org/2001/XMLSchema#string">Georgakopoulos</foaf:lastName>
        <eContactInfo rdf:datatype="http://www.w3.org/2001/XMLSchema#anyURI">ggeo@csd.uoc.gr</eContactInfo>
    </owl:NamedIndividual>
    


    <!-- http://xworks.gr/ontologies/ccso#Gramma_Joanna -->

    <owl:NamedIndividual rdf:about="http://xworks.gr/ontologies/ccso#Gramma_Joanna">
        <rdf:type rdf:resource="http://xmlns.com/foaf/0.1/Person"/>
        <rdf:type rdf:resource="http://xworks.gr/ontologies/ccso#Assistant"/>
        <rdf:type rdf:resource="http://xworks.gr/ontologies/ccso#Employee"/>
        <affiliatedWith rdf:resource="http://xworks.gr/ontologies/ccso#CS100s1/CS_BSc/CSD/SSE/UoC"/>
        <affiliatedWith rdf:resource="http://xworks.gr/ontologies/ccso#CS110s1/CS_BSc/CSD/SSE/UoC"/>
        <affiliatedWith rdf:resource="http://xworks.gr/ontologies/ccso#CS118s1/CS_BSc/CSD/SSE/UoC"/>
        <affiliatedWith rdf:resource="http://xworks.gr/ontologies/ccso#CS119s1/CS_BSc/CSD/SSE/UoC"/>
        <affiliatedWith rdf:resource="http://xworks.gr/ontologies/ccso#CS150s1/CS_BSc/CSD/SSE/UoC"/>
        <affiliatedWith rdf:resource="http://xworks.gr/ontologies/ccso#CS180s1/CS_BSc/CSD/SSE/UoC"/>
        <affiliatedWith rdf:resource="http://xworks.gr/ontologies/ccso#CS215s1/CS_BSc/CSD/SSE/UoC"/>
        <affiliatedWith rdf:resource="http://xworks.gr/ontologies/ccso#CS225s1/CS_BSc/CSD/SSE/UoC"/>
        <affiliatedWith rdf:resource="http://xworks.gr/ontologies/ccso#CS252s1/CS_BSc/CSD/SSE/UoC"/>
        <affiliatedWith rdf:resource="http://xworks.gr/ontologies/ccso#CS380s1/CS_BSc/CSD/SSE/UoC"/>
        <assistsInCourse rdf:resource="http://xworks.gr/ontologies/ccso#CS100s1/CS_BSc/CSD/SSE/UoC"/>
        <assistsInCourse rdf:resource="http://xworks.gr/ontologies/ccso#CS110s1/CS_BSc/CSD/SSE/UoC"/>
        <assistsInCourse rdf:resource="http://xworks.gr/ontologies/ccso#CS118s1/CS_BSc/CSD/SSE/UoC"/>
        <assistsInCourse rdf:resource="http://xworks.gr/ontologies/ccso#CS119s1/CS_BSc/CSD/SSE/UoC"/>
        <assistsInCourse rdf:resource="http://xworks.gr/ontologies/ccso#CS150s1/CS_BSc/CSD/SSE/UoC"/>
        <assistsInCourse rdf:resource="http://xworks.gr/ontologies/ccso#CS180s1/CS_BSc/CSD/SSE/UoC"/>
        <assistsInCourse rdf:resource="http://xworks.gr/ontologies/ccso#CS215s1/CS_BSc/CSD/SSE/UoC"/>
        <assistsInCourse rdf:resource="http://xworks.gr/ontologies/ccso#CS225s1/CS_BSc/CSD/SSE/UoC"/>
        <assistsInCourse rdf:resource="http://xworks.gr/ontologies/ccso#CS252s1/CS_BSc/CSD/SSE/UoC"/>
        <assistsInCourse rdf:resource="http://xworks.gr/ontologies/ccso#CS380s1/CS_BSc/CSD/SSE/UoC"/>
        <worksFor rdf:resource="http://xworks.gr/ontologies/ccso#Computers_Sciences_Department_of_University_of_Crete"/>
        <schema:email rdf:datatype="http://www.w3.org/2001/XMLSchema#anyURI">jgramma@mail.gr</schema:email>
        <foaf:firstName rdf:datatype="http://www.w3.org/2001/XMLSchema#string">Joanna</foaf:firstName>
        <foaf:lastName rdf:datatype="http://www.w3.org/2001/XMLSchema#string">Gramma</foaf:lastName>
        <eContactInfo rdf:datatype="http://www.w3.org/2001/XMLSchema#anyURI">jgramma@mail.gr</eContactInfo>
    </owl:NamedIndividual>
    


    <!-- http://xworks.gr/ontologies/ccso#Grammatikakis_Miltiadis -->

    <owl:NamedIndividual rdf:about="http://xworks.gr/ontologies/ccso#Grammatikakis_Miltiadis">
        <rdf:type rdf:resource="http://xmlns.com/foaf/0.1/Person"/>
        <rdf:type rdf:resource="http://xworks.gr/ontologies/ccso#AcademicStaff"/>
        <rdf:type rdf:resource="http://xworks.gr/ontologies/ccso#Employee"/>
        <rdf:type rdf:resource="http://xworks.gr/ontologies/ccso#Professor"/>
        <affiliatedWith rdf:resource="http://xworks.gr/ontologies/ccso#Department_of_Informatics_Engineering_of_TEI_of_Crete"/>
        <affiliatedWith rdf:resource="http://xworks.gr/ontologies/ccso#TP30K1s1/IE_BSc/IED/STEF/TEIC"/>
        <affiliatedWith rdf:resource="http://xworks.gr/ontologies/ccso#TP60Y6s1/IE_BSc/IED/STEF/TEIC"/>
        <affiliatedWith rdf:resource="http://xworks.gr/ontologies/ccso#TP70L3s1/IE_BSc/IED/STEF/TEIC"/>
        <instructorOf rdf:resource="http://xworks.gr/ontologies/ccso#TP30K1s1/IE_BSc/IED/STEF/TEIC"/>
        <instructorOf rdf:resource="http://xworks.gr/ontologies/ccso#TP60Y6s1/IE_BSc/IED/STEF/TEIC"/>
        <instructorOf rdf:resource="http://xworks.gr/ontologies/ccso#TP70L3s1/IE_BSc/IED/STEF/TEIC"/>
        <memberOf rdf:resource="http://xworks.gr/ontologies/ccso#Department_of_Informatics_Engineering_of_TEI_of_Crete"/>
        <supervisorOf rdf:resource="http://xworks.gr/ontologies/ccso#TP30K1s1/IE_BSc/IED/STEF/TEIC"/>
        <supervisorOf rdf:resource="http://xworks.gr/ontologies/ccso#TP60Y6s1/IE_BSc/IED/STEF/TEIC"/>
        <supervisorOf rdf:resource="http://xworks.gr/ontologies/ccso#TP70L3s1/IE_BSc/IED/STEF/TEIC"/>
        <worksFor rdf:resource="http://xworks.gr/ontologies/ccso#Department_of_Informatics_Engineering_of_TEI_of_Crete"/>
        <schema:email rdf:datatype="http://www.w3.org/2001/XMLSchema#anyURI">grammatikakis@ie.teicrete.gr</schema:email>
        <foaf:firstName rdf:datatype="http://www.w3.org/2001/XMLSchema#string">Miltiadis</foaf:firstName>
        <foaf:lastName rdf:datatype="http://www.w3.org/2001/XMLSchema#string">Grammatikakis</foaf:lastName>
        <eContactInfo rdf:datatype="http://www.w3.org/2001/XMLSchema#anyURI">grammatikakis@ie.teicrete.gr</eContactInfo>
    </owl:NamedIndividual>
    


    <!-- http://xworks.gr/ontologies/ccso#Grizakis_Jacob -->

    <owl:NamedIndividual rdf:about="http://xworks.gr/ontologies/ccso#Grizakis_Jacob">
        <rdf:type rdf:resource="http://xmlns.com/foaf/0.1/Person"/>
        <rdf:type rdf:resource="http://xworks.gr/ontologies/ccso#Student"/>
        <foaf:firstName rdf:datatype="http://www.w3.org/2001/XMLSchema#string">Jacob</foaf:firstName>
        <foaf:lastName rdf:datatype="http://www.w3.org/2001/XMLSchema#string">Grizakis</foaf:lastName>
    </owl:NamedIndividual>
    


    <!-- http://xworks.gr/ontologies/ccso#Grizos_Thanos -->

    <owl:NamedIndividual rdf:about="http://xworks.gr/ontologies/ccso#Grizos_Thanos">
        <rdf:type rdf:resource="http://xmlns.com/foaf/0.1/Agent"/>
        <rdf:type rdf:resource="http://xmlns.com/foaf/0.1/Person"/>
        <rdf:type rdf:resource="http://xworks.gr/ontologies/ccso#Student"/>
        <schema:email rdf:datatype="http://www.w3.org/2001/XMLSchema#anyURI">Grizos_Thanos@mail.gr</schema:email>
        <foaf:familyName rdf:datatype="http://www.w3.org/2001/XMLSchema#string">Grizos</foaf:familyName>
        <foaf:firstName rdf:datatype="http://www.w3.org/2001/XMLSchema#string">Thanos</foaf:firstName>
        <foaf:gender rdf:datatype="http://www.w3.org/2001/XMLSchema#string">Male</foaf:gender>
        <foaf:lastName rdf:datatype="http://www.w3.org/2001/XMLSchema#string">Grizos</foaf:lastName>
        <eContactInfo rdf:datatype="http://www.w3.org/2001/XMLSchema#anyURI">Grizos_Thanos@mail.gr</eContactInfo>
    </owl:NamedIndividual>
    


    <!-- http://xworks.gr/ontologies/ccso#Halkas_Gregory -->

    <owl:NamedIndividual rdf:about="http://xworks.gr/ontologies/ccso#Halkas_Gregory">
        <rdf:type rdf:resource="http://xmlns.com/foaf/0.1/Person"/>
        <rdf:type rdf:resource="http://xworks.gr/ontologies/ccso#Student"/>
        <foaf:firstName rdf:datatype="http://www.w3.org/2001/XMLSchema#string">Gregory</foaf:firstName>
        <foaf:lastName rdf:datatype="http://www.w3.org/2001/XMLSchema#string">Halkas</foaf:lastName>
    </owl:NamedIndividual>
    


    <!-- http://xworks.gr/ontologies/ccso#Halkas_Sotiris -->

    <owl:NamedIndividual rdf:about="http://xworks.gr/ontologies/ccso#Halkas_Sotiris">
        <rdf:type rdf:resource="http://xmlns.com/foaf/0.1/Person"/>
        <rdf:type rdf:resource="http://xworks.gr/ontologies/ccso#Student"/>
        <foaf:firstName rdf:datatype="http://www.w3.org/2001/XMLSchema#string">Sotiris</foaf:firstName>
        <foaf:lastName rdf:datatype="http://www.w3.org/2001/XMLSchema#string">Halkas</foaf:lastName>
    </owl:NamedIndividual>
    


    <!-- http://xworks.gr/ontologies/ccso#Hatzivasilis2014ReasoningSystem -->

    <owl:NamedIndividual rdf:about="http://xworks.gr/ontologies/ccso#Hatzivasilis2014ReasoningSystem">
        <rdf:type rdf:resource="http://xworks.gr/ontologies/ccso#Resource"/>
        <dc:creator rdf:resource="http://xworks.gr/ontologies/ccso#Manifavas_Harry"/>
        <dc:creator rdf:resource="http://xworks.gr/ontologies/ccso#Papadakis_Nikos"/>
        <dc:date rdf:datatype="http://www.w3.org/2001/XMLSchema#date">2014</dc:date>
        <dc:date rdf:datatype="internal:anonymous-constants">2014</dc:date>
        <dc:publisher rdf:datatype="http://www.w3.org/2001/XMLSchema#string">IEEE</dc:publisher>
        <dc:source rdf:datatype="http://www.w3.org/2001/XMLSchema#string">6th International Conference on New Technologies, Mobility and Security (NTMS), 2014  (pp. 1-4). IEEE</dc:source>
        <dc:subject rdf:datatype="http://www.w3.org/2001/XMLSchema#string">Reasoning</dc:subject>
        <dc:title rdf:datatype="http://www.w3.org/2001/XMLSchema#string">A Reasoning System for composition verification and security validation</dc:title>
        <dc:type rdf:datatype="http://www.w3.org/2001/XMLSchema#string">Conference</dc:type>
        <dates rdf:datatype="internal:anonymous-constants">2014</dates>
        <resourceCitation rdf:datatype="http://www.w3.org/2001/XMLSchema#string">Hatzivasilis, G., Papaefstathiou, I., Manifavas, C., &amp; Papadakis, N. (2014, March). A reasoning system for composition verification and security validation. In New Technologies, Mobility and Security (NTMS), 2014 6th International Conference on (pp. 1-4). IEEE.</resourceCitation>
        <rdfs:label xml:lang="en">Hatzivasilis,Papaefstathiou,Manifavas,Papadakis (2014) A Reasoning System for composition verification and security validation</rdfs:label>
    </owl:NamedIndividual>
    


    <!-- http://xworks.gr/ontologies/ccso#High_School_Diploma -->

    <owl:NamedIndividual rdf:about="http://xworks.gr/ontologies/ccso#High_School_Diploma">
        <rdf:type rdf:resource="http://xworks.gr/ontologies/ccso#ProgramofStudy"/>
        <rdf:type rdf:resource="http://xworks.gr/ontologies/ccso#SchoolDiploma"/>
        <rdfs:label xml:lang="en">High School Diploma</rdfs:label>
        <rdfs:label xml:lang="gr">Απολυτήριο Λυκείου</rdfs:label>
    </owl:NamedIndividual>
    


    <!-- http://xworks.gr/ontologies/ccso#Hionis_John -->

    <owl:NamedIndividual rdf:about="http://xworks.gr/ontologies/ccso#Hionis_John">
        <rdf:type rdf:resource="http://xmlns.com/foaf/0.1/Agent"/>
        <rdf:type rdf:resource="http://xmlns.com/foaf/0.1/Person"/>
        <rdf:type rdf:resource="http://xworks.gr/ontologies/ccso#PostgraduateStudent"/>
        <rdf:type rdf:resource="http://xworks.gr/ontologies/ccso#Student"/>
        <affiliatedWith rdf:resource="http://xworks.gr/ontologies/ccso#Computers_Sciences_Department_of_University_of_Crete"/>
        <affiliatedWith rdf:resource="http://xworks.gr/ontologies/ccso#BSc_Computer_Science/CS_BSc/CSD/SSE/UoC"/>
        <affiliatedWith rdf:resource="http://xworks.gr/ontologies/ccso#IM101/IM_MSc/IED/STEF/TEIC"/>
        <affiliatedWith rdf:resource="http://xworks.gr/ontologies/ccso#IM104/IM_MSc/IED/STEF/TEIC"/>
        <affiliatedWith rdf:resource="http://xworks.gr/ontologies/ccso#IM105/IM_MSc/IED/STEF/TEIC"/>
        <affiliatedWith rdf:resource="http://xworks.gr/ontologies/ccso#IM107/IM_MSc/IED/STEF/TEIC"/>
        <affiliatedWith rdf:resource="http://xworks.gr/ontologies/ccso#IM201/IM_MSc/IED/STEF/TEIC"/>
        <affiliatedWith rdf:resource="http://xworks.gr/ontologies/ccso#IM207/IM_MSc/IED/STEF/TEIC"/>
        <affiliatedWith rdf:resource="http://xworks.gr/ontologies/ccso#IM208/IM_MSc/IED/STEF/TEIC"/>
        <affiliatedWith rdf:resource="http://xworks.gr/ontologies/ccso#IM209/IM_MSc/IED/STEF/TEIC"/>
        <affiliatedWith rdf:resource="http://xworks.gr/ontologies/ccso#IM210/IM_MSc/IED/STEF/TEIC"/>
        <affiliatedWith rdf:resource="http://xworks.gr/ontologies/ccso#MSc_Informatics_&amp;_Multimedia/IM_MSc/IED/STEF/TEIC"/>
        <alumnusOf rdf:resource="http://xworks.gr/ontologies/ccso#Computers_Sciences_Department_of_University_of_Crete"/>
        <attendsCourse rdf:resource="http://xworks.gr/ontologies/ccso#IM201/IM_MSc/IED/STEF/TEIC"/>
        <attendsCourse rdf:resource="http://xworks.gr/ontologies/ccso#IM207/IM_MSc/IED/STEF/TEIC"/>
        <attendsCourse rdf:resource="http://xworks.gr/ontologies/ccso#IM208/IM_MSc/IED/STEF/TEIC"/>
        <attendsCourse rdf:resource="http://xworks.gr/ontologies/ccso#IM209/IM_MSc/IED/STEF/TEIC"/>
        <enrolledIn rdf:resource="http://xworks.gr/ontologies/ccso#MSc_Informatics_&amp;_Multimedia/IM_MSc/IED/STEF/TEIC"/>
        <hasCompleted rdf:resource="http://xworks.gr/ontologies/ccso#IM101/IM_MSc/IED/STEF/TEIC"/>
        <hasCompleted rdf:resource="http://xworks.gr/ontologies/ccso#IM104/IM_MSc/IED/STEF/TEIC"/>
        <hasCompleted rdf:resource="http://xworks.gr/ontologies/ccso#IM105/IM_MSc/IED/STEF/TEIC"/>
        <hasCompleted rdf:resource="http://xworks.gr/ontologies/ccso#IM107/IM_MSc/IED/STEF/TEIC"/>
        <hasCompleted rdf:resource="http://xworks.gr/ontologies/ccso#IM210/IM_MSc/IED/STEF/TEIC"/>
        <hasDegree rdf:resource="http://xworks.gr/ontologies/ccso#BSc_Computer_Science/CS_BSc/CSD/SSE/UoC"/>
        <schema:email rdf:datatype="http://www.w3.org/2001/XMLSchema#anyURI">Hionis_John@ie.teicrete.gr</schema:email>
        <foaf:firstName rdf:datatype="http://www.w3.org/2001/XMLSchema#string">John</foaf:firstName>
        <foaf:gender rdf:datatype="http://www.w3.org/2001/XMLSchema#string">Male</foaf:gender>
        <foaf:lastName rdf:datatype="http://www.w3.org/2001/XMLSchema#string">Hionis</foaf:lastName>
        <eContactInfo rdf:datatype="http://www.w3.org/2001/XMLSchema#anyURI">Hionis_John@ie.teicrete.gr</eContactInfo>
    </owl:NamedIndividual>
    


    <!-- http://xworks.gr/ontologies/ccso#Hogg2010SocialPsychology -->

    <owl:NamedIndividual rdf:about="http://xworks.gr/ontologies/ccso#Hogg2010SocialPsychology">
        <rdf:type rdf:resource="http://xworks.gr/ontologies/ccso#Resource"/>
        <dc:publisher rdf:datatype="http://www.w3.org/2001/XMLSchema#string">Αθήνα: Gutenberg</dc:publisher>
        <dc:title rdf:datatype="http://www.w3.org/2001/XMLSchema#string">Κοινωνική Ψυχολογία</dc:title>
        <resourceCitation rdf:datatype="http://www.w3.org/2001/XMLSchema#string">Hogg, M.A. &amp; Vaughan, G.M. (2010) Κοινωνική Ψυχολογία. Αθήνα:Gutenberg</resourceCitation>
        <rdfs:label xml:lang="en">Hogg, Vaughan (2010) Social Psychology</rdfs:label>
    </owl:NamedIndividual>
    


    <!-- http://xworks.gr/ontologies/ccso#Homework -->

    <owl:NamedIndividual rdf:about="http://xworks.gr/ontologies/ccso#Homework">
        <rdf:type rdf:resource="http://xworks.gr/ontologies/ccso#TeachingEvaluationMethod"/>
        <methodName rdf:datatype="http://www.w3.org/2001/XMLSchema#string">Homework</methodName>
    </owl:NamedIndividual>
    


    <!-- http://xworks.gr/ontologies/ccso#Human_Geography -->

    <owl:NamedIndividual rdf:about="http://xworks.gr/ontologies/ccso#Human_Geography">
        <rdf:type rdf:resource="http://xworks.gr/ontologies/ccso#Discipline"/>
        <rdf:type rdf:resource="http://xworks.gr/ontologies/ccso#FieldofStudy"/>
        <fsName rdf:datatype="http://www.w3.org/2001/XMLSchema#string">Human Geography</fsName>
    </owl:NamedIndividual>
    


    <!-- http://xworks.gr/ontologies/ccso#Kafetsios_Konstantinos -->

    <owl:NamedIndividual rdf:about="http://xworks.gr/ontologies/ccso#Kafetsios_Konstantinos">
        <rdf:type rdf:resource="http://xmlns.com/foaf/0.1/Agent"/>
        <rdf:type rdf:resource="http://xmlns.com/foaf/0.1/Person"/>
        <rdf:type rdf:resource="http://xworks.gr/ontologies/ccso#AcademicStaff"/>
        <rdf:type rdf:resource="http://xworks.gr/ontologies/ccso#Employee"/>
        <rdf:type rdf:resource="http://xworks.gr/ontologies/ccso#Professor"/>
        <affiliatedWith rdf:resource="http://xworks.gr/ontologies/ccso#Psychology_Department_of_University_of_Crete"/>
        <affiliatedWith rdf:resource="http://xworks.gr/ontologies/ccso#PSY1501_s2017-18-L01/PSY_BSc/SoC/Uoc"/>
        <affiliatedWith rdf:resource="http://xworks.gr/ontologies/ccso#PSY1501s1/PSY_BSc/SoC/Uoc"/>
        <affiliatedWith rdf:resource="http://xworks.gr/ontologies/ccso#PSY3601s1/PSY_BSc/SoC/Uoc"/>
        <instructorOf rdf:resource="http://xworks.gr/ontologies/ccso#PSY1501s1/PSY_BSc/SoC/Uoc"/>
        <instructorOf rdf:resource="http://xworks.gr/ontologies/ccso#PSY3601s1/PSY_BSc/SoC/Uoc"/>
        <memberOf rdf:resource="http://xworks.gr/ontologies/ccso#Psychology_Department_of_University_of_Crete"/>
        <supervisorOf rdf:resource="http://xworks.gr/ontologies/ccso#PSY1501s1/PSY_BSc/SoC/Uoc"/>
        <teachesIn rdf:resource="http://xworks.gr/ontologies/ccso#PSY1501_s2017-18-L01/PSY_BSc/SoC/Uoc"/>
        <worksFor rdf:resource="http://xworks.gr/ontologies/ccso#Psychology_Department_of_University_of_Crete"/>
        <schema:email rdf:datatype="http://www.w3.org/2001/XMLSchema#anyURI">kaffetsios@psy.soc.uoc.gr</schema:email>
        <foaf:firstName rdf:datatype="http://www.w3.org/2001/XMLSchema#string">Konstantinos</foaf:firstName>
        <foaf:gender rdf:datatype="http://www.w3.org/2001/XMLSchema#string">Male</foaf:gender>
        <foaf:lastName rdf:datatype="http://www.w3.org/2001/XMLSchema#string">Kafetsios</foaf:lastName>
        <foaf:title rdf:datatype="http://www.w3.org/2001/XMLSchema#string">Dr</foaf:title>
        <eContactInfo rdf:datatype="http://www.w3.org/2001/XMLSchema#anyURI">kaffetsios@psy.soc.uoc.gr</eContactInfo>
    </owl:NamedIndividual>
    


    <!-- http://xworks.gr/ontologies/ccso#Kalogiannakis2009AdultEducationLifelongLearning -->

    <owl:NamedIndividual rdf:about="http://xworks.gr/ontologies/ccso#Kalogiannakis2009AdultEducationLifelongLearning">
        <rdf:type rdf:resource="http://xworks.gr/ontologies/ccso#Resource"/>
        <dc:creator rdf:resource="http://xworks.gr/ontologies/ccso#Kalogiannakis_Michail"/>
        <dc:creator rdf:resource="http://xworks.gr/ontologies/ccso#Vassilakis_Kostas"/>
        <dc:date rdf:datatype="http://www.w3.org/2001/XMLSchema#date">2009</dc:date>
        <dc:date rdf:datatype="internal:anonymous-constants">2009</dc:date>
        <dc:source rdf:datatype="http://www.w3.org/2001/XMLSchema#string">International Journal of Advanced Corporate Learning (iJAC) 2, no. 4 (2009): 15-20</dc:source>
        <dc:subject rdf:datatype="http://www.w3.org/2001/XMLSchema#string">Adult Education</dc:subject>
        <dc:subject rdf:datatype="http://www.w3.org/2001/XMLSchema#string">Lifelong Learning</dc:subject>
        <dc:title rdf:datatype="http://www.w3.org/2001/XMLSchema#string">Adult Education and Lifelong Learning. The case of GSAE (General Secretary for Adult Education) in Greece</dc:title>
        <dc:type rdf:datatype="http://www.w3.org/2001/XMLSchema#string">Article</dc:type>
        <dates rdf:datatype="internal:anonymous-constants">2009</dates>
        <rdfs:label xml:lang="en">Kalogiannakis,Vassilakis,Alafodimos,Papadakis,Papachristos,Zafeiri (2009) Adult Education and Lifelong Learning. The case of GSAE</rdfs:label>
    </owl:NamedIndividual>
    


    <!-- http://xworks.gr/ontologies/ccso#Kalogiannakis_Michail -->

    <owl:NamedIndividual rdf:about="http://xworks.gr/ontologies/ccso#Kalogiannakis_Michail">
        <rdf:type rdf:resource="http://www.w3.org/2000/10/swap/pim/contact#Person"/>
        <rdf:type rdf:resource="http://xmlns.com/foaf/0.1/Agent"/>
        <rdf:type rdf:resource="http://xmlns.com/foaf/0.1/Person"/>
        <rdf:type rdf:resource="http://xworks.gr/ontologies/ccso#AcademicStaff"/>
        <rdf:type rdf:resource="http://xworks.gr/ontologies/ccso#Employee"/>
        <rdf:type rdf:resource="http://xworks.gr/ontologies/ccso#Professor"/>
        <affiliatedWith rdf:resource="http://xworks.gr/ontologies/ccso#Computers_Sciences_Department_of_University_of_Crete"/>
        <affiliatedWith rdf:resource="http://xworks.gr/ontologies/ccso#Department_of_Informatics_Engineering_of_TEI_of_Crete"/>
        <affiliatedWith rdf:resource="http://xworks.gr/ontologies/ccso#BSc_Computer_Science/CS_BSc/CSD/SSE/UoC"/>
        <affiliatedWith rdf:resource="http://xworks.gr/ontologies/ccso#CS118s1/CS_BSc/CSD/SSE/UoC"/>
        <affiliatedWith rdf:resource="http://xworks.gr/ontologies/ccso#CS150s1/CS_BSc/CSD/SSE/UoC"/>
        <affiliatedWith rdf:resource="http://xworks.gr/ontologies/ccso#IM106s1/IM_MSc/IED/STEF/TEI"/>
        <affiliatedWith rdf:resource="http://xworks.gr/ontologies/ccso#IM209s1/IM_MSc/IED/STEF/TEI"/>
        <affiliatedWith rdf:resource="http://xworks.gr/ontologies/ccso#MSc_Computer_Science_and_Engineering/CSE_MSc/CSD/SSE/UoC"/>
        <affiliatedWith rdf:resource="http://xworks.gr/ontologies/ccso#PhD_Computer_Science_and_Engineering/CSE_PhD/CSD/SSE/UoC"/>
        <affiliatedWith rdf:resource="http://xworks.gr/ontologies/ccso#TP10K5s1/IE_BSc/IED/STEF/TEIC"/>
        <affiliatedWith rdf:resource="http://xworks.gr/ontologies/ccso#TP20K7s1/IE_BSc/IED/STEF/TEIC"/>
        <alumnusOf rdf:resource="http://xworks.gr/ontologies/ccso#Computers_Sciences_Department_of_University_of_Crete"/>
        <hasDegree rdf:resource="http://xworks.gr/ontologies/ccso#BSc_Computer_Science/CS_BSc/CSD/SSE/UoC"/>
        <hasDegree rdf:resource="http://xworks.gr/ontologies/ccso#MSc_Computer_Science_and_Engineering/CSE_MSc/CSD/SSE/UoC"/>
        <hasDegree rdf:resource="http://xworks.gr/ontologies/ccso#PhD_Computer_Science_and_Engineering/CSE_PhD/CSD/SSE/UoC"/>
        <hasPublication rdf:resource="http://xworks.gr/ontologies/ccso#Kalogiannakis2009AdultEducationLifelongLearning"/>
        <hasPublication rdf:resource="http://xworks.gr/ontologies/ccso#Papachristou2010EducationalModel"/>
        <hasPublication rdf:resource="http://xworks.gr/ontologies/ccso#Papadakis2014NoviceProgrammingEnvironments"/>
        <hasPublication rdf:resource="http://xworks.gr/ontologies/ccso#Papadakis2017MobileEducationalApplications"/>
        <hasPublication rdf:resource="http://xworks.gr/ontologies/ccso#Vassilakis2005AsynchronousTeleTeaching"/>
        <hasPublication rdf:resource="http://xworks.gr/ontologies/ccso#Kalogiannakis(2010)TrainingICT"/>
        <instructorOf rdf:resource="http://xworks.gr/ontologies/ccso#CS118s1/CS_BSc/CSD/SSE/UoC"/>
        <instructorOf rdf:resource="http://xworks.gr/ontologies/ccso#CS150s1/CS_BSc/CSD/SSE/UoC"/>
        <instructorOf rdf:resource="http://xworks.gr/ontologies/ccso#IM106s1/IM_MSc/IED/STEF/TEI"/>
        <instructorOf rdf:resource="http://xworks.gr/ontologies/ccso#IM209s1/IM_MSc/IED/STEF/TEI"/>
        <instructorOf rdf:resource="http://xworks.gr/ontologies/ccso#TP10K5s1/IE_BSc/IED/STEF/TEIC"/>
        <instructorOf rdf:resource="http://xworks.gr/ontologies/ccso#TP20K7s1/IE_BSc/IED/STEF/TEIC"/>
        <memberOf rdf:resource="http://xworks.gr/ontologies/ccso#Computers_Sciences_Department_of_University_of_Crete"/>
        <memberOf rdf:resource="http://xworks.gr/ontologies/ccso#Department_of_Informatics_Engineering_of_TEI_of_Crete"/>
        <supervisorOf rdf:resource="http://xworks.gr/ontologies/ccso#IM106s1/IM_MSc/IED/STEF/TEI"/>
        <supervisorOf rdf:resource="http://xworks.gr/ontologies/ccso#TP10K5s1/IE_BSc/IED/STEF/TEIC"/>
        <supervisorOf rdf:resource="http://xworks.gr/ontologies/ccso#TP20K7s1/IE_BSc/IED/STEF/TEIC"/>
        <worksFor rdf:resource="http://xworks.gr/ontologies/ccso#Computers_Sciences_Department_of_University_of_Crete"/>
        <worksFor rdf:resource="http://xworks.gr/ontologies/ccso#Department_of_Informatics_Engineering_of_TEI_of_Crete"/>
        <schema:email rdf:datatype="http://www.w3.org/2001/XMLSchema#anyURI">kalogiannakis@ie.teicrete.gr</schema:email>
        <foaf:firstName rdf:datatype="http://www.w3.org/2001/XMLSchema#string">Michail</foaf:firstName>
        <foaf:gender rdf:datatype="http://www.w3.org/2001/XMLSchema#string">Male</foaf:gender>
        <foaf:lastName rdf:datatype="http://www.w3.org/2001/XMLSchema#string">Kalogiannakis</foaf:lastName>
        <eContactInfo rdf:datatype="http://www.w3.org/2001/XMLSchema#anyURI">kalogiannakis@ie.teicrete.gr</eContactInfo>
        <label rdf:datatype="http://www.w3.org/2001/XMLSchema#string">Dr</label>
        <staffPosition rdf:datatype="http://www.w3.org/2001/XMLSchema#string">Lecturer</staffPosition>
        <rdfs:label xml:lang="en">Kalogiannakis Michail</rdfs:label>
    </owl:NamedIndividual>
    


    <!-- http://xworks.gr/ontologies/ccso#Karagiannakis_Dimitrios -->

    <owl:NamedIndividual rdf:about="http://xworks.gr/ontologies/ccso#Karagiannakis_Dimitrios">
        <rdf:type rdf:resource="http://xmlns.com/foaf/0.1/Person"/>
        <rdf:type rdf:resource="http://xworks.gr/ontologies/ccso#AcademicStaff"/>
        <rdf:type rdf:resource="http://xworks.gr/ontologies/ccso#Employee"/>
        <rdf:type rdf:resource="http://xworks.gr/ontologies/ccso#Professor"/>
        <affiliatedWith rdf:resource="http://xworks.gr/ontologies/ccso#Department_of_Informatics_Engineering_of_TEI_of_Crete"/>
        <affiliatedWith rdf:resource="http://xworks.gr/ontologies/ccso#IM109s1/IM_MSc/IED/STEF/TEI"/>
        <affiliatedWith rdf:resource="http://xworks.gr/ontologies/ccso#TP30K5s1/IE_BSc/IED/STEF/TEIC"/>
        <affiliatedWith rdf:resource="http://xworks.gr/ontologies/ccso#TP40K5s1/IE_BSc/IED/STEF/TEIC"/>
        <instructorOf rdf:resource="http://xworks.gr/ontologies/ccso#IM109s1/IM_MSc/IED/STEF/TEI"/>
        <instructorOf rdf:resource="http://xworks.gr/ontologies/ccso#TP30K5s1/IE_BSc/IED/STEF/TEIC"/>
        <instructorOf rdf:resource="http://xworks.gr/ontologies/ccso#TP40K5s1/IE_BSc/IED/STEF/TEIC"/>
        <memberOf rdf:resource="http://xworks.gr/ontologies/ccso#Department_of_Informatics_Engineering_of_TEI_of_Crete"/>
        <supervisorOf rdf:resource="http://xworks.gr/ontologies/ccso#IM109s1/IM_MSc/IED/STEF/TEI"/>
        <supervisorOf rdf:resource="http://xworks.gr/ontologies/ccso#TP30K5s1/IE_BSc/IED/STEF/TEIC"/>
        <supervisorOf rdf:resource="http://xworks.gr/ontologies/ccso#TP40K5s1/IE_BSc/IED/STEF/TEIC"/>
        <worksFor rdf:resource="http://xworks.gr/ontologies/ccso#Department_of_Informatics_Engineering_of_TEI_of_Crete"/>
        <schema:email rdf:datatype="http://www.w3.org/2001/XMLSchema#anyURI">karagiannakis@ie.teicrete.gr</schema:email>
        <foaf:firstName rdf:datatype="http://www.w3.org/2001/XMLSchema#string">Dimitrios</foaf:firstName>
        <foaf:lastName rdf:datatype="http://www.w3.org/2001/XMLSchema#string">Karagiannakis</foaf:lastName>
        <eContactInfo rdf:datatype="http://www.w3.org/2001/XMLSchema#anyURI">karagiannakis@ie.teicrete.gr</eContactInfo>
    </owl:NamedIndividual>
    


    <!-- http://xworks.gr/ontologies/ccso#Katevenis_Manolis -->

    <owl:NamedIndividual rdf:about="http://xworks.gr/ontologies/ccso#Katevenis_Manolis">
        <rdf:type rdf:resource="http://xmlns.com/foaf/0.1/Person"/>
        <rdf:type rdf:resource="http://xworks.gr/ontologies/ccso#AcademicStaff"/>
        <rdf:type rdf:resource="http://xworks.gr/ontologies/ccso#Employee"/>
        <rdf:type rdf:resource="http://xworks.gr/ontologies/ccso#Professor"/>
        <affiliatedWith rdf:resource="http://xworks.gr/ontologies/ccso#Computers_Sciences_Department_of_University_of_Crete"/>
        <affiliatedWith rdf:resource="http://xworks.gr/ontologies/ccso#CS120s1/CS_BSc/CSD/SSE/UoC"/>
        <affiliatedWith rdf:resource="http://xworks.gr/ontologies/ccso#CS225s1/CS_BSc/CSD/SSE/UoC"/>
        <instructorOf rdf:resource="http://xworks.gr/ontologies/ccso#CS120s1/CS_BSc/CSD/SSE/UoC"/>
        <instructorOf rdf:resource="http://xworks.gr/ontologies/ccso#CS225s1/CS_BSc/CSD/SSE/UoC"/>
        <memberOf rdf:resource="http://xworks.gr/ontologies/ccso#Computers_Sciences_Department_of_University_of_Crete"/>
        <supervisorOf rdf:resource="http://xworks.gr/ontologies/ccso#CS120s1/CS_BSc/CSD/SSE/UoC"/>
        <supervisorOf rdf:resource="http://xworks.gr/ontologies/ccso#CS225s1/CS_BSc/CSD/SSE/UoC"/>
        <worksFor rdf:resource="http://xworks.gr/ontologies/ccso#Computers_Sciences_Department_of_University_of_Crete"/>
        <schema:email rdf:datatype="http://www.w3.org/2001/XMLSchema#anyURI">kateveni@csd.uoc.gr</schema:email>
        <foaf:firstName rdf:datatype="http://www.w3.org/2001/XMLSchema#string">Manolis</foaf:firstName>
        <foaf:lastName rdf:datatype="http://www.w3.org/2001/XMLSchema#string">Katevenis</foaf:lastName>
        <eContactInfo rdf:datatype="http://www.w3.org/2001/XMLSchema#anyURI">kateveni@csd.uoc.gr</eContactInfo>
    </owl:NamedIndividual>
    


    <!-- http://xworks.gr/ontologies/ccso#Katis_Evangelos -->

    <owl:NamedIndividual rdf:about="http://xworks.gr/ontologies/ccso#Katis_Evangelos">
        <rdf:type rdf:resource="http://xmlns.com/foaf/0.1/Agent"/>
        <rdf:type rdf:resource="http://xmlns.com/foaf/0.1/Person"/>
        <rdf:type rdf:resource="http://xworks.gr/ontologies/ccso#Assistant"/>
        <rdf:type rdf:resource="http://xworks.gr/ontologies/ccso#Employee"/>
        <affiliatedWith rdf:resource="http://xworks.gr/ontologies/ccso#IM102s1/IM_MSc/IED/STEF/TEI"/>
        <affiliatedWith rdf:resource="http://xworks.gr/ontologies/ccso#IM105s1/IM_MSc/IED/STEF/TEI"/>
        <affiliatedWith rdf:resource="http://xworks.gr/ontologies/ccso#IM201s1/IM_MSc/IED/STEF/TEI"/>
        <affiliatedWith rdf:resource="http://xworks.gr/ontologies/ccso#IM209s1/IM_MSc/IED/STEF/TEI"/>
        <assistsInCourse rdf:resource="http://xworks.gr/ontologies/ccso#IM102s1/IM_MSc/IED/STEF/TEI"/>
        <assistsInCourse rdf:resource="http://xworks.gr/ontologies/ccso#IM105s1/IM_MSc/IED/STEF/TEI"/>
        <assistsInCourse rdf:resource="http://xworks.gr/ontologies/ccso#IM201s1/IM_MSc/IED/STEF/TEI"/>
        <assistsInCourse rdf:resource="http://xworks.gr/ontologies/ccso#IM209s1/IM_MSc/IED/STEF/TEI"/>
        <worksFor rdf:resource="http://xworks.gr/ontologies/ccso#Department_of_Informatics_Engineering_of_TEI_of_Crete"/>
        <schema:email rdf:datatype="http://www.w3.org/2001/XMLSchema#anyURI">evskg@mail.gr</schema:email>
        <foaf:firstName rdf:datatype="http://www.w3.org/2001/XMLSchema#anyURI">Evangelos</foaf:firstName>
        <foaf:gender rdf:datatype="http://www.w3.org/2001/XMLSchema#string">Male</foaf:gender>
        <foaf:lastName rdf:datatype="http://www.w3.org/2001/XMLSchema#string">Katis</foaf:lastName>
        <eContactInfo rdf:datatype="http://www.w3.org/2001/XMLSchema#anyURI">evskg@cs.teicrete.gr</eContactInfo>
        <eContactInfo rdf:datatype="http://www.w3.org/2001/XMLSchema#anyURI">evskg@mail.gr</eContactInfo>
        <workEmail rdf:datatype="http://www.w3.org/2001/XMLSchema#anyURI">evskg@cs.teicrete.gr</workEmail>
    </owl:NamedIndividual>
    


    <!-- http://xworks.gr/ontologies/ccso#Kekili_Souzan -->

    <owl:NamedIndividual rdf:about="http://xworks.gr/ontologies/ccso#Kekili_Souzan">
        <rdf:type rdf:resource="http://xmlns.com/foaf/0.1/Person"/>
        <rdf:type rdf:resource="http://xworks.gr/ontologies/ccso#Student"/>
        <rdf:type rdf:resource="http://xworks.gr/ontologies/ccso#UndergraduateStudent"/>
        <affiliatedWith rdf:resource="http://xworks.gr/ontologies/ccso#BSc_Psychology/PSY_BSc/SoC/UoC"/>
        <affiliatedWith rdf:resource="http://xworks.gr/ontologies/ccso#PSY1501/PSY_BSc/SoC/Uoc"/>
        <attendsCourse rdf:resource="http://xworks.gr/ontologies/ccso#PSY1501/PSY_BSc/SoC/Uoc"/>
        <enrolledIn rdf:resource="http://xworks.gr/ontologies/ccso#BSc_Psychology/PSY_BSc/SoC/UoC"/>
        <schema:email rdf:datatype="http://www.w3.org/2001/XMLSchema#anyURI">Kekili_Souzan@psy.uoc.gr</schema:email>
        <foaf:firstName rdf:datatype="http://www.w3.org/2001/XMLSchema#string">Souzan</foaf:firstName>
        <foaf:lastName rdf:datatype="http://www.w3.org/2001/XMLSchema#string">Kekili</foaf:lastName>
        <eContactInfo rdf:datatype="http://www.w3.org/2001/XMLSchema#anyURI">Kekili_Souzan@psy.uoc.gr</eContactInfo>
    </owl:NamedIndividual>
    


    <!-- http://xworks.gr/ontologies/ccso#Kokkinos_Heraklis -->

    <owl:NamedIndividual rdf:about="http://xworks.gr/ontologies/ccso#Kokkinos_Heraklis">
        <rdf:type rdf:resource="http://xmlns.com/foaf/0.1/Agent"/>
        <rdf:type rdf:resource="http://xmlns.com/foaf/0.1/Person"/>
        <rdf:type rdf:resource="http://xworks.gr/ontologies/ccso#PostgraduateStudent"/>
        <rdf:type rdf:resource="http://xworks.gr/ontologies/ccso#Student"/>
        <affiliatedWith rdf:resource="http://xworks.gr/ontologies/ccso#Department_of_Informatics_Engineering_of_TEI_of_Crete"/>
        <affiliatedWith rdf:resource="http://xworks.gr/ontologies/ccso#BSc_Informatics_Engineering/IE_BSc/IED/STEF/TEIC"/>
        <affiliatedWith rdf:resource="http://xworks.gr/ontologies/ccso#IM101/IM_MSc/IED/STEF/TEIC"/>
        <affiliatedWith rdf:resource="http://xworks.gr/ontologies/ccso#IM102/IM_MSc/IED/STEF/TEIC"/>
        <affiliatedWith rdf:resource="http://xworks.gr/ontologies/ccso#IM105/IM_MSc/IED/STEF/TEIC"/>
        <affiliatedWith rdf:resource="http://xworks.gr/ontologies/ccso#IM107/IM_MSc/IED/STEF/TEIC"/>
        <affiliatedWith rdf:resource="http://xworks.gr/ontologies/ccso#IM201/IM_MSc/IED/STEF/TEIC"/>
        <affiliatedWith rdf:resource="http://xworks.gr/ontologies/ccso#IM207/IM_MSc/IED/STEF/TEIC"/>
        <affiliatedWith rdf:resource="http://xworks.gr/ontologies/ccso#IM209/IM_MSc/IED/STEF/TEIC"/>
        <affiliatedWith rdf:resource="http://xworks.gr/ontologies/ccso#MSc_Informatics_&amp;_Multimedia/IM_MSc/IED/STEF/TEIC"/>
        <alumnusOf rdf:resource="http://xworks.gr/ontologies/ccso#Department_of_Informatics_Engineering_of_TEI_of_Crete"/>
        <attendsCourse rdf:resource="http://xworks.gr/ontologies/ccso#IM201/IM_MSc/IED/STEF/TEIC"/>
        <attendsCourse rdf:resource="http://xworks.gr/ontologies/ccso#IM207/IM_MSc/IED/STEF/TEIC"/>
        <attendsCourse rdf:resource="http://xworks.gr/ontologies/ccso#IM209/IM_MSc/IED/STEF/TEIC"/>
        <enrolledIn rdf:resource="http://xworks.gr/ontologies/ccso#MSc_Informatics_&amp;_Multimedia/IM_MSc/IED/STEF/TEIC"/>
        <hasCompleted rdf:resource="http://xworks.gr/ontologies/ccso#IM101/IM_MSc/IED/STEF/TEIC"/>
        <hasCompleted rdf:resource="http://xworks.gr/ontologies/ccso#IM102/IM_MSc/IED/STEF/TEIC"/>
        <hasCompleted rdf:resource="http://xworks.gr/ontologies/ccso#IM105/IM_MSc/IED/STEF/TEIC"/>
        <hasCompleted rdf:resource="http://xworks.gr/ontologies/ccso#IM107/IM_MSc/IED/STEF/TEIC"/>
        <hasDegree rdf:resource="http://xworks.gr/ontologies/ccso#BSc_Informatics_Engineering/IE_BSc/IED/STEF/TEIC"/>
        <schema:email rdf:datatype="http://www.w3.org/2001/XMLSchema#anyURI">Kokkinos_Heraklis@ie.teicrete.gr</schema:email>
        <foaf:firstName rdf:datatype="http://www.w3.org/2001/XMLSchema#string">Heraklis</foaf:firstName>
        <foaf:gender rdf:datatype="http://www.w3.org/2001/XMLSchema#string">Male</foaf:gender>
        <foaf:lastName rdf:datatype="http://www.w3.org/2001/XMLSchema#string">Kokkinos</foaf:lastName>
        <eContactInfo rdf:datatype="http://www.w3.org/2001/XMLSchema#anyURI">Kokkinos_Heraklis@ie.teicrete.gr</eContactInfo>
    </owl:NamedIndividual>
    


    <!-- http://xworks.gr/ontologies/ccso#Kondylakis_Haridimos -->

    <owl:NamedIndividual rdf:about="http://xworks.gr/ontologies/ccso#Kondylakis_Haridimos">
        <rdf:type rdf:resource="http://www.w3.org/2000/10/swap/pim/contact#Person"/>
        <rdf:type rdf:resource="http://xmlns.com/foaf/0.1/Agent"/>
        <rdf:type rdf:resource="http://xmlns.com/foaf/0.1/Person"/>
        <rdf:type rdf:resource="http://xworks.gr/ontologies/ccso#Assistant"/>
        <rdf:type rdf:resource="http://xworks.gr/ontologies/ccso#Employee"/>
        <affiliatedWith rdf:resource="http://xworks.gr/ontologies/ccso#Computers_Sciences_Department_of_University_of_Crete"/>
        <affiliatedWith rdf:resource="http://xworks.gr/ontologies/ccso#BSc_Computer_Science/CS_BSc/CSD/SSE/UoC"/>
        <affiliatedWith rdf:resource="http://xworks.gr/ontologies/ccso#CS150s1/CS_BSc/CSD/SSE/UoC"/>
        <affiliatedWith rdf:resource="http://xworks.gr/ontologies/ccso#CS335_s2017-18-L02/CS_BSc/CSD/SSE/UoC"/>
        <affiliatedWith rdf:resource="http://xworks.gr/ontologies/ccso#CS335_s2017-18-L03/CS_BSc/CSD/SSE/UoC"/>
        <affiliatedWith rdf:resource="http://xworks.gr/ontologies/ccso#CS335_s2017-18-L04/CS_BSc/CSD/SSE/UoC"/>
        <affiliatedWith rdf:resource="http://xworks.gr/ontologies/ccso#CS335_s2017-18/CS_BSc/CSD/SSE/UoC"/>
        <affiliatedWith rdf:resource="http://xworks.gr/ontologies/ccso#CS340s1/CS_BSc/CSD/SSE/UoC"/>
        <affiliatedWith rdf:resource="http://xworks.gr/ontologies/ccso#CS345s1/CS_BSc/CSD/SSE/UoC"/>
        <affiliatedWith rdf:resource="http://xworks.gr/ontologies/ccso#CS360s1/CS_BSc/CSD/SSE/UoC"/>
        <affiliatedWith rdf:resource="http://xworks.gr/ontologies/ccso#IM105s1/IM_MSc/IED/STEF/TEI"/>
        <affiliatedWith rdf:resource="http://xworks.gr/ontologies/ccso#IM202s1/IM_MSc/IED/STEF/TEI"/>
        <affiliatedWith rdf:resource="http://xworks.gr/ontologies/ccso#MSc_Computer_Science_and_Engineering/CSE_MSc/CSD/SSE/UoC"/>
        <affiliatedWith rdf:resource="http://xworks.gr/ontologies/ccso#PhD_Computer_Science_and_Engineering/CSE_PhD/CSD/SSE/UoC"/>
        <alumnusOf rdf:resource="http://xworks.gr/ontologies/ccso#Computers_Sciences_Department_of_University_of_Crete"/>
        <assistsInCourse rdf:resource="http://xworks.gr/ontologies/ccso#CS150s1/CS_BSc/CSD/SSE/UoC"/>
        <assistsInCourse rdf:resource="http://xworks.gr/ontologies/ccso#CS335_s2017-18/CS_BSc/CSD/SSE/UoC"/>
        <assistsInCourse rdf:resource="http://xworks.gr/ontologies/ccso#CS340s1/CS_BSc/CSD/SSE/UoC"/>
        <assistsInCourse rdf:resource="http://xworks.gr/ontologies/ccso#CS345s1/CS_BSc/CSD/SSE/UoC"/>
        <assistsInCourse rdf:resource="http://xworks.gr/ontologies/ccso#CS360s1/CS_BSc/CSD/SSE/UoC"/>
        <assistsInCourse rdf:resource="http://xworks.gr/ontologies/ccso#IM105s1/IM_MSc/IED/STEF/TEI"/>
        <assistsInCourse rdf:resource="http://xworks.gr/ontologies/ccso#IM202s1/IM_MSc/IED/STEF/TEI"/>
        <assistsInEvent rdf:resource="http://xworks.gr/ontologies/ccso#CS335_s2017-18-L02/CS_BSc/CSD/SSE/UoC"/>
        <assistsInEvent rdf:resource="http://xworks.gr/ontologies/ccso#CS335_s2017-18-L03/CS_BSc/CSD/SSE/UoC"/>
        <assistsInEvent rdf:resource="http://xworks.gr/ontologies/ccso#CS335_s2017-18-L04/CS_BSc/CSD/SSE/UoC"/>
        <hasDegree rdf:resource="http://xworks.gr/ontologies/ccso#BSc_Computer_Science/CS_BSc/CSD/SSE/UoC"/>
        <hasDegree rdf:resource="http://xworks.gr/ontologies/ccso#MSc_Computer_Science_and_Engineering/CSE_MSc/CSD/SSE/UoC"/>
        <hasDegree rdf:resource="http://xworks.gr/ontologies/ccso#PhD_Computer_Science_and_Engineering/CSE_PhD/CSD/SSE/UoC"/>
        <hasPublication rdf:resource="http://xworks.gr/ontologies/ccso#Marakakis2012KnowledgeRepresentation"/>
        <worksFor rdf:resource="http://xworks.gr/ontologies/ccso#Computers_Sciences_Department_of_University_of_Crete"/>
        <worksFor rdf:resource="http://xworks.gr/ontologies/ccso#Department_of_Informatics_Engineering_of_TEI_of_Crete"/>
        <schema:email rdf:datatype="http://www.w3.org/2001/XMLSchema#anyURI">kondylak@ics.forth.gr</schema:email>
        <foaf:firstName rdf:datatype="http://www.w3.org/2001/XMLSchema#string">Haridimos</foaf:firstName>
        <foaf:gender rdf:datatype="http://www.w3.org/2001/XMLSchema#string">Male</foaf:gender>
        <foaf:lastName rdf:datatype="http://www.w3.org/2001/XMLSchema#string">Kondylakis</foaf:lastName>
        <eContactInfo rdf:datatype="http://www.w3.org/2001/XMLSchema#anyURI">kondylak@ics.forth.gr</eContactInfo>
        <workEmail rdf:datatype="http://www.w3.org/2001/XMLSchema#anyURI">kondylak@ics.forth.gr</workEmail>
        <rdfs:label xml:lang="en">Kondylakis Haridimos</rdfs:label>
    </owl:NamedIndividual>
    


    <!-- http://xworks.gr/ontologies/ccso#Kornaros_George -->

    <owl:NamedIndividual rdf:about="http://xworks.gr/ontologies/ccso#Kornaros_George">
        <rdf:type rdf:resource="http://xmlns.com/foaf/0.1/Person"/>
        <rdf:type rdf:resource="http://xworks.gr/ontologies/ccso#AcademicStaff"/>
        <rdf:type rdf:resource="http://xworks.gr/ontologies/ccso#Employee"/>
        <rdf:type rdf:resource="http://xworks.gr/ontologies/ccso#Professor"/>
        <affiliatedWith rdf:resource="http://xworks.gr/ontologies/ccso#Computers_Sciences_Department_of_University_of_Crete"/>
        <affiliatedWith rdf:resource="http://xworks.gr/ontologies/ccso#Department_of_Informatics_Engineering_of_TEI_of_Crete"/>
        <affiliatedWith rdf:resource="http://xworks.gr/ontologies/ccso#BSc_Informatics_Engineering/IE_BSc/IED/STEF/TEIC"/>
        <affiliatedWith rdf:resource="http://xworks.gr/ontologies/ccso#IM108s1/IM_MSc/IED/STEF/TEI"/>
        <affiliatedWith rdf:resource="http://xworks.gr/ontologies/ccso#MSc_Informatics_&amp;_Multimedia/IM_MSc/IED/STEF/TEIC"/>
        <affiliatedWith rdf:resource="http://xworks.gr/ontologies/ccso#PhD_Computer_Science_and_Engineering/CSE_PhD/CSD/SSE/UoC"/>
        <affiliatedWith rdf:resource="http://xworks.gr/ontologies/ccso#TP10K3s1/IE_BSc/IED/STEF/TEIC"/>
        <affiliatedWith rdf:resource="http://xworks.gr/ontologies/ccso#TP20K2s1/IE_BSc/IED/STEF/TEIC"/>
        <affiliatedWith rdf:resource="http://xworks.gr/ontologies/ccso#TP60Y2s1/IE_BSc/IED/STEF/TEIC"/>
        <affiliatedWith rdf:resource="http://xworks.gr/ontologies/ccso#TP70Y1s1/IE_BSc/IED/STEF/TEIC"/>
        <affiliatedWith rdf:resource="http://xworks.gr/ontologies/ccso#TP70Y2s1/IE_BSc/IED/STEF/TEIC"/>
        <alumnusOf rdf:resource="http://xworks.gr/ontologies/ccso#Computers_Sciences_Department_of_University_of_Crete"/>
        <alumnusOf rdf:resource="http://xworks.gr/ontologies/ccso#Department_of_Informatics_Engineering_of_TEI_of_Crete"/>
        <hasDegree rdf:resource="http://xworks.gr/ontologies/ccso#BSc_Informatics_Engineering/IE_BSc/IED/STEF/TEIC"/>
        <hasDegree rdf:resource="http://xworks.gr/ontologies/ccso#MSc_Informatics_&amp;_Multimedia/IM_MSc/IED/STEF/TEIC"/>
        <hasDegree rdf:resource="http://xworks.gr/ontologies/ccso#PhD_Computer_Science_and_Engineering/CSE_PhD/CSD/SSE/UoC"/>
        <instructorOf rdf:resource="http://xworks.gr/ontologies/ccso#IM108s1/IM_MSc/IED/STEF/TEI"/>
        <instructorOf rdf:resource="http://xworks.gr/ontologies/ccso#TP10K3s1/IE_BSc/IED/STEF/TEIC"/>
        <instructorOf rdf:resource="http://xworks.gr/ontologies/ccso#TP20K2s1/IE_BSc/IED/STEF/TEIC"/>
        <instructorOf rdf:resource="http://xworks.gr/ontologies/ccso#TP60Y2s1/IE_BSc/IED/STEF/TEIC"/>
        <instructorOf rdf:resource="http://xworks.gr/ontologies/ccso#TP70Y1s1/IE_BSc/IED/STEF/TEIC"/>
        <instructorOf rdf:resource="http://xworks.gr/ontologies/ccso#TP70Y2s1/IE_BSc/IED/STEF/TEIC"/>
        <memberOf rdf:resource="http://xworks.gr/ontologies/ccso#Department_of_Informatics_Engineering_of_TEI_of_Crete"/>
        <supervisorOf rdf:resource="http://xworks.gr/ontologies/ccso#IM108s1/IM_MSc/IED/STEF/TEI"/>
        <supervisorOf rdf:resource="http://xworks.gr/ontologies/ccso#TP10K3s1/IE_BSc/IED/STEF/TEIC"/>
        <supervisorOf rdf:resource="http://xworks.gr/ontologies/ccso#TP20K2s1/IE_BSc/IED/STEF/TEIC"/>
        <supervisorOf rdf:resource="http://xworks.gr/ontologies/ccso#TP60Y2s1/IE_BSc/IED/STEF/TEIC"/>
        <supervisorOf rdf:resource="http://xworks.gr/ontologies/ccso#TP70Y1s1/IE_BSc/IED/STEF/TEIC"/>
        <worksFor rdf:resource="http://xworks.gr/ontologies/ccso#Department_of_Informatics_Engineering_of_TEI_of_Crete"/>
        <schema:email rdf:datatype="http://www.w3.org/2001/XMLSchema#anyURI">kornaros@ie.teicrete.gr</schema:email>
        <foaf:firstName rdf:datatype="http://www.w3.org/2001/XMLSchema#string">George</foaf:firstName>
        <foaf:lastName rdf:datatype="http://www.w3.org/2001/XMLSchema#string">Kornaros</foaf:lastName>
        <eContactInfo rdf:datatype="http://www.w3.org/2001/XMLSchema#anyURI">kornaros@ie.teicrete.gr</eContactInfo>
    </owl:NamedIndividual>
    


    <!-- http://xworks.gr/ontologies/ccso#Lecture -->

    <owl:NamedIndividual rdf:about="http://xworks.gr/ontologies/ccso#Lecture">
        <rdf:type rdf:resource="http://xworks.gr/ontologies/ccso#TeachingEvaluationMethod"/>
        <mediaUsed rdf:datatype="http://www.w3.org/2001/XMLSchema#string">Computer, Projector</mediaUsed>
        <methodName rdf:datatype="http://www.w3.org/2001/XMLSchema#string">Lecture</methodName>
    </owl:NamedIndividual>
    


    <!-- http://xworks.gr/ontologies/ccso#Lioni_Catherine -->

    <owl:NamedIndividual rdf:about="http://xworks.gr/ontologies/ccso#Lioni_Catherine">
        <rdf:type rdf:resource="http://xmlns.com/foaf/0.1/Agent"/>
        <rdf:type rdf:resource="http://xmlns.com/foaf/0.1/Person"/>
        <rdf:type rdf:resource="http://xworks.gr/ontologies/ccso#PostgraduateStudent"/>
        <rdf:type rdf:resource="http://xworks.gr/ontologies/ccso#Student"/>
        <affiliatedWith rdf:resource="http://xworks.gr/ontologies/ccso#Psychology_Department_of_University_of_Crete"/>
        <affiliatedWith rdf:resource="http://xworks.gr/ontologies/ccso#BSc_Psychology/PSY_BSc/SoC/UoC"/>
        <affiliatedWith rdf:resource="http://xworks.gr/ontologies/ccso#MSc_School_Psychology/SP_MSc/PSY/SoC/UoC"/>
        <affiliatedWith rdf:resource="http://xworks.gr/ontologies/ccso#PSY1501/PSY_BSc/SoC/Uoc"/>
        <alumnusOf rdf:resource="http://xworks.gr/ontologies/ccso#Psychology_Department_of_University_of_Crete"/>
        <enrolledIn rdf:resource="http://xworks.gr/ontologies/ccso#MSc_School_Psychology/SP_MSc/PSY/SoC/UoC"/>
        <hasCompleted rdf:resource="http://xworks.gr/ontologies/ccso#PSY1501/PSY_BSc/SoC/Uoc"/>
        <hasDegree rdf:resource="http://xworks.gr/ontologies/ccso#BSc_Psychology/PSY_BSc/SoC/UoC"/>
        <schema:email rdf:datatype="http://www.w3.org/2001/XMLSchema#anyURI">Lioni_Catherine@psy.uoc.gr</schema:email>
        <foaf:familyName rdf:datatype="http://www.w3.org/2001/XMLSchema#string">Lioni</foaf:familyName>
        <foaf:firstName rdf:datatype="http://www.w3.org/2001/XMLSchema#string">Catherine</foaf:firstName>
        <foaf:gender rdf:datatype="http://www.w3.org/2001/XMLSchema#string">Female</foaf:gender>
        <foaf:lastName rdf:datatype="http://www.w3.org/2001/XMLSchema#string">Lioni</foaf:lastName>
        <eContactInfo rdf:datatype="http://www.w3.org/2001/XMLSchema#anyURI">Lioni_Catherine@psy.uoc.gr</eContactInfo>
    </owl:NamedIndividual>
    


    <!-- http://xworks.gr/ontologies/ccso#Lionis_Joshua -->

    <owl:NamedIndividual rdf:about="http://xworks.gr/ontologies/ccso#Lionis_Joshua">
        <rdf:type rdf:resource="http://xmlns.com/foaf/0.1/Agent"/>
        <rdf:type rdf:resource="http://xmlns.com/foaf/0.1/Person"/>
        <rdf:type rdf:resource="http://xworks.gr/ontologies/ccso#PostgraduateStudent"/>
        <rdf:type rdf:resource="http://xworks.gr/ontologies/ccso#Student"/>
        <affiliatedWith rdf:resource="http://xworks.gr/ontologies/ccso#Computers_Sciences_Department_of_University_of_Crete"/>
        <affiliatedWith rdf:resource="http://xworks.gr/ontologies/ccso#BSc_Computer_Science/CS_BSc/CSD/SSE/UoC"/>
        <affiliatedWith rdf:resource="http://xworks.gr/ontologies/ccso#MSc_Computer_Science_and_Engineering/CSE_MSc/CSD/SSE/UoC"/>
        <alumnusOf rdf:resource="http://xworks.gr/ontologies/ccso#Computers_Sciences_Department_of_University_of_Crete"/>
        <enrolledIn rdf:resource="http://xworks.gr/ontologies/ccso#MSc_Computer_Science_and_Engineering/CSE_MSc/CSD/SSE/UoC"/>
        <hasDegree rdf:resource="http://xworks.gr/ontologies/ccso#BSc_Computer_Science/CS_BSc/CSD/SSE/UoC"/>
        <schema:email rdf:datatype="http://www.w3.org/2001/XMLSchema#anyURI">Lionis_Joshua@csd.uoc.gr</schema:email>
        <foaf:firstName rdf:datatype="http://www.w3.org/2001/XMLSchema#string">Joshua</foaf:firstName>
        <foaf:gender rdf:datatype="http://www.w3.org/2001/XMLSchema#string">Male</foaf:gender>
        <foaf:lastName rdf:datatype="http://www.w3.org/2001/XMLSchema#string">Lionis</foaf:lastName>
        <eContactInfo rdf:datatype="http://www.w3.org/2001/XMLSchema#anyURI">Lionis_Joshua@csd.uoc.gr</eContactInfo>
    </owl:NamedIndividual>
    


    <!-- http://xworks.gr/ontologies/ccso#Lionis_Tim -->

    <owl:NamedIndividual rdf:about="http://xworks.gr/ontologies/ccso#Lionis_Tim">
        <rdf:type rdf:resource="http://xmlns.com/foaf/0.1/Agent"/>
        <rdf:type rdf:resource="http://xmlns.com/foaf/0.1/Person"/>
        <rdf:type rdf:resource="http://xworks.gr/ontologies/ccso#Student"/>
        <schema:email rdf:datatype="http://www.w3.org/2001/XMLSchema#anyURI">Lionis_Tim@mail.gr</schema:email>
        <foaf:familyName rdf:datatype="http://www.w3.org/2001/XMLSchema#string">Lionis</foaf:familyName>
        <foaf:firstName rdf:datatype="http://www.w3.org/2001/XMLSchema#string">Tim</foaf:firstName>
        <foaf:gender rdf:datatype="http://www.w3.org/2001/XMLSchema#string">Male</foaf:gender>
        <foaf:lastName rdf:datatype="http://www.w3.org/2001/XMLSchema#string">Lionis</foaf:lastName>
        <eContactInfo rdf:datatype="http://www.w3.org/2001/XMLSchema#anyURI">Lionis_Tim@mail.gr</eContactInfo>
    </owl:NamedIndividual>
    


    <!-- http://xworks.gr/ontologies/ccso#Lourakis_Stelios -->

    <owl:NamedIndividual rdf:about="http://xworks.gr/ontologies/ccso#Lourakis_Stelios">
        <rdf:type rdf:resource="http://xmlns.com/foaf/0.1/Person"/>
        <rdf:type rdf:resource="http://xworks.gr/ontologies/ccso#Student"/>
        <foaf:firstName rdf:datatype="http://www.w3.org/2001/XMLSchema#string">Stelios</foaf:firstName>
        <foaf:lastName rdf:datatype="http://www.w3.org/2001/XMLSchema#string">Lourakis</foaf:lastName>
    </owl:NamedIndividual>
    


    <!-- http://xworks.gr/ontologies/ccso#Malamos_Athanasios -->

    <owl:NamedIndividual rdf:about="http://xworks.gr/ontologies/ccso#Malamos_Athanasios">
        <rdf:type rdf:resource="http://xmlns.com/foaf/0.1/Person"/>
        <rdf:type rdf:resource="http://xworks.gr/ontologies/ccso#AcademicStaff"/>
        <rdf:type rdf:resource="http://xworks.gr/ontologies/ccso#Employee"/>
        <rdf:type rdf:resource="http://xworks.gr/ontologies/ccso#Professor"/>
        <affiliatedWith rdf:resource="http://xworks.gr/ontologies/ccso#Department_of_Informatics_Engineering_of_TEI_of_Crete"/>
        <affiliatedWith rdf:resource="http://xworks.gr/ontologies/ccso#IM103s1/IM_MSc/IED/STEF/TEI"/>
        <affiliatedWith rdf:resource="http://xworks.gr/ontologies/ccso#IM201s1/IM_MSc/IED/STEF/TEI"/>
        <affiliatedWith rdf:resource="http://xworks.gr/ontologies/ccso#TP40K3s1/IE_BSc/IED/STEF/TEIC"/>
        <affiliatedWith rdf:resource="http://xworks.gr/ontologies/ccso#TP50Y1s1/IE_BSc/IED/STEF/TEIC"/>
        <affiliatedWith rdf:resource="http://xworks.gr/ontologies/ccso#TP60D3s1/IE_BSc/IED/STEF/TEIC"/>
        <affiliatedWith rdf:resource="http://xworks.gr/ontologies/ccso#TP70D5s1/IE_BSc/IED/STEF/TEIC"/>
        <instructorOf rdf:resource="http://xworks.gr/ontologies/ccso#IM103s1/IM_MSc/IED/STEF/TEI"/>
        <instructorOf rdf:resource="http://xworks.gr/ontologies/ccso#TP40K3s1/IE_BSc/IED/STEF/TEIC"/>
        <instructorOf rdf:resource="http://xworks.gr/ontologies/ccso#TP50Y1s1/IE_BSc/IED/STEF/TEIC"/>
        <instructorOf rdf:resource="http://xworks.gr/ontologies/ccso#TP60D3s1/IE_BSc/IED/STEF/TEIC"/>
        <instructorOf rdf:resource="http://xworks.gr/ontologies/ccso#TP70D5s1/IE_BSc/IED/STEF/TEIC"/>
        <memberOf rdf:resource="http://xworks.gr/ontologies/ccso#Department_of_Informatics_Engineering_of_TEI_of_Crete"/>
        <supervisorOf rdf:resource="http://xworks.gr/ontologies/ccso#IM103s1/IM_MSc/IED/STEF/TEI"/>
        <supervisorOf rdf:resource="http://xworks.gr/ontologies/ccso#IM201s1/IM_MSc/IED/STEF/TEI"/>
        <supervisorOf rdf:resource="http://xworks.gr/ontologies/ccso#TP40K3s1/IE_BSc/IED/STEF/TEIC"/>
        <supervisorOf rdf:resource="http://xworks.gr/ontologies/ccso#TP50Y1s1/IE_BSc/IED/STEF/TEIC"/>
        <supervisorOf rdf:resource="http://xworks.gr/ontologies/ccso#TP60D3s1/IE_BSc/IED/STEF/TEIC"/>
        <supervisorOf rdf:resource="http://xworks.gr/ontologies/ccso#TP70D5s1/IE_BSc/IED/STEF/TEIC"/>
        <worksFor rdf:resource="http://xworks.gr/ontologies/ccso#Department_of_Informatics_Engineering_of_TEI_of_Crete"/>
        <schema:email rdf:datatype="http://www.w3.org/2001/XMLSchema#anyURI">malamos@ie.teicrete.gr</schema:email>
        <foaf:firstName rdf:datatype="http://www.w3.org/2001/XMLSchema#string">Athanasios</foaf:firstName>
        <foaf:lastName rdf:datatype="http://www.w3.org/2001/XMLSchema#string">Malamos</foaf:lastName>
        <foaf:title rdf:datatype="http://www.w3.org/2001/XMLSchema#string">Dr</foaf:title>
        <foaf:title rdf:datatype="http://www.w3.org/2001/XMLSchema#string">Male</foaf:title>
        <eContactInfo rdf:datatype="http://www.w3.org/2001/XMLSchema#anyURI">malamos@ie.teicrete.gr</eContactInfo>
        <phone rdf:datatype="http://www.w3.org/2001/XMLSchema#string">2810379884</phone>
        <profilePic rdf:datatype="http://www.w3.org/2001/XMLSchema#anyURI">https://www.teicrete.gr/mscie/sites/teicrete.gr.mscie/files/styles/profile_pic/public/pictures/picture-56-1389092221.jpg?itok=coVrW_rK</profilePic>
        <staffPosition rdf:datatype="http://www.w3.org/2001/XMLSchema#string">Associate Professor</staffPosition>
        <workPhone rdf:datatype="http://www.w3.org/2001/XMLSchema#string">2810379884</workPhone>
    </owl:NamedIndividual>
    


    <!-- http://xworks.gr/ontologies/ccso#Manifavas_Harry -->

    <owl:NamedIndividual rdf:about="http://xworks.gr/ontologies/ccso#Manifavas_Harry">
        <rdf:type rdf:resource="http://www.w3.org/2000/10/swap/pim/contact#Person"/>
        <rdf:type rdf:resource="http://xmlns.com/foaf/0.1/Person"/>
        <rdf:type rdf:resource="http://xworks.gr/ontologies/ccso#AcademicStaff"/>
        <rdf:type rdf:resource="http://xworks.gr/ontologies/ccso#Employee"/>
        <rdf:type rdf:resource="http://xworks.gr/ontologies/ccso#Professor"/>
        <affiliatedWith rdf:resource="http://xworks.gr/ontologies/ccso#Department_of_Informatics_Engineering_of_TEI_of_Crete"/>
        <affiliatedWith rdf:resource="http://xworks.gr/ontologies/ccso#IM205s1/IM_MSc/IED/STEF/TEI"/>
        <hasPublication rdf:resource="http://xworks.gr/ontologies/ccso#Hatzivasilis2014ReasoningSystem"/>
        <instructorOf rdf:resource="http://xworks.gr/ontologies/ccso#IM205s1/IM_MSc/IED/STEF/TEI"/>
        <memberOf rdf:resource="http://xworks.gr/ontologies/ccso#Department_of_Informatics_Engineering_of_TEI_of_Crete"/>
        <supervisorOf rdf:resource="http://xworks.gr/ontologies/ccso#IM205s1/IM_MSc/IED/STEF/TEI"/>
        <worksFor rdf:resource="http://xworks.gr/ontologies/ccso#Department_of_Informatics_Engineering_of_TEI_of_Crete"/>
        <schema:email rdf:datatype="http://www.w3.org/2001/XMLSchema#anyURI">manifavas@ie.teicrete.gr</schema:email>
        <foaf:firstName rdf:datatype="http://www.w3.org/2001/XMLSchema#string">Harry</foaf:firstName>
        <foaf:lastName rdf:datatype="http://www.w3.org/2001/XMLSchema#string">Manifavas</foaf:lastName>
        <eContactInfo rdf:datatype="http://www.w3.org/2001/XMLSchema#anyURI">manifavas@ie.teicrete.gr</eContactInfo>
    </owl:NamedIndividual>
    


    <!-- http://xworks.gr/ontologies/ccso#Marakakis2005ExpertSystem -->

    <owl:NamedIndividual rdf:about="http://xworks.gr/ontologies/ccso#Marakakis2005ExpertSystem">
        <rdf:type rdf:resource="http://xworks.gr/ontologies/ccso#Resource"/>
        <dc:creator rdf:resource="http://xworks.gr/ontologies/ccso#Marakakis_Manolis"/>
        <dc:creator rdf:resource="http://xworks.gr/ontologies/ccso#Vassilakis_Kostas"/>
        <dc:date rdf:datatype="http://www.w3.org/2001/XMLSchema#date">2005</dc:date>
        <dc:date rdf:datatype="internal:anonymous-constants">2005</dc:date>
        <dc:source rdf:datatype="http://www.w3.org/2001/XMLSchema#string">AIML 05 Conference Proceeedings</dc:source>
        <dc:title rdf:datatype="http://www.w3.org/2001/XMLSchema#string">Expert System for Epilepsy with Uncertainty</dc:title>
        <dc:type rdf:datatype="http://www.w3.org/2001/XMLSchema#string">Proceedings</dc:type>
        <dates rdf:datatype="internal:anonymous-constants">2005</dates>
        <rdfs:label xml:lang="en">Marakakis, Vassilakis (2005) Expert System for Epilepsy with Uncertainty</rdfs:label>
    </owl:NamedIndividual>
    


    <!-- http://xworks.gr/ontologies/ccso#Marakakis2012KnowledgeRepresentation -->

    <owl:NamedIndividual rdf:about="http://xworks.gr/ontologies/ccso#Marakakis2012KnowledgeRepresentation">
        <rdf:type rdf:resource="http://xworks.gr/ontologies/ccso#Resource"/>
        <dc:creator rdf:resource="http://xworks.gr/ontologies/ccso#Kondylakis_Haridimos"/>
        <dc:creator rdf:resource="http://xworks.gr/ontologies/ccso#Papadakis_Nikos"/>
        <dc:date rdf:datatype="http://www.w3.org/2001/XMLSchema#date">2012</dc:date>
        <dc:date rdf:datatype="internal:anonymous-constants">2012</dc:date>
        <dc:source rdf:datatype="http://www.w3.org/2001/XMLSchema#string">In Advances in Knowledge Representation. InTech.</dc:source>
        <dc:title rdf:datatype="http://www.w3.org/2001/XMLSchema#string">Knowledge Representation in a proof checker for logic programs</dc:title>
        <dc:type rdf:datatype="http://www.w3.org/2001/XMLSchema#string">Article</dc:type>
        <dates rdf:datatype="internal:anonymous-constants">2012</dates>
        <resourceCitation rdf:datatype="http://www.w3.org/2001/XMLSchema#string">Marakakis, E., Kondylakis, H., &amp; Papadakis, N. (2012). Knowledge representation in a proof checker for logic programs. In Advances in Knowledge Representation. InTech</resourceCitation>
        <rdfs:label xml:lang="en">Marakakis,Kondylakis,Papadakis (2012) Knowledge Representation in a proof checker for logic programs</rdfs:label>
    </owl:NamedIndividual>
    


    <!-- http://xworks.gr/ontologies/ccso#Marakakis_Manolis -->

    <owl:NamedIndividual rdf:about="http://xworks.gr/ontologies/ccso#Marakakis_Manolis">
        <rdf:type rdf:resource="http://www.w3.org/2000/10/swap/pim/contact#Person"/>
        <rdf:type rdf:resource="http://xmlns.com/foaf/0.1/Person"/>
        <rdf:type rdf:resource="http://xworks.gr/ontologies/ccso#AcademicStaff"/>
        <rdf:type rdf:resource="http://xworks.gr/ontologies/ccso#Employee"/>
        <rdf:type rdf:resource="http://xworks.gr/ontologies/ccso#Professor"/>
        <affiliatedWith rdf:resource="http://xworks.gr/ontologies/ccso#Department_of_Informatics_Engineering_of_TEI_of_Crete"/>
        <affiliatedWith rdf:resource="http://xworks.gr/ontologies/ccso#IM207s1/IM_MSc/IED/STEF/TEI"/>
        <affiliatedWith rdf:resource="http://xworks.gr/ontologies/ccso#TP50L3s1/IE_BSc/IED/STEF/TEIC"/>
        <affiliatedWith rdf:resource="http://xworks.gr/ontologies/ccso#TP60L2s1/IE_BSc/IED/STEF/TEIC"/>
        <affiliatedWith rdf:resource="http://xworks.gr/ontologies/ccso#TP70L1s1/IE_BSc/IED/STEF/TEIC"/>
        <hasPublication rdf:resource="http://xworks.gr/ontologies/ccso#Marakakis2005ExpertSystem"/>
        <instructorOf rdf:resource="http://xworks.gr/ontologies/ccso#IM207s1/IM_MSc/IED/STEF/TEI"/>
        <instructorOf rdf:resource="http://xworks.gr/ontologies/ccso#TP50L3s1/IE_BSc/IED/STEF/TEIC"/>
        <instructorOf rdf:resource="http://xworks.gr/ontologies/ccso#TP60L2s1/IE_BSc/IED/STEF/TEIC"/>
        <instructorOf rdf:resource="http://xworks.gr/ontologies/ccso#TP70L1s1/IE_BSc/IED/STEF/TEIC"/>
        <memberOf rdf:resource="http://xworks.gr/ontologies/ccso#Department_of_Informatics_Engineering_of_TEI_of_Crete"/>
        <supervisorOf rdf:resource="http://xworks.gr/ontologies/ccso#IM207s1/IM_MSc/IED/STEF/TEI"/>
        <supervisorOf rdf:resource="http://xworks.gr/ontologies/ccso#TP50L3s1/IE_BSc/IED/STEF/TEIC"/>
        <supervisorOf rdf:resource="http://xworks.gr/ontologies/ccso#TP60L2s1/IE_BSc/IED/STEF/TEIC"/>
        <supervisorOf rdf:resource="http://xworks.gr/ontologies/ccso#TP70L1s1/IE_BSc/IED/STEF/TEIC"/>
        <worksFor rdf:resource="http://xworks.gr/ontologies/ccso#Department_of_Informatics_Engineering_of_TEI_of_Crete"/>
        <schema:email rdf:datatype="http://www.w3.org/2001/XMLSchema#anyURI">marakakis@ie.teicrete.gr</schema:email>
        <foaf:firstName rdf:datatype="http://www.w3.org/2001/XMLSchema#string">Manolis</foaf:firstName>
        <foaf:lastName rdf:datatype="http://www.w3.org/2001/XMLSchema#string">Marakakis</foaf:lastName>
        <eContactInfo rdf:datatype="http://www.w3.org/2001/XMLSchema#anyURI">marakakis@ie.teicrete.gr</eContactInfo>
    </owl:NamedIndividual>
    


    <!-- http://xworks.gr/ontologies/ccso#Marias_Kostas -->

    <owl:NamedIndividual rdf:about="http://xworks.gr/ontologies/ccso#Marias_Kostas">
        <rdf:type rdf:resource="http://xmlns.com/foaf/0.1/Person"/>
        <rdf:type rdf:resource="http://xworks.gr/ontologies/ccso#AcademicStaff"/>
        <rdf:type rdf:resource="http://xworks.gr/ontologies/ccso#Employee"/>
        <rdf:type rdf:resource="http://xworks.gr/ontologies/ccso#Professor"/>
        <affiliatedWith rdf:resource="http://xworks.gr/ontologies/ccso#Department_of_Informatics_Engineering_of_TEI_of_Crete"/>
        <affiliatedWith rdf:resource="http://xworks.gr/ontologies/ccso#TP50Y2s1/IE_BSc/IED/STEF/TEIC"/>
        <affiliatedWith rdf:resource="http://xworks.gr/ontologies/ccso#TP70Y2s1/IE_BSc/IED/STEF/TEIC"/>
        <instructorOf rdf:resource="http://xworks.gr/ontologies/ccso#TP50Y2s1/IE_BSc/IED/STEF/TEIC"/>
        <memberOf rdf:resource="http://xworks.gr/ontologies/ccso#Department_of_Informatics_Engineering_of_TEI_of_Crete"/>
        <supervisorOf rdf:resource="http://xworks.gr/ontologies/ccso#TP50Y2s1/IE_BSc/IED/STEF/TEIC"/>
        <supervisorOf rdf:resource="http://xworks.gr/ontologies/ccso#TP70Y2s1/IE_BSc/IED/STEF/TEIC"/>
        <worksFor rdf:resource="http://xworks.gr/ontologies/ccso#Department_of_Informatics_Engineering_of_TEI_of_Crete"/>
        <schema:email rdf:datatype="http://www.w3.org/2001/XMLSchema#anyURI">marias@ie.teicrete.gr</schema:email>
        <foaf:firstName rdf:datatype="http://www.w3.org/2001/XMLSchema#string">Kostas</foaf:firstName>
        <foaf:lastName rdf:datatype="http://www.w3.org/2001/XMLSchema#string">Marias</foaf:lastName>
        <eContactInfo rdf:datatype="http://www.w3.org/2001/XMLSchema#anyURI">marias@ie.teicrete.gr</eContactInfo>
    </owl:NamedIndividual>
    


    <!-- http://xworks.gr/ontologies/ccso#Markatos_Evangelos -->

    <owl:NamedIndividual rdf:about="http://xworks.gr/ontologies/ccso#Markatos_Evangelos">
        <rdf:type rdf:resource="http://xmlns.com/foaf/0.1/Agent"/>
        <rdf:type rdf:resource="http://xmlns.com/foaf/0.1/Person"/>
        <rdf:type rdf:resource="http://xworks.gr/ontologies/ccso#AcademicStaff"/>
        <rdf:type rdf:resource="http://xworks.gr/ontologies/ccso#Employee"/>
        <rdf:type rdf:resource="http://xworks.gr/ontologies/ccso#Professor"/>
        <affiliatedWith rdf:resource="http://xworks.gr/ontologies/ccso#Computers_Sciences_Department_of_University_of_Crete"/>
        <affiliatedWith rdf:resource="http://xworks.gr/ontologies/ccso#CS345_s2017-18-L02/CS_BSc/CSD/SSE/UoC"/>
        <affiliatedWith rdf:resource="http://xworks.gr/ontologies/ccso#CS345s1/CS_BSc/CSD/SSE/UoC"/>
        <instructorOf rdf:resource="http://xworks.gr/ontologies/ccso#CS345s1/CS_BSc/CSD/SSE/UoC"/>
        <memberOf rdf:resource="http://xworks.gr/ontologies/ccso#Computers_Sciences_Department_of_University_of_Crete"/>
        <supervisorOf rdf:resource="http://xworks.gr/ontologies/ccso#CS345s1/CS_BSc/CSD/SSE/UoC"/>
        <teachesIn rdf:resource="http://xworks.gr/ontologies/ccso#CS345_s2017-18-L02/CS_BSc/CSD/SSE/UoC"/>
        <worksFor rdf:resource="http://xworks.gr/ontologies/ccso#Computers_Sciences_Department_of_University_of_Crete"/>
        <foaf:firstName rdf:datatype="http://www.w3.org/2001/XMLSchema#string">Evangelos</foaf:firstName>
        <foaf:gender rdf:datatype="http://www.w3.org/2001/XMLSchema#string">Male</foaf:gender>
        <foaf:lastName rdf:datatype="http://www.w3.org/2001/XMLSchema#string">Markatos</foaf:lastName>
        <eContactInfo rdf:datatype="http://www.w3.org/2001/XMLSchema#anyURI">markatos@csd.uoc.gr</eContactInfo>
        <officeHours rdf:datatype="http://www.w3.org/2001/XMLSchema#string">Monday 14:00-14:30</officeHours>
        <workEmail rdf:datatype="http://www.w3.org/2001/XMLSchema#anyURI">markatos@csd.uoc.gr</workEmail>
    </owl:NamedIndividual>
    


    <!-- http://xworks.gr/ontologies/ccso#Martelis_Stelios -->

    <owl:NamedIndividual rdf:about="http://xworks.gr/ontologies/ccso#Martelis_Stelios">
        <rdf:type rdf:resource="http://xmlns.com/foaf/0.1/Agent"/>
        <rdf:type rdf:resource="http://xmlns.com/foaf/0.1/Person"/>
        <rdf:type rdf:resource="http://xworks.gr/ontologies/ccso#PostgraduateStudent"/>
        <rdf:type rdf:resource="http://xworks.gr/ontologies/ccso#Student"/>
        <affiliatedWith rdf:resource="http://xworks.gr/ontologies/ccso#Department_of_Informatics_Engineering_of_TEI_of_Crete"/>
        <affiliatedWith rdf:resource="http://xworks.gr/ontologies/ccso#BSc_Informatics_Engineering/IE_BSc/IED/STEF/TEIC"/>
        <affiliatedWith rdf:resource="http://xworks.gr/ontologies/ccso#IM101/IM_MSc/IED/STEF/TEIC"/>
        <affiliatedWith rdf:resource="http://xworks.gr/ontologies/ccso#IM104/IM_MSc/IED/STEF/TEIC"/>
        <affiliatedWith rdf:resource="http://xworks.gr/ontologies/ccso#IM107/IM_MSc/IED/STEF/TEIC"/>
        <affiliatedWith rdf:resource="http://xworks.gr/ontologies/ccso#IM201/IM_MSc/IED/STEF/TEIC"/>
        <affiliatedWith rdf:resource="http://xworks.gr/ontologies/ccso#IM205/IM_MSc/IED/STEF/TEIC"/>
        <affiliatedWith rdf:resource="http://xworks.gr/ontologies/ccso#IM209/IM_MSc/IED/STEF/TEIC"/>
        <affiliatedWith rdf:resource="http://xworks.gr/ontologies/ccso#MSc_Informatics_&amp;_Multimedia/IM_MSc/IED/STEF/TEIC"/>
        <alumnusOf rdf:resource="http://xworks.gr/ontologies/ccso#Department_of_Informatics_Engineering_of_TEI_of_Crete"/>
        <attendsCourse rdf:resource="http://xworks.gr/ontologies/ccso#IM201/IM_MSc/IED/STEF/TEIC"/>
        <attendsCourse rdf:resource="http://xworks.gr/ontologies/ccso#IM205/IM_MSc/IED/STEF/TEIC"/>
        <attendsCourse rdf:resource="http://xworks.gr/ontologies/ccso#IM209/IM_MSc/IED/STEF/TEIC"/>
        <enrolledIn rdf:resource="http://xworks.gr/ontologies/ccso#MSc_Informatics_&amp;_Multimedia/IM_MSc/IED/STEF/TEIC"/>
        <hasCompleted rdf:resource="http://xworks.gr/ontologies/ccso#IM101/IM_MSc/IED/STEF/TEIC"/>
        <hasCompleted rdf:resource="http://xworks.gr/ontologies/ccso#IM104/IM_MSc/IED/STEF/TEIC"/>
        <hasCompleted rdf:resource="http://xworks.gr/ontologies/ccso#IM107/IM_MSc/IED/STEF/TEIC"/>
        <hasDegree rdf:resource="http://xworks.gr/ontologies/ccso#BSc_Informatics_Engineering/IE_BSc/IED/STEF/TEIC"/>
        <schema:email rdf:datatype="http://www.w3.org/2001/XMLSchema#anyURI">Martelis_Stelios@ie.teicrete.gr</schema:email>
        <foaf:familyName rdf:datatype="http://www.w3.org/2001/XMLSchema#string">Martelis</foaf:familyName>
        <foaf:firstName rdf:datatype="http://www.w3.org/2001/XMLSchema#string">Stelios</foaf:firstName>
        <foaf:gender rdf:datatype="http://www.w3.org/2001/XMLSchema#string">Male</foaf:gender>
        <foaf:lastName rdf:datatype="http://www.w3.org/2001/XMLSchema#string">Martelis</foaf:lastName>
        <eContactInfo rdf:datatype="http://www.w3.org/2001/XMLSchema#anyURI">Martelis_Stelios@ie.teicrete.gr</eContactInfo>
    </owl:NamedIndividual>
    


    <!-- http://xworks.gr/ontologies/ccso#Mastorakis_George -->

    <owl:NamedIndividual rdf:about="http://xworks.gr/ontologies/ccso#Mastorakis_George">
        <rdf:type rdf:resource="http://xmlns.com/foaf/0.1/Person"/>
        <rdf:type rdf:resource="http://xworks.gr/ontologies/ccso#AcademicStaff"/>
        <rdf:type rdf:resource="http://xworks.gr/ontologies/ccso#Employee"/>
        <rdf:type rdf:resource="http://xworks.gr/ontologies/ccso#Professor"/>
        <affiliatedWith rdf:resource="http://xworks.gr/ontologies/ccso#Department_of_Informatics_Engineering_of_TEI_of_Crete"/>
        <memberOf rdf:resource="http://xworks.gr/ontologies/ccso#Department_of_Informatics_Engineering_of_TEI_of_Crete"/>
        <schema:email rdf:datatype="http://www.w3.org/2001/XMLSchema#anyURI">mastorakis@ie.teicrete.gr</schema:email>
        <foaf:firstName rdf:datatype="http://www.w3.org/2001/XMLSchema#string">George</foaf:firstName>
        <foaf:lastName rdf:datatype="http://www.w3.org/2001/XMLSchema#string">Mastorakis</foaf:lastName>
        <eContactInfo rdf:datatype="http://www.w3.org/2001/XMLSchema#anyURI">mastorakis@ie.teicrete.gr</eContactInfo>
    </owl:NamedIndividual>
    


    <!-- http://xworks.gr/ontologies/ccso#Mathematics -->

    <owl:NamedIndividual rdf:about="http://xworks.gr/ontologies/ccso#Mathematics">
        <rdf:type rdf:resource="http://xworks.gr/ontologies/ccso#Discipline"/>
        <rdf:type rdf:resource="http://xworks.gr/ontologies/ccso#FieldofStudy"/>
        <abbreviation rdf:datatype="http://www.w3.org/2001/XMLSchema#string">Maths</abbreviation>
        <fsName rdf:datatype="http://www.w3.org/2001/XMLSchema#string">Mathematics</fsName>
    </owl:NamedIndividual>
    


    <!-- http://xworks.gr/ontologies/ccso#Mourati_Ginna -->

    <owl:NamedIndividual rdf:about="http://xworks.gr/ontologies/ccso#Mourati_Ginna">
        <rdf:type rdf:resource="http://xmlns.com/foaf/0.1/Person"/>
        <rdf:type rdf:resource="http://xworks.gr/ontologies/ccso#PostgraduateStudent"/>
        <rdf:type rdf:resource="http://xworks.gr/ontologies/ccso#Student"/>
        <affiliatedWith rdf:resource="http://xworks.gr/ontologies/ccso#Psychology_Department_of_University_of_Crete"/>
        <affiliatedWith rdf:resource="http://xworks.gr/ontologies/ccso#BSc_Psychology/PSY_BSc/SoC/UoC"/>
        <affiliatedWith rdf:resource="http://xworks.gr/ontologies/ccso#MSc_School_Psychology/SP_MSc/PSY/SoC/UoC"/>
        <alumnusOf rdf:resource="http://xworks.gr/ontologies/ccso#Psychology_Department_of_University_of_Crete"/>
        <enrolledIn rdf:resource="http://xworks.gr/ontologies/ccso#MSc_School_Psychology/SP_MSc/PSY/SoC/UoC"/>
        <hasDegree rdf:resource="http://xworks.gr/ontologies/ccso#BSc_Psychology/PSY_BSc/SoC/UoC"/>
        <foaf:firstName rdf:datatype="http://www.w3.org/2001/XMLSchema#string">Ginna</foaf:firstName>
        <foaf:lastName rdf:datatype="http://www.w3.org/2001/XMLSchema#string">Mourati</foaf:lastName>
    </owl:NamedIndividual>
    


    <!-- http://xworks.gr/ontologies/ccso#Mouratidis_Jordan -->

    <owl:NamedIndividual rdf:about="http://xworks.gr/ontologies/ccso#Mouratidis_Jordan">
        <rdf:type rdf:resource="http://xmlns.com/foaf/0.1/Agent"/>
        <rdf:type rdf:resource="http://xmlns.com/foaf/0.1/Person"/>
        <rdf:type rdf:resource="http://xworks.gr/ontologies/ccso#Student"/>
        <schema:email rdf:datatype="http://www.w3.org/2001/XMLSchema#anyURI">Mouratidis_Jordan@mail.gr</schema:email>
        <foaf:familyName rdf:datatype="http://www.w3.org/2001/XMLSchema#string">Mouratidis</foaf:familyName>
        <foaf:firstName rdf:datatype="http://www.w3.org/2001/XMLSchema#string">Jordan</foaf:firstName>
        <foaf:gender rdf:datatype="http://www.w3.org/2001/XMLSchema#string">Male</foaf:gender>
        <foaf:lastName rdf:datatype="http://www.w3.org/2001/XMLSchema#string">Mouratidis</foaf:lastName>
        <eContactInfo rdf:datatype="http://www.w3.org/2001/XMLSchema#anyURI">Mouratidis_Jordan@mail.gr</eContactInfo>
    </owl:NamedIndividual>
    


    <!-- http://xworks.gr/ontologies/ccso#Mouxtaris_Athanasios -->

    <owl:NamedIndividual rdf:about="http://xworks.gr/ontologies/ccso#Mouxtaris_Athanasios">
        <rdf:type rdf:resource="http://xmlns.com/foaf/0.1/Person"/>
        <rdf:type rdf:resource="http://xworks.gr/ontologies/ccso#AcademicStaff"/>
        <rdf:type rdf:resource="http://xworks.gr/ontologies/ccso#Employee"/>
        <rdf:type rdf:resource="http://xworks.gr/ontologies/ccso#Professor"/>
        <affiliatedWith rdf:resource="http://xworks.gr/ontologies/ccso#Computers_Sciences_Department_of_University_of_Crete"/>
        <affiliatedWith rdf:resource="http://xworks.gr/ontologies/ccso#CS110s1/CS_BSc/CSD/SSE/UoC"/>
        <instructorOf rdf:resource="http://xworks.gr/ontologies/ccso#CS110s1/CS_BSc/CSD/SSE/UoC"/>
        <memberOf rdf:resource="http://xworks.gr/ontologies/ccso#Computers_Sciences_Department_of_University_of_Crete"/>
        <supervisorOf rdf:resource="http://xworks.gr/ontologies/ccso#CS110s1/CS_BSc/CSD/SSE/UoC"/>
        <worksFor rdf:resource="http://xworks.gr/ontologies/ccso#Computers_Sciences_Department_of_University_of_Crete"/>
        <schema:email rdf:datatype="http://www.w3.org/2001/XMLSchema#anyURI">mouchtar@csd.uoc.gr</schema:email>
        <foaf:firstName rdf:datatype="http://www.w3.org/2001/XMLSchema#string">Athanasios</foaf:firstName>
        <foaf:lastName rdf:datatype="http://www.w3.org/2001/XMLSchema#string">Mouxtaris</foaf:lastName>
        <eContactInfo rdf:datatype="http://www.w3.org/2001/XMLSchema#anyURI">mouchtar@csd.uoc.gr</eContactInfo>
    </owl:NamedIndividual>
    


    <!-- http://xworks.gr/ontologies/ccso#OralExam -->

    <owl:NamedIndividual rdf:about="http://xworks.gr/ontologies/ccso#OralExam">
        <rdf:type rdf:resource="http://xworks.gr/ontologies/ccso#TeachingEvaluationMethod"/>
        <methodName rdf:datatype="http://www.w3.org/2001/XMLSchema#string">OralExamination</methodName>
    </owl:NamedIndividual>
    


    <!-- http://xworks.gr/ontologies/ccso#Pachoulakis_Ioannis -->

    <owl:NamedIndividual rdf:about="http://xworks.gr/ontologies/ccso#Pachoulakis_Ioannis">
        <rdf:type rdf:resource="http://xmlns.com/foaf/0.1/Person"/>
        <rdf:type rdf:resource="http://xworks.gr/ontologies/ccso#AcademicStaff"/>
        <rdf:type rdf:resource="http://xworks.gr/ontologies/ccso#Employee"/>
        <rdf:type rdf:resource="http://xworks.gr/ontologies/ccso#Professor"/>
        <affiliatedWith rdf:resource="http://xworks.gr/ontologies/ccso#Department_of_Informatics_Engineering_of_TEI_of_Crete"/>
        <affiliatedWith rdf:resource="http://xworks.gr/ontologies/ccso#IM206s1/IM_MSc/IED/STEF/TEI"/>
        <affiliatedWith rdf:resource="http://xworks.gr/ontologies/ccso#TP10K1s2015-16/IE_BSc/IED/STEF/TEIC"/>
        <affiliatedWith rdf:resource="http://xworks.gr/ontologies/ccso#TP10K1s2016-17/IE_BSc/IED/STEF/TEIC"/>
        <affiliatedWith rdf:resource="http://xworks.gr/ontologies/ccso#TP10K1s2017-18/IE_BSc/IED/STEF/TEIC"/>
        <affiliatedWith rdf:resource="http://xworks.gr/ontologies/ccso#TP30K7s1/IE_BSc/IED/STEF/TEIC"/>
        <affiliatedWith rdf:resource="http://xworks.gr/ontologies/ccso#TP60D4s1/IE_BSc/IED/STEF/TEIC"/>
        <instructorOf rdf:resource="http://xworks.gr/ontologies/ccso#IM206s1/IM_MSc/IED/STEF/TEI"/>
        <instructorOf rdf:resource="http://xworks.gr/ontologies/ccso#TP10K1s2015-16/IE_BSc/IED/STEF/TEIC"/>
        <instructorOf rdf:resource="http://xworks.gr/ontologies/ccso#TP10K1s2016-17/IE_BSc/IED/STEF/TEIC"/>
        <instructorOf rdf:resource="http://xworks.gr/ontologies/ccso#TP30K7s1/IE_BSc/IED/STEF/TEIC"/>
        <instructorOf rdf:resource="http://xworks.gr/ontologies/ccso#TP60D4s1/IE_BSc/IED/STEF/TEIC"/>
        <memberOf rdf:resource="http://xworks.gr/ontologies/ccso#Department_of_Informatics_Engineering_of_TEI_of_Crete"/>
        <supervisorOf rdf:resource="http://xworks.gr/ontologies/ccso#IM206s1/IM_MSc/IED/STEF/TEI"/>
        <supervisorOf rdf:resource="http://xworks.gr/ontologies/ccso#TP10K1s2015-16/IE_BSc/IED/STEF/TEIC"/>
        <supervisorOf rdf:resource="http://xworks.gr/ontologies/ccso#TP10K1s2016-17/IE_BSc/IED/STEF/TEIC"/>
        <supervisorOf rdf:resource="http://xworks.gr/ontologies/ccso#TP10K1s2017-18/IE_BSc/IED/STEF/TEIC"/>
        <supervisorOf rdf:resource="http://xworks.gr/ontologies/ccso#TP30K7s1/IE_BSc/IED/STEF/TEIC"/>
        <supervisorOf rdf:resource="http://xworks.gr/ontologies/ccso#TP60D4s1/IE_BSc/IED/STEF/TEIC"/>
        <worksFor rdf:resource="http://xworks.gr/ontologies/ccso#Department_of_Informatics_Engineering_of_TEI_of_Crete"/>
        <schema:email rdf:datatype="http://www.w3.org/2001/XMLSchema#anyURI">pachoulakis@ie.teicrete.gr</schema:email>
        <foaf:firstName rdf:datatype="http://www.w3.org/2001/XMLSchema#string">Ioannis</foaf:firstName>
        <foaf:lastName rdf:datatype="http://www.w3.org/2001/XMLSchema#string">Pachoulakis</foaf:lastName>
        <eContactInfo rdf:datatype="http://www.w3.org/2001/XMLSchema#anyURI">pachoulakis@ie.teicrete.gr</eContactInfo>
    </owl:NamedIndividual>
    


    <!-- http://xworks.gr/ontologies/ccso#Palaiologou_Ifigeneia -->

    <owl:NamedIndividual rdf:about="http://xworks.gr/ontologies/ccso#Palaiologou_Ifigeneia">
        <rdf:type rdf:resource="http://xmlns.com/foaf/0.1/Agent"/>
        <rdf:type rdf:resource="http://xmlns.com/foaf/0.1/Person"/>
        <rdf:type rdf:resource="http://xworks.gr/ontologies/ccso#PostgraduateStudent"/>
        <rdf:type rdf:resource="http://xworks.gr/ontologies/ccso#Student"/>
        <affiliatedWith rdf:resource="http://xworks.gr/ontologies/ccso#Psychology_Department_of_University_of_Crete"/>
        <affiliatedWith rdf:resource="http://xworks.gr/ontologies/ccso#BSc_Psychology/PSY_BSc/SoC/UoC"/>
        <affiliatedWith rdf:resource="http://xworks.gr/ontologies/ccso#MSc_School_Psychology/SP_MSc/PSY/SoC/UoC"/>
        <alumnusOf rdf:resource="http://xworks.gr/ontologies/ccso#Psychology_Department_of_University_of_Crete"/>
        <enrolledIn rdf:resource="http://xworks.gr/ontologies/ccso#MSc_School_Psychology/SP_MSc/PSY/SoC/UoC"/>
        <hasDegree rdf:resource="http://xworks.gr/ontologies/ccso#BSc_Psychology/PSY_BSc/SoC/UoC"/>
        <schema:email rdf:datatype="http://www.w3.org/2001/XMLSchema#anyURI">Palaiologou_Ifigeneia@psy.uoc.gr</schema:email>
        <foaf:familyName rdf:datatype="http://www.w3.org/2001/XMLSchema#string">Triantafyllou</foaf:familyName>
        <foaf:firstName rdf:datatype="http://www.w3.org/2001/XMLSchema#string">Ifigeneia</foaf:firstName>
        <foaf:gender rdf:datatype="http://www.w3.org/2001/XMLSchema#string">Female</foaf:gender>
        <foaf:lastName rdf:datatype="http://www.w3.org/2001/XMLSchema#string">Palaiologou</foaf:lastName>
        <eContactInfo rdf:datatype="http://www.w3.org/2001/XMLSchema#anyURI">Palaiologou_Ifigeneia@psy.uoc.gr</eContactInfo>
    </owl:NamedIndividual>
    


    <!-- http://xworks.gr/ontologies/ccso#Pallis_Evangelos -->

    <owl:NamedIndividual rdf:about="http://xworks.gr/ontologies/ccso#Pallis_Evangelos">
        <rdf:type rdf:resource="http://xmlns.com/foaf/0.1/Person"/>
        <rdf:type rdf:resource="http://xworks.gr/ontologies/ccso#AcademicStaff"/>
        <rdf:type rdf:resource="http://xworks.gr/ontologies/ccso#Employee"/>
        <rdf:type rdf:resource="http://xworks.gr/ontologies/ccso#Professor"/>
        <affiliatedWith rdf:resource="http://xworks.gr/ontologies/ccso#Department_of_Informatics_Engineering_of_TEI_of_Crete"/>
        <affiliatedWith rdf:resource="http://xworks.gr/ontologies/ccso#IM202s1/IM_MSc/IED/STEF/TEI"/>
        <affiliatedWith rdf:resource="http://xworks.gr/ontologies/ccso#TP50D5s1/IE_BSc/IED/STEF/TEIC"/>
        <affiliatedWith rdf:resource="http://xworks.gr/ontologies/ccso#TP60D2s1/IE_BSc/IED/STEF/TEIC"/>
        <instructorOf rdf:resource="http://xworks.gr/ontologies/ccso#IM202s1/IM_MSc/IED/STEF/TEI"/>
        <instructorOf rdf:resource="http://xworks.gr/ontologies/ccso#TP50D5s1/IE_BSc/IED/STEF/TEIC"/>
        <instructorOf rdf:resource="http://xworks.gr/ontologies/ccso#TP60D2s1/IE_BSc/IED/STEF/TEIC"/>
        <memberOf rdf:resource="http://xworks.gr/ontologies/ccso#Department_of_Informatics_Engineering_of_TEI_of_Crete"/>
        <supervisorOf rdf:resource="http://xworks.gr/ontologies/ccso#IM202s1/IM_MSc/IED/STEF/TEI"/>
        <supervisorOf rdf:resource="http://xworks.gr/ontologies/ccso#TP50D5s1/IE_BSc/IED/STEF/TEIC"/>
        <supervisorOf rdf:resource="http://xworks.gr/ontologies/ccso#TP60D2s1/IE_BSc/IED/STEF/TEIC"/>
        <worksFor rdf:resource="http://xworks.gr/ontologies/ccso#Department_of_Informatics_Engineering_of_TEI_of_Crete"/>
        <schema:email rdf:datatype="http://www.w3.org/2001/XMLSchema#anyURI">pallis@ie.teicrete.gr</schema:email>
        <foaf:firstName rdf:datatype="http://www.w3.org/2001/XMLSchema#string">Evangelos</foaf:firstName>
        <foaf:lastName rdf:datatype="http://www.w3.org/2001/XMLSchema#string">Pallis</foaf:lastName>
        <eContactInfo rdf:datatype="http://www.w3.org/2001/XMLSchema#anyURI">pallis@ie.teicrete.gr</eContactInfo>
    </owl:NamedIndividual>
    


    <!-- http://xworks.gr/ontologies/ccso#Panagiotakis_Spyros -->

    <owl:NamedIndividual rdf:about="http://xworks.gr/ontologies/ccso#Panagiotakis_Spyros">
        <rdf:type rdf:resource="http://xmlns.com/foaf/0.1/Person"/>
        <rdf:type rdf:resource="http://xworks.gr/ontologies/ccso#AcademicStaff"/>
        <rdf:type rdf:resource="http://xworks.gr/ontologies/ccso#Employee"/>
        <rdf:type rdf:resource="http://xworks.gr/ontologies/ccso#Professor"/>
        <affiliatedWith rdf:resource="http://xworks.gr/ontologies/ccso#Department_of_Informatics_Engineering_of_TEI_of_Crete"/>
        <affiliatedWith rdf:resource="http://xworks.gr/ontologies/ccso#IM102s1/IM_MSc/IED/STEF/TEI"/>
        <affiliatedWith rdf:resource="http://xworks.gr/ontologies/ccso#TP20K1s1/IE_BSc/IED/STEF/TEIC"/>
        <affiliatedWith rdf:resource="http://xworks.gr/ontologies/ccso#TP40K2s1/IE_BSc/IED/STEF/TEIC"/>
        <affiliatedWith rdf:resource="http://xworks.gr/ontologies/ccso#TP50D4s1/IE_BSc/IED/STEF/TEIC"/>
        <affiliatedWith rdf:resource="http://xworks.gr/ontologies/ccso#TP70D2s1/IE_BSc/IED/STEF/TEIC"/>
        <affiliatedWith rdf:resource="http://xworks.gr/ontologies/ccso#TP70Y6s1/IE_BSc/IED/STEF/TEIC"/>
        <instructorOf rdf:resource="http://xworks.gr/ontologies/ccso#IM102s1/IM_MSc/IED/STEF/TEI"/>
        <instructorOf rdf:resource="http://xworks.gr/ontologies/ccso#TP20K1s1/IE_BSc/IED/STEF/TEIC"/>
        <instructorOf rdf:resource="http://xworks.gr/ontologies/ccso#TP40K2s1/IE_BSc/IED/STEF/TEIC"/>
        <instructorOf rdf:resource="http://xworks.gr/ontologies/ccso#TP50D4s1/IE_BSc/IED/STEF/TEIC"/>
        <instructorOf rdf:resource="http://xworks.gr/ontologies/ccso#TP70D2s1/IE_BSc/IED/STEF/TEIC"/>
        <instructorOf rdf:resource="http://xworks.gr/ontologies/ccso#TP70Y6s1/IE_BSc/IED/STEF/TEIC"/>
        <memberOf rdf:resource="http://xworks.gr/ontologies/ccso#Department_of_Informatics_Engineering_of_TEI_of_Crete"/>
        <supervisorOf rdf:resource="http://xworks.gr/ontologies/ccso#IM102s1/IM_MSc/IED/STEF/TEI"/>
        <supervisorOf rdf:resource="http://xworks.gr/ontologies/ccso#TP20K1s1/IE_BSc/IED/STEF/TEIC"/>
        <supervisorOf rdf:resource="http://xworks.gr/ontologies/ccso#TP40K2s1/IE_BSc/IED/STEF/TEIC"/>
        <supervisorOf rdf:resource="http://xworks.gr/ontologies/ccso#TP50D4s1/IE_BSc/IED/STEF/TEIC"/>
        <supervisorOf rdf:resource="http://xworks.gr/ontologies/ccso#TP70D2s1/IE_BSc/IED/STEF/TEIC"/>
        <supervisorOf rdf:resource="http://xworks.gr/ontologies/ccso#TP70Y6s1/IE_BSc/IED/STEF/TEIC"/>
        <worksFor rdf:resource="http://xworks.gr/ontologies/ccso#Department_of_Informatics_Engineering_of_TEI_of_Crete"/>
        <schema:email rdf:datatype="http://www.w3.org/2001/XMLSchema#anyURI">panagiotakis@ie.teicrete.gr</schema:email>
        <foaf:firstName rdf:datatype="http://www.w3.org/2001/XMLSchema#string">Spyros</foaf:firstName>
        <foaf:lastName rdf:datatype="http://www.w3.org/2001/XMLSchema#string">Panagiotakis</foaf:lastName>
        <eContactInfo rdf:datatype="http://www.w3.org/2001/XMLSchema#anyURI">panagiotakis@ie.teicrete.gr</eContactInfo>
    </owl:NamedIndividual>
    


    <!-- http://xworks.gr/ontologies/ccso#Panelis_Panos -->

    <owl:NamedIndividual rdf:about="http://xworks.gr/ontologies/ccso#Panelis_Panos">
        <rdf:type rdf:resource="http://xmlns.com/foaf/0.1/Person"/>
        <rdf:type rdf:resource="http://xworks.gr/ontologies/ccso#Student"/>
        <foaf:firstName rdf:datatype="http://www.w3.org/2001/XMLSchema#string">Panos</foaf:firstName>
        <foaf:lastName rdf:datatype="http://www.w3.org/2001/XMLSchema#string">Panelis</foaf:lastName>
    </owl:NamedIndividual>
    


    <!-- http://xworks.gr/ontologies/ccso#Papachristou2010EducationalModel -->

    <owl:NamedIndividual rdf:about="http://xworks.gr/ontologies/ccso#Papachristou2010EducationalModel">
        <rdf:type rdf:resource="http://xworks.gr/ontologies/ccso#Resource"/>
        <dc:creator rdf:resource="http://xworks.gr/ontologies/ccso#Kalogiannakis_Michail"/>
        <dc:creator rdf:resource="http://xworks.gr/ontologies/ccso#Vassilakis_Kostas"/>
        <dc:date rdf:datatype="http://www.w3.org/2001/XMLSchema#date">2010</dc:date>
        <dc:date rdf:datatype="internal:anonymous-constants">2010</dc:date>
        <dc:format rdf:datatype="http://www.w3.org/2001/XMLSchema#string">Text</dc:format>
        <dc:language rdf:datatype="http://www.w3.org/2001/XMLSchema#language">en</dc:language>
        <dc:source rdf:datatype="http://www.w3.org/2001/XMLSchema#string">International Journal of Advanced Corporate Learning</dc:source>
        <dc:title rdf:datatype="http://www.w3.org/2001/XMLSchema#string">An Educational Model for Asynchronous E-Learning. A Case Study in a Higher Technology Education</dc:title>
        <dc:type rdf:datatype="http://www.w3.org/2001/XMLSchema#string">Article</dc:type>
        <dates rdf:datatype="internal:anonymous-constants">2010</dates>
        <rdfs:label xml:lang="en">Papachristou, Kalogiannakis, Vassilakis (2010) An Educational Model for Asynchronous E-Learning. A Case Study in a Higher Technology Education</rdfs:label>
    </owl:NamedIndividual>
    


    <!-- http://xworks.gr/ontologies/ccso#Papadakis2014NoviceProgrammingEnvironments -->

    <owl:NamedIndividual rdf:about="http://xworks.gr/ontologies/ccso#Papadakis2014NoviceProgrammingEnvironments">
        <rdf:type rdf:resource="http://xworks.gr/ontologies/ccso#Resource"/>
        <dc:creator rdf:resource="http://xworks.gr/ontologies/ccso#Kalogiannakis_Michail"/>
        <dc:date rdf:datatype="http://www.w3.org/2001/XMLSchema#date">2014</dc:date>
        <dc:date rdf:datatype="internal:anonymous-constants">2014</dc:date>
        <dc:publisher rdf:datatype="http://www.w3.org/2001/XMLSchema#string">ACM</dc:publisher>
        <dc:source rdf:datatype="http://www.w3.org/2001/XMLSchema#string">In Proceedings of the 2014 Workshop on Interaction Design in Educational Environments</dc:source>
        <dc:title rdf:datatype="http://www.w3.org/2001/XMLSchema#string">Novice programming environments. Scratch &amp; app inventor: a first comparison</dc:title>
        <dates rdf:datatype="internal:anonymous-constants">2014</dates>
        <resourceCitation rdf:datatype="http://www.w3.org/2001/XMLSchema#string">Papadakis, Stamatios, Michail Kalogiannakis, Vasileios Orfanakis, and Nicholas Zaranis. &quot;Novice programming environments. Scratch &amp; app inventor: a first comparison.&quot; In Proceedings of the 2014 Workshop on Interaction Design in Educational Environments, p. 1. ACM, 2014.</resourceCitation>
        <rdfs:label xml:lang="en">Papadakis,Kalogiannakis,Orfanakis,Zaranis (2014) Novice Programming Environments</rdfs:label>
    </owl:NamedIndividual>
    


    <!-- http://xworks.gr/ontologies/ccso#Papadakis2017MobileEducationalApplications -->

    <owl:NamedIndividual rdf:about="http://xworks.gr/ontologies/ccso#Papadakis2017MobileEducationalApplications">
        <rdf:type rdf:resource="http://xworks.gr/ontologies/ccso#Resource"/>
        <dc:creator rdf:resource="http://xworks.gr/ontologies/ccso#Kalogiannakis_Michail"/>
        <dc:date rdf:datatype="http://www.w3.org/2001/XMLSchema#date">2017</dc:date>
        <dc:date rdf:datatype="internal:anonymous-constants">2017</dc:date>
        <dc:source rdf:datatype="http://www.w3.org/2001/XMLSchema#string">International Journal of Mobile Learning and Organisation</dc:source>
        <dc:title rdf:datatype="http://www.w3.org/2001/XMLSchema#string">Mobile educational applications for children: what educators and parents need to know</dc:title>
        <dc:type rdf:datatype="http://www.w3.org/2001/XMLSchema#string">Article</dc:type>
        <dates rdf:datatype="internal:anonymous-constants">2017</dates>
        <resourceCitation rdf:datatype="http://www.w3.org/2001/XMLSchema#string">Papadakis, Stamatios, and Michail Kalogiannakis. &quot;Mobile educational applications for children: what educators and parents need to know.&quot; International Journal of Mobile Learning and Organisation 11, no. 3 (2017): 256-277</resourceCitation>
        <rdfs:label xml:lang="en">Papadakis,Kalogiannakis (2017) Mobile Educational Applications for Children: what educators and parents need to know</rdfs:label>
    </owl:NamedIndividual>
    


    <!-- http://xworks.gr/ontologies/ccso#Papadakis_Nikos -->

    <owl:NamedIndividual rdf:about="http://xworks.gr/ontologies/ccso#Papadakis_Nikos">
        <rdf:type rdf:resource="http://www.w3.org/2000/10/swap/pim/contact#Person"/>
        <rdf:type rdf:resource="http://xmlns.com/foaf/0.1/Agent"/>
        <rdf:type rdf:resource="http://xmlns.com/foaf/0.1/Person"/>
        <rdf:type rdf:resource="http://xworks.gr/ontologies/ccso#AcademicStaff"/>
        <rdf:type rdf:resource="http://xworks.gr/ontologies/ccso#Employee"/>
        <rdf:type rdf:resource="http://xworks.gr/ontologies/ccso#Professor"/>
        <affiliatedWith rdf:resource="http://xworks.gr/ontologies/ccso#Computers_Sciences_Department_of_University_of_Crete"/>
        <affiliatedWith rdf:resource="http://xworks.gr/ontologies/ccso#Department_of_Informatics_Engineering_of_TEI_of_Crete"/>
        <affiliatedWith rdf:resource="http://xworks.gr/ontologies/ccso#BSc_Computer_Science/CS_BSc/CSD/SSE/UoC"/>
        <affiliatedWith rdf:resource="http://xworks.gr/ontologies/ccso#IM105s1/IM_MSc/IED/STEF/TEI"/>
        <affiliatedWith rdf:resource="http://xworks.gr/ontologies/ccso#MSc_Computer_Science_and_Engineering/CSE_MSc/CSD/SSE/UoC"/>
        <affiliatedWith rdf:resource="http://xworks.gr/ontologies/ccso#PhD_Computer_Science_and_Engineering/CSE_PhD/CSD/SSE/UoC"/>
        <affiliatedWith rdf:resource="http://xworks.gr/ontologies/ccso#TP10K2s1/IE_BSc/IED/STEF/TEIC"/>
        <affiliatedWith rdf:resource="http://xworks.gr/ontologies/ccso#TP50L5s1/IE_BSc/IED/STEF/TEIC"/>
        <affiliatedWith rdf:resource="http://xworks.gr/ontologies/ccso#TP50Y5s1/IE_BSc/IED/STEF/TEIC"/>
        <affiliatedWith rdf:resource="http://xworks.gr/ontologies/ccso#TP70L5s1/IE_BSc/IED/STEF/TEIC"/>
        <alumnusOf rdf:resource="http://xworks.gr/ontologies/ccso#Computers_Sciences_Department_of_University_of_Crete"/>
        <hasDegree rdf:resource="http://xworks.gr/ontologies/ccso#BSc_Computer_Science/CS_BSc/CSD/SSE/UoC"/>
        <hasDegree rdf:resource="http://xworks.gr/ontologies/ccso#MSc_Computer_Science_and_Engineering/CSE_MSc/CSD/SSE/UoC"/>
        <hasDegree rdf:resource="http://xworks.gr/ontologies/ccso#PhD_Computer_Science_and_Engineering/CSE_PhD/CSD/SSE/UoC"/>
        <hasPublication rdf:resource="http://xworks.gr/ontologies/ccso#Hatzivasilis2014ReasoningSystem"/>
        <hasPublication rdf:resource="http://xworks.gr/ontologies/ccso#Marakakis2012KnowledgeRepresentation"/>
        <instructorOf rdf:resource="http://xworks.gr/ontologies/ccso#IM105s1/IM_MSc/IED/STEF/TEI"/>
        <instructorOf rdf:resource="http://xworks.gr/ontologies/ccso#TP10K2s1/IE_BSc/IED/STEF/TEIC"/>
        <instructorOf rdf:resource="http://xworks.gr/ontologies/ccso#TP50L5s1/IE_BSc/IED/STEF/TEIC"/>
        <instructorOf rdf:resource="http://xworks.gr/ontologies/ccso#TP50Y5s1/IE_BSc/IED/STEF/TEIC"/>
        <instructorOf rdf:resource="http://xworks.gr/ontologies/ccso#TP70L5s1/IE_BSc/IED/STEF/TEIC"/>
        <memberOf rdf:resource="http://xworks.gr/ontologies/ccso#Department_of_Informatics_Engineering_of_TEI_of_Crete"/>
        <supervisorOf rdf:resource="http://xworks.gr/ontologies/ccso#IM105s1/IM_MSc/IED/STEF/TEI"/>
        <supervisorOf rdf:resource="http://xworks.gr/ontologies/ccso#TP10K2s1/IE_BSc/IED/STEF/TEIC"/>
        <supervisorOf rdf:resource="http://xworks.gr/ontologies/ccso#TP50L5s1/IE_BSc/IED/STEF/TEIC"/>
        <supervisorOf rdf:resource="http://xworks.gr/ontologies/ccso#TP50Y5s1/IE_BSc/IED/STEF/TEIC"/>
        <supervisorOf rdf:resource="http://xworks.gr/ontologies/ccso#TP70L5s1/IE_BSc/IED/STEF/TEIC"/>
        <worksFor rdf:resource="http://xworks.gr/ontologies/ccso#Department_of_Informatics_Engineering_of_TEI_of_Crete"/>
        <schema:email rdf:datatype="http://www.w3.org/2001/XMLSchema#anyURI">papadakisn@ie.teicrete.gr</schema:email>
        <foaf:firstName rdf:datatype="http://www.w3.org/2001/XMLSchema#string">Nikolaos</foaf:firstName>
        <foaf:gender rdf:datatype="http://www.w3.org/2001/XMLSchema#string">Male</foaf:gender>
        <foaf:lastName rdf:datatype="http://www.w3.org/2001/XMLSchema#string">Papadakis</foaf:lastName>
        <foaf:title rdf:datatype="http://www.w3.org/2001/XMLSchema#string">Dr</foaf:title>
        <eContactInfo rdf:datatype="http://www.w3.org/2001/XMLSchema#anyURI">papadakisn@ie.teicrete.gr</eContactInfo>
        <phone rdf:datatype="http://www.w3.org/2001/XMLSchema#string">2810379196</phone>
        <profilePic rdf:datatype="http://www.w3.org/2001/XMLSchema#anyURI">https://www.teicrete.gr/mscie/sites/teicrete.gr.mscie/files/styles/profile_pic/public/pictures/picture-65-1388084885.jpg?itok=_8dAMBI5</profilePic>
        <staffPosition rdf:datatype="http://www.w3.org/2001/XMLSchema#string">Assistant Professor</staffPosition>
        <workPhone rdf:datatype="http://www.w3.org/2001/XMLSchema#string">2810379196</workPhone>
        <rdfs:label xml:lang="en">Papadakis Nikos</rdfs:label>
    </owl:NamedIndividual>
    


    <!-- http://xworks.gr/ontologies/ccso#Papadopouli_Maria -->

    <owl:NamedIndividual rdf:about="http://xworks.gr/ontologies/ccso#Papadopouli_Maria">
        <rdf:type rdf:resource="http://xmlns.com/foaf/0.1/Person"/>
        <rdf:type rdf:resource="http://xworks.gr/ontologies/ccso#AcademicStaff"/>
        <rdf:type rdf:resource="http://xworks.gr/ontologies/ccso#Employee"/>
        <rdf:type rdf:resource="http://xworks.gr/ontologies/ccso#Professor"/>
        <affiliatedWith rdf:resource="http://xworks.gr/ontologies/ccso#Computers_Sciences_Department_of_University_of_Crete"/>
        <affiliatedWith rdf:resource="http://xworks.gr/ontologies/ccso#CS280s1/CS_BSc/CSD/SSE/UoC"/>
        <instructorOf rdf:resource="http://xworks.gr/ontologies/ccso#CS280s1/CS_BSc/CSD/SSE/UoC"/>
        <memberOf rdf:resource="http://xworks.gr/ontologies/ccso#Computers_Sciences_Department_of_University_of_Crete"/>
        <supervisorOf rdf:resource="http://xworks.gr/ontologies/ccso#CS280s1/CS_BSc/CSD/SSE/UoC"/>
        <worksFor rdf:resource="http://xworks.gr/ontologies/ccso#Computers_Sciences_Department_of_University_of_Crete"/>
        <schema:email rdf:datatype="http://www.w3.org/2001/XMLSchema#anyURI">mpap@csd.uoc.gr</schema:email>
        <foaf:firstName rdf:datatype="http://www.w3.org/2001/XMLSchema#string">Maria</foaf:firstName>
        <foaf:lastName rdf:datatype="http://www.w3.org/2001/XMLSchema#string">Papadopouli</foaf:lastName>
        <eContactInfo rdf:datatype="http://www.w3.org/2001/XMLSchema#anyURI">mpap@csd.uoc.gr</eContactInfo>
    </owl:NamedIndividual>
    


    <!-- http://xworks.gr/ontologies/ccso#Papadourakis_George -->

    <owl:NamedIndividual rdf:about="http://xworks.gr/ontologies/ccso#Papadourakis_George">
        <rdf:type rdf:resource="http://xmlns.com/foaf/0.1/Person"/>
        <rdf:type rdf:resource="http://xworks.gr/ontologies/ccso#AcademicStaff"/>
        <rdf:type rdf:resource="http://xworks.gr/ontologies/ccso#Employee"/>
        <rdf:type rdf:resource="http://xworks.gr/ontologies/ccso#Professor"/>
        <affiliatedWith rdf:resource="http://xworks.gr/ontologies/ccso#Department_of_Informatics_Engineering_of_TEI_of_Crete"/>
        <affiliatedWith rdf:resource="http://xworks.gr/ontologies/ccso#IM107s1/IM_MSc/IED/STEF/TEI"/>
        <affiliatedWith rdf:resource="http://xworks.gr/ontologies/ccso#TP10K1s2017-18/IE_BSc/IED/STEF/TEIC"/>
        <affiliatedWith rdf:resource="http://xworks.gr/ontologies/ccso#TP40K1s1/IE_BSc/IED/STEF/TEIC"/>
        <affiliatedWith rdf:resource="http://xworks.gr/ontologies/ccso#TP50Y3s1/IE_BSc/IED/STEF/TEIC"/>
        <affiliatedWith rdf:resource="http://xworks.gr/ontologies/ccso#TP50Y4s1/IE_BSc/IED/STEF/TEIC"/>
        <affiliatedWith rdf:resource="http://xworks.gr/ontologies/ccso#TP60Y1s1/IE_BSc/IED/STEF/TEIC"/>
        <instructorOf rdf:resource="http://xworks.gr/ontologies/ccso#IM107s1/IM_MSc/IED/STEF/TEI"/>
        <instructorOf rdf:resource="http://xworks.gr/ontologies/ccso#TP10K1s2017-18/IE_BSc/IED/STEF/TEIC"/>
        <instructorOf rdf:resource="http://xworks.gr/ontologies/ccso#TP40K1s1/IE_BSc/IED/STEF/TEIC"/>
        <instructorOf rdf:resource="http://xworks.gr/ontologies/ccso#TP50Y3s1/IE_BSc/IED/STEF/TEIC"/>
        <instructorOf rdf:resource="http://xworks.gr/ontologies/ccso#TP50Y4s1/IE_BSc/IED/STEF/TEIC"/>
        <instructorOf rdf:resource="http://xworks.gr/ontologies/ccso#TP60Y1s1/IE_BSc/IED/STEF/TEIC"/>
        <memberOf rdf:resource="http://xworks.gr/ontologies/ccso#Department_of_Informatics_Engineering_of_TEI_of_Crete"/>
        <supervisorOf rdf:resource="http://xworks.gr/ontologies/ccso#IM107s1/IM_MSc/IED/STEF/TEI"/>
        <supervisorOf rdf:resource="http://xworks.gr/ontologies/ccso#TP40K1s1/IE_BSc/IED/STEF/TEIC"/>
        <supervisorOf rdf:resource="http://xworks.gr/ontologies/ccso#TP50Y3s1/IE_BSc/IED/STEF/TEIC"/>
        <supervisorOf rdf:resource="http://xworks.gr/ontologies/ccso#TP50Y4s1/IE_BSc/IED/STEF/TEIC"/>
        <supervisorOf rdf:resource="http://xworks.gr/ontologies/ccso#TP60Y1s1/IE_BSc/IED/STEF/TEIC"/>
        <worksFor rdf:resource="http://xworks.gr/ontologies/ccso#Department_of_Informatics_Engineering_of_TEI_of_Crete"/>
        <schema:email rdf:datatype="http://www.w3.org/2001/XMLSchema#anyURI">papadourakis@ie.teicrete.gr</schema:email>
        <foaf:firstName rdf:datatype="http://www.w3.org/2001/XMLSchema#string">George</foaf:firstName>
        <foaf:lastName rdf:datatype="http://www.w3.org/2001/XMLSchema#string">Papadourakis</foaf:lastName>
        <eContactInfo rdf:datatype="http://www.w3.org/2001/XMLSchema#anyURI">papadourakis@ie.teicrete.gr</eContactInfo>
    </owl:NamedIndividual>
    


    <!-- http://xworks.gr/ontologies/ccso#Papastamou2008EpistimologikoiProvlimatismoi -->

    <owl:NamedIndividual rdf:about="http://xworks.gr/ontologies/ccso#Papastamou2008EpistimologikoiProvlimatismoi">
        <rdf:type rdf:resource="http://xworks.gr/ontologies/ccso#Resource"/>
        <dc:publisher rdf:datatype="http://www.w3.org/2001/XMLSchema#string">Αθήνα: Πεδίο</dc:publisher>
        <dc:title rdf:datatype="http://www.w3.org/2001/XMLSchema#string">Επιστημολογικοί προβληματισμοί και μεθοδολογικές κατευθύνσεις</dc:title>
        <resourceCitation rdf:datatype="http://www.w3.org/2001/XMLSchema#string">Παπαστάμου, Σ. (2008) Επιστημολογικοί προβληματισμοί και μεθοδολογικές κατευθύνσεις. Αθήνα:Πεδίο</resourceCitation>
        <rdfs:label xml:lang="gr">Παπαστάμου (2008) Επιστημολογικοί προβληματισμοί και μεθοδολογικές κατευθύνσεις</rdfs:label>
    </owl:NamedIndividual>
    


    <!-- http://xworks.gr/ontologies/ccso#Pappa_Pepi -->

    <owl:NamedIndividual rdf:about="http://xworks.gr/ontologies/ccso#Pappa_Pepi">
        <rdf:type rdf:resource="http://xmlns.com/foaf/0.1/Agent"/>
        <rdf:type rdf:resource="http://xmlns.com/foaf/0.1/Person"/>
        <rdf:type rdf:resource="http://xworks.gr/ontologies/ccso#Assistant"/>
        <rdf:type rdf:resource="http://xworks.gr/ontologies/ccso#Employee"/>
        <affiliatedWith rdf:resource="http://xworks.gr/ontologies/ccso#CS119s2017-18/CS_BSc/CSD/SSE/UoC"/>
        <affiliatedWith rdf:resource="http://xworks.gr/ontologies/ccso#CS120s1/CS_BSc/CSD/SSE/UoC"/>
        <affiliatedWith rdf:resource="http://xworks.gr/ontologies/ccso#CS150s1/CS_BSc/CSD/SSE/UoC"/>
        <affiliatedWith rdf:resource="http://xworks.gr/ontologies/ccso#CS335_s2017-18-L05/CS_BSc/CSD/SSE/UoC"/>
        <affiliatedWith rdf:resource="http://xworks.gr/ontologies/ccso#IM106s1/IM_MSc/IED/STEF/TEI"/>
        <assistsInCourse rdf:resource="http://xworks.gr/ontologies/ccso#CS119s2017-18/CS_BSc/CSD/SSE/UoC"/>
        <assistsInCourse rdf:resource="http://xworks.gr/ontologies/ccso#CS120s1/CS_BSc/CSD/SSE/UoC"/>
        <assistsInCourse rdf:resource="http://xworks.gr/ontologies/ccso#CS150s1/CS_BSc/CSD/SSE/UoC"/>
        <assistsInCourse rdf:resource="http://xworks.gr/ontologies/ccso#IM106s1/IM_MSc/IED/STEF/TEI"/>
        <assistsInEvent rdf:resource="http://xworks.gr/ontologies/ccso#CS335_s2017-18-L05/CS_BSc/CSD/SSE/UoC"/>
        <worksFor rdf:resource="http://xworks.gr/ontologies/ccso#Computers_Sciences_Department_of_University_of_Crete"/>
        <worksFor rdf:resource="http://xworks.gr/ontologies/ccso#Department_of_Informatics_Engineering_of_TEI_of_Crete"/>
        <schema:email rdf:datatype="http://www.w3.org/2001/XMLSchema#anyURI">ppappa@mail.gr</schema:email>
        <foaf:firstName rdf:datatype="http://www.w3.org/2001/XMLSchema#string">Pepi</foaf:firstName>
        <foaf:gender rdf:datatype="http://www.w3.org/2001/XMLSchema#string">Female</foaf:gender>
        <foaf:lastName rdf:datatype="http://www.w3.org/2001/XMLSchema#string">Pappa</foaf:lastName>
        <eContactInfo rdf:datatype="http://www.w3.org/2001/XMLSchema#anyURI">ppappa@csd.uoc.gr</eContactInfo>
        <eContactInfo rdf:datatype="http://www.w3.org/2001/XMLSchema#anyURI">ppappa@mail.gr</eContactInfo>
        <workEmail rdf:datatype="http://www.w3.org/2001/XMLSchema#anyURI">ppappa@csd.uoc.gr</workEmail>
    </owl:NamedIndividual>
    


    <!-- http://xworks.gr/ontologies/ccso#Pasta_Flora -->

    <owl:NamedIndividual rdf:about="http://xworks.gr/ontologies/ccso#Pasta_Flora">
        <rdf:type rdf:resource="http://xmlns.com/foaf/0.1/Person"/>
        <rdf:type rdf:resource="http://xworks.gr/ontologies/ccso#Assistant"/>
        <rdf:type rdf:resource="http://xworks.gr/ontologies/ccso#Employee"/>
        <affiliatedWith rdf:resource="http://xworks.gr/ontologies/ccso#CS108s1/CS_BSc/CSD/SSE/UoC"/>
        <affiliatedWith rdf:resource="http://xworks.gr/ontologies/ccso#CS109s1/CS_BSc/CSD/SSE/UoC"/>
        <affiliatedWith rdf:resource="http://xworks.gr/ontologies/ccso#CS208s1/CS_BSc/CSD/SSE/UoC"/>
        <affiliatedWith rdf:resource="http://xworks.gr/ontologies/ccso#CS255s1/CS_BSc/CSD/SSE/UoC"/>
        <assistsInCourse rdf:resource="http://xworks.gr/ontologies/ccso#CS108s1/CS_BSc/CSD/SSE/UoC"/>
        <assistsInCourse rdf:resource="http://xworks.gr/ontologies/ccso#CS109s1/CS_BSc/CSD/SSE/UoC"/>
        <assistsInCourse rdf:resource="http://xworks.gr/ontologies/ccso#CS208s1/CS_BSc/CSD/SSE/UoC"/>
        <assistsInCourse rdf:resource="http://xworks.gr/ontologies/ccso#CS255s1/CS_BSc/CSD/SSE/UoC"/>
        <worksFor rdf:resource="http://xworks.gr/ontologies/ccso#Computers_Sciences_Department_of_University_of_Crete"/>
        <schema:email rdf:datatype="http://www.w3.org/2001/XMLSchema#anyURI">pasta@mail.gr</schema:email>
        <foaf:firstName rdf:datatype="http://www.w3.org/2001/XMLSchema#string">Flora</foaf:firstName>
        <foaf:lastName rdf:datatype="http://www.w3.org/2001/XMLSchema#string">Pasta</foaf:lastName>
        <eContactInfo rdf:datatype="http://www.w3.org/2001/XMLSchema#anyURI">pasta@csd.uoc.gr</eContactInfo>
        <eContactInfo rdf:datatype="http://www.w3.org/2001/XMLSchema#anyURI">pasta@mail.gr</eContactInfo>
        <workEmail rdf:datatype="http://www.w3.org/2001/XMLSchema#anyURI">pasta@csd.uoc.gr</workEmail>
    </owl:NamedIndividual>
    


    <!-- http://xworks.gr/ontologies/ccso#Peterson2007ComputerNetworks -->

    <owl:NamedIndividual rdf:about="http://xworks.gr/ontologies/ccso#Peterson2007ComputerNetworks">
        <rdf:type rdf:resource="http://xworks.gr/ontologies/ccso#Resource"/>
        <dc:source rdf:datatype="http://www.w3.org/2001/XMLSchema#string">Book</dc:source>
        <dc:title rdf:datatype="http://www.w3.org/2001/XMLSchema#string">Computer Networks: A Systems Approach, 3rd edition</dc:title>
        <resourceCitation rdf:datatype="http://www.w3.org/2001/XMLSchema#string">Larry Peterson and Bruce Davie (2007) Computer Networks: A Systems Approach, 3rd edition</resourceCitation>
        <rdfs:label xml:lang="en">Larry Peterson and Bruce Davie (2007) Computer Networks: A Systems Approach, 3rd edition</rdfs:label>
    </owl:NamedIndividual>
    


    <!-- http://xworks.gr/ontologies/ccso#Physics -->

    <owl:NamedIndividual rdf:about="http://xworks.gr/ontologies/ccso#Physics">
        <rdf:type rdf:resource="http://xworks.gr/ontologies/ccso#Discipline"/>
        <rdf:type rdf:resource="http://xworks.gr/ontologies/ccso#FieldofStudy"/>
        <fsName rdf:datatype="http://www.w3.org/2001/XMLSchema#string">Physics</fsName>
    </owl:NamedIndividual>
    


    <!-- http://xworks.gr/ontologies/ccso#Plexousakis_Dimitris -->

    <owl:NamedIndividual rdf:about="http://xworks.gr/ontologies/ccso#Plexousakis_Dimitris">
        <rdf:type rdf:resource="http://xmlns.com/foaf/0.1/Person"/>
        <rdf:type rdf:resource="http://xworks.gr/ontologies/ccso#AcademicStaff"/>
        <rdf:type rdf:resource="http://xworks.gr/ontologies/ccso#Employee"/>
        <rdf:type rdf:resource="http://xworks.gr/ontologies/ccso#Professor"/>
        <affiliatedWith rdf:resource="http://xworks.gr/ontologies/ccso#Computers_Sciences_Department_of_University_of_Crete"/>
        <affiliatedWith rdf:resource="http://xworks.gr/ontologies/ccso#CS100s1/CS_BSc/CSD/SSE/UoC"/>
        <affiliatedWith rdf:resource="http://xworks.gr/ontologies/ccso#CS180s1/CS_BSc/CSD/SSE/UoC"/>
        <affiliatedWith rdf:resource="http://xworks.gr/ontologies/ccso#CS360s1/CS_BSc/CSD/SSE/UoC"/>
        <instructorOf rdf:resource="http://xworks.gr/ontologies/ccso#CS100s1/CS_BSc/CSD/SSE/UoC"/>
        <instructorOf rdf:resource="http://xworks.gr/ontologies/ccso#CS180s1/CS_BSc/CSD/SSE/UoC"/>
        <instructorOf rdf:resource="http://xworks.gr/ontologies/ccso#CS360s1/CS_BSc/CSD/SSE/UoC"/>
        <memberOf rdf:resource="http://xworks.gr/ontologies/ccso#Computers_Sciences_Department_of_University_of_Crete"/>
        <supervisorOf rdf:resource="http://xworks.gr/ontologies/ccso#CS180s1/CS_BSc/CSD/SSE/UoC"/>
        <supervisorOf rdf:resource="http://xworks.gr/ontologies/ccso#CS360s1/CS_BSc/CSD/SSE/UoC"/>
        <worksFor rdf:resource="http://xworks.gr/ontologies/ccso#Computers_Sciences_Department_of_University_of_Crete"/>
        <schema:email rdf:datatype="http://www.w3.org/2001/XMLSchema#anyURI">dp@csd.uoc.gr</schema:email>
        <foaf:firstName rdf:datatype="http://www.w3.org/2001/XMLSchema#string">Dimitris</foaf:firstName>
        <foaf:lastName rdf:datatype="http://www.w3.org/2001/XMLSchema#string">Plexousakis</foaf:lastName>
        <eContactInfo rdf:datatype="http://www.w3.org/2001/XMLSchema#anyURI">dp@csd.uoc.gr</eContactInfo>
    </owl:NamedIndividual>
    


    <!-- http://xworks.gr/ontologies/ccso#Political_Science -->

    <owl:NamedIndividual rdf:about="http://xworks.gr/ontologies/ccso#Political_Science">
        <rdf:type rdf:resource="http://xworks.gr/ontologies/ccso#Discipline"/>
        <rdf:type rdf:resource="http://xworks.gr/ontologies/ccso#FieldofStudy"/>
        <fsName rdf:datatype="http://www.w3.org/2001/XMLSchema#string">Political Science</fsName>
    </owl:NamedIndividual>
    


    <!-- http://xworks.gr/ontologies/ccso#Pratikakis_Polyvios -->

    <owl:NamedIndividual rdf:about="http://xworks.gr/ontologies/ccso#Pratikakis_Polyvios">
        <rdf:type rdf:resource="http://xmlns.com/foaf/0.1/Person"/>
        <rdf:type rdf:resource="http://xworks.gr/ontologies/ccso#AcademicStaff"/>
        <rdf:type rdf:resource="http://xworks.gr/ontologies/ccso#Employee"/>
        <rdf:type rdf:resource="http://xworks.gr/ontologies/ccso#Professor"/>
        <affiliatedWith rdf:resource="http://xworks.gr/ontologies/ccso#Computers_Sciences_Department_of_University_of_Crete"/>
        <affiliatedWith rdf:resource="http://xworks.gr/ontologies/ccso#CS100s1/CS_BSc/CSD/SSE/UoC"/>
        <memberOf rdf:resource="http://xworks.gr/ontologies/ccso#Computers_Sciences_Department_of_University_of_Crete"/>
        <supervisorOf rdf:resource="http://xworks.gr/ontologies/ccso#CS100s1/CS_BSc/CSD/SSE/UoC"/>
        <schema:email rdf:datatype="http://www.w3.org/2001/XMLSchema#anyURI">polyvios@ics.forth.gr</schema:email>
        <foaf:firstName rdf:datatype="http://www.w3.org/2001/XMLSchema#string">Polyvios</foaf:firstName>
        <foaf:lastName rdf:datatype="http://www.w3.org/2001/XMLSchema#string">Pratikakis</foaf:lastName>
        <eContactInfo rdf:datatype="http://www.w3.org/2001/XMLSchema#anyURI">polyvios@ics.forth.gr</eContactInfo>
    </owl:NamedIndividual>
    


    <!-- http://xworks.gr/ontologies/ccso#Project -->

    <owl:NamedIndividual rdf:about="http://xworks.gr/ontologies/ccso#Project">
        <rdf:type rdf:resource="http://xworks.gr/ontologies/ccso#TeachingEvaluationMethod"/>
        <methodName rdf:datatype="http://www.w3.org/2001/XMLSchema#string">Project</methodName>
    </owl:NamedIndividual>
    


    <!-- http://xworks.gr/ontologies/ccso#Psychology -->

    <owl:NamedIndividual rdf:about="http://xworks.gr/ontologies/ccso#Psychology">
        <rdf:type rdf:resource="http://xworks.gr/ontologies/ccso#Discipline"/>
        <rdf:type rdf:resource="http://xworks.gr/ontologies/ccso#FieldofStudy"/>
        <abbreviation rdf:datatype="http://www.w3.org/2001/XMLSchema#string">Psy</abbreviation>
        <fsName rdf:datatype="http://www.w3.org/2001/XMLSchema#string">Psychology</fsName>
    </owl:NamedIndividual>
    


    <!-- http://xworks.gr/ontologies/ccso#Psychology_Department_of_University_of_Crete -->

    <owl:NamedIndividual rdf:about="http://xworks.gr/ontologies/ccso#Psychology_Department_of_University_of_Crete">
        <rdf:type rdf:resource="http://schema.org/EducationalOrganization"/>
        <rdf:type rdf:resource="http://schema.org/Organization"/>
        <rdf:type rdf:resource="http://xmlns.com/foaf/0.1/Person"/>
        <rdf:type rdf:resource="http://xworks.gr/ontologies/ccso#AcademicStaff"/>
        <rdf:type rdf:resource="http://xworks.gr/ontologies/ccso#Department"/>
        <rdf:type rdf:resource="http://xworks.gr/ontologies/ccso#Employee"/>
        <affiliatedWith rdf:resource="http://xworks.gr/ontologies/ccso#Assarioti_Mellisandri"/>
        <affiliatedWith rdf:resource="http://xworks.gr/ontologies/ccso#Kafetsios_Konstantinos"/>
        <affiliatedWith rdf:resource="http://xworks.gr/ontologies/ccso#Lioni_Catherine"/>
        <affiliatedWith rdf:resource="http://xworks.gr/ontologies/ccso#Mourati_Ginna"/>
        <affiliatedWith rdf:resource="http://xworks.gr/ontologies/ccso#Palaiologou_Ifigeneia"/>
        <affiliatedWith rdf:resource="http://xworks.gr/ontologies/ccso#Psychology_Department_of_University_of_Crete"/>
        <affiliatedWith rdf:resource="http://xworks.gr/ontologies/ccso#Sotiriou_Sara"/>
        <affiliatedWith rdf:resource="http://xworks.gr/ontologies/ccso#Sotiropoulou_Mikela"/>
        <affiliatedWith rdf:resource="http://xworks.gr/ontologies/ccso#Starkeiou_Catherine"/>
        <affiliatedWith rdf:resource="http://xworks.gr/ontologies/ccso#Tarla_Elena"/>
        <affiliatedWith rdf:resource="http://xworks.gr/ontologies/ccso#Tsaeri_Elena"/>
        <belongsTo rdf:resource="http://xworks.gr/ontologies/ccso#School_of_Social_Sciences_of_University_of_Crete"/>
        <belongsTo rdf:resource="http://xworks.gr/ontologies/ccso#University_of_Crete"/>
        <hasAcademicStaff rdf:resource="http://xworks.gr/ontologies/ccso#Kafetsios_Konstantinos"/>
        <hasAcademicStaff rdf:resource="http://xworks.gr/ontologies/ccso#Psychology_Department_of_University_of_Crete"/>
        <hasAcademicStaff rdf:resource="http://xworks.gr/ontologies/ccso#Tsaeri_Elena"/>
        <hasAlumnus rdf:resource="http://xworks.gr/ontologies/ccso#Assarioti_Mellisandri"/>
        <hasAlumnus rdf:resource="http://xworks.gr/ontologies/ccso#Lioni_Catherine"/>
        <hasAlumnus rdf:resource="http://xworks.gr/ontologies/ccso#Mourati_Ginna"/>
        <hasAlumnus rdf:resource="http://xworks.gr/ontologies/ccso#Palaiologou_Ifigeneia"/>
        <hasAlumnus rdf:resource="http://xworks.gr/ontologies/ccso#Sotiriou_Sara"/>
        <hasAlumnus rdf:resource="http://xworks.gr/ontologies/ccso#Sotiropoulou_Mikela"/>
        <hasAlumnus rdf:resource="http://xworks.gr/ontologies/ccso#Starkeiou_Catherine"/>
        <hasAlumnus rdf:resource="http://xworks.gr/ontologies/ccso#Tarla_Elena"/>
        <hasEmployee rdf:resource="http://xworks.gr/ontologies/ccso#Kafetsios_Konstantinos"/>
        <hasEmployee rdf:resource="http://xworks.gr/ontologies/ccso#Tsaeri_Elena"/>
        <memberOf rdf:resource="http://xworks.gr/ontologies/ccso#Psychology_Department_of_University_of_Crete"/>
        <offersCourse rdf:resource="http://xworks.gr/ontologies/ccso#PSY131/CIA_MSc/Psy-Med/UoC"/>
        <offersCourse rdf:resource="http://xworks.gr/ontologies/ccso#PSY132/CIA_MSc/Psy-Med/UoC"/>
        <offersCourse rdf:resource="http://xworks.gr/ontologies/ccso#PSY1501/PSY_BSc/SoC/Uoc"/>
        <offersCourse rdf:resource="http://xworks.gr/ontologies/ccso#PSY2401/PSY_BSc/SoC/Uoc"/>
        <offersCourse rdf:resource="http://xworks.gr/ontologies/ccso#PSY3601/PSY_BSc/SoC/Uoc"/>
        <offersCourse rdf:resource="http://xworks.gr/ontologies/ccso#PSY642/CP_PhD/Psy/SoC/UoC"/>
        <providesProgram rdf:resource="http://xworks.gr/ontologies/ccso#BSc_Psychology/PSY_BSc/SoC/UoC"/>
        <providesProgram rdf:resource="http://xworks.gr/ontologies/ccso#MSc_School_Psychology/SP_MSc/PSY/SoC/UoC"/>
        <providesProgram rdf:resource="http://xworks.gr/ontologies/ccso#PhD_Clinical_Psychology/CP_PhD/Psy/SoC/UoC"/>
        <schema:address rdf:datatype="http://www.w3.org/2001/XMLSchema#string">Psychology Department
Faculty of Social Sciences
University of Crete
Gallos Campus
74100 - Rethymno</schema:address>
        <schema:email rdf:datatype="http://www.w3.org/2001/XMLSchema#anyURI">psychology_registry@uoc.gr</schema:email>
        <schema:faxNumber rdf:datatype="http://www.w3.org/2001/XMLSchema#string">+30 28310 77578</schema:faxNumber>
        <schema:identifier rdf:datatype="http://www.w3.org/2001/XMLSchema#string">PSY/SoC/UoC</schema:identifier>
        <schema:legalName rdf:datatype="http://www.w3.org/2001/XMLSchema#string">Psychology Department of University of Crete</schema:legalName>
        <schema:legalName rdf:datatype="http://www.w3.org/2001/XMLSchema#string">Τμήμα Ψυχολογίας του Πανεπιστημίου Κρήτης</schema:legalName>
        <schema:location rdf:datatype="http://www.w3.org/2001/XMLSchema#string">Gallos Campus</schema:location>
        <schema:logo rdf:datatype="http://www.w3.org/2001/XMLSchema#anyURI">http://www.psychology.uoc.gr/templates/basic/images/logo_psyxol_en.png</schema:logo>
        <schema:url rdf:datatype="http://www.w3.org/2001/XMLSchema#anyURI">http://www.psychology.uoc.gr/en/home</schema:url>
        <eContactInfo rdf:datatype="http://www.w3.org/2001/XMLSchema#anyURI">http://www.psychology.uoc.gr/en/home</eContactInfo>
        <eContactInfo rdf:datatype="http://www.w3.org/2001/XMLSchema#anyURI">psychology_registry@uoc.gr</eContactInfo>
        <phone rdf:datatype="http://www.w3.org/2001/XMLSchema#string">+30 28310 77522, 28310 77522</phone>
        <phone rdf:datatype="http://www.w3.org/2001/XMLSchema#string">+30 28310 77578</phone>
        <workPhone rdf:datatype="http://www.w3.org/2001/XMLSchema#string">+30 28310 77522, 28310 77522</workPhone>
        <rdfs:label xml:lang="en">Psychology Department | University of Crete</rdfs:label>
        <rdfs:label xml:lang="gr">Τμήμα Ψυχολογίας | Πανεπιστήμιο Κρήτης</rdfs:label>
    </owl:NamedIndividual>
    


    <!-- http://xworks.gr/ontologies/ccso#Raderis_Jim -->

    <owl:NamedIndividual rdf:about="http://xworks.gr/ontologies/ccso#Raderis_Jim">
        <rdf:type rdf:resource="http://xmlns.com/foaf/0.1/Person"/>
        <rdf:type rdf:resource="http://xworks.gr/ontologies/ccso#Student"/>
        <affiliatedWith rdf:resource="http://xworks.gr/ontologies/ccso#Department_of_Informatics_Engineering_of_TEI_of_Crete"/>
        <affiliatedWith rdf:resource="http://xworks.gr/ontologies/ccso#BSc_Informatics_Engineering/IE_BSc/IED/STEF/TEIC"/>
        <alumnusOf rdf:resource="http://xworks.gr/ontologies/ccso#Department_of_Informatics_Engineering_of_TEI_of_Crete"/>
        <hasDegree rdf:resource="http://xworks.gr/ontologies/ccso#BSc_Informatics_Engineering/IE_BSc/IED/STEF/TEIC"/>
        <schema:email rdf:datatype="http://www.w3.org/2001/XMLSchema#anyURI">Raderis_Jim@ie.teicrete.gr</schema:email>
        <foaf:firstName rdf:datatype="http://www.w3.org/2001/XMLSchema#string">Jim</foaf:firstName>
        <foaf:lastName rdf:datatype="http://www.w3.org/2001/XMLSchema#string">Raderis</foaf:lastName>
        <eContactInfo rdf:datatype="http://www.w3.org/2001/XMLSchema#anyURI">Raderis_Jim@ie.teicrete.gr</eContactInfo>
    </owl:NamedIndividual>
    


    <!-- http://xworks.gr/ontologies/ccso#Ralli_Mary -->

    <owl:NamedIndividual rdf:about="http://xworks.gr/ontologies/ccso#Ralli_Mary">
        <rdf:type rdf:resource="http://xmlns.com/foaf/0.1/Agent"/>
        <rdf:type rdf:resource="http://xmlns.com/foaf/0.1/Person"/>
        <rdf:type rdf:resource="http://xworks.gr/ontologies/ccso#Student"/>
        <rdf:type rdf:resource="http://xworks.gr/ontologies/ccso#UndergraduateStudent"/>
        <affiliatedWith rdf:resource="http://xworks.gr/ontologies/ccso#BSc_Psychology/PSY_BSc/SoC/UoC"/>
        <affiliatedWith rdf:resource="http://xworks.gr/ontologies/ccso#PSY1501/PSY_BSc/SoC/Uoc"/>
        <attendsCourse rdf:resource="http://xworks.gr/ontologies/ccso#PSY1501/PSY_BSc/SoC/Uoc"/>
        <enrolledIn rdf:resource="http://xworks.gr/ontologies/ccso#BSc_Psychology/PSY_BSc/SoC/UoC"/>
        <schema:email rdf:datatype="http://www.w3.org/2001/XMLSchema#anyURI">Ralli_Mary@psy.uoc.gr</schema:email>
        <foaf:familyName rdf:datatype="http://www.w3.org/2001/XMLSchema#string">Ralli</foaf:familyName>
        <foaf:firstName rdf:datatype="http://www.w3.org/2001/XMLSchema#string">Mary</foaf:firstName>
        <foaf:gender rdf:datatype="http://www.w3.org/2001/XMLSchema#string">Female</foaf:gender>
        <foaf:lastName rdf:datatype="http://www.w3.org/2001/XMLSchema#string">Ralli</foaf:lastName>
        <eContactInfo rdf:datatype="http://www.w3.org/2001/XMLSchema#anyURI">Ralli_Mary@psy.uoc.gr</eContactInfo>
    </owl:NamedIndividual>
    


    <!-- http://xworks.gr/ontologies/ccso#Rallis_John -->

    <owl:NamedIndividual rdf:about="http://xworks.gr/ontologies/ccso#Rallis_John">
        <rdf:type rdf:resource="http://xmlns.com/foaf/0.1/Agent"/>
        <rdf:type rdf:resource="http://xmlns.com/foaf/0.1/Person"/>
        <rdf:type rdf:resource="http://xworks.gr/ontologies/ccso#Student"/>
        <rdf:type rdf:resource="http://xworks.gr/ontologies/ccso#UndergraduateStudent"/>
        <affiliatedWith rdf:resource="http://xworks.gr/ontologies/ccso#BSc_Psychology/PSY_BSc/SoC/UoC"/>
        <affiliatedWith rdf:resource="http://xworks.gr/ontologies/ccso#PSY1501/PSY_BSc/SoC/Uoc"/>
        <attendsCourse rdf:resource="http://xworks.gr/ontologies/ccso#PSY1501/PSY_BSc/SoC/Uoc"/>
        <enrolledIn rdf:resource="http://xworks.gr/ontologies/ccso#BSc_Psychology/PSY_BSc/SoC/UoC"/>
        <schema:email rdf:datatype="http://www.w3.org/2001/XMLSchema#anyURI">Rallis_John@psy.uoc.gr</schema:email>
        <foaf:firstName rdf:datatype="http://www.w3.org/2001/XMLSchema#string">John</foaf:firstName>
        <foaf:gender rdf:datatype="http://www.w3.org/2001/XMLSchema#string">Male</foaf:gender>
        <foaf:lastName rdf:datatype="http://www.w3.org/2001/XMLSchema#string">Rallis</foaf:lastName>
        <eContactInfo rdf:datatype="http://www.w3.org/2001/XMLSchema#anyURI">Rallis_John@psy.uoc.gr</eContactInfo>
    </owl:NamedIndividual>
    


    <!-- http://xworks.gr/ontologies/ccso#Rizopoulou_Noni -->

    <owl:NamedIndividual rdf:about="http://xworks.gr/ontologies/ccso#Rizopoulou_Noni">
        <rdf:type rdf:resource="http://xmlns.com/foaf/0.1/Person"/>
        <rdf:type rdf:resource="http://xworks.gr/ontologies/ccso#AcademicStaff"/>
        <rdf:type rdf:resource="http://xworks.gr/ontologies/ccso#Employee"/>
        <rdf:type rdf:resource="http://xworks.gr/ontologies/ccso#Professor"/>
        <affiliatedWith rdf:resource="http://xworks.gr/ontologies/ccso#Computers_Sciences_Department_of_University_of_Crete"/>
        <affiliatedWith rdf:resource="http://xworks.gr/ontologies/ccso#CS108s1/CS_BSc/CSD/SSE/UoC"/>
        <affiliatedWith rdf:resource="http://xworks.gr/ontologies/ccso#CS109s1/CS_BSc/CSD/SSE/UoC"/>
        <affiliatedWith rdf:resource="http://xworks.gr/ontologies/ccso#CS208s1/CS_BSc/CSD/SSE/UoC"/>
        <affiliatedWith rdf:resource="http://xworks.gr/ontologies/ccso#CS209s1/CS_BSc/CSD/SSE/UoC"/>
        <instructorOf rdf:resource="http://xworks.gr/ontologies/ccso#CS108s1/CS_BSc/CSD/SSE/UoC"/>
        <instructorOf rdf:resource="http://xworks.gr/ontologies/ccso#CS109s1/CS_BSc/CSD/SSE/UoC"/>
        <instructorOf rdf:resource="http://xworks.gr/ontologies/ccso#CS208s1/CS_BSc/CSD/SSE/UoC"/>
        <instructorOf rdf:resource="http://xworks.gr/ontologies/ccso#CS209s1/CS_BSc/CSD/SSE/UoC"/>
        <memberOf rdf:resource="http://xworks.gr/ontologies/ccso#Computers_Sciences_Department_of_University_of_Crete"/>
        <supervisorOf rdf:resource="http://xworks.gr/ontologies/ccso#CS108s1/CS_BSc/CSD/SSE/UoC"/>
        <supervisorOf rdf:resource="http://xworks.gr/ontologies/ccso#CS109s1/CS_BSc/CSD/SSE/UoC"/>
        <supervisorOf rdf:resource="http://xworks.gr/ontologies/ccso#CS208s1/CS_BSc/CSD/SSE/UoC"/>
        <supervisorOf rdf:resource="http://xworks.gr/ontologies/ccso#CS209s1/CS_BSc/CSD/SSE/UoC"/>
        <worksFor rdf:resource="http://xworks.gr/ontologies/ccso#Computers_Sciences_Department_of_University_of_Crete"/>
        <schema:email rdf:datatype="http://www.w3.org/2001/XMLSchema#anyURI">nrizop@csd.uoc.gr</schema:email>
        <foaf:firstName rdf:datatype="http://www.w3.org/2001/XMLSchema#string">Noni</foaf:firstName>
        <foaf:lastName rdf:datatype="http://www.w3.org/2001/XMLSchema#string">Rizopoulou</foaf:lastName>
        <eContactInfo rdf:datatype="http://www.w3.org/2001/XMLSchema#anyURI">nrizop@csd.uoc.gr</eContactInfo>
    </owl:NamedIndividual>
    


    <!-- http://xworks.gr/ontologies/ccso#Sandi_Elina -->

    <owl:NamedIndividual rdf:about="http://xworks.gr/ontologies/ccso#Sandi_Elina">
        <rdf:type rdf:resource="http://xmlns.com/foaf/0.1/Agent"/>
        <rdf:type rdf:resource="http://xmlns.com/foaf/0.1/Person"/>
        <rdf:type rdf:resource="http://xworks.gr/ontologies/ccso#PostgraduateStudent"/>
        <rdf:type rdf:resource="http://xworks.gr/ontologies/ccso#Student"/>
        <affiliatedWith rdf:resource="http://xworks.gr/ontologies/ccso#Department_of_Informatics_Engineering_of_TEI_of_Crete"/>
        <affiliatedWith rdf:resource="http://xworks.gr/ontologies/ccso#BSc_Informatics_Engineering/IE_BSc/IED/STEF/TEIC"/>
        <affiliatedWith rdf:resource="http://xworks.gr/ontologies/ccso#IM101/IM_MSc/IED/STEF/TEIC"/>
        <affiliatedWith rdf:resource="http://xworks.gr/ontologies/ccso#IM105/IM_MSc/IED/STEF/TEIC"/>
        <affiliatedWith rdf:resource="http://xworks.gr/ontologies/ccso#IM106/IM_MSc/IED/STEF/TEIC"/>
        <affiliatedWith rdf:resource="http://xworks.gr/ontologies/ccso#IM108/IM_MSc/IED/STEF/TEIC"/>
        <affiliatedWith rdf:resource="http://xworks.gr/ontologies/ccso#MSc_Informatics_&amp;_Multimedia/IM_MSc/IED/STEF/TEIC"/>
        <alumnusOf rdf:resource="http://xworks.gr/ontologies/ccso#Department_of_Informatics_Engineering_of_TEI_of_Crete"/>
        <attendsCourse rdf:resource="http://xworks.gr/ontologies/ccso#IM101/IM_MSc/IED/STEF/TEIC"/>
        <attendsCourse rdf:resource="http://xworks.gr/ontologies/ccso#IM105/IM_MSc/IED/STEF/TEIC"/>
        <attendsCourse rdf:resource="http://xworks.gr/ontologies/ccso#IM106/IM_MSc/IED/STEF/TEIC"/>
        <attendsCourse rdf:resource="http://xworks.gr/ontologies/ccso#IM108/IM_MSc/IED/STEF/TEIC"/>
        <enrolledIn rdf:resource="http://xworks.gr/ontologies/ccso#MSc_Informatics_&amp;_Multimedia/IM_MSc/IED/STEF/TEIC"/>
        <hasDegree rdf:resource="http://xworks.gr/ontologies/ccso#BSc_Informatics_Engineering/IE_BSc/IED/STEF/TEIC"/>
        <schema:email rdf:datatype="http://www.w3.org/2001/XMLSchema#anyURI">Sandi_Elina@ie.teicrete.gr</schema:email>
        <foaf:familyName rdf:datatype="http://www.w3.org/2001/XMLSchema#string">Sandi</foaf:familyName>
        <foaf:firstName rdf:datatype="http://www.w3.org/2001/XMLSchema#string">Elina</foaf:firstName>
        <foaf:gender rdf:datatype="http://www.w3.org/2001/XMLSchema#string">Female</foaf:gender>
        <foaf:lastName rdf:datatype="http://www.w3.org/2001/XMLSchema#string">Sandi</foaf:lastName>
        <eContactInfo rdf:datatype="http://www.w3.org/2001/XMLSchema#anyURI">Sandi_Elina@ie.teicrete.gr</eContactInfo>
    </owl:NamedIndividual>
    


    <!-- http://xworks.gr/ontologies/ccso#Sandi_Tzina -->

    <owl:NamedIndividual rdf:about="http://xworks.gr/ontologies/ccso#Sandi_Tzina">
        <rdf:type rdf:resource="http://xmlns.com/foaf/0.1/Person"/>
        <rdf:type rdf:resource="http://xworks.gr/ontologies/ccso#Student"/>
        <foaf:familyName rdf:datatype="http://www.w3.org/2001/XMLSchema#string">Sandi</foaf:familyName>
        <foaf:firstName rdf:datatype="http://www.w3.org/2001/XMLSchema#string">Tzina</foaf:firstName>
        <foaf:lastName rdf:datatype="http://www.w3.org/2001/XMLSchema#string">Sandi</foaf:lastName>
    </owl:NamedIndividual>
    


    <!-- http://xworks.gr/ontologies/ccso#Sapsford2006TheorySocialPsychology -->

    <owl:NamedIndividual rdf:about="http://xworks.gr/ontologies/ccso#Sapsford2006TheorySocialPsychology">
        <rdf:type rdf:resource="http://xworks.gr/ontologies/ccso#Resource"/>
        <dc:date rdf:datatype="http://www.w3.org/2001/XMLSchema#date">2006</dc:date>
        <dc:date rdf:datatype="internal:anonymous-constants">2006</dc:date>
        <dc:publisher rdf:datatype="http://www.w3.org/2001/XMLSchema#string">Αθήνα: Μεταίχμιο</dc:publisher>
        <dc:title rdf:datatype="http://www.w3.org/2001/XMLSchema#string">Η Θεωρία στην Κοινωνική Ψυχολογία</dc:title>
        <dates rdf:datatype="internal:anonymous-constants">2006</dates>
        <resourceCitation rdf:datatype="http://www.w3.org/2001/XMLSchema#string">Sapsford, R., Still, A., Miel, D., Stevens, R. &amp; Wetherell, M. (2006) Η Θεωρία στην Κοινωνική Ψυχολογία. Αθήνα:Μεταίχμιο</resourceCitation>
        <rdfs:label xml:lang="gr">Sapsford, R., Still, A., Miel, D., Stevens, R. &amp; Wetherell, M. (2006) Η Θεωρία στην Κοινωνική Ψυχολογία</rdfs:label>
    </owl:NamedIndividual>
    


    <!-- http://xworks.gr/ontologies/ccso#Savidis_Anthony -->

    <owl:NamedIndividual rdf:about="http://xworks.gr/ontologies/ccso#Savidis_Anthony">
        <rdf:type rdf:resource="http://xmlns.com/foaf/0.1/Person"/>
        <rdf:type rdf:resource="http://xworks.gr/ontologies/ccso#AcademicStaff"/>
        <rdf:type rdf:resource="http://xworks.gr/ontologies/ccso#Employee"/>
        <rdf:type rdf:resource="http://xworks.gr/ontologies/ccso#Professor"/>
        <affiliatedWith rdf:resource="http://xworks.gr/ontologies/ccso#Computers_Sciences_Department_of_University_of_Crete"/>
        <affiliatedWith rdf:resource="http://xworks.gr/ontologies/ccso#CS317s1/CS_BSc/CSD/SSE/UoC"/>
        <affiliatedWith rdf:resource="http://xworks.gr/ontologies/ccso#CS340s1/CS_BSc/CSD/SSE/UoC"/>
        <affiliatedWith rdf:resource="http://xworks.gr/ontologies/ccso#CS342s1/CS_BSc/CSD/SSE/UoC"/>
        <instructorOf rdf:resource="http://xworks.gr/ontologies/ccso#CS317s1/CS_BSc/CSD/SSE/UoC"/>
        <instructorOf rdf:resource="http://xworks.gr/ontologies/ccso#CS340s1/CS_BSc/CSD/SSE/UoC"/>
        <instructorOf rdf:resource="http://xworks.gr/ontologies/ccso#CS342s1/CS_BSc/CSD/SSE/UoC"/>
        <memberOf rdf:resource="http://xworks.gr/ontologies/ccso#Computers_Sciences_Department_of_University_of_Crete"/>
        <supervisorOf rdf:resource="http://xworks.gr/ontologies/ccso#CS317s1/CS_BSc/CSD/SSE/UoC"/>
        <supervisorOf rdf:resource="http://xworks.gr/ontologies/ccso#CS340s1/CS_BSc/CSD/SSE/UoC"/>
        <supervisorOf rdf:resource="http://xworks.gr/ontologies/ccso#CS342s1/CS_BSc/CSD/SSE/UoC"/>
        <worksFor rdf:resource="http://xworks.gr/ontologies/ccso#Computers_Sciences_Department_of_University_of_Crete"/>
        <schema:email rdf:datatype="http://www.w3.org/2001/XMLSchema#anyURI">as@ics.forth.gr</schema:email>
        <foaf:firstName rdf:datatype="http://www.w3.org/2001/XMLSchema#string">Anthony</foaf:firstName>
        <foaf:lastName rdf:datatype="http://www.w3.org/2001/XMLSchema#string">Savidis</foaf:lastName>
        <eContactInfo rdf:datatype="http://www.w3.org/2001/XMLSchema#anyURI">as@ics.forth.gr</eContactInfo>
    </owl:NamedIndividual>
    


    <!-- http://xworks.gr/ontologies/ccso#School_of_Engineering_of_TEI_of_Crete -->

    <owl:NamedIndividual rdf:about="http://xworks.gr/ontologies/ccso#School_of_Engineering_of_TEI_of_Crete">
        <rdf:type rdf:resource="http://schema.org/EducationalOrganization"/>
        <rdf:type rdf:resource="http://schema.org/Organization"/>
        <rdf:type rdf:resource="http://xworks.gr/ontologies/ccso#School"/>
        <belongsTo rdf:resource="http://xworks.gr/ontologies/ccso#TEI_of_Crete"/>
        <schema:address rdf:datatype="http://www.w3.org/2001/XMLSchema#string">Technological Educational Institute (TEI) of Crete
School of Engineeering
P.O box 1939
Heraklion 71004, Crete
Greece</schema:address>
        <schema:email rdf:datatype="http://www.w3.org/2001/XMLSchema#anyURI">secrstef@staff.teicrete.gr</schema:email>
        <schema:faxNumber rdf:datatype="http://www.w3.org/2001/XMLSchema#string">2810-379830, 2810-260752</schema:faxNumber>
        <schema:identifier rdf:datatype="http://www.w3.org/2001/XMLSchema#string">STEF/TEIC</schema:identifier>
        <schema:legalName rdf:datatype="http://www.w3.org/2001/XMLSchema#string">School of Engineering of the Technological Educational Institute (TEI) of Crete</schema:legalName>
        <schema:legalName rdf:datatype="http://www.w3.org/2001/XMLSchema#string">Σχολή Μηχανικών του ΤΕΙ Κρήτης</schema:legalName>
        <schema:location rdf:datatype="http://www.w3.org/2001/XMLSchema#string">Estavromenos Heraklion</schema:location>
        <schema:url rdf:datatype="http://www.w3.org/2001/XMLSchema#anyURI">https://www.teicrete.gr/en/stef</schema:url>
        <eContactInfo rdf:datatype="http://www.w3.org/2001/XMLSchema#anyURI">https://www.teicrete.gr/en/stef</eContactInfo>
        <eContactInfo rdf:datatype="http://www.w3.org/2001/XMLSchema#anyURI">secrstef@staff.teicrete.gr</eContactInfo>
        <phone rdf:datatype="http://www.w3.org/2001/XMLSchema#string">2810 - 379710</phone>
        <phone rdf:datatype="http://www.w3.org/2001/XMLSchema#string">2810-379830, 2810-260752</phone>
        <workPhone rdf:datatype="http://www.w3.org/2001/XMLSchema#string">2810 - 379710</workPhone>
        <rdfs:label xml:lang="en">School of Engineering | TEI of Crete</rdfs:label>
    </owl:NamedIndividual>
    


    <!-- http://xworks.gr/ontologies/ccso#School_of_Sciences_and_Engineering_of_University_of_Crete -->

    <owl:NamedIndividual rdf:about="http://xworks.gr/ontologies/ccso#School_of_Sciences_and_Engineering_of_University_of_Crete">
        <rdf:type rdf:resource="http://schema.org/EducationalOrganization"/>
        <rdf:type rdf:resource="http://schema.org/Organization"/>
        <rdf:type rdf:resource="http://xworks.gr/ontologies/ccso#School"/>
        <belongsTo rdf:resource="http://xworks.gr/ontologies/ccso#University_of_Crete"/>
        <schema:address rdf:datatype="http://www.w3.org/2001/XMLSchema#string">School of Sciences and Engineering
University of Crete
Voutes Campus
70013, Heraklion
Crete</schema:address>
        <schema:email rdf:datatype="http://www.w3.org/2001/XMLSchema#anyURI">tsalimi@admin.uoc.gr</schema:email>
        <schema:faxNumber rdf:datatype="http://www.w3.org/2001/XMLSchema#string">+30 2810 393202</schema:faxNumber>
        <schema:identifier rdf:datatype="http://www.w3.org/2001/XMLSchema#string">SSE/UoC</schema:identifier>
        <schema:legalName rdf:datatype="http://www.w3.org/2001/XMLSchema#string">School of Sciences and Engineering of University of Crete</schema:legalName>
        <schema:legalName rdf:datatype="http://www.w3.org/2001/XMLSchema#string">Σχολή Θετικών και Τεχνολογικών Επιστημών του Πανεπιστημίου Κρήτης</schema:legalName>
        <schema:location rdf:datatype="http://www.w3.org/2001/XMLSchema#string">Voutes Campus</schema:location>
        <schema:url rdf:datatype="http://www.w3.org/2001/XMLSchema#anyURI">http://www.sse.uoc.gr</schema:url>
        <eContactInfo rdf:datatype="http://www.w3.org/2001/XMLSchema#anyURI">http://www.sse.uoc.gr</eContactInfo>
        <eContactInfo rdf:datatype="http://www.w3.org/2001/XMLSchema#anyURI">tsalimi@admin.uoc.gr</eContactInfo>
        <phone rdf:datatype="http://www.w3.org/2001/XMLSchema#string">+30 2810 393200</phone>
        <phone rdf:datatype="http://www.w3.org/2001/XMLSchema#string">+30 2810 393202</phone>
        <workPhone rdf:datatype="http://www.w3.org/2001/XMLSchema#string">+30 2810 393200</workPhone>
        <rdfs:label xml:lang="en">School of Sciences and Engineering | University of Crete</rdfs:label>
    </owl:NamedIndividual>
    


    <!-- http://xworks.gr/ontologies/ccso#School_of_Social_Sciences_of_University_of_Crete -->

    <owl:NamedIndividual rdf:about="http://xworks.gr/ontologies/ccso#School_of_Social_Sciences_of_University_of_Crete">
        <rdf:type rdf:resource="http://schema.org/EducationalOrganization"/>
        <rdf:type rdf:resource="http://schema.org/Organization"/>
        <rdf:type rdf:resource="http://xworks.gr/ontologies/ccso#School"/>
        <belongsTo rdf:resource="http://xworks.gr/ontologies/ccso#University_of_Crete"/>
        <schema:address rdf:datatype="http://www.w3.org/2001/XMLSchema#string">University of Crete
Faculty of Social Sciences
Dean’s Office
Gallos Campus
74100 - Rethymno</schema:address>
        <schema:email rdf:datatype="http://www.w3.org/2001/XMLSchema#anyURI">deansocial@econ.soc.uoc.gr</schema:email>
        <schema:faxNumber rdf:datatype="http://www.w3.org/2001/XMLSchema#string">+30 28310 77860</schema:faxNumber>
        <schema:identifier rdf:datatype="http://www.w3.org/2001/XMLSchema#string">SoC/UoC</schema:identifier>
        <schema:legalName rdf:datatype="http://www.w3.org/2001/XMLSchema#string">School of Social Sciences of University of Crete</schema:legalName>
        <schema:legalName rdf:datatype="http://www.w3.org/2001/XMLSchema#string">Σχολή Κοινωνικών Επιστημών του Πανεπιστημίου Κρήτης</schema:legalName>
        <schema:location rdf:datatype="http://www.w3.org/2001/XMLSchema#string">Gallos Campus</schema:location>
        <schema:logo rdf:datatype="http://www.w3.org/2001/XMLSchema#anyURI">http://www.soc.uoc.gr/wp-content/uploads/2017/04/30yearslogo.png</schema:logo>
        <schema:url rdf:datatype="http://www.w3.org/2001/XMLSchema#anyURI">http://www.soc.uoc.gr</schema:url>
        <eContactInfo rdf:datatype="http://www.w3.org/2001/XMLSchema#anyURI">deansocial@econ.soc.uoc.gr</eContactInfo>
        <eContactInfo rdf:datatype="http://www.w3.org/2001/XMLSchema#anyURI">http://www.soc.uoc.gr</eContactInfo>
        <phone rdf:datatype="http://www.w3.org/2001/XMLSchema#string">+30 28310 77860</phone>
        <phone rdf:datatype="http://www.w3.org/2001/XMLSchema#string">+30 28310 77861</phone>
        <workPhone rdf:datatype="http://www.w3.org/2001/XMLSchema#string">+30 28310 77861</workPhone>
        <rdfs:label xml:lang="en">School of Social Sciences | University of Crete</rdfs:label>
    </owl:NamedIndividual>
    


    <!-- http://xworks.gr/ontologies/ccso#Seakis_Dimitris -->

    <owl:NamedIndividual rdf:about="http://xworks.gr/ontologies/ccso#Seakis_Dimitris">
        <rdf:type rdf:resource="http://xmlns.com/foaf/0.1/Agent"/>
        <rdf:type rdf:resource="http://xmlns.com/foaf/0.1/Person"/>
        <rdf:type rdf:resource="http://xworks.gr/ontologies/ccso#Student"/>
        <schema:email rdf:datatype="http://www.w3.org/2001/XMLSchema#anyURI">Seakis_Dimitris@mail.gr</schema:email>
        <foaf:familyName rdf:datatype="http://www.w3.org/2001/XMLSchema#string">Seakis</foaf:familyName>
        <foaf:firstName rdf:datatype="http://www.w3.org/2001/XMLSchema#string">Davos</foaf:firstName>
        <foaf:gender rdf:datatype="http://www.w3.org/2001/XMLSchema#string">Male</foaf:gender>
        <foaf:lastName rdf:datatype="http://www.w3.org/2001/XMLSchema#string">Seakis</foaf:lastName>
        <eContactInfo rdf:datatype="http://www.w3.org/2001/XMLSchema#anyURI">Seakis_Dimitris@mail.gr</eContactInfo>
    </owl:NamedIndividual>
    


    <!-- http://xworks.gr/ontologies/ccso#Seminar -->

    <owl:NamedIndividual rdf:about="http://xworks.gr/ontologies/ccso#Seminar">
        <rdf:type rdf:resource="http://xworks.gr/ontologies/ccso#TeachingEvaluationMethod"/>
        <methodName rdf:datatype="http://www.w3.org/2001/XMLSchema#string">Seminar</methodName>
    </owl:NamedIndividual>
    


    <!-- http://xworks.gr/ontologies/ccso#Sociology -->

    <owl:NamedIndividual rdf:about="http://xworks.gr/ontologies/ccso#Sociology">
        <rdf:type rdf:resource="http://xworks.gr/ontologies/ccso#Discipline"/>
        <rdf:type rdf:resource="http://xworks.gr/ontologies/ccso#FieldofStudy"/>
        <abbreviation rdf:datatype="http://www.w3.org/2001/XMLSchema#string">Soc</abbreviation>
        <fsName rdf:datatype="http://www.w3.org/2001/XMLSchema#string">Sociology</fsName>
    </owl:NamedIndividual>
    


    <!-- http://xworks.gr/ontologies/ccso#Sotiriou_Sara -->

    <owl:NamedIndividual rdf:about="http://xworks.gr/ontologies/ccso#Sotiriou_Sara">
        <rdf:type rdf:resource="http://xmlns.com/foaf/0.1/Agent"/>
        <rdf:type rdf:resource="http://xmlns.com/foaf/0.1/Person"/>
        <rdf:type rdf:resource="http://xworks.gr/ontologies/ccso#Student"/>
        <affiliatedWith rdf:resource="http://xworks.gr/ontologies/ccso#Psychology_Department_of_University_of_Crete"/>
        <affiliatedWith rdf:resource="http://xworks.gr/ontologies/ccso#BSc_Psychology/PSY_BSc/SoC/UoC"/>
        <affiliatedWith rdf:resource="http://xworks.gr/ontologies/ccso#MSc_School_Psychology/SP_MSc/PSY/SoC/UoC"/>
        <alumnusOf rdf:resource="http://xworks.gr/ontologies/ccso#Psychology_Department_of_University_of_Crete"/>
        <hasDegree rdf:resource="http://xworks.gr/ontologies/ccso#BSc_Psychology/PSY_BSc/SoC/UoC"/>
        <hasDegree rdf:resource="http://xworks.gr/ontologies/ccso#MSc_School_Psychology/SP_MSc/PSY/SoC/UoC"/>
        <schema:email rdf:datatype="http://www.w3.org/2001/XMLSchema#anyURI">Sotiriou_Sara@psy.uoc.gr</schema:email>
        <foaf:firstName rdf:datatype="http://www.w3.org/2001/XMLSchema#string">Sara</foaf:firstName>
        <foaf:gender rdf:datatype="http://www.w3.org/2001/XMLSchema#string">Female</foaf:gender>
        <foaf:lastName rdf:datatype="http://www.w3.org/2001/XMLSchema#string">Sotiriou</foaf:lastName>
        <eContactInfo rdf:datatype="http://www.w3.org/2001/XMLSchema#anyURI">Sotiriou_Sara@psy.uoc.gr</eContactInfo>
    </owl:NamedIndividual>
    


    <!-- http://xworks.gr/ontologies/ccso#Sotiropoulou_Mikela -->

    <owl:NamedIndividual rdf:about="http://xworks.gr/ontologies/ccso#Sotiropoulou_Mikela">
        <rdf:type rdf:resource="http://xmlns.com/foaf/0.1/Agent"/>
        <rdf:type rdf:resource="http://xmlns.com/foaf/0.1/Person"/>
        <rdf:type rdf:resource="http://xworks.gr/ontologies/ccso#Student"/>
        <affiliatedWith rdf:resource="http://xworks.gr/ontologies/ccso#Psychology_Department_of_University_of_Crete"/>
        <affiliatedWith rdf:resource="http://xworks.gr/ontologies/ccso#BSc_Psychology/PSY_BSc/SoC/UoC"/>
        <affiliatedWith rdf:resource="http://xworks.gr/ontologies/ccso#PSY131/CIA_MSc/Psy-Med/UoC"/>
        <affiliatedWith rdf:resource="http://xworks.gr/ontologies/ccso#PSY132/CIA_MSc/Psy-Med/UoC"/>
        <alumnusOf rdf:resource="http://xworks.gr/ontologies/ccso#Psychology_Department_of_University_of_Crete"/>
        <attendsCourse rdf:resource="http://xworks.gr/ontologies/ccso#PSY132/CIA_MSc/Psy-Med/UoC"/>
        <hasCompleted rdf:resource="http://xworks.gr/ontologies/ccso#PSY131/CIA_MSc/Psy-Med/UoC"/>
        <hasDegree rdf:resource="http://xworks.gr/ontologies/ccso#BSc_Psychology/PSY_BSc/SoC/UoC"/>
        <schema:email rdf:datatype="http://www.w3.org/2001/XMLSchema#anyURI">Sotiropoulou_Mikela@psy.uoc.gr</schema:email>
        <foaf:firstName rdf:datatype="http://www.w3.org/2001/XMLSchema#string">Mikela</foaf:firstName>
        <foaf:gender rdf:datatype="http://www.w3.org/2001/XMLSchema#string">Female</foaf:gender>
        <foaf:lastName rdf:datatype="http://www.w3.org/2001/XMLSchema#string">Sotiropoulou</foaf:lastName>
        <eContactInfo rdf:datatype="http://www.w3.org/2001/XMLSchema#anyURI">Sotiropoulou_Mikela@psy.uoc.gr</eContactInfo>
    </owl:NamedIndividual>
    


    <!-- http://xworks.gr/ontologies/ccso#Space_Sciences -->

    <owl:NamedIndividual rdf:about="http://xworks.gr/ontologies/ccso#Space_Sciences">
        <rdf:type rdf:resource="http://xworks.gr/ontologies/ccso#Discipline"/>
        <rdf:type rdf:resource="http://xworks.gr/ontologies/ccso#FieldofStudy"/>
        <fsName rdf:datatype="http://www.w3.org/2001/XMLSchema#string">Space Sciences</fsName>
    </owl:NamedIndividual>
    


    <!-- http://xworks.gr/ontologies/ccso#Starkeiou_Alexandros -->

    <owl:NamedIndividual rdf:about="http://xworks.gr/ontologies/ccso#Starkeiou_Alexandros">
        <rdf:type rdf:resource="http://xmlns.com/foaf/0.1/Agent"/>
        <rdf:type rdf:resource="http://xmlns.com/foaf/0.1/Person"/>
        <rdf:type rdf:resource="http://xworks.gr/ontologies/ccso#PostgraduateStudent"/>
        <rdf:type rdf:resource="http://xworks.gr/ontologies/ccso#Student"/>
        <affiliatedWith rdf:resource="http://xworks.gr/ontologies/ccso#Department_of_Informatics_Engineering_of_TEI_of_Crete"/>
        <affiliatedWith rdf:resource="http://xworks.gr/ontologies/ccso#BSc_Informatics_Engineering/IE_BSc/IED/STEF/TEIC"/>
        <affiliatedWith rdf:resource="http://xworks.gr/ontologies/ccso#MSc_Informatics_&amp;_Multimedia/IM_MSc/IED/STEF/TEIC"/>
        <alumnusOf rdf:resource="http://xworks.gr/ontologies/ccso#Department_of_Informatics_Engineering_of_TEI_of_Crete"/>
        <enrolledIn rdf:resource="http://xworks.gr/ontologies/ccso#MSc_Informatics_&amp;_Multimedia/IM_MSc/IED/STEF/TEIC"/>
        <hasDegree rdf:resource="http://xworks.gr/ontologies/ccso#BSc_Informatics_Engineering/IE_BSc/IED/STEF/TEIC"/>
        <schema:email rdf:datatype="http://www.w3.org/2001/XMLSchema#anyURI">Starkeiou_Alexandros@ie.teicrete.gr</schema:email>
        <foaf:familyName rdf:datatype="http://www.w3.org/2001/XMLSchema#string">Starkeiou</foaf:familyName>
        <foaf:firstName rdf:datatype="http://www.w3.org/2001/XMLSchema#string">Alexandros</foaf:firstName>
        <foaf:gender rdf:datatype="http://www.w3.org/2001/XMLSchema#string">Male</foaf:gender>
        <foaf:lastName rdf:datatype="http://www.w3.org/2001/XMLSchema#string">Starkeiou</foaf:lastName>
        <eContactInfo rdf:datatype="http://www.w3.org/2001/XMLSchema#anyURI">Starkeiou_Alexandros@ie.teicrete.gr</eContactInfo>
    </owl:NamedIndividual>
    


    <!-- http://xworks.gr/ontologies/ccso#Starkeiou_Aria -->

    <owl:NamedIndividual rdf:about="http://xworks.gr/ontologies/ccso#Starkeiou_Aria">
        <rdf:type rdf:resource="http://xmlns.com/foaf/0.1/Agent"/>
        <rdf:type rdf:resource="http://xmlns.com/foaf/0.1/Person"/>
        <rdf:type rdf:resource="http://xworks.gr/ontologies/ccso#PostgraduateStudent"/>
        <rdf:type rdf:resource="http://xworks.gr/ontologies/ccso#Student"/>
        <affiliatedWith rdf:resource="http://xworks.gr/ontologies/ccso#Department_of_Informatics_Engineering_of_TEI_of_Crete"/>
        <affiliatedWith rdf:resource="http://xworks.gr/ontologies/ccso#BSc_Informatics_Engineering/IE_BSc/IED/STEF/TEIC"/>
        <affiliatedWith rdf:resource="http://xworks.gr/ontologies/ccso#IM101/IM_MSc/IED/STEF/TEIC"/>
        <affiliatedWith rdf:resource="http://xworks.gr/ontologies/ccso#IM104/IM_MSc/IED/STEF/TEIC"/>
        <affiliatedWith rdf:resource="http://xworks.gr/ontologies/ccso#IM109/IM_MSc/IED/STEF/TEIC"/>
        <affiliatedWith rdf:resource="http://xworks.gr/ontologies/ccso#IM201/IM_MSc/IED/STEF/TEIC"/>
        <affiliatedWith rdf:resource="http://xworks.gr/ontologies/ccso#IM205/IM_MSc/IED/STEF/TEIC"/>
        <affiliatedWith rdf:resource="http://xworks.gr/ontologies/ccso#IM209/IM_MSc/IED/STEF/TEIC"/>
        <affiliatedWith rdf:resource="http://xworks.gr/ontologies/ccso#MSc_Informatics_&amp;_Multimedia/IM_MSc/IED/STEF/TEIC"/>
        <alumnusOf rdf:resource="http://xworks.gr/ontologies/ccso#Department_of_Informatics_Engineering_of_TEI_of_Crete"/>
        <attendsCourse rdf:resource="http://xworks.gr/ontologies/ccso#IM201/IM_MSc/IED/STEF/TEIC"/>
        <attendsCourse rdf:resource="http://xworks.gr/ontologies/ccso#IM205/IM_MSc/IED/STEF/TEIC"/>
        <attendsCourse rdf:resource="http://xworks.gr/ontologies/ccso#IM209/IM_MSc/IED/STEF/TEIC"/>
        <enrolledIn rdf:resource="http://xworks.gr/ontologies/ccso#MSc_Informatics_&amp;_Multimedia/IM_MSc/IED/STEF/TEIC"/>
        <hasCompleted rdf:resource="http://xworks.gr/ontologies/ccso#IM101/IM_MSc/IED/STEF/TEIC"/>
        <hasCompleted rdf:resource="http://xworks.gr/ontologies/ccso#IM104/IM_MSc/IED/STEF/TEIC"/>
        <hasCompleted rdf:resource="http://xworks.gr/ontologies/ccso#IM109/IM_MSc/IED/STEF/TEIC"/>
        <hasDegree rdf:resource="http://xworks.gr/ontologies/ccso#BSc_Informatics_Engineering/IE_BSc/IED/STEF/TEIC"/>
        <schema:email rdf:datatype="http://www.w3.org/2001/XMLSchema#anyURI">Starkeiou_Aria@edu.teicrete.gr</schema:email>
        <foaf:firstName rdf:datatype="http://www.w3.org/2001/XMLSchema#string">Aria</foaf:firstName>
        <foaf:gender rdf:datatype="http://www.w3.org/2001/XMLSchema#string">Female</foaf:gender>
        <foaf:lastName rdf:datatype="http://www.w3.org/2001/XMLSchema#string">Starkeiou</foaf:lastName>
        <eContactInfo rdf:datatype="http://www.w3.org/2001/XMLSchema#anyURI">Starkeiou_Aria@edu.teicrete.gr</eContactInfo>
    </owl:NamedIndividual>
    


    <!-- http://xworks.gr/ontologies/ccso#Starkeiou_Catherine -->

    <owl:NamedIndividual rdf:about="http://xworks.gr/ontologies/ccso#Starkeiou_Catherine">
        <rdf:type rdf:resource="http://xmlns.com/foaf/0.1/Person"/>
        <rdf:type rdf:resource="http://xworks.gr/ontologies/ccso#Student"/>
        <affiliatedWith rdf:resource="http://xworks.gr/ontologies/ccso#Psychology_Department_of_University_of_Crete"/>
        <affiliatedWith rdf:resource="http://xworks.gr/ontologies/ccso#BSc_Psychology/PSY_BSc/SoC/UoC"/>
        <affiliatedWith rdf:resource="http://xworks.gr/ontologies/ccso#MSc_School_Psychology/SP_MSc/PSY/SoC/UoC"/>
        <affiliatedWith rdf:resource="http://xworks.gr/ontologies/ccso#PhD_Clinical_Psychology/CP_PhD/Psy/SoC/UoC"/>
        <alumnusOf rdf:resource="http://xworks.gr/ontologies/ccso#Psychology_Department_of_University_of_Crete"/>
        <hasDegree rdf:resource="http://xworks.gr/ontologies/ccso#BSc_Psychology/PSY_BSc/SoC/UoC"/>
        <hasDegree rdf:resource="http://xworks.gr/ontologies/ccso#MSc_School_Psychology/SP_MSc/PSY/SoC/UoC"/>
        <hasDegree rdf:resource="http://xworks.gr/ontologies/ccso#PhD_Clinical_Psychology/CP_PhD/Psy/SoC/UoC"/>
        <schema:email rdf:datatype="http://www.w3.org/2001/XMLSchema#anyURI">Starkeiou_Catherine@psy.uoc.gr</schema:email>
        <foaf:familyName rdf:datatype="http://www.w3.org/2001/XMLSchema#string">Starkeiou</foaf:familyName>
        <foaf:firstName rdf:datatype="http://www.w3.org/2001/XMLSchema#string">Catherine</foaf:firstName>
        <foaf:lastName rdf:datatype="http://www.w3.org/2001/XMLSchema#string">Starkeiou</foaf:lastName>
        <eContactInfo rdf:datatype="http://www.w3.org/2001/XMLSchema#anyURI">Starkeiou_Catherine@psy.uoc.gr</eContactInfo>
    </owl:NamedIndividual>
    


    <!-- http://xworks.gr/ontologies/ccso#Starkeiou_Michael -->

    <owl:NamedIndividual rdf:about="http://xworks.gr/ontologies/ccso#Starkeiou_Michael">
        <rdf:type rdf:resource="http://xmlns.com/foaf/0.1/Agent"/>
        <rdf:type rdf:resource="http://xmlns.com/foaf/0.1/Person"/>
        <rdf:type rdf:resource="http://xworks.gr/ontologies/ccso#Student"/>
        <affiliatedWith rdf:resource="http://xworks.gr/ontologies/ccso#Computers_Sciences_Department_of_University_of_Crete"/>
        <affiliatedWith rdf:resource="http://xworks.gr/ontologies/ccso#BSc_Computer_Science/CS_BSc/CSD/SSE/UoC"/>
        <affiliatedWith rdf:resource="http://xworks.gr/ontologies/ccso#MSc_Computer_Science_and_Engineering/CSE_MSc/CSD/SSE/UoC"/>
        <affiliatedWith rdf:resource="http://xworks.gr/ontologies/ccso#PhD_Computer_Science_and_Engineering/CSE_PhD/CSD/SSE/UoC"/>
        <alumnusOf rdf:resource="http://xworks.gr/ontologies/ccso#Computers_Sciences_Department_of_University_of_Crete"/>
        <enrolledIn rdf:resource="http://xworks.gr/ontologies/ccso#PhD_Computer_Science_and_Engineering/CSE_PhD/CSD/SSE/UoC"/>
        <hasDegree rdf:resource="http://xworks.gr/ontologies/ccso#BSc_Computer_Science/CS_BSc/CSD/SSE/UoC"/>
        <hasDegree rdf:resource="http://xworks.gr/ontologies/ccso#MSc_Computer_Science_and_Engineering/CSE_MSc/CSD/SSE/UoC"/>
        <schema:email rdf:datatype="http://www.w3.org/2001/XMLSchema#anyURI">Starkeiou_Michael@csd.uoc.gr</schema:email>
        <foaf:familyName rdf:datatype="http://www.w3.org/2001/XMLSchema#string">Starkeiou</foaf:familyName>
        <foaf:firstName rdf:datatype="http://www.w3.org/2001/XMLSchema#string">Michael</foaf:firstName>
        <foaf:gender rdf:datatype="http://www.w3.org/2001/XMLSchema#string">Male</foaf:gender>
        <foaf:lastName rdf:datatype="http://www.w3.org/2001/XMLSchema#string">Starkeiou</foaf:lastName>
        <eContactInfo rdf:datatype="http://www.w3.org/2001/XMLSchema#anyURI">Starkeiou_Michael@csd.uoc.gr</eContactInfo>
    </owl:NamedIndividual>
    


    <!-- http://xworks.gr/ontologies/ccso#Starkeiou_Nick -->

    <owl:NamedIndividual rdf:about="http://xworks.gr/ontologies/ccso#Starkeiou_Nick">
        <rdf:type rdf:resource="http://xmlns.com/foaf/0.1/Person"/>
        <rdf:type rdf:resource="http://xworks.gr/ontologies/ccso#Student"/>
        <rdf:type rdf:resource="http://xworks.gr/ontologies/ccso#UndergraduateStudent"/>
        <affiliatedWith rdf:resource="http://xworks.gr/ontologies/ccso#BSc_Computer_Science/CS_BSc/CSD/SSE/UoC"/>
        <affiliatedWith rdf:resource="http://xworks.gr/ontologies/ccso#CS100/CS_BSc/CSD/SSE/UoC"/>
        <affiliatedWith rdf:resource="http://xworks.gr/ontologies/ccso#CS108/CS_BSc/CSD/SSE/UoC"/>
        <affiliatedWith rdf:resource="http://xworks.gr/ontologies/ccso#CS109/CS_BSc/CSD/SSE/UoC"/>
        <affiliatedWith rdf:resource="http://xworks.gr/ontologies/ccso#CS110/CS_BSc/CSD/SSE/UoC"/>
        <affiliatedWith rdf:resource="http://xworks.gr/ontologies/ccso#CS120/CS_BSc/CSD/SSE/UoC"/>
        <affiliatedWith rdf:resource="http://xworks.gr/ontologies/ccso#CS150/CS_BSc/CSD/SSE/UoC"/>
        <attendsCourse rdf:resource="http://xworks.gr/ontologies/ccso#CS109/CS_BSc/CSD/SSE/UoC"/>
        <attendsCourse rdf:resource="http://xworks.gr/ontologies/ccso#CS110/CS_BSc/CSD/SSE/UoC"/>
        <attendsCourse rdf:resource="http://xworks.gr/ontologies/ccso#CS150/CS_BSc/CSD/SSE/UoC"/>
        <enrolledIn rdf:resource="http://xworks.gr/ontologies/ccso#BSc_Computer_Science/CS_BSc/CSD/SSE/UoC"/>
        <hasCompleted rdf:resource="http://xworks.gr/ontologies/ccso#CS100/CS_BSc/CSD/SSE/UoC"/>
        <hasCompleted rdf:resource="http://xworks.gr/ontologies/ccso#CS108/CS_BSc/CSD/SSE/UoC"/>
        <hasCompleted rdf:resource="http://xworks.gr/ontologies/ccso#CS120/CS_BSc/CSD/SSE/UoC"/>
        <schema:email rdf:datatype="http://www.w3.org/2001/XMLSchema#anyURI">Starkeiou_Nick@csd.uoc.gr</schema:email>
        <foaf:familyName rdf:datatype="http://www.w3.org/2001/XMLSchema#string">Starkeiou</foaf:familyName>
        <foaf:firstName rdf:datatype="http://www.w3.org/2001/XMLSchema#string">Nick</foaf:firstName>
        <foaf:lastName rdf:datatype="http://www.w3.org/2001/XMLSchema#string">Starkeiou</foaf:lastName>
        <eContactInfo rdf:datatype="http://www.w3.org/2001/XMLSchema#anyURI">Starkeiou_Nick@csd.uoc.gr</eContactInfo>
    </owl:NamedIndividual>
    


    <!-- http://xworks.gr/ontologies/ccso#Starkeiou_Vakis -->

    <owl:NamedIndividual rdf:about="http://xworks.gr/ontologies/ccso#Starkeiou_Vakis">
        <rdf:type rdf:resource="http://xmlns.com/foaf/0.1/Agent"/>
        <rdf:type rdf:resource="http://xmlns.com/foaf/0.1/Person"/>
        <rdf:type rdf:resource="http://xworks.gr/ontologies/ccso#Student"/>
        <rdf:type rdf:resource="http://xworks.gr/ontologies/ccso#UndergraduateStudent"/>
        <affiliatedWith rdf:resource="http://xworks.gr/ontologies/ccso#BSc_Computer_Science/CS_BSc/CSD/SSE/UoC"/>
        <affiliatedWith rdf:resource="http://xworks.gr/ontologies/ccso#CS100/CS_BSc/CSD/SSE/UoC"/>
        <affiliatedWith rdf:resource="http://xworks.gr/ontologies/ccso#CS108/CS_BSc/CSD/SSE/UoC"/>
        <affiliatedWith rdf:resource="http://xworks.gr/ontologies/ccso#CS109/CS_BSc/CSD/SSE/UoC"/>
        <affiliatedWith rdf:resource="http://xworks.gr/ontologies/ccso#CS110/CS_BSc/CSD/SSE/UoC"/>
        <affiliatedWith rdf:resource="http://xworks.gr/ontologies/ccso#CS118/CS_BSc/CSD/SSE/UoC"/>
        <affiliatedWith rdf:resource="http://xworks.gr/ontologies/ccso#CS119/CS_BSc/CSD/SSE/UoC"/>
        <affiliatedWith rdf:resource="http://xworks.gr/ontologies/ccso#CS120/CS_BSc/CSD/SSE/UoC"/>
        <affiliatedWith rdf:resource="http://xworks.gr/ontologies/ccso#CS150/CS_BSc/CSD/SSE/UoC"/>
        <affiliatedWith rdf:resource="http://xworks.gr/ontologies/ccso#CS180/CS_BSc/CSD/SSE/UoC"/>
        <attendsCourse rdf:resource="http://xworks.gr/ontologies/ccso#CS109/CS_BSc/CSD/SSE/UoC"/>
        <attendsCourse rdf:resource="http://xworks.gr/ontologies/ccso#CS118/CS_BSc/CSD/SSE/UoC"/>
        <attendsCourse rdf:resource="http://xworks.gr/ontologies/ccso#CS120/CS_BSc/CSD/SSE/UoC"/>
        <attendsCourse rdf:resource="http://xworks.gr/ontologies/ccso#CS180/CS_BSc/CSD/SSE/UoC"/>
        <enrolledIn rdf:resource="http://xworks.gr/ontologies/ccso#BSc_Computer_Science/CS_BSc/CSD/SSE/UoC"/>
        <hasCompleted rdf:resource="http://xworks.gr/ontologies/ccso#CS100/CS_BSc/CSD/SSE/UoC"/>
        <hasCompleted rdf:resource="http://xworks.gr/ontologies/ccso#CS108/CS_BSc/CSD/SSE/UoC"/>
        <hasCompleted rdf:resource="http://xworks.gr/ontologies/ccso#CS110/CS_BSc/CSD/SSE/UoC"/>
        <hasCompleted rdf:resource="http://xworks.gr/ontologies/ccso#CS119/CS_BSc/CSD/SSE/UoC"/>
        <hasCompleted rdf:resource="http://xworks.gr/ontologies/ccso#CS150/CS_BSc/CSD/SSE/UoC"/>
        <schema:email rdf:datatype="http://www.w3.org/2001/XMLSchema#anyURI">Starkeiou_Vakis@csd.uoc.gr</schema:email>
        <foaf:familyName rdf:datatype="http://www.w3.org/2001/XMLSchema#string">Starkeiou</foaf:familyName>
        <foaf:firstName rdf:datatype="http://www.w3.org/2001/XMLSchema#string">Vakis</foaf:firstName>
        <foaf:gender rdf:datatype="http://www.w3.org/2001/XMLSchema#string">Male</foaf:gender>
        <foaf:lastName rdf:datatype="http://www.w3.org/2001/XMLSchema#string">Lykas</foaf:lastName>
        <eContactInfo rdf:datatype="http://www.w3.org/2001/XMLSchema#anyURI">Starkeiou_Vakis@csd.uoc.gr</eContactInfo>
    </owl:NamedIndividual>
    


    <!-- http://xworks.gr/ontologies/ccso#Statistics -->

    <owl:NamedIndividual rdf:about="http://xworks.gr/ontologies/ccso#Statistics">
        <rdf:type rdf:resource="http://xworks.gr/ontologies/ccso#Discipline"/>
        <rdf:type rdf:resource="http://xworks.gr/ontologies/ccso#FieldofStudy"/>
        <abbreviation rdf:datatype="http://www.w3.org/2001/XMLSchema#string">Stats</abbreviation>
        <fsName rdf:datatype="http://www.w3.org/2001/XMLSchema#string">Statistics</fsName>
    </owl:NamedIndividual>
    


    <!-- http://xworks.gr/ontologies/ccso#Stratakis_Dimitrios -->

    <owl:NamedIndividual rdf:about="http://xworks.gr/ontologies/ccso#Stratakis_Dimitrios">
        <rdf:type rdf:resource="http://xmlns.com/foaf/0.1/Person"/>
        <rdf:type rdf:resource="http://xworks.gr/ontologies/ccso#AcademicStaff"/>
        <rdf:type rdf:resource="http://xworks.gr/ontologies/ccso#Employee"/>
        <rdf:type rdf:resource="http://xworks.gr/ontologies/ccso#Professor"/>
        <affiliatedWith rdf:resource="http://xworks.gr/ontologies/ccso#Department_of_Informatics_Engineering_of_TEI_of_Crete"/>
        <affiliatedWith rdf:resource="http://xworks.gr/ontologies/ccso#IM203s1/IM_MSc/IED/STEF/TEI"/>
        <affiliatedWith rdf:resource="http://xworks.gr/ontologies/ccso#TP20K3s1/IE_BSc/IED/STEF/TEIC"/>
        <affiliatedWith rdf:resource="http://xworks.gr/ontologies/ccso#TP50D2s1/IE_BSc/IED/STEF/TEIC"/>
        <affiliatedWith rdf:resource="http://xworks.gr/ontologies/ccso#TP50D6s1/IE_BSc/IED/STEF/TEIC"/>
        <affiliatedWith rdf:resource="http://xworks.gr/ontologies/ccso#TP70D1s1/IE_BSc/IED/STEF/TEIC"/>
        <instructorOf rdf:resource="http://xworks.gr/ontologies/ccso#IM203s1/IM_MSc/IED/STEF/TEI"/>
        <instructorOf rdf:resource="http://xworks.gr/ontologies/ccso#TP20K3s1/IE_BSc/IED/STEF/TEIC"/>
        <instructorOf rdf:resource="http://xworks.gr/ontologies/ccso#TP50D2s1/IE_BSc/IED/STEF/TEIC"/>
        <instructorOf rdf:resource="http://xworks.gr/ontologies/ccso#TP50D6s1/IE_BSc/IED/STEF/TEIC"/>
        <instructorOf rdf:resource="http://xworks.gr/ontologies/ccso#TP70D1s1/IE_BSc/IED/STEF/TEIC"/>
        <memberOf rdf:resource="http://xworks.gr/ontologies/ccso#Department_of_Informatics_Engineering_of_TEI_of_Crete"/>
        <supervisorOf rdf:resource="http://xworks.gr/ontologies/ccso#IM203s1/IM_MSc/IED/STEF/TEI"/>
        <supervisorOf rdf:resource="http://xworks.gr/ontologies/ccso#TP20K3s1/IE_BSc/IED/STEF/TEIC"/>
        <supervisorOf rdf:resource="http://xworks.gr/ontologies/ccso#TP50D2s1/IE_BSc/IED/STEF/TEIC"/>
        <supervisorOf rdf:resource="http://xworks.gr/ontologies/ccso#TP50D6s1/IE_BSc/IED/STEF/TEIC"/>
        <supervisorOf rdf:resource="http://xworks.gr/ontologies/ccso#TP70D1s1/IE_BSc/IED/STEF/TEIC"/>
        <worksFor rdf:resource="http://xworks.gr/ontologies/ccso#Department_of_Informatics_Engineering_of_TEI_of_Crete"/>
        <schema:email rdf:datatype="http://www.w3.org/2001/XMLSchema#anyURI">stratakis@ie.teicrete.gr</schema:email>
        <foaf:firstName rdf:datatype="http://www.w3.org/2001/XMLSchema#string">Dimitrios</foaf:firstName>
        <foaf:lastName rdf:datatype="http://www.w3.org/2001/XMLSchema#string">Stratakis</foaf:lastName>
        <eContactInfo rdf:datatype="http://www.w3.org/2001/XMLSchema#anyURI">stratakis@ie.teicrete.gr</eContactInfo>
    </owl:NamedIndividual>
    


    <!-- http://xworks.gr/ontologies/ccso#TEI_of_Crete -->

    <owl:NamedIndividual rdf:about="http://xworks.gr/ontologies/ccso#TEI_of_Crete">
        <rdf:type rdf:resource="http://schema.org/EducationalOrganization"/>
        <rdf:type rdf:resource="http://schema.org/Organization"/>
        <rdf:type rdf:resource="http://xworks.gr/ontologies/ccso#University"/>
        <schema:address rdf:datatype="http://www.w3.org/2001/XMLSchema#string">TEI of Crete  Agios Nikolaos
Fournia Lakonia
PC 72100</schema:address>
        <schema:address rdf:datatype="http://www.w3.org/2001/XMLSchema#string">TEI of Crete  Chania
Romanou 3 Chalepa
Chania PC 73133</schema:address>
        <schema:address rdf:datatype="http://www.w3.org/2001/XMLSchema#string">TEI of Crete  Heraklion
Stauromenos, 71410</schema:address>
        <schema:address rdf:datatype="http://www.w3.org/2001/XMLSchema#string">TEI of Crete  Ierapetra
K. Palama &amp; I. Kakridi
Ierapetra, PC 72200</schema:address>
        <schema:address rdf:datatype="http://www.w3.org/2001/XMLSchema#string">TEI of Crete  Rethymno
E Daskalaki
Peribolia PC 74133</schema:address>
        <schema:address rdf:datatype="http://www.w3.org/2001/XMLSchema#string">TEI of Crete  Sitia
Tripitos 
PC 72300</schema:address>
        <schema:email rdf:datatype="http://www.w3.org/2001/XMLSchema#anyURI">info@staff.teicrete.gr</schema:email>
        <schema:faxNumber rdf:datatype="http://www.w3.org/2001/XMLSchema#string">2810-23003</schema:faxNumber>
        <schema:faxNumber rdf:datatype="http://www.w3.org/2001/XMLSchema#string">2810-379328</schema:faxNumber>
        <schema:faxNumber rdf:datatype="http://www.w3.org/2001/XMLSchema#string">28310-21912</schema:faxNumber>
        <schema:faxNumber rdf:datatype="http://www.w3.org/2001/XMLSchema#string">28410-82879</schema:faxNumber>
        <schema:faxNumber rdf:datatype="http://www.w3.org/2001/XMLSchema#string">28420 89797</schema:faxNumber>
        <schema:identifier rdf:datatype="http://www.w3.org/2001/XMLSchema#string">TEIC</schema:identifier>
        <schema:legalName rdf:datatype="http://www.w3.org/2001/XMLSchema#string">Technological Educational Institute of Crete</schema:legalName>
        <schema:legalName rdf:datatype="http://www.w3.org/2001/XMLSchema#string">Τεχνολογικό Εκπαιδευτικό Ίδρυμα Κρήτης</schema:legalName>
        <schema:logo rdf:datatype="http://www.w3.org/2001/XMLSchema#anyURI">https://www.teicrete.gr/sites/all/themes/teicrete/logo.png</schema:logo>
        <schema:url rdf:datatype="http://www.w3.org/2001/XMLSchema#anyURI">https://www.teicrete.gr</schema:url>
        <eContactInfo rdf:datatype="http://www.w3.org/2001/XMLSchema#anyURI">https://www.teicrete.gr</eContactInfo>
        <eContactInfo rdf:datatype="http://www.w3.org/2001/XMLSchema#anyURI">info@staff.teicrete.gr</eContactInfo>
        <phone rdf:datatype="http://www.w3.org/2001/XMLSchema#string">2810-23000, 23058</phone>
        <phone rdf:datatype="http://www.w3.org/2001/XMLSchema#string">2810-23003</phone>
        <phone rdf:datatype="http://www.w3.org/2001/XMLSchema#string">2810-379110</phone>
        <phone rdf:datatype="http://www.w3.org/2001/XMLSchema#string">2810-379328</phone>
        <phone rdf:datatype="http://www.w3.org/2001/XMLSchema#string">28310-21902</phone>
        <phone rdf:datatype="http://www.w3.org/2001/XMLSchema#string">28310-21912</phone>
        <phone rdf:datatype="http://www.w3.org/2001/XMLSchema#string">28410-82879</phone>
        <phone rdf:datatype="http://www.w3.org/2001/XMLSchema#string">28410-91103, 91102</phone>
        <phone rdf:datatype="http://www.w3.org/2001/XMLSchema#string">28420 89797</phone>
        <phone rdf:datatype="http://www.w3.org/2001/XMLSchema#string">28420-89480-1</phone>
        <phone rdf:datatype="http://www.w3.org/2001/XMLSchema#string">28430-26683</phone>
        <phone rdf:datatype="http://www.w3.org/2001/XMLSchema#string">28430-29497</phone>
        <workPhone rdf:datatype="http://www.w3.org/2001/XMLSchema#string">2810-23000, 23058</workPhone>
        <workPhone rdf:datatype="http://www.w3.org/2001/XMLSchema#string">2810-379110</workPhone>
        <workPhone rdf:datatype="http://www.w3.org/2001/XMLSchema#string">28310-21902</workPhone>
        <workPhone rdf:datatype="http://www.w3.org/2001/XMLSchema#string">28410-91103, 91102</workPhone>
        <workPhone rdf:datatype="http://www.w3.org/2001/XMLSchema#string">28420-89480-1</workPhone>
        <workPhone rdf:datatype="http://www.w3.org/2001/XMLSchema#string">28430-26683</workPhone>
        <workPhone rdf:datatype="http://www.w3.org/2001/XMLSchema#string">28430-29497</workPhone>
        <rdfs:label xml:lang="en">TEI of Crete</rdfs:label>
        <rdfs:label xml:lang="gr">TEI Κρήτης</rdfs:label>
    </owl:NamedIndividual>
    


    <!-- http://xworks.gr/ontologies/ccso#Tarla_Elena -->

    <owl:NamedIndividual rdf:about="http://xworks.gr/ontologies/ccso#Tarla_Elena">
        <rdf:type rdf:resource="http://xmlns.com/foaf/0.1/Person"/>
        <rdf:type rdf:resource="http://xworks.gr/ontologies/ccso#Student"/>
        <affiliatedWith rdf:resource="http://xworks.gr/ontologies/ccso#Psychology_Department_of_University_of_Crete"/>
        <affiliatedWith rdf:resource="http://xworks.gr/ontologies/ccso#BSc_Psychology/PSY_BSc/SoC/UoC"/>
        <affiliatedWith rdf:resource="http://xworks.gr/ontologies/ccso#MSc_School_Psychology/SP_MSc/PSY/SoC/UoC"/>
        <affiliatedWith rdf:resource="http://xworks.gr/ontologies/ccso#PhD_Clinical_Psychology/CP_PhD/Psy/SoC/UoC"/>
        <alumnusOf rdf:resource="http://xworks.gr/ontologies/ccso#Psychology_Department_of_University_of_Crete"/>
        <enrolledIn rdf:resource="http://xworks.gr/ontologies/ccso#PhD_Clinical_Psychology/CP_PhD/Psy/SoC/UoC"/>
        <hasDegree rdf:resource="http://xworks.gr/ontologies/ccso#BSc_Psychology/PSY_BSc/SoC/UoC"/>
        <hasDegree rdf:resource="http://xworks.gr/ontologies/ccso#MSc_School_Psychology/SP_MSc/PSY/SoC/UoC"/>
        <schema:email rdf:datatype="http://www.w3.org/2001/XMLSchema#anyURI">Tarla_Elena@psy.uoc.gr</schema:email>
        <foaf:familyName rdf:datatype="http://www.w3.org/2001/XMLSchema#string">Tarla</foaf:familyName>
        <foaf:firstName rdf:datatype="http://www.w3.org/2001/XMLSchema#string">Elena</foaf:firstName>
        <foaf:lastName rdf:datatype="http://www.w3.org/2001/XMLSchema#string">Tarla</foaf:lastName>
        <eContactInfo rdf:datatype="http://www.w3.org/2001/XMLSchema#anyURI">Tarla_Elena@psy.uoc.gr</eContactInfo>
    </owl:NamedIndividual>
    


    <!-- http://xworks.gr/ontologies/ccso#Tarla_Margaret -->

    <owl:NamedIndividual rdf:about="http://xworks.gr/ontologies/ccso#Tarla_Margaret">
        <rdf:type rdf:resource="http://xmlns.com/foaf/0.1/Agent"/>
        <rdf:type rdf:resource="http://xmlns.com/foaf/0.1/Person"/>
        <rdf:type rdf:resource="http://xworks.gr/ontologies/ccso#Student"/>
        <schema:email rdf:datatype="http://www.w3.org/2001/XMLSchema#anyURI">Tarla_Margaret@mail.gr</schema:email>
        <foaf:familyName rdf:datatype="http://www.w3.org/2001/XMLSchema#string">Tarla</foaf:familyName>
        <foaf:firstName rdf:datatype="http://www.w3.org/2001/XMLSchema#string">Margaret</foaf:firstName>
        <foaf:gender rdf:datatype="http://www.w3.org/2001/XMLSchema#string">Female</foaf:gender>
        <foaf:lastName rdf:datatype="http://www.w3.org/2001/XMLSchema#string">Tarla</foaf:lastName>
        <eContactInfo rdf:datatype="http://www.w3.org/2001/XMLSchema#anyURI">Tarla_Margaret@mail.gr</eContactInfo>
    </owl:NamedIndividual>
    


    <!-- http://xworks.gr/ontologies/ccso#Tarlas_Lefteris -->

    <owl:NamedIndividual rdf:about="http://xworks.gr/ontologies/ccso#Tarlas_Lefteris">
        <rdf:type rdf:resource="http://xmlns.com/foaf/0.1/Person"/>
        <rdf:type rdf:resource="http://xworks.gr/ontologies/ccso#Student"/>
        <foaf:familyName rdf:datatype="http://www.w3.org/2001/XMLSchema#string">Tarlas</foaf:familyName>
        <foaf:firstName rdf:datatype="http://www.w3.org/2001/XMLSchema#string">Lefteris</foaf:firstName>
        <foaf:lastName rdf:datatype="http://www.w3.org/2001/XMLSchema#string">Tarlas</foaf:lastName>
    </owl:NamedIndividual>
    


    <!-- http://xworks.gr/ontologies/ccso#Tarlis_Kostas -->

    <owl:NamedIndividual rdf:about="http://xworks.gr/ontologies/ccso#Tarlis_Kostas">
        <rdf:type rdf:resource="http://xmlns.com/foaf/0.1/Agent"/>
        <rdf:type rdf:resource="http://xmlns.com/foaf/0.1/Person"/>
        <rdf:type rdf:resource="http://xworks.gr/ontologies/ccso#Student"/>
        <rdf:type rdf:resource="http://xworks.gr/ontologies/ccso#UndergraduateStudent"/>
        <affiliatedWith rdf:resource="http://xworks.gr/ontologies/ccso#BSc_Informatics_Engineering/IE_BSc/IED/STEF/TEIC"/>
        <affiliatedWith rdf:resource="http://xworks.gr/ontologies/ccso#TP10K1/IE_BSc/IED/STEF/TEIC"/>
        <affiliatedWith rdf:resource="http://xworks.gr/ontologies/ccso#TP10K2/IE_BSc/IED/STEF/TEIC"/>
        <affiliatedWith rdf:resource="http://xworks.gr/ontologies/ccso#TP10K3/IE_BSc/IED/STEF/TEIC"/>
        <affiliatedWith rdf:resource="http://xworks.gr/ontologies/ccso#TP10K4/IE_BSc/IED/STEF/TEIC"/>
        <affiliatedWith rdf:resource="http://xworks.gr/ontologies/ccso#TP10K5/IE_BSc/IED/STEF/TEIC"/>
        <affiliatedWith rdf:resource="http://xworks.gr/ontologies/ccso#TP10K6/IE_BSc/IED/STEF/TEIC"/>
        <affiliatedWith rdf:resource="http://xworks.gr/ontologies/ccso#TP20K1/IE_BSc/IED/STEF/TEIC"/>
        <affiliatedWith rdf:resource="http://xworks.gr/ontologies/ccso#TP20K2/IE_BSc/IED/STEF/TEIC"/>
        <affiliatedWith rdf:resource="http://xworks.gr/ontologies/ccso#TP20K3/IE_BSc/IED/STEF/TEIC"/>
        <affiliatedWith rdf:resource="http://xworks.gr/ontologies/ccso#TP20K4/IE_BSc/IED/STEF/TEIC"/>
        <affiliatedWith rdf:resource="http://xworks.gr/ontologies/ccso#TP20K6/IE_BSc/IED/STEF/TEIC"/>
        <affiliatedWith rdf:resource="http://xworks.gr/ontologies/ccso#TP30K1/IE_BSc/IED/STEF/TEIC"/>
        <affiliatedWith rdf:resource="http://xworks.gr/ontologies/ccso#TP30K2/IE_BSc/IED/STEF/TEIC"/>
        <affiliatedWith rdf:resource="http://xworks.gr/ontologies/ccso#TP30K4/IE_BSc/IED/STEF/TEIC"/>
        <affiliatedWith rdf:resource="http://xworks.gr/ontologies/ccso#TP30K6/IE_BSc/IED/STEF/TEIC"/>
        <affiliatedWith rdf:resource="http://xworks.gr/ontologies/ccso#TP30K7/IE_BSc/IED/STEF/TEIC"/>
        <affiliatedWith rdf:resource="http://xworks.gr/ontologies/ccso#TP40K1/IE_BSc/IED/STEF/TEIC"/>
        <affiliatedWith rdf:resource="http://xworks.gr/ontologies/ccso#TP40K2/IE_BSc/IED/STEF/TEIC"/>
        <affiliatedWith rdf:resource="http://xworks.gr/ontologies/ccso#TP40K3/IE_BSc/IED/STEF/TEIC"/>
        <affiliatedWith rdf:resource="http://xworks.gr/ontologies/ccso#TP40K4/IE_BSc/IED/STEF/TEIC"/>
        <affiliatedWith rdf:resource="http://xworks.gr/ontologies/ccso#TP40K6/IE_BSc/IED/STEF/TEIC"/>
        <attendsCourse rdf:resource="http://xworks.gr/ontologies/ccso#TP10K5/IE_BSc/IED/STEF/TEIC"/>
        <attendsCourse rdf:resource="http://xworks.gr/ontologies/ccso#TP40K1/IE_BSc/IED/STEF/TEIC"/>
        <attendsCourse rdf:resource="http://xworks.gr/ontologies/ccso#TP40K2/IE_BSc/IED/STEF/TEIC"/>
        <attendsCourse rdf:resource="http://xworks.gr/ontologies/ccso#TP40K3/IE_BSc/IED/STEF/TEIC"/>
        <attendsCourse rdf:resource="http://xworks.gr/ontologies/ccso#TP40K4/IE_BSc/IED/STEF/TEIC"/>
        <attendsCourse rdf:resource="http://xworks.gr/ontologies/ccso#TP40K6/IE_BSc/IED/STEF/TEIC"/>
        <enrolledIn rdf:resource="http://xworks.gr/ontologies/ccso#BSc_Informatics_Engineering/IE_BSc/IED/STEF/TEIC"/>
        <hasCompleted rdf:resource="http://xworks.gr/ontologies/ccso#TP10K1/IE_BSc/IED/STEF/TEIC"/>
        <hasCompleted rdf:resource="http://xworks.gr/ontologies/ccso#TP10K2/IE_BSc/IED/STEF/TEIC"/>
        <hasCompleted rdf:resource="http://xworks.gr/ontologies/ccso#TP10K3/IE_BSc/IED/STEF/TEIC"/>
        <hasCompleted rdf:resource="http://xworks.gr/ontologies/ccso#TP10K4/IE_BSc/IED/STEF/TEIC"/>
        <hasCompleted rdf:resource="http://xworks.gr/ontologies/ccso#TP10K6/IE_BSc/IED/STEF/TEIC"/>
        <hasCompleted rdf:resource="http://xworks.gr/ontologies/ccso#TP20K1/IE_BSc/IED/STEF/TEIC"/>
        <hasCompleted rdf:resource="http://xworks.gr/ontologies/ccso#TP20K2/IE_BSc/IED/STEF/TEIC"/>
        <hasCompleted rdf:resource="http://xworks.gr/ontologies/ccso#TP20K3/IE_BSc/IED/STEF/TEIC"/>
        <hasCompleted rdf:resource="http://xworks.gr/ontologies/ccso#TP20K4/IE_BSc/IED/STEF/TEIC"/>
        <hasCompleted rdf:resource="http://xworks.gr/ontologies/ccso#TP20K6/IE_BSc/IED/STEF/TEIC"/>
        <hasCompleted rdf:resource="http://xworks.gr/ontologies/ccso#TP30K1/IE_BSc/IED/STEF/TEIC"/>
        <hasCompleted rdf:resource="http://xworks.gr/ontologies/ccso#TP30K2/IE_BSc/IED/STEF/TEIC"/>
        <hasCompleted rdf:resource="http://xworks.gr/ontologies/ccso#TP30K4/IE_BSc/IED/STEF/TEIC"/>
        <hasCompleted rdf:resource="http://xworks.gr/ontologies/ccso#TP30K6/IE_BSc/IED/STEF/TEIC"/>
        <hasCompleted rdf:resource="http://xworks.gr/ontologies/ccso#TP30K7/IE_BSc/IED/STEF/TEIC"/>
        <schema:email rdf:datatype="http://www.w3.org/2001/XMLSchema#anyURI">SamTarly@ie.teicrete.gr</schema:email>
        <foaf:familyName rdf:datatype="http://www.w3.org/2001/XMLSchema#string">Tarly</foaf:familyName>
        <foaf:firstName rdf:datatype="http://www.w3.org/2001/XMLSchema#string">Samwell</foaf:firstName>
        <foaf:gender rdf:datatype="http://www.w3.org/2001/XMLSchema#string">Male</foaf:gender>
        <foaf:lastName rdf:datatype="http://www.w3.org/2001/XMLSchema#string">Tarly</foaf:lastName>
        <eContactInfo rdf:datatype="http://www.w3.org/2001/XMLSchema#anyURI">SamTarly@ie.teicrete.gr</eContactInfo>
    </owl:NamedIndividual>
    


    <!-- http://xworks.gr/ontologies/ccso#Tatheli_Vicky -->

    <owl:NamedIndividual rdf:about="http://xworks.gr/ontologies/ccso#Tatheli_Vicky">
        <rdf:type rdf:resource="http://xmlns.com/foaf/0.1/Person"/>
        <rdf:type rdf:resource="http://xworks.gr/ontologies/ccso#Student"/>
        <foaf:firstName rdf:datatype="http://www.w3.org/2001/XMLSchema#string">Vicky</foaf:firstName>
        <foaf:lastName rdf:datatype="http://www.w3.org/2001/XMLSchema#string">Tatheli</foaf:lastName>
    </owl:NamedIndividual>
    


    <!-- http://xworks.gr/ontologies/ccso#Tollis_Ioannis -->

    <owl:NamedIndividual rdf:about="http://xworks.gr/ontologies/ccso#Tollis_Ioannis">
        <rdf:type rdf:resource="http://xmlns.com/foaf/0.1/Person"/>
        <rdf:type rdf:resource="http://xworks.gr/ontologies/ccso#AcademicStaff"/>
        <rdf:type rdf:resource="http://xworks.gr/ontologies/ccso#Employee"/>
        <rdf:type rdf:resource="http://xworks.gr/ontologies/ccso#Professor"/>
        <affiliatedWith rdf:resource="http://xworks.gr/ontologies/ccso#Computers_Sciences_Department_of_University_of_Crete"/>
        <affiliatedWith rdf:resource="http://xworks.gr/ontologies/ccso#CS380s1/CS_BSc/CSD/SSE/UoC"/>
        <instructorOf rdf:resource="http://xworks.gr/ontologies/ccso#CS380s1/CS_BSc/CSD/SSE/UoC"/>
        <memberOf rdf:resource="http://xworks.gr/ontologies/ccso#Computers_Sciences_Department_of_University_of_Crete"/>
        <supervisorOf rdf:resource="http://xworks.gr/ontologies/ccso#CS380s1/CS_BSc/CSD/SSE/UoC"/>
        <worksFor rdf:resource="http://xworks.gr/ontologies/ccso#Computers_Sciences_Department_of_University_of_Crete"/>
        <schema:email rdf:datatype="http://www.w3.org/2001/XMLSchema#anyURI">tollis@csd.uoc.gr</schema:email>
        <foaf:firstName rdf:datatype="http://www.w3.org/2001/XMLSchema#string">Ioannis</foaf:firstName>
        <foaf:lastName rdf:datatype="http://www.w3.org/2001/XMLSchema#string">Tollis</foaf:lastName>
        <eContactInfo rdf:datatype="http://www.w3.org/2001/XMLSchema#anyURI">tollis@csd.uoc.gr</eContactInfo>
    </owl:NamedIndividual>
    


    <!-- http://xworks.gr/ontologies/ccso#Triantafillou_Irene -->

    <owl:NamedIndividual rdf:about="http://xworks.gr/ontologies/ccso#Triantafillou_Irene">
        <rdf:type rdf:resource="http://xmlns.com/foaf/0.1/Person"/>
        <rdf:type rdf:resource="http://xworks.gr/ontologies/ccso#PostgraduateStudent"/>
        <rdf:type rdf:resource="http://xworks.gr/ontologies/ccso#Student"/>
        <affiliatedWith rdf:resource="http://xworks.gr/ontologies/ccso#Computers_Sciences_Department_of_University_of_Crete"/>
        <affiliatedWith rdf:resource="http://xworks.gr/ontologies/ccso#BSc_Computer_Science/CS_BSc/CSD/SSE/UoC"/>
        <affiliatedWith rdf:resource="http://xworks.gr/ontologies/ccso#IM101/IM_MSc/IED/STEF/TEIC"/>
        <affiliatedWith rdf:resource="http://xworks.gr/ontologies/ccso#IM102/IM_MSc/IED/STEF/TEIC"/>
        <affiliatedWith rdf:resource="http://xworks.gr/ontologies/ccso#IM103/IM_MSc/IED/STEF/TEIC"/>
        <affiliatedWith rdf:resource="http://xworks.gr/ontologies/ccso#IM201/IM_MSc/IED/STEF/TEIC"/>
        <affiliatedWith rdf:resource="http://xworks.gr/ontologies/ccso#IM202/IM_MSc/IED/STEF/TEIC"/>
        <affiliatedWith rdf:resource="http://xworks.gr/ontologies/ccso#IM203/IM_MSc/IED/STEF/TEIC"/>
        <affiliatedWith rdf:resource="http://xworks.gr/ontologies/ccso#IM205/IM_MSc/IED/STEF/TEIC"/>
        <affiliatedWith rdf:resource="http://xworks.gr/ontologies/ccso#MSc_Informatics_&amp;_Multimedia/IM_MSc/IED/STEF/TEIC"/>
        <alumnusOf rdf:resource="http://xworks.gr/ontologies/ccso#Computers_Sciences_Department_of_University_of_Crete"/>
        <attendsCourse rdf:resource="http://xworks.gr/ontologies/ccso#IM201/IM_MSc/IED/STEF/TEIC"/>
        <attendsCourse rdf:resource="http://xworks.gr/ontologies/ccso#IM203/IM_MSc/IED/STEF/TEIC"/>
        <attendsCourse rdf:resource="http://xworks.gr/ontologies/ccso#IM205/IM_MSc/IED/STEF/TEIC"/>
        <enrolledIn rdf:resource="http://xworks.gr/ontologies/ccso#MSc_Informatics_&amp;_Multimedia/IM_MSc/IED/STEF/TEIC"/>
        <hasCompleted rdf:resource="http://xworks.gr/ontologies/ccso#IM101/IM_MSc/IED/STEF/TEIC"/>
        <hasCompleted rdf:resource="http://xworks.gr/ontologies/ccso#IM102/IM_MSc/IED/STEF/TEIC"/>
        <hasCompleted rdf:resource="http://xworks.gr/ontologies/ccso#IM103/IM_MSc/IED/STEF/TEIC"/>
        <hasCompleted rdf:resource="http://xworks.gr/ontologies/ccso#IM202/IM_MSc/IED/STEF/TEIC"/>
        <hasDegree rdf:resource="http://xworks.gr/ontologies/ccso#BSc_Computer_Science/CS_BSc/CSD/SSE/UoC"/>
        <schema:email rdf:datatype="http://www.w3.org/2001/XMLSchema#anyURI">Triantafillou_Irene@csd.uoc.gr</schema:email>
        <foaf:firstName rdf:datatype="http://www.w3.org/2001/XMLSchema#string">Irene</foaf:firstName>
        <foaf:lastName rdf:datatype="http://www.w3.org/2001/XMLSchema#string">Triantafillou</foaf:lastName>
        <eContactInfo rdf:datatype="http://www.w3.org/2001/XMLSchema#anyURI">Triantafillou_Irene@csd.uoc.gr</eContactInfo>
    </owl:NamedIndividual>
    


    <!-- http://xworks.gr/ontologies/ccso#Triantafyllidis_George -->

    <owl:NamedIndividual rdf:about="http://xworks.gr/ontologies/ccso#Triantafyllidis_George">
        <rdf:type rdf:resource="http://xmlns.com/foaf/0.1/Agent"/>
        <rdf:type rdf:resource="http://xmlns.com/foaf/0.1/Person"/>
        <rdf:type rdf:resource="http://xworks.gr/ontologies/ccso#AcademicStaff"/>
        <rdf:type rdf:resource="http://xworks.gr/ontologies/ccso#Employee"/>
        <rdf:type rdf:resource="http://xworks.gr/ontologies/ccso#Professor"/>
        <affiliatedWith rdf:resource="http://xworks.gr/ontologies/ccso#Department_of_Informatics_Engineering_of_TEI_of_Crete"/>
        <affiliatedWith rdf:resource="http://xworks.gr/ontologies/ccso#IM210s1/IM_MSc/IED/STEF/TEI"/>
        <affiliatedWith rdf:resource="http://xworks.gr/ontologies/ccso#IM211s1/IM_MSc/IED/STEF/TEI"/>
        <instructorOf rdf:resource="http://xworks.gr/ontologies/ccso#IM210s1/IM_MSc/IED/STEF/TEI"/>
        <instructorOf rdf:resource="http://xworks.gr/ontologies/ccso#IM211s1/IM_MSc/IED/STEF/TEI"/>
        <memberOf rdf:resource="http://xworks.gr/ontologies/ccso#Department_of_Informatics_Engineering_of_TEI_of_Crete"/>
        <supervisorOf rdf:resource="http://xworks.gr/ontologies/ccso#IM210s1/IM_MSc/IED/STEF/TEI"/>
        <supervisorOf rdf:resource="http://xworks.gr/ontologies/ccso#IM211s1/IM_MSc/IED/STEF/TEI"/>
        <worksFor rdf:resource="http://xworks.gr/ontologies/ccso#Department_of_Informatics_Engineering_of_TEI_of_Crete"/>
        <schema:email rdf:datatype="http://www.w3.org/2001/XMLSchema#anyURI">triantafyllidis@ie.teicrete.gr</schema:email>
        <foaf:firstName rdf:datatype="http://www.w3.org/2001/XMLSchema#string">George</foaf:firstName>
        <foaf:gender rdf:datatype="http://www.w3.org/2001/XMLSchema#string">Male</foaf:gender>
        <foaf:lastName rdf:datatype="http://www.w3.org/2001/XMLSchema#string">Triantafyllidis</foaf:lastName>
        <eContactInfo rdf:datatype="http://www.w3.org/2001/XMLSchema#anyURI">triantafyllidis@ie.teicrete.gr</eContactInfo>
    </owl:NamedIndividual>
    


    <!-- http://xworks.gr/ontologies/ccso#Tsaeri_Elena -->

    <owl:NamedIndividual rdf:about="http://xworks.gr/ontologies/ccso#Tsaeri_Elena">
        <rdf:type rdf:resource="http://xmlns.com/foaf/0.1/Person"/>
        <rdf:type rdf:resource="http://xworks.gr/ontologies/ccso#AcademicStaff"/>
        <rdf:type rdf:resource="http://xworks.gr/ontologies/ccso#Employee"/>
        <rdf:type rdf:resource="http://xworks.gr/ontologies/ccso#Professor"/>
        <affiliatedWith rdf:resource="http://xworks.gr/ontologies/ccso#Psychology_Department_of_University_of_Crete"/>
        <affiliatedWith rdf:resource="http://xworks.gr/ontologies/ccso#PSY1501_s2017-18-L01/PSY_BSc/SoC/Uoc"/>
        <affiliatedWith rdf:resource="http://xworks.gr/ontologies/ccso#PSY1501s1/PSY_BSc/SoC/Uoc"/>
        <instructorOf rdf:resource="http://xworks.gr/ontologies/ccso#PSY1501s1/PSY_BSc/SoC/Uoc"/>
        <memberOf rdf:resource="http://xworks.gr/ontologies/ccso#Psychology_Department_of_University_of_Crete"/>
        <teachesIn rdf:resource="http://xworks.gr/ontologies/ccso#PSY1501_s2017-18-L01/PSY_BSc/SoC/Uoc"/>
        <worksFor rdf:resource="http://xworks.gr/ontologies/ccso#Psychology_Department_of_University_of_Crete"/>
        <schema:email rdf:datatype="http://www.w3.org/2001/XMLSchema#anyURI">TsaeriElena@psy.uoc.gr</schema:email>
        <foaf:firstName rdf:datatype="http://www.w3.org/2001/XMLSchema#string">Elena</foaf:firstName>
        <foaf:lastName rdf:datatype="http://www.w3.org/2001/XMLSchema#string">Tsaeri</foaf:lastName>
        <eContactInfo rdf:datatype="http://www.w3.org/2001/XMLSchema#anyURI">TsaeriElena@psy.uoc.gr</eContactInfo>
    </owl:NamedIndividual>
    


    <!-- http://xworks.gr/ontologies/ccso#Tsakalidis_Panayiotis -->

    <owl:NamedIndividual rdf:about="http://xworks.gr/ontologies/ccso#Tsakalidis_Panayiotis">
        <rdf:type rdf:resource="http://xmlns.com/foaf/0.1/Person"/>
        <rdf:type rdf:resource="http://xworks.gr/ontologies/ccso#AcademicStaff"/>
        <rdf:type rdf:resource="http://xworks.gr/ontologies/ccso#Employee"/>
        <rdf:type rdf:resource="http://xworks.gr/ontologies/ccso#Professor"/>
        <affiliatedWith rdf:resource="http://xworks.gr/ontologies/ccso#Computers_Sciences_Department_of_University_of_Crete"/>
        <affiliatedWith rdf:resource="http://xworks.gr/ontologies/ccso#CS215s1/CS_BSc/CSD/SSE/UoC"/>
        <affiliatedWith rdf:resource="http://xworks.gr/ontologies/ccso#CS217s1/CS_BSc/CSD/SSE/UoC"/>
        <instructorOf rdf:resource="http://xworks.gr/ontologies/ccso#CS215s1/CS_BSc/CSD/SSE/UoC"/>
        <instructorOf rdf:resource="http://xworks.gr/ontologies/ccso#CS217s1/CS_BSc/CSD/SSE/UoC"/>
        <memberOf rdf:resource="http://xworks.gr/ontologies/ccso#Computers_Sciences_Department_of_University_of_Crete"/>
        <supervisorOf rdf:resource="http://xworks.gr/ontologies/ccso#CS215s1/CS_BSc/CSD/SSE/UoC"/>
        <supervisorOf rdf:resource="http://xworks.gr/ontologies/ccso#CS217s1/CS_BSc/CSD/SSE/UoC"/>
        <worksFor rdf:resource="http://xworks.gr/ontologies/ccso#Computers_Sciences_Department_of_University_of_Crete"/>
        <schema:email rdf:datatype="http://www.w3.org/2001/XMLSchema#anyURI">tsakalid@csd.uoc.gr</schema:email>
        <foaf:firstName rdf:datatype="http://www.w3.org/2001/XMLSchema#string">Panayiotis</foaf:firstName>
        <foaf:lastName rdf:datatype="http://www.w3.org/2001/XMLSchema#string">Tsakalidis</foaf:lastName>
        <eContactInfo rdf:datatype="http://www.w3.org/2001/XMLSchema#anyURI">tsakalid@csd.uoc.gr</eContactInfo>
    </owl:NamedIndividual>
    


    <!-- http://xworks.gr/ontologies/ccso#Tsiknakis_Manolis -->

    <owl:NamedIndividual rdf:about="http://xworks.gr/ontologies/ccso#Tsiknakis_Manolis">
        <rdf:type rdf:resource="http://xmlns.com/foaf/0.1/Agent"/>
        <rdf:type rdf:resource="http://xmlns.com/foaf/0.1/Person"/>
        <rdf:type rdf:resource="http://xworks.gr/ontologies/ccso#AcademicStaff"/>
        <rdf:type rdf:resource="http://xworks.gr/ontologies/ccso#Employee"/>
        <rdf:type rdf:resource="http://xworks.gr/ontologies/ccso#Professor"/>
        <affiliatedWith rdf:resource="http://xworks.gr/ontologies/ccso#Computers_Sciences_Department_of_University_of_Crete"/>
        <affiliatedWith rdf:resource="http://xworks.gr/ontologies/ccso#Department_of_Informatics_Engineering_of_TEI_of_Crete"/>
        <affiliatedWith rdf:resource="http://xworks.gr/ontologies/ccso#BSc_Computer_Science/CS_BSc/CSD/SSE/UoC"/>
        <affiliatedWith rdf:resource="http://xworks.gr/ontologies/ccso#CS335_s2017-18-L02/CS_BSc/CSD/SSE/UoC"/>
        <affiliatedWith rdf:resource="http://xworks.gr/ontologies/ccso#CS335_s2017-18-L03/CS_BSc/CSD/SSE/UoC"/>
        <affiliatedWith rdf:resource="http://xworks.gr/ontologies/ccso#CS335_s2017-18-L04/CS_BSc/CSD/SSE/UoC"/>
        <affiliatedWith rdf:resource="http://xworks.gr/ontologies/ccso#CS335_s2017-18-L05/CS_BSc/CSD/SSE/UoC"/>
        <affiliatedWith rdf:resource="http://xworks.gr/ontologies/ccso#CS335_s2017-18/CS_BSc/CSD/SSE/UoC"/>
        <affiliatedWith rdf:resource="http://xworks.gr/ontologies/ccso#IM101s1/IM_MSc/IED/STEF/TEI"/>
        <affiliatedWith rdf:resource="http://xworks.gr/ontologies/ccso#MSc_Computer_Science_and_Engineering/CSE_MSc/CSD/SSE/UoC"/>
        <affiliatedWith rdf:resource="http://xworks.gr/ontologies/ccso#PhD_Computer_Science_and_Engineering/CSE_PhD/CSD/SSE/UoC"/>
        <affiliatedWith rdf:resource="http://xworks.gr/ontologies/ccso#TP20K6s1/IE_BSc/IED/STEF/TEIC"/>
        <affiliatedWith rdf:resource="http://xworks.gr/ontologies/ccso#TP30K6s1/IE_BSc/IED/STEF/TEIC"/>
        <affiliatedWith rdf:resource="http://xworks.gr/ontologies/ccso#TP50L1s1/IE_BSc/IED/STEF/TEIC"/>
        <affiliatedWith rdf:resource="http://xworks.gr/ontologies/ccso#TP60L3s1/IE_BSc/IED/STEF/TEIC"/>
        <affiliatedWith rdf:resource="http://xworks.gr/ontologies/ccso#TP60L4s1/IE_BSc/IED/STEF/TEIC"/>
        <alumnusOf rdf:resource="http://xworks.gr/ontologies/ccso#Computers_Sciences_Department_of_University_of_Crete"/>
        <hasDegree rdf:resource="http://xworks.gr/ontologies/ccso#BSc_Computer_Science/CS_BSc/CSD/SSE/UoC"/>
        <hasDegree rdf:resource="http://xworks.gr/ontologies/ccso#MSc_Computer_Science_and_Engineering/CSE_MSc/CSD/SSE/UoC"/>
        <hasDegree rdf:resource="http://xworks.gr/ontologies/ccso#PhD_Computer_Science_and_Engineering/CSE_PhD/CSD/SSE/UoC"/>
        <instructorOf rdf:resource="http://xworks.gr/ontologies/ccso#CS335_s2017-18/CS_BSc/CSD/SSE/UoC"/>
        <instructorOf rdf:resource="http://xworks.gr/ontologies/ccso#IM101s1/IM_MSc/IED/STEF/TEI"/>
        <instructorOf rdf:resource="http://xworks.gr/ontologies/ccso#TP20K6s1/IE_BSc/IED/STEF/TEIC"/>
        <instructorOf rdf:resource="http://xworks.gr/ontologies/ccso#TP30K6s1/IE_BSc/IED/STEF/TEIC"/>
        <instructorOf rdf:resource="http://xworks.gr/ontologies/ccso#TP50L1s1/IE_BSc/IED/STEF/TEIC"/>
        <instructorOf rdf:resource="http://xworks.gr/ontologies/ccso#TP60L3s1/IE_BSc/IED/STEF/TEIC"/>
        <instructorOf rdf:resource="http://xworks.gr/ontologies/ccso#TP60L4s1/IE_BSc/IED/STEF/TEIC"/>
        <memberOf rdf:resource="http://xworks.gr/ontologies/ccso#Computers_Sciences_Department_of_University_of_Crete"/>
        <memberOf rdf:resource="http://xworks.gr/ontologies/ccso#Department_of_Informatics_Engineering_of_TEI_of_Crete"/>
        <supervisorOf rdf:resource="http://xworks.gr/ontologies/ccso#CS335_s2017-18/CS_BSc/CSD/SSE/UoC"/>
        <supervisorOf rdf:resource="http://xworks.gr/ontologies/ccso#IM101s1/IM_MSc/IED/STEF/TEI"/>
        <supervisorOf rdf:resource="http://xworks.gr/ontologies/ccso#TP20K6s1/IE_BSc/IED/STEF/TEIC"/>
        <supervisorOf rdf:resource="http://xworks.gr/ontologies/ccso#TP30K6s1/IE_BSc/IED/STEF/TEIC"/>
        <supervisorOf rdf:resource="http://xworks.gr/ontologies/ccso#TP50L1s1/IE_BSc/IED/STEF/TEIC"/>
        <supervisorOf rdf:resource="http://xworks.gr/ontologies/ccso#TP60L3s1/IE_BSc/IED/STEF/TEIC"/>
        <supervisorOf rdf:resource="http://xworks.gr/ontologies/ccso#TP60L4s1/IE_BSc/IED/STEF/TEIC"/>
        <teachesIn rdf:resource="http://xworks.gr/ontologies/ccso#CS335_s2017-18-L02/CS_BSc/CSD/SSE/UoC"/>
        <teachesIn rdf:resource="http://xworks.gr/ontologies/ccso#CS335_s2017-18-L03/CS_BSc/CSD/SSE/UoC"/>
        <teachesIn rdf:resource="http://xworks.gr/ontologies/ccso#CS335_s2017-18-L04/CS_BSc/CSD/SSE/UoC"/>
        <teachesIn rdf:resource="http://xworks.gr/ontologies/ccso#CS335_s2017-18-L05/CS_BSc/CSD/SSE/UoC"/>
        <worksFor rdf:resource="http://xworks.gr/ontologies/ccso#Computers_Sciences_Department_of_University_of_Crete"/>
        <worksFor rdf:resource="http://xworks.gr/ontologies/ccso#Department_of_Informatics_Engineering_of_TEI_of_Crete"/>
        <schema:email rdf:datatype="http://www.w3.org/2001/XMLSchema#anyURI">tsiknakis@ie.teicrete.gr</schema:email>
        <foaf:firstName rdf:datatype="http://www.w3.org/2001/XMLSchema#string">Manolis</foaf:firstName>
        <foaf:gender rdf:datatype="http://www.w3.org/2001/XMLSchema#string">Male</foaf:gender>
        <foaf:lastName rdf:datatype="http://www.w3.org/2001/XMLSchema#string">Tsiknakis</foaf:lastName>
        <eContactInfo rdf:datatype="http://www.w3.org/2001/XMLSchema#anyURI">tsiknakis@ie.teicrete.gr</eContactInfo>
    </owl:NamedIndividual>
    


    <!-- http://xworks.gr/ontologies/ccso#Tziritas_George -->

    <owl:NamedIndividual rdf:about="http://xworks.gr/ontologies/ccso#Tziritas_George">
        <rdf:type rdf:resource="http://xmlns.com/foaf/0.1/Person"/>
        <rdf:type rdf:resource="http://xworks.gr/ontologies/ccso#AcademicStaff"/>
        <rdf:type rdf:resource="http://xworks.gr/ontologies/ccso#Employee"/>
        <rdf:type rdf:resource="http://xworks.gr/ontologies/ccso#Professor"/>
        <affiliatedWith rdf:resource="http://xworks.gr/ontologies/ccso#Computers_Sciences_Department_of_University_of_Crete"/>
        <affiliatedWith rdf:resource="http://xworks.gr/ontologies/ccso#CS119s1/CS_BSc/CSD/SSE/UoC"/>
        <affiliatedWith rdf:resource="http://xworks.gr/ontologies/ccso#CS119s2017-18/CS_BSc/CSD/SSE/UoC"/>
        <instructorOf rdf:resource="http://xworks.gr/ontologies/ccso#CS119s1/CS_BSc/CSD/SSE/UoC"/>
        <instructorOf rdf:resource="http://xworks.gr/ontologies/ccso#CS119s2017-18/CS_BSc/CSD/SSE/UoC"/>
        <memberOf rdf:resource="http://xworks.gr/ontologies/ccso#Computers_Sciences_Department_of_University_of_Crete"/>
        <supervisorOf rdf:resource="http://xworks.gr/ontologies/ccso#CS119s1/CS_BSc/CSD/SSE/UoC"/>
        <supervisorOf rdf:resource="http://xworks.gr/ontologies/ccso#CS119s2017-18/CS_BSc/CSD/SSE/UoC"/>
        <worksFor rdf:resource="http://xworks.gr/ontologies/ccso#Computers_Sciences_Department_of_University_of_Crete"/>
        <schema:email rdf:datatype="http://www.w3.org/2001/XMLSchema#anyURI">tziritas@csd.uoc.gr</schema:email>
        <foaf:firstName rdf:datatype="http://www.w3.org/2001/XMLSchema#string">George</foaf:firstName>
        <foaf:lastName rdf:datatype="http://www.w3.org/2001/XMLSchema#string">Tziritas</foaf:lastName>
        <eContactInfo rdf:datatype="http://www.w3.org/2001/XMLSchema#anyURI">tziritas@csd.uoc.gr</eContactInfo>
    </owl:NamedIndividual>
    


    <!-- http://xworks.gr/ontologies/ccso#University_of_Crete -->

    <owl:NamedIndividual rdf:about="http://xworks.gr/ontologies/ccso#University_of_Crete">
        <rdf:type rdf:resource="http://schema.org/EducationalOrganization"/>
        <rdf:type rdf:resource="http://schema.org/Organization"/>
        <rdf:type rdf:resource="http://xworks.gr/ontologies/ccso#University"/>
        <schema:address rdf:datatype="http://www.w3.org/2001/XMLSchema#string">Univesity of Crete
Gallos Campus
74100, Rethymno</schema:address>
        <schema:address rdf:datatype="http://www.w3.org/2001/XMLSchema#string">Univesity of Crete
Voutes Campus
70013, Heraklion
Crete</schema:address>
        <schema:address rdf:datatype="http://www.w3.org/2001/XMLSchema#string">Πανεπιστήμιο Κρήτης
Πανεπιστημιούπολη Βουτών 
Ταχ. Κώδικας: 70013 Βασιλικά Βουτών
Ηράκλειο</schema:address>
        <schema:address rdf:datatype="http://www.w3.org/2001/XMLSchema#string">Πανεπιστήμιο Κρήτης
Πανεπιστημιούπολη Ρεθύμνου
Ταχ. Κώδικας: 74100
Ρέθυμνο</schema:address>
        <schema:email rdf:datatype="http://www.w3.org/2001/XMLSchema#anyURI">secretary@rector.uoc.gr</schema:email>
        <schema:faxNumber rdf:datatype="http://www.w3.org/2001/XMLSchema#string">+30 2810 545212</schema:faxNumber>
        <schema:faxNumber rdf:datatype="http://www.w3.org/2001/XMLSchema#string">+30 28310 77909</schema:faxNumber>
        <schema:identifier rdf:datatype="http://www.w3.org/2001/XMLSchema#string">UoC</schema:identifier>
        <schema:legalName rdf:datatype="http://www.w3.org/2001/XMLSchema#string">University of Crete</schema:legalName>
        <schema:legalName rdf:datatype="http://www.w3.org/2001/XMLSchema#string">Πανεπιστήμιο Κρήτης</schema:legalName>
        <schema:location rdf:datatype="http://www.w3.org/2001/XMLSchema#string">Voutes, Heraklion</schema:location>
        <schema:location rdf:datatype="http://www.w3.org/2001/XMLSchema#string">Γάλλος, Ρέθυμνο</schema:location>
        <schema:logo rdf:datatype="http://www.w3.org/2001/XMLSchema#anyURI">http://www.uoc.gr/images/logo.png</schema:logo>
        <schema:url rdf:datatype="http://www.w3.org/2001/XMLSchema#anyURI">http://www.uoc.gr</schema:url>
        <eContactInfo rdf:datatype="http://www.w3.org/2001/XMLSchema#anyURI">http://www.uoc.gr</eContactInfo>
        <eContactInfo rdf:datatype="http://www.w3.org/2001/XMLSchema#anyURI">secretary@rector.uoc.gr</eContactInfo>
        <phone rdf:datatype="http://www.w3.org/2001/XMLSchema#string">+30 2810 545200</phone>
        <phone rdf:datatype="http://www.w3.org/2001/XMLSchema#string">+30 2810 545212</phone>
        <phone rdf:datatype="http://www.w3.org/2001/XMLSchema#string">+30 28310 77900</phone>
        <phone rdf:datatype="http://www.w3.org/2001/XMLSchema#string">+30 28310 77909</phone>
        <workPhone rdf:datatype="http://www.w3.org/2001/XMLSchema#string">+30 2810 545200</workPhone>
        <workPhone rdf:datatype="http://www.w3.org/2001/XMLSchema#string">+30 28310 77900</workPhone>
        <rdfs:label xml:lang="en">University of Crete</rdfs:label>
        <rdfs:label xml:lang="gr">Πανεπιστήμιο Κρήτης</rdfs:label>
    </owl:NamedIndividual>
    


    <!-- http://xworks.gr/ontologies/ccso#Vassilakis2005AsynchronousTeleTeaching -->

    <owl:NamedIndividual rdf:about="http://xworks.gr/ontologies/ccso#Vassilakis2005AsynchronousTeleTeaching">
        <rdf:type rdf:resource="http://xworks.gr/ontologies/ccso#Resource"/>
        <dc:creator rdf:resource="http://xworks.gr/ontologies/ccso#Kalogiannakis_Michail"/>
        <dc:creator rdf:resource="http://xworks.gr/ontologies/ccso#Vassilakis_Kostas"/>
        <dc:date rdf:datatype="http://www.w3.org/2001/XMLSchema#date">2005</dc:date>
        <dc:date rdf:datatype="internal:anonymous-constants">2005</dc:date>
        <dc:source rdf:datatype="http://www.w3.org/2001/XMLSchema#string">In Proceedings of the 4th international conference on new horizons in industry business and education, NHIBE (pp. 216-221)</dc:source>
        <dc:title rdf:datatype="http://www.w3.org/2001/XMLSchema#string">Asynchronous Tele-Teaching at TEI of Crete. Primary results of an empirical research</dc:title>
        <dc:type rdf:datatype="http://www.w3.org/2001/XMLSchema#string">Proceeedings</dc:type>
        <dates rdf:datatype="internal:anonymous-constants">2005</dates>
        <resourceCitation rdf:datatype="http://www.w3.org/2001/XMLSchema#string">Vassilakis, K., Psarros, M., &amp; Kalogiannakis, M. (2005). Asynchronous tele-teaching at TEI of Crete. Primary results of an empirical research. In Proceedings of the 4th international conference on new horizons in industry business and education, NHIBE (pp. 216-221)</resourceCitation>
        <rdfs:label xml:lang="en">Vassilakis,Psarros,Kalogiannakis (2005) Asynchronous Tele-Teaching at TEI of Crete. Primary results of an empirical research</rdfs:label>
    </owl:NamedIndividual>
    


    <!-- http://xworks.gr/ontologies/ccso#Vassilakis_Kostas -->

    <owl:NamedIndividual rdf:about="http://xworks.gr/ontologies/ccso#Vassilakis_Kostas">
        <rdf:type rdf:resource="http://www.w3.org/2000/10/swap/pim/contact#Person"/>
        <rdf:type rdf:resource="http://xmlns.com/foaf/0.1/Agent"/>
        <rdf:type rdf:resource="http://xmlns.com/foaf/0.1/Person"/>
        <rdf:type rdf:resource="http://xworks.gr/ontologies/ccso#AcademicStaff"/>
        <rdf:type rdf:resource="http://xworks.gr/ontologies/ccso#Employee"/>
        <rdf:type rdf:resource="http://xworks.gr/ontologies/ccso#Professor"/>
        <affiliatedWith rdf:resource="http://xworks.gr/ontologies/ccso#Computers_Sciences_Department_of_University_of_Crete"/>
        <affiliatedWith rdf:resource="http://xworks.gr/ontologies/ccso#Department_of_Informatics_Engineering_of_TEI_of_Crete"/>
        <affiliatedWith rdf:resource="http://xworks.gr/ontologies/ccso#BSc_Computer_Science/CS_BSc/CSD/SSE/UoC"/>
        <affiliatedWith rdf:resource="http://xworks.gr/ontologies/ccso#IM209s1/IM_MSc/IED/STEF/TEI"/>
        <affiliatedWith rdf:resource="http://xworks.gr/ontologies/ccso#MSc_Computer_Science_and_Engineering/CSE_MSc/CSD/SSE/UoC"/>
        <affiliatedWith rdf:resource="http://xworks.gr/ontologies/ccso#PhD_Computer_Science_and_Engineering/CSE_PhD/CSD/SSE/UoC"/>
        <affiliatedWith rdf:resource="http://xworks.gr/ontologies/ccso#TP10K4s1/IE_BSc/IED/STEF/TEIC"/>
        <affiliatedWith rdf:resource="http://xworks.gr/ontologies/ccso#TP20K4s1/IE_BSc/IED/STEF/TEIC"/>
        <alumnusOf rdf:resource="http://xworks.gr/ontologies/ccso#Computers_Sciences_Department_of_University_of_Crete"/>
        <hasDegree rdf:resource="http://xworks.gr/ontologies/ccso#BSc_Computer_Science/CS_BSc/CSD/SSE/UoC"/>
        <hasDegree rdf:resource="http://xworks.gr/ontologies/ccso#MSc_Computer_Science_and_Engineering/CSE_MSc/CSD/SSE/UoC"/>
        <hasDegree rdf:resource="http://xworks.gr/ontologies/ccso#PhD_Computer_Science_and_Engineering/CSE_PhD/CSD/SSE/UoC"/>
        <hasPublication rdf:resource="http://xworks.gr/ontologies/ccso#Kalogiannakis2009AdultEducationLifelongLearning"/>
        <hasPublication rdf:resource="http://xworks.gr/ontologies/ccso#Marakakis2005ExpertSystem"/>
        <hasPublication rdf:resource="http://xworks.gr/ontologies/ccso#Papachristou2010EducationalModel"/>
        <hasPublication rdf:resource="http://xworks.gr/ontologies/ccso#Vassilakis2005AsynchronousTeleTeaching"/>
        <instructorOf rdf:resource="http://xworks.gr/ontologies/ccso#IM209s1/IM_MSc/IED/STEF/TEI"/>
        <instructorOf rdf:resource="http://xworks.gr/ontologies/ccso#TP10K4s1/IE_BSc/IED/STEF/TEIC"/>
        <instructorOf rdf:resource="http://xworks.gr/ontologies/ccso#TP20K4s1/IE_BSc/IED/STEF/TEIC"/>
        <memberOf rdf:resource="http://xworks.gr/ontologies/ccso#Department_of_Informatics_Engineering_of_TEI_of_Crete"/>
        <supervisorOf rdf:resource="http://xworks.gr/ontologies/ccso#IM209s1/IM_MSc/IED/STEF/TEI"/>
        <supervisorOf rdf:resource="http://xworks.gr/ontologies/ccso#TP10K4s1/IE_BSc/IED/STEF/TEIC"/>
        <supervisorOf rdf:resource="http://xworks.gr/ontologies/ccso#TP20K4s1/IE_BSc/IED/STEF/TEIC"/>
        <worksFor rdf:resource="http://xworks.gr/ontologies/ccso#Department_of_Informatics_Engineering_of_TEI_of_Crete"/>
        <schema:email rdf:datatype="http://www.w3.org/2001/XMLSchema#anyURI">kostas@cs.teicrete.gr</schema:email>
        <foaf:firstName rdf:datatype="http://www.w3.org/2001/XMLSchema#string">Konstantinos</foaf:firstName>
        <foaf:gender rdf:datatype="http://www.w3.org/2001/XMLSchema#string">Male</foaf:gender>
        <foaf:lastName rdf:datatype="http://www.w3.org/2001/XMLSchema#string">Vassilakis</foaf:lastName>
        <foaf:title rdf:datatype="http://www.w3.org/2001/XMLSchema#string">Dr</foaf:title>
        <eContactInfo rdf:datatype="http://www.w3.org/2001/XMLSchema#anyURI">kostas@cs.teicrete.gr</eContactInfo>
        <workEmail rdf:datatype="http://www.w3.org/2001/XMLSchema#anyURI">kostas@cs.teicrete.gr</workEmail>
        <rdfs:label xml:lang="en">Vassilakis Kostas</rdfs:label>
    </owl:NamedIndividual>
    


    <!-- http://xworks.gr/ontologies/ccso#Vassilakis_Vassilis -->

    <owl:NamedIndividual rdf:about="http://xworks.gr/ontologies/ccso#Vassilakis_Vassilis">
        <rdf:type rdf:resource="http://xmlns.com/foaf/0.1/Agent"/>
        <rdf:type rdf:resource="http://xmlns.com/foaf/0.1/Person"/>
        <rdf:type rdf:resource="http://xworks.gr/ontologies/ccso#PostgraduateStudent"/>
        <rdf:type rdf:resource="http://xworks.gr/ontologies/ccso#Student"/>
        <affiliatedWith rdf:resource="http://xworks.gr/ontologies/ccso#Computers_Sciences_Department_of_University_of_Crete"/>
        <affiliatedWith rdf:resource="http://xworks.gr/ontologies/ccso#BSc_Computer_Science/CS_BSc/CSD/SSE/UoC"/>
        <affiliatedWith rdf:resource="http://xworks.gr/ontologies/ccso#MSc_Computer_Science_and_Engineering/CSE_MSc/CSD/SSE/UoC"/>
        <alumnusOf rdf:resource="http://xworks.gr/ontologies/ccso#Computers_Sciences_Department_of_University_of_Crete"/>
        <enrolledIn rdf:resource="http://xworks.gr/ontologies/ccso#MSc_Computer_Science_and_Engineering/CSE_MSc/CSD/SSE/UoC"/>
        <hasDegree rdf:resource="http://xworks.gr/ontologies/ccso#BSc_Computer_Science/CS_BSc/CSD/SSE/UoC"/>
        <schema:email rdf:datatype="http://www.w3.org/2001/XMLSchema#anyURI">Vassilakis_Vassilis@csd.uoc.gr</schema:email>
        <foaf:firstName rdf:datatype="http://www.w3.org/2001/XMLSchema#string">Vassilis</foaf:firstName>
        <foaf:gender rdf:datatype="http://www.w3.org/2001/XMLSchema#string">Male</foaf:gender>
        <foaf:lastName rdf:datatype="http://www.w3.org/2001/XMLSchema#string">Vassilakis</foaf:lastName>
        <eContactInfo rdf:datatype="http://www.w3.org/2001/XMLSchema#anyURI">Vassilakis_Vassilis@csd.uoc.gr</eContactInfo>
    </owl:NamedIndividual>
    


    <!-- http://xworks.gr/ontologies/ccso#Vassileiou_George -->

    <owl:NamedIndividual rdf:about="http://xworks.gr/ontologies/ccso#Vassileiou_George">
        <rdf:type rdf:resource="http://xmlns.com/foaf/0.1/Person"/>
        <rdf:type rdf:resource="http://xworks.gr/ontologies/ccso#Student"/>
        <rdf:type rdf:resource="http://xworks.gr/ontologies/ccso#UndergraduateStudent"/>
        <affiliatedWith rdf:resource="http://xworks.gr/ontologies/ccso#BSc_Informatics_Engineering/IE_BSc/IED/STEF/TEIC"/>
        <affiliatedWith rdf:resource="http://xworks.gr/ontologies/ccso#TP10K1/IE_BSc/IED/STEF/TEIC"/>
        <affiliatedWith rdf:resource="http://xworks.gr/ontologies/ccso#TP10K2/IE_BSc/IED/STEF/TEIC"/>
        <affiliatedWith rdf:resource="http://xworks.gr/ontologies/ccso#TP10K3/IE_BSc/IED/STEF/TEIC"/>
        <affiliatedWith rdf:resource="http://xworks.gr/ontologies/ccso#TP10K4/IE_BSc/IED/STEF/TEIC"/>
        <affiliatedWith rdf:resource="http://xworks.gr/ontologies/ccso#TP10K5/IE_BSc/IED/STEF/TEIC"/>
        <affiliatedWith rdf:resource="http://xworks.gr/ontologies/ccso#TP10K6/IE_BSc/IED/STEF/TEIC"/>
        <affiliatedWith rdf:resource="http://xworks.gr/ontologies/ccso#TP20K1/IE_BSc/IED/STEF/TEIC"/>
        <affiliatedWith rdf:resource="http://xworks.gr/ontologies/ccso#TP20K2/IE_BSc/IED/STEF/TEIC"/>
        <affiliatedWith rdf:resource="http://xworks.gr/ontologies/ccso#TP20K3/IE_BSc/IED/STEF/TEIC"/>
        <affiliatedWith rdf:resource="http://xworks.gr/ontologies/ccso#TP20K4/IE_BSc/IED/STEF/TEIC"/>
        <affiliatedWith rdf:resource="http://xworks.gr/ontologies/ccso#TP20K6/IE_BSc/IED/STEF/TEIC"/>
        <affiliatedWith rdf:resource="http://xworks.gr/ontologies/ccso#TP20K7/IE_BSc/IED/STEF/TEIC"/>
        <enrolledIn rdf:resource="http://xworks.gr/ontologies/ccso#BSc_Informatics_Engineering/IE_BSc/IED/STEF/TEIC"/>
        <hasCompleted rdf:resource="http://xworks.gr/ontologies/ccso#TP10K1/IE_BSc/IED/STEF/TEIC"/>
        <hasCompleted rdf:resource="http://xworks.gr/ontologies/ccso#TP10K2/IE_BSc/IED/STEF/TEIC"/>
        <hasCompleted rdf:resource="http://xworks.gr/ontologies/ccso#TP10K3/IE_BSc/IED/STEF/TEIC"/>
        <hasCompleted rdf:resource="http://xworks.gr/ontologies/ccso#TP10K4/IE_BSc/IED/STEF/TEIC"/>
        <hasCompleted rdf:resource="http://xworks.gr/ontologies/ccso#TP10K5/IE_BSc/IED/STEF/TEIC"/>
        <hasCompleted rdf:resource="http://xworks.gr/ontologies/ccso#TP10K6/IE_BSc/IED/STEF/TEIC"/>
        <hasCompleted rdf:resource="http://xworks.gr/ontologies/ccso#TP20K1/IE_BSc/IED/STEF/TEIC"/>
        <hasCompleted rdf:resource="http://xworks.gr/ontologies/ccso#TP20K2/IE_BSc/IED/STEF/TEIC"/>
        <hasCompleted rdf:resource="http://xworks.gr/ontologies/ccso#TP20K3/IE_BSc/IED/STEF/TEIC"/>
        <hasCompleted rdf:resource="http://xworks.gr/ontologies/ccso#TP20K4/IE_BSc/IED/STEF/TEIC"/>
        <hasCompleted rdf:resource="http://xworks.gr/ontologies/ccso#TP20K6/IE_BSc/IED/STEF/TEIC"/>
        <hasCompleted rdf:resource="http://xworks.gr/ontologies/ccso#TP20K7/IE_BSc/IED/STEF/TEIC"/>
        <schema:email rdf:datatype="http://www.w3.org/2001/XMLSchema#anyURI">Vassileiou_George@ie.teic.gr</schema:email>
        <foaf:firstName rdf:datatype="http://www.w3.org/2001/XMLSchema#string">George</foaf:firstName>
        <foaf:lastName rdf:datatype="http://www.w3.org/2001/XMLSchema#string">Vassileiou</foaf:lastName>
        <eContactInfo rdf:datatype="http://www.w3.org/2001/XMLSchema#anyURI">Vassileiou_George@ie.teic.gr</eContactInfo>
    </owl:NamedIndividual>
    


    <!-- http://xworks.gr/ontologies/ccso#Vassileiou_Joshua -->

    <owl:NamedIndividual rdf:about="http://xworks.gr/ontologies/ccso#Vassileiou_Joshua">
        <rdf:type rdf:resource="http://xmlns.com/foaf/0.1/Person"/>
        <rdf:type rdf:resource="http://xworks.gr/ontologies/ccso#Student"/>
        <rdf:type rdf:resource="http://xworks.gr/ontologies/ccso#UndergraduateStudent"/>
        <affiliatedWith rdf:resource="http://xworks.gr/ontologies/ccso#BSc_Informatics_Engineering/IE_BSc/IED/STEF/TEIC"/>
        <affiliatedWith rdf:resource="http://xworks.gr/ontologies/ccso#TP10K1/IE_BSc/IED/STEF/TEIC"/>
        <affiliatedWith rdf:resource="http://xworks.gr/ontologies/ccso#TP10K2/IE_BSc/IED/STEF/TEIC"/>
        <affiliatedWith rdf:resource="http://xworks.gr/ontologies/ccso#TP10K3/IE_BSc/IED/STEF/TEIC"/>
        <affiliatedWith rdf:resource="http://xworks.gr/ontologies/ccso#TP10K4/IE_BSc/IED/STEF/TEIC"/>
        <affiliatedWith rdf:resource="http://xworks.gr/ontologies/ccso#TP10K5/IE_BSc/IED/STEF/TEIC"/>
        <affiliatedWith rdf:resource="http://xworks.gr/ontologies/ccso#TP10K6/IE_BSc/IED/STEF/TEIC"/>
        <attendsCourse rdf:resource="http://xworks.gr/ontologies/ccso#TP10K4/IE_BSc/IED/STEF/TEIC"/>
        <enrolledIn rdf:resource="http://xworks.gr/ontologies/ccso#BSc_Informatics_Engineering/IE_BSc/IED/STEF/TEIC"/>
        <hasCompleted rdf:resource="http://xworks.gr/ontologies/ccso#TP10K1/IE_BSc/IED/STEF/TEIC"/>
        <hasCompleted rdf:resource="http://xworks.gr/ontologies/ccso#TP10K2/IE_BSc/IED/STEF/TEIC"/>
        <hasCompleted rdf:resource="http://xworks.gr/ontologies/ccso#TP10K3/IE_BSc/IED/STEF/TEIC"/>
        <hasCompleted rdf:resource="http://xworks.gr/ontologies/ccso#TP10K5/IE_BSc/IED/STEF/TEIC"/>
        <hasCompleted rdf:resource="http://xworks.gr/ontologies/ccso#TP10K6/IE_BSc/IED/STEF/TEIC"/>
        <schema:email rdf:datatype="http://www.w3.org/2001/XMLSchema#anyURI">Vassileiou_Joshua@ie.teic.gr</schema:email>
        <foaf:familyName rdf:datatype="http://www.w3.org/2001/XMLSchema#string">Vassileiou</foaf:familyName>
        <foaf:firstName rdf:datatype="http://www.w3.org/2001/XMLSchema#string">Joshua</foaf:firstName>
        <foaf:lastName rdf:datatype="http://www.w3.org/2001/XMLSchema#string">Vassileiou</foaf:lastName>
        <eContactInfo rdf:datatype="http://www.w3.org/2001/XMLSchema#anyURI">Vassileiou_Joshua@ie.teic.gr</eContactInfo>
    </owl:NamedIndividual>
    


    <!-- http://xworks.gr/ontologies/ccso#Vassileiou_Marcela -->

    <owl:NamedIndividual rdf:about="http://xworks.gr/ontologies/ccso#Vassileiou_Marcela">
        <rdf:type rdf:resource="http://xmlns.com/foaf/0.1/Agent"/>
        <rdf:type rdf:resource="http://xmlns.com/foaf/0.1/Person"/>
        <rdf:type rdf:resource="http://xworks.gr/ontologies/ccso#Student"/>
        <rdf:type rdf:resource="http://xworks.gr/ontologies/ccso#UndergraduateStudent"/>
        <affiliatedWith rdf:resource="http://xworks.gr/ontologies/ccso#BSc_Informatics_Engineering/IE_BSc/IED/STEF/TEIC"/>
        <affiliatedWith rdf:resource="http://xworks.gr/ontologies/ccso#TP10K1/IE_BSc/IED/STEF/TEIC"/>
        <affiliatedWith rdf:resource="http://xworks.gr/ontologies/ccso#TP10K2/IE_BSc/IED/STEF/TEIC"/>
        <affiliatedWith rdf:resource="http://xworks.gr/ontologies/ccso#TP10K3/IE_BSc/IED/STEF/TEIC"/>
        <affiliatedWith rdf:resource="http://xworks.gr/ontologies/ccso#TP10K4/IE_BSc/IED/STEF/TEIC"/>
        <affiliatedWith rdf:resource="http://xworks.gr/ontologies/ccso#TP10K5/IE_BSc/IED/STEF/TEIC"/>
        <affiliatedWith rdf:resource="http://xworks.gr/ontologies/ccso#TP10K6/IE_BSc/IED/STEF/TEIC"/>
        <affiliatedWith rdf:resource="http://xworks.gr/ontologies/ccso#TP20K1/IE_BSc/IED/STEF/TEIC"/>
        <affiliatedWith rdf:resource="http://xworks.gr/ontologies/ccso#TP20K2/IE_BSc/IED/STEF/TEIC"/>
        <affiliatedWith rdf:resource="http://xworks.gr/ontologies/ccso#TP20K3/IE_BSc/IED/STEF/TEIC"/>
        <affiliatedWith rdf:resource="http://xworks.gr/ontologies/ccso#TP20K4/IE_BSc/IED/STEF/TEIC"/>
        <affiliatedWith rdf:resource="http://xworks.gr/ontologies/ccso#TP20K6/IE_BSc/IED/STEF/TEIC"/>
        <affiliatedWith rdf:resource="http://xworks.gr/ontologies/ccso#TP20K7/IE_BSc/IED/STEF/TEIC"/>
        <affiliatedWith rdf:resource="http://xworks.gr/ontologies/ccso#TP30K1/IE_BSc/IED/STEF/TEIC"/>
        <affiliatedWith rdf:resource="http://xworks.gr/ontologies/ccso#TP30K2/IE_BSc/IED/STEF/TEIC"/>
        <affiliatedWith rdf:resource="http://xworks.gr/ontologies/ccso#TP30K4/IE_BSc/IED/STEF/TEIC"/>
        <affiliatedWith rdf:resource="http://xworks.gr/ontologies/ccso#TP30K5/IE_BSc/IED/STEF/TEIC"/>
        <affiliatedWith rdf:resource="http://xworks.gr/ontologies/ccso#TP30K6/IE_BSc/IED/STEF/TEIC"/>
        <attendsCourse rdf:resource="http://xworks.gr/ontologies/ccso#TP30K1/IE_BSc/IED/STEF/TEIC"/>
        <attendsCourse rdf:resource="http://xworks.gr/ontologies/ccso#TP30K2/IE_BSc/IED/STEF/TEIC"/>
        <attendsCourse rdf:resource="http://xworks.gr/ontologies/ccso#TP30K4/IE_BSc/IED/STEF/TEIC"/>
        <attendsCourse rdf:resource="http://xworks.gr/ontologies/ccso#TP30K5/IE_BSc/IED/STEF/TEIC"/>
        <attendsCourse rdf:resource="http://xworks.gr/ontologies/ccso#TP30K6/IE_BSc/IED/STEF/TEIC"/>
        <enrolledIn rdf:resource="http://xworks.gr/ontologies/ccso#BSc_Informatics_Engineering/IE_BSc/IED/STEF/TEIC"/>
        <hasCompleted rdf:resource="http://xworks.gr/ontologies/ccso#TP10K1/IE_BSc/IED/STEF/TEIC"/>
        <hasCompleted rdf:resource="http://xworks.gr/ontologies/ccso#TP10K2/IE_BSc/IED/STEF/TEIC"/>
        <hasCompleted rdf:resource="http://xworks.gr/ontologies/ccso#TP10K3/IE_BSc/IED/STEF/TEIC"/>
        <hasCompleted rdf:resource="http://xworks.gr/ontologies/ccso#TP10K4/IE_BSc/IED/STEF/TEIC"/>
        <hasCompleted rdf:resource="http://xworks.gr/ontologies/ccso#TP10K5/IE_BSc/IED/STEF/TEIC"/>
        <hasCompleted rdf:resource="http://xworks.gr/ontologies/ccso#TP10K6/IE_BSc/IED/STEF/TEIC"/>
        <hasCompleted rdf:resource="http://xworks.gr/ontologies/ccso#TP20K1/IE_BSc/IED/STEF/TEIC"/>
        <hasCompleted rdf:resource="http://xworks.gr/ontologies/ccso#TP20K2/IE_BSc/IED/STEF/TEIC"/>
        <hasCompleted rdf:resource="http://xworks.gr/ontologies/ccso#TP20K3/IE_BSc/IED/STEF/TEIC"/>
        <hasCompleted rdf:resource="http://xworks.gr/ontologies/ccso#TP20K4/IE_BSc/IED/STEF/TEIC"/>
        <hasCompleted rdf:resource="http://xworks.gr/ontologies/ccso#TP20K6/IE_BSc/IED/STEF/TEIC"/>
        <hasCompleted rdf:resource="http://xworks.gr/ontologies/ccso#TP20K7/IE_BSc/IED/STEF/TEIC"/>
        <schema:email rdf:datatype="http://www.w3.org/2001/XMLSchema#anyURI">Vassileiou_Marcela@ie.teicrete.gr</schema:email>
        <foaf:familyName rdf:datatype="http://www.w3.org/2001/XMLSchema#string">Vassileiou</foaf:familyName>
        <foaf:firstName rdf:datatype="http://www.w3.org/2001/XMLSchema#string">Marcela</foaf:firstName>
        <foaf:gender rdf:datatype="http://www.w3.org/2001/XMLSchema#string">Female</foaf:gender>
        <foaf:lastName rdf:datatype="http://www.w3.org/2001/XMLSchema#string">Vassileiou</foaf:lastName>
        <eContactInfo rdf:datatype="http://www.w3.org/2001/XMLSchema#anyURI">Vassileiou_Marcela@ie.teicrete.gr</eContactInfo>
    </owl:NamedIndividual>
    


    <!-- http://xworks.gr/ontologies/ccso#Vassileiou_Stathis -->

    <owl:NamedIndividual rdf:about="http://xworks.gr/ontologies/ccso#Vassileiou_Stathis">
        <rdf:type rdf:resource="http://xmlns.com/foaf/0.1/Agent"/>
        <rdf:type rdf:resource="http://xmlns.com/foaf/0.1/Person"/>
        <rdf:type rdf:resource="http://xworks.gr/ontologies/ccso#Student"/>
        <schema:email rdf:datatype="http://www.w3.org/2001/XMLSchema#anyURI">Vassileiou_Stathis@mail.gr</schema:email>
        <foaf:familyName rdf:datatype="http://www.w3.org/2001/XMLSchema#string">Vassileiou</foaf:familyName>
        <foaf:firstName rdf:datatype="http://www.w3.org/2001/XMLSchema#string">Stathis</foaf:firstName>
        <foaf:gender rdf:datatype="http://www.w3.org/2001/XMLSchema#string">Male</foaf:gender>
        <foaf:lastName rdf:datatype="http://www.w3.org/2001/XMLSchema#string">Vassileiou</foaf:lastName>
        <eContactInfo rdf:datatype="http://www.w3.org/2001/XMLSchema#anyURI">Vassileiou_Stathis@mail.gr</eContactInfo>
    </owl:NamedIndividual>
    


    <!-- http://xworks.gr/ontologies/ccso#Vassileiou_Tom -->

    <owl:NamedIndividual rdf:about="http://xworks.gr/ontologies/ccso#Vassileiou_Tom">
        <rdf:type rdf:resource="http://xmlns.com/foaf/0.1/Agent"/>
        <rdf:type rdf:resource="http://xmlns.com/foaf/0.1/Person"/>
        <rdf:type rdf:resource="http://xworks.gr/ontologies/ccso#PostgraduateStudent"/>
        <rdf:type rdf:resource="http://xworks.gr/ontologies/ccso#Student"/>
        <affiliatedWith rdf:resource="http://xworks.gr/ontologies/ccso#Department_of_Informatics_Engineering_of_TEI_of_Crete"/>
        <affiliatedWith rdf:resource="http://xworks.gr/ontologies/ccso#BSc_Informatics_Engineering/IE_BSc/IED/STEF/TEIC"/>
        <affiliatedWith rdf:resource="http://xworks.gr/ontologies/ccso#IM101/IM_MSc/IED/STEF/TEIC"/>
        <affiliatedWith rdf:resource="http://xworks.gr/ontologies/ccso#IM102/IM_MSc/IED/STEF/TEIC"/>
        <affiliatedWith rdf:resource="http://xworks.gr/ontologies/ccso#IM103/IM_MSc/IED/STEF/TEIC"/>
        <affiliatedWith rdf:resource="http://xworks.gr/ontologies/ccso#IM104/IM_MSc/IED/STEF/TEIC"/>
        <affiliatedWith rdf:resource="http://xworks.gr/ontologies/ccso#IM105/IM_MSc/IED/STEF/TEIC"/>
        <affiliatedWith rdf:resource="http://xworks.gr/ontologies/ccso#IM106/IM_MSc/IED/STEF/TEIC"/>
        <affiliatedWith rdf:resource="http://xworks.gr/ontologies/ccso#IM108/IM_MSc/IED/STEF/TEIC"/>
        <affiliatedWith rdf:resource="http://xworks.gr/ontologies/ccso#IM109/IM_MSc/IED/STEF/TEIC"/>
        <affiliatedWith rdf:resource="http://xworks.gr/ontologies/ccso#IM201/IM_MSc/IED/STEF/TEIC"/>
        <affiliatedWith rdf:resource="http://xworks.gr/ontologies/ccso#IM202/IM_MSc/IED/STEF/TEIC"/>
        <affiliatedWith rdf:resource="http://xworks.gr/ontologies/ccso#IM203/IM_MSc/IED/STEF/TEIC"/>
        <affiliatedWith rdf:resource="http://xworks.gr/ontologies/ccso#IM205/IM_MSc/IED/STEF/TEIC"/>
        <affiliatedWith rdf:resource="http://xworks.gr/ontologies/ccso#IM208/IM_MSc/IED/STEF/TEIC"/>
        <affiliatedWith rdf:resource="http://xworks.gr/ontologies/ccso#IM209/IM_MSc/IED/STEF/TEIC"/>
        <affiliatedWith rdf:resource="http://xworks.gr/ontologies/ccso#MSc_Informatics_&amp;_Multimedia/IM_MSc/IED/STEF/TEIC"/>
        <alumnusOf rdf:resource="http://xworks.gr/ontologies/ccso#Department_of_Informatics_Engineering_of_TEI_of_Crete"/>
        <attendsCourse rdf:resource="http://xworks.gr/ontologies/ccso#IM201/IM_MSc/IED/STEF/TEIC"/>
        <attendsCourse rdf:resource="http://xworks.gr/ontologies/ccso#IM202/IM_MSc/IED/STEF/TEIC"/>
        <attendsCourse rdf:resource="http://xworks.gr/ontologies/ccso#IM203/IM_MSc/IED/STEF/TEIC"/>
        <attendsCourse rdf:resource="http://xworks.gr/ontologies/ccso#IM205/IM_MSc/IED/STEF/TEIC"/>
        <attendsCourse rdf:resource="http://xworks.gr/ontologies/ccso#IM208/IM_MSc/IED/STEF/TEIC"/>
        <attendsCourse rdf:resource="http://xworks.gr/ontologies/ccso#IM209/IM_MSc/IED/STEF/TEIC"/>
        <enrolledIn rdf:resource="http://xworks.gr/ontologies/ccso#MSc_Informatics_&amp;_Multimedia/IM_MSc/IED/STEF/TEIC"/>
        <hasCompleted rdf:resource="http://xworks.gr/ontologies/ccso#IM101/IM_MSc/IED/STEF/TEIC"/>
        <hasCompleted rdf:resource="http://xworks.gr/ontologies/ccso#IM102/IM_MSc/IED/STEF/TEIC"/>
        <hasCompleted rdf:resource="http://xworks.gr/ontologies/ccso#IM103/IM_MSc/IED/STEF/TEIC"/>
        <hasCompleted rdf:resource="http://xworks.gr/ontologies/ccso#IM104/IM_MSc/IED/STEF/TEIC"/>
        <hasCompleted rdf:resource="http://xworks.gr/ontologies/ccso#IM105/IM_MSc/IED/STEF/TEIC"/>
        <hasCompleted rdf:resource="http://xworks.gr/ontologies/ccso#IM106/IM_MSc/IED/STEF/TEIC"/>
        <hasCompleted rdf:resource="http://xworks.gr/ontologies/ccso#IM108/IM_MSc/IED/STEF/TEIC"/>
        <hasCompleted rdf:resource="http://xworks.gr/ontologies/ccso#IM109/IM_MSc/IED/STEF/TEIC"/>
        <hasDegree rdf:resource="http://xworks.gr/ontologies/ccso#BSc_Informatics_Engineering/IE_BSc/IED/STEF/TEIC"/>
        <schema:email rdf:datatype="http://www.w3.org/2001/XMLSchema#anyURI">Vassileiou_Tom@ie.teicrete.gr</schema:email>
        <foaf:familyName rdf:datatype="http://www.w3.org/2001/XMLSchema#string">Vassileiou</foaf:familyName>
        <foaf:firstName rdf:datatype="http://www.w3.org/2001/XMLSchema#string">Tom</foaf:firstName>
        <foaf:gender rdf:datatype="http://www.w3.org/2001/XMLSchema#string">Male</foaf:gender>
        <foaf:lastName rdf:datatype="http://www.w3.org/2001/XMLSchema#string">Vassileiou</foaf:lastName>
        <eContactInfo rdf:datatype="http://www.w3.org/2001/XMLSchema#anyURI">Vassileiou_Tom@ie.teicrete.gr</eContactInfo>
    </owl:NamedIndividual>
    


    <!-- http://xworks.gr/ontologies/ccso#Vassileiou_Vassilis -->

    <owl:NamedIndividual rdf:about="http://xworks.gr/ontologies/ccso#Vassileiou_Vassilis">
        <rdf:type rdf:resource="http://xmlns.com/foaf/0.1/Agent"/>
        <rdf:type rdf:resource="http://xmlns.com/foaf/0.1/Person"/>
        <rdf:type rdf:resource="http://xworks.gr/ontologies/ccso#Student"/>
        <schema:email rdf:datatype="http://www.w3.org/2001/XMLSchema#anyURI">Vassileiou_Vassilis@mail.gr</schema:email>
        <foaf:familyName rdf:datatype="http://www.w3.org/2001/XMLSchema#string">Vassileiou</foaf:familyName>
        <foaf:firstName rdf:datatype="http://www.w3.org/2001/XMLSchema#string">Vassilis</foaf:firstName>
        <foaf:gender rdf:datatype="http://www.w3.org/2001/XMLSchema#string">Male</foaf:gender>
        <foaf:lastName rdf:datatype="http://www.w3.org/2001/XMLSchema#string">Vassileiou</foaf:lastName>
        <eContactInfo rdf:datatype="http://www.w3.org/2001/XMLSchema#anyURI">Vassileiou_Vassilis@mail.gr</eContactInfo>
    </owl:NamedIndividual>
    


    <!-- http://xworks.gr/ontologies/ccso#Vidakis_Nikolaos -->

    <owl:NamedIndividual rdf:about="http://xworks.gr/ontologies/ccso#Vidakis_Nikolaos">
        <rdf:type rdf:resource="http://xmlns.com/foaf/0.1/Person"/>
        <rdf:type rdf:resource="http://xworks.gr/ontologies/ccso#AcademicStaff"/>
        <rdf:type rdf:resource="http://xworks.gr/ontologies/ccso#Employee"/>
        <rdf:type rdf:resource="http://xworks.gr/ontologies/ccso#Professor"/>
        <affiliatedWith rdf:resource="http://xworks.gr/ontologies/ccso#Department_of_Informatics_Engineering_of_TEI_of_Crete"/>
        <affiliatedWith rdf:resource="http://xworks.gr/ontologies/ccso#IM104s1/IM_MSc/IED/STEF/TEI"/>
        <affiliatedWith rdf:resource="http://xworks.gr/ontologies/ccso#IM202s1/IM_MSc/IED/STEF/TEI"/>
        <affiliatedWith rdf:resource="http://xworks.gr/ontologies/ccso#TP40K4s1/IE_BSc/IED/STEF/TEIC"/>
        <affiliatedWith rdf:resource="http://xworks.gr/ontologies/ccso#TP50L2s1/IE_BSc/IED/STEF/TEIC"/>
        <instructorOf rdf:resource="http://xworks.gr/ontologies/ccso#IM104s1/IM_MSc/IED/STEF/TEI"/>
        <instructorOf rdf:resource="http://xworks.gr/ontologies/ccso#IM202s1/IM_MSc/IED/STEF/TEI"/>
        <instructorOf rdf:resource="http://xworks.gr/ontologies/ccso#TP40K4s1/IE_BSc/IED/STEF/TEIC"/>
        <instructorOf rdf:resource="http://xworks.gr/ontologies/ccso#TP50L2s1/IE_BSc/IED/STEF/TEIC"/>
        <memberOf rdf:resource="http://xworks.gr/ontologies/ccso#Department_of_Informatics_Engineering_of_TEI_of_Crete"/>
        <supervisorOf rdf:resource="http://xworks.gr/ontologies/ccso#IM104s1/IM_MSc/IED/STEF/TEI"/>
        <supervisorOf rdf:resource="http://xworks.gr/ontologies/ccso#TP40K4s1/IE_BSc/IED/STEF/TEIC"/>
        <supervisorOf rdf:resource="http://xworks.gr/ontologies/ccso#TP50L2s1/IE_BSc/IED/STEF/TEIC"/>
        <worksFor rdf:resource="http://xworks.gr/ontologies/ccso#Department_of_Informatics_Engineering_of_TEI_of_Crete"/>
        <schema:email rdf:datatype="http://www.w3.org/2001/XMLSchema#anyURI">vidakis@ie.teicrete.gr</schema:email>
        <foaf:firstName rdf:datatype="http://www.w3.org/2001/XMLSchema#string">Nikolaos</foaf:firstName>
        <foaf:lastName rdf:datatype="http://www.w3.org/2001/XMLSchema#string">Vidakis</foaf:lastName>
        <eContactInfo rdf:datatype="http://www.w3.org/2001/XMLSchema#anyURI">vidakis@ie.teicrete.gr</eContactInfo>
    </owl:NamedIndividual>
    


    <!-- http://xworks.gr/ontologies/ccso#Vourkas_Michail -->

    <owl:NamedIndividual rdf:about="http://xworks.gr/ontologies/ccso#Vourkas_Michail">
        <rdf:type rdf:resource="http://xmlns.com/foaf/0.1/Person"/>
        <rdf:type rdf:resource="http://xworks.gr/ontologies/ccso#AcademicStaff"/>
        <rdf:type rdf:resource="http://xworks.gr/ontologies/ccso#Employee"/>
        <rdf:type rdf:resource="http://xworks.gr/ontologies/ccso#Professor"/>
        <affiliatedWith rdf:resource="http://xworks.gr/ontologies/ccso#Department_of_Informatics_Engineering_of_TEI_of_Crete"/>
        <affiliatedWith rdf:resource="http://xworks.gr/ontologies/ccso#IM102s1/IM_MSc/IED/STEF/TEI"/>
        <instructorOf rdf:resource="http://xworks.gr/ontologies/ccso#IM102s1/IM_MSc/IED/STEF/TEI"/>
        <memberOf rdf:resource="http://xworks.gr/ontologies/ccso#Department_of_Informatics_Engineering_of_TEI_of_Crete"/>
        <worksFor rdf:resource="http://xworks.gr/ontologies/ccso#Department_of_Informatics_Engineering_of_TEI_of_Crete"/>
        <schema:email rdf:datatype="http://www.w3.org/2001/XMLSchema#anyURI">vourkas@ie.teicrete.gr</schema:email>
        <foaf:firstName rdf:datatype="http://www.w3.org/2001/XMLSchema#string">Michail</foaf:firstName>
        <foaf:lastName rdf:datatype="http://www.w3.org/2001/XMLSchema#string">Vourkas</foaf:lastName>
        <eContactInfo rdf:datatype="http://www.w3.org/2001/XMLSchema#anyURI">vourkas@ie.teicrete.gr</eContactInfo>
    </owl:NamedIndividual>
    


    <!-- http://xworks.gr/ontologies/ccso#WrittenExam -->

    <owl:NamedIndividual rdf:about="http://xworks.gr/ontologies/ccso#WrittenExam">
        <rdf:type rdf:resource="http://xworks.gr/ontologies/ccso#TeachingEvaluationMethod"/>
        <methodName rdf:datatype="http://www.w3.org/2001/XMLSchema#string">WrittenExamination</methodName>
    </owl:NamedIndividual>
    


    <!-- http://xworks.gr/ontologies/ccso#Xezonakis_Ioannis -->

    <owl:NamedIndividual rdf:about="http://xworks.gr/ontologies/ccso#Xezonakis_Ioannis">
        <rdf:type rdf:resource="http://xmlns.com/foaf/0.1/Person"/>
        <rdf:type rdf:resource="http://xworks.gr/ontologies/ccso#AcademicStaff"/>
        <rdf:type rdf:resource="http://xworks.gr/ontologies/ccso#Employee"/>
        <rdf:type rdf:resource="http://xworks.gr/ontologies/ccso#Professor"/>
        <affiliatedWith rdf:resource="http://xworks.gr/ontologies/ccso#Department_of_Informatics_Engineering_of_TEI_of_Crete"/>
        <affiliatedWith rdf:resource="http://xworks.gr/ontologies/ccso#TP10K6s1/IE_BSc/IED/STEF/TEIC"/>
        <affiliatedWith rdf:resource="http://xworks.gr/ontologies/ccso#TP40K6s1/IE_BSc/IED/STEF/TEIC"/>
        <instructorOf rdf:resource="http://xworks.gr/ontologies/ccso#TP10K6s1/IE_BSc/IED/STEF/TEIC"/>
        <instructorOf rdf:resource="http://xworks.gr/ontologies/ccso#TP40K6s1/IE_BSc/IED/STEF/TEIC"/>
        <memberOf rdf:resource="http://xworks.gr/ontologies/ccso#Department_of_Informatics_Engineering_of_TEI_of_Crete"/>
        <supervisorOf rdf:resource="http://xworks.gr/ontologies/ccso#TP10K6s1/IE_BSc/IED/STEF/TEIC"/>
        <supervisorOf rdf:resource="http://xworks.gr/ontologies/ccso#TP40K6s1/IE_BSc/IED/STEF/TEIC"/>
        <worksFor rdf:resource="http://xworks.gr/ontologies/ccso#Department_of_Informatics_Engineering_of_TEI_of_Crete"/>
        <schema:email rdf:datatype="http://www.w3.org/2001/XMLSchema#anyURI">xezonakis@ie.teicrete.gr</schema:email>
        <foaf:firstName rdf:datatype="http://www.w3.org/2001/XMLSchema#string">Ioannis</foaf:firstName>
        <foaf:lastName rdf:datatype="http://www.w3.org/2001/XMLSchema#string">Xezonakis</foaf:lastName>
        <eContactInfo rdf:datatype="http://www.w3.org/2001/XMLSchema#anyURI">xezonakis@ie.teicrete.gr</eContactInfo>
    </owl:NamedIndividual>
    


    <!-- http://xworks.gr/ontologies/ccso#1o_IEK_Irakleiou -->

    <owl:NamedIndividual rdf:about="http://xworks.gr/ontologies/ccso#1o_IEK_Irakleiou">
        <rdf:type rdf:resource="http://schema.org/EducationalOrganization"/>
        <rdf:type rdf:resource="http://schema.org/Organization"/>
        <rdf:type rdf:resource="http://xworks.gr/ontologies/ccso#Institute"/>
    </owl:NamedIndividual>
    


    <!-- http://xworks.gr/ontologies/ccso#BSc_Computer_Science/CS_BSc/CSD/SSE/UoC -->

    <owl:NamedIndividual rdf:about="http://xworks.gr/ontologies/ccso#BSc_Computer_Science/CS_BSc/CSD/SSE/UoC">
        <rdf:type rdf:resource="http://xworks.gr/ontologies/ccso#Bachelor"/>
        <rdf:type rdf:resource="http://xworks.gr/ontologies/ccso#ProgramofStudy"/>
        <affiliatedWith rdf:resource="http://xworks.gr/ontologies/ccso#Starkeiou_Nick"/>
        <affiliatedWith rdf:resource="http://xworks.gr/ontologies/ccso#Starkeiou_Vakis"/>
        <hasRegistered rdf:resource="http://xworks.gr/ontologies/ccso#Starkeiou_Nick"/>
        <hasRegistered rdf:resource="http://xworks.gr/ontologies/ccso#Starkeiou_Vakis"/>
        <includesCourse rdf:resource="http://xworks.gr/ontologies/ccso#CS100/CS_BSc/CSD/SSE/UoC"/>
        <includesCourse rdf:resource="http://xworks.gr/ontologies/ccso#CS108/CS_BSc/CSD/SSE/UoC"/>
        <includesCourse rdf:resource="http://xworks.gr/ontologies/ccso#CS109/CS_BSc/CSD/SSE/UoC"/>
        <includesCourse rdf:resource="http://xworks.gr/ontologies/ccso#CS110/CS_BSc/CSD/SSE/UoC"/>
        <includesCourse rdf:resource="http://xworks.gr/ontologies/ccso#CS118/CS_BSc/CSD/SSE/UoC"/>
        <includesCourse rdf:resource="http://xworks.gr/ontologies/ccso#CS119/CS_BSc/CSD/SSE/UoC"/>
        <includesCourse rdf:resource="http://xworks.gr/ontologies/ccso#CS120/CS_BSc/CSD/SSE/UoC"/>
        <includesCourse rdf:resource="http://xworks.gr/ontologies/ccso#CS150/CS_BSc/CSD/SSE/UoC"/>
        <includesCourse rdf:resource="http://xworks.gr/ontologies/ccso#CS180/CS_BSc/CSD/SSE/UoC"/>
        <includesCourse rdf:resource="http://xworks.gr/ontologies/ccso#CS208/CS_BSc/CSD/SSE/UoC"/>
        <includesCourse rdf:resource="http://xworks.gr/ontologies/ccso#CS209/CS_BSc/CSD/SSE/UoC"/>
        <includesCourse rdf:resource="http://xworks.gr/ontologies/ccso#CS215/CS_BSc/CSD/SSE/UoC"/>
        <includesCourse rdf:resource="http://xworks.gr/ontologies/ccso#CS217/CS_BSc/CSD/SSE/UoC"/>
        <includesCourse rdf:resource="http://xworks.gr/ontologies/ccso#CS220/CS_BSc/CSD/SSE/UoC"/>
        <includesCourse rdf:resource="http://xworks.gr/ontologies/ccso#CS225/CS_BSc/CSD/SSE/UoC"/>
        <includesCourse rdf:resource="http://xworks.gr/ontologies/ccso#CS240/CS_BSc/CSD/SSE/UoC"/>
        <includesCourse rdf:resource="http://xworks.gr/ontologies/ccso#CS252/CS_BSc/CSD/SSE/UoC"/>
        <includesCourse rdf:resource="http://xworks.gr/ontologies/ccso#CS255/CS_BSc/CSD/SSE/UoC"/>
        <includesCourse rdf:resource="http://xworks.gr/ontologies/ccso#CS280/CS_BSc/CSD/SSE/UoC"/>
        <includesCourse rdf:resource="http://xworks.gr/ontologies/ccso#CS302/CS_BSc/CSD/SSE/UoC"/>
        <includesCourse rdf:resource="http://xworks.gr/ontologies/ccso#CS317/CS_BSc/CSD/SSE/UoC"/>
        <includesCourse rdf:resource="http://xworks.gr/ontologies/ccso#CS330/CS_BSc/CSD/SSE/UoC"/>
        <includesCourse rdf:resource="http://xworks.gr/ontologies/ccso#CS335/CS_BSc/CSD/SSE/UoC"/>
        <includesCourse rdf:resource="http://xworks.gr/ontologies/ccso#CS340/CS_BSc/CSD/SSE/UoC"/>
        <includesCourse rdf:resource="http://xworks.gr/ontologies/ccso#CS342/CS_BSc/CSD/SSE/UoC"/>
        <includesCourse rdf:resource="http://xworks.gr/ontologies/ccso#CS345/CS_BSc/CSD/SSE/UoC"/>
        <includesCourse rdf:resource="http://xworks.gr/ontologies/ccso#CS351/CS_BSc/CSD/SSE/UoC"/>
        <includesCourse rdf:resource="http://xworks.gr/ontologies/ccso#CS352/CS_BSc/CSD/SSE/UoC"/>
        <includesCourse rdf:resource="http://xworks.gr/ontologies/ccso#CS358/CS_BSc/CSD/SSE/UoC"/>
        <includesCourse rdf:resource="http://xworks.gr/ontologies/ccso#CS360/CS_BSc/CSD/SSE/UoC"/>
        <includesCourse rdf:resource="http://xworks.gr/ontologies/ccso#CS364/CS_BSc/CSD/SSE/UoC"/>
        <includesCourse rdf:resource="http://xworks.gr/ontologies/ccso#CS370/CS_BSc/CSD/SSE/UoC"/>
        <includesCourse rdf:resource="http://xworks.gr/ontologies/ccso#CS371/CS_BSc/CSD/SSE/UoC"/>
        <includesCourse rdf:resource="http://xworks.gr/ontologies/ccso#CS380/CS_BSc/CSD/SSE/UoC"/>
        <includesCourse rdf:resource="http://xworks.gr/ontologies/ccso#CS383/CS_BSc/CSD/SSE/UoC"/>
        <includesCourse rdf:resource="http://xworks.gr/ontologies/ccso#CS387/CS_BSc/CSD/SSE/UoC"/>
        <includesCourse rdf:resource="http://xworks.gr/ontologies/ccso#CS404/CS_BSc/CSD/SSE/UoC"/>
        <includesCourse rdf:resource="http://xworks.gr/ontologies/ccso#CS422/CS_BSc/CSD/SSE/UoC"/>
        <includesCourse rdf:resource="http://xworks.gr/ontologies/ccso#CS425/CS_BSc/CSD/SSE/UoC"/>
        <includesCourse rdf:resource="http://xworks.gr/ontologies/ccso#CS428/CS_BSc/CSD/SSE/UoC"/>
        <includesCourse rdf:resource="http://xworks.gr/ontologies/ccso#CS435/CS_BSc/CSD/SSE/UoC"/>
        <includesCourse rdf:resource="http://xworks.gr/ontologies/ccso#CS436/CS_BSc/CSD/SSE/UoC"/>
        <includesCourse rdf:resource="http://xworks.gr/ontologies/ccso#CS439/CS_BSc/CSD/SSE/UoC"/>
        <includesCourse rdf:resource="http://xworks.gr/ontologies/ccso#CS446/CS_BSc/CSD/SSE/UoC"/>
        <includesCourse rdf:resource="http://xworks.gr/ontologies/ccso#CS452/CS_BSc/CSD/SSE/UoC"/>
        <includesCourse rdf:resource="http://xworks.gr/ontologies/ccso#CS455/CS_BSc/CSD/SSE/UoC"/>
        <includesCourse rdf:resource="http://xworks.gr/ontologies/ccso#CS457/CS_BSc/CSD/SSE/UoC"/>
        <includesCourse rdf:resource="http://xworks.gr/ontologies/ccso#CS459/CS_BSc/CSD/SSE/UoC"/>
        <includesCourse rdf:resource="http://xworks.gr/ontologies/ccso#CS460/CS_BSc/CSD/SSE/UoC"/>
        <includesCourse rdf:resource="http://xworks.gr/ontologies/ccso#CS463/CS_BSc/CSD/SSE/UoC"/>
        <includesCourse rdf:resource="http://xworks.gr/ontologies/ccso#CS468/CS_BSc/CSD/SSE/UoC"/>
        <includesCourse rdf:resource="http://xworks.gr/ontologies/ccso#CS469/CS_BSc/CSD/SSE/UoC"/>
        <includesCourse rdf:resource="http://xworks.gr/ontologies/ccso#CS471/CS_BSc/CSD/SSE/UoC"/>
        <includesCourse rdf:resource="http://xworks.gr/ontologies/ccso#CS472/CS_BSc/CSD/SSE/UoC"/>
        <includesCourse rdf:resource="http://xworks.gr/ontologies/ccso#CS473/CS_BSc/CSD/SSE/UoC"/>
        <includesCourse rdf:resource="http://xworks.gr/ontologies/ccso#CS474/CS_BSc/CSD/SSE/UoC"/>
        <includesCourse rdf:resource="http://xworks.gr/ontologies/ccso#CS475/CS_BSc/CSD/SSE/UoC"/>
        <includesCourse rdf:resource="http://xworks.gr/ontologies/ccso#CS482/CS_BSc/CSD/SSE/UoC"/>
        <includesCourse rdf:resource="http://xworks.gr/ontologies/ccso#CS486/CS_BSc/CSD/SSE/UoC"/>
        <includesCourse rdf:resource="http://xworks.gr/ontologies/ccso#CS499/CS_BSc/CSD/SSE/UoC"/>
        <providedBy rdf:resource="http://xworks.gr/ontologies/ccso#Computers_Sciences_Department_of_University_of_Crete"/>
        <code rdf:datatype="http://www.w3.org/2001/XMLSchema#string">CS_BSc/CSD/SSE/UoC</code>
        <creditsECTS rdf:datatype="http://www.w3.org/2001/XMLSchema#short">240</creditsECTS>
        <degreeTitle rdf:datatype="http://www.w3.org/2001/XMLSchema#string">Bachelor of Science in Computer Science of University of Crete</degreeTitle>
        <degreeType rdf:datatype="http://www.w3.org/2001/XMLSchema#string">BSc</degreeType>
        <degreeType rdf:datatype="http://www.w3.org/2001/XMLSchema#string">Bachelor of Science</degreeType>
        <degreeURL rdf:datatype="http://www.w3.org/2001/XMLSchema#anyURI">http://csd.uoc.gr/CSD/index.jsp?content=undergrad_regulation&amp;openmenu=demoAcc3&amp;lang=gr</degreeURL>
        <duration rdf:datatype="http://www.w3.org/2001/XMLSchema#duration">P4Y</duration>
        <duration rdf:datatype="internal:anonymous-constants">P4Y</duration>
        <psName rdf:datatype="http://www.w3.org/2001/XMLSchema#string">Bachelor of Science (BSc) in Computer Science of Computers Sciences Department (CSD) of University of Crete</psName>
        <webaddressURL rdf:datatype="http://www.w3.org/2001/XMLSchema#anyURI">http://csd.uoc.gr/CSD/index.jsp?content=undergrad_regulation&amp;openmenu=demoAcc3&amp;lang=gr</webaddressURL>
        <rdfs:label xml:lang="en">Bachelor of Science in Computer Science of University of Crete</rdfs:label>
    </owl:NamedIndividual>
    


    <!-- http://xworks.gr/ontologies/ccso#BSc_Informatics_Engineering/IE_BSc/IED/STEF/TEIC -->

    <owl:NamedIndividual rdf:about="http://xworks.gr/ontologies/ccso#BSc_Informatics_Engineering/IE_BSc/IED/STEF/TEIC">
        <rdf:type rdf:resource="http://xworks.gr/ontologies/ccso#Bachelor"/>
        <rdf:type rdf:resource="http://xworks.gr/ontologies/ccso#ProgramofStudy"/>
        <affiliatedWith rdf:resource="http://xworks.gr/ontologies/ccso#Tarlis_Kostas"/>
        <affiliatedWith rdf:resource="http://xworks.gr/ontologies/ccso#Vassileiou_George"/>
        <affiliatedWith rdf:resource="http://xworks.gr/ontologies/ccso#Vassileiou_Joshua"/>
        <affiliatedWith rdf:resource="http://xworks.gr/ontologies/ccso#Vassileiou_Marcela"/>
        <hasRegistered rdf:resource="http://xworks.gr/ontologies/ccso#Tarlis_Kostas"/>
        <hasRegistered rdf:resource="http://xworks.gr/ontologies/ccso#Vassileiou_George"/>
        <hasRegistered rdf:resource="http://xworks.gr/ontologies/ccso#Vassileiou_Joshua"/>
        <hasRegistered rdf:resource="http://xworks.gr/ontologies/ccso#Vassileiou_Marcela"/>
        <includesCourse rdf:resource="http://xworks.gr/ontologies/ccso#TP10K1/IE_BSc/IED/STEF/TEIC"/>
        <includesCourse rdf:resource="http://xworks.gr/ontologies/ccso#TP10K2/IE_BSc/IED/STEF/TEIC"/>
        <includesCourse rdf:resource="http://xworks.gr/ontologies/ccso#TP10K3/IE_BSc/IED/STEF/TEIC"/>
        <includesCourse rdf:resource="http://xworks.gr/ontologies/ccso#TP10K4/IE_BSc/IED/STEF/TEIC"/>
        <includesCourse rdf:resource="http://xworks.gr/ontologies/ccso#TP10K5/IE_BSc/IED/STEF/TEIC"/>
        <includesCourse rdf:resource="http://xworks.gr/ontologies/ccso#TP10K6/IE_BSc/IED/STEF/TEIC"/>
        <includesCourse rdf:resource="http://xworks.gr/ontologies/ccso#TP20K1/IE_BSc/IED/STEF/TEIC"/>
        <includesCourse rdf:resource="http://xworks.gr/ontologies/ccso#TP20K2/IE_BSc/IED/STEF/TEIC"/>
        <includesCourse rdf:resource="http://xworks.gr/ontologies/ccso#TP20K3/IE_BSc/IED/STEF/TEIC"/>
        <includesCourse rdf:resource="http://xworks.gr/ontologies/ccso#TP20K4/IE_BSc/IED/STEF/TEIC"/>
        <includesCourse rdf:resource="http://xworks.gr/ontologies/ccso#TP20K6/IE_BSc/IED/STEF/TEIC"/>
        <includesCourse rdf:resource="http://xworks.gr/ontologies/ccso#TP20K7/IE_BSc/IED/STEF/TEIC"/>
        <includesCourse rdf:resource="http://xworks.gr/ontologies/ccso#TP30K1/IE_BSc/IED/STEF/TEIC"/>
        <includesCourse rdf:resource="http://xworks.gr/ontologies/ccso#TP30K2/IE_BSc/IED/STEF/TEIC"/>
        <includesCourse rdf:resource="http://xworks.gr/ontologies/ccso#TP30K4/IE_BSc/IED/STEF/TEIC"/>
        <includesCourse rdf:resource="http://xworks.gr/ontologies/ccso#TP30K5/IE_BSc/IED/STEF/TEIC"/>
        <includesCourse rdf:resource="http://xworks.gr/ontologies/ccso#TP30K6/IE_BSc/IED/STEF/TEIC"/>
        <includesCourse rdf:resource="http://xworks.gr/ontologies/ccso#TP30K7/IE_BSc/IED/STEF/TEIC"/>
        <includesCourse rdf:resource="http://xworks.gr/ontologies/ccso#TP40K1/IE_BSc/IED/STEF/TEIC"/>
        <includesCourse rdf:resource="http://xworks.gr/ontologies/ccso#TP40K2/IE_BSc/IED/STEF/TEIC"/>
        <includesCourse rdf:resource="http://xworks.gr/ontologies/ccso#TP40K3/IE_BSc/IED/STEF/TEIC"/>
        <includesCourse rdf:resource="http://xworks.gr/ontologies/ccso#TP40K4/IE_BSc/IED/STEF/TEIC"/>
        <includesCourse rdf:resource="http://xworks.gr/ontologies/ccso#TP40K5/IE_BSc/IED/STEF/TEIC"/>
        <includesCourse rdf:resource="http://xworks.gr/ontologies/ccso#TP40K6/IE_BSc/IED/STEF/TEIC"/>
        <includesCourse rdf:resource="http://xworks.gr/ontologies/ccso#TP50D2/IE_BSc/IED/STEF/TEIC"/>
        <includesCourse rdf:resource="http://xworks.gr/ontologies/ccso#TP50D4/IE_BSc/IED/STEF/TEIC"/>
        <includesCourse rdf:resource="http://xworks.gr/ontologies/ccso#TP50D5/IE_BSc/IED/STEF/TEIC"/>
        <includesCourse rdf:resource="http://xworks.gr/ontologies/ccso#TP50D6/IE_BSc/IED/STEF/TEIC"/>
        <includesCourse rdf:resource="http://xworks.gr/ontologies/ccso#TP50L1/IE_BSc/IED/STEF/TEIC"/>
        <includesCourse rdf:resource="http://xworks.gr/ontologies/ccso#TP50L2/IE_BSc/IED/STEF/TEIC"/>
        <includesCourse rdf:resource="http://xworks.gr/ontologies/ccso#TP50L3/IE_BSc/IED/STEF/TEIC"/>
        <includesCourse rdf:resource="http://xworks.gr/ontologies/ccso#TP50L4/IE_BSc/IED/STEF/TEIC"/>
        <includesCourse rdf:resource="http://xworks.gr/ontologies/ccso#TP50L5/IE_BSc/IED/STEF/TEIC"/>
        <includesCourse rdf:resource="http://xworks.gr/ontologies/ccso#TP50Y1/IE_BSc/IED/STEF/TEIC"/>
        <includesCourse rdf:resource="http://xworks.gr/ontologies/ccso#TP50Y2/IE_BSc/IED/STEF/TEIC"/>
        <includesCourse rdf:resource="http://xworks.gr/ontologies/ccso#TP50Y3/IE_BSc/IED/STEF/TEIC"/>
        <includesCourse rdf:resource="http://xworks.gr/ontologies/ccso#TP50Y4/IE_BSc/IED/STEF/TEIC"/>
        <includesCourse rdf:resource="http://xworks.gr/ontologies/ccso#TP50Y5/IE_BSc/IED/STEF/TEIC"/>
        <includesCourse rdf:resource="http://xworks.gr/ontologies/ccso#TP60D1/IE_BSc/IED/STEF/TEIC"/>
        <includesCourse rdf:resource="http://xworks.gr/ontologies/ccso#TP60D2/IE_BSc/IED/STEF/TEIC"/>
        <includesCourse rdf:resource="http://xworks.gr/ontologies/ccso#TP60D3/IE_BSc/IED/STEF/TEIC"/>
        <includesCourse rdf:resource="http://xworks.gr/ontologies/ccso#TP60D4/IE_BSc/IED/STEF/TEIC"/>
        <includesCourse rdf:resource="http://xworks.gr/ontologies/ccso#TP60D5/IE_BSc/IED/STEF/TEIC"/>
        <includesCourse rdf:resource="http://xworks.gr/ontologies/ccso#TP60L1/IE_BSc/IED/STEF/TEIC"/>
        <includesCourse rdf:resource="http://xworks.gr/ontologies/ccso#TP60L2/IE_BSc/IED/STEF/TEIC"/>
        <includesCourse rdf:resource="http://xworks.gr/ontologies/ccso#TP60L3/IE_BSc/IED/STEF/TEIC"/>
        <includesCourse rdf:resource="http://xworks.gr/ontologies/ccso#TP60L4/IE_BSc/IED/STEF/TEIC"/>
        <includesCourse rdf:resource="http://xworks.gr/ontologies/ccso#TP60L5/IE_BSc/IED/STEF/TEIC"/>
        <includesCourse rdf:resource="http://xworks.gr/ontologies/ccso#TP60Y1/IE_BSc/IED/STEF/TEIC"/>
        <includesCourse rdf:resource="http://xworks.gr/ontologies/ccso#TP60Y2/IE_BSc/IED/STEF/TEIC"/>
        <includesCourse rdf:resource="http://xworks.gr/ontologies/ccso#TP60Y6/IE_BSc/IED/STEF/TEIC"/>
        <includesCourse rdf:resource="http://xworks.gr/ontologies/ccso#TP70D1/IE_BSc/IED/STEF/TEIC"/>
        <includesCourse rdf:resource="http://xworks.gr/ontologies/ccso#TP70D2/IE_BSc/IED/STEF/TEIC"/>
        <includesCourse rdf:resource="http://xworks.gr/ontologies/ccso#TP70D3/IE_BSc/IED/STEF/TEIC"/>
        <includesCourse rdf:resource="http://xworks.gr/ontologies/ccso#TP70D5/IE_BSc/IED/STEF/TEIC"/>
        <includesCourse rdf:resource="http://xworks.gr/ontologies/ccso#TP70L1/IE_BSc/IED/STEF/TEIC"/>
        <includesCourse rdf:resource="http://xworks.gr/ontologies/ccso#TP70L2/IE_BSc/IED/STEF/TEIC"/>
        <includesCourse rdf:resource="http://xworks.gr/ontologies/ccso#TP70L3/IE_BSc/IED/STEF/TEIC"/>
        <includesCourse rdf:resource="http://xworks.gr/ontologies/ccso#TP70L4/IE_BSc/IED/STEF/TEIC"/>
        <includesCourse rdf:resource="http://xworks.gr/ontologies/ccso#TP70L5/IE_BSc/IED/STEF/TEIC"/>
        <includesCourse rdf:resource="http://xworks.gr/ontologies/ccso#TP70Y1/IE_BSc/IED/STEF/TEIC"/>
        <includesCourse rdf:resource="http://xworks.gr/ontologies/ccso#TP70Y2/IE_BSc/IED/STEF/TEIC"/>
        <includesCourse rdf:resource="http://xworks.gr/ontologies/ccso#TP70Y6/IE_BSc/IED/STEF/TEIC"/>
        <includesCourse rdf:resource="http://xworks.gr/ontologies/ccso#TP80/IE_BSc/IED/STEF/TEIC"/>
        <providedBy rdf:resource="http://xworks.gr/ontologies/ccso#Department_of_Informatics_Engineering_of_TEI_of_Crete"/>
        <code rdf:datatype="http://www.w3.org/2001/XMLSchema#string">IE_BSc/IED/STEF/TEIC</code>
        <creditsECTS rdf:datatype="http://www.w3.org/2001/XMLSchema#short">240</creditsECTS>
        <degreeTitle rdf:datatype="http://www.w3.org/2001/XMLSchema#string">Bachelor of Science in Informatics Engineering of TEI of Crete</degreeTitle>
        <degreeType rdf:datatype="http://www.w3.org/2001/XMLSchema#string">BSc</degreeType>
        <degreeType rdf:datatype="http://www.w3.org/2001/XMLSchema#string">Bachelor of Science</degreeType>
        <degreeURL rdf:datatype="http://www.w3.org/2001/XMLSchema#anyURI">https://www.teicrete.gr/ie/en/%CF%83%CE%B5%CE%BB%CE%AF%CE%B4%CE%B5%CF%82-%CF%84%CE%BC%CE%AE%CE%BC%CE%B1%CF%84%CE%BF%CF%82/undergraduate-programme</degreeURL>
        <duration rdf:datatype="http://www.w3.org/2001/XMLSchema#duration">P4Y</duration>
        <duration rdf:datatype="internal:anonymous-constants">P4Y</duration>
        <psName rdf:datatype="http://www.w3.org/2001/XMLSchema#string">Bachelor of Science (BSc) in Informatics Engineering of Department of Informatics Engineering of School of Engineering (STEF) of Technological Educational Institute (TEI) of Crete</psName>
        <webaddressURL rdf:datatype="http://www.w3.org/2001/XMLSchema#anyURI">https://www.teicrete.gr/ie/en/%CF%83%CE%B5%CE%BB%CE%AF%CE%B4%CE%B5%CF%82-%CF%84%CE%BC%CE%AE%CE%BC%CE%B1%CF%84%CE%BF%CF%82/undergraduate-programme</webaddressURL>
        <rdfs:label xml:lang="en">Bachelor of Science in Informatics Engineering of TEI of Crete</rdfs:label>
    </owl:NamedIndividual>
    


    <!-- http://xworks.gr/ontologies/ccso#BSc_Psychology/PSY_BSc/SoC/UoC -->

    <owl:NamedIndividual rdf:about="http://xworks.gr/ontologies/ccso#BSc_Psychology/PSY_BSc/SoC/UoC">
        <rdf:type rdf:resource="http://xworks.gr/ontologies/ccso#Bachelor"/>
        <rdf:type rdf:resource="http://xworks.gr/ontologies/ccso#ProgramofStudy"/>
        <affiliatedWith rdf:resource="http://xworks.gr/ontologies/ccso#Kekili_Souzan"/>
        <affiliatedWith rdf:resource="http://xworks.gr/ontologies/ccso#Ralli_Mary"/>
        <affiliatedWith rdf:resource="http://xworks.gr/ontologies/ccso#Rallis_John"/>
        <hasRegistered rdf:resource="http://xworks.gr/ontologies/ccso#Kekili_Souzan"/>
        <hasRegistered rdf:resource="http://xworks.gr/ontologies/ccso#Ralli_Mary"/>
        <hasRegistered rdf:resource="http://xworks.gr/ontologies/ccso#Rallis_John"/>
        <includesCourse rdf:resource="http://xworks.gr/ontologies/ccso#PSY1501/PSY_BSc/SoC/Uoc"/>
        <includesCourse rdf:resource="http://xworks.gr/ontologies/ccso#PSY2401/PSY_BSc/SoC/Uoc"/>
        <includesCourse rdf:resource="http://xworks.gr/ontologies/ccso#PSY3601/PSY_BSc/SoC/Uoc"/>
        <providedBy rdf:resource="http://xworks.gr/ontologies/ccso#Psychology_Department_of_University_of_Crete"/>
        <code rdf:datatype="http://www.w3.org/2001/XMLSchema#string">PSY_BSc/SoC/Uoc</code>
        <creditsECTS rdf:datatype="http://www.w3.org/2001/XMLSchema#short">240</creditsECTS>
        <degreeTitle rdf:datatype="http://www.w3.org/2001/XMLSchema#string">Bachelor of Science in Psychology of University of Crete</degreeTitle>
        <degreeType rdf:datatype="http://www.w3.org/2001/XMLSchema#string">BSc</degreeType>
        <degreeType rdf:datatype="http://www.w3.org/2001/XMLSchema#string">Bachelor of Science</degreeType>
        <duration rdf:datatype="http://www.w3.org/2001/XMLSchema#duration">P4Y</duration>
        <duration rdf:datatype="internal:anonymous-constants">P4Y</duration>
        <psName rdf:datatype="http://www.w3.org/2001/XMLSchema#string">Bachelor of Science (BSc) in Psychology of Psychology Department of School of Social Sciences of University of Crete</psName>
        <rdfs:label xml:lang="en">Bachelor of Science in Psychology of University of Crete</rdfs:label>
    </owl:NamedIndividual>
    


    <!-- http://xworks.gr/ontologies/ccso#CS/AL_Algorithms_and_Computation_Theory -->

    <owl:NamedIndividual rdf:about="http://xworks.gr/ontologies/ccso#CS/AL_Algorithms_and_Computation_Theory">
        <rdf:type rdf:resource="http://xworks.gr/ontologies/ccso#FieldofStudy"/>
        <rdf:type rdf:resource="http://xworks.gr/ontologies/ccso#KnowledgeArea"/>
        <partOfFS rdf:resource="http://xworks.gr/ontologies/ccso#Computer_Science"/>
        <partOfFS rdf:resource="http://xworks.gr/ontologies/ccso#Computer_Science_Curricula_2013"/>
        <fsName rdf:datatype="http://www.w3.org/2001/XMLSchema#string">Algorithms and Computation Theory</fsName>
    </owl:NamedIndividual>
    


    <!-- http://xworks.gr/ontologies/ccso#CS/CS_Computational_Science -->

    <owl:NamedIndividual rdf:about="http://xworks.gr/ontologies/ccso#CS/CS_Computational_Science">
        <rdf:type rdf:resource="http://xworks.gr/ontologies/ccso#FieldofStudy"/>
        <rdf:type rdf:resource="http://xworks.gr/ontologies/ccso#KnowledgeArea"/>
        <areaOfCourse rdf:resource="http://xworks.gr/ontologies/ccso#IM107/IM_MSc/IED/STEF/TEIC"/>
        <areaOfCourse rdf:resource="http://xworks.gr/ontologies/ccso#IM109/IM_MSc/IED/STEF/TEIC"/>
        <fsName rdf:datatype="http://www.w3.org/2001/XMLSchema#string">Computational Science</fsName>
    </owl:NamedIndividual>
    


    <!-- http://xworks.gr/ontologies/ccso#CS/CVR_Computer_Vision_and_Robotics -->

    <owl:NamedIndividual rdf:about="http://xworks.gr/ontologies/ccso#CS/CVR_Computer_Vision_and_Robotics">
        <rdf:type rdf:resource="http://xworks.gr/ontologies/ccso#FieldofStudy"/>
        <rdf:type rdf:resource="http://xworks.gr/ontologies/ccso#KnowledgeArea"/>
        <areaOfCourse rdf:resource="http://xworks.gr/ontologies/ccso#IM207/IM_MSc/IED/STEF/TEIC"/>
        <areaOfCourse rdf:resource="http://xworks.gr/ontologies/ccso#IM210/IM_MSc/IED/STEF/TEIC"/>
        <areaOfCourse rdf:resource="http://xworks.gr/ontologies/ccso#TP70Y2/IE_BSc/IED/STEF/TEIC"/>
        <fsName rdf:datatype="http://www.w3.org/2001/XMLSchema#string">Computer Vision and Robotics</fsName>
    </owl:NamedIndividual>
    


    <!-- http://xworks.gr/ontologies/ccso#CS/HW_Hardware_and_Computer_Systems -->

    <owl:NamedIndividual rdf:about="http://xworks.gr/ontologies/ccso#CS/HW_Hardware_and_Computer_Systems">
        <rdf:type rdf:resource="http://xworks.gr/ontologies/ccso#FieldofStudy"/>
        <rdf:type rdf:resource="http://xworks.gr/ontologies/ccso#KnowledgeArea"/>
        <areaOfCourse rdf:resource="http://xworks.gr/ontologies/ccso#CS220/CS_BSc/CSD/SSE/UoC"/>
        <areaOfCourse rdf:resource="http://xworks.gr/ontologies/ccso#CS422/CS_BSc/CSD/SSE/UoC"/>
        <areaOfCourse rdf:resource="http://xworks.gr/ontologies/ccso#CS425/CS_BSc/CSD/SSE/UoC"/>
        <areaOfCourse rdf:resource="http://xworks.gr/ontologies/ccso#CS428/CS_BSc/CSD/SSE/UoC"/>
        <areaOfCourse rdf:resource="http://xworks.gr/ontologies/ccso#CS446/CS_BSc/CSD/SSE/UoC"/>
        <areaOfCourse rdf:resource="http://xworks.gr/ontologies/ccso#TP50Y1/IE_BSc/IED/STEF/TEIC"/>
        <areaOfCourse rdf:resource="http://xworks.gr/ontologies/ccso#TP50Y2/IE_BSc/IED/STEF/TEIC"/>
        <areaOfCourse rdf:resource="http://xworks.gr/ontologies/ccso#TP50Y3/IE_BSc/IED/STEF/TEIC"/>
        <areaOfCourse rdf:resource="http://xworks.gr/ontologies/ccso#TP50Y4/IE_BSc/IED/STEF/TEIC"/>
        <areaOfCourse rdf:resource="http://xworks.gr/ontologies/ccso#TP50Y5/IE_BSc/IED/STEF/TEIC"/>
        <areaOfCourse rdf:resource="http://xworks.gr/ontologies/ccso#TP60D4/IE_BSc/IED/STEF/TEIC"/>
        <areaOfCourse rdf:resource="http://xworks.gr/ontologies/ccso#TP60D5/IE_BSc/IED/STEF/TEIC"/>
        <areaOfCourse rdf:resource="http://xworks.gr/ontologies/ccso#TP60Y1/IE_BSc/IED/STEF/TEIC"/>
        <areaOfCourse rdf:resource="http://xworks.gr/ontologies/ccso#TP60Y2/IE_BSc/IED/STEF/TEIC"/>
        <areaOfCourse rdf:resource="http://xworks.gr/ontologies/ccso#TP60Y6/IE_BSc/IED/STEF/TEIC"/>
        <areaOfCourse rdf:resource="http://xworks.gr/ontologies/ccso#TP70D5/IE_BSc/IED/STEF/TEIC"/>
        <areaOfCourse rdf:resource="http://xworks.gr/ontologies/ccso#TP70Y1/IE_BSc/IED/STEF/TEIC"/>
        <areaOfCourse rdf:resource="http://xworks.gr/ontologies/ccso#TP70Y2/IE_BSc/IED/STEF/TEIC"/>
        <areaOfCourse rdf:resource="http://xworks.gr/ontologies/ccso#TP70Y6/IE_BSc/IED/STEF/TEIC"/>
        <partOfFS rdf:resource="http://xworks.gr/ontologies/ccso#Computer_Science"/>
        <partOfFS rdf:resource="http://xworks.gr/ontologies/ccso#Computer_Science_Curricula_2013"/>
        <fsName rdf:datatype="http://www.w3.org/2001/XMLSchema#string">Hardware and Computer Systems</fsName>
    </owl:NamedIndividual>
    


    <!-- http://xworks.gr/ontologies/ccso#CS/IAS_Security_and_Information_Assurance -->

    <owl:NamedIndividual rdf:about="http://xworks.gr/ontologies/ccso#CS/IAS_Security_and_Information_Assurance">
        <rdf:type rdf:resource="http://xworks.gr/ontologies/ccso#FieldofStudy"/>
        <rdf:type rdf:resource="http://xworks.gr/ontologies/ccso#KnowledgeArea"/>
        <partOfFS rdf:resource="http://xworks.gr/ontologies/ccso#Computer_Science"/>
        <partOfFS rdf:resource="http://xworks.gr/ontologies/ccso#Computer_Science_Curricula_2013"/>
    </owl:NamedIndividual>
    


    <!-- http://xworks.gr/ontologies/ccso#CS/IM_Information_Management -->

    <owl:NamedIndividual rdf:about="http://xworks.gr/ontologies/ccso#CS/IM_Information_Management">
        <rdf:type rdf:resource="http://xworks.gr/ontologies/ccso#FieldofStudy"/>
        <rdf:type rdf:resource="http://xworks.gr/ontologies/ccso#KnowledgeArea"/>
        <areaOfCourse rdf:resource="http://xworks.gr/ontologies/ccso#IM209/IM_MSc/IED/STEF/TEIC"/>
        <partOfFS rdf:resource="http://xworks.gr/ontologies/ccso#Computer_Science"/>
        <partOfFS rdf:resource="http://xworks.gr/ontologies/ccso#Computer_Science_Curricula_2013"/>
        <fsName rdf:datatype="http://www.w3.org/2001/XMLSchema#string">Information Management</fsName>
    </owl:NamedIndividual>
    


    <!-- http://xworks.gr/ontologies/ccso#CS/IS_Advanced_Representation_and_Reasoning -->

    <owl:NamedIndividual rdf:about="http://xworks.gr/ontologies/ccso#CS/IS_Advanced_Representation_and_Reasoning">
        <rdf:type rdf:resource="http://xworks.gr/ontologies/ccso#Discipline"/>
        <rdf:type rdf:resource="http://xworks.gr/ontologies/ccso#FieldofStudy"/>
        <rdf:type rdf:resource="http://xworks.gr/ontologies/ccso#KnowledgeUnit"/>
        <lists rdf:resource="http://xworks.gr/ontologies/ccso#CS/IS/T_GraphPlan"/>
        <lists rdf:resource="http://xworks.gr/ontologies/ccso#CS/IS/T_Nonmonotonic_Reasoning"/>
        <lists rdf:resource="http://xworks.gr/ontologies/ccso#CS/IS/T_Ontologies"/>
        <lists rdf:resource="http://xworks.gr/ontologies/ccso#CS/IS/T_STRIPS_and_partial-order_planning"/>
        <lists rdf:resource="http://xworks.gr/ontologies/ccso#CS/IS/T_Situation_Calculus"/>
        <partOfFS rdf:resource="http://xworks.gr/ontologies/ccso#Computer_Science"/>
        <partOfFS rdf:resource="http://xworks.gr/ontologies/ccso#Computer_Science_Curricula_2013"/>
        <partOfFS rdf:resource="http://xworks.gr/ontologies/ccso#CS/IS_Intelligent_Systems"/>
        <abbreviation rdf:datatype="http://www.w3.org/2001/XMLSchema#string">CS/IS/ARR</abbreviation>
        <fsName rdf:datatype="http://www.w3.org/2001/XMLSchema#string">Advanced Representation and Reasoning</fsName>
    </owl:NamedIndividual>
    


    <!-- http://xworks.gr/ontologies/ccso#CS/IS_Intelligent_Systems -->

    <owl:NamedIndividual rdf:about="http://xworks.gr/ontologies/ccso#CS/IS_Intelligent_Systems">
        <rdf:type rdf:resource="http://xworks.gr/ontologies/ccso#Discipline"/>
        <rdf:type rdf:resource="http://xworks.gr/ontologies/ccso#FieldofStudy"/>
        <rdf:type rdf:resource="http://xworks.gr/ontologies/ccso#KnowledgeArea"/>
        <areaOfCourse rdf:resource="http://xworks.gr/ontologies/ccso#IM104/IM_MSc/IED/STEF/TEIC"/>
        <areaOfCourse rdf:resource="http://xworks.gr/ontologies/ccso#IM105/IM_MSc/IED/STEF/TEIC"/>
        <areaOfCourse rdf:resource="http://xworks.gr/ontologies/ccso#IM107/IM_MSc/IED/STEF/TEIC"/>
        <areaOfCourse rdf:resource="http://xworks.gr/ontologies/ccso#IM108/IM_MSc/IED/STEF/TEIC"/>
        <areaOfCourse rdf:resource="http://xworks.gr/ontologies/ccso#IM109/IM_MSc/IED/STEF/TEIC"/>
        <areaOfCourse rdf:resource="http://xworks.gr/ontologies/ccso#IM205/IM_MSc/IED/STEF/TEIC"/>
        <areaOfCourse rdf:resource="http://xworks.gr/ontologies/ccso#IM207/IM_MSc/IED/STEF/TEIC"/>
        <areaOfCourse rdf:resource="http://xworks.gr/ontologies/ccso#IM210/IM_MSc/IED/STEF/TEIC"/>
        <areaOfCourse rdf:resource="http://xworks.gr/ontologies/ccso#IM211/IM_MSc/IED/STEF/TEIC"/>
        <partOfFS rdf:resource="http://xworks.gr/ontologies/ccso#Computer_Science"/>
        <partOfFS rdf:resource="http://xworks.gr/ontologies/ccso#Computer_Science_Curricula_2013"/>
        <abbreviation rdf:datatype="http://www.w3.org/2001/XMLSchema#string">CS/IS</abbreviation>
        <fsName rdf:datatype="http://www.w3.org/2001/XMLSchema#string">Intelligent Systems</fsName>
    </owl:NamedIndividual>
    


    <!-- http://xworks.gr/ontologies/ccso#CS/NC_Networking_and_Communication -->

    <owl:NamedIndividual rdf:about="http://xworks.gr/ontologies/ccso#CS/NC_Networking_and_Communication">
        <rdf:type rdf:resource="http://xworks.gr/ontologies/ccso#Discipline"/>
        <rdf:type rdf:resource="http://xworks.gr/ontologies/ccso#FieldofStudy"/>
        <rdf:type rdf:resource="http://xworks.gr/ontologies/ccso#KnowledgeArea"/>
        <areaOfCourse rdf:resource="http://xworks.gr/ontologies/ccso#CS330/CS_BSc/CSD/SSE/UoC"/>
        <areaOfCourse rdf:resource="http://xworks.gr/ontologies/ccso#CS370/CS_BSc/CSD/SSE/UoC"/>
        <areaOfCourse rdf:resource="http://xworks.gr/ontologies/ccso#CS435/CS_BSc/CSD/SSE/UoC"/>
        <areaOfCourse rdf:resource="http://xworks.gr/ontologies/ccso#CS436/CS_BSc/CSD/SSE/UoC"/>
        <areaOfCourse rdf:resource="http://xworks.gr/ontologies/ccso#CS439/CS_BSc/CSD/SSE/UoC"/>
        <areaOfCourse rdf:resource="http://xworks.gr/ontologies/ccso#CS474/CS_BSc/CSD/SSE/UoC"/>
        <areaOfCourse rdf:resource="http://xworks.gr/ontologies/ccso#IM102/IM_MSc/IED/STEF/TEIC"/>
        <areaOfCourse rdf:resource="http://xworks.gr/ontologies/ccso#IM103/IM_MSc/IED/STEF/TEIC"/>
        <areaOfCourse rdf:resource="http://xworks.gr/ontologies/ccso#IM202/IM_MSc/IED/STEF/TEIC"/>
        <areaOfCourse rdf:resource="http://xworks.gr/ontologies/ccso#IM203/IM_MSc/IED/STEF/TEIC"/>
        <areaOfCourse rdf:resource="http://xworks.gr/ontologies/ccso#IM204/IM_MSc/IED/STEF/TEIC"/>
        <areaOfCourse rdf:resource="http://xworks.gr/ontologies/ccso#IM205/IM_MSc/IED/STEF/TEIC"/>
        <areaOfCourse rdf:resource="http://xworks.gr/ontologies/ccso#TP50D2/IE_BSc/IED/STEF/TEIC"/>
        <areaOfCourse rdf:resource="http://xworks.gr/ontologies/ccso#TP50D4/IE_BSc/IED/STEF/TEIC"/>
        <areaOfCourse rdf:resource="http://xworks.gr/ontologies/ccso#TP50D5/IE_BSc/IED/STEF/TEIC"/>
        <areaOfCourse rdf:resource="http://xworks.gr/ontologies/ccso#TP50D6/IE_BSc/IED/STEF/TEIC"/>
        <areaOfCourse rdf:resource="http://xworks.gr/ontologies/ccso#TP50L1/IE_BSc/IED/STEF/TEIC"/>
        <areaOfCourse rdf:resource="http://xworks.gr/ontologies/ccso#TP60D1/IE_BSc/IED/STEF/TEIC"/>
        <areaOfCourse rdf:resource="http://xworks.gr/ontologies/ccso#TP60D2/IE_BSc/IED/STEF/TEIC"/>
        <areaOfCourse rdf:resource="http://xworks.gr/ontologies/ccso#TP60D3/IE_BSc/IED/STEF/TEIC"/>
        <areaOfCourse rdf:resource="http://xworks.gr/ontologies/ccso#TP60D4/IE_BSc/IED/STEF/TEIC"/>
        <areaOfCourse rdf:resource="http://xworks.gr/ontologies/ccso#TP60D5/IE_BSc/IED/STEF/TEIC"/>
        <areaOfCourse rdf:resource="http://xworks.gr/ontologies/ccso#TP70D1/IE_BSc/IED/STEF/TEIC"/>
        <areaOfCourse rdf:resource="http://xworks.gr/ontologies/ccso#TP70D2/IE_BSc/IED/STEF/TEIC"/>
        <areaOfCourse rdf:resource="http://xworks.gr/ontologies/ccso#TP70D3/IE_BSc/IED/STEF/TEIC"/>
        <areaOfCourse rdf:resource="http://xworks.gr/ontologies/ccso#TP70D5/IE_BSc/IED/STEF/TEIC"/>
        <areaOfCourse rdf:resource="http://xworks.gr/ontologies/ccso#TP70Y6/IE_BSc/IED/STEF/TEIC"/>
        <partOfFS rdf:resource="http://xworks.gr/ontologies/ccso#Computer_Science"/>
        <partOfFS rdf:resource="http://xworks.gr/ontologies/ccso#Computer_Science_Curricula_2013"/>
        <abbreviation rdf:datatype="http://www.w3.org/2001/XMLSchema#string">CS/NC</abbreviation>
        <fsName rdf:datatype="http://www.w3.org/2001/XMLSchema#string">Networking and Communication</fsName>
    </owl:NamedIndividual>
    


    <!-- http://xworks.gr/ontologies/ccso#CS/OS_Operating_Systems -->

    <owl:NamedIndividual rdf:about="http://xworks.gr/ontologies/ccso#CS/OS_Operating_Systems">
        <rdf:type rdf:resource="http://xworks.gr/ontologies/ccso#Discipline"/>
        <rdf:type rdf:resource="http://xworks.gr/ontologies/ccso#FieldofStudy"/>
        <rdf:type rdf:resource="http://xworks.gr/ontologies/ccso#KnowledgeArea"/>
        <partOfFS rdf:resource="http://xworks.gr/ontologies/ccso#Computer_Science"/>
        <partOfFS rdf:resource="http://xworks.gr/ontologies/ccso#Computer_Science_Curricula_2013"/>
        <abbreviation rdf:datatype="http://www.w3.org/2001/XMLSchema#string">CS/OS</abbreviation>
        <fsName rdf:datatype="http://www.w3.org/2001/XMLSchema#string">Operating Systems</fsName>
    </owl:NamedIndividual>
    


    <!-- http://xworks.gr/ontologies/ccso#CS/PD_Parallel_and_Distributed_Computing -->

    <owl:NamedIndividual rdf:about="http://xworks.gr/ontologies/ccso#CS/PD_Parallel_and_Distributed_Computing">
        <rdf:type rdf:resource="http://xworks.gr/ontologies/ccso#FieldofStudy"/>
        <rdf:type rdf:resource="http://xworks.gr/ontologies/ccso#KnowledgeArea"/>
        <areaOfCourse rdf:resource="http://xworks.gr/ontologies/ccso#IM204/IM_MSc/IED/STEF/TEIC"/>
        <areaOfCourse rdf:resource="http://xworks.gr/ontologies/ccso#IM211/IM_MSc/IED/STEF/TEIC"/>
        <partOfFS rdf:resource="http://xworks.gr/ontologies/ccso#Computer_Science"/>
        <partOfFS rdf:resource="http://xworks.gr/ontologies/ccso#Computer_Science_Curricula_2013"/>
        <fsName rdf:datatype="http://www.w3.org/2001/XMLSchema#string">Parallel and Distributed Computing</fsName>
    </owl:NamedIndividual>
    


    <!-- http://xworks.gr/ontologies/ccso#CS/PL_Programming_Languages -->

    <owl:NamedIndividual rdf:about="http://xworks.gr/ontologies/ccso#CS/PL_Programming_Languages">
        <rdf:type rdf:resource="http://xworks.gr/ontologies/ccso#Discipline"/>
        <rdf:type rdf:resource="http://xworks.gr/ontologies/ccso#FieldofStudy"/>
        <rdf:type rdf:resource="http://xworks.gr/ontologies/ccso#KnowledgeArea"/>
        <areaOfCourse rdf:resource="http://xworks.gr/ontologies/ccso#CS150/CS_BSc/CSD/SSE/UoC"/>
        <areaOfCourse rdf:resource="http://xworks.gr/ontologies/ccso#CS240/CS_BSc/CSD/SSE/UoC"/>
        <areaOfCourse rdf:resource="http://xworks.gr/ontologies/ccso#CS252/CS_BSc/CSD/SSE/UoC"/>
        <areaOfCourse rdf:resource="http://xworks.gr/ontologies/ccso#CS317/CS_BSc/CSD/SSE/UoC"/>
        <areaOfCourse rdf:resource="http://xworks.gr/ontologies/ccso#CS340/CS_BSc/CSD/SSE/UoC"/>
        <areaOfCourse rdf:resource="http://xworks.gr/ontologies/ccso#CS342/CS_BSc/CSD/SSE/UoC"/>
        <areaOfCourse rdf:resource="http://xworks.gr/ontologies/ccso#CS380/CS_BSc/CSD/SSE/UoC"/>
        <areaOfCourse rdf:resource="http://xworks.gr/ontologies/ccso#CS387/CS_BSc/CSD/SSE/UoC"/>
        <areaOfCourse rdf:resource="http://xworks.gr/ontologies/ccso#CS486/CS_BSc/CSD/SSE/UoC"/>
        <areaOfCourse rdf:resource="http://xworks.gr/ontologies/ccso#TP10K4/IE_BSc/IED/STEF/TEIC"/>
        <areaOfCourse rdf:resource="http://xworks.gr/ontologies/ccso#TP30K4/IE_BSc/IED/STEF/TEIC"/>
        <areaOfCourse rdf:resource="http://xworks.gr/ontologies/ccso#TP40K3/IE_BSc/IED/STEF/TEIC"/>
        <partOfFS rdf:resource="http://xworks.gr/ontologies/ccso#Computer_Science"/>
        <partOfFS rdf:resource="http://xworks.gr/ontologies/ccso#Computer_Science_Curricula_2013"/>
        <abbreviation rdf:datatype="http://www.w3.org/2001/XMLSchema#string">PL</abbreviation>
        <fsName rdf:datatype="http://www.w3.org/2001/XMLSchema#string">Programming Languages</fsName>
    </owl:NamedIndividual>
    


    <!-- http://xworks.gr/ontologies/ccso#CS/SIP_Social_Issues_and_Professional_Practice -->

    <owl:NamedIndividual rdf:about="http://xworks.gr/ontologies/ccso#CS/SIP_Social_Issues_and_Professional_Practice">
        <rdf:type rdf:resource="http://xworks.gr/ontologies/ccso#FieldofStudy"/>
        <rdf:type rdf:resource="http://xworks.gr/ontologies/ccso#KnowledgeArea"/>
        <areaOfCourse rdf:resource="http://xworks.gr/ontologies/ccso#IM101/IM_MSc/IED/STEF/TEIC"/>
        <areaOfCourse rdf:resource="http://xworks.gr/ontologies/ccso#TP10K6/IE_BSc/IED/STEF/TEIC"/>
        <partOfFS rdf:resource="http://xworks.gr/ontologies/ccso#Computer_Science"/>
        <partOfFS rdf:resource="http://xworks.gr/ontologies/ccso#Computer_Science_Curricula_2013"/>
        <fsName rdf:datatype="http://www.w3.org/2001/XMLSchema#string">Social Issues and Professional Practice</fsName>
    </owl:NamedIndividual>
    


    <!-- http://xworks.gr/ontologies/ccso#CS/SI_Society_and_Informatics -->

    <owl:NamedIndividual rdf:about="http://xworks.gr/ontologies/ccso#CS/SI_Society_and_Informatics">
        <rdf:type rdf:resource="http://xworks.gr/ontologies/ccso#FieldofStudy"/>
        <rdf:type rdf:resource="http://xworks.gr/ontologies/ccso#KnowledgeArea"/>
        <partOfFS rdf:resource="http://xworks.gr/ontologies/ccso#Computer_Science"/>
        <partOfFS rdf:resource="http://xworks.gr/ontologies/ccso#Computer_Science_Curricula_2013"/>
    </owl:NamedIndividual>
    


    <!-- http://xworks.gr/ontologies/ccso#CS/SW_Software_Engineering_Software_Systems_and_Applications -->

    <owl:NamedIndividual rdf:about="http://xworks.gr/ontologies/ccso#CS/SW_Software_Engineering_Software_Systems_and_Applications">
        <rdf:type rdf:resource="http://xworks.gr/ontologies/ccso#FieldofStudy"/>
        <rdf:type rdf:resource="http://xworks.gr/ontologies/ccso#KnowledgeArea"/>
        <areaOfCourse rdf:resource="http://xworks.gr/ontologies/ccso#CS342/CS_BSc/CSD/SSE/UoC"/>
        <areaOfCourse rdf:resource="http://xworks.gr/ontologies/ccso#CS351/CS_BSc/CSD/SSE/UoC"/>
        <areaOfCourse rdf:resource="http://xworks.gr/ontologies/ccso#CS352/CS_BSc/CSD/SSE/UoC"/>
        <areaOfCourse rdf:resource="http://xworks.gr/ontologies/ccso#CS358/CS_BSc/CSD/SSE/UoC"/>
        <areaOfCourse rdf:resource="http://xworks.gr/ontologies/ccso#CS452/CS_BSc/CSD/SSE/UoC"/>
        <areaOfCourse rdf:resource="http://xworks.gr/ontologies/ccso#CS455/CS_BSc/CSD/SSE/UoC"/>
        <areaOfCourse rdf:resource="http://xworks.gr/ontologies/ccso#CS457/CS_BSc/CSD/SSE/UoC"/>
        <areaOfCourse rdf:resource="http://xworks.gr/ontologies/ccso#CS459/CS_BSc/CSD/SSE/UoC"/>
        <areaOfCourse rdf:resource="http://xworks.gr/ontologies/ccso#IM104/IM_MSc/IED/STEF/TEIC"/>
        <areaOfCourse rdf:resource="http://xworks.gr/ontologies/ccso#IM105/IM_MSc/IED/STEF/TEIC"/>
        <areaOfCourse rdf:resource="http://xworks.gr/ontologies/ccso#IM106/IM_MSc/IED/STEF/TEIC"/>
        <areaOfCourse rdf:resource="http://xworks.gr/ontologies/ccso#IM108/IM_MSc/IED/STEF/TEIC"/>
        <areaOfCourse rdf:resource="http://xworks.gr/ontologies/ccso#IM206/IM_MSc/IED/STEF/TEIC"/>
        <areaOfCourse rdf:resource="http://xworks.gr/ontologies/ccso#IM208/IM_MSc/IED/STEF/TEIC"/>
        <areaOfCourse rdf:resource="http://xworks.gr/ontologies/ccso#IM209/IM_MSc/IED/STEF/TEIC"/>
        <areaOfCourse rdf:resource="http://xworks.gr/ontologies/ccso#IM210/IM_MSc/IED/STEF/TEIC"/>
        <areaOfCourse rdf:resource="http://xworks.gr/ontologies/ccso#TP50L1/IE_BSc/IED/STEF/TEIC"/>
        <areaOfCourse rdf:resource="http://xworks.gr/ontologies/ccso#TP50L2/IE_BSc/IED/STEF/TEIC"/>
        <areaOfCourse rdf:resource="http://xworks.gr/ontologies/ccso#TP50L3/IE_BSc/IED/STEF/TEIC"/>
        <areaOfCourse rdf:resource="http://xworks.gr/ontologies/ccso#TP50L4/IE_BSc/IED/STEF/TEIC"/>
        <areaOfCourse rdf:resource="http://xworks.gr/ontologies/ccso#TP50L5/IE_BSc/IED/STEF/TEIC"/>
        <areaOfCourse rdf:resource="http://xworks.gr/ontologies/ccso#TP60L1/IE_BSc/IED/STEF/TEIC"/>
        <areaOfCourse rdf:resource="http://xworks.gr/ontologies/ccso#TP60L2/IE_BSc/IED/STEF/TEIC"/>
        <areaOfCourse rdf:resource="http://xworks.gr/ontologies/ccso#TP60L3/IE_BSc/IED/STEF/TEIC"/>
        <areaOfCourse rdf:resource="http://xworks.gr/ontologies/ccso#TP60L4/IE_BSc/IED/STEF/TEIC"/>
        <areaOfCourse rdf:resource="http://xworks.gr/ontologies/ccso#TP60L5/IE_BSc/IED/STEF/TEIC"/>
        <areaOfCourse rdf:resource="http://xworks.gr/ontologies/ccso#TP70L1/IE_BSc/IED/STEF/TEIC"/>
        <areaOfCourse rdf:resource="http://xworks.gr/ontologies/ccso#TP70L2/IE_BSc/IED/STEF/TEIC"/>
        <areaOfCourse rdf:resource="http://xworks.gr/ontologies/ccso#TP70L3/IE_BSc/IED/STEF/TEIC"/>
        <areaOfCourse rdf:resource="http://xworks.gr/ontologies/ccso#TP70L4/IE_BSc/IED/STEF/TEIC"/>
        <areaOfCourse rdf:resource="http://xworks.gr/ontologies/ccso#TP70L5/IE_BSc/IED/STEF/TEIC"/>
        <partOfFS rdf:resource="http://xworks.gr/ontologies/ccso#Computer_Science"/>
        <partOfFS rdf:resource="http://xworks.gr/ontologies/ccso#Computer_Science_Curricula_2013"/>
        <fsName rdf:datatype="http://www.w3.org/2001/XMLSchema#string">Software Engineering, Software Systems and Applications</fsName>
    </owl:NamedIndividual>
    


    <!-- http://xworks.gr/ontologies/ccso#CS/IS/T_GraphPlan -->

    <owl:NamedIndividual rdf:about="http://xworks.gr/ontologies/ccso#CS/IS/T_GraphPlan">
        <rdf:type rdf:resource="http://xworks.gr/ontologies/ccso#Topic"/>
        <coveredInCourse rdf:resource="http://xworks.gr/ontologies/ccso#IM105s1/IM_MSc/IED/STEF/TEI"/>
        <listedInKU rdf:resource="http://xworks.gr/ontologies/ccso#CS/IS_Advanced_Representation_and_Reasoning"/>
        <label rdf:datatype="http://www.w3.org/2001/XMLSchema#string">CS/IS GraphPlan</label>
    </owl:NamedIndividual>
    


    <!-- http://xworks.gr/ontologies/ccso#CS/IS/T_Nonmonotonic_Reasoning -->

    <owl:NamedIndividual rdf:about="http://xworks.gr/ontologies/ccso#CS/IS/T_Nonmonotonic_Reasoning">
        <rdf:type rdf:resource="http://xworks.gr/ontologies/ccso#Topic"/>
        <coveredInCourse rdf:resource="http://xworks.gr/ontologies/ccso#IM105s1/IM_MSc/IED/STEF/TEI"/>
        <listedInKU rdf:resource="http://xworks.gr/ontologies/ccso#CS/IS_Advanced_Representation_and_Reasoning"/>
        <label rdf:datatype="http://www.w3.org/2001/XMLSchema#string">CS/IS Nonmonotonic Reasoning</label>
    </owl:NamedIndividual>
    


    <!-- http://xworks.gr/ontologies/ccso#CS/IS/T_Ontologies -->

    <owl:NamedIndividual rdf:about="http://xworks.gr/ontologies/ccso#CS/IS/T_Ontologies">
        <rdf:type rdf:resource="http://xworks.gr/ontologies/ccso#Topic"/>
        <coveredInCourse rdf:resource="http://xworks.gr/ontologies/ccso#IM105s1/IM_MSc/IED/STEF/TEI"/>
        <listedInKU rdf:resource="http://xworks.gr/ontologies/ccso#CS/IS_Advanced_Representation_and_Reasoning"/>
        <label rdf:datatype="http://www.w3.org/2001/XMLSchema#string">CS/IS Ontologies</label>
    </owl:NamedIndividual>
    


    <!-- http://xworks.gr/ontologies/ccso#CS/IS/T_Query_Languages -->

    <owl:NamedIndividual rdf:about="http://xworks.gr/ontologies/ccso#CS/IS/T_Query_Languages">
        <rdf:type rdf:resource="http://xworks.gr/ontologies/ccso#Topic"/>
        <coveredInCourse rdf:resource="http://xworks.gr/ontologies/ccso#IM105s1/IM_MSc/IED/STEF/TEI"/>
        <label rdf:datatype="http://www.w3.org/2001/XMLSchema#string">CS/IS Query Languages</label>
    </owl:NamedIndividual>
    


    <!-- http://xworks.gr/ontologies/ccso#CS/IS/T_STRIPS_and_partial-order_planning -->

    <owl:NamedIndividual rdf:about="http://xworks.gr/ontologies/ccso#CS/IS/T_STRIPS_and_partial-order_planning">
        <rdf:type rdf:resource="http://xworks.gr/ontologies/ccso#Topic"/>
        <listedInKU rdf:resource="http://xworks.gr/ontologies/ccso#CS/IS_Advanced_Representation_and_Reasoning"/>
        <label rdf:datatype="http://www.w3.org/2001/XMLSchema#string">CS/IS STRIPS and partial-order planning</label>
    </owl:NamedIndividual>
    


    <!-- http://xworks.gr/ontologies/ccso#CS/IS/T_Situation_Calculus -->

    <owl:NamedIndividual rdf:about="http://xworks.gr/ontologies/ccso#CS/IS/T_Situation_Calculus">
        <rdf:type rdf:resource="http://xworks.gr/ontologies/ccso#Topic"/>
        <listedInKU rdf:resource="http://xworks.gr/ontologies/ccso#CS/IS_Advanced_Representation_and_Reasoning"/>
        <label rdf:datatype="http://www.w3.org/2001/XMLSchema#string">CS/IS Situation Calculus</label>
    </owl:NamedIndividual>
    


    <!-- http://xworks.gr/ontologies/ccso#CS/NC/LAN_Local_Area_Networks -->

    <owl:NamedIndividual rdf:about="http://xworks.gr/ontologies/ccso#CS/NC/LAN_Local_Area_Networks">
        <rdf:type rdf:resource="http://xworks.gr/ontologies/ccso#Discipline"/>
        <rdf:type rdf:resource="http://xworks.gr/ontologies/ccso#FieldofStudy"/>
        <rdf:type rdf:resource="http://xworks.gr/ontologies/ccso#KnowledgeUnit"/>
        <lists rdf:resource="http://xworks.gr/ontologies/ccso#CS/NC/LAN/LO_Describe_how_frames_are_forwarded_in_an_Ethernet_network"/>
        <lists rdf:resource="http://xworks.gr/ontologies/ccso#CS/NC/LAN/LO_Describe_the_interrelations_between_IP_and_Ethernet"/>
        <lists rdf:resource="http://xworks.gr/ontologies/ccso#CS/NC/LAN/LO_Describe_the_steps_used_in_one_common_approach_to_the_multiple_access_problem"/>
        <lists rdf:resource="http://xworks.gr/ontologies/ccso#CS/NC/LAN/LO_Identify_the_differences_between_IP_and_Ethernet"/>
        <lists rdf:resource="http://xworks.gr/ontologies/ccso#CS/NC/LAN/T_Common_approaches_to_multiple_access"/>
        <lists rdf:resource="http://xworks.gr/ontologies/ccso#CS/NC/LAN/T_Ethernet"/>
        <lists rdf:resource="http://xworks.gr/ontologies/ccso#CS/NC/LAN/T_Local_Area_Networks"/>
        <lists rdf:resource="http://xworks.gr/ontologies/ccso#CS/NC/LAN/T_Multiple_Access_Problem"/>
        <lists rdf:resource="http://xworks.gr/ontologies/ccso#CS/NC/LAN/T_Switching"/>
        <partOfFS rdf:resource="http://xworks.gr/ontologies/ccso#Computer_Science"/>
        <partOfFS rdf:resource="http://xworks.gr/ontologies/ccso#Computer_Science_Curricula_2013"/>
        <partOfFS rdf:resource="http://xworks.gr/ontologies/ccso#CS/NC_Networking_and_Communication"/>
        <abbreviation rdf:datatype="http://www.w3.org/2001/XMLSchema#string">CS/NC/LAN</abbreviation>
        <fsName rdf:datatype="http://www.w3.org/2001/XMLSchema#string">Local Area Networks</fsName>
    </owl:NamedIndividual>
    


    <!-- http://xworks.gr/ontologies/ccso#CS/NC/RF_Routing_and_Forwarding -->

    <owl:NamedIndividual rdf:about="http://xworks.gr/ontologies/ccso#CS/NC/RF_Routing_and_Forwarding">
        <rdf:type rdf:resource="http://xworks.gr/ontologies/ccso#Discipline"/>
        <rdf:type rdf:resource="http://xworks.gr/ontologies/ccso#FieldofStudy"/>
        <rdf:type rdf:resource="http://xworks.gr/ontologies/ccso#KnowledgeUnit"/>
        <lists rdf:resource="http://xworks.gr/ontologies/ccso#CS/NC/RF/LO_Describe_how_packets_are_forwarded_in_an_IP_networks"/>
        <lists rdf:resource="http://xworks.gr/ontologies/ccso#CS/NC/RF/LO_Describe_the_organization_of_the_network_layer"/>
        <lists rdf:resource="http://xworks.gr/ontologies/ccso#CS/NC/RF/LO_List_the_scalability_benefits_of_hierarchical_addressing"/>
        <lists rdf:resource="http://xworks.gr/ontologies/ccso#CS/NC/RF/T_Internet_Protocol"/>
        <lists rdf:resource="http://xworks.gr/ontologies/ccso#CS/NC/RF/T_Routing_versus_forwarding"/>
        <lists rdf:resource="http://xworks.gr/ontologies/ccso#CS/NC/RF/T_Scalability_issues"/>
        <lists rdf:resource="http://xworks.gr/ontologies/ccso#CS/NC/RF/T_Static_routing"/>
        <partOfFS rdf:resource="http://xworks.gr/ontologies/ccso#Computer_Science"/>
        <partOfFS rdf:resource="http://xworks.gr/ontologies/ccso#Computer_Science_Curricula_2013"/>
        <partOfFS rdf:resource="http://xworks.gr/ontologies/ccso#CS/NC_Networking_and_Communication"/>
        <abbreviation rdf:datatype="http://www.w3.org/2001/XMLSchema#string">CS/NC/RF</abbreviation>
        <fsName rdf:datatype="http://www.w3.org/2001/XMLSchema#string">Routing and Forwarding</fsName>
    </owl:NamedIndividual>
    


    <!-- http://xworks.gr/ontologies/ccso#CS/NC/LAN/LO_Describe_how_frames_are_forwarded_in_an_Ethernet_network -->

    <owl:NamedIndividual rdf:about="http://xworks.gr/ontologies/ccso#CS/NC/LAN/LO_Describe_how_frames_are_forwarded_in_an_Ethernet_network">
        <rdf:type rdf:resource="http://xworks.gr/ontologies/ccso#LearningOutcome"/>
        <acquiredInCourse rdf:resource="http://xworks.gr/ontologies/ccso#CS335_s2017-18/CS_BSc/CSD/SSE/UoC"/>
        <acquiredInCourse rdf:resource="http://xworks.gr/ontologies/ccso#CS435s1/CS_BSc/CSD/SSE/UoC"/>
        <acquiredInCourse rdf:resource="http://xworks.gr/ontologies/ccso#IM102s1/IM_MSc/IED/STEF/TEI"/>
        <acquiredInCourse rdf:resource="http://xworks.gr/ontologies/ccso#TP40K2s1/IE_BSc/IED/STEF/TEIC"/>
        <acquiredInCourse rdf:resource="http://xworks.gr/ontologies/ccso#TP50D2s1/IE_BSc/IED/STEF/TEIC"/>
        <listedInKU rdf:resource="http://xworks.gr/ontologies/ccso#CS/NC/LAN_Local_Area_Networks"/>
        <label rdf:datatype="http://www.w3.org/2001/XMLSchema#string">Describe how frames are forwarded in an Ethernet network</label>
        <levelofMastery rdf:datatype="http://www.w3.org/2001/XMLSchema#string">Familiarity</levelofMastery>
    </owl:NamedIndividual>
    


    <!-- http://xworks.gr/ontologies/ccso#CS/NC/LAN/LO_Describe_the_interrelations_between_IP_and_Ethernet -->

    <owl:NamedIndividual rdf:about="http://xworks.gr/ontologies/ccso#CS/NC/LAN/LO_Describe_the_interrelations_between_IP_and_Ethernet">
        <rdf:type rdf:resource="http://xworks.gr/ontologies/ccso#LearningOutcome"/>
        <acquiredInCourse rdf:resource="http://xworks.gr/ontologies/ccso#CS335_s2017-18/CS_BSc/CSD/SSE/UoC"/>
        <acquiredInCourse rdf:resource="http://xworks.gr/ontologies/ccso#CS435s1/CS_BSc/CSD/SSE/UoC"/>
        <acquiredInCourse rdf:resource="http://xworks.gr/ontologies/ccso#IM102s1/IM_MSc/IED/STEF/TEI"/>
        <acquiredInCourse rdf:resource="http://xworks.gr/ontologies/ccso#TP50D2s1/IE_BSc/IED/STEF/TEIC"/>
        <listedInKU rdf:resource="http://xworks.gr/ontologies/ccso#CS/NC/LAN_Local_Area_Networks"/>
        <label rdf:datatype="http://www.w3.org/2001/XMLSchema#string">Describe the interrelations between IP and Ethernet</label>
        <levelofMastery rdf:datatype="http://www.w3.org/2001/XMLSchema#string">Familiarity</levelofMastery>
    </owl:NamedIndividual>
    


    <!-- http://xworks.gr/ontologies/ccso#CS/NC/LAN/LO_Describe_the_steps_used_in_one_common_approach_to_the_multiple_access_problem -->

    <owl:NamedIndividual rdf:about="http://xworks.gr/ontologies/ccso#CS/NC/LAN/LO_Describe_the_steps_used_in_one_common_approach_to_the_multiple_access_problem">
        <rdf:type rdf:resource="http://xworks.gr/ontologies/ccso#LearningOutcome"/>
        <acquiredInCourse rdf:resource="http://xworks.gr/ontologies/ccso#CS335_s2017-18/CS_BSc/CSD/SSE/UoC"/>
        <acquiredInCourse rdf:resource="http://xworks.gr/ontologies/ccso#CS435s1/CS_BSc/CSD/SSE/UoC"/>
        <acquiredInCourse rdf:resource="http://xworks.gr/ontologies/ccso#IM102s1/IM_MSc/IED/STEF/TEI"/>
        <acquiredInCourse rdf:resource="http://xworks.gr/ontologies/ccso#TP40K2s1/IE_BSc/IED/STEF/TEIC"/>
        <listedInKU rdf:resource="http://xworks.gr/ontologies/ccso#CS/NC/LAN_Local_Area_Networks"/>
        <label rdf:datatype="http://www.w3.org/2001/XMLSchema#string">Describe the steps used in one common approach to the multiple access problem</label>
        <levelofMastery rdf:datatype="http://www.w3.org/2001/XMLSchema#string">Familiarity</levelofMastery>
    </owl:NamedIndividual>
    


    <!-- http://xworks.gr/ontologies/ccso#CS/NC/LAN/LO_Identify_the_differences_between_IP_and_Ethernet -->

    <owl:NamedIndividual rdf:about="http://xworks.gr/ontologies/ccso#CS/NC/LAN/LO_Identify_the_differences_between_IP_and_Ethernet">
        <rdf:type rdf:resource="http://xworks.gr/ontologies/ccso#LearningOutcome"/>
        <acquiredInCourse rdf:resource="http://xworks.gr/ontologies/ccso#CS335_s2017-18/CS_BSc/CSD/SSE/UoC"/>
        <acquiredInCourse rdf:resource="http://xworks.gr/ontologies/ccso#CS435s1/CS_BSc/CSD/SSE/UoC"/>
        <acquiredInCourse rdf:resource="http://xworks.gr/ontologies/ccso#IM102s1/IM_MSc/IED/STEF/TEI"/>
        <acquiredInCourse rdf:resource="http://xworks.gr/ontologies/ccso#TP40K2s1/IE_BSc/IED/STEF/TEIC"/>
        <acquiredInCourse rdf:resource="http://xworks.gr/ontologies/ccso#TP50D2s1/IE_BSc/IED/STEF/TEIC"/>
        <listedInKU rdf:resource="http://xworks.gr/ontologies/ccso#CS/NC/LAN_Local_Area_Networks"/>
        <label rdf:datatype="http://www.w3.org/2001/XMLSchema#string">Identify the differences between IP and Ethernet</label>
        <levelofMastery rdf:datatype="http://www.w3.org/2001/XMLSchema#string">Familiarity</levelofMastery>
    </owl:NamedIndividual>
    


    <!-- http://xworks.gr/ontologies/ccso#CS/NC/LAN/T_Common_approaches_to_multiple_access -->

    <owl:NamedIndividual rdf:about="http://xworks.gr/ontologies/ccso#CS/NC/LAN/T_Common_approaches_to_multiple_access">
        <rdf:type rdf:resource="http://xworks.gr/ontologies/ccso#Topic"/>
        <coveredInCourse rdf:resource="http://xworks.gr/ontologies/ccso#CS335_s2017-18/CS_BSc/CSD/SSE/UoC"/>
        <coveredInCourse rdf:resource="http://xworks.gr/ontologies/ccso#CS435s1/CS_BSc/CSD/SSE/UoC"/>
        <coveredInCourse rdf:resource="http://xworks.gr/ontologies/ccso#IM102s1/IM_MSc/IED/STEF/TEI"/>
        <coveredInCourse rdf:resource="http://xworks.gr/ontologies/ccso#TP50D2s1/IE_BSc/IED/STEF/TEIC"/>
        <listedInKU rdf:resource="http://xworks.gr/ontologies/ccso#CS/NC/LAN_Local_Area_Networks"/>
        <label rdf:datatype="http://www.w3.org/2001/XMLSchema#string">Common approaches to multiple access (exponential-backoff, time division multiplexing, etc)</label>
        <topicType rdf:datatype="http://www.w3.org/2001/XMLSchema#string">Core-Tier-2</topicType>
    </owl:NamedIndividual>
    


    <!-- http://xworks.gr/ontologies/ccso#CS/NC/LAN/T_Ethernet -->

    <owl:NamedIndividual rdf:about="http://xworks.gr/ontologies/ccso#CS/NC/LAN/T_Ethernet">
        <rdf:type rdf:resource="http://xworks.gr/ontologies/ccso#Topic"/>
        <coveredInCourse rdf:resource="http://xworks.gr/ontologies/ccso#CS335_s2017-18/CS_BSc/CSD/SSE/UoC"/>
        <coveredInCourse rdf:resource="http://xworks.gr/ontologies/ccso#CS435s1/CS_BSc/CSD/SSE/UoC"/>
        <coveredInCourse rdf:resource="http://xworks.gr/ontologies/ccso#TP40K2s1/IE_BSc/IED/STEF/TEIC"/>
        <listedInKU rdf:resource="http://xworks.gr/ontologies/ccso#CS/NC/LAN_Local_Area_Networks"/>
        <label rdf:datatype="http://www.w3.org/2001/XMLSchema#string">Ethernet</label>
        <topicType rdf:datatype="http://www.w3.org/2001/XMLSchema#string">Core-Tier-2</topicType>
    </owl:NamedIndividual>
    


    <!-- http://xworks.gr/ontologies/ccso#CS/NC/LAN/T_Local_Area_Networks -->

    <owl:NamedIndividual rdf:about="http://xworks.gr/ontologies/ccso#CS/NC/LAN/T_Local_Area_Networks">
        <rdf:type rdf:resource="http://xworks.gr/ontologies/ccso#Topic"/>
        <coveredInCourse rdf:resource="http://xworks.gr/ontologies/ccso#CS335_s2017-18/CS_BSc/CSD/SSE/UoC"/>
        <coveredInCourse rdf:resource="http://xworks.gr/ontologies/ccso#CS435s1/CS_BSc/CSD/SSE/UoC"/>
        <listedInKU rdf:resource="http://xworks.gr/ontologies/ccso#CS/NC/LAN_Local_Area_Networks"/>
        <label rdf:datatype="http://www.w3.org/2001/XMLSchema#string">Local Area Networks</label>
        <topicType rdf:datatype="http://www.w3.org/2001/XMLSchema#string">Core-Tier-2</topicType>
    </owl:NamedIndividual>
    


    <!-- http://xworks.gr/ontologies/ccso#CS/NC/LAN/T_Multiple_Access_Problem -->

    <owl:NamedIndividual rdf:about="http://xworks.gr/ontologies/ccso#CS/NC/LAN/T_Multiple_Access_Problem">
        <rdf:type rdf:resource="http://xworks.gr/ontologies/ccso#Topic"/>
        <coveredInCourse rdf:resource="http://xworks.gr/ontologies/ccso#CS335_s2017-18/CS_BSc/CSD/SSE/UoC"/>
        <coveredInCourse rdf:resource="http://xworks.gr/ontologies/ccso#CS435s1/CS_BSc/CSD/SSE/UoC"/>
        <coveredInCourse rdf:resource="http://xworks.gr/ontologies/ccso#IM102s1/IM_MSc/IED/STEF/TEI"/>
        <coveredInCourse rdf:resource="http://xworks.gr/ontologies/ccso#TP40K2s1/IE_BSc/IED/STEF/TEIC"/>
        <coveredInCourse rdf:resource="http://xworks.gr/ontologies/ccso#TP50D2s1/IE_BSc/IED/STEF/TEIC"/>
        <listedInKU rdf:resource="http://xworks.gr/ontologies/ccso#CS/NC/LAN_Local_Area_Networks"/>
        <label rdf:datatype="http://www.w3.org/2001/XMLSchema#string">Multiple Access Problem</label>
        <topicType rdf:datatype="http://www.w3.org/2001/XMLSchema#string">Core-Tier-2</topicType>
    </owl:NamedIndividual>
    


    <!-- http://xworks.gr/ontologies/ccso#CS/NC/LAN/T_Switching -->

    <owl:NamedIndividual rdf:about="http://xworks.gr/ontologies/ccso#CS/NC/LAN/T_Switching">
        <rdf:type rdf:resource="http://xworks.gr/ontologies/ccso#Topic"/>
        <coveredInCourse rdf:resource="http://xworks.gr/ontologies/ccso#CS335_s2017-18/CS_BSc/CSD/SSE/UoC"/>
        <coveredInCourse rdf:resource="http://xworks.gr/ontologies/ccso#CS435s1/CS_BSc/CSD/SSE/UoC"/>
        <coveredInCourse rdf:resource="http://xworks.gr/ontologies/ccso#IM102s1/IM_MSc/IED/STEF/TEI"/>
        <coveredInCourse rdf:resource="http://xworks.gr/ontologies/ccso#TP40K2s1/IE_BSc/IED/STEF/TEIC"/>
        <listedInKU rdf:resource="http://xworks.gr/ontologies/ccso#CS/NC/LAN_Local_Area_Networks"/>
        <label rdf:datatype="http://www.w3.org/2001/XMLSchema#string">Switching</label>
        <topicType rdf:datatype="http://www.w3.org/2001/XMLSchema#string">Core-Tier-2</topicType>
    </owl:NamedIndividual>
    


    <!-- http://xworks.gr/ontologies/ccso#CS/NC/RF/LO_Describe_how_packets_are_forwarded_in_an_IP_networks -->

    <owl:NamedIndividual rdf:about="http://xworks.gr/ontologies/ccso#CS/NC/RF/LO_Describe_how_packets_are_forwarded_in_an_IP_networks">
        <rdf:type rdf:resource="http://xworks.gr/ontologies/ccso#LearningOutcome"/>
        <acquiredInCourse rdf:resource="http://xworks.gr/ontologies/ccso#CS335_s2017-18/CS_BSc/CSD/SSE/UoC"/>
        <listedInKU rdf:resource="http://xworks.gr/ontologies/ccso#CS/NC/RF_Routing_and_Forwarding"/>
        <label rdf:datatype="http://www.w3.org/2001/XMLSchema#string">Describe how packets are forwarded in an IP networks</label>
        <levelofMastery rdf:datatype="http://www.w3.org/2001/XMLSchema#string">Familiarity</levelofMastery>
    </owl:NamedIndividual>
    


    <!-- http://xworks.gr/ontologies/ccso#CS/NC/RF/LO_Describe_the_organization_of_the_network_layer -->

    <owl:NamedIndividual rdf:about="http://xworks.gr/ontologies/ccso#CS/NC/RF/LO_Describe_the_organization_of_the_network_layer">
        <rdf:type rdf:resource="http://xworks.gr/ontologies/ccso#LearningOutcome"/>
        <acquiredInCourse rdf:resource="http://xworks.gr/ontologies/ccso#CS335_s2017-18/CS_BSc/CSD/SSE/UoC"/>
        <listedInKU rdf:resource="http://xworks.gr/ontologies/ccso#CS/NC/RF_Routing_and_Forwarding"/>
        <label rdf:datatype="http://www.w3.org/2001/XMLSchema#string">Describe the organization of the network layer</label>
        <levelofMastery rdf:datatype="http://www.w3.org/2001/XMLSchema#string">Familiarity</levelofMastery>
    </owl:NamedIndividual>
    


    <!-- http://xworks.gr/ontologies/ccso#CS/NC/RF/LO_List_the_scalability_benefits_of_hierarchical_addressing -->

    <owl:NamedIndividual rdf:about="http://xworks.gr/ontologies/ccso#CS/NC/RF/LO_List_the_scalability_benefits_of_hierarchical_addressing">
        <rdf:type rdf:resource="http://xworks.gr/ontologies/ccso#LearningOutcome"/>
        <acquiredInCourse rdf:resource="http://xworks.gr/ontologies/ccso#CS335_s2017-18/CS_BSc/CSD/SSE/UoC"/>
        <listedInKU rdf:resource="http://xworks.gr/ontologies/ccso#CS/NC/RF_Routing_and_Forwarding"/>
        <label rdf:datatype="http://www.w3.org/2001/XMLSchema#string">List the scalability benefits of hierarchical addressing</label>
        <levelofMastery rdf:datatype="http://www.w3.org/2001/XMLSchema#string">Familiarity</levelofMastery>
    </owl:NamedIndividual>
    


    <!-- http://xworks.gr/ontologies/ccso#CS/NC/RF/T_Internet_Protocol -->

    <owl:NamedIndividual rdf:about="http://xworks.gr/ontologies/ccso#CS/NC/RF/T_Internet_Protocol">
        <rdf:type rdf:resource="http://xworks.gr/ontologies/ccso#Topic"/>
        <coveredInCourse rdf:resource="http://xworks.gr/ontologies/ccso#CS335_s2017-18/CS_BSc/CSD/SSE/UoC"/>
        <listedInKU rdf:resource="http://xworks.gr/ontologies/ccso#CS/NC/RF_Routing_and_Forwarding"/>
        <label rdf:datatype="http://www.w3.org/2001/XMLSchema#string">Internet Protocol (IP)</label>
        <topicType rdf:datatype="http://www.w3.org/2001/XMLSchema#string">Core-Tier-2</topicType>
    </owl:NamedIndividual>
    


    <!-- http://xworks.gr/ontologies/ccso#CS/NC/RF/T_Routing_versus_forwarding -->

    <owl:NamedIndividual rdf:about="http://xworks.gr/ontologies/ccso#CS/NC/RF/T_Routing_versus_forwarding">
        <rdf:type rdf:resource="http://xworks.gr/ontologies/ccso#Topic"/>
        <coveredInCourse rdf:resource="http://xworks.gr/ontologies/ccso#CS335_s2017-18/CS_BSc/CSD/SSE/UoC"/>
        <listedInKU rdf:resource="http://xworks.gr/ontologies/ccso#CS/NC/RF_Routing_and_Forwarding"/>
        <label rdf:datatype="http://www.w3.org/2001/XMLSchema#string">Routing versus forwarding</label>
        <topicType rdf:datatype="http://www.w3.org/2001/XMLSchema#string">Core-Tier-2</topicType>
    </owl:NamedIndividual>
    


    <!-- http://xworks.gr/ontologies/ccso#CS/NC/RF/T_Scalability_issues -->

    <owl:NamedIndividual rdf:about="http://xworks.gr/ontologies/ccso#CS/NC/RF/T_Scalability_issues">
        <rdf:type rdf:resource="http://xworks.gr/ontologies/ccso#Topic"/>
        <coveredInCourse rdf:resource="http://xworks.gr/ontologies/ccso#CS335_s2017-18/CS_BSc/CSD/SSE/UoC"/>
        <listedInKU rdf:resource="http://xworks.gr/ontologies/ccso#CS/NC/RF_Routing_and_Forwarding"/>
        <label rdf:datatype="http://www.w3.org/2001/XMLSchema#string">Scalability issues (hierarchical addressing)</label>
        <topicType rdf:datatype="http://www.w3.org/2001/XMLSchema#string">Core-Tier-2</topicType>
    </owl:NamedIndividual>
    


    <!-- http://xworks.gr/ontologies/ccso#CS/NC/RF/T_Static_routing -->

    <owl:NamedIndividual rdf:about="http://xworks.gr/ontologies/ccso#CS/NC/RF/T_Static_routing">
        <rdf:type rdf:resource="http://xworks.gr/ontologies/ccso#Topic"/>
        <coveredInCourse rdf:resource="http://xworks.gr/ontologies/ccso#CS335_s2017-18/CS_BSc/CSD/SSE/UoC"/>
        <listedInKU rdf:resource="http://xworks.gr/ontologies/ccso#CS/NC/RF_Routing_and_Forwarding"/>
        <label rdf:datatype="http://www.w3.org/2001/XMLSchema#string">Static routing</label>
        <topicType rdf:datatype="http://www.w3.org/2001/XMLSchema#string">Core-Tier-2</topicType>
    </owl:NamedIndividual>
    


    <!-- http://xworks.gr/ontologies/ccso#CS/OS/OSP_Operating_System_Principles -->

    <owl:NamedIndividual rdf:about="http://xworks.gr/ontologies/ccso#CS/OS/OSP_Operating_System_Principles">
        <rdf:type rdf:resource="http://xworks.gr/ontologies/ccso#Discipline"/>
        <rdf:type rdf:resource="http://xworks.gr/ontologies/ccso#FieldofStudy"/>
        <rdf:type rdf:resource="http://xworks.gr/ontologies/ccso#KnowledgeUnit"/>
        <partOfFS rdf:resource="http://xworks.gr/ontologies/ccso#Computer_Science"/>
        <partOfFS rdf:resource="http://xworks.gr/ontologies/ccso#Computer_Science_Curricula_2013"/>
        <partOfFS rdf:resource="http://xworks.gr/ontologies/ccso#CS/SW_Software_Engineering_Software_Systems_and_Applications"/>
        <abbreviation rdf:datatype="http://www.w3.org/2001/XMLSchema#string">CS/OS/OSP</abbreviation>
        <fsName rdf:datatype="http://www.w3.org/2001/XMLSchema#string">Operating System Principles</fsName>
    </owl:NamedIndividual>
    


    <!-- http://xworks.gr/ontologies/ccso#CS/OS/OSP/LO_Defend_the_need_for_APIs_and_middleware -->

    <owl:NamedIndividual rdf:about="http://xworks.gr/ontologies/ccso#CS/OS/OSP/LO_Defend_the_need_for_APIs_and_middleware">
        <rdf:type rdf:resource="http://xworks.gr/ontologies/ccso#LearningOutcome"/>
        <label rdf:datatype="http://www.w3.org/2001/XMLSchema#string">Defend the need for APIs and middleware</label>
        <levelofMastery rdf:datatype="http://www.w3.org/2001/XMLSchema#string">Assessment</levelofMastery>
    </owl:NamedIndividual>
    


    <!-- http://xworks.gr/ontologies/ccso#CS/OS/OSP/LO_Describe_how_computing_resources_are_used -->

    <owl:NamedIndividual rdf:about="http://xworks.gr/ontologies/ccso#CS/OS/OSP/LO_Describe_how_computing_resources_are_used">
        <rdf:type rdf:resource="http://xworks.gr/ontologies/ccso#LearningOutcome"/>
        <label rdf:datatype="http://www.w3.org/2001/XMLSchema#string">Describe how computing resources are used by application software and managed by system software</label>
        <levelofMastery rdf:datatype="http://www.w3.org/2001/XMLSchema#string">Familiarity</levelofMastery>
    </owl:NamedIndividual>
    


    <!-- http://xworks.gr/ontologies/ccso#CS/OS/OSP/LO_Explain_the_concept_of_a_logical_layer -->

    <owl:NamedIndividual rdf:about="http://xworks.gr/ontologies/ccso#CS/OS/OSP/LO_Explain_the_concept_of_a_logical_layer">
        <rdf:type rdf:resource="http://xworks.gr/ontologies/ccso#LearningOutcome"/>
        <label rdf:datatype="http://www.w3.org/2001/XMLSchema#string">Explain the concept of a logical layer</label>
        <levelofMastery rdf:datatype="http://www.w3.org/2001/XMLSchema#string">Familiarity</levelofMastery>
    </owl:NamedIndividual>
    


    <!-- http://xworks.gr/ontologies/ccso#CS/OS/OSP/T_Concepts_of_APIs -->

    <owl:NamedIndividual rdf:about="http://xworks.gr/ontologies/ccso#CS/OS/OSP/T_Concepts_of_APIs">
        <rdf:type rdf:resource="http://xworks.gr/ontologies/ccso#Topic"/>
        <label rdf:datatype="http://www.w3.org/2001/XMLSchema#string">Concepts of application program interfaces (APIs)</label>
        <topicType rdf:datatype="http://www.w3.org/2001/XMLSchema#string">Core-Tier-1</topicType>
    </owl:NamedIndividual>
    


    <!-- http://xworks.gr/ontologies/ccso#CS/OS/OSP/T_Structuring_methods -->

    <owl:NamedIndividual rdf:about="http://xworks.gr/ontologies/ccso#CS/OS/OSP/T_Structuring_methods">
        <rdf:type rdf:resource="http://xworks.gr/ontologies/ccso#Topic"/>
        <label rdf:datatype="http://www.w3.org/2001/XMLSchema#string">Structuring methods (monolithic, layered, modular, micro-kernel models)</label>
        <topicType rdf:datatype="http://www.w3.org/2001/XMLSchema#string">Core-Tier-1</topicType>
    </owl:NamedIndividual>
    


    <!-- http://xworks.gr/ontologies/ccso#CS/OS/OSP/T_Abstractions,_processes,_and_resources -->

    <owl:NamedIndividual rdf:about="http://xworks.gr/ontologies/ccso#CS/OS/OSP/T_Abstractions,_processes,_and_resources">
        <rdf:type rdf:resource="http://xworks.gr/ontologies/ccso#Topic"/>
        <label rdf:datatype="http://www.w3.org/2001/XMLSchema#string">Abstractions, processes, and resources</label>
        <topicType rdf:datatype="http://www.w3.org/2001/XMLSchema#string">Core-Tier-1</topicType>
    </owl:NamedIndividual>
    


    <!-- http://xworks.gr/ontologies/ccso#CS/PL/LO_Correctly_reason_about_control_flow_in_a_program_using_dynamic_dispatch -->

    <owl:NamedIndividual rdf:about="http://xworks.gr/ontologies/ccso#CS/PL/LO_Correctly_reason_about_control_flow_in_a_program_using_dynamic_dispatch">
        <rdf:type rdf:resource="http://xworks.gr/ontologies/ccso#LearningOutcome"/>
        <acquiredInCourse rdf:resource="http://xworks.gr/ontologies/ccso#CS150s1/CS_BSc/CSD/SSE/UoC"/>
        <acquiredInCourse rdf:resource="http://xworks.gr/ontologies/ccso#CS252s1/CS_BSc/CSD/SSE/UoC"/>
        <acquiredInCourse rdf:resource="http://xworks.gr/ontologies/ccso#CS342s1/CS_BSc/CSD/SSE/UoC"/>
        <listedInKU rdf:resource="http://xworks.gr/ontologies/ccso#CS/PL/OOP_Object-Oriented_Programming"/>
        <label rdf:datatype="http://www.w3.org/2001/XMLSchema#string">Correctly reason about control flow in a program using dynamic dispatch</label>
        <levelofMastery rdf:datatype="http://www.w3.org/2001/XMLSchema#string">Usage</levelofMastery>
    </owl:NamedIndividual>
    


    <!-- http://xworks.gr/ontologies/ccso#CS/PL/LO_Use_subclassing_to_design_simple_class_hierarchies_that_allow_code_to_be_reused_for_distinct_subclasses -->

    <owl:NamedIndividual rdf:about="http://xworks.gr/ontologies/ccso#CS/PL/LO_Use_subclassing_to_design_simple_class_hierarchies_that_allow_code_to_be_reused_for_distinct_subclasses">
        <rdf:type rdf:resource="http://xworks.gr/ontologies/ccso#LearningOutcome"/>
        <acquiredInCourse rdf:resource="http://xworks.gr/ontologies/ccso#CS150s1/CS_BSc/CSD/SSE/UoC"/>
        <acquiredInCourse rdf:resource="http://xworks.gr/ontologies/ccso#CS342s1/CS_BSc/CSD/SSE/UoC"/>
        <acquiredInCourse rdf:resource="http://xworks.gr/ontologies/ccso#TP10K4s1/IE_BSc/IED/STEF/TEIC"/>
        <listedInKU rdf:resource="http://xworks.gr/ontologies/ccso#CS/PL/OOP_Object-Oriented_Programming"/>
        <label rdf:datatype="http://www.w3.org/2001/XMLSchema#string">Use subclassing to design simple class hierarchies that allow code to be reused for distinct subclasses</label>
        <levelofMastery rdf:datatype="http://www.w3.org/2001/XMLSchema#string">Usage</levelofMastery>
    </owl:NamedIndividual>
    


    <!-- http://xworks.gr/ontologies/ccso#CS/PL/LP_Logic_Programming -->

    <owl:NamedIndividual rdf:about="http://xworks.gr/ontologies/ccso#CS/PL/LP_Logic_Programming">
        <rdf:type rdf:resource="http://xworks.gr/ontologies/ccso#Discipline"/>
        <rdf:type rdf:resource="http://xworks.gr/ontologies/ccso#FieldofStudy"/>
        <rdf:type rdf:resource="http://xworks.gr/ontologies/ccso#KnowledgeUnit"/>
        <partOfFS rdf:resource="http://xworks.gr/ontologies/ccso#Computer_Science"/>
        <partOfFS rdf:resource="http://xworks.gr/ontologies/ccso#Computer_Science_Curricula_2013"/>
        <partOfFS rdf:resource="http://xworks.gr/ontologies/ccso#CS/PL_Programming_Languages"/>
        <abbreviation rdf:datatype="http://www.w3.org/2001/XMLSchema#string">CS/PL/LP</abbreviation>
        <fsName rdf:datatype="http://www.w3.org/2001/XMLSchema#string">CS/PL/LP Logic Programming</fsName>
    </owl:NamedIndividual>
    


    <!-- http://xworks.gr/ontologies/ccso#CS/PL/OOP_Object-Oriented_Programming -->

    <owl:NamedIndividual rdf:about="http://xworks.gr/ontologies/ccso#CS/PL/OOP_Object-Oriented_Programming">
        <rdf:type rdf:resource="http://xworks.gr/ontologies/ccso#Discipline"/>
        <rdf:type rdf:resource="http://xworks.gr/ontologies/ccso#FieldofStudy"/>
        <rdf:type rdf:resource="http://xworks.gr/ontologies/ccso#KnowledgeUnit"/>
        <lists rdf:resource="http://xworks.gr/ontologies/ccso#CS/PL/LO_Correctly_reason_about_control_flow_in_a_program_using_dynamic_dispatch"/>
        <lists rdf:resource="http://xworks.gr/ontologies/ccso#CS/PL/LO_Use_subclassing_to_design_simple_class_hierarchies_that_allow_code_to_be_reused_for_distinct_subclasses"/>
        <lists rdf:resource="http://xworks.gr/ontologies/ccso#CS/PL/LO_Compare_and_contrast_the_procedural/functional_approach_and_the_object-oriented_approach"/>
        <lists rdf:resource="http://xworks.gr/ontologies/ccso#CS/PL/T_Definition_of_classes:fields,methods,and_constructors"/>
        <lists rdf:resource="http://xworks.gr/ontologies/ccso#CS/PL/T_Dynamic_dispatch:Definition_of_Method-Call"/>
        <lists rdf:resource="http://xworks.gr/ontologies/ccso#CS/PL/T_Object-Oriented_Design,Class-Hierarchy_design_for_modeling"/>
        <lists rdf:resource="http://xworks.gr/ontologies/ccso#CS/PL/T_Object-Oriented_Design,_Decomposition_into_objects_carrying_state_and_having_behavior"/>
        <lists rdf:resource="http://xworks.gr/ontologies/ccso#CS/PL/T_Subclasses,Inheritance,and_Method_Overriding"/>
        <partOfFS rdf:resource="http://xworks.gr/ontologies/ccso#Computer_Science"/>
        <partOfFS rdf:resource="http://xworks.gr/ontologies/ccso#Computer_Science_Curricula_2013"/>
        <partOfFS rdf:resource="http://xworks.gr/ontologies/ccso#CS/PL_Programming_Languages"/>
        <abbreviation rdf:datatype="http://www.w3.org/2001/XMLSchema#string">CS/PL/OOP</abbreviation>
        <fsName rdf:datatype="http://www.w3.org/2001/XMLSchema#string">CS/PL/OOP Object-Oriented Programming</fsName>
    </owl:NamedIndividual>
    


    <!-- http://xworks.gr/ontologies/ccso#CS/PL/LO_Compare_and_contrast_the_procedural/functional_approach_and_the_object-oriented_approach -->

    <owl:NamedIndividual rdf:about="http://xworks.gr/ontologies/ccso#CS/PL/LO_Compare_and_contrast_the_procedural/functional_approach_and_the_object-oriented_approach">
        <rdf:type rdf:resource="http://xworks.gr/ontologies/ccso#LearningOutcome"/>
        <acquiredInCourse rdf:resource="http://xworks.gr/ontologies/ccso#CS150s1/CS_BSc/CSD/SSE/UoC"/>
        <acquiredInCourse rdf:resource="http://xworks.gr/ontologies/ccso#CS252s1/CS_BSc/CSD/SSE/UoC"/>
        <acquiredInCourse rdf:resource="http://xworks.gr/ontologies/ccso#CS342s1/CS_BSc/CSD/SSE/UoC"/>
        <acquiredInCourse rdf:resource="http://xworks.gr/ontologies/ccso#TP10K4s1/IE_BSc/IED/STEF/TEIC"/>
        <acquiredInCourse rdf:resource="http://xworks.gr/ontologies/ccso#TP20K4s1/IE_BSc/IED/STEF/TEIC"/>
        <listedInKU rdf:resource="http://xworks.gr/ontologies/ccso#CS/PL/OOP_Object-Oriented_Programming"/>
        <label rdf:datatype="http://www.w3.org/2001/XMLSchema#string">Compare and contrast the procedural/functional approach and the object-oriented approach</label>
        <levelofMastery rdf:datatype="http://www.w3.org/2001/XMLSchema#string">Assessment</levelofMastery>
    </owl:NamedIndividual>
    


    <!-- http://xworks.gr/ontologies/ccso#CS/PL/T_Definition_of_classes:fields,methods,and_constructors -->

    <owl:NamedIndividual rdf:about="http://xworks.gr/ontologies/ccso#CS/PL/T_Definition_of_classes:fields,methods,and_constructors">
        <rdf:type rdf:resource="http://xworks.gr/ontologies/ccso#Topic"/>
        <coveredInCourse rdf:resource="http://xworks.gr/ontologies/ccso#CS150s1/CS_BSc/CSD/SSE/UoC"/>
        <coveredInCourse rdf:resource="http://xworks.gr/ontologies/ccso#CS340s1/CS_BSc/CSD/SSE/UoC"/>
        <coveredInCourse rdf:resource="http://xworks.gr/ontologies/ccso#CS342s1/CS_BSc/CSD/SSE/UoC"/>
        <coveredInCourse rdf:resource="http://xworks.gr/ontologies/ccso#TP10K4s1/IE_BSc/IED/STEF/TEIC"/>
        <coveredInCourse rdf:resource="http://xworks.gr/ontologies/ccso#TP20K4s1/IE_BSc/IED/STEF/TEIC"/>
        <coveredInCourse rdf:resource="http://xworks.gr/ontologies/ccso#TP50L5s1/IE_BSc/IED/STEF/TEIC"/>
        <listedInKU rdf:resource="http://xworks.gr/ontologies/ccso#CS/PL/OOP_Object-Oriented_Programming"/>
        <label rdf:datatype="http://www.w3.org/2001/XMLSchema#string">Definition of classes: fields, methods, and constructors</label>
    </owl:NamedIndividual>
    


    <!-- http://xworks.gr/ontologies/ccso#CS/PL/T_Dynamic_dispatch:Definition_of_Method-Call -->

    <owl:NamedIndividual rdf:about="http://xworks.gr/ontologies/ccso#CS/PL/T_Dynamic_dispatch:Definition_of_Method-Call">
        <rdf:type rdf:resource="http://xworks.gr/ontologies/ccso#Topic"/>
        <coveredInCourse rdf:resource="http://xworks.gr/ontologies/ccso#CS150s1/CS_BSc/CSD/SSE/UoC"/>
        <coveredInCourse rdf:resource="http://xworks.gr/ontologies/ccso#CS342s1/CS_BSc/CSD/SSE/UoC"/>
        <coveredInCourse rdf:resource="http://xworks.gr/ontologies/ccso#TP20K4s1/IE_BSc/IED/STEF/TEIC"/>
        <coveredInCourse rdf:resource="http://xworks.gr/ontologies/ccso#TP50L5s1/IE_BSc/IED/STEF/TEIC"/>
        <coveredInCourse rdf:resource="http://xworks.gr/ontologies/ccso#TP60D5s1/IE_BSc/IED/STEF/TEIC"/>
        <listedInKU rdf:resource="http://xworks.gr/ontologies/ccso#CS/PL/OOP_Object-Oriented_Programming"/>
        <label rdf:datatype="http://www.w3.org/2001/XMLSchema#string">Dynamic dispatch: definition of method-call</label>
    </owl:NamedIndividual>
    


    <!-- http://xworks.gr/ontologies/ccso#CS/PL/T_Object-Oriented_Design,Class-Hierarchy_design_for_modeling -->

    <owl:NamedIndividual rdf:about="http://xworks.gr/ontologies/ccso#CS/PL/T_Object-Oriented_Design,Class-Hierarchy_design_for_modeling">
        <rdf:type rdf:resource="http://xworks.gr/ontologies/ccso#Topic"/>
        <coveredInCourse rdf:resource="http://xworks.gr/ontologies/ccso#CS150s1/CS_BSc/CSD/SSE/UoC"/>
        <coveredInCourse rdf:resource="http://xworks.gr/ontologies/ccso#CS252s1/CS_BSc/CSD/SSE/UoC"/>
        <coveredInCourse rdf:resource="http://xworks.gr/ontologies/ccso#CS342s1/CS_BSc/CSD/SSE/UoC"/>
        <coveredInCourse rdf:resource="http://xworks.gr/ontologies/ccso#IM201s1/IM_MSc/IED/STEF/TEI"/>
        <coveredInCourse rdf:resource="http://xworks.gr/ontologies/ccso#TP10K4s1/IE_BSc/IED/STEF/TEIC"/>
        <coveredInCourse rdf:resource="http://xworks.gr/ontologies/ccso#TP50L5s1/IE_BSc/IED/STEF/TEIC"/>
        <listedInKU rdf:resource="http://xworks.gr/ontologies/ccso#CS/PL/OOP_Object-Oriented_Programming"/>
        <label rdf:datatype="http://www.w3.org/2001/XMLSchema#string">Object-Oriented Design, Class-hierarchy design for modeling</label>
    </owl:NamedIndividual>
    


    <!-- http://xworks.gr/ontologies/ccso#CS/PL/T_Object-Oriented_Design,_Decomposition_into_objects_carrying_state_and_having_behavior -->

    <owl:NamedIndividual rdf:about="http://xworks.gr/ontologies/ccso#CS/PL/T_Object-Oriented_Design,_Decomposition_into_objects_carrying_state_and_having_behavior">
        <rdf:type rdf:resource="http://xworks.gr/ontologies/ccso#Topic"/>
        <coveredInCourse rdf:resource="http://xworks.gr/ontologies/ccso#CS150s1/CS_BSc/CSD/SSE/UoC"/>
        <coveredInCourse rdf:resource="http://xworks.gr/ontologies/ccso#CS252s1/CS_BSc/CSD/SSE/UoC"/>
        <coveredInCourse rdf:resource="http://xworks.gr/ontologies/ccso#TP10K4s1/IE_BSc/IED/STEF/TEIC"/>
        <coveredInCourse rdf:resource="http://xworks.gr/ontologies/ccso#TP50L3s1/IE_BSc/IED/STEF/TEIC"/>
        <coveredInCourse rdf:resource="http://xworks.gr/ontologies/ccso#TP50L5s1/IE_BSc/IED/STEF/TEIC"/>
        <listedInKU rdf:resource="http://xworks.gr/ontologies/ccso#CS/PL/OOP_Object-Oriented_Programming"/>
        <label rdf:datatype="http://www.w3.org/2001/XMLSchema#string">Object-Oriented Design, Decomposition into objects carrying state and having behavior</label>
    </owl:NamedIndividual>
    


    <!-- http://xworks.gr/ontologies/ccso#CS/PL/T_Subclasses,Inheritance,and_Method_Overriding -->

    <owl:NamedIndividual rdf:about="http://xworks.gr/ontologies/ccso#CS/PL/T_Subclasses,Inheritance,and_Method_Overriding">
        <rdf:type rdf:resource="http://xworks.gr/ontologies/ccso#Topic"/>
        <coveredInCourse rdf:resource="http://xworks.gr/ontologies/ccso#CS150s1/CS_BSc/CSD/SSE/UoC"/>
        <coveredInCourse rdf:resource="http://xworks.gr/ontologies/ccso#CS252s1/CS_BSc/CSD/SSE/UoC"/>
        <coveredInCourse rdf:resource="http://xworks.gr/ontologies/ccso#CS342s1/CS_BSc/CSD/SSE/UoC"/>
        <coveredInCourse rdf:resource="http://xworks.gr/ontologies/ccso#IM201s1/IM_MSc/IED/STEF/TEI"/>
        <coveredInCourse rdf:resource="http://xworks.gr/ontologies/ccso#TP20K4s1/IE_BSc/IED/STEF/TEIC"/>
        <coveredInCourse rdf:resource="http://xworks.gr/ontologies/ccso#TP50L3s1/IE_BSc/IED/STEF/TEIC"/>
        <coveredInCourse rdf:resource="http://xworks.gr/ontologies/ccso#TP50L5s1/IE_BSc/IED/STEF/TEIC"/>
        <coveredInCourse rdf:resource="http://xworks.gr/ontologies/ccso#TP60D5s1/IE_BSc/IED/STEF/TEIC"/>
        <listedInKU rdf:resource="http://xworks.gr/ontologies/ccso#CS/PL/OOP_Object-Oriented_Programming"/>
        <label rdf:datatype="http://www.w3.org/2001/XMLSchema#string">Subclasses, inheritance, and method overriding</label>
    </owl:NamedIndividual>
    


    <!-- http://xworks.gr/ontologies/ccso#CS100/CS_BSc/CSD/SSE/UoC -->

    <owl:NamedIndividual rdf:about="http://xworks.gr/ontologies/ccso#CS100/CS_BSc/CSD/SSE/UoC">
        <rdf:type rdf:resource="http://xworks.gr/ontologies/ccso#Course"/>
        <hasSyllabus rdf:resource="http://xworks.gr/ontologies/ccso#CS100s1/CS_BSc/CSD/SSE/UoC"/>
        <includedIn rdf:resource="http://xworks.gr/ontologies/ccso#BSc_Computer_Science/CS_BSc/CSD/SSE/UoC"/>
        <offeredBy rdf:resource="http://xworks.gr/ontologies/ccso#Computers_Sciences_Department_of_University_of_Crete"/>
        <code rdf:datatype="http://www.w3.org/2001/XMLSchema#string">CS100</code>
        <courseType rdf:datatype="http://www.w3.org/2001/XMLSchema#string">Core</courseType>
        <csName rdf:datatype="http://www.w3.org/2001/XMLSchema#string">Introduction to Computer Science</csName>
    </owl:NamedIndividual>
    


    <!-- http://xworks.gr/ontologies/ccso#CS100s1/CS_BSc/CSD/SSE/UoC -->

    <owl:NamedIndividual rdf:about="http://xworks.gr/ontologies/ccso#CS100s1/CS_BSc/CSD/SSE/UoC">
        <rdf:type rdf:resource="http://xworks.gr/ontologies/ccso#Syllabus"/>
        <affiliatedWith rdf:resource="http://xworks.gr/ontologies/ccso#Gramma_Joanna"/>
        <affiliatedWith rdf:resource="http://xworks.gr/ontologies/ccso#Plexousakis_Dimitris"/>
        <affiliatedWith rdf:resource="http://xworks.gr/ontologies/ccso#Pratikakis_Polyvios"/>
        <hasCourseAssistant rdf:resource="http://xworks.gr/ontologies/ccso#Gramma_Joanna"/>
        <hasInstructor rdf:resource="http://xworks.gr/ontologies/ccso#Plexousakis_Dimitris"/>
        <hasSupervisor rdf:resource="http://xworks.gr/ontologies/ccso#Pratikakis_Polyvios"/>
        <syllabusOf rdf:resource="http://xworks.gr/ontologies/ccso#CS100/CS_BSc/CSD/SSE/UoC"/>
        <courseType rdf:datatype="http://www.w3.org/2001/XMLSchema#string">Core</courseType>
        <creditsECTS rdf:datatype="http://www.w3.org/2001/XMLSchema#short">8</creditsECTS>
        <csName rdf:datatype="http://www.w3.org/2001/XMLSchema#string">Syllabus of course CS100 Introduction to Computer Science</csName>
        <semesterinProgram rdf:datatype="http://www.w3.org/2001/XMLSchema#short">1</semesterinProgram>
    </owl:NamedIndividual>
    


    <!-- http://xworks.gr/ontologies/ccso#CS108/CS_BSc/CSD/SSE/UoC -->

    <owl:NamedIndividual rdf:about="http://xworks.gr/ontologies/ccso#CS108/CS_BSc/CSD/SSE/UoC">
        <rdf:type rdf:resource="http://xworks.gr/ontologies/ccso#Course"/>
        <hasSyllabus rdf:resource="http://xworks.gr/ontologies/ccso#CS108s1/CS_BSc/CSD/SSE/UoC"/>
        <includedIn rdf:resource="http://xworks.gr/ontologies/ccso#BSc_Computer_Science/CS_BSc/CSD/SSE/UoC"/>
        <offeredBy rdf:resource="http://xworks.gr/ontologies/ccso#Computers_Sciences_Department_of_University_of_Crete"/>
        <code rdf:datatype="http://www.w3.org/2001/XMLSchema#string">CS108</code>
        <courseType rdf:datatype="http://www.w3.org/2001/XMLSchema#string">Core</courseType>
        <csName rdf:datatype="http://www.w3.org/2001/XMLSchema#string">English I</csName>
    </owl:NamedIndividual>
    


    <!-- http://xworks.gr/ontologies/ccso#CS108s1/CS_BSc/CSD/SSE/UoC -->

    <owl:NamedIndividual rdf:about="http://xworks.gr/ontologies/ccso#CS108s1/CS_BSc/CSD/SSE/UoC">
        <rdf:type rdf:resource="http://xworks.gr/ontologies/ccso#Syllabus"/>
        <affiliatedWith rdf:resource="http://xworks.gr/ontologies/ccso#Pasta_Flora"/>
        <affiliatedWith rdf:resource="http://xworks.gr/ontologies/ccso#Rizopoulou_Noni"/>
        <hasCourseAssistant rdf:resource="http://xworks.gr/ontologies/ccso#Pasta_Flora"/>
        <hasInstructor rdf:resource="http://xworks.gr/ontologies/ccso#Rizopoulou_Noni"/>
        <hasSupervisor rdf:resource="http://xworks.gr/ontologies/ccso#Rizopoulou_Noni"/>
        <syllabusOf rdf:resource="http://xworks.gr/ontologies/ccso#CS108/CS_BSc/CSD/SSE/UoC"/>
        <courseType rdf:datatype="http://www.w3.org/2001/XMLSchema#string">Core</courseType>
        <creditsECTS rdf:datatype="http://www.w3.org/2001/XMLSchema#short">4</creditsECTS>
        <csName rdf:datatype="http://www.w3.org/2001/XMLSchema#string">Syllabus of course CS108 English I</csName>
        <semesterinProgram rdf:datatype="http://www.w3.org/2001/XMLSchema#short">1</semesterinProgram>
    </owl:NamedIndividual>
    


    <!-- http://xworks.gr/ontologies/ccso#CS109/CS_BSc/CSD/SSE/UoC -->

    <owl:NamedIndividual rdf:about="http://xworks.gr/ontologies/ccso#CS109/CS_BSc/CSD/SSE/UoC">
        <rdf:type rdf:resource="http://xworks.gr/ontologies/ccso#Course"/>
        <affiliatedWith rdf:resource="http://xworks.gr/ontologies/ccso#Starkeiou_Nick"/>
        <affiliatedWith rdf:resource="http://xworks.gr/ontologies/ccso#Starkeiou_Vakis"/>
        <hasAttender rdf:resource="http://xworks.gr/ontologies/ccso#Starkeiou_Nick"/>
        <hasAttender rdf:resource="http://xworks.gr/ontologies/ccso#Starkeiou_Vakis"/>
        <hasPrerequisite rdf:resource="http://xworks.gr/ontologies/ccso#CS108/CS_BSc/CSD/SSE/UoC"/>
        <hasSyllabus rdf:resource="http://xworks.gr/ontologies/ccso#CS109s1/CS_BSc/CSD/SSE/UoC"/>
        <includedIn rdf:resource="http://xworks.gr/ontologies/ccso#BSc_Computer_Science/CS_BSc/CSD/SSE/UoC"/>
        <offeredBy rdf:resource="http://xworks.gr/ontologies/ccso#Computers_Sciences_Department_of_University_of_Crete"/>
        <courseType rdf:datatype="http://www.w3.org/2001/XMLSchema#string">Core</courseType>
        <csName rdf:datatype="http://www.w3.org/2001/XMLSchema#string">English II</csName>
    </owl:NamedIndividual>
    


    <!-- http://xworks.gr/ontologies/ccso#CS109s1/CS_BSc/CSD/SSE/UoC -->

    <owl:NamedIndividual rdf:about="http://xworks.gr/ontologies/ccso#CS109s1/CS_BSc/CSD/SSE/UoC">
        <rdf:type rdf:resource="http://xworks.gr/ontologies/ccso#Syllabus"/>
        <affiliatedWith rdf:resource="http://xworks.gr/ontologies/ccso#Pasta_Flora"/>
        <affiliatedWith rdf:resource="http://xworks.gr/ontologies/ccso#Rizopoulou_Noni"/>
        <hasCourseAssistant rdf:resource="http://xworks.gr/ontologies/ccso#Pasta_Flora"/>
        <hasInstructor rdf:resource="http://xworks.gr/ontologies/ccso#Rizopoulou_Noni"/>
        <hasSupervisor rdf:resource="http://xworks.gr/ontologies/ccso#Rizopoulou_Noni"/>
        <syllabusOf rdf:resource="http://xworks.gr/ontologies/ccso#CS109/CS_BSc/CSD/SSE/UoC"/>
        <courseType rdf:datatype="http://www.w3.org/2001/XMLSchema#string">Core</courseType>
        <creditsECTS rdf:datatype="http://www.w3.org/2001/XMLSchema#short">4</creditsECTS>
        <csName rdf:datatype="http://www.w3.org/2001/XMLSchema#string">Syllabus of course CS109 English II</csName>
        <semesterinProgram rdf:datatype="http://www.w3.org/2001/XMLSchema#short">2</semesterinProgram>
    </owl:NamedIndividual>
    


    <!-- http://xworks.gr/ontologies/ccso#CS110/CS_BSc/CSD/SSE/UoC -->

    <owl:NamedIndividual rdf:about="http://xworks.gr/ontologies/ccso#CS110/CS_BSc/CSD/SSE/UoC">
        <rdf:type rdf:resource="http://xworks.gr/ontologies/ccso#Course"/>
        <affiliatedWith rdf:resource="http://xworks.gr/ontologies/ccso#Starkeiou_Nick"/>
        <hasAttender rdf:resource="http://xworks.gr/ontologies/ccso#Starkeiou_Nick"/>
        <hasSyllabus rdf:resource="http://xworks.gr/ontologies/ccso#CS110s1/CS_BSc/CSD/SSE/UoC"/>
        <includedIn rdf:resource="http://xworks.gr/ontologies/ccso#BSc_Computer_Science/CS_BSc/CSD/SSE/UoC"/>
        <offeredBy rdf:resource="http://xworks.gr/ontologies/ccso#Computers_Sciences_Department_of_University_of_Crete"/>
        <courseType rdf:datatype="http://www.w3.org/2001/XMLSchema#string">Core</courseType>
        <csName rdf:datatype="http://www.w3.org/2001/XMLSchema#string">Calculus I</csName>
    </owl:NamedIndividual>
    


    <!-- http://xworks.gr/ontologies/ccso#CS110s1/CS_BSc/CSD/SSE/UoC -->

    <owl:NamedIndividual rdf:about="http://xworks.gr/ontologies/ccso#CS110s1/CS_BSc/CSD/SSE/UoC">
        <rdf:type rdf:resource="http://xworks.gr/ontologies/ccso#Syllabus"/>
        <affiliatedWith rdf:resource="http://xworks.gr/ontologies/ccso#Gramma_Joanna"/>
        <affiliatedWith rdf:resource="http://xworks.gr/ontologies/ccso#Mouxtaris_Athanasios"/>
        <hasCourseAssistant rdf:resource="http://xworks.gr/ontologies/ccso#Gramma_Joanna"/>
        <hasInstructor rdf:resource="http://xworks.gr/ontologies/ccso#Mouxtaris_Athanasios"/>
        <hasSupervisor rdf:resource="http://xworks.gr/ontologies/ccso#Mouxtaris_Athanasios"/>
        <syllabusOf rdf:resource="http://xworks.gr/ontologies/ccso#CS110/CS_BSc/CSD/SSE/UoC"/>
        <courseType rdf:datatype="http://www.w3.org/2001/XMLSchema#string">Core</courseType>
        <creditsECTS rdf:datatype="http://www.w3.org/2001/XMLSchema#short">8</creditsECTS>
        <csName rdf:datatype="http://www.w3.org/2001/XMLSchema#string">Syllabus of course CS110 Calculus I</csName>
        <semesterinProgram rdf:datatype="http://www.w3.org/2001/XMLSchema#short">1</semesterinProgram>
    </owl:NamedIndividual>
    


    <!-- http://xworks.gr/ontologies/ccso#CS118/CS_BSc/CSD/SSE/UoC -->

    <owl:NamedIndividual rdf:about="http://xworks.gr/ontologies/ccso#CS118/CS_BSc/CSD/SSE/UoC">
        <rdf:type rdf:resource="http://xworks.gr/ontologies/ccso#Course"/>
        <affiliatedWith rdf:resource="http://xworks.gr/ontologies/ccso#Starkeiou_Vakis"/>
        <hasAttender rdf:resource="http://xworks.gr/ontologies/ccso#Starkeiou_Vakis"/>
        <hasSyllabus rdf:resource="http://xworks.gr/ontologies/ccso#CS118s1/CS_BSc/CSD/SSE/UoC"/>
        <includedIn rdf:resource="http://xworks.gr/ontologies/ccso#BSc_Computer_Science/CS_BSc/CSD/SSE/UoC"/>
        <offeredBy rdf:resource="http://xworks.gr/ontologies/ccso#Computers_Sciences_Department_of_University_of_Crete"/>
        <code rdf:datatype="http://www.w3.org/2001/XMLSchema#string">CS118/CS_BSc/CSD/SSE/UoC</code>
        <courseType rdf:datatype="http://www.w3.org/2001/XMLSchema#string">Core</courseType>
        <csName rdf:datatype="http://www.w3.org/2001/XMLSchema#string">Discrete Mathematics</csName>
    </owl:NamedIndividual>
    


    <!-- http://xworks.gr/ontologies/ccso#CS118s1/CS_BSc/CSD/SSE/UoC -->

    <owl:NamedIndividual rdf:about="http://xworks.gr/ontologies/ccso#CS118s1/CS_BSc/CSD/SSE/UoC">
        <rdf:type rdf:resource="http://xworks.gr/ontologies/ccso#Syllabus"/>
        <affiliatedWith rdf:resource="http://xworks.gr/ontologies/ccso#Argyros_Antonis"/>
        <affiliatedWith rdf:resource="http://xworks.gr/ontologies/ccso#Gramma_Joanna"/>
        <affiliatedWith rdf:resource="http://xworks.gr/ontologies/ccso#Kalogiannakis_Michail"/>
        <hasCourseAssistant rdf:resource="http://xworks.gr/ontologies/ccso#Gramma_Joanna"/>
        <hasInstructor rdf:resource="http://xworks.gr/ontologies/ccso#Kalogiannakis_Michail"/>
        <hasSupervisor rdf:resource="http://xworks.gr/ontologies/ccso#Argyros_Antonis"/>
        <syllabusOf rdf:resource="http://xworks.gr/ontologies/ccso#CS118/CS_BSc/CSD/SSE/UoC"/>
        <code rdf:datatype="http://www.w3.org/2001/XMLSchema#string">CS118s1/CS_BSc/CSD/SSE/UoC</code>
        <courseType rdf:datatype="http://www.w3.org/2001/XMLSchema#string">Core</courseType>
        <creditsECTS rdf:datatype="http://www.w3.org/2001/XMLSchema#short">6</creditsECTS>
        <csName rdf:datatype="http://www.w3.org/2001/XMLSchema#string">Syllabus of course CS118 Discrete Mathematics</csName>
        <semesterinProgram rdf:datatype="http://www.w3.org/2001/XMLSchema#short">1</semesterinProgram>
    </owl:NamedIndividual>
    


    <!-- http://xworks.gr/ontologies/ccso#CS119/CS_BSc/CSD/SSE/UoC -->

    <owl:NamedIndividual rdf:about="http://xworks.gr/ontologies/ccso#CS119/CS_BSc/CSD/SSE/UoC">
        <rdf:type rdf:resource="http://xworks.gr/ontologies/ccso#Course"/>
        <hasSyllabus rdf:resource="http://xworks.gr/ontologies/ccso#CS119s1/CS_BSc/CSD/SSE/UoC"/>
        <hasSyllabus rdf:resource="http://xworks.gr/ontologies/ccso#CS119s2017-18/CS_BSc/CSD/SSE/UoC"/>
        <includedIn rdf:resource="http://xworks.gr/ontologies/ccso#BSc_Computer_Science/CS_BSc/CSD/SSE/UoC"/>
        <offeredBy rdf:resource="http://xworks.gr/ontologies/ccso#Computers_Sciences_Department_of_University_of_Crete"/>
        <code rdf:datatype="http://www.w3.org/2001/XMLSchema#string">CS119/CS_BSc/CSD/SSE/UoC</code>
        <courseType rdf:datatype="http://www.w3.org/2001/XMLSchema#string">Core</courseType>
        <csName rdf:datatype="http://www.w3.org/2001/XMLSchema#string">Linear Algebra</csName>
    </owl:NamedIndividual>
    


    <!-- http://xworks.gr/ontologies/ccso#CS119s1/CS_BSc/CSD/SSE/UoC -->

    <owl:NamedIndividual rdf:about="http://xworks.gr/ontologies/ccso#CS119s1/CS_BSc/CSD/SSE/UoC">
        <rdf:type rdf:resource="http://xworks.gr/ontologies/ccso#Syllabus"/>
        <affiliatedWith rdf:resource="http://xworks.gr/ontologies/ccso#Gramma_Joanna"/>
        <affiliatedWith rdf:resource="http://xworks.gr/ontologies/ccso#Tziritas_George"/>
        <hasCourseAssistant rdf:resource="http://xworks.gr/ontologies/ccso#Gramma_Joanna"/>
        <hasInstructor rdf:resource="http://xworks.gr/ontologies/ccso#Tziritas_George"/>
        <hasSupervisor rdf:resource="http://xworks.gr/ontologies/ccso#Tziritas_George"/>
        <syllabusOf rdf:resource="http://xworks.gr/ontologies/ccso#CS119/CS_BSc/CSD/SSE/UoC"/>
        <code rdf:datatype="http://www.w3.org/2001/XMLSchema#string">CS119s1/CS_BSc/CSD/SSE/UoC</code>
        <courseType rdf:datatype="http://www.w3.org/2001/XMLSchema#string">Core</courseType>
        <creditsECTS rdf:datatype="http://www.w3.org/2001/XMLSchema#short">6</creditsECTS>
        <csName rdf:datatype="http://www.w3.org/2001/XMLSchema#string">Syllabus of course CS119 Linear Algebra</csName>
        <semesterinProgram rdf:datatype="http://www.w3.org/2001/XMLSchema#short">2</semesterinProgram>
    </owl:NamedIndividual>
    


    <!-- http://xworks.gr/ontologies/ccso#CS119s2017-18/CS_BSc/CSD/SSE/UoC -->

    <owl:NamedIndividual rdf:about="http://xworks.gr/ontologies/ccso#CS119s2017-18/CS_BSc/CSD/SSE/UoC">
        <rdf:type rdf:resource="http://xworks.gr/ontologies/ccso#Syllabus"/>
        <affiliatedWith rdf:resource="http://xworks.gr/ontologies/ccso#Pappa_Pepi"/>
        <affiliatedWith rdf:resource="http://xworks.gr/ontologies/ccso#Tziritas_George"/>
        <hasCourseAssistant rdf:resource="http://xworks.gr/ontologies/ccso#Pappa_Pepi"/>
        <hasInstructor rdf:resource="http://xworks.gr/ontologies/ccso#Tziritas_George"/>
        <hasSupervisor rdf:resource="http://xworks.gr/ontologies/ccso#Tziritas_George"/>
        <syllabusOf rdf:resource="http://xworks.gr/ontologies/ccso#CS119/CS_BSc/CSD/SSE/UoC"/>
        <code rdf:datatype="http://www.w3.org/2001/XMLSchema#string">CS119s2017-18/CS_BSc/CSD/SSE/UoC</code>
        <courseType rdf:datatype="http://www.w3.org/2001/XMLSchema#string">Core</courseType>
        <creditsECTS rdf:datatype="http://www.w3.org/2001/XMLSchema#short">6</creditsECTS>
        <csName rdf:datatype="http://www.w3.org/2001/XMLSchema#string">Syllabus of course CS119 Linear Algebra
fro Academic Year 2017-18</csName>
        <semesterinProgram rdf:datatype="http://www.w3.org/2001/XMLSchema#short">2</semesterinProgram>
    </owl:NamedIndividual>
    


    <!-- http://xworks.gr/ontologies/ccso#CS120/CS_BSc/CSD/SSE/UoC -->

    <owl:NamedIndividual rdf:about="http://xworks.gr/ontologies/ccso#CS120/CS_BSc/CSD/SSE/UoC">
        <rdf:type rdf:resource="http://xworks.gr/ontologies/ccso#Course"/>
        <affiliatedWith rdf:resource="http://xworks.gr/ontologies/ccso#Starkeiou_Vakis"/>
        <hasAttender rdf:resource="http://xworks.gr/ontologies/ccso#Starkeiou_Vakis"/>
        <hasSyllabus rdf:resource="http://xworks.gr/ontologies/ccso#CS120s1/CS_BSc/CSD/SSE/UoC"/>
        <includedIn rdf:resource="http://xworks.gr/ontologies/ccso#BSc_Computer_Science/CS_BSc/CSD/SSE/UoC"/>
        <offeredBy rdf:resource="http://xworks.gr/ontologies/ccso#Computers_Sciences_Department_of_University_of_Crete"/>
        <code rdf:datatype="http://www.w3.org/2001/XMLSchema#string">CS120/CS_BSc/CSD/SSE/UoC</code>
        <courseType rdf:datatype="http://www.w3.org/2001/XMLSchema#string">Core</courseType>
        <csName rdf:datatype="http://www.w3.org/2001/XMLSchema#string">Digital Design</csName>
    </owl:NamedIndividual>
    


    <!-- http://xworks.gr/ontologies/ccso#CS120s1/CS_BSc/CSD/SSE/UoC -->

    <owl:NamedIndividual rdf:about="http://xworks.gr/ontologies/ccso#CS120s1/CS_BSc/CSD/SSE/UoC">
        <rdf:type rdf:resource="http://xworks.gr/ontologies/ccso#Syllabus"/>
        <affiliatedWith rdf:resource="http://xworks.gr/ontologies/ccso#Katevenis_Manolis"/>
        <affiliatedWith rdf:resource="http://xworks.gr/ontologies/ccso#Pappa_Pepi"/>
        <hasCourseAssistant rdf:resource="http://xworks.gr/ontologies/ccso#Pappa_Pepi"/>
        <hasInstructor rdf:resource="http://xworks.gr/ontologies/ccso#Katevenis_Manolis"/>
        <hasSupervisor rdf:resource="http://xworks.gr/ontologies/ccso#Katevenis_Manolis"/>
        <syllabusOf rdf:resource="http://xworks.gr/ontologies/ccso#CS120/CS_BSc/CSD/SSE/UoC"/>
        <code rdf:datatype="http://www.w3.org/2001/XMLSchema#string">CS120s1/CS_BSc/CSD/SSE/UoC</code>
        <courseType rdf:datatype="http://www.w3.org/2001/XMLSchema#string">Core</courseType>
        <creditsECTS rdf:datatype="http://www.w3.org/2001/XMLSchema#short">8</creditsECTS>
        <csName rdf:datatype="http://www.w3.org/2001/XMLSchema#string">Syllabus of course CS120 Digital Design</csName>
        <semesterinProgram rdf:datatype="http://www.w3.org/2001/XMLSchema#short">2</semesterinProgram>
    </owl:NamedIndividual>
    


    <!-- http://xworks.gr/ontologies/ccso#CS150/CS_BSc/CSD/SSE/UoC -->

    <owl:NamedIndividual rdf:about="http://xworks.gr/ontologies/ccso#CS150/CS_BSc/CSD/SSE/UoC">
        <rdf:type rdf:resource="http://xworks.gr/ontologies/ccso#Course"/>
        <affiliatedWith rdf:resource="http://xworks.gr/ontologies/ccso#Starkeiou_Nick"/>
        <coversKA rdf:resource="http://xworks.gr/ontologies/ccso#CS/PL_Programming_Languages"/>
        <hasAttender rdf:resource="http://xworks.gr/ontologies/ccso#Starkeiou_Nick"/>
        <hasSyllabus rdf:resource="http://xworks.gr/ontologies/ccso#CS150s1/CS_BSc/CSD/SSE/UoC"/>
        <includedIn rdf:resource="http://xworks.gr/ontologies/ccso#BSc_Computer_Science/CS_BSc/CSD/SSE/UoC"/>
        <offeredBy rdf:resource="http://xworks.gr/ontologies/ccso#Computers_Sciences_Department_of_University_of_Crete"/>
        <code rdf:datatype="http://www.w3.org/2001/XMLSchema#string">CS150/CS_BSc/CSD/SSE/UoC</code>
        <courseType rdf:datatype="http://www.w3.org/2001/XMLSchema#string">Core</courseType>
        <csName rdf:datatype="http://www.w3.org/2001/XMLSchema#string">Programming</csName>
    </owl:NamedIndividual>
    


    <!-- http://xworks.gr/ontologies/ccso#CS150s1/CS_BSc/CSD/SSE/UoC -->

    <owl:NamedIndividual rdf:about="http://xworks.gr/ontologies/ccso#CS150s1/CS_BSc/CSD/SSE/UoC">
        <rdf:type rdf:resource="http://xworks.gr/ontologies/ccso#Syllabus"/>
        <affiliatedWith rdf:resource="http://xworks.gr/ontologies/ccso#Gramma_Joanna"/>
        <affiliatedWith rdf:resource="http://xworks.gr/ontologies/ccso#Kalogiannakis_Michail"/>
        <affiliatedWith rdf:resource="http://xworks.gr/ontologies/ccso#Kondylakis_Haridimos"/>
        <affiliatedWith rdf:resource="http://xworks.gr/ontologies/ccso#Pappa_Pepi"/>
        <aimsToLO rdf:resource="http://xworks.gr/ontologies/ccso#CS/PL/LO_Correctly_reason_about_control_flow_in_a_program_using_dynamic_dispatch"/>
        <aimsToLO rdf:resource="http://xworks.gr/ontologies/ccso#CS/PL/LO_Use_subclassing_to_design_simple_class_hierarchies_that_allow_code_to_be_reused_for_distinct_subclasses"/>
        <aimsToLO rdf:resource="http://xworks.gr/ontologies/ccso#CS/PL/LO_Compare_and_contrast_the_procedural/functional_approach_and_the_object-oriented_approach"/>
        <coversTopic rdf:resource="http://xworks.gr/ontologies/ccso#CS/PL/T_Definition_of_classes:fields,methods,and_constructors"/>
        <coversTopic rdf:resource="http://xworks.gr/ontologies/ccso#CS/PL/T_Dynamic_dispatch:Definition_of_Method-Call"/>
        <coversTopic rdf:resource="http://xworks.gr/ontologies/ccso#CS/PL/T_Object-Oriented_Design,Class-Hierarchy_design_for_modeling"/>
        <coversTopic rdf:resource="http://xworks.gr/ontologies/ccso#CS/PL/T_Object-Oriented_Design,_Decomposition_into_objects_carrying_state_and_having_behavior"/>
        <coversTopic rdf:resource="http://xworks.gr/ontologies/ccso#CS/PL/T_Subclasses,Inheritance,and_Method_Overriding"/>
        <hasCourseAssistant rdf:resource="http://xworks.gr/ontologies/ccso#Gramma_Joanna"/>
        <hasCourseAssistant rdf:resource="http://xworks.gr/ontologies/ccso#Kondylakis_Haridimos"/>
        <hasCourseAssistant rdf:resource="http://xworks.gr/ontologies/ccso#Pappa_Pepi"/>
        <hasInstructor rdf:resource="http://xworks.gr/ontologies/ccso#Kalogiannakis_Michail"/>
        <syllabusOf rdf:resource="http://xworks.gr/ontologies/ccso#CS150/CS_BSc/CSD/SSE/UoC"/>
        <code rdf:datatype="http://www.w3.org/2001/XMLSchema#string">CS150s1/CS_BSc/CSD/SSE/UoC</code>
        <courseType rdf:datatype="http://www.w3.org/2001/XMLSchema#string">Core</courseType>
        <creditsECTS rdf:datatype="http://www.w3.org/2001/XMLSchema#short">8</creditsECTS>
        <csName rdf:datatype="http://www.w3.org/2001/XMLSchema#string">Syllabus of course CS150 Programming</csName>
        <semesterinProgram rdf:datatype="http://www.w3.org/2001/XMLSchema#short">2</semesterinProgram>
    </owl:NamedIndividual>
    


    <!-- http://xworks.gr/ontologies/ccso#CS180/CS_BSc/CSD/SSE/UoC -->

    <owl:NamedIndividual rdf:about="http://xworks.gr/ontologies/ccso#CS180/CS_BSc/CSD/SSE/UoC">
        <rdf:type rdf:resource="http://xworks.gr/ontologies/ccso#Course"/>
        <affiliatedWith rdf:resource="http://xworks.gr/ontologies/ccso#Starkeiou_Vakis"/>
        <hasAttender rdf:resource="http://xworks.gr/ontologies/ccso#Starkeiou_Vakis"/>
        <hasSyllabus rdf:resource="http://xworks.gr/ontologies/ccso#CS180s1/CS_BSc/CSD/SSE/UoC"/>
        <includedIn rdf:resource="http://xworks.gr/ontologies/ccso#BSc_Computer_Science/CS_BSc/CSD/SSE/UoC"/>
        <offeredBy rdf:resource="http://xworks.gr/ontologies/ccso#Computers_Sciences_Department_of_University_of_Crete"/>
        <courseType rdf:datatype="http://www.w3.org/2001/XMLSchema#string">Core</courseType>
        <csName rdf:datatype="http://www.w3.org/2001/XMLSchema#string">Logic</csName>
    </owl:NamedIndividual>
    


    <!-- http://xworks.gr/ontologies/ccso#CS180s1/CS_BSc/CSD/SSE/UoC -->

    <owl:NamedIndividual rdf:about="http://xworks.gr/ontologies/ccso#CS180s1/CS_BSc/CSD/SSE/UoC">
        <rdf:type rdf:resource="http://xworks.gr/ontologies/ccso#Syllabus"/>
        <affiliatedWith rdf:resource="http://xworks.gr/ontologies/ccso#Gramma_Joanna"/>
        <affiliatedWith rdf:resource="http://xworks.gr/ontologies/ccso#Plexousakis_Dimitris"/>
        <hasCourseAssistant rdf:resource="http://xworks.gr/ontologies/ccso#Gramma_Joanna"/>
        <hasInstructor rdf:resource="http://xworks.gr/ontologies/ccso#Plexousakis_Dimitris"/>
        <hasSupervisor rdf:resource="http://xworks.gr/ontologies/ccso#Plexousakis_Dimitris"/>
        <syllabusOf rdf:resource="http://xworks.gr/ontologies/ccso#CS180/CS_BSc/CSD/SSE/UoC"/>
        <courseType rdf:datatype="http://www.w3.org/2001/XMLSchema#string">Core</courseType>
        <creditsECTS rdf:datatype="http://www.w3.org/2001/XMLSchema#short">6</creditsECTS>
        <csName rdf:datatype="http://www.w3.org/2001/XMLSchema#string">Syllabus of course CS180 Logic</csName>
        <semesterinProgram rdf:datatype="http://www.w3.org/2001/XMLSchema#short">1</semesterinProgram>
    </owl:NamedIndividual>
    


    <!-- http://xworks.gr/ontologies/ccso#CS208/CS_BSc/CSD/SSE/UoC -->

    <owl:NamedIndividual rdf:about="http://xworks.gr/ontologies/ccso#CS208/CS_BSc/CSD/SSE/UoC">
        <rdf:type rdf:resource="http://xworks.gr/ontologies/ccso#Course"/>
        <hasPrerequisite rdf:resource="http://xworks.gr/ontologies/ccso#CS109/CS_BSc/CSD/SSE/UoC"/>
        <hasSyllabus rdf:resource="http://xworks.gr/ontologies/ccso#CS208s1/CS_BSc/CSD/SSE/UoC"/>
        <includedIn rdf:resource="http://xworks.gr/ontologies/ccso#BSc_Computer_Science/CS_BSc/CSD/SSE/UoC"/>
        <offeredBy rdf:resource="http://xworks.gr/ontologies/ccso#Computers_Sciences_Department_of_University_of_Crete"/>
        <courseType rdf:datatype="http://www.w3.org/2001/XMLSchema#string">Core</courseType>
        <csName rdf:datatype="http://www.w3.org/2001/XMLSchema#string">English III</csName>
    </owl:NamedIndividual>
    


    <!-- http://xworks.gr/ontologies/ccso#CS208s1/CS_BSc/CSD/SSE/UoC -->

    <owl:NamedIndividual rdf:about="http://xworks.gr/ontologies/ccso#CS208s1/CS_BSc/CSD/SSE/UoC">
        <rdf:type rdf:resource="http://xworks.gr/ontologies/ccso#Syllabus"/>
        <affiliatedWith rdf:resource="http://xworks.gr/ontologies/ccso#Pasta_Flora"/>
        <affiliatedWith rdf:resource="http://xworks.gr/ontologies/ccso#Rizopoulou_Noni"/>
        <hasCourseAssistant rdf:resource="http://xworks.gr/ontologies/ccso#Pasta_Flora"/>
        <hasInstructor rdf:resource="http://xworks.gr/ontologies/ccso#Rizopoulou_Noni"/>
        <hasSupervisor rdf:resource="http://xworks.gr/ontologies/ccso#Rizopoulou_Noni"/>
        <syllabusOf rdf:resource="http://xworks.gr/ontologies/ccso#CS208/CS_BSc/CSD/SSE/UoC"/>
        <courseType rdf:datatype="http://www.w3.org/2001/XMLSchema#string">Core</courseType>
        <creditsECTS rdf:datatype="http://www.w3.org/2001/XMLSchema#short">4</creditsECTS>
        <csName rdf:datatype="http://www.w3.org/2001/XMLSchema#string">Syllabus of course CS208 English III</csName>
        <semesterinProgram rdf:datatype="http://www.w3.org/2001/XMLSchema#short">3</semesterinProgram>
    </owl:NamedIndividual>
    


    <!-- http://xworks.gr/ontologies/ccso#CS209/CS_BSc/CSD/SSE/UoC -->

    <owl:NamedIndividual rdf:about="http://xworks.gr/ontologies/ccso#CS209/CS_BSc/CSD/SSE/UoC">
        <rdf:type rdf:resource="http://xworks.gr/ontologies/ccso#Course"/>
        <hasPrerequisite rdf:resource="http://xworks.gr/ontologies/ccso#CS208/CS_BSc/CSD/SSE/UoC"/>
        <hasSyllabus rdf:resource="http://xworks.gr/ontologies/ccso#CS209s1/CS_BSc/CSD/SSE/UoC"/>
        <includedIn rdf:resource="http://xworks.gr/ontologies/ccso#BSc_Computer_Science/CS_BSc/CSD/SSE/UoC"/>
        <offeredBy rdf:resource="http://xworks.gr/ontologies/ccso#Computers_Sciences_Department_of_University_of_Crete"/>
        <courseType rdf:datatype="http://www.w3.org/2001/XMLSchema#string">Core</courseType>
        <csName rdf:datatype="http://www.w3.org/2001/XMLSchema#string">English IV</csName>
    </owl:NamedIndividual>
    


    <!-- http://xworks.gr/ontologies/ccso#CS209s1/CS_BSc/CSD/SSE/UoC -->

    <owl:NamedIndividual rdf:about="http://xworks.gr/ontologies/ccso#CS209s1/CS_BSc/CSD/SSE/UoC">
        <rdf:type rdf:resource="http://xworks.gr/ontologies/ccso#Syllabus"/>
        <affiliatedWith rdf:resource="http://xworks.gr/ontologies/ccso#Rizopoulou_Noni"/>
        <hasInstructor rdf:resource="http://xworks.gr/ontologies/ccso#Rizopoulou_Noni"/>
        <hasSupervisor rdf:resource="http://xworks.gr/ontologies/ccso#Rizopoulou_Noni"/>
        <syllabusOf rdf:resource="http://xworks.gr/ontologies/ccso#CS209/CS_BSc/CSD/SSE/UoC"/>
        <courseType rdf:datatype="http://www.w3.org/2001/XMLSchema#string">Core</courseType>
        <creditsECTS rdf:datatype="http://www.w3.org/2001/XMLSchema#short">4</creditsECTS>
        <csName rdf:datatype="http://www.w3.org/2001/XMLSchema#string">Syllabus of course CS209 English IV</csName>
        <semesterinProgram rdf:datatype="http://www.w3.org/2001/XMLSchema#short">4</semesterinProgram>
    </owl:NamedIndividual>
    


    <!-- http://xworks.gr/ontologies/ccso#CS215/CS_BSc/CSD/SSE/UoC -->

    <owl:NamedIndividual rdf:about="http://xworks.gr/ontologies/ccso#CS215/CS_BSc/CSD/SSE/UoC">
        <rdf:type rdf:resource="http://xworks.gr/ontologies/ccso#Course"/>
        <hasPrerequisite rdf:resource="http://xworks.gr/ontologies/ccso#CS110/CS_BSc/CSD/SSE/UoC"/>
        <hasSyllabus rdf:resource="http://xworks.gr/ontologies/ccso#CS215s1/CS_BSc/CSD/SSE/UoC"/>
        <includedIn rdf:resource="http://xworks.gr/ontologies/ccso#BSc_Computer_Science/CS_BSc/CSD/SSE/UoC"/>
        <offeredBy rdf:resource="http://xworks.gr/ontologies/ccso#Computers_Sciences_Department_of_University_of_Crete"/>
        <courseType rdf:datatype="http://www.w3.org/2001/XMLSchema#string">Core</courseType>
        <csName rdf:datatype="http://www.w3.org/2001/XMLSchema#string">Applied Mathematics for Engineers</csName>
    </owl:NamedIndividual>
    


    <!-- http://xworks.gr/ontologies/ccso#CS215s1/CS_BSc/CSD/SSE/UoC -->

    <owl:NamedIndividual rdf:about="http://xworks.gr/ontologies/ccso#CS215s1/CS_BSc/CSD/SSE/UoC">
        <rdf:type rdf:resource="http://xworks.gr/ontologies/ccso#Syllabus"/>
        <affiliatedWith rdf:resource="http://xworks.gr/ontologies/ccso#Gramma_Joanna"/>
        <affiliatedWith rdf:resource="http://xworks.gr/ontologies/ccso#Tsakalidis_Panayiotis"/>
        <hasCourseAssistant rdf:resource="http://xworks.gr/ontologies/ccso#Gramma_Joanna"/>
        <hasInstructor rdf:resource="http://xworks.gr/ontologies/ccso#Tsakalidis_Panayiotis"/>
        <hasSupervisor rdf:resource="http://xworks.gr/ontologies/ccso#Tsakalidis_Panayiotis"/>
        <syllabusOf rdf:resource="http://xworks.gr/ontologies/ccso#CS215/CS_BSc/CSD/SSE/UoC"/>
        <courseType rdf:datatype="http://www.w3.org/2001/XMLSchema#string">Core</courseType>
        <creditsECTS rdf:datatype="http://www.w3.org/2001/XMLSchema#short">8</creditsECTS>
        <csName rdf:datatype="http://www.w3.org/2001/XMLSchema#string">Syllabus of course CS215 Applied Mathematics for Engineers</csName>
        <semesterinProgram rdf:datatype="http://www.w3.org/2001/XMLSchema#short">3</semesterinProgram>
    </owl:NamedIndividual>
    


    <!-- http://xworks.gr/ontologies/ccso#CS217/CS_BSc/CSD/SSE/UoC -->

    <owl:NamedIndividual rdf:about="http://xworks.gr/ontologies/ccso#CS217/CS_BSc/CSD/SSE/UoC">
        <rdf:type rdf:resource="http://xworks.gr/ontologies/ccso#Course"/>
        <hasPrerequisite rdf:resource="http://xworks.gr/ontologies/ccso#CS110/CS_BSc/CSD/SSE/UoC"/>
        <hasSyllabus rdf:resource="http://xworks.gr/ontologies/ccso#CS217s1/CS_BSc/CSD/SSE/UoC"/>
        <includedIn rdf:resource="http://xworks.gr/ontologies/ccso#BSc_Computer_Science/CS_BSc/CSD/SSE/UoC"/>
        <offeredBy rdf:resource="http://xworks.gr/ontologies/ccso#Computers_Sciences_Department_of_University_of_Crete"/>
        <courseType rdf:datatype="http://www.w3.org/2001/XMLSchema#string">Core</courseType>
        <csName rdf:datatype="http://www.w3.org/2001/XMLSchema#string">Probability</csName>
    </owl:NamedIndividual>
    


    <!-- http://xworks.gr/ontologies/ccso#CS217s1/CS_BSc/CSD/SSE/UoC -->

    <owl:NamedIndividual rdf:about="http://xworks.gr/ontologies/ccso#CS217s1/CS_BSc/CSD/SSE/UoC">
        <rdf:type rdf:resource="http://xworks.gr/ontologies/ccso#Syllabus"/>
        <affiliatedWith rdf:resource="http://xworks.gr/ontologies/ccso#Tsakalidis_Panayiotis"/>
        <hasInstructor rdf:resource="http://xworks.gr/ontologies/ccso#Tsakalidis_Panayiotis"/>
        <hasSupervisor rdf:resource="http://xworks.gr/ontologies/ccso#Tsakalidis_Panayiotis"/>
        <syllabusOf rdf:resource="http://xworks.gr/ontologies/ccso#CS217/CS_BSc/CSD/SSE/UoC"/>
        <courseType rdf:datatype="http://www.w3.org/2001/XMLSchema#string">Core</courseType>
        <creditsECTS rdf:datatype="http://www.w3.org/2001/XMLSchema#short">6</creditsECTS>
        <csName rdf:datatype="http://www.w3.org/2001/XMLSchema#string">Syllabus of course CS217 Probability</csName>
        <semesterinProgram rdf:datatype="http://www.w3.org/2001/XMLSchema#short">4</semesterinProgram>
    </owl:NamedIndividual>
    


    <!-- http://xworks.gr/ontologies/ccso#CS220/CS_BSc/CSD/SSE/UoC -->

    <owl:NamedIndividual rdf:about="http://xworks.gr/ontologies/ccso#CS220/CS_BSc/CSD/SSE/UoC">
        <rdf:type rdf:resource="http://xworks.gr/ontologies/ccso#Course"/>
        <coversKA rdf:resource="http://xworks.gr/ontologies/ccso#CS/HW_Hardware_and_Computer_Systems"/>
        <hasPrerequisite rdf:resource="http://xworks.gr/ontologies/ccso#CS120/CS_BSc/CSD/SSE/UoC"/>
        <hasSyllabus rdf:resource="http://xworks.gr/ontologies/ccso#CS220s1/CS_BSc/CSD/SSE/UoC"/>
        <includedIn rdf:resource="http://xworks.gr/ontologies/ccso#BSc_Computer_Science/CS_BSc/CSD/SSE/UoC"/>
        <offeredBy rdf:resource="http://xworks.gr/ontologies/ccso#Computers_Sciences_Department_of_University_of_Crete"/>
        <courseType rdf:datatype="http://www.w3.org/2001/XMLSchema#string">Elective</courseType>
        <csName rdf:datatype="http://www.w3.org/2001/XMLSchema#string">Digital Circuits Lab</csName>
    </owl:NamedIndividual>
    


    <!-- http://xworks.gr/ontologies/ccso#CS220s1/CS_BSc/CSD/SSE/UoC -->

    <owl:NamedIndividual rdf:about="http://xworks.gr/ontologies/ccso#CS220s1/CS_BSc/CSD/SSE/UoC">
        <rdf:type rdf:resource="http://xworks.gr/ontologies/ccso#Syllabus"/>
        <syllabusOf rdf:resource="http://xworks.gr/ontologies/ccso#CS220/CS_BSc/CSD/SSE/UoC"/>
        <courseType rdf:datatype="http://www.w3.org/2001/XMLSchema#string">Elective</courseType>
        <creditsECTS rdf:datatype="http://www.w3.org/2001/XMLSchema#short">6</creditsECTS>
        <csName rdf:datatype="http://www.w3.org/2001/XMLSchema#string">Syllabus of course CS220 Digital Circuits Lab</csName>
        <semesterinProgram rdf:datatype="http://www.w3.org/2001/XMLSchema#short">3</semesterinProgram>
    </owl:NamedIndividual>
    


    <!-- http://xworks.gr/ontologies/ccso#CS225/CS_BSc/CSD/SSE/UoC -->

    <owl:NamedIndividual rdf:about="http://xworks.gr/ontologies/ccso#CS225/CS_BSc/CSD/SSE/UoC">
        <rdf:type rdf:resource="http://xworks.gr/ontologies/ccso#Course"/>
        <hasPrerequisite rdf:resource="http://xworks.gr/ontologies/ccso#CS120/CS_BSc/CSD/SSE/UoC"/>
        <hasSyllabus rdf:resource="http://xworks.gr/ontologies/ccso#CS225s1/CS_BSc/CSD/SSE/UoC"/>
        <includedIn rdf:resource="http://xworks.gr/ontologies/ccso#BSc_Computer_Science/CS_BSc/CSD/SSE/UoC"/>
        <offeredBy rdf:resource="http://xworks.gr/ontologies/ccso#Computers_Sciences_Department_of_University_of_Crete"/>
        <courseType rdf:datatype="http://www.w3.org/2001/XMLSchema#string">Core</courseType>
        <csName rdf:datatype="http://www.w3.org/2001/XMLSchema#string">Computer Organization</csName>
    </owl:NamedIndividual>
    


    <!-- http://xworks.gr/ontologies/ccso#CS225s1/CS_BSc/CSD/SSE/UoC -->

    <owl:NamedIndividual rdf:about="http://xworks.gr/ontologies/ccso#CS225s1/CS_BSc/CSD/SSE/UoC">
        <rdf:type rdf:resource="http://xworks.gr/ontologies/ccso#Syllabus"/>
        <affiliatedWith rdf:resource="http://xworks.gr/ontologies/ccso#Gramma_Joanna"/>
        <affiliatedWith rdf:resource="http://xworks.gr/ontologies/ccso#Katevenis_Manolis"/>
        <hasCourseAssistant rdf:resource="http://xworks.gr/ontologies/ccso#Gramma_Joanna"/>
        <hasInstructor rdf:resource="http://xworks.gr/ontologies/ccso#Katevenis_Manolis"/>
        <hasSupervisor rdf:resource="http://xworks.gr/ontologies/ccso#Katevenis_Manolis"/>
        <syllabusOf rdf:resource="http://xworks.gr/ontologies/ccso#CS225/CS_BSc/CSD/SSE/UoC"/>
        <courseType rdf:datatype="http://www.w3.org/2001/XMLSchema#string">Core</courseType>
        <creditsECTS rdf:datatype="http://www.w3.org/2001/XMLSchema#short">8</creditsECTS>
        <csName rdf:datatype="http://www.w3.org/2001/XMLSchema#string">Syllabus of course CS225 Computer Organization</csName>
        <semesterinProgram rdf:datatype="http://www.w3.org/2001/XMLSchema#short">3</semesterinProgram>
    </owl:NamedIndividual>
    


    <!-- http://xworks.gr/ontologies/ccso#CS240/CS_BSc/CSD/SSE/UoC -->

    <owl:NamedIndividual rdf:about="http://xworks.gr/ontologies/ccso#CS240/CS_BSc/CSD/SSE/UoC">
        <rdf:type rdf:resource="http://xworks.gr/ontologies/ccso#Course"/>
        <coversKA rdf:resource="http://xworks.gr/ontologies/ccso#CS/PL_Programming_Languages"/>
        <hasPrerequisite rdf:resource="http://xworks.gr/ontologies/ccso#CS100/CS_BSc/CSD/SSE/UoC"/>
        <hasPrerequisite rdf:resource="http://xworks.gr/ontologies/ccso#CS150/CS_BSc/CSD/SSE/UoC"/>
        <hasSyllabus rdf:resource="http://xworks.gr/ontologies/ccso#CS240s1/CS_BSc/CSD/SSE/UoC"/>
        <includedIn rdf:resource="http://xworks.gr/ontologies/ccso#BSc_Computer_Science/CS_BSc/CSD/SSE/UoC"/>
        <offeredBy rdf:resource="http://xworks.gr/ontologies/ccso#Computers_Sciences_Department_of_University_of_Crete"/>
        <courseType rdf:datatype="http://www.w3.org/2001/XMLSchema#string">Core</courseType>
        <csName rdf:datatype="http://www.w3.org/2001/XMLSchema#string">Data Structures</csName>
    </owl:NamedIndividual>
    


    <!-- http://xworks.gr/ontologies/ccso#CS240s1/CS_BSc/CSD/SSE/UoC -->

    <owl:NamedIndividual rdf:about="http://xworks.gr/ontologies/ccso#CS240s1/CS_BSc/CSD/SSE/UoC">
        <rdf:type rdf:resource="http://xworks.gr/ontologies/ccso#Syllabus"/>
        <affiliatedWith rdf:resource="http://xworks.gr/ontologies/ccso#Faturou_Panagiota"/>
        <hasInstructor rdf:resource="http://xworks.gr/ontologies/ccso#Faturou_Panagiota"/>
        <hasSupervisor rdf:resource="http://xworks.gr/ontologies/ccso#Faturou_Panagiota"/>
        <syllabusOf rdf:resource="http://xworks.gr/ontologies/ccso#CS240/CS_BSc/CSD/SSE/UoC"/>
        <courseType rdf:datatype="http://www.w3.org/2001/XMLSchema#string">Core</courseType>
        <creditsECTS rdf:datatype="http://www.w3.org/2001/XMLSchema#short">8</creditsECTS>
        <csName rdf:datatype="http://www.w3.org/2001/XMLSchema#string">Syllabus of course CS240 Data Structures</csName>
        <semesterinProgram rdf:datatype="http://www.w3.org/2001/XMLSchema#short">4</semesterinProgram>
    </owl:NamedIndividual>
    


    <!-- http://xworks.gr/ontologies/ccso#CS252/CS_BSc/CSD/SSE/UoC -->

    <owl:NamedIndividual rdf:about="http://xworks.gr/ontologies/ccso#CS252/CS_BSc/CSD/SSE/UoC">
        <rdf:type rdf:resource="http://xworks.gr/ontologies/ccso#Course"/>
        <coversKA rdf:resource="http://xworks.gr/ontologies/ccso#CS/PL_Programming_Languages"/>
        <hasPrerequisite rdf:resource="http://xworks.gr/ontologies/ccso#CS150/CS_BSc/CSD/SSE/UoC"/>
        <hasSyllabus rdf:resource="http://xworks.gr/ontologies/ccso#CS252s1/CS_BSc/CSD/SSE/UoC"/>
        <includedIn rdf:resource="http://xworks.gr/ontologies/ccso#BSc_Computer_Science/CS_BSc/CSD/SSE/UoC"/>
        <offeredBy rdf:resource="http://xworks.gr/ontologies/ccso#Computers_Sciences_Department_of_University_of_Crete"/>
        <courseType rdf:datatype="http://www.w3.org/2001/XMLSchema#string">Core</courseType>
        <csName rdf:datatype="http://www.w3.org/2001/XMLSchema#string">Object-Oriented Programming</csName>
    </owl:NamedIndividual>
    


    <!-- http://xworks.gr/ontologies/ccso#CS252s1/CS_BSc/CSD/SSE/UoC -->

    <owl:NamedIndividual rdf:about="http://xworks.gr/ontologies/ccso#CS252s1/CS_BSc/CSD/SSE/UoC">
        <rdf:type rdf:resource="http://xworks.gr/ontologies/ccso#Syllabus"/>
        <affiliatedWith rdf:resource="http://xworks.gr/ontologies/ccso#Christofides_Vassilis"/>
        <affiliatedWith rdf:resource="http://xworks.gr/ontologies/ccso#Gramma_Joanna"/>
        <aimsToLO rdf:resource="http://xworks.gr/ontologies/ccso#CS/PL/LO_Correctly_reason_about_control_flow_in_a_program_using_dynamic_dispatch"/>
        <aimsToLO rdf:resource="http://xworks.gr/ontologies/ccso#CS/PL/LO_Compare_and_contrast_the_procedural/functional_approach_and_the_object-oriented_approach"/>
        <coversTopic rdf:resource="http://xworks.gr/ontologies/ccso#CS/PL/T_Object-Oriented_Design,Class-Hierarchy_design_for_modeling"/>
        <coversTopic rdf:resource="http://xworks.gr/ontologies/ccso#CS/PL/T_Object-Oriented_Design,_Decomposition_into_objects_carrying_state_and_having_behavior"/>
        <coversTopic rdf:resource="http://xworks.gr/ontologies/ccso#CS/PL/T_Subclasses,Inheritance,and_Method_Overriding"/>
        <hasCourseAssistant rdf:resource="http://xworks.gr/ontologies/ccso#Gramma_Joanna"/>
        <hasInstructor rdf:resource="http://xworks.gr/ontologies/ccso#Christofides_Vassilis"/>
        <hasSupervisor rdf:resource="http://xworks.gr/ontologies/ccso#Christofides_Vassilis"/>
        <syllabusOf rdf:resource="http://xworks.gr/ontologies/ccso#CS252/CS_BSc/CSD/SSE/UoC"/>
        <courseType rdf:datatype="http://www.w3.org/2001/XMLSchema#string">Core</courseType>
        <creditsECTS rdf:datatype="http://www.w3.org/2001/XMLSchema#short">8</creditsECTS>
        <csName rdf:datatype="http://www.w3.org/2001/XMLSchema#string">Syllabus of course CS252 Object-Oriented Programming</csName>
        <semesterinProgram rdf:datatype="http://www.w3.org/2001/XMLSchema#short">4</semesterinProgram>
    </owl:NamedIndividual>
    


    <!-- http://xworks.gr/ontologies/ccso#CS255/CS_BSc/CSD/SSE/UoC -->

    <owl:NamedIndividual rdf:about="http://xworks.gr/ontologies/ccso#CS255/CS_BSc/CSD/SSE/UoC">
        <rdf:type rdf:resource="http://xworks.gr/ontologies/ccso#Course"/>
        <hasSyllabus rdf:resource="http://xworks.gr/ontologies/ccso#CS255s1/CS_BSc/CSD/SSE/UoC"/>
        <includedIn rdf:resource="http://xworks.gr/ontologies/ccso#BSc_Computer_Science/CS_BSc/CSD/SSE/UoC"/>
        <offeredBy rdf:resource="http://xworks.gr/ontologies/ccso#Computers_Sciences_Department_of_University_of_Crete"/>
        <courseType rdf:datatype="http://www.w3.org/2001/XMLSchema#string">Core</courseType>
        <csName rdf:datatype="http://www.w3.org/2001/XMLSchema#string">Software Technology Laboratory</csName>
    </owl:NamedIndividual>
    


    <!-- http://xworks.gr/ontologies/ccso#CS255s1/CS_BSc/CSD/SSE/UoC -->

    <owl:NamedIndividual rdf:about="http://xworks.gr/ontologies/ccso#CS255s1/CS_BSc/CSD/SSE/UoC">
        <rdf:type rdf:resource="http://xworks.gr/ontologies/ccso#Syllabus"/>
        <affiliatedWith rdf:resource="http://xworks.gr/ontologies/ccso#Georgakopoulos_George"/>
        <affiliatedWith rdf:resource="http://xworks.gr/ontologies/ccso#Pasta_Flora"/>
        <hasCourseAssistant rdf:resource="http://xworks.gr/ontologies/ccso#Pasta_Flora"/>
        <hasInstructor rdf:resource="http://xworks.gr/ontologies/ccso#Georgakopoulos_George"/>
        <hasSupervisor rdf:resource="http://xworks.gr/ontologies/ccso#Georgakopoulos_George"/>
        <syllabusOf rdf:resource="http://xworks.gr/ontologies/ccso#CS255/CS_BSc/CSD/SSE/UoC"/>
        <courseType rdf:datatype="http://www.w3.org/2001/XMLSchema#string">Core</courseType>
        <creditsECTS rdf:datatype="http://www.w3.org/2001/XMLSchema#short">6</creditsECTS>
        <csName rdf:datatype="http://www.w3.org/2001/XMLSchema#string">Syllabus of course CS255 Software Technology Laboratory</csName>
        <semesterinProgram rdf:datatype="http://www.w3.org/2001/XMLSchema#short">3</semesterinProgram>
    </owl:NamedIndividual>
    


    <!-- http://xworks.gr/ontologies/ccso#CS280/CS_BSc/CSD/SSE/UoC -->

    <owl:NamedIndividual rdf:about="http://xworks.gr/ontologies/ccso#CS280/CS_BSc/CSD/SSE/UoC">
        <rdf:type rdf:resource="http://xworks.gr/ontologies/ccso#Course"/>
        <hasSyllabus rdf:resource="http://xworks.gr/ontologies/ccso#CS280s1/CS_BSc/CSD/SSE/UoC"/>
        <includedIn rdf:resource="http://xworks.gr/ontologies/ccso#BSc_Computer_Science/CS_BSc/CSD/SSE/UoC"/>
        <offeredBy rdf:resource="http://xworks.gr/ontologies/ccso#Computers_Sciences_Department_of_University_of_Crete"/>
        <courseType rdf:datatype="http://www.w3.org/2001/XMLSchema#string">Core</courseType>
        <csName rdf:datatype="http://www.w3.org/2001/XMLSchema#string">Theory of Computation</csName>
    </owl:NamedIndividual>
    


    <!-- http://xworks.gr/ontologies/ccso#CS280s1/CS_BSc/CSD/SSE/UoC -->

    <owl:NamedIndividual rdf:about="http://xworks.gr/ontologies/ccso#CS280s1/CS_BSc/CSD/SSE/UoC">
        <rdf:type rdf:resource="http://xworks.gr/ontologies/ccso#Syllabus"/>
        <affiliatedWith rdf:resource="http://xworks.gr/ontologies/ccso#Papadopouli_Maria"/>
        <hasInstructor rdf:resource="http://xworks.gr/ontologies/ccso#Papadopouli_Maria"/>
        <hasSupervisor rdf:resource="http://xworks.gr/ontologies/ccso#Papadopouli_Maria"/>
        <syllabusOf rdf:resource="http://xworks.gr/ontologies/ccso#CS280/CS_BSc/CSD/SSE/UoC"/>
        <courseType rdf:datatype="http://www.w3.org/2001/XMLSchema#string">Core</courseType>
        <creditsECTS rdf:datatype="http://www.w3.org/2001/XMLSchema#short">6</creditsECTS>
        <csName rdf:datatype="http://www.w3.org/2001/XMLSchema#string">Syllabus of course CS280 Theory of Computation</csName>
        <semesterinProgram rdf:datatype="http://www.w3.org/2001/XMLSchema#short">3</semesterinProgram>
    </owl:NamedIndividual>
    


    <!-- http://xworks.gr/ontologies/ccso#CS302/CS_BSc/CSD/SSE/UoC -->

    <owl:NamedIndividual rdf:about="http://xworks.gr/ontologies/ccso#CS302/CS_BSc/CSD/SSE/UoC">
        <rdf:type rdf:resource="http://xworks.gr/ontologies/ccso#Course"/>
        <hasPrerequisite rdf:resource="http://xworks.gr/ontologies/ccso#CS100/CS_BSc/CSD/SSE/UoC"/>
        <hasPrerequisite rdf:resource="http://xworks.gr/ontologies/ccso#CS120/CS_BSc/CSD/SSE/UoC"/>
        <hasPrerequisite rdf:resource="http://xworks.gr/ontologies/ccso#CS150/CS_BSc/CSD/SSE/UoC"/>
        <hasSyllabus rdf:resource="http://xworks.gr/ontologies/ccso#CS302s1/CS_BSc/CSD/SSE/UoC"/>
        <includedIn rdf:resource="http://xworks.gr/ontologies/ccso#BSc_Computer_Science/CS_BSc/CSD/SSE/UoC"/>
        <offeredBy rdf:resource="http://xworks.gr/ontologies/ccso#Computers_Sciences_Department_of_University_of_Crete"/>
        <courseType rdf:datatype="http://www.w3.org/2001/XMLSchema#string">Elective</courseType>
        <csName rdf:datatype="http://www.w3.org/2001/XMLSchema#string">Teaching of Computer Science</csName>
    </owl:NamedIndividual>
    


    <!-- http://xworks.gr/ontologies/ccso#CS302s1/CS_BSc/CSD/SSE/UoC -->

    <owl:NamedIndividual rdf:about="http://xworks.gr/ontologies/ccso#CS302s1/CS_BSc/CSD/SSE/UoC">
        <rdf:type rdf:resource="http://xworks.gr/ontologies/ccso#Syllabus"/>
        <syllabusOf rdf:resource="http://xworks.gr/ontologies/ccso#CS302/CS_BSc/CSD/SSE/UoC"/>
        <courseType rdf:datatype="http://www.w3.org/2001/XMLSchema#string">Elective</courseType>
        <creditsECTS rdf:datatype="http://www.w3.org/2001/XMLSchema#short">6</creditsECTS>
        <csName rdf:datatype="http://www.w3.org/2001/XMLSchema#string">Syllabus of course CS302 Teaching of Computer Science</csName>
        <semesterinProgram rdf:datatype="http://www.w3.org/2001/XMLSchema#short">3</semesterinProgram>
    </owl:NamedIndividual>
    


    <!-- http://xworks.gr/ontologies/ccso#CS317/CS_BSc/CSD/SSE/UoC -->

    <owl:NamedIndividual rdf:about="http://xworks.gr/ontologies/ccso#CS317/CS_BSc/CSD/SSE/UoC">
        <rdf:type rdf:resource="http://xworks.gr/ontologies/ccso#Course"/>
        <coversKA rdf:resource="http://xworks.gr/ontologies/ccso#CS/PL_Programming_Languages"/>
        <hasPrerequisite rdf:resource="http://xworks.gr/ontologies/ccso#CS217/CS_BSc/CSD/SSE/UoC"/>
        <hasSyllabus rdf:resource="http://xworks.gr/ontologies/ccso#CS317s1/CS_BSc/CSD/SSE/UoC"/>
        <includedIn rdf:resource="http://xworks.gr/ontologies/ccso#BSc_Computer_Science/CS_BSc/CSD/SSE/UoC"/>
        <offeredBy rdf:resource="http://xworks.gr/ontologies/ccso#Computers_Sciences_Department_of_University_of_Crete"/>
        <courseType rdf:datatype="http://www.w3.org/2001/XMLSchema#string">Elective</courseType>
        <csName rdf:datatype="http://www.w3.org/2001/XMLSchema#string">Applied Stochastic Processes</csName>
    </owl:NamedIndividual>
    


    <!-- http://xworks.gr/ontologies/ccso#CS317s1/CS_BSc/CSD/SSE/UoC -->

    <owl:NamedIndividual rdf:about="http://xworks.gr/ontologies/ccso#CS317s1/CS_BSc/CSD/SSE/UoC">
        <rdf:type rdf:resource="http://xworks.gr/ontologies/ccso#Syllabus"/>
        <affiliatedWith rdf:resource="http://xworks.gr/ontologies/ccso#Savidis_Anthony"/>
        <hasInstructor rdf:resource="http://xworks.gr/ontologies/ccso#Savidis_Anthony"/>
        <hasSupervisor rdf:resource="http://xworks.gr/ontologies/ccso#Savidis_Anthony"/>
        <syllabusOf rdf:resource="http://xworks.gr/ontologies/ccso#CS317/CS_BSc/CSD/SSE/UoC"/>
        <courseType rdf:datatype="http://www.w3.org/2001/XMLSchema#string">Elective</courseType>
        <creditsECTS rdf:datatype="http://www.w3.org/2001/XMLSchema#short">6</creditsECTS>
        <csName rdf:datatype="http://www.w3.org/2001/XMLSchema#string">Syllabus of course CS317 Applied Stochastic Processes</csName>
        <semesterinProgram rdf:datatype="http://www.w3.org/2001/XMLSchema#short">4</semesterinProgram>
    </owl:NamedIndividual>
    


    <!-- http://xworks.gr/ontologies/ccso#CS330/CS_BSc/CSD/SSE/UoC -->

    <owl:NamedIndividual rdf:about="http://xworks.gr/ontologies/ccso#CS330/CS_BSc/CSD/SSE/UoC">
        <rdf:type rdf:resource="http://xworks.gr/ontologies/ccso#Course"/>
        <coversKA rdf:resource="http://xworks.gr/ontologies/ccso#CS/NC_Networking_and_Communication"/>
        <hasSyllabus rdf:resource="http://xworks.gr/ontologies/ccso#CS330s1/CS_BSc/CSD/SSE/UoC"/>
        <includedIn rdf:resource="http://xworks.gr/ontologies/ccso#BSc_Computer_Science/CS_BSc/CSD/SSE/UoC"/>
        <offeredBy rdf:resource="http://xworks.gr/ontologies/ccso#Computers_Sciences_Department_of_University_of_Crete"/>
        <courseType rdf:datatype="http://www.w3.org/2001/XMLSchema#string">Elective</courseType>
        <csName rdf:datatype="http://www.w3.org/2001/XMLSchema#string">Introduction to Telecommunication Theory</csName>
    </owl:NamedIndividual>
    


    <!-- http://xworks.gr/ontologies/ccso#CS330s1/CS_BSc/CSD/SSE/UoC -->

    <owl:NamedIndividual rdf:about="http://xworks.gr/ontologies/ccso#CS330s1/CS_BSc/CSD/SSE/UoC">
        <rdf:type rdf:resource="http://xworks.gr/ontologies/ccso#Syllabus"/>
        <syllabusOf rdf:resource="http://xworks.gr/ontologies/ccso#CS330/CS_BSc/CSD/SSE/UoC"/>
        <courseType rdf:datatype="http://www.w3.org/2001/XMLSchema#string">Elective</courseType>
        <creditsECTS rdf:datatype="http://www.w3.org/2001/XMLSchema#short">6</creditsECTS>
        <csName rdf:datatype="http://www.w3.org/2001/XMLSchema#string">Syllabus of course CS330 Introduction to Telecommunication Theory</csName>
        <semesterinProgram rdf:datatype="http://www.w3.org/2001/XMLSchema#short">3</semesterinProgram>
    </owl:NamedIndividual>
    


    <!-- http://xworks.gr/ontologies/ccso#CS335/CS_BSc/CSD/SSE/UoC -->

    <owl:NamedIndividual rdf:about="http://xworks.gr/ontologies/ccso#CS335/CS_BSc/CSD/SSE/UoC">
        <rdf:type rdf:resource="http://xworks.gr/ontologies/ccso#Course"/>
        <hasPrerequisite rdf:resource="http://xworks.gr/ontologies/ccso#CS118/CS_BSc/CSD/SSE/UoC"/>
        <hasSyllabus rdf:resource="http://xworks.gr/ontologies/ccso#CS335_s2015-16/CS_BSc/CSD/SSE/UoC"/>
        <hasSyllabus rdf:resource="http://xworks.gr/ontologies/ccso#CS335_s2016-17/CS_BSc/CSD/SSE/UoC"/>
        <hasSyllabus rdf:resource="http://xworks.gr/ontologies/ccso#CS335_s2017-18/CS_BSc/CSD/SSE/UoC"/>
        <includedIn rdf:resource="http://xworks.gr/ontologies/ccso#BSc_Computer_Science/CS_BSc/CSD/SSE/UoC"/>
        <offeredBy rdf:resource="http://xworks.gr/ontologies/ccso#Computers_Sciences_Department_of_University_of_Crete"/>
        <code rdf:datatype="http://www.w3.org/2001/XMLSchema#string">CS335/CS_BSc/CSD/SSE/UoC</code>
        <courseType rdf:datatype="http://www.w3.org/2001/XMLSchema#string">Core</courseType>
        <csName rdf:datatype="http://www.w3.org/2001/XMLSchema#string">Computer Networks</csName>
    </owl:NamedIndividual>
    


    <!-- http://xworks.gr/ontologies/ccso#CS335_s2015-16/CS_BSc/CSD/SSE/UoC -->

    <owl:NamedIndividual rdf:about="http://xworks.gr/ontologies/ccso#CS335_s2015-16/CS_BSc/CSD/SSE/UoC">
        <rdf:type rdf:resource="http://xworks.gr/ontologies/ccso#Syllabus"/>
        <syllabusOf rdf:resource="http://xworks.gr/ontologies/ccso#CS335/CS_BSc/CSD/SSE/UoC"/>
        <code rdf:datatype="http://www.w3.org/2001/XMLSchema#string">CS335_s2017-18/CS_BSc/CSD/SSE/UoC</code>
        <csName rdf:datatype="http://www.w3.org/2001/XMLSchema#string">Syllabus of course CS335 Computer Networks</csName>
    </owl:NamedIndividual>
    


    <!-- http://xworks.gr/ontologies/ccso#CS335_s2016-17/CS_BSc/CSD/SSE/UoC -->

    <owl:NamedIndividual rdf:about="http://xworks.gr/ontologies/ccso#CS335_s2016-17/CS_BSc/CSD/SSE/UoC">
        <rdf:type rdf:resource="http://xworks.gr/ontologies/ccso#Syllabus"/>
        <syllabusOf rdf:resource="http://xworks.gr/ontologies/ccso#CS335/CS_BSc/CSD/SSE/UoC"/>
        <code rdf:datatype="http://www.w3.org/2001/XMLSchema#string">CS335_s2017-18/CS_BSc/CSD/SSE/UoC</code>
        <csName rdf:datatype="http://www.w3.org/2001/XMLSchema#string">Syllabus of course CS335 Computer Networks</csName>
    </owl:NamedIndividual>
    


    <!-- http://xworks.gr/ontologies/ccso#CS335_s2017-18-FE01/CS_BSc/CSD/SSE/UoC -->

    <owl:NamedIndividual rdf:about="http://xworks.gr/ontologies/ccso#CS335_s2017-18-FE01/CS_BSc/CSD/SSE/UoC">
        <rdf:type rdf:resource="http://xworks.gr/ontologies/ccso#EvaluationEvent"/>
        <rdf:type rdf:resource="http://xworks.gr/ontologies/ccso#Event"/>
        <affiliatedWith rdf:resource="http://xworks.gr/ontologies/ccso#Tsiknakis_Manolis"/>
        <hasGrader rdf:resource="http://xworks.gr/ontologies/ccso#Tsiknakis_Manolis"/>
        <dates rdf:datatype="http://www.w3.org/2001/XMLSchema#dateTime">2018-02-28T12:00:00</dates>
        <duration rdf:datatype="http://www.w3.org/2001/XMLSchema#duration">PT2H</duration>
        <duration rdf:datatype="internal:anonymous-constants">PT2H</duration>
        <eventClassroom rdf:datatype="http://www.w3.org/2001/XMLSchema#string">A113</eventClassroom>
        <eventDateTime rdf:datatype="http://www.w3.org/2001/XMLSchema#dateTime">2018-02-28T12:00:00</eventDateTime>
        <label rdf:datatype="http://www.w3.org/2001/XMLSchema#string">Final Examination
CS335 Computer Networks</label>
    </owl:NamedIndividual>
    


    <!-- http://xworks.gr/ontologies/ccso#CS335_s2017-18-L02/CS_BSc/CSD/SSE/UoC -->

    <owl:NamedIndividual rdf:about="http://xworks.gr/ontologies/ccso#CS335_s2017-18-L02/CS_BSc/CSD/SSE/UoC">
        <rdf:type rdf:resource="http://xworks.gr/ontologies/ccso#Event"/>
        <rdf:type rdf:resource="http://xworks.gr/ontologies/ccso#TeachingEvent"/>
        <affiliatedWith rdf:resource="http://xworks.gr/ontologies/ccso#Kondylakis_Haridimos"/>
        <affiliatedWith rdf:resource="http://xworks.gr/ontologies/ccso#Tsiknakis_Manolis"/>
        <expectsLO rdf:resource="http://xworks.gr/ontologies/ccso#CS/NC/RF/LO_Describe_how_packets_are_forwarded_in_an_IP_networks"/>
        <hasEventAssistant rdf:resource="http://xworks.gr/ontologies/ccso#Kondylakis_Haridimos"/>
        <hasTeacher rdf:resource="http://xworks.gr/ontologies/ccso#Tsiknakis_Manolis"/>
        <hasTopic rdf:resource="http://xworks.gr/ontologies/ccso#CS/NC/RF/T_Routing_versus_forwarding"/>
        <hasTopic rdf:resource="http://xworks.gr/ontologies/ccso#CS/NC/RF/T_Static_routing"/>
        <dates rdf:datatype="http://www.w3.org/2001/XMLSchema#dateTime">2017-09-27T12:00:00</dates>
        <duration rdf:datatype="http://www.w3.org/2001/XMLSchema#duration">PT2H</duration>
        <duration rdf:datatype="internal:anonymous-constants">PT2H</duration>
        <eventClassroom rdf:datatype="http://www.w3.org/2001/XMLSchema#string">A113</eventClassroom>
        <eventDateTime rdf:datatype="http://www.w3.org/2001/XMLSchema#dateTime">2017-09-27T12:00:00</eventDateTime>
        <label rdf:datatype="http://www.w3.org/2001/XMLSchema#string">Lesson 02
CS335 Computer Networks</label>
    </owl:NamedIndividual>
    


    <!-- http://xworks.gr/ontologies/ccso#CS335_s2017-18-L03/CS_BSc/CSD/SSE/UoC -->

    <owl:NamedIndividual rdf:about="http://xworks.gr/ontologies/ccso#CS335_s2017-18-L03/CS_BSc/CSD/SSE/UoC">
        <rdf:type rdf:resource="http://xworks.gr/ontologies/ccso#Event"/>
        <rdf:type rdf:resource="http://xworks.gr/ontologies/ccso#TeachingEvent"/>
        <affiliatedWith rdf:resource="http://xworks.gr/ontologies/ccso#Kondylakis_Haridimos"/>
        <affiliatedWith rdf:resource="http://xworks.gr/ontologies/ccso#Tsiknakis_Manolis"/>
        <expectsLO rdf:resource="http://xworks.gr/ontologies/ccso#CS/NC/RF/LO_Describe_the_organization_of_the_network_layer"/>
        <expectsLO rdf:resource="http://xworks.gr/ontologies/ccso#CS/NC/RF/LO_List_the_scalability_benefits_of_hierarchical_addressing"/>
        <hasEventAssistant rdf:resource="http://xworks.gr/ontologies/ccso#Kondylakis_Haridimos"/>
        <hasTeacher rdf:resource="http://xworks.gr/ontologies/ccso#Tsiknakis_Manolis"/>
        <hasTopic rdf:resource="http://xworks.gr/ontologies/ccso#CS/NC/RF/T_Internet_Protocol"/>
        <hasTopic rdf:resource="http://xworks.gr/ontologies/ccso#CS/NC/RF/T_Scalability_issues"/>
        <dates rdf:datatype="http://www.w3.org/2001/XMLSchema#dateTime">2017-10-02T12:00:00</dates>
        <duration rdf:datatype="http://www.w3.org/2001/XMLSchema#duration">PT2H</duration>
        <duration rdf:datatype="internal:anonymous-constants">PT2H</duration>
        <eventClassroom rdf:datatype="http://www.w3.org/2001/XMLSchema#string">A113</eventClassroom>
        <eventDateTime rdf:datatype="http://www.w3.org/2001/XMLSchema#dateTime">2017-10-02T12:00:00</eventDateTime>
        <label rdf:datatype="http://www.w3.org/2001/XMLSchema#string">Lesson 03
CS335 Computer Networks</label>
    </owl:NamedIndividual>
    


    <!-- http://xworks.gr/ontologies/ccso#CS335_s2017-18-L04/CS_BSc/CSD/SSE/UoC -->

    <owl:NamedIndividual rdf:about="http://xworks.gr/ontologies/ccso#CS335_s2017-18-L04/CS_BSc/CSD/SSE/UoC">
        <rdf:type rdf:resource="http://xworks.gr/ontologies/ccso#Event"/>
        <rdf:type rdf:resource="http://xworks.gr/ontologies/ccso#TeachingEvent"/>
        <affiliatedWith rdf:resource="http://xworks.gr/ontologies/ccso#Kondylakis_Haridimos"/>
        <affiliatedWith rdf:resource="http://xworks.gr/ontologies/ccso#Tsiknakis_Manolis"/>
        <expectsLO rdf:resource="http://xworks.gr/ontologies/ccso#CS/NC/LAN/LO_Describe_the_steps_used_in_one_common_approach_to_the_multiple_access_problem"/>
        <hasEventAssistant rdf:resource="http://xworks.gr/ontologies/ccso#Kondylakis_Haridimos"/>
        <hasTeacher rdf:resource="http://xworks.gr/ontologies/ccso#Tsiknakis_Manolis"/>
        <hasTopic rdf:resource="http://xworks.gr/ontologies/ccso#CS/NC/LAN/T_Common_approaches_to_multiple_access"/>
        <hasTopic rdf:resource="http://xworks.gr/ontologies/ccso#CS/NC/LAN/T_Multiple_Access_Problem"/>
        <dates rdf:datatype="http://www.w3.org/2001/XMLSchema#dateTime">2017-10-04T12:00:00</dates>
        <duration rdf:datatype="http://www.w3.org/2001/XMLSchema#duration">PT2H</duration>
        <duration rdf:datatype="internal:anonymous-constants">PT2H</duration>
        <eventClassroom rdf:datatype="http://www.w3.org/2001/XMLSchema#string">A113</eventClassroom>
        <eventDateTime rdf:datatype="http://www.w3.org/2001/XMLSchema#dateTime">2017-10-04T12:00:00</eventDateTime>
        <label rdf:datatype="http://www.w3.org/2001/XMLSchema#string">Lesson 04
CS335 Computer Networks</label>
    </owl:NamedIndividual>
    


    <!-- http://xworks.gr/ontologies/ccso#CS335_s2017-18-L05/CS_BSc/CSD/SSE/UoC -->

    <owl:NamedIndividual rdf:about="http://xworks.gr/ontologies/ccso#CS335_s2017-18-L05/CS_BSc/CSD/SSE/UoC">
        <rdf:type rdf:resource="http://xworks.gr/ontologies/ccso#Event"/>
        <rdf:type rdf:resource="http://xworks.gr/ontologies/ccso#TeachingEvent"/>
        <affiliatedWith rdf:resource="http://xworks.gr/ontologies/ccso#Pappa_Pepi"/>
        <affiliatedWith rdf:resource="http://xworks.gr/ontologies/ccso#Tsiknakis_Manolis"/>
        <expectsLO rdf:resource="http://xworks.gr/ontologies/ccso#CS/NC/LAN/LO_Describe_how_frames_are_forwarded_in_an_Ethernet_network"/>
        <expectsLO rdf:resource="http://xworks.gr/ontologies/ccso#CS/NC/LAN/LO_Identify_the_differences_between_IP_and_Ethernet"/>
        <hasEventAssistant rdf:resource="http://xworks.gr/ontologies/ccso#Pappa_Pepi"/>
        <hasTeacher rdf:resource="http://xworks.gr/ontologies/ccso#Tsiknakis_Manolis"/>
        <hasTopic rdf:resource="http://xworks.gr/ontologies/ccso#CS/NC/LAN/T_Ethernet"/>
        <hasTopic rdf:resource="http://xworks.gr/ontologies/ccso#CS/NC/LAN/T_Local_Area_Networks"/>
        <hasTopic rdf:resource="http://xworks.gr/ontologies/ccso#CS/NC/LAN/T_Switching"/>
        <dates rdf:datatype="http://www.w3.org/2001/XMLSchema#dateTime">2017-10-09T12:00:00</dates>
        <duration rdf:datatype="http://www.w3.org/2001/XMLSchema#duration">PT2H</duration>
        <duration rdf:datatype="internal:anonymous-constants">PT2H</duration>
        <eventClassroom rdf:datatype="http://www.w3.org/2001/XMLSchema#string">A113</eventClassroom>
        <eventDateTime rdf:datatype="http://www.w3.org/2001/XMLSchema#dateTime">2017-10-09T12:00:00</eventDateTime>
        <label rdf:datatype="http://www.w3.org/2001/XMLSchema#string">Lesson 05
CS335 Computer Networks</label>
    </owl:NamedIndividual>
    


    <!-- http://xworks.gr/ontologies/ccso#CS335_s2017-18/CS_BSc/CSD/SSE/UoC -->

    <owl:NamedIndividual rdf:about="http://xworks.gr/ontologies/ccso#CS335_s2017-18/CS_BSc/CSD/SSE/UoC">
        <rdf:type rdf:resource="http://xworks.gr/ontologies/ccso#Syllabus"/>
        <affiliatedWith rdf:resource="http://xworks.gr/ontologies/ccso#Kondylakis_Haridimos"/>
        <affiliatedWith rdf:resource="http://xworks.gr/ontologies/ccso#Tsiknakis_Manolis"/>
        <aimsToLO rdf:resource="http://xworks.gr/ontologies/ccso#CS/NC/LAN/LO_Describe_how_frames_are_forwarded_in_an_Ethernet_network"/>
        <aimsToLO rdf:resource="http://xworks.gr/ontologies/ccso#CS/NC/LAN/LO_Describe_the_interrelations_between_IP_and_Ethernet"/>
        <aimsToLO rdf:resource="http://xworks.gr/ontologies/ccso#CS/NC/LAN/LO_Describe_the_steps_used_in_one_common_approach_to_the_multiple_access_problem"/>
        <aimsToLO rdf:resource="http://xworks.gr/ontologies/ccso#CS/NC/LAN/LO_Identify_the_differences_between_IP_and_Ethernet"/>
        <aimsToLO rdf:resource="http://xworks.gr/ontologies/ccso#CS/NC/RF/LO_Describe_how_packets_are_forwarded_in_an_IP_networks"/>
        <aimsToLO rdf:resource="http://xworks.gr/ontologies/ccso#CS/NC/RF/LO_Describe_the_organization_of_the_network_layer"/>
        <aimsToLO rdf:resource="http://xworks.gr/ontologies/ccso#CS/NC/RF/LO_List_the_scalability_benefits_of_hierarchical_addressing"/>
        <coversTopic rdf:resource="http://xworks.gr/ontologies/ccso#CS/NC/LAN/T_Common_approaches_to_multiple_access"/>
        <coversTopic rdf:resource="http://xworks.gr/ontologies/ccso#CS/NC/LAN/T_Ethernet"/>
        <coversTopic rdf:resource="http://xworks.gr/ontologies/ccso#CS/NC/LAN/T_Local_Area_Networks"/>
        <coversTopic rdf:resource="http://xworks.gr/ontologies/ccso#CS/NC/LAN/T_Multiple_Access_Problem"/>
        <coversTopic rdf:resource="http://xworks.gr/ontologies/ccso#CS/NC/LAN/T_Switching"/>
        <coversTopic rdf:resource="http://xworks.gr/ontologies/ccso#CS/NC/RF/T_Internet_Protocol"/>
        <coversTopic rdf:resource="http://xworks.gr/ontologies/ccso#CS/NC/RF/T_Routing_versus_forwarding"/>
        <coversTopic rdf:resource="http://xworks.gr/ontologies/ccso#CS/NC/RF/T_Scalability_issues"/>
        <coversTopic rdf:resource="http://xworks.gr/ontologies/ccso#CS/NC/RF/T_Static_routing"/>
        <hasCourseAssistant rdf:resource="http://xworks.gr/ontologies/ccso#Kondylakis_Haridimos"/>
        <hasEvent rdf:resource="http://xworks.gr/ontologies/ccso#CS335_s2017-18-FE01/CS_BSc/CSD/SSE/UoC"/>
        <hasEvent rdf:resource="http://xworks.gr/ontologies/ccso#CS335_s2017-18-L02/CS_BSc/CSD/SSE/UoC"/>
        <hasEvent rdf:resource="http://xworks.gr/ontologies/ccso#CS335_s2017-18-L03/CS_BSc/CSD/SSE/UoC"/>
        <hasEvent rdf:resource="http://xworks.gr/ontologies/ccso#CS335_s2017-18-L04/CS_BSc/CSD/SSE/UoC"/>
        <hasEvent rdf:resource="http://xworks.gr/ontologies/ccso#CS335_s2017-18-L05/CS_BSc/CSD/SSE/UoC"/>
        <hasInstructor rdf:resource="http://xworks.gr/ontologies/ccso#Tsiknakis_Manolis"/>
        <hasLM rdf:resource="http://xworks.gr/ontologies/ccso#Peterson2007ComputerNetworks"/>
        <hasSupervisor rdf:resource="http://xworks.gr/ontologies/ccso#Tsiknakis_Manolis"/>
        <syllabusOf rdf:resource="http://xworks.gr/ontologies/ccso#CS335/CS_BSc/CSD/SSE/UoC"/>
        <code rdf:datatype="http://www.w3.org/2001/XMLSchema#string">CS335_s2017-18/CS_BSc/CSD/SSE/UoC</code>
        <courseType rdf:datatype="http://www.w3.org/2001/XMLSchema#string">Core</courseType>
        <courseURL rdf:datatype="http://www.w3.org/2001/XMLSchema#anyURI">http://www.csd.uoc.gr/~hy335a</courseURL>
        <creditsECTS rdf:datatype="http://www.w3.org/2001/XMLSchema#short">6</creditsECTS>
        <csName rdf:datatype="http://www.w3.org/2001/XMLSchema#string">Syllabus of course CS335 Computer Networks</csName>
        <description rdf:datatype="http://www.w3.org/2001/XMLSchema#string">This course covers the basic principles and technologies of computer networks. Its contents include: Introduction to communications networks and the services they offer. Design principles, layered architecture, information transmission, switching, mutliplexing. The OSI model and the Internet model. Physical layer: signal propagation, optical transmission, synchronization and framing, digitization of information. Data link layer: protocols, alternating bit protocol, go-back-N, selective repeat, examples. Local area networks: ALOHA, Ethernet, token ring, FDDI, DQDB. Network layer: naming and addressing, IP routing, address resolution, congestion control, network design, examples. Transport, session, presentation and application layers: TCP, session establishment, syntax conversion, main applications.</description>
        <evaluationInfo rdf:datatype="http://www.w3.org/2001/XMLSchema#string">Βαθμός = MAX(65%*ΤΕΛΙΚΗ ΕΞΕΤΑΣΗ + 10%*ΜΟ ΑΣΚΗΣΕΩΝ + 25%*PROJECT,
50%*ΤΕΛΙΚΗ ΕΞΕΤΑΣΗ + 10%*ΜΟ ΑΣΚΗΣΕΩΝ + 25%*PROJECT + 15%*ΠΡΟΟΔΟΣ)</evaluationInfo>
        <language rdf:datatype="http://www.w3.org/2001/XMLSchema#string">Greek</language>
        <semesterinProgram rdf:datatype="http://www.w3.org/2001/XMLSchema#short">5</semesterinProgram>
        <webaddressURL rdf:datatype="http://www.w3.org/2001/XMLSchema#anyURI">http://www.csd.uoc.gr/~hy335a</webaddressURL>
        <weeklyClassSchedule rdf:datatype="http://www.w3.org/2001/XMLSchema#string">Monday 12:00-14:00 Α113
Wednesday 12:00-14:00 Α113</weeklyClassSchedule>
        <weeklyHours rdf:datatype="http://www.w3.org/2001/XMLSchema#short">4</weeklyHours>
    </owl:NamedIndividual>
    


    <!-- http://xworks.gr/ontologies/ccso#CS340/CS_BSc/CSD/SSE/UoC -->

    <owl:NamedIndividual rdf:about="http://xworks.gr/ontologies/ccso#CS340/CS_BSc/CSD/SSE/UoC">
        <rdf:type rdf:resource="http://xworks.gr/ontologies/ccso#Course"/>
        <coversKA rdf:resource="http://xworks.gr/ontologies/ccso#CS/PL_Programming_Languages"/>
        <hasPrerequisite rdf:resource="http://xworks.gr/ontologies/ccso#CS240/CS_BSc/CSD/SSE/UoC"/>
        <hasPrerequisite rdf:resource="http://xworks.gr/ontologies/ccso#CS280/CS_BSc/CSD/SSE/UoC"/>
        <hasSyllabus rdf:resource="http://xworks.gr/ontologies/ccso#CS340s1/CS_BSc/CSD/SSE/UoC"/>
        <includedIn rdf:resource="http://xworks.gr/ontologies/ccso#BSc_Computer_Science/CS_BSc/CSD/SSE/UoC"/>
        <offeredBy rdf:resource="http://xworks.gr/ontologies/ccso#Computers_Sciences_Department_of_University_of_Crete"/>
        <courseType rdf:datatype="http://www.w3.org/2001/XMLSchema#string">Core</courseType>
        <csName rdf:datatype="http://www.w3.org/2001/XMLSchema#string">Languages and Compilers</csName>
    </owl:NamedIndividual>
    


    <!-- http://xworks.gr/ontologies/ccso#CS340s1/CS_BSc/CSD/SSE/UoC -->

    <owl:NamedIndividual rdf:about="http://xworks.gr/ontologies/ccso#CS340s1/CS_BSc/CSD/SSE/UoC">
        <rdf:type rdf:resource="http://xworks.gr/ontologies/ccso#Syllabus"/>
        <affiliatedWith rdf:resource="http://xworks.gr/ontologies/ccso#Kondylakis_Haridimos"/>
        <affiliatedWith rdf:resource="http://xworks.gr/ontologies/ccso#Savidis_Anthony"/>
        <coversTopic rdf:resource="http://xworks.gr/ontologies/ccso#CS/PL/T_Definition_of_classes:fields,methods,and_constructors"/>
        <hasCourseAssistant rdf:resource="http://xworks.gr/ontologies/ccso#Kondylakis_Haridimos"/>
        <hasInstructor rdf:resource="http://xworks.gr/ontologies/ccso#Savidis_Anthony"/>
        <hasSupervisor rdf:resource="http://xworks.gr/ontologies/ccso#Savidis_Anthony"/>
        <syllabusOf rdf:resource="http://xworks.gr/ontologies/ccso#CS340/CS_BSc/CSD/SSE/UoC"/>
        <courseType rdf:datatype="http://www.w3.org/2001/XMLSchema#string">Core</courseType>
        <creditsECTS rdf:datatype="http://www.w3.org/2001/XMLSchema#short">8</creditsECTS>
        <csName rdf:datatype="http://www.w3.org/2001/XMLSchema#string">Syllabus of course CS340 Languages and Compilers</csName>
        <semesterinProgram rdf:datatype="http://www.w3.org/2001/XMLSchema#short">3</semesterinProgram>
    </owl:NamedIndividual>
    


    <!-- http://xworks.gr/ontologies/ccso#CS342/CS_BSc/CSD/SSE/UoC -->

    <owl:NamedIndividual rdf:about="http://xworks.gr/ontologies/ccso#CS342/CS_BSc/CSD/SSE/UoC">
        <rdf:type rdf:resource="http://xworks.gr/ontologies/ccso#Course"/>
        <coversKA rdf:resource="http://xworks.gr/ontologies/ccso#CS/PL_Programming_Languages"/>
        <coversKA rdf:resource="http://xworks.gr/ontologies/ccso#CS/SW_Software_Engineering_Software_Systems_and_Applications"/>
        <hasPrerequisite rdf:resource="http://xworks.gr/ontologies/ccso#CS252/CS_BSc/CSD/SSE/UoC"/>
        <hasSyllabus rdf:resource="http://xworks.gr/ontologies/ccso#CS342s1/CS_BSc/CSD/SSE/UoC"/>
        <includedIn rdf:resource="http://xworks.gr/ontologies/ccso#BSc_Computer_Science/CS_BSc/CSD/SSE/UoC"/>
        <offeredBy rdf:resource="http://xworks.gr/ontologies/ccso#Computers_Sciences_Department_of_University_of_Crete"/>
        <courseType rdf:datatype="http://www.w3.org/2001/XMLSchema#string">Elective</courseType>
        <csName rdf:datatype="http://www.w3.org/2001/XMLSchema#string">Parallel Programming</csName>
    </owl:NamedIndividual>
    


    <!-- http://xworks.gr/ontologies/ccso#CS342s1/CS_BSc/CSD/SSE/UoC -->

    <owl:NamedIndividual rdf:about="http://xworks.gr/ontologies/ccso#CS342s1/CS_BSc/CSD/SSE/UoC">
        <rdf:type rdf:resource="http://xworks.gr/ontologies/ccso#Syllabus"/>
        <affiliatedWith rdf:resource="http://xworks.gr/ontologies/ccso#Savidis_Anthony"/>
        <aimsToLO rdf:resource="http://xworks.gr/ontologies/ccso#CS/PL/LO_Correctly_reason_about_control_flow_in_a_program_using_dynamic_dispatch"/>
        <aimsToLO rdf:resource="http://xworks.gr/ontologies/ccso#CS/PL/LO_Use_subclassing_to_design_simple_class_hierarchies_that_allow_code_to_be_reused_for_distinct_subclasses"/>
        <aimsToLO rdf:resource="http://xworks.gr/ontologies/ccso#CS/PL/LO_Compare_and_contrast_the_procedural/functional_approach_and_the_object-oriented_approach"/>
        <coversTopic rdf:resource="http://xworks.gr/ontologies/ccso#CS/PL/T_Definition_of_classes:fields,methods,and_constructors"/>
        <coversTopic rdf:resource="http://xworks.gr/ontologies/ccso#CS/PL/T_Dynamic_dispatch:Definition_of_Method-Call"/>
        <coversTopic rdf:resource="http://xworks.gr/ontologies/ccso#CS/PL/T_Object-Oriented_Design,Class-Hierarchy_design_for_modeling"/>
        <coversTopic rdf:resource="http://xworks.gr/ontologies/ccso#CS/PL/T_Subclasses,Inheritance,and_Method_Overriding"/>
        <hasInstructor rdf:resource="http://xworks.gr/ontologies/ccso#Savidis_Anthony"/>
        <hasSupervisor rdf:resource="http://xworks.gr/ontologies/ccso#Savidis_Anthony"/>
        <syllabusOf rdf:resource="http://xworks.gr/ontologies/ccso#CS342/CS_BSc/CSD/SSE/UoC"/>
        <courseType rdf:datatype="http://www.w3.org/2001/XMLSchema#string">Elective</courseType>
        <creditsECTS rdf:datatype="http://www.w3.org/2001/XMLSchema#short">6</creditsECTS>
        <csName rdf:datatype="http://www.w3.org/2001/XMLSchema#string">Syllabus of course CS342 Parallel Programming</csName>
        <semesterinProgram rdf:datatype="http://www.w3.org/2001/XMLSchema#short">4</semesterinProgram>
    </owl:NamedIndividual>
    


    <!-- http://xworks.gr/ontologies/ccso#CS345/CS_BSc/CSD/SSE/UoC -->

    <owl:NamedIndividual rdf:about="http://xworks.gr/ontologies/ccso#CS345/CS_BSc/CSD/SSE/UoC">
        <rdf:type rdf:resource="http://xworks.gr/ontologies/ccso#Course"/>
        <hasPrerequisite rdf:resource="http://xworks.gr/ontologies/ccso#CS118/CS_BSc/CSD/SSE/UoC"/>
        <hasPrerequisite rdf:resource="http://xworks.gr/ontologies/ccso#CS240/CS_BSc/CSD/SSE/UoC"/>
        <hasSyllabus rdf:resource="http://xworks.gr/ontologies/ccso#CS345s1/CS_BSc/CSD/SSE/UoC"/>
        <includedIn rdf:resource="http://xworks.gr/ontologies/ccso#BSc_Computer_Science/CS_BSc/CSD/SSE/UoC"/>
        <offeredBy rdf:resource="http://xworks.gr/ontologies/ccso#Computers_Sciences_Department_of_University_of_Crete"/>
        <code rdf:datatype="http://www.w3.org/2001/XMLSchema#string">CS345/CS_BSc/CSD/SSE/UoC</code>
        <courseType rdf:datatype="http://www.w3.org/2001/XMLSchema#string">Core</courseType>
        <csName rdf:datatype="http://www.w3.org/2001/XMLSchema#string">Operating Systems</csName>
    </owl:NamedIndividual>
    


    <!-- http://xworks.gr/ontologies/ccso#CS345_s2017-18-FE01/CS_BSc/CSD/SSE/UoC -->

    <owl:NamedIndividual rdf:about="http://xworks.gr/ontologies/ccso#CS345_s2017-18-FE01/CS_BSc/CSD/SSE/UoC">
        <rdf:type rdf:resource="http://xworks.gr/ontologies/ccso#EvaluationEvent"/>
        <rdf:type rdf:resource="http://xworks.gr/ontologies/ccso#Event"/>
        <affiliatedWith rdf:resource="http://xworks.gr/ontologies/ccso#Markatos_Evangelos"/>
        <hasGrader rdf:resource="http://xworks.gr/ontologies/ccso#Markatos_Evangelos"/>
        <dates rdf:datatype="http://www.w3.org/2001/XMLSchema#dateTime">2018-02-01T12:00:00</dates>
        <duration rdf:datatype="http://www.w3.org/2001/XMLSchema#duration">PT2H</duration>
        <duration rdf:datatype="internal:anonymous-constants">PT2H</duration>
        <eventClassroom rdf:datatype="http://www.w3.org/2001/XMLSchema#string">A113</eventClassroom>
        <eventDateTime rdf:datatype="http://www.w3.org/2001/XMLSchema#dateTime">2018-02-01T12:00:00</eventDateTime>
        <label rdf:datatype="http://www.w3.org/2001/XMLSchema#string">Final Examination
CS345 Operating Systems</label>
    </owl:NamedIndividual>
    


    <!-- http://xworks.gr/ontologies/ccso#CS345_s2017-18-L02/CS_BSc/CSD/SSE/UoC -->

    <owl:NamedIndividual rdf:about="http://xworks.gr/ontologies/ccso#CS345_s2017-18-L02/CS_BSc/CSD/SSE/UoC">
        <rdf:type rdf:resource="http://xworks.gr/ontologies/ccso#Event"/>
        <rdf:type rdf:resource="http://xworks.gr/ontologies/ccso#TeachingEvent"/>
        <affiliatedWith rdf:resource="http://xworks.gr/ontologies/ccso#Markatos_Evangelos"/>
        <hasTeacher rdf:resource="http://xworks.gr/ontologies/ccso#Markatos_Evangelos"/>
        <dates rdf:datatype="http://www.w3.org/2001/XMLSchema#dateTime">2017-02-07T10:00:00</dates>
        <duration rdf:datatype="http://www.w3.org/2001/XMLSchema#duration">PT2H</duration>
        <duration rdf:datatype="internal:anonymous-constants">PT2H</duration>
        <eventClassroom rdf:datatype="http://www.w3.org/2001/XMLSchema#string">A113</eventClassroom>
        <eventDateTime rdf:datatype="http://www.w3.org/2001/XMLSchema#dateTime">2017-02-07T10:00:00</eventDateTime>
        <eventWeekNo rdf:datatype="http://www.w3.org/2001/XMLSchema#short">1</eventWeekNo>
        <label rdf:datatype="http://www.w3.org/2001/XMLSchema#string">Lesson 02 in
CS345 Operating Systems</label>
    </owl:NamedIndividual>
    


    <!-- http://xworks.gr/ontologies/ccso#CS345s1/CS_BSc/CSD/SSE/UoC -->

    <owl:NamedIndividual rdf:about="http://xworks.gr/ontologies/ccso#CS345s1/CS_BSc/CSD/SSE/UoC">
        <rdf:type rdf:resource="http://xworks.gr/ontologies/ccso#Syllabus"/>
        <affiliatedWith rdf:resource="http://xworks.gr/ontologies/ccso#Kondylakis_Haridimos"/>
        <affiliatedWith rdf:resource="http://xworks.gr/ontologies/ccso#Markatos_Evangelos"/>
        <hasCourseAssistant rdf:resource="http://xworks.gr/ontologies/ccso#Kondylakis_Haridimos"/>
        <hasEvent rdf:resource="http://xworks.gr/ontologies/ccso#CS345_s2017-18-FE01/CS_BSc/CSD/SSE/UoC"/>
        <hasEvent rdf:resource="http://xworks.gr/ontologies/ccso#CS345_s2017-18-L02/CS_BSc/CSD/SSE/UoC"/>
        <hasInstructor rdf:resource="http://xworks.gr/ontologies/ccso#Markatos_Evangelos"/>
        <hasSupervisor rdf:resource="http://xworks.gr/ontologies/ccso#Markatos_Evangelos"/>
        <syllabusOf rdf:resource="http://xworks.gr/ontologies/ccso#CS345/CS_BSc/CSD/SSE/UoC"/>
        <code rdf:datatype="http://www.w3.org/2001/XMLSchema#string">CS345/CS_BSc/CSD/SSE/UoC</code>
        <courseType rdf:datatype="http://www.w3.org/2001/XMLSchema#string">Core</courseType>
        <courseURL rdf:datatype="http://www.w3.org/2001/XMLSchema#anyURI">http://www.csd.uoc.gr/~hy345</courseURL>
        <creditsECTS rdf:datatype="http://www.w3.org/2001/XMLSchema#short">8</creditsECTS>
        <csName rdf:datatype="http://www.w3.org/2001/XMLSchema#string">Syllabus of course CS345 Operating Systems</csName>
        <description rdf:datatype="http://www.w3.org/2001/XMLSchema#string">Description of operating system procedures and their implementation: multiprogramming, process communication (synchronization, semaphores), context switching, process scheduling, system calls, interrupt handlers, deadlock, device independent I/O, device drivers, disk scheduling, memory management, virtual memory, paging algorithms, file systems, distributed operating systems. Laboratory exercises in modifying and augmenting a simple operating system.</description>
        <semesterinProgram rdf:datatype="http://www.w3.org/2001/XMLSchema#short">3</semesterinProgram>
        <webaddressURL rdf:datatype="http://www.w3.org/2001/XMLSchema#anyURI">http://www.csd.uoc.gr/~hy345</webaddressURL>
        <weeklyClassSchedule rdf:datatype="http://www.w3.org/2001/XMLSchema#string">Monday 10:00-12:00 (Α113)
Wednesday 10:00-12:00 (A113)</weeklyClassSchedule>
        <weeklyHours rdf:datatype="http://www.w3.org/2001/XMLSchema#short">4</weeklyHours>
    </owl:NamedIndividual>
    


    <!-- http://xworks.gr/ontologies/ccso#CS351/CS_BSc/CSD/SSE/UoC -->

    <owl:NamedIndividual rdf:about="http://xworks.gr/ontologies/ccso#CS351/CS_BSc/CSD/SSE/UoC">
        <rdf:type rdf:resource="http://xworks.gr/ontologies/ccso#Course"/>
        <coversKA rdf:resource="http://xworks.gr/ontologies/ccso#CS/SW_Software_Engineering_Software_Systems_and_Applications"/>
        <hasPrerequisite rdf:resource="http://xworks.gr/ontologies/ccso#CS252/CS_BSc/CSD/SSE/UoC"/>
        <hasSyllabus rdf:resource="http://xworks.gr/ontologies/ccso#CS351s1/CS_BSc/CSD/SSE/UoC"/>
        <includedIn rdf:resource="http://xworks.gr/ontologies/ccso#BSc_Computer_Science/CS_BSc/CSD/SSE/UoC"/>
        <offeredBy rdf:resource="http://xworks.gr/ontologies/ccso#Computers_Sciences_Department_of_University_of_Crete"/>
        <courseType rdf:datatype="http://www.w3.org/2001/XMLSchema#string">Elective</courseType>
        <csName rdf:datatype="http://www.w3.org/2001/XMLSchema#string">Information System Analysis and Design</csName>
    </owl:NamedIndividual>
    


    <!-- http://xworks.gr/ontologies/ccso#CS351s1/CS_BSc/CSD/SSE/UoC -->

    <owl:NamedIndividual rdf:about="http://xworks.gr/ontologies/ccso#CS351s1/CS_BSc/CSD/SSE/UoC">
        <rdf:type rdf:resource="http://xworks.gr/ontologies/ccso#Syllabus"/>
        <syllabusOf rdf:resource="http://xworks.gr/ontologies/ccso#CS351/CS_BSc/CSD/SSE/UoC"/>
        <courseType rdf:datatype="http://www.w3.org/2001/XMLSchema#string">Elective</courseType>
        <creditsECTS rdf:datatype="http://www.w3.org/2001/XMLSchema#short">6</creditsECTS>
        <csName rdf:datatype="http://www.w3.org/2001/XMLSchema#string">Syllabus of course CS351 Information System Analysis and Design</csName>
        <semesterinProgram rdf:datatype="http://www.w3.org/2001/XMLSchema#short">4</semesterinProgram>
    </owl:NamedIndividual>
    


    <!-- http://xworks.gr/ontologies/ccso#CS352/CS_BSc/CSD/SSE/UoC -->

    <owl:NamedIndividual rdf:about="http://xworks.gr/ontologies/ccso#CS352/CS_BSc/CSD/SSE/UoC">
        <rdf:type rdf:resource="http://xworks.gr/ontologies/ccso#Course"/>
        <coversKA rdf:resource="http://xworks.gr/ontologies/ccso#CS/SW_Software_Engineering_Software_Systems_and_Applications"/>
        <hasPrerequisite rdf:resource="http://xworks.gr/ontologies/ccso#CS252/CS_BSc/CSD/SSE/UoC"/>
        <hasSyllabus rdf:resource="http://xworks.gr/ontologies/ccso#CS352s1/CS_BSc/CSD/SSE/UoC"/>
        <includedIn rdf:resource="http://xworks.gr/ontologies/ccso#BSc_Computer_Science/CS_BSc/CSD/SSE/UoC"/>
        <offeredBy rdf:resource="http://xworks.gr/ontologies/ccso#Computers_Sciences_Department_of_University_of_Crete"/>
        <courseType rdf:datatype="http://www.w3.org/2001/XMLSchema#string">Elective</courseType>
        <csName rdf:datatype="http://www.w3.org/2001/XMLSchema#string">Software Engineering</csName>
    </owl:NamedIndividual>
    


    <!-- http://xworks.gr/ontologies/ccso#CS352s1/CS_BSc/CSD/SSE/UoC -->

    <owl:NamedIndividual rdf:about="http://xworks.gr/ontologies/ccso#CS352s1/CS_BSc/CSD/SSE/UoC">
        <rdf:type rdf:resource="http://xworks.gr/ontologies/ccso#Syllabus"/>
        <syllabusOf rdf:resource="http://xworks.gr/ontologies/ccso#CS352/CS_BSc/CSD/SSE/UoC"/>
        <courseType rdf:datatype="http://www.w3.org/2001/XMLSchema#string">Elective</courseType>
        <creditsECTS rdf:datatype="http://www.w3.org/2001/XMLSchema#short">6</creditsECTS>
        <csName rdf:datatype="http://www.w3.org/2001/XMLSchema#string">Syllabus of course CS352 Software Engineering</csName>
        <semesterinProgram rdf:datatype="http://www.w3.org/2001/XMLSchema#short">4</semesterinProgram>
    </owl:NamedIndividual>
    


    <!-- http://xworks.gr/ontologies/ccso#CS358/CS_BSc/CSD/SSE/UoC -->

    <owl:NamedIndividual rdf:about="http://xworks.gr/ontologies/ccso#CS358/CS_BSc/CSD/SSE/UoC">
        <rdf:type rdf:resource="http://xworks.gr/ontologies/ccso#Course"/>
        <coversKA rdf:resource="http://xworks.gr/ontologies/ccso#CS/SW_Software_Engineering_Software_Systems_and_Applications"/>
        <hasPrerequisite rdf:resource="http://xworks.gr/ontologies/ccso#CS240/CS_BSc/CSD/SSE/UoC"/>
        <hasSyllabus rdf:resource="http://xworks.gr/ontologies/ccso#CS358s1/CS_BSc/CSD/SSE/UoC"/>
        <includedIn rdf:resource="http://xworks.gr/ontologies/ccso#BSc_Computer_Science/CS_BSc/CSD/SSE/UoC"/>
        <offeredBy rdf:resource="http://xworks.gr/ontologies/ccso#Computers_Sciences_Department_of_University_of_Crete"/>
        <courseType rdf:datatype="http://www.w3.org/2001/XMLSchema#string">Elective</courseType>
        <csName rdf:datatype="http://www.w3.org/2001/XMLSchema#string">Computer Graphics</csName>
    </owl:NamedIndividual>
    


    <!-- http://xworks.gr/ontologies/ccso#CS358s1/CS_BSc/CSD/SSE/UoC -->

    <owl:NamedIndividual rdf:about="http://xworks.gr/ontologies/ccso#CS358s1/CS_BSc/CSD/SSE/UoC">
        <rdf:type rdf:resource="http://xworks.gr/ontologies/ccso#Syllabus"/>
        <syllabusOf rdf:resource="http://xworks.gr/ontologies/ccso#CS358/CS_BSc/CSD/SSE/UoC"/>
        <courseType rdf:datatype="http://www.w3.org/2001/XMLSchema#string">Elective</courseType>
        <creditsECTS rdf:datatype="http://www.w3.org/2001/XMLSchema#short">6</creditsECTS>
        <csName rdf:datatype="http://www.w3.org/2001/XMLSchema#string">Syllabus of course CS358 Computer Graphics</csName>
        <semesterinProgram rdf:datatype="http://www.w3.org/2001/XMLSchema#short">4</semesterinProgram>
    </owl:NamedIndividual>
    


    <!-- http://xworks.gr/ontologies/ccso#CS360/CS_BSc/CSD/SSE/UoC -->

    <owl:NamedIndividual rdf:about="http://xworks.gr/ontologies/ccso#CS360/CS_BSc/CSD/SSE/UoC">
        <rdf:type rdf:resource="http://xworks.gr/ontologies/ccso#Course"/>
        <hasPrerequisite rdf:resource="http://xworks.gr/ontologies/ccso#CS118/CS_BSc/CSD/SSE/UoC"/>
        <hasPrerequisite rdf:resource="http://xworks.gr/ontologies/ccso#CS240/CS_BSc/CSD/SSE/UoC"/>
        <hasSyllabus rdf:resource="http://xworks.gr/ontologies/ccso#CS360s1/CS_BSc/CSD/SSE/UoC"/>
        <includedIn rdf:resource="http://xworks.gr/ontologies/ccso#BSc_Computer_Science/CS_BSc/CSD/SSE/UoC"/>
        <offeredBy rdf:resource="http://xworks.gr/ontologies/ccso#Computers_Sciences_Department_of_University_of_Crete"/>
        <courseType rdf:datatype="http://www.w3.org/2001/XMLSchema#string">Core</courseType>
        <csName rdf:datatype="http://www.w3.org/2001/XMLSchema#string">Files and Databases</csName>
    </owl:NamedIndividual>
    


    <!-- http://xworks.gr/ontologies/ccso#CS360s1/CS_BSc/CSD/SSE/UoC -->

    <owl:NamedIndividual rdf:about="http://xworks.gr/ontologies/ccso#CS360s1/CS_BSc/CSD/SSE/UoC">
        <rdf:type rdf:resource="http://xworks.gr/ontologies/ccso#Syllabus"/>
        <affiliatedWith rdf:resource="http://xworks.gr/ontologies/ccso#Kondylakis_Haridimos"/>
        <affiliatedWith rdf:resource="http://xworks.gr/ontologies/ccso#Plexousakis_Dimitris"/>
        <hasCourseAssistant rdf:resource="http://xworks.gr/ontologies/ccso#Kondylakis_Haridimos"/>
        <hasInstructor rdf:resource="http://xworks.gr/ontologies/ccso#Plexousakis_Dimitris"/>
        <hasSupervisor rdf:resource="http://xworks.gr/ontologies/ccso#Plexousakis_Dimitris"/>
        <syllabusOf rdf:resource="http://xworks.gr/ontologies/ccso#CS360/CS_BSc/CSD/SSE/UoC"/>
        <courseType rdf:datatype="http://www.w3.org/2001/XMLSchema#string">Core</courseType>
        <creditsECTS rdf:datatype="http://www.w3.org/2001/XMLSchema#short">8</creditsECTS>
        <csName rdf:datatype="http://www.w3.org/2001/XMLSchema#string">Syllabus of course CS360 Files and Databases</csName>
        <semesterinProgram rdf:datatype="http://www.w3.org/2001/XMLSchema#short">5</semesterinProgram>
    </owl:NamedIndividual>
    


    <!-- http://xworks.gr/ontologies/ccso#CS364/CS_BSc/CSD/SSE/UoC -->

    <owl:NamedIndividual rdf:about="http://xworks.gr/ontologies/ccso#CS364/CS_BSc/CSD/SSE/UoC">
        <rdf:type rdf:resource="http://xworks.gr/ontologies/ccso#Course"/>
        <hasPrerequisite rdf:resource="http://xworks.gr/ontologies/ccso#CS150/CS_BSc/CSD/SSE/UoC"/>
        <hasSyllabus rdf:resource="http://xworks.gr/ontologies/ccso#CS364s1/CS_BSc/CSD/SSE/UoC"/>
        <includedIn rdf:resource="http://xworks.gr/ontologies/ccso#BSc_Computer_Science/CS_BSc/CSD/SSE/UoC"/>
        <offeredBy rdf:resource="http://xworks.gr/ontologies/ccso#Computers_Sciences_Department_of_University_of_Crete"/>
        <courseType rdf:datatype="http://www.w3.org/2001/XMLSchema#string">Elective</courseType>
        <csName rdf:datatype="http://www.w3.org/2001/XMLSchema#string">Introduction to Human-Computer Interaction</csName>
    </owl:NamedIndividual>
    


    <!-- http://xworks.gr/ontologies/ccso#CS364s1/CS_BSc/CSD/SSE/UoC -->

    <owl:NamedIndividual rdf:about="http://xworks.gr/ontologies/ccso#CS364s1/CS_BSc/CSD/SSE/UoC">
        <rdf:type rdf:resource="http://xworks.gr/ontologies/ccso#Syllabus"/>
        <syllabusOf rdf:resource="http://xworks.gr/ontologies/ccso#CS364/CS_BSc/CSD/SSE/UoC"/>
        <courseType rdf:datatype="http://www.w3.org/2001/XMLSchema#string">Elective</courseType>
        <creditsECTS rdf:datatype="http://www.w3.org/2001/XMLSchema#short">6</creditsECTS>
        <csName rdf:datatype="http://www.w3.org/2001/XMLSchema#string">Syllabus of course CS364 Introduction to Human-Computer Interaction</csName>
        <semesterinProgram rdf:datatype="http://www.w3.org/2001/XMLSchema#short">5</semesterinProgram>
    </owl:NamedIndividual>
    


    <!-- http://xworks.gr/ontologies/ccso#CS370/CS_BSc/CSD/SSE/UoC -->

    <owl:NamedIndividual rdf:about="http://xworks.gr/ontologies/ccso#CS370/CS_BSc/CSD/SSE/UoC">
        <rdf:type rdf:resource="http://xworks.gr/ontologies/ccso#Course"/>
        <coversKA rdf:resource="http://xworks.gr/ontologies/ccso#CS/NC_Networking_and_Communication"/>
        <hasPrerequisite rdf:resource="http://xworks.gr/ontologies/ccso#CS215/CS_BSc/CSD/SSE/UoC"/>
        <hasSyllabus rdf:resource="http://xworks.gr/ontologies/ccso#CS370s1/CS_BSc/CSD/SSE/UoC"/>
        <includedIn rdf:resource="http://xworks.gr/ontologies/ccso#BSc_Computer_Science/CS_BSc/CSD/SSE/UoC"/>
        <offeredBy rdf:resource="http://xworks.gr/ontologies/ccso#Computers_Sciences_Department_of_University_of_Crete"/>
        <courseType rdf:datatype="http://www.w3.org/2001/XMLSchema#string">Elective</courseType>
        <csName rdf:datatype="http://www.w3.org/2001/XMLSchema#string">Digital Signal Processing</csName>
    </owl:NamedIndividual>
    


    <!-- http://xworks.gr/ontologies/ccso#CS370s1/CS_BSc/CSD/SSE/UoC -->

    <owl:NamedIndividual rdf:about="http://xworks.gr/ontologies/ccso#CS370s1/CS_BSc/CSD/SSE/UoC">
        <rdf:type rdf:resource="http://xworks.gr/ontologies/ccso#Syllabus"/>
        <syllabusOf rdf:resource="http://xworks.gr/ontologies/ccso#CS370/CS_BSc/CSD/SSE/UoC"/>
        <courseType rdf:datatype="http://www.w3.org/2001/XMLSchema#string">Elective</courseType>
        <creditsECTS rdf:datatype="http://www.w3.org/2001/XMLSchema#short">6</creditsECTS>
        <csName rdf:datatype="http://www.w3.org/2001/XMLSchema#string">Syllabus of course CS370 Digital Signal Processing</csName>
        <semesterinProgram rdf:datatype="http://www.w3.org/2001/XMLSchema#short">5</semesterinProgram>
    </owl:NamedIndividual>
    


    <!-- http://xworks.gr/ontologies/ccso#CS371/CS_BSc/CSD/SSE/UoC -->

    <owl:NamedIndividual rdf:about="http://xworks.gr/ontologies/ccso#CS371/CS_BSc/CSD/SSE/UoC">
        <rdf:type rdf:resource="http://xworks.gr/ontologies/ccso#Course"/>
        <hasPrerequisite rdf:resource="http://xworks.gr/ontologies/ccso#CS119/CS_BSc/CSD/SSE/UoC"/>
        <hasSyllabus rdf:resource="http://xworks.gr/ontologies/ccso#CS371s1/CS_BSc/CSD/SSE/UoC"/>
        <includedIn rdf:resource="http://xworks.gr/ontologies/ccso#BSc_Computer_Science/CS_BSc/CSD/SSE/UoC"/>
        <offeredBy rdf:resource="http://xworks.gr/ontologies/ccso#Computers_Sciences_Department_of_University_of_Crete"/>
        <courseType rdf:datatype="http://www.w3.org/2001/XMLSchema#string">Elective</courseType>
        <csName rdf:datatype="http://www.w3.org/2001/XMLSchema#string">Digital Image Processing</csName>
    </owl:NamedIndividual>
    


    <!-- http://xworks.gr/ontologies/ccso#CS371s1/CS_BSc/CSD/SSE/UoC -->

    <owl:NamedIndividual rdf:about="http://xworks.gr/ontologies/ccso#CS371s1/CS_BSc/CSD/SSE/UoC">
        <rdf:type rdf:resource="http://xworks.gr/ontologies/ccso#Syllabus"/>
        <syllabusOf rdf:resource="http://xworks.gr/ontologies/ccso#CS371/CS_BSc/CSD/SSE/UoC"/>
        <courseType rdf:datatype="http://www.w3.org/2001/XMLSchema#string">Elective</courseType>
        <creditsECTS rdf:datatype="http://www.w3.org/2001/XMLSchema#short">6</creditsECTS>
        <csName rdf:datatype="http://www.w3.org/2001/XMLSchema#string">Syllabus of course CS371 Digital Image Processing</csName>
        <semesterinProgram rdf:datatype="http://www.w3.org/2001/XMLSchema#short">6</semesterinProgram>
    </owl:NamedIndividual>
    


    <!-- http://xworks.gr/ontologies/ccso#CS380/CS_BSc/CSD/SSE/UoC -->

    <owl:NamedIndividual rdf:about="http://xworks.gr/ontologies/ccso#CS380/CS_BSc/CSD/SSE/UoC">
        <rdf:type rdf:resource="http://xworks.gr/ontologies/ccso#Course"/>
        <coversKA rdf:resource="http://xworks.gr/ontologies/ccso#CS/PL_Programming_Languages"/>
        <hasPrerequisite rdf:resource="http://xworks.gr/ontologies/ccso#CS118/CS_BSc/CSD/SSE/UoC"/>
        <hasPrerequisite rdf:resource="http://xworks.gr/ontologies/ccso#CS240/CS_BSc/CSD/SSE/UoC"/>
        <hasSyllabus rdf:resource="http://xworks.gr/ontologies/ccso#CS380s1/CS_BSc/CSD/SSE/UoC"/>
        <includedIn rdf:resource="http://xworks.gr/ontologies/ccso#BSc_Computer_Science/CS_BSc/CSD/SSE/UoC"/>
        <offeredBy rdf:resource="http://xworks.gr/ontologies/ccso#Computers_Sciences_Department_of_University_of_Crete"/>
        <courseType rdf:datatype="http://www.w3.org/2001/XMLSchema#string">Core</courseType>
        <csName rdf:datatype="http://www.w3.org/2001/XMLSchema#string">Algorithms and Complexity</csName>
    </owl:NamedIndividual>
    


    <!-- http://xworks.gr/ontologies/ccso#CS380s1/CS_BSc/CSD/SSE/UoC -->

    <owl:NamedIndividual rdf:about="http://xworks.gr/ontologies/ccso#CS380s1/CS_BSc/CSD/SSE/UoC">
        <rdf:type rdf:resource="http://xworks.gr/ontologies/ccso#Syllabus"/>
        <affiliatedWith rdf:resource="http://xworks.gr/ontologies/ccso#Gramma_Joanna"/>
        <affiliatedWith rdf:resource="http://xworks.gr/ontologies/ccso#Tollis_Ioannis"/>
        <hasCourseAssistant rdf:resource="http://xworks.gr/ontologies/ccso#Gramma_Joanna"/>
        <hasInstructor rdf:resource="http://xworks.gr/ontologies/ccso#Tollis_Ioannis"/>
        <hasSupervisor rdf:resource="http://xworks.gr/ontologies/ccso#Tollis_Ioannis"/>
        <syllabusOf rdf:resource="http://xworks.gr/ontologies/ccso#CS380/CS_BSc/CSD/SSE/UoC"/>
        <courseType rdf:datatype="http://www.w3.org/2001/XMLSchema#string">Core</courseType>
        <creditsECTS rdf:datatype="http://www.w3.org/2001/XMLSchema#short">8</creditsECTS>
        <csName rdf:datatype="http://www.w3.org/2001/XMLSchema#string">Syllabus of course CS380 Algorithms and Complexity</csName>
        <semesterinProgram rdf:datatype="http://www.w3.org/2001/XMLSchema#short">5</semesterinProgram>
    </owl:NamedIndividual>
    


    <!-- http://xworks.gr/ontologies/ccso#CS383/CS_BSc/CSD/SSE/UoC -->

    <owl:NamedIndividual rdf:about="http://xworks.gr/ontologies/ccso#CS383/CS_BSc/CSD/SSE/UoC">
        <rdf:type rdf:resource="http://xworks.gr/ontologies/ccso#Course"/>
        <hasPrerequisite rdf:resource="http://xworks.gr/ontologies/ccso#CS118/CS_BSc/CSD/SSE/UoC"/>
        <hasPrerequisite rdf:resource="http://xworks.gr/ontologies/ccso#CS240/CS_BSc/CSD/SSE/UoC"/>
        <hasSyllabus rdf:resource="http://xworks.gr/ontologies/ccso#CS383s1/CS_BSc/CSD/SSE/UoC"/>
        <includedIn rdf:resource="http://xworks.gr/ontologies/ccso#BSc_Computer_Science/CS_BSc/CSD/SSE/UoC"/>
        <offeredBy rdf:resource="http://xworks.gr/ontologies/ccso#Computers_Sciences_Department_of_University_of_Crete"/>
        <courseType rdf:datatype="http://www.w3.org/2001/XMLSchema#string">Elective</courseType>
        <csName rdf:datatype="http://www.w3.org/2001/XMLSchema#string">Complex Network Dynamics</csName>
    </owl:NamedIndividual>
    


    <!-- http://xworks.gr/ontologies/ccso#CS383s1/CS_BSc/CSD/SSE/UoC -->

    <owl:NamedIndividual rdf:about="http://xworks.gr/ontologies/ccso#CS383s1/CS_BSc/CSD/SSE/UoC">
        <rdf:type rdf:resource="http://xworks.gr/ontologies/ccso#Syllabus"/>
        <syllabusOf rdf:resource="http://xworks.gr/ontologies/ccso#CS383/CS_BSc/CSD/SSE/UoC"/>
        <courseType rdf:datatype="http://www.w3.org/2001/XMLSchema#string">Elective</courseType>
        <creditsECTS rdf:datatype="http://www.w3.org/2001/XMLSchema#short">6</creditsECTS>
        <csName rdf:datatype="http://www.w3.org/2001/XMLSchema#string">Syllabus of course CS383 Complex Network Dynamics</csName>
        <semesterinProgram rdf:datatype="http://www.w3.org/2001/XMLSchema#short">6</semesterinProgram>
    </owl:NamedIndividual>
    


    <!-- http://xworks.gr/ontologies/ccso#CS387/CS_BSc/CSD/SSE/UoC -->

    <owl:NamedIndividual rdf:about="http://xworks.gr/ontologies/ccso#CS387/CS_BSc/CSD/SSE/UoC">
        <rdf:type rdf:resource="http://xworks.gr/ontologies/ccso#Course"/>
        <coversKA rdf:resource="http://xworks.gr/ontologies/ccso#CS/PL_Programming_Languages"/>
        <hasPrerequisite rdf:resource="http://xworks.gr/ontologies/ccso#CS180/CS_BSc/CSD/SSE/UoC"/>
        <hasPrerequisite rdf:resource="http://xworks.gr/ontologies/ccso#CS240/CS_BSc/CSD/SSE/UoC"/>
        <hasSyllabus rdf:resource="http://xworks.gr/ontologies/ccso#CS387s1/CS_BSc/CSD/SSE/UoC"/>
        <includedIn rdf:resource="http://xworks.gr/ontologies/ccso#BSc_Computer_Science/CS_BSc/CSD/SSE/UoC"/>
        <offeredBy rdf:resource="http://xworks.gr/ontologies/ccso#Computers_Sciences_Department_of_University_of_Crete"/>
        <courseType rdf:datatype="http://www.w3.org/2001/XMLSchema#string">Elective</courseType>
        <csName rdf:datatype="http://www.w3.org/2001/XMLSchema#string">Introduction to Artificial Intelligence</csName>
    </owl:NamedIndividual>
    


    <!-- http://xworks.gr/ontologies/ccso#CS387s1/CS_BSc/CSD/SSE/UoC -->

    <owl:NamedIndividual rdf:about="http://xworks.gr/ontologies/ccso#CS387s1/CS_BSc/CSD/SSE/UoC">
        <rdf:type rdf:resource="http://xworks.gr/ontologies/ccso#Syllabus"/>
        <syllabusOf rdf:resource="http://xworks.gr/ontologies/ccso#CS387/CS_BSc/CSD/SSE/UoC"/>
        <courseType rdf:datatype="http://www.w3.org/2001/XMLSchema#string">Elective</courseType>
        <creditsECTS rdf:datatype="http://www.w3.org/2001/XMLSchema#short">6</creditsECTS>
        <csName rdf:datatype="http://www.w3.org/2001/XMLSchema#string">Syllabus of course CS387 Introduction to Artificial Intelligence</csName>
        <semesterinProgram rdf:datatype="http://www.w3.org/2001/XMLSchema#short">6</semesterinProgram>
    </owl:NamedIndividual>
    


    <!-- http://xworks.gr/ontologies/ccso#CS404/CS_BSc/CSD/SSE/UoC -->

    <owl:NamedIndividual rdf:about="http://xworks.gr/ontologies/ccso#CS404/CS_BSc/CSD/SSE/UoC">
        <rdf:type rdf:resource="http://xworks.gr/ontologies/ccso#Course"/>
        <hasSyllabus rdf:resource="http://xworks.gr/ontologies/ccso#CS404s1/CS_BSc/CSD/SSE/UoC"/>
        <includedIn rdf:resource="http://xworks.gr/ontologies/ccso#BSc_Computer_Science/CS_BSc/CSD/SSE/UoC"/>
        <offeredBy rdf:resource="http://xworks.gr/ontologies/ccso#Computers_Sciences_Department_of_University_of_Crete"/>
        <courseType rdf:datatype="http://www.w3.org/2001/XMLSchema#string">Elective</courseType>
        <csName rdf:datatype="http://www.w3.org/2001/XMLSchema#string">Small Business Management - Entrepreneurship</csName>
    </owl:NamedIndividual>
    


    <!-- http://xworks.gr/ontologies/ccso#CS404s1/CS_BSc/CSD/SSE/UoC -->

    <owl:NamedIndividual rdf:about="http://xworks.gr/ontologies/ccso#CS404s1/CS_BSc/CSD/SSE/UoC">
        <rdf:type rdf:resource="http://xworks.gr/ontologies/ccso#Syllabus"/>
        <syllabusOf rdf:resource="http://xworks.gr/ontologies/ccso#CS404/CS_BSc/CSD/SSE/UoC"/>
        <courseType rdf:datatype="http://www.w3.org/2001/XMLSchema#string">Elective</courseType>
        <creditsECTS rdf:datatype="http://www.w3.org/2001/XMLSchema#short">6</creditsECTS>
        <csName rdf:datatype="http://www.w3.org/2001/XMLSchema#string">Syllabus of course CS404 Small Business Management - Entrepreneurship</csName>
        <semesterinProgram rdf:datatype="http://www.w3.org/2001/XMLSchema#short">8</semesterinProgram>
    </owl:NamedIndividual>
    


    <!-- http://xworks.gr/ontologies/ccso#CS408/CS_BSc/CSD/SSE/UoC -->

    <owl:NamedIndividual rdf:about="http://xworks.gr/ontologies/ccso#CS408/CS_BSc/CSD/SSE/UoC">
        <rdf:type rdf:resource="http://xworks.gr/ontologies/ccso#Course"/>
        <hasSyllabus rdf:resource="http://xworks.gr/ontologies/ccso#CS408s1/CS_BSc/CSD/SSE/UoC"/>
        <courseType rdf:datatype="http://www.w3.org/2001/XMLSchema#string">Elective</courseType>
        <csName rdf:datatype="http://www.w3.org/2001/XMLSchema#string">Principles of Distributed Computing</csName>
    </owl:NamedIndividual>
    


    <!-- http://xworks.gr/ontologies/ccso#CS408s1/CS_BSc/CSD/SSE/UoC -->

    <owl:NamedIndividual rdf:about="http://xworks.gr/ontologies/ccso#CS408s1/CS_BSc/CSD/SSE/UoC">
        <rdf:type rdf:resource="http://xworks.gr/ontologies/ccso#Syllabus"/>
        <syllabusOf rdf:resource="http://xworks.gr/ontologies/ccso#CS408/CS_BSc/CSD/SSE/UoC"/>
        <courseType rdf:datatype="http://www.w3.org/2001/XMLSchema#string">Elective</courseType>
        <creditsECTS rdf:datatype="http://www.w3.org/2001/XMLSchema#short">6</creditsECTS>
        <csName rdf:datatype="http://www.w3.org/2001/XMLSchema#string">Syllabus of course CS408 Technological Innovation and Entrepreneurship</csName>
        <semesterinProgram rdf:datatype="http://www.w3.org/2001/XMLSchema#short">7</semesterinProgram>
    </owl:NamedIndividual>
    


    <!-- http://xworks.gr/ontologies/ccso#CS422/CS_BSc/CSD/SSE/UoC -->

    <owl:NamedIndividual rdf:about="http://xworks.gr/ontologies/ccso#CS422/CS_BSc/CSD/SSE/UoC">
        <rdf:type rdf:resource="http://xworks.gr/ontologies/ccso#Course"/>
        <coversKA rdf:resource="http://xworks.gr/ontologies/ccso#CS/HW_Hardware_and_Computer_Systems"/>
        <hasPrerequisite rdf:resource="http://xworks.gr/ontologies/ccso#CS225/CS_BSc/CSD/SSE/UoC"/>
        <hasSyllabus rdf:resource="http://xworks.gr/ontologies/ccso#CS422s1/CS_BSc/CSD/SSE/UoC"/>
        <includedIn rdf:resource="http://xworks.gr/ontologies/ccso#BSc_Computer_Science/CS_BSc/CSD/SSE/UoC"/>
        <offeredBy rdf:resource="http://xworks.gr/ontologies/ccso#Computers_Sciences_Department_of_University_of_Crete"/>
        <courseType rdf:datatype="http://www.w3.org/2001/XMLSchema#string">Elective</courseType>
        <csName rdf:datatype="http://www.w3.org/2001/XMLSchema#string">Introduction to VLSI Systems</csName>
    </owl:NamedIndividual>
    


    <!-- http://xworks.gr/ontologies/ccso#CS422s1/CS_BSc/CSD/SSE/UoC -->

    <owl:NamedIndividual rdf:about="http://xworks.gr/ontologies/ccso#CS422s1/CS_BSc/CSD/SSE/UoC">
        <rdf:type rdf:resource="http://xworks.gr/ontologies/ccso#Syllabus"/>
        <syllabusOf rdf:resource="http://xworks.gr/ontologies/ccso#CS422/CS_BSc/CSD/SSE/UoC"/>
        <courseType rdf:datatype="http://www.w3.org/2001/XMLSchema#string">Elective</courseType>
        <creditsECTS rdf:datatype="http://www.w3.org/2001/XMLSchema#short">6</creditsECTS>
        <csName rdf:datatype="http://www.w3.org/2001/XMLSchema#string">Syllabus of course CS422 Introduction to VLSI Systems</csName>
        <semesterinProgram rdf:datatype="http://www.w3.org/2001/XMLSchema#short">7</semesterinProgram>
    </owl:NamedIndividual>
    


    <!-- http://xworks.gr/ontologies/ccso#CS425/CS_BSc/CSD/SSE/UoC -->

    <owl:NamedIndividual rdf:about="http://xworks.gr/ontologies/ccso#CS425/CS_BSc/CSD/SSE/UoC">
        <rdf:type rdf:resource="http://xworks.gr/ontologies/ccso#Course"/>
        <coversKA rdf:resource="http://xworks.gr/ontologies/ccso#CS/HW_Hardware_and_Computer_Systems"/>
        <hasPrerequisite rdf:resource="http://xworks.gr/ontologies/ccso#CS225/CS_BSc/CSD/SSE/UoC"/>
        <hasSyllabus rdf:resource="http://xworks.gr/ontologies/ccso#CS425s1/CS_BSc/CSD/SSE/UoC"/>
        <includedIn rdf:resource="http://xworks.gr/ontologies/ccso#BSc_Computer_Science/CS_BSc/CSD/SSE/UoC"/>
        <offeredBy rdf:resource="http://xworks.gr/ontologies/ccso#Computers_Sciences_Department_of_University_of_Crete"/>
        <courseType rdf:datatype="http://www.w3.org/2001/XMLSchema#string">Elective</courseType>
        <csName rdf:datatype="http://www.w3.org/2001/XMLSchema#string">Computer Systems Architecture</csName>
    </owl:NamedIndividual>
    


    <!-- http://xworks.gr/ontologies/ccso#CS425s1/CS_BSc/CSD/SSE/UoC -->

    <owl:NamedIndividual rdf:about="http://xworks.gr/ontologies/ccso#CS425s1/CS_BSc/CSD/SSE/UoC">
        <rdf:type rdf:resource="http://xworks.gr/ontologies/ccso#Syllabus"/>
        <syllabusOf rdf:resource="http://xworks.gr/ontologies/ccso#CS425/CS_BSc/CSD/SSE/UoC"/>
        <courseType rdf:datatype="http://www.w3.org/2001/XMLSchema#string">Elective</courseType>
        <creditsECTS rdf:datatype="http://www.w3.org/2001/XMLSchema#short">6</creditsECTS>
        <csName rdf:datatype="http://www.w3.org/2001/XMLSchema#string">Syllabus of course CS425 Computer Systems Architecture</csName>
        <semesterinProgram rdf:datatype="http://www.w3.org/2001/XMLSchema#short">8</semesterinProgram>
    </owl:NamedIndividual>
    


    <!-- http://xworks.gr/ontologies/ccso#CS428/CS_BSc/CSD/SSE/UoC -->

    <owl:NamedIndividual rdf:about="http://xworks.gr/ontologies/ccso#CS428/CS_BSc/CSD/SSE/UoC">
        <rdf:type rdf:resource="http://xworks.gr/ontologies/ccso#Course"/>
        <coversKA rdf:resource="http://xworks.gr/ontologies/ccso#CS/HW_Hardware_and_Computer_Systems"/>
        <hasPrerequisite rdf:resource="http://xworks.gr/ontologies/ccso#CS225/CS_BSc/CSD/SSE/UoC"/>
        <hasSyllabus rdf:resource="http://xworks.gr/ontologies/ccso#CS428s1/CS_BSc/CSD/SSE/UoC"/>
        <includedIn rdf:resource="http://xworks.gr/ontologies/ccso#BSc_Computer_Science/CS_BSc/CSD/SSE/UoC"/>
        <offeredBy rdf:resource="http://xworks.gr/ontologies/ccso#Computers_Sciences_Department_of_University_of_Crete"/>
        <courseType rdf:datatype="http://www.w3.org/2001/XMLSchema#string">Elective</courseType>
        <csName rdf:datatype="http://www.w3.org/2001/XMLSchema#string">Microprocessors and Peripherals Laboratory</csName>
    </owl:NamedIndividual>
    


    <!-- http://xworks.gr/ontologies/ccso#CS428s1/CS_BSc/CSD/SSE/UoC -->

    <owl:NamedIndividual rdf:about="http://xworks.gr/ontologies/ccso#CS428s1/CS_BSc/CSD/SSE/UoC">
        <rdf:type rdf:resource="http://xworks.gr/ontologies/ccso#Syllabus"/>
        <syllabusOf rdf:resource="http://xworks.gr/ontologies/ccso#CS428/CS_BSc/CSD/SSE/UoC"/>
        <courseType rdf:datatype="http://www.w3.org/2001/XMLSchema#string">Elective</courseType>
        <creditsECTS rdf:datatype="http://www.w3.org/2001/XMLSchema#short">6</creditsECTS>
        <csName rdf:datatype="http://www.w3.org/2001/XMLSchema#string">Syllabus of course CS428 Microprocessors and Peripherals Laboratory</csName>
        <semesterinProgram rdf:datatype="http://www.w3.org/2001/XMLSchema#short">8</semesterinProgram>
    </owl:NamedIndividual>
    


    <!-- http://xworks.gr/ontologies/ccso#CS435/CS_BSc/CSD/SSE/UoC -->

    <owl:NamedIndividual rdf:about="http://xworks.gr/ontologies/ccso#CS435/CS_BSc/CSD/SSE/UoC">
        <rdf:type rdf:resource="http://xworks.gr/ontologies/ccso#Course"/>
        <coversKA rdf:resource="http://xworks.gr/ontologies/ccso#CS/NC_Networking_and_Communication"/>
        <hasPrerequisite rdf:resource="http://xworks.gr/ontologies/ccso#CS335/CS_BSc/CSD/SSE/UoC"/>
        <hasSyllabus rdf:resource="http://xworks.gr/ontologies/ccso#CS435s1/CS_BSc/CSD/SSE/UoC"/>
        <includedIn rdf:resource="http://xworks.gr/ontologies/ccso#BSc_Computer_Science/CS_BSc/CSD/SSE/UoC"/>
        <offeredBy rdf:resource="http://xworks.gr/ontologies/ccso#Computers_Sciences_Department_of_University_of_Crete"/>
        <courseType rdf:datatype="http://www.w3.org/2001/XMLSchema#string">Elective</courseType>
        <csName rdf:datatype="http://www.w3.org/2001/XMLSchema#string">Network Technology &amp; Programming Lab</csName>
    </owl:NamedIndividual>
    


    <!-- http://xworks.gr/ontologies/ccso#CS435s1/CS_BSc/CSD/SSE/UoC -->

    <owl:NamedIndividual rdf:about="http://xworks.gr/ontologies/ccso#CS435s1/CS_BSc/CSD/SSE/UoC">
        <rdf:type rdf:resource="http://xworks.gr/ontologies/ccso#Syllabus"/>
        <aimsToLO rdf:resource="http://xworks.gr/ontologies/ccso#CS/NC/LAN/LO_Describe_how_frames_are_forwarded_in_an_Ethernet_network"/>
        <aimsToLO rdf:resource="http://xworks.gr/ontologies/ccso#CS/NC/LAN/LO_Describe_the_interrelations_between_IP_and_Ethernet"/>
        <aimsToLO rdf:resource="http://xworks.gr/ontologies/ccso#CS/NC/LAN/LO_Describe_the_steps_used_in_one_common_approach_to_the_multiple_access_problem"/>
        <aimsToLO rdf:resource="http://xworks.gr/ontologies/ccso#CS/NC/LAN/LO_Identify_the_differences_between_IP_and_Ethernet"/>
        <coversTopic rdf:resource="http://xworks.gr/ontologies/ccso#CS/NC/LAN/T_Common_approaches_to_multiple_access"/>
        <coversTopic rdf:resource="http://xworks.gr/ontologies/ccso#CS/NC/LAN/T_Ethernet"/>
        <coversTopic rdf:resource="http://xworks.gr/ontologies/ccso#CS/NC/LAN/T_Local_Area_Networks"/>
        <coversTopic rdf:resource="http://xworks.gr/ontologies/ccso#CS/NC/LAN/T_Multiple_Access_Problem"/>
        <coversTopic rdf:resource="http://xworks.gr/ontologies/ccso#CS/NC/LAN/T_Switching"/>
        <syllabusOf rdf:resource="http://xworks.gr/ontologies/ccso#CS435/CS_BSc/CSD/SSE/UoC"/>
        <courseType rdf:datatype="http://www.w3.org/2001/XMLSchema#string">Elective</courseType>
        <creditsECTS rdf:datatype="http://www.w3.org/2001/XMLSchema#short">6</creditsECTS>
        <csName rdf:datatype="http://www.w3.org/2001/XMLSchema#string">Syllabus of course CS435 Network Technology &amp; Programming Lab</csName>
        <semesterinProgram rdf:datatype="http://www.w3.org/2001/XMLSchema#short">7</semesterinProgram>
    </owl:NamedIndividual>
    


    <!-- http://xworks.gr/ontologies/ccso#CS436/CS_BSc/CSD/SSE/UoC -->

    <owl:NamedIndividual rdf:about="http://xworks.gr/ontologies/ccso#CS436/CS_BSc/CSD/SSE/UoC">
        <rdf:type rdf:resource="http://xworks.gr/ontologies/ccso#Course"/>
        <coversKA rdf:resource="http://xworks.gr/ontologies/ccso#CS/NC_Networking_and_Communication"/>
        <hasPrerequisite rdf:resource="http://xworks.gr/ontologies/ccso#CS335/CS_BSc/CSD/SSE/UoC"/>
        <hasSyllabus rdf:resource="http://xworks.gr/ontologies/ccso#CS436s1/CS_BSc/CSD/SSE/UoC"/>
        <includedIn rdf:resource="http://xworks.gr/ontologies/ccso#BSc_Computer_Science/CS_BSc/CSD/SSE/UoC"/>
        <offeredBy rdf:resource="http://xworks.gr/ontologies/ccso#Computers_Sciences_Department_of_University_of_Crete"/>
        <courseType rdf:datatype="http://www.w3.org/2001/XMLSchema#string">Elective</courseType>
        <csName rdf:datatype="http://www.w3.org/2001/XMLSchema#string">Software Defined Networks (SDN)</csName>
    </owl:NamedIndividual>
    


    <!-- http://xworks.gr/ontologies/ccso#CS436s1/CS_BSc/CSD/SSE/UoC -->

    <owl:NamedIndividual rdf:about="http://xworks.gr/ontologies/ccso#CS436s1/CS_BSc/CSD/SSE/UoC">
        <rdf:type rdf:resource="http://xworks.gr/ontologies/ccso#Syllabus"/>
        <syllabusOf rdf:resource="http://xworks.gr/ontologies/ccso#CS436/CS_BSc/CSD/SSE/UoC"/>
        <courseType rdf:datatype="http://www.w3.org/2001/XMLSchema#string">Elective</courseType>
        <creditsECTS rdf:datatype="http://www.w3.org/2001/XMLSchema#short">6</creditsECTS>
        <csName rdf:datatype="http://www.w3.org/2001/XMLSchema#string">Syllabus of course CS436 Software Defined Networks (SDN)</csName>
        <semesterinProgram rdf:datatype="http://www.w3.org/2001/XMLSchema#short">7</semesterinProgram>
    </owl:NamedIndividual>
    


    <!-- http://xworks.gr/ontologies/ccso#CS439/CS_BSc/CSD/SSE/UoC -->

    <owl:NamedIndividual rdf:about="http://xworks.gr/ontologies/ccso#CS439/CS_BSc/CSD/SSE/UoC">
        <rdf:type rdf:resource="http://xworks.gr/ontologies/ccso#Course"/>
        <coversKA rdf:resource="http://xworks.gr/ontologies/ccso#CS/NC_Networking_and_Communication"/>
        <hasPrerequisite rdf:resource="http://xworks.gr/ontologies/ccso#CS335/CS_BSc/CSD/SSE/UoC"/>
        <hasSyllabus rdf:resource="http://xworks.gr/ontologies/ccso#CS439s1/CS_BSc/CSD/SSE/UoC"/>
        <includedIn rdf:resource="http://xworks.gr/ontologies/ccso#BSc_Computer_Science/CS_BSc/CSD/SSE/UoC"/>
        <offeredBy rdf:resource="http://xworks.gr/ontologies/ccso#Computers_Sciences_Department_of_University_of_Crete"/>
        <courseType rdf:datatype="http://www.w3.org/2001/XMLSchema#string">Elective</courseType>
        <csName rdf:datatype="http://www.w3.org/2001/XMLSchema#string">Wireless Networks and Moblile Computing</csName>
    </owl:NamedIndividual>
    


    <!-- http://xworks.gr/ontologies/ccso#CS439s1/CS_BSc/CSD/SSE/UoC -->

    <owl:NamedIndividual rdf:about="http://xworks.gr/ontologies/ccso#CS439s1/CS_BSc/CSD/SSE/UoC">
        <rdf:type rdf:resource="http://xworks.gr/ontologies/ccso#Syllabus"/>
        <syllabusOf rdf:resource="http://xworks.gr/ontologies/ccso#CS439/CS_BSc/CSD/SSE/UoC"/>
        <courseType rdf:datatype="http://www.w3.org/2001/XMLSchema#string">Elective</courseType>
        <creditsECTS rdf:datatype="http://www.w3.org/2001/XMLSchema#short">6</creditsECTS>
        <csName rdf:datatype="http://www.w3.org/2001/XMLSchema#string">Syllabus of course CS439 Wireless Networks and Moblile Computing</csName>
        <semesterinProgram rdf:datatype="http://www.w3.org/2001/XMLSchema#short">8</semesterinProgram>
    </owl:NamedIndividual>
    


    <!-- http://xworks.gr/ontologies/ccso#CS446/CS_BSc/CSD/SSE/UoC -->

    <owl:NamedIndividual rdf:about="http://xworks.gr/ontologies/ccso#CS446/CS_BSc/CSD/SSE/UoC">
        <rdf:type rdf:resource="http://xworks.gr/ontologies/ccso#Course"/>
        <coversKA rdf:resource="http://xworks.gr/ontologies/ccso#CS/HW_Hardware_and_Computer_Systems"/>
        <hasPrerequisite rdf:resource="http://xworks.gr/ontologies/ccso#CS252/CS_BSc/CSD/SSE/UoC"/>
        <hasPrerequisite rdf:resource="http://xworks.gr/ontologies/ccso#CS345/CS_BSc/CSD/SSE/UoC"/>
        <hasSyllabus rdf:resource="http://xworks.gr/ontologies/ccso#CS446s1/CS_BSc/CSD/SSE/UoC"/>
        <includedIn rdf:resource="http://xworks.gr/ontologies/ccso#BSc_Computer_Science/CS_BSc/CSD/SSE/UoC"/>
        <offeredBy rdf:resource="http://xworks.gr/ontologies/ccso#Computers_Sciences_Department_of_University_of_Crete"/>
        <courseType rdf:datatype="http://www.w3.org/2001/XMLSchema#string">Elective</courseType>
        <csName rdf:datatype="http://www.w3.org/2001/XMLSchema#string">Managed Runtime Systems</csName>
    </owl:NamedIndividual>
    


    <!-- http://xworks.gr/ontologies/ccso#CS446s1/CS_BSc/CSD/SSE/UoC -->

    <owl:NamedIndividual rdf:about="http://xworks.gr/ontologies/ccso#CS446s1/CS_BSc/CSD/SSE/UoC">
        <rdf:type rdf:resource="http://xworks.gr/ontologies/ccso#Syllabus"/>
        <syllabusOf rdf:resource="http://xworks.gr/ontologies/ccso#CS446/CS_BSc/CSD/SSE/UoC"/>
        <courseType rdf:datatype="http://www.w3.org/2001/XMLSchema#string">Elective</courseType>
        <creditsECTS rdf:datatype="http://www.w3.org/2001/XMLSchema#short">6</creditsECTS>
        <csName rdf:datatype="http://www.w3.org/2001/XMLSchema#string">Syllabus of course CS446 Managed Runtime Systems</csName>
        <semesterinProgram rdf:datatype="http://www.w3.org/2001/XMLSchema#short">7</semesterinProgram>
    </owl:NamedIndividual>
    


    <!-- http://xworks.gr/ontologies/ccso#CS452/CS_BSc/CSD/SSE/UoC -->

    <owl:NamedIndividual rdf:about="http://xworks.gr/ontologies/ccso#CS452/CS_BSc/CSD/SSE/UoC">
        <rdf:type rdf:resource="http://xworks.gr/ontologies/ccso#Course"/>
        <coversKA rdf:resource="http://xworks.gr/ontologies/ccso#CS/SW_Software_Engineering_Software_Systems_and_Applications"/>
        <hasSyllabus rdf:resource="http://xworks.gr/ontologies/ccso#CS452s1/CS_BSc/CSD/SSE/UoC"/>
        <includedIn rdf:resource="http://xworks.gr/ontologies/ccso#BSc_Computer_Science/CS_BSc/CSD/SSE/UoC"/>
        <offeredBy rdf:resource="http://xworks.gr/ontologies/ccso#Computers_Sciences_Department_of_University_of_Crete"/>
        <courseType rdf:datatype="http://www.w3.org/2001/XMLSchema#string">Elective</courseType>
        <csName rdf:datatype="http://www.w3.org/2001/XMLSchema#string">Introduction to science and technology of Services</csName>
    </owl:NamedIndividual>
    


    <!-- http://xworks.gr/ontologies/ccso#CS452s1/CS_BSc/CSD/SSE/UoC -->

    <owl:NamedIndividual rdf:about="http://xworks.gr/ontologies/ccso#CS452s1/CS_BSc/CSD/SSE/UoC">
        <rdf:type rdf:resource="http://xworks.gr/ontologies/ccso#Syllabus"/>
        <syllabusOf rdf:resource="http://xworks.gr/ontologies/ccso#CS452/CS_BSc/CSD/SSE/UoC"/>
        <courseType rdf:datatype="http://www.w3.org/2001/XMLSchema#string">Elective</courseType>
        <creditsECTS rdf:datatype="http://www.w3.org/2001/XMLSchema#short">6</creditsECTS>
        <csName rdf:datatype="http://www.w3.org/2001/XMLSchema#string">Syllabus of course CS452 Introduction to science and technology of Services</csName>
        <semesterinProgram rdf:datatype="http://www.w3.org/2001/XMLSchema#short">8</semesterinProgram>
    </owl:NamedIndividual>
    


    <!-- http://xworks.gr/ontologies/ccso#CS455/CS_BSc/CSD/SSE/UoC -->

    <owl:NamedIndividual rdf:about="http://xworks.gr/ontologies/ccso#CS455/CS_BSc/CSD/SSE/UoC">
        <rdf:type rdf:resource="http://xworks.gr/ontologies/ccso#Course"/>
        <coversKA rdf:resource="http://xworks.gr/ontologies/ccso#CS/SW_Software_Engineering_Software_Systems_and_Applications"/>
        <hasPrerequisite rdf:resource="http://xworks.gr/ontologies/ccso#CS335/CS_BSc/CSD/SSE/UoC"/>
        <hasPrerequisite rdf:resource="http://xworks.gr/ontologies/ccso#CS345/CS_BSc/CSD/SSE/UoC"/>
        <hasSyllabus rdf:resource="http://xworks.gr/ontologies/ccso#CS455s1/CS_BSc/CSD/SSE/UoC"/>
        <includedIn rdf:resource="http://xworks.gr/ontologies/ccso#BSc_Computer_Science/CS_BSc/CSD/SSE/UoC"/>
        <offeredBy rdf:resource="http://xworks.gr/ontologies/ccso#Computers_Sciences_Department_of_University_of_Crete"/>
        <courseType rdf:datatype="http://www.w3.org/2001/XMLSchema#string">Elective</courseType>
        <csName rdf:datatype="http://www.w3.org/2001/XMLSchema#string">Internet Attacks</csName>
    </owl:NamedIndividual>
    


    <!-- http://xworks.gr/ontologies/ccso#CS455s1/CS_BSc/CSD/SSE/UoC -->

    <owl:NamedIndividual rdf:about="http://xworks.gr/ontologies/ccso#CS455s1/CS_BSc/CSD/SSE/UoC">
        <rdf:type rdf:resource="http://xworks.gr/ontologies/ccso#Syllabus"/>
        <syllabusOf rdf:resource="http://xworks.gr/ontologies/ccso#CS455/CS_BSc/CSD/SSE/UoC"/>
        <courseType rdf:datatype="http://www.w3.org/2001/XMLSchema#string">Elective</courseType>
        <creditsECTS rdf:datatype="http://www.w3.org/2001/XMLSchema#short">6</creditsECTS>
        <csName rdf:datatype="http://www.w3.org/2001/XMLSchema#string">Syllabus of course CS455 Internet Attacks</csName>
        <semesterinProgram rdf:datatype="http://www.w3.org/2001/XMLSchema#short">8</semesterinProgram>
    </owl:NamedIndividual>
    


    <!-- http://xworks.gr/ontologies/ccso#CS457/CS_BSc/CSD/SSE/UoC -->

    <owl:NamedIndividual rdf:about="http://xworks.gr/ontologies/ccso#CS457/CS_BSc/CSD/SSE/UoC">
        <rdf:type rdf:resource="http://xworks.gr/ontologies/ccso#Course"/>
        <coversKA rdf:resource="http://xworks.gr/ontologies/ccso#CS/SW_Software_Engineering_Software_Systems_and_Applications"/>
        <hasPrerequisite rdf:resource="http://xworks.gr/ontologies/ccso#CS150/CS_BSc/CSD/SSE/UoC"/>
        <hasSyllabus rdf:resource="http://xworks.gr/ontologies/ccso#CS457s1/CS_BSc/CSD/SSE/UoC"/>
        <includedIn rdf:resource="http://xworks.gr/ontologies/ccso#BSc_Computer_Science/CS_BSc/CSD/SSE/UoC"/>
        <offeredBy rdf:resource="http://xworks.gr/ontologies/ccso#Computers_Sciences_Department_of_University_of_Crete"/>
        <courseType rdf:datatype="http://www.w3.org/2001/XMLSchema#string">Elective</courseType>
        <csName rdf:datatype="http://www.w3.org/2001/XMLSchema#string">Introduction to Secure Systems</csName>
    </owl:NamedIndividual>
    


    <!-- http://xworks.gr/ontologies/ccso#CS457s1/CS_BSc/CSD/SSE/UoC -->

    <owl:NamedIndividual rdf:about="http://xworks.gr/ontologies/ccso#CS457s1/CS_BSc/CSD/SSE/UoC">
        <rdf:type rdf:resource="http://xworks.gr/ontologies/ccso#Syllabus"/>
        <syllabusOf rdf:resource="http://xworks.gr/ontologies/ccso#CS457/CS_BSc/CSD/SSE/UoC"/>
        <courseType rdf:datatype="http://www.w3.org/2001/XMLSchema#string">Elective</courseType>
        <creditsECTS rdf:datatype="http://www.w3.org/2001/XMLSchema#short">6</creditsECTS>
        <csName rdf:datatype="http://www.w3.org/2001/XMLSchema#string">Syllabus of course CS457 Introduction to Secure Systems</csName>
        <semesterinProgram rdf:datatype="http://www.w3.org/2001/XMLSchema#short">7</semesterinProgram>
    </owl:NamedIndividual>
    


    <!-- http://xworks.gr/ontologies/ccso#CS459/CS_BSc/CSD/SSE/UoC -->

    <owl:NamedIndividual rdf:about="http://xworks.gr/ontologies/ccso#CS459/CS_BSc/CSD/SSE/UoC">
        <rdf:type rdf:resource="http://xworks.gr/ontologies/ccso#Course"/>
        <coversKA rdf:resource="http://xworks.gr/ontologies/ccso#CS/SW_Software_Engineering_Software_Systems_and_Applications"/>
        <hasPrerequisite rdf:resource="http://xworks.gr/ontologies/ccso#CS345/CS_BSc/CSD/SSE/UoC"/>
        <hasSyllabus rdf:resource="http://xworks.gr/ontologies/ccso#CS459s1/CS_BSc/CSD/SSE/UoC"/>
        <includedIn rdf:resource="http://xworks.gr/ontologies/ccso#BSc_Computer_Science/CS_BSc/CSD/SSE/UoC"/>
        <offeredBy rdf:resource="http://xworks.gr/ontologies/ccso#Computers_Sciences_Department_of_University_of_Crete"/>
        <courseType rdf:datatype="http://www.w3.org/2001/XMLSchema#string">Elective</courseType>
        <csName rdf:datatype="http://www.w3.org/2001/XMLSchema#string">Internet Measurement and Monitoring</csName>
    </owl:NamedIndividual>
    


    <!-- http://xworks.gr/ontologies/ccso#CS459s1/CS_BSc/CSD/SSE/UoC -->

    <owl:NamedIndividual rdf:about="http://xworks.gr/ontologies/ccso#CS459s1/CS_BSc/CSD/SSE/UoC">
        <rdf:type rdf:resource="http://xworks.gr/ontologies/ccso#Syllabus"/>
        <syllabusOf rdf:resource="http://xworks.gr/ontologies/ccso#CS459/CS_BSc/CSD/SSE/UoC"/>
        <courseType rdf:datatype="http://www.w3.org/2001/XMLSchema#string">Elective</courseType>
        <creditsECTS rdf:datatype="http://www.w3.org/2001/XMLSchema#short">6</creditsECTS>
        <csName rdf:datatype="http://www.w3.org/2001/XMLSchema#string">Syllabus of course CS459 Internet Measurement and Monitoring</csName>
        <semesterinProgram rdf:datatype="http://www.w3.org/2001/XMLSchema#short">8</semesterinProgram>
    </owl:NamedIndividual>
    


    <!-- http://xworks.gr/ontologies/ccso#CS460/CS_BSc/CSD/SSE/UoC -->

    <owl:NamedIndividual rdf:about="http://xworks.gr/ontologies/ccso#CS460/CS_BSc/CSD/SSE/UoC">
        <rdf:type rdf:resource="http://xworks.gr/ontologies/ccso#Course"/>
        <hasPrerequisite rdf:resource="http://xworks.gr/ontologies/ccso#CS360/CS_BSc/CSD/SSE/UoC"/>
        <hasSyllabus rdf:resource="http://xworks.gr/ontologies/ccso#CS460s1/CS_BSc/CSD/SSE/UoC"/>
        <includedIn rdf:resource="http://xworks.gr/ontologies/ccso#BSc_Computer_Science/CS_BSc/CSD/SSE/UoC"/>
        <offeredBy rdf:resource="http://xworks.gr/ontologies/ccso#Computers_Sciences_Department_of_University_of_Crete"/>
        <courseType rdf:datatype="http://www.w3.org/2001/XMLSchema#string">Elective</courseType>
        <csName rdf:datatype="http://www.w3.org/2001/XMLSchema#string">Database Management Systems</csName>
    </owl:NamedIndividual>
    


    <!-- http://xworks.gr/ontologies/ccso#CS460s1/CS_BSc/CSD/SSE/UoC -->

    <owl:NamedIndividual rdf:about="http://xworks.gr/ontologies/ccso#CS460s1/CS_BSc/CSD/SSE/UoC">
        <rdf:type rdf:resource="http://xworks.gr/ontologies/ccso#Syllabus"/>
        <syllabusOf rdf:resource="http://xworks.gr/ontologies/ccso#CS460/CS_BSc/CSD/SSE/UoC"/>
        <courseType rdf:datatype="http://www.w3.org/2001/XMLSchema#string">Elective</courseType>
        <creditsECTS rdf:datatype="http://www.w3.org/2001/XMLSchema#short">6</creditsECTS>
        <csName rdf:datatype="http://www.w3.org/2001/XMLSchema#string">Syllabus of course CS460 Database Management Systems</csName>
        <semesterinProgram rdf:datatype="http://www.w3.org/2001/XMLSchema#short">7</semesterinProgram>
    </owl:NamedIndividual>
    


    <!-- http://xworks.gr/ontologies/ccso#CS463/CS_BSc/CSD/SSE/UoC -->

    <owl:NamedIndividual rdf:about="http://xworks.gr/ontologies/ccso#CS463/CS_BSc/CSD/SSE/UoC">
        <rdf:type rdf:resource="http://xworks.gr/ontologies/ccso#Course"/>
        <hasPrerequisite rdf:resource="http://xworks.gr/ontologies/ccso#CS240/CS_BSc/CSD/SSE/UoC"/>
        <hasSyllabus rdf:resource="http://xworks.gr/ontologies/ccso#CS463s1/CS_BSc/CSD/SSE/UoC"/>
        <includedIn rdf:resource="http://xworks.gr/ontologies/ccso#BSc_Computer_Science/CS_BSc/CSD/SSE/UoC"/>
        <offeredBy rdf:resource="http://xworks.gr/ontologies/ccso#Computers_Sciences_Department_of_University_of_Crete"/>
        <courseType rdf:datatype="http://www.w3.org/2001/XMLSchema#string">Elective</courseType>
        <csName rdf:datatype="http://www.w3.org/2001/XMLSchema#string">Information Retrieval Systems</csName>
    </owl:NamedIndividual>
    


    <!-- http://xworks.gr/ontologies/ccso#CS463s1/CS_BSc/CSD/SSE/UoC -->

    <owl:NamedIndividual rdf:about="http://xworks.gr/ontologies/ccso#CS463s1/CS_BSc/CSD/SSE/UoC">
        <rdf:type rdf:resource="http://xworks.gr/ontologies/ccso#Syllabus"/>
        <syllabusOf rdf:resource="http://xworks.gr/ontologies/ccso#CS463/CS_BSc/CSD/SSE/UoC"/>
        <courseType rdf:datatype="http://www.w3.org/2001/XMLSchema#string">Elective</courseType>
        <creditsECTS rdf:datatype="http://www.w3.org/2001/XMLSchema#short">6</creditsECTS>
        <csName rdf:datatype="http://www.w3.org/2001/XMLSchema#string">Syllabus of course CS463 Information Retrieval Systems</csName>
        <semesterinProgram rdf:datatype="http://www.w3.org/2001/XMLSchema#short">8</semesterinProgram>
    </owl:NamedIndividual>
    


    <!-- http://xworks.gr/ontologies/ccso#CS468/CS_BSc/CSD/SSE/UoC -->

    <owl:NamedIndividual rdf:about="http://xworks.gr/ontologies/ccso#CS468/CS_BSc/CSD/SSE/UoC">
        <rdf:type rdf:resource="http://xworks.gr/ontologies/ccso#Course"/>
        <hasPrerequisite rdf:resource="http://xworks.gr/ontologies/ccso#CS217/CS_BSc/CSD/SSE/UoC"/>
        <hasPrerequisite rdf:resource="http://xworks.gr/ontologies/ccso#CS317/CS_BSc/CSD/SSE/UoC"/>
        <hasSyllabus rdf:resource="http://xworks.gr/ontologies/ccso#CS468s1/CS_BSc/CSD/SSE/UoC"/>
        <includedIn rdf:resource="http://xworks.gr/ontologies/ccso#BSc_Computer_Science/CS_BSc/CSD/SSE/UoC"/>
        <offeredBy rdf:resource="http://xworks.gr/ontologies/ccso#Computers_Sciences_Department_of_University_of_Crete"/>
        <courseType rdf:datatype="http://www.w3.org/2001/XMLSchema#string">Elective</courseType>
        <csName rdf:datatype="http://www.w3.org/2001/XMLSchema#string">Game Theory and Decision Making in Service Systems</csName>
    </owl:NamedIndividual>
    


    <!-- http://xworks.gr/ontologies/ccso#CS468s1/CS_BSc/CSD/SSE/UoC -->

    <owl:NamedIndividual rdf:about="http://xworks.gr/ontologies/ccso#CS468s1/CS_BSc/CSD/SSE/UoC">
        <rdf:type rdf:resource="http://xworks.gr/ontologies/ccso#Syllabus"/>
        <syllabusOf rdf:resource="http://xworks.gr/ontologies/ccso#CS468/CS_BSc/CSD/SSE/UoC"/>
        <courseType rdf:datatype="http://www.w3.org/2001/XMLSchema#string">Elective</courseType>
        <creditsECTS rdf:datatype="http://www.w3.org/2001/XMLSchema#short">6</creditsECTS>
        <csName rdf:datatype="http://www.w3.org/2001/XMLSchema#string">Syllabus of course CS468 Game Theory and Decision Making in Service Systems</csName>
        <semesterinProgram rdf:datatype="http://www.w3.org/2001/XMLSchema#short">7</semesterinProgram>
    </owl:NamedIndividual>
    


    <!-- http://xworks.gr/ontologies/ccso#CS469/CS_BSc/CSD/SSE/UoC -->

    <owl:NamedIndividual rdf:about="http://xworks.gr/ontologies/ccso#CS469/CS_BSc/CSD/SSE/UoC">
        <rdf:type rdf:resource="http://xworks.gr/ontologies/ccso#Course"/>
        <hasPrerequisite rdf:resource="http://xworks.gr/ontologies/ccso#CS364/CS_BSc/CSD/SSE/UoC"/>
        <hasSyllabus rdf:resource="http://xworks.gr/ontologies/ccso#CS469s1/CS_BSc/CSD/SSE/UoC"/>
        <includedIn rdf:resource="http://xworks.gr/ontologies/ccso#BSc_Computer_Science/CS_BSc/CSD/SSE/UoC"/>
        <offeredBy rdf:resource="http://xworks.gr/ontologies/ccso#Computers_Sciences_Department_of_University_of_Crete"/>
        <courseType rdf:datatype="http://www.w3.org/2001/XMLSchema#string">Elective</courseType>
        <csName rdf:datatype="http://www.w3.org/2001/XMLSchema#string">Modern Topics in Human-Computer Interaction</csName>
    </owl:NamedIndividual>
    


    <!-- http://xworks.gr/ontologies/ccso#CS469s1/CS_BSc/CSD/SSE/UoC -->

    <owl:NamedIndividual rdf:about="http://xworks.gr/ontologies/ccso#CS469s1/CS_BSc/CSD/SSE/UoC">
        <rdf:type rdf:resource="http://xworks.gr/ontologies/ccso#Syllabus"/>
        <syllabusOf rdf:resource="http://xworks.gr/ontologies/ccso#CS469/CS_BSc/CSD/SSE/UoC"/>
        <courseType rdf:datatype="http://www.w3.org/2001/XMLSchema#string">Elective</courseType>
        <creditsECTS rdf:datatype="http://www.w3.org/2001/XMLSchema#short">6</creditsECTS>
        <csName rdf:datatype="http://www.w3.org/2001/XMLSchema#string">Syllabus of course CS469 Modern Topics in Human-Computer Interaction</csName>
        <semesterinProgram rdf:datatype="http://www.w3.org/2001/XMLSchema#short">7</semesterinProgram>
    </owl:NamedIndividual>
    


    <!-- http://xworks.gr/ontologies/ccso#CS471/CS_BSc/CSD/SSE/UoC -->

    <owl:NamedIndividual rdf:about="http://xworks.gr/ontologies/ccso#CS471/CS_BSc/CSD/SSE/UoC">
        <rdf:type rdf:resource="http://xworks.gr/ontologies/ccso#Course"/>
        <hasPrerequisite rdf:resource="http://xworks.gr/ontologies/ccso#CS371/CS_BSc/CSD/SSE/UoC"/>
        <hasSyllabus rdf:resource="http://xworks.gr/ontologies/ccso#CS471s1/CS_BSc/CSD/SSE/UoC"/>
        <includedIn rdf:resource="http://xworks.gr/ontologies/ccso#BSc_Computer_Science/CS_BSc/CSD/SSE/UoC"/>
        <offeredBy rdf:resource="http://xworks.gr/ontologies/ccso#Computers_Sciences_Department_of_University_of_Crete"/>
        <courseType rdf:datatype="http://www.w3.org/2001/XMLSchema#string">Elective</courseType>
        <csName rdf:datatype="http://www.w3.org/2001/XMLSchema#string">Image Analysis</csName>
    </owl:NamedIndividual>
    


    <!-- http://xworks.gr/ontologies/ccso#CS471s1/CS_BSc/CSD/SSE/UoC -->

    <owl:NamedIndividual rdf:about="http://xworks.gr/ontologies/ccso#CS471s1/CS_BSc/CSD/SSE/UoC">
        <rdf:type rdf:resource="http://xworks.gr/ontologies/ccso#Syllabus"/>
        <syllabusOf rdf:resource="http://xworks.gr/ontologies/ccso#CS471/CS_BSc/CSD/SSE/UoC"/>
        <courseType rdf:datatype="http://www.w3.org/2001/XMLSchema#string">Elective</courseType>
        <creditsECTS rdf:datatype="http://www.w3.org/2001/XMLSchema#short">6</creditsECTS>
        <csName rdf:datatype="http://www.w3.org/2001/XMLSchema#string">Syllabus of course CS471 Image Analysis</csName>
        <semesterinProgram rdf:datatype="http://www.w3.org/2001/XMLSchema#short">7</semesterinProgram>
    </owl:NamedIndividual>
    


    <!-- http://xworks.gr/ontologies/ccso#CS472/CS_BSc/CSD/SSE/UoC -->

    <owl:NamedIndividual rdf:about="http://xworks.gr/ontologies/ccso#CS472/CS_BSc/CSD/SSE/UoC">
        <rdf:type rdf:resource="http://xworks.gr/ontologies/ccso#Course"/>
        <hasPrerequisite rdf:resource="http://xworks.gr/ontologies/ccso#CS371/CS_BSc/CSD/SSE/UoC"/>
        <hasSyllabus rdf:resource="http://xworks.gr/ontologies/ccso#CS472s1/CS_BSc/CSD/SSE/UoC"/>
        <includedIn rdf:resource="http://xworks.gr/ontologies/ccso#BSc_Computer_Science/CS_BSc/CSD/SSE/UoC"/>
        <offeredBy rdf:resource="http://xworks.gr/ontologies/ccso#Computers_Sciences_Department_of_University_of_Crete"/>
        <courseType rdf:datatype="http://www.w3.org/2001/XMLSchema#string">Elective</courseType>
        <csName rdf:datatype="http://www.w3.org/2001/XMLSchema#string">Computer Vision</csName>
    </owl:NamedIndividual>
    


    <!-- http://xworks.gr/ontologies/ccso#CS472s1/CS_BSc/CSD/SSE/UoC -->

    <owl:NamedIndividual rdf:about="http://xworks.gr/ontologies/ccso#CS472s1/CS_BSc/CSD/SSE/UoC">
        <rdf:type rdf:resource="http://xworks.gr/ontologies/ccso#Syllabus"/>
        <syllabusOf rdf:resource="http://xworks.gr/ontologies/ccso#CS472/CS_BSc/CSD/SSE/UoC"/>
        <courseType rdf:datatype="http://www.w3.org/2001/XMLSchema#string">Elective</courseType>
        <creditsECTS rdf:datatype="http://www.w3.org/2001/XMLSchema#short">6</creditsECTS>
        <csName rdf:datatype="http://www.w3.org/2001/XMLSchema#string">Syllabus of course CS472 Computer Vision</csName>
        <semesterinProgram rdf:datatype="http://www.w3.org/2001/XMLSchema#short">8</semesterinProgram>
    </owl:NamedIndividual>
    


    <!-- http://xworks.gr/ontologies/ccso#CS473/CS_BSc/CSD/SSE/UoC -->

    <owl:NamedIndividual rdf:about="http://xworks.gr/ontologies/ccso#CS473/CS_BSc/CSD/SSE/UoC">
        <rdf:type rdf:resource="http://xworks.gr/ontologies/ccso#Course"/>
        <hasPrerequisite rdf:resource="http://xworks.gr/ontologies/ccso#CS119/CS_BSc/CSD/SSE/UoC"/>
        <hasPrerequisite rdf:resource="http://xworks.gr/ontologies/ccso#CS217/CS_BSc/CSD/SSE/UoC"/>
        <hasSyllabus rdf:resource="http://xworks.gr/ontologies/ccso#CS473s1/CS_BSc/CSD/SSE/UoC"/>
        <includedIn rdf:resource="http://xworks.gr/ontologies/ccso#BSc_Computer_Science/CS_BSc/CSD/SSE/UoC"/>
        <offeredBy rdf:resource="http://xworks.gr/ontologies/ccso#Computers_Sciences_Department_of_University_of_Crete"/>
        <courseType rdf:datatype="http://www.w3.org/2001/XMLSchema#string">Elective</courseType>
        <csName rdf:datatype="http://www.w3.org/2001/XMLSchema#string">Pattern Recognition</csName>
    </owl:NamedIndividual>
    


    <!-- http://xworks.gr/ontologies/ccso#CS473s1/CS_BSc/CSD/SSE/UoC -->

    <owl:NamedIndividual rdf:about="http://xworks.gr/ontologies/ccso#CS473s1/CS_BSc/CSD/SSE/UoC">
        <rdf:type rdf:resource="http://xworks.gr/ontologies/ccso#Syllabus"/>
        <syllabusOf rdf:resource="http://xworks.gr/ontologies/ccso#CS473/CS_BSc/CSD/SSE/UoC"/>
        <courseType rdf:datatype="http://www.w3.org/2001/XMLSchema#string">Elective</courseType>
        <creditsECTS rdf:datatype="http://www.w3.org/2001/XMLSchema#short">6</creditsECTS>
        <csName rdf:datatype="http://www.w3.org/2001/XMLSchema#string">Syllabus of course CS473 Pattern Recognition</csName>
        <semesterinProgram rdf:datatype="http://www.w3.org/2001/XMLSchema#short">8</semesterinProgram>
    </owl:NamedIndividual>
    


    <!-- http://xworks.gr/ontologies/ccso#CS474/CS_BSc/CSD/SSE/UoC -->

    <owl:NamedIndividual rdf:about="http://xworks.gr/ontologies/ccso#CS474/CS_BSc/CSD/SSE/UoC">
        <rdf:type rdf:resource="http://xworks.gr/ontologies/ccso#Course"/>
        <coversKA rdf:resource="http://xworks.gr/ontologies/ccso#CS/NC_Networking_and_Communication"/>
        <hasPrerequisite rdf:resource="http://xworks.gr/ontologies/ccso#CS215/CS_BSc/CSD/SSE/UoC"/>
        <hasSyllabus rdf:resource="http://xworks.gr/ontologies/ccso#CS474s1/CS_BSc/CSD/SSE/UoC"/>
        <includedIn rdf:resource="http://xworks.gr/ontologies/ccso#BSc_Computer_Science/CS_BSc/CSD/SSE/UoC"/>
        <offeredBy rdf:resource="http://xworks.gr/ontologies/ccso#Computers_Sciences_Department_of_University_of_Crete"/>
        <courseType rdf:datatype="http://www.w3.org/2001/XMLSchema#string">Elective</courseType>
        <csName rdf:datatype="http://www.w3.org/2001/XMLSchema#string">Multimedia Technology</csName>
    </owl:NamedIndividual>
    


    <!-- http://xworks.gr/ontologies/ccso#CS474s1/CS_BSc/CSD/SSE/UoC -->

    <owl:NamedIndividual rdf:about="http://xworks.gr/ontologies/ccso#CS474s1/CS_BSc/CSD/SSE/UoC">
        <rdf:type rdf:resource="http://xworks.gr/ontologies/ccso#Syllabus"/>
        <syllabusOf rdf:resource="http://xworks.gr/ontologies/ccso#CS474/CS_BSc/CSD/SSE/UoC"/>
        <courseType rdf:datatype="http://www.w3.org/2001/XMLSchema#string">Elective</courseType>
        <creditsECTS rdf:datatype="http://www.w3.org/2001/XMLSchema#short">6</creditsECTS>
        <csName rdf:datatype="http://www.w3.org/2001/XMLSchema#string">Syllabus of course CS474 Multimedia Technology</csName>
        <semesterinProgram rdf:datatype="http://www.w3.org/2001/XMLSchema#short">7</semesterinProgram>
    </owl:NamedIndividual>
    


    <!-- http://xworks.gr/ontologies/ccso#CS475/CS_BSc/CSD/SSE/UoC -->

    <owl:NamedIndividual rdf:about="http://xworks.gr/ontologies/ccso#CS475/CS_BSc/CSD/SSE/UoC">
        <rdf:type rdf:resource="http://xworks.gr/ontologies/ccso#Course"/>
        <hasPrerequisite rdf:resource="http://xworks.gr/ontologies/ccso#CS119/CS_BSc/CSD/SSE/UoC"/>
        <hasPrerequisite rdf:resource="http://xworks.gr/ontologies/ccso#CS217/CS_BSc/CSD/SSE/UoC"/>
        <hasSyllabus rdf:resource="http://xworks.gr/ontologies/ccso#CS475s1/CS_BSc/CSD/SSE/UoC"/>
        <includedIn rdf:resource="http://xworks.gr/ontologies/ccso#BSc_Computer_Science/CS_BSc/CSD/SSE/UoC"/>
        <offeredBy rdf:resource="http://xworks.gr/ontologies/ccso#Computers_Sciences_Department_of_University_of_Crete"/>
        <courseType rdf:datatype="http://www.w3.org/2001/XMLSchema#string">Elective</courseType>
        <csName rdf:datatype="http://www.w3.org/2001/XMLSchema#string">Autonomous Robotic Navigation</csName>
    </owl:NamedIndividual>
    


    <!-- http://xworks.gr/ontologies/ccso#CS475s1/CS_BSc/CSD/SSE/UoC -->

    <owl:NamedIndividual rdf:about="http://xworks.gr/ontologies/ccso#CS475s1/CS_BSc/CSD/SSE/UoC">
        <rdf:type rdf:resource="http://xworks.gr/ontologies/ccso#Syllabus"/>
        <syllabusOf rdf:resource="http://xworks.gr/ontologies/ccso#CS475/CS_BSc/CSD/SSE/UoC"/>
        <courseType rdf:datatype="http://www.w3.org/2001/XMLSchema#string">Elective</courseType>
        <creditsECTS rdf:datatype="http://www.w3.org/2001/XMLSchema#short">6</creditsECTS>
        <csName rdf:datatype="http://www.w3.org/2001/XMLSchema#string">Syllabus of course CS475 Autonomous Robotic Navigation</csName>
        <semesterinProgram rdf:datatype="http://www.w3.org/2001/XMLSchema#short">8</semesterinProgram>
    </owl:NamedIndividual>
    


    <!-- http://xworks.gr/ontologies/ccso#CS482/CS_BSc/CSD/SSE/UoC -->

    <owl:NamedIndividual rdf:about="http://xworks.gr/ontologies/ccso#CS482/CS_BSc/CSD/SSE/UoC">
        <rdf:type rdf:resource="http://xworks.gr/ontologies/ccso#Course"/>
        <hasPrerequisite rdf:resource="http://xworks.gr/ontologies/ccso#CS119/CS_BSc/CSD/SSE/UoC"/>
        <hasSyllabus rdf:resource="http://xworks.gr/ontologies/ccso#CS482s1/CS_BSc/CSD/SSE/UoC"/>
        <includedIn rdf:resource="http://xworks.gr/ontologies/ccso#BSc_Computer_Science/CS_BSc/CSD/SSE/UoC"/>
        <offeredBy rdf:resource="http://xworks.gr/ontologies/ccso#Computers_Sciences_Department_of_University_of_Crete"/>
        <courseType rdf:datatype="http://www.w3.org/2001/XMLSchema#string">Elective</courseType>
        <csName rdf:datatype="http://www.w3.org/2001/XMLSchema#string">Algorithms in Bioinformatics</csName>
    </owl:NamedIndividual>
    


    <!-- http://xworks.gr/ontologies/ccso#CS482s1/CS_BSc/CSD/SSE/UoC -->

    <owl:NamedIndividual rdf:about="http://xworks.gr/ontologies/ccso#CS482s1/CS_BSc/CSD/SSE/UoC">
        <rdf:type rdf:resource="http://xworks.gr/ontologies/ccso#Syllabus"/>
        <syllabusOf rdf:resource="http://xworks.gr/ontologies/ccso#CS482/CS_BSc/CSD/SSE/UoC"/>
        <courseType rdf:datatype="http://www.w3.org/2001/XMLSchema#string">Elective</courseType>
        <creditsECTS rdf:datatype="http://www.w3.org/2001/XMLSchema#short">6</creditsECTS>
        <csName rdf:datatype="http://www.w3.org/2001/XMLSchema#string">Syllabus of course CS482 Algorithms in Bioinformatics</csName>
        <semesterinProgram rdf:datatype="http://www.w3.org/2001/XMLSchema#short">7</semesterinProgram>
    </owl:NamedIndividual>
    


    <!-- http://xworks.gr/ontologies/ccso#CS486/CS_BSc/CSD/SSE/UoC -->

    <owl:NamedIndividual rdf:about="http://xworks.gr/ontologies/ccso#CS486/CS_BSc/CSD/SSE/UoC">
        <rdf:type rdf:resource="http://xworks.gr/ontologies/ccso#Course"/>
        <coversKA rdf:resource="http://xworks.gr/ontologies/ccso#CS/PL_Programming_Languages"/>
        <hasPrerequisite rdf:resource="http://xworks.gr/ontologies/ccso#CS240/CS_BSc/CSD/SSE/UoC"/>
        <hasSyllabus rdf:resource="http://xworks.gr/ontologies/ccso#CS486s1/CS_BSc/CSD/SSE/UoC"/>
        <includedIn rdf:resource="http://xworks.gr/ontologies/ccso#BSc_Computer_Science/CS_BSc/CSD/SSE/UoC"/>
        <offeredBy rdf:resource="http://xworks.gr/ontologies/ccso#Computers_Sciences_Department_of_University_of_Crete"/>
        <courseType rdf:datatype="http://www.w3.org/2001/XMLSchema#string">Elective</courseType>
        <csName rdf:datatype="http://www.w3.org/2001/XMLSchema#string">Principles of Distributed Computing</csName>
    </owl:NamedIndividual>
    


    <!-- http://xworks.gr/ontologies/ccso#CS486s1/CS_BSc/CSD/SSE/UoC -->

    <owl:NamedIndividual rdf:about="http://xworks.gr/ontologies/ccso#CS486s1/CS_BSc/CSD/SSE/UoC">
        <rdf:type rdf:resource="http://xworks.gr/ontologies/ccso#Syllabus"/>
        <syllabusOf rdf:resource="http://xworks.gr/ontologies/ccso#CS486/CS_BSc/CSD/SSE/UoC"/>
        <courseType rdf:datatype="http://www.w3.org/2001/XMLSchema#string">Elective</courseType>
        <creditsECTS rdf:datatype="http://www.w3.org/2001/XMLSchema#short">6</creditsECTS>
        <csName rdf:datatype="http://www.w3.org/2001/XMLSchema#string">Syllabus of course CS486 Principles of Distributed Computing</csName>
        <semesterinProgram rdf:datatype="http://www.w3.org/2001/XMLSchema#short">7</semesterinProgram>
    </owl:NamedIndividual>
    


    <!-- http://xworks.gr/ontologies/ccso#CS499/CS_BSc/CSD/SSE/UoC -->

    <owl:NamedIndividual rdf:about="http://xworks.gr/ontologies/ccso#CS499/CS_BSc/CSD/SSE/UoC">
        <rdf:type rdf:resource="http://xworks.gr/ontologies/ccso#Course"/>
        <hasSyllabus rdf:resource="http://xworks.gr/ontologies/ccso#CS499s1/CS_BSc/CSD/SSE/UoC"/>
        <includedIn rdf:resource="http://xworks.gr/ontologies/ccso#BSc_Computer_Science/CS_BSc/CSD/SSE/UoC"/>
        <offeredBy rdf:resource="http://xworks.gr/ontologies/ccso#Computers_Sciences_Department_of_University_of_Crete"/>
        <courseType rdf:datatype="http://www.w3.org/2001/XMLSchema#string">Core</courseType>
        <csName rdf:datatype="http://www.w3.org/2001/XMLSchema#string">Bachelor΄s Thesis</csName>
    </owl:NamedIndividual>
    


    <!-- http://xworks.gr/ontologies/ccso#CS499s1/CS_BSc/CSD/SSE/UoC -->

    <owl:NamedIndividual rdf:about="http://xworks.gr/ontologies/ccso#CS499s1/CS_BSc/CSD/SSE/UoC">
        <rdf:type rdf:resource="http://xworks.gr/ontologies/ccso#Syllabus"/>
        <syllabusOf rdf:resource="http://xworks.gr/ontologies/ccso#CS499/CS_BSc/CSD/SSE/UoC"/>
        <courseType rdf:datatype="http://www.w3.org/2001/XMLSchema#string">Elective</courseType>
        <creditsECTS rdf:datatype="http://www.w3.org/2001/XMLSchema#short">6</creditsECTS>
        <csName rdf:datatype="http://www.w3.org/2001/XMLSchema#string">Syllabus of course CS499 Bachelor΄s Thesis</csName>
        <semesterinProgram rdf:datatype="http://www.w3.org/2001/XMLSchema#short">8</semesterinProgram>
    </owl:NamedIndividual>
    


    <!-- http://xworks.gr/ontologies/ccso#CS539/CSE_MSc/CSD/SSE/UoC -->

    <owl:NamedIndividual rdf:about="http://xworks.gr/ontologies/ccso#CS539/CSE_MSc/CSD/SSE/UoC">
        <rdf:type rdf:resource="http://xworks.gr/ontologies/ccso#Course"/>
        <hasPrerequisite rdf:resource="http://xworks.gr/ontologies/ccso#CS335/CS_BSc/CSD/SSE/UoC"/>
        <hasSyllabus rdf:resource="http://xworks.gr/ontologies/ccso#CS539s1/CSE_MSc/CSD/SSE/UoC"/>
        <includedIn rdf:resource="http://xworks.gr/ontologies/ccso#MSc_Computer_Science_and_Engineering/CSE_MSc/CSD/SSE/UoC"/>
        <offeredBy rdf:resource="http://xworks.gr/ontologies/ccso#Computers_Sciences_Department_of_University_of_Crete"/>
        <code rdf:datatype="http://www.w3.org/2001/XMLSchema#string">CS539/CSE_MSc/CSD/SSE/UoC</code>
        <courseType rdf:datatype="http://www.w3.org/2001/XMLSchema#string">Core</courseType>
        <csName rdf:datatype="http://www.w3.org/2001/XMLSchema#string">CS539 Advanced Topics on Wireless Networks and Mobile Systems
Course in Computer Science and Engineering MSc of Computers Sciences Department (CSD) of University of Crete of University of Crete</csName>
        <rdfs:comment xml:lang="en">CS539 Advanced Topics on Wireless Networks and Mobile Systems
Course in Computer Science and Engineering MSc of Computers Sciences Department (CSD) of University of Crete of University of Crete</rdfs:comment>
    </owl:NamedIndividual>
    


    <!-- http://xworks.gr/ontologies/ccso#CS539s1/CSE_MSc/CSD/SSE/UoC -->

    <owl:NamedIndividual rdf:about="http://xworks.gr/ontologies/ccso#CS539s1/CSE_MSc/CSD/SSE/UoC">
        <rdf:type rdf:resource="http://xworks.gr/ontologies/ccso#Syllabus"/>
        <syllabusOf rdf:resource="http://xworks.gr/ontologies/ccso#CS539/CSE_MSc/CSD/SSE/UoC"/>
        <code rdf:datatype="http://www.w3.org/2001/XMLSchema#string">CS539s1/CSE_MSc/CSD/SSE/UoC</code>
        <csName rdf:datatype="http://www.w3.org/2001/XMLSchema#string">Syllabus of course CS539 Advanced Topics on Wireless Networks and Mobile Systems</csName>
    </owl:NamedIndividual>
    


    <!-- http://xworks.gr/ontologies/ccso#CS540/CSE_MSc/CSD/SSE/UoC -->

    <owl:NamedIndividual rdf:about="http://xworks.gr/ontologies/ccso#CS540/CSE_MSc/CSD/SSE/UoC">
        <rdf:type rdf:resource="http://xworks.gr/ontologies/ccso#Course"/>
        <hasSyllabus rdf:resource="http://xworks.gr/ontologies/ccso#CS540s1/CSE_MSc/CSD/SSE/UoC"/>
        <includedIn rdf:resource="http://xworks.gr/ontologies/ccso#MSc_Computer_Science_and_Engineering/CSE_MSc/CSD/SSE/UoC"/>
        <offeredBy rdf:resource="http://xworks.gr/ontologies/ccso#Computers_Sciences_Department_of_University_of_Crete"/>
        <code rdf:datatype="http://www.w3.org/2001/XMLSchema#string">CS540/CSE_MSc/CSD/SSE/UoC</code>
        <courseType rdf:datatype="http://www.w3.org/2001/XMLSchema#string">Core</courseType>
        <csName rdf:datatype="http://www.w3.org/2001/XMLSchema#string">Advanced Topics in Programming Languages Development</csName>
        <rdfs:comment xml:lang="en">CS540 Advanced Topics in Programming Languages Development
Course in Computer Science and Engineering MSc of Computers Sciences Department (CSD) of University of Crete of University of Crete</rdfs:comment>
    </owl:NamedIndividual>
    


    <!-- http://xworks.gr/ontologies/ccso#CS540s1/CSE_MSc/CSD/SSE/UoC -->

    <owl:NamedIndividual rdf:about="http://xworks.gr/ontologies/ccso#CS540s1/CSE_MSc/CSD/SSE/UoC">
        <rdf:type rdf:resource="http://xworks.gr/ontologies/ccso#Syllabus"/>
        <syllabusOf rdf:resource="http://xworks.gr/ontologies/ccso#CS540/CSE_MSc/CSD/SSE/UoC"/>
        <code rdf:datatype="http://www.w3.org/2001/XMLSchema#string">CS540s1/CSE_MSc/CSD/SSE/UoC</code>
        <csName rdf:datatype="http://www.w3.org/2001/XMLSchema#string">Syllabus of course CS540 Advanced Topics in Programming Languages Development</csName>
    </owl:NamedIndividual>
    


    <!-- http://xworks.gr/ontologies/ccso#CS672/CSE_PhD/CSD/SSE/UoC -->

    <owl:NamedIndividual rdf:about="http://xworks.gr/ontologies/ccso#CS672/CSE_PhD/CSD/SSE/UoC">
        <rdf:type rdf:resource="http://xworks.gr/ontologies/ccso#Course"/>
        <includedIn rdf:resource="http://xworks.gr/ontologies/ccso#PhD_Computer_Science_and_Engineering/CSE_PhD/CSD/SSE/UoC"/>
        <offeredBy rdf:resource="http://xworks.gr/ontologies/ccso#Computers_Sciences_Department_of_University_of_Crete"/>
        <code rdf:datatype="http://www.w3.org/2001/XMLSchema#string">CS672/CSE_PhD/CSD/SSE/UoC</code>
        <csName rdf:datatype="http://www.w3.org/2001/XMLSchema#string">Advanced Topics in Computational Vision</csName>
    </owl:NamedIndividual>
    


    <!-- http://xworks.gr/ontologies/ccso#IM101/IM_MSc/IED/STEF/TEIC -->

    <owl:NamedIndividual rdf:about="http://xworks.gr/ontologies/ccso#IM101/IM_MSc/IED/STEF/TEIC">
        <rdf:type rdf:resource="http://xworks.gr/ontologies/ccso#Course"/>
        <affiliatedWith rdf:resource="http://xworks.gr/ontologies/ccso#Sandi_Elina"/>
        <coversKA rdf:resource="http://xworks.gr/ontologies/ccso#CS/SIP_Social_Issues_and_Professional_Practice"/>
        <hasAttender rdf:resource="http://xworks.gr/ontologies/ccso#Sandi_Elina"/>
        <hasSyllabus rdf:resource="http://xworks.gr/ontologies/ccso#IM101s1/IM_MSc/IED/STEF/TEI"/>
        <includedIn rdf:resource="http://xworks.gr/ontologies/ccso#MSc_Informatics_&amp;_Multimedia/IM_MSc/IED/STEF/TEIC"/>
        <offeredBy rdf:resource="http://xworks.gr/ontologies/ccso#Department_of_Informatics_Engineering_of_TEI_of_Crete"/>
        <code rdf:datatype="http://www.w3.org/2001/XMLSchema#string">IM101/IM_MSc/IED/STEF/TEIC</code>
        <courseType rdf:datatype="http://www.w3.org/2001/XMLSchema#string">Core</courseType>
        <csName rdf:datatype="http://www.w3.org/2001/XMLSchema#string">Project Management and Research Methodologies</csName>
    </owl:NamedIndividual>
    


    <!-- http://xworks.gr/ontologies/ccso#IM101s1/IM_MSc/IED/STEF/TEI -->

    <owl:NamedIndividual rdf:about="http://xworks.gr/ontologies/ccso#IM101s1/IM_MSc/IED/STEF/TEI">
        <rdf:type rdf:resource="http://xworks.gr/ontologies/ccso#Syllabus"/>
        <affiliatedWith rdf:resource="http://xworks.gr/ontologies/ccso#Tsiknakis_Manolis"/>
        <hasInstructor rdf:resource="http://xworks.gr/ontologies/ccso#Tsiknakis_Manolis"/>
        <hasSupervisor rdf:resource="http://xworks.gr/ontologies/ccso#Tsiknakis_Manolis"/>
        <syllabusOf rdf:resource="http://xworks.gr/ontologies/ccso#IM101/IM_MSc/IED/STEF/TEIC"/>
        <courseType rdf:datatype="http://www.w3.org/2001/XMLSchema#string">Core</courseType>
        <creditsECTS rdf:datatype="http://www.w3.org/2001/XMLSchema#decimal">7.5</creditsECTS>
        <csName rdf:datatype="http://www.w3.org/2001/XMLSchema#string">Syllabus of course IM101 Project Management and Research Methodologies</csName>
        <semesterinProgram rdf:datatype="http://www.w3.org/2001/XMLSchema#short">1</semesterinProgram>
    </owl:NamedIndividual>
    


    <!-- http://xworks.gr/ontologies/ccso#IM102/IM_MSc/IED/STEF/TEIC -->

    <owl:NamedIndividual rdf:about="http://xworks.gr/ontologies/ccso#IM102/IM_MSc/IED/STEF/TEIC">
        <rdf:type rdf:resource="http://xworks.gr/ontologies/ccso#Course"/>
        <coversKA rdf:resource="http://xworks.gr/ontologies/ccso#CS/NC_Networking_and_Communication"/>
        <hasSyllabus rdf:resource="http://xworks.gr/ontologies/ccso#IM102s1/IM_MSc/IED/STEF/TEI"/>
        <includedIn rdf:resource="http://xworks.gr/ontologies/ccso#MSc_Informatics_&amp;_Multimedia/IM_MSc/IED/STEF/TEIC"/>
        <offeredBy rdf:resource="http://xworks.gr/ontologies/ccso#Department_of_Informatics_Engineering_of_TEI_of_Crete"/>
        <code rdf:datatype="http://www.w3.org/2001/XMLSchema#string">IM102/IM_MSc/IED/STEF/TEIC</code>
        <courseType rdf:datatype="http://www.w3.org/2001/XMLSchema#string">Elective</courseType>
        <csName rdf:datatype="http://www.w3.org/2001/XMLSchema#string">Computer Networks</csName>
    </owl:NamedIndividual>
    


    <!-- http://xworks.gr/ontologies/ccso#IM102s1/IM_MSc/IED/STEF/TEI -->

    <owl:NamedIndividual rdf:about="http://xworks.gr/ontologies/ccso#IM102s1/IM_MSc/IED/STEF/TEI">
        <rdf:type rdf:resource="http://xworks.gr/ontologies/ccso#Syllabus"/>
        <affiliatedWith rdf:resource="http://xworks.gr/ontologies/ccso#Katis_Evangelos"/>
        <affiliatedWith rdf:resource="http://xworks.gr/ontologies/ccso#Panagiotakis_Spyros"/>
        <affiliatedWith rdf:resource="http://xworks.gr/ontologies/ccso#Vourkas_Michail"/>
        <aimsToLO rdf:resource="http://xworks.gr/ontologies/ccso#CS/NC/LAN/LO_Describe_how_frames_are_forwarded_in_an_Ethernet_network"/>
        <aimsToLO rdf:resource="http://xworks.gr/ontologies/ccso#CS/NC/LAN/LO_Describe_the_interrelations_between_IP_and_Ethernet"/>
        <aimsToLO rdf:resource="http://xworks.gr/ontologies/ccso#CS/NC/LAN/LO_Describe_the_steps_used_in_one_common_approach_to_the_multiple_access_problem"/>
        <aimsToLO rdf:resource="http://xworks.gr/ontologies/ccso#CS/NC/LAN/LO_Identify_the_differences_between_IP_and_Ethernet"/>
        <coversTopic rdf:resource="http://xworks.gr/ontologies/ccso#CS/NC/LAN/T_Common_approaches_to_multiple_access"/>
        <coversTopic rdf:resource="http://xworks.gr/ontologies/ccso#CS/NC/LAN/T_Multiple_Access_Problem"/>
        <coversTopic rdf:resource="http://xworks.gr/ontologies/ccso#CS/NC/LAN/T_Switching"/>
        <hasCourseAssistant rdf:resource="http://xworks.gr/ontologies/ccso#Katis_Evangelos"/>
        <hasInstructor rdf:resource="http://xworks.gr/ontologies/ccso#Panagiotakis_Spyros"/>
        <hasInstructor rdf:resource="http://xworks.gr/ontologies/ccso#Vourkas_Michail"/>
        <hasSupervisor rdf:resource="http://xworks.gr/ontologies/ccso#Panagiotakis_Spyros"/>
        <syllabusOf rdf:resource="http://xworks.gr/ontologies/ccso#IM102/IM_MSc/IED/STEF/TEIC"/>
        <courseType rdf:datatype="http://www.w3.org/2001/XMLSchema#string">Elective</courseType>
        <creditsECTS rdf:datatype="http://www.w3.org/2001/XMLSchema#decimal">7.5</creditsECTS>
        <csName rdf:datatype="http://www.w3.org/2001/XMLSchema#string">Syllabus of course IM102 Computer Networks</csName>
        <semesterinProgram rdf:datatype="http://www.w3.org/2001/XMLSchema#short">1</semesterinProgram>
    </owl:NamedIndividual>
    


    <!-- http://xworks.gr/ontologies/ccso#IM103/IM_MSc/IED/STEF/TEIC -->

    <owl:NamedIndividual rdf:about="http://xworks.gr/ontologies/ccso#IM103/IM_MSc/IED/STEF/TEIC">
        <rdf:type rdf:resource="http://xworks.gr/ontologies/ccso#Course"/>
        <coversKA rdf:resource="http://xworks.gr/ontologies/ccso#CS/NC_Networking_and_Communication"/>
        <hasSyllabus rdf:resource="http://xworks.gr/ontologies/ccso#IM103s1/IM_MSc/IED/STEF/TEI"/>
        <includedIn rdf:resource="http://xworks.gr/ontologies/ccso#MSc_Informatics_&amp;_Multimedia/IM_MSc/IED/STEF/TEIC"/>
        <offeredBy rdf:resource="http://xworks.gr/ontologies/ccso#Department_of_Informatics_Engineering_of_TEI_of_Crete"/>
        <code rdf:datatype="http://www.w3.org/2001/XMLSchema#string">IM103/IM_MSc/IED/STEF/TEIC</code>
        <courseType rdf:datatype="http://www.w3.org/2001/XMLSchema#string">Elective</courseType>
        <csName rdf:datatype="http://www.w3.org/2001/XMLSchema#string">Advanced Multimedia Technologies</csName>
    </owl:NamedIndividual>
    


    <!-- http://xworks.gr/ontologies/ccso#IM103s1/IM_MSc/IED/STEF/TEI -->

    <owl:NamedIndividual rdf:about="http://xworks.gr/ontologies/ccso#IM103s1/IM_MSc/IED/STEF/TEI">
        <rdf:type rdf:resource="http://xworks.gr/ontologies/ccso#Syllabus"/>
        <affiliatedWith rdf:resource="http://xworks.gr/ontologies/ccso#Malamos_Athanasios"/>
        <hasInstructor rdf:resource="http://xworks.gr/ontologies/ccso#Malamos_Athanasios"/>
        <hasSupervisor rdf:resource="http://xworks.gr/ontologies/ccso#Malamos_Athanasios"/>
        <syllabusOf rdf:resource="http://xworks.gr/ontologies/ccso#IM103/IM_MSc/IED/STEF/TEIC"/>
        <courseType rdf:datatype="http://www.w3.org/2001/XMLSchema#string">Elective</courseType>
        <creditsECTS rdf:datatype="http://www.w3.org/2001/XMLSchema#decimal">7.5</creditsECTS>
        <csName rdf:datatype="http://www.w3.org/2001/XMLSchema#string">Syllabus of course IM103 Advanced Multimedia Technologies</csName>
        <semesterinProgram rdf:datatype="http://www.w3.org/2001/XMLSchema#short">1</semesterinProgram>
    </owl:NamedIndividual>
    


    <!-- http://xworks.gr/ontologies/ccso#IM104/IM_MSc/IED/STEF/TEIC -->

    <owl:NamedIndividual rdf:about="http://xworks.gr/ontologies/ccso#IM104/IM_MSc/IED/STEF/TEIC">
        <rdf:type rdf:resource="http://xworks.gr/ontologies/ccso#Course"/>
        <coversKA rdf:resource="http://xworks.gr/ontologies/ccso#CS/IS_Intelligent_Systems"/>
        <coversKA rdf:resource="http://xworks.gr/ontologies/ccso#CS/SW_Software_Engineering_Software_Systems_and_Applications"/>
        <hasSyllabus rdf:resource="http://xworks.gr/ontologies/ccso#IM105s1/IM_MSc/IED/STEF/TEI"/>
        <includedIn rdf:resource="http://xworks.gr/ontologies/ccso#MSc_Informatics_&amp;_Multimedia/IM_MSc/IED/STEF/TEIC"/>
        <offeredBy rdf:resource="http://xworks.gr/ontologies/ccso#Department_of_Informatics_Engineering_of_TEI_of_Crete"/>
        <code rdf:datatype="http://www.w3.org/2001/XMLSchema#string">IM104/IM_MSc/IED/STEF/TEIC</code>
        <courseType rdf:datatype="http://www.w3.org/2001/XMLSchema#string">Elective</courseType>
        <csName rdf:datatype="http://www.w3.org/2001/XMLSchema#string">Advanced Software Engineering</csName>
    </owl:NamedIndividual>
    


    <!-- http://xworks.gr/ontologies/ccso#IM104s1/IM_MSc/IED/STEF/TEI -->

    <owl:NamedIndividual rdf:about="http://xworks.gr/ontologies/ccso#IM104s1/IM_MSc/IED/STEF/TEI">
        <rdf:type rdf:resource="http://xworks.gr/ontologies/ccso#Syllabus"/>
        <affiliatedWith rdf:resource="http://xworks.gr/ontologies/ccso#Vidakis_Nikolaos"/>
        <hasInstructor rdf:resource="http://xworks.gr/ontologies/ccso#Vidakis_Nikolaos"/>
        <hasSupervisor rdf:resource="http://xworks.gr/ontologies/ccso#Vidakis_Nikolaos"/>
        <courseType rdf:datatype="http://www.w3.org/2001/XMLSchema#string">Elective</courseType>
        <creditsECTS rdf:datatype="http://www.w3.org/2001/XMLSchema#decimal">7.5</creditsECTS>
        <csName rdf:datatype="http://www.w3.org/2001/XMLSchema#string">Syllabus of course IM104 Advanced Software Engineering</csName>
        <semesterinProgram rdf:datatype="http://www.w3.org/2001/XMLSchema#short">1</semesterinProgram>
    </owl:NamedIndividual>
    


    <!-- http://xworks.gr/ontologies/ccso#IM105/IM_MSc/IED/STEF/TEIC -->

    <owl:NamedIndividual rdf:about="http://xworks.gr/ontologies/ccso#IM105/IM_MSc/IED/STEF/TEIC">
        <rdf:type rdf:resource="http://xworks.gr/ontologies/ccso#Course"/>
        <affiliatedWith rdf:resource="http://xworks.gr/ontologies/ccso#Sandi_Elina"/>
        <coversKA rdf:resource="http://xworks.gr/ontologies/ccso#CS/IS_Intelligent_Systems"/>
        <coversKA rdf:resource="http://xworks.gr/ontologies/ccso#CS/SW_Software_Engineering_Software_Systems_and_Applications"/>
        <hasAttender rdf:resource="http://xworks.gr/ontologies/ccso#Sandi_Elina"/>
        <hasSyllabus rdf:resource="http://xworks.gr/ontologies/ccso#IM105s1/IM_MSc/IED/STEF/TEI"/>
        <includedIn rdf:resource="http://xworks.gr/ontologies/ccso#MSc_Informatics_&amp;_Multimedia/IM_MSc/IED/STEF/TEIC"/>
        <offeredBy rdf:resource="http://xworks.gr/ontologies/ccso#Department_of_Informatics_Engineering_of_TEI_of_Crete"/>
        <code rdf:datatype="http://www.w3.org/2001/XMLSchema#string">IM105/IM_MSc/IED/STEF/TEIC</code>
        <courseType rdf:datatype="http://www.w3.org/2001/XMLSchema#string">Elective</courseType>
        <csName rdf:datatype="http://www.w3.org/2001/XMLSchema#string">Semantic Web</csName>
    </owl:NamedIndividual>
    


    <!-- http://xworks.gr/ontologies/ccso#IM105s1/IM_MSc/IED/STEF/TEI -->

    <owl:NamedIndividual rdf:about="http://xworks.gr/ontologies/ccso#IM105s1/IM_MSc/IED/STEF/TEI">
        <rdf:type rdf:resource="http://xworks.gr/ontologies/ccso#Syllabus"/>
        <affiliatedWith rdf:resource="http://xworks.gr/ontologies/ccso#Katis_Evangelos"/>
        <affiliatedWith rdf:resource="http://xworks.gr/ontologies/ccso#Kondylakis_Haridimos"/>
        <affiliatedWith rdf:resource="http://xworks.gr/ontologies/ccso#Papadakis_Nikos"/>
        <coversTopic rdf:resource="http://xworks.gr/ontologies/ccso#CS/IS/T_GraphPlan"/>
        <coversTopic rdf:resource="http://xworks.gr/ontologies/ccso#CS/IS/T_Nonmonotonic_Reasoning"/>
        <coversTopic rdf:resource="http://xworks.gr/ontologies/ccso#CS/IS/T_Ontologies"/>
        <coversTopic rdf:resource="http://xworks.gr/ontologies/ccso#CS/IS/T_Query_Languages"/>
        <followsTEMethod rdf:resource="http://xworks.gr/ontologies/ccso#Lecture"/>
        <followsTEMethod rdf:resource="http://xworks.gr/ontologies/ccso#Project"/>
        <hasCourseAssistant rdf:resource="http://xworks.gr/ontologies/ccso#Katis_Evangelos"/>
        <hasCourseAssistant rdf:resource="http://xworks.gr/ontologies/ccso#Kondylakis_Haridimos"/>
        <hasInstructor rdf:resource="http://xworks.gr/ontologies/ccso#Papadakis_Nikos"/>
        <hasLM rdf:resource="http://xworks.gr/ontologies/ccso#BernersLee1998RoadmapSemanticWeb"/>
        <hasLM rdf:resource="http://xworks.gr/ontologies/ccso#BernersLee2001SemanticWeb"/>
        <hasSupervisor rdf:resource="http://xworks.gr/ontologies/ccso#Papadakis_Nikos"/>
        <syllabusOf rdf:resource="http://xworks.gr/ontologies/ccso#IM104/IM_MSc/IED/STEF/TEIC"/>
        <syllabusOf rdf:resource="http://xworks.gr/ontologies/ccso#IM105/IM_MSc/IED/STEF/TEIC"/>
        <code rdf:datatype="http://www.w3.org/2001/XMLSchema#string">IM105s1/IM_MSc/IED/STEF/TEI</code>
        <courseType rdf:datatype="http://www.w3.org/2001/XMLSchema#string">Elective</courseType>
        <creditsECTS rdf:datatype="http://www.w3.org/2001/XMLSchema#decimal">7.5</creditsECTS>
        <csName rdf:datatype="http://www.w3.org/2001/XMLSchema#string">Syllabus of course IM105 Semantic Web</csName>
        <language rdf:datatype="http://www.w3.org/2001/XMLSchema#string">Greek</language>
        <semesterinProgram rdf:datatype="http://www.w3.org/2001/XMLSchema#short">1</semesterinProgram>
    </owl:NamedIndividual>
    


    <!-- http://xworks.gr/ontologies/ccso#IM106/IM_MSc/IED/STEF/TEIC -->

    <owl:NamedIndividual rdf:about="http://xworks.gr/ontologies/ccso#IM106/IM_MSc/IED/STEF/TEIC">
        <rdf:type rdf:resource="http://xworks.gr/ontologies/ccso#Course"/>
        <affiliatedWith rdf:resource="http://xworks.gr/ontologies/ccso#Sandi_Elina"/>
        <coversKA rdf:resource="http://xworks.gr/ontologies/ccso#CS/SW_Software_Engineering_Software_Systems_and_Applications"/>
        <hasAttender rdf:resource="http://xworks.gr/ontologies/ccso#Sandi_Elina"/>
        <hasSyllabus rdf:resource="http://xworks.gr/ontologies/ccso#IM106s1/IM_MSc/IED/STEF/TEI"/>
        <includedIn rdf:resource="http://xworks.gr/ontologies/ccso#MSc_Informatics_&amp;_Multimedia/IM_MSc/IED/STEF/TEIC"/>
        <offeredBy rdf:resource="http://xworks.gr/ontologies/ccso#Department_of_Informatics_Engineering_of_TEI_of_Crete"/>
        <code rdf:datatype="http://www.w3.org/2001/XMLSchema#string">IM106/IM_MSc/IED/STEF/TEIC</code>
        <courseType rdf:datatype="http://www.w3.org/2001/XMLSchema#string">Elective</courseType>
        <csName rdf:datatype="http://www.w3.org/2001/XMLSchema#string">Usability Engineering</csName>
    </owl:NamedIndividual>
    


    <!-- http://xworks.gr/ontologies/ccso#IM106s1/IM_MSc/IED/STEF/TEI -->

    <owl:NamedIndividual rdf:about="http://xworks.gr/ontologies/ccso#IM106s1/IM_MSc/IED/STEF/TEI">
        <rdf:type rdf:resource="http://xworks.gr/ontologies/ccso#Syllabus"/>
        <affiliatedWith rdf:resource="http://xworks.gr/ontologies/ccso#Kalogiannakis_Michail"/>
        <affiliatedWith rdf:resource="http://xworks.gr/ontologies/ccso#Pappa_Pepi"/>
        <hasCourseAssistant rdf:resource="http://xworks.gr/ontologies/ccso#Pappa_Pepi"/>
        <hasInstructor rdf:resource="http://xworks.gr/ontologies/ccso#Kalogiannakis_Michail"/>
        <hasSupervisor rdf:resource="http://xworks.gr/ontologies/ccso#Kalogiannakis_Michail"/>
        <syllabusOf rdf:resource="http://xworks.gr/ontologies/ccso#IM106/IM_MSc/IED/STEF/TEIC"/>
        <courseType rdf:datatype="http://www.w3.org/2001/XMLSchema#string">Elective</courseType>
        <creditsECTS rdf:datatype="http://www.w3.org/2001/XMLSchema#decimal">7.5</creditsECTS>
        <csName rdf:datatype="http://www.w3.org/2001/XMLSchema#string">Syllabus of course IM106 Usability Engineering</csName>
        <semesterinProgram rdf:datatype="http://www.w3.org/2001/XMLSchema#short">1</semesterinProgram>
    </owl:NamedIndividual>
    


    <!-- http://xworks.gr/ontologies/ccso#IM107/IM_MSc/IED/STEF/TEIC -->

    <owl:NamedIndividual rdf:about="http://xworks.gr/ontologies/ccso#IM107/IM_MSc/IED/STEF/TEIC">
        <rdf:type rdf:resource="http://xworks.gr/ontologies/ccso#Course"/>
        <coversKA rdf:resource="http://xworks.gr/ontologies/ccso#CS/CS_Computational_Science"/>
        <coversKA rdf:resource="http://xworks.gr/ontologies/ccso#CS/IS_Intelligent_Systems"/>
        <hasSyllabus rdf:resource="http://xworks.gr/ontologies/ccso#IM107s1/IM_MSc/IED/STEF/TEI"/>
        <includedIn rdf:resource="http://xworks.gr/ontologies/ccso#MSc_Informatics_&amp;_Multimedia/IM_MSc/IED/STEF/TEIC"/>
        <offeredBy rdf:resource="http://xworks.gr/ontologies/ccso#Department_of_Informatics_Engineering_of_TEI_of_Crete"/>
        <code rdf:datatype="http://www.w3.org/2001/XMLSchema#string">IM107/IM_MSc/IED/STEF/TEIC</code>
        <courseType rdf:datatype="http://www.w3.org/2001/XMLSchema#string">Elective</courseType>
        <csName rdf:datatype="http://www.w3.org/2001/XMLSchema#string">Computational Intelligence</csName>
    </owl:NamedIndividual>
    


    <!-- http://xworks.gr/ontologies/ccso#IM107s1/IM_MSc/IED/STEF/TEI -->

    <owl:NamedIndividual rdf:about="http://xworks.gr/ontologies/ccso#IM107s1/IM_MSc/IED/STEF/TEI">
        <rdf:type rdf:resource="http://xworks.gr/ontologies/ccso#Syllabus"/>
        <affiliatedWith rdf:resource="http://xworks.gr/ontologies/ccso#Papadourakis_George"/>
        <hasInstructor rdf:resource="http://xworks.gr/ontologies/ccso#Papadourakis_George"/>
        <hasSupervisor rdf:resource="http://xworks.gr/ontologies/ccso#Papadourakis_George"/>
        <syllabusOf rdf:resource="http://xworks.gr/ontologies/ccso#IM107/IM_MSc/IED/STEF/TEIC"/>
        <courseType rdf:datatype="http://www.w3.org/2001/XMLSchema#string">Elective</courseType>
        <creditsECTS rdf:datatype="http://www.w3.org/2001/XMLSchema#decimal">7.5</creditsECTS>
        <csName rdf:datatype="http://www.w3.org/2001/XMLSchema#string">Syllabus of course IM107 Computational Intelligence</csName>
        <semesterinProgram rdf:datatype="http://www.w3.org/2001/XMLSchema#short">1</semesterinProgram>
    </owl:NamedIndividual>
    


    <!-- http://xworks.gr/ontologies/ccso#IM108/IM_MSc/IED/STEF/TEIC -->

    <owl:NamedIndividual rdf:about="http://xworks.gr/ontologies/ccso#IM108/IM_MSc/IED/STEF/TEIC">
        <rdf:type rdf:resource="http://xworks.gr/ontologies/ccso#Course"/>
        <affiliatedWith rdf:resource="http://xworks.gr/ontologies/ccso#Sandi_Elina"/>
        <coversKA rdf:resource="http://xworks.gr/ontologies/ccso#CS/IS_Intelligent_Systems"/>
        <coversKA rdf:resource="http://xworks.gr/ontologies/ccso#CS/SW_Software_Engineering_Software_Systems_and_Applications"/>
        <hasAttender rdf:resource="http://xworks.gr/ontologies/ccso#Sandi_Elina"/>
        <hasSyllabus rdf:resource="http://xworks.gr/ontologies/ccso#IM108s1/IM_MSc/IED/STEF/TEI"/>
        <includedIn rdf:resource="http://xworks.gr/ontologies/ccso#MSc_Informatics_&amp;_Multimedia/IM_MSc/IED/STEF/TEIC"/>
        <offeredBy rdf:resource="http://xworks.gr/ontologies/ccso#Department_of_Informatics_Engineering_of_TEI_of_Crete"/>
        <code rdf:datatype="http://www.w3.org/2001/XMLSchema#string">IM108/IM_MSc/IED/STEF/TEIC</code>
        <courseType rdf:datatype="http://www.w3.org/2001/XMLSchema#string">Elective</courseType>
        <csName rdf:datatype="http://www.w3.org/2001/XMLSchema#string">Embedded Systems</csName>
    </owl:NamedIndividual>
    


    <!-- http://xworks.gr/ontologies/ccso#IM108s1/IM_MSc/IED/STEF/TEI -->

    <owl:NamedIndividual rdf:about="http://xworks.gr/ontologies/ccso#IM108s1/IM_MSc/IED/STEF/TEI">
        <rdf:type rdf:resource="http://xworks.gr/ontologies/ccso#Syllabus"/>
        <affiliatedWith rdf:resource="http://xworks.gr/ontologies/ccso#Kornaros_George"/>
        <hasInstructor rdf:resource="http://xworks.gr/ontologies/ccso#Kornaros_George"/>
        <hasSupervisor rdf:resource="http://xworks.gr/ontologies/ccso#Kornaros_George"/>
        <syllabusOf rdf:resource="http://xworks.gr/ontologies/ccso#IM108/IM_MSc/IED/STEF/TEIC"/>
        <courseType rdf:datatype="http://www.w3.org/2001/XMLSchema#string">Elective</courseType>
        <creditsECTS rdf:datatype="http://www.w3.org/2001/XMLSchema#decimal">7.5</creditsECTS>
        <csName rdf:datatype="http://www.w3.org/2001/XMLSchema#string">Syllabus of course IM108 Embedded Systems</csName>
        <semesterinProgram rdf:datatype="http://www.w3.org/2001/XMLSchema#short">1</semesterinProgram>
    </owl:NamedIndividual>
    


    <!-- http://xworks.gr/ontologies/ccso#IM109/IM_MSc/IED/STEF/TEIC -->

    <owl:NamedIndividual rdf:about="http://xworks.gr/ontologies/ccso#IM109/IM_MSc/IED/STEF/TEIC">
        <rdf:type rdf:resource="http://xworks.gr/ontologies/ccso#Course"/>
        <coversKA rdf:resource="http://xworks.gr/ontologies/ccso#CS/CS_Computational_Science"/>
        <coversKA rdf:resource="http://xworks.gr/ontologies/ccso#CS/IS_Intelligent_Systems"/>
        <hasSyllabus rdf:resource="http://xworks.gr/ontologies/ccso#IM109s1/IM_MSc/IED/STEF/TEI"/>
        <includedIn rdf:resource="http://xworks.gr/ontologies/ccso#MSc_Informatics_&amp;_Multimedia/IM_MSc/IED/STEF/TEIC"/>
        <offeredBy rdf:resource="http://xworks.gr/ontologies/ccso#Department_of_Informatics_Engineering_of_TEI_of_Crete"/>
        <code rdf:datatype="http://www.w3.org/2001/XMLSchema#string">IM109/IM_MSc/IED/STEF/TEIC</code>
        <courseType rdf:datatype="http://www.w3.org/2001/XMLSchema#string">Elective</courseType>
        <csName rdf:datatype="http://www.w3.org/2001/XMLSchema#string">Applied Mathematics</csName>
    </owl:NamedIndividual>
    


    <!-- http://xworks.gr/ontologies/ccso#IM109s1/IM_MSc/IED/STEF/TEI -->

    <owl:NamedIndividual rdf:about="http://xworks.gr/ontologies/ccso#IM109s1/IM_MSc/IED/STEF/TEI">
        <rdf:type rdf:resource="http://xworks.gr/ontologies/ccso#Syllabus"/>
        <affiliatedWith rdf:resource="http://xworks.gr/ontologies/ccso#Karagiannakis_Dimitrios"/>
        <hasInstructor rdf:resource="http://xworks.gr/ontologies/ccso#Karagiannakis_Dimitrios"/>
        <hasSupervisor rdf:resource="http://xworks.gr/ontologies/ccso#Karagiannakis_Dimitrios"/>
        <syllabusOf rdf:resource="http://xworks.gr/ontologies/ccso#IM109/IM_MSc/IED/STEF/TEIC"/>
        <courseType rdf:datatype="http://www.w3.org/2001/XMLSchema#string">Elective</courseType>
        <creditsECTS rdf:datatype="http://www.w3.org/2001/XMLSchema#decimal">7.5</creditsECTS>
        <csName rdf:datatype="http://www.w3.org/2001/XMLSchema#string">Syllabus of course IM109 Applied Mathematics</csName>
        <semesterinProgram rdf:datatype="http://www.w3.org/2001/XMLSchema#short">1</semesterinProgram>
    </owl:NamedIndividual>
    


    <!-- http://xworks.gr/ontologies/ccso#IM201/IM_MSc/IED/STEF/TEIC -->

    <owl:NamedIndividual rdf:about="http://xworks.gr/ontologies/ccso#IM201/IM_MSc/IED/STEF/TEIC">
        <rdf:type rdf:resource="http://xworks.gr/ontologies/ccso#Course"/>
        <affiliatedWith rdf:resource="http://xworks.gr/ontologies/ccso#Agrimakis_Samson"/>
        <affiliatedWith rdf:resource="http://xworks.gr/ontologies/ccso#Dallas_Nektarios"/>
        <affiliatedWith rdf:resource="http://xworks.gr/ontologies/ccso#Hionis_John"/>
        <affiliatedWith rdf:resource="http://xworks.gr/ontologies/ccso#Kokkinos_Heraklis"/>
        <affiliatedWith rdf:resource="http://xworks.gr/ontologies/ccso#Martelis_Stelios"/>
        <affiliatedWith rdf:resource="http://xworks.gr/ontologies/ccso#Starkeiou_Aria"/>
        <affiliatedWith rdf:resource="http://xworks.gr/ontologies/ccso#Triantafillou_Irene"/>
        <affiliatedWith rdf:resource="http://xworks.gr/ontologies/ccso#Vassileiou_Tom"/>
        <hasAttender rdf:resource="http://xworks.gr/ontologies/ccso#Agrimakis_Samson"/>
        <hasAttender rdf:resource="http://xworks.gr/ontologies/ccso#Dallas_Nektarios"/>
        <hasAttender rdf:resource="http://xworks.gr/ontologies/ccso#Hionis_John"/>
        <hasAttender rdf:resource="http://xworks.gr/ontologies/ccso#Kokkinos_Heraklis"/>
        <hasAttender rdf:resource="http://xworks.gr/ontologies/ccso#Martelis_Stelios"/>
        <hasAttender rdf:resource="http://xworks.gr/ontologies/ccso#Starkeiou_Aria"/>
        <hasAttender rdf:resource="http://xworks.gr/ontologies/ccso#Triantafillou_Irene"/>
        <hasAttender rdf:resource="http://xworks.gr/ontologies/ccso#Vassileiou_Tom"/>
        <hasSyllabus rdf:resource="http://xworks.gr/ontologies/ccso#IM201s1/IM_MSc/IED/STEF/TEI"/>
        <includedIn rdf:resource="http://xworks.gr/ontologies/ccso#MSc_Informatics_&amp;_Multimedia/IM_MSc/IED/STEF/TEIC"/>
        <offeredBy rdf:resource="http://xworks.gr/ontologies/ccso#Department_of_Informatics_Engineering_of_TEI_of_Crete"/>
        <code rdf:datatype="http://www.w3.org/2001/XMLSchema#string">IM201/IM_MSc/IED/STEF/TEIC</code>
        <courseType rdf:datatype="http://www.w3.org/2001/XMLSchema#string">Core</courseType>
        <csName rdf:datatype="http://www.w3.org/2001/XMLSchema#string">Data Structures and Algorithms</csName>
    </owl:NamedIndividual>
    


    <!-- http://xworks.gr/ontologies/ccso#IM201s1/IM_MSc/IED/STEF/TEI -->

    <owl:NamedIndividual rdf:about="http://xworks.gr/ontologies/ccso#IM201s1/IM_MSc/IED/STEF/TEI">
        <rdf:type rdf:resource="http://xworks.gr/ontologies/ccso#Syllabus"/>
        <affiliatedWith rdf:resource="http://xworks.gr/ontologies/ccso#Fragopoulou_Paraskevi"/>
        <affiliatedWith rdf:resource="http://xworks.gr/ontologies/ccso#Katis_Evangelos"/>
        <affiliatedWith rdf:resource="http://xworks.gr/ontologies/ccso#Malamos_Athanasios"/>
        <coversTopic rdf:resource="http://xworks.gr/ontologies/ccso#CS/PL/T_Object-Oriented_Design,Class-Hierarchy_design_for_modeling"/>
        <coversTopic rdf:resource="http://xworks.gr/ontologies/ccso#CS/PL/T_Subclasses,Inheritance,and_Method_Overriding"/>
        <followsTEMethod rdf:resource="http://xworks.gr/ontologies/ccso#Homework"/>
        <followsTEMethod rdf:resource="http://xworks.gr/ontologies/ccso#Lecture"/>
        <followsTEMethod rdf:resource="http://xworks.gr/ontologies/ccso#WrittenExam"/>
        <hasCourseAssistant rdf:resource="http://xworks.gr/ontologies/ccso#Katis_Evangelos"/>
        <hasInstructor rdf:resource="http://xworks.gr/ontologies/ccso#Fragopoulou_Paraskevi"/>
        <hasLM rdf:resource="http://xworks.gr/ontologies/ccso#AlgorithmDesign_F-A-IE"/>
        <hasSupervisor rdf:resource="http://xworks.gr/ontologies/ccso#Malamos_Athanasios"/>
        <syllabusOf rdf:resource="http://xworks.gr/ontologies/ccso#IM201/IM_MSc/IED/STEF/TEIC"/>
        <code rdf:datatype="http://www.w3.org/2001/XMLSchema#string">IM201s1/IM_MSc/IED/STEF/TEI</code>
        <courseType rdf:datatype="http://www.w3.org/2001/XMLSchema#string">Core</courseType>
        <courseURL rdf:datatype="http://www.w3.org/2001/XMLSchema#anyURI">https://www.teicrete.gr/mscie/en/department-informatics-engineering/%CE%BC%CE%AC%CE%B8%CE%B7%CE%BC%CE%B1/data-structures-and-algorithms</courseURL>
        <creditsECTS rdf:datatype="http://www.w3.org/2001/XMLSchema#decimal">7.5</creditsECTS>
        <csName rdf:datatype="http://www.w3.org/2001/XMLSchema#string">Syllabus of course IM201 Data Structures and Algorithms</csName>
        <description rdf:datatype="http://www.w3.org/2001/XMLSchema#string">The course commands a central role in computer science it both theoretical and practical levels, in many cases covering themes beyond the subject of informatics. The course strives for students to understand fundamental ways or data organization in computer memory and to learn and implement techniques for the handling of that data. Special attention is placed on creating new data algorithms with an obvious result on the dexterities of students to handle such problems.</description>
        <language rdf:datatype="http://www.w3.org/2001/XMLSchema#string">Greek</language>
        <semesterinProgram rdf:datatype="http://www.w3.org/2001/XMLSchema#short">2</semesterinProgram>
        <webaddressURL rdf:datatype="http://www.w3.org/2001/XMLSchema#anyURI">https://www.teicrete.gr/mscie/en/department-informatics-engineering/%CE%BC%CE%AC%CE%B8%CE%B7%CE%BC%CE%B1/data-structures-and-algorithms</webaddressURL>
        <weeklyHours rdf:datatype="http://www.w3.org/2001/XMLSchema#short">3</weeklyHours>
    </owl:NamedIndividual>
    


    <!-- http://xworks.gr/ontologies/ccso#IM202/IM_MSc/IED/STEF/TEIC -->

    <owl:NamedIndividual rdf:about="http://xworks.gr/ontologies/ccso#IM202/IM_MSc/IED/STEF/TEIC">
        <rdf:type rdf:resource="http://xworks.gr/ontologies/ccso#Course"/>
        <affiliatedWith rdf:resource="http://xworks.gr/ontologies/ccso#Vassileiou_Tom"/>
        <coversKA rdf:resource="http://xworks.gr/ontologies/ccso#CS/NC_Networking_and_Communication"/>
        <hasAttender rdf:resource="http://xworks.gr/ontologies/ccso#Vassileiou_Tom"/>
        <hasSyllabus rdf:resource="http://xworks.gr/ontologies/ccso#IM202s1/IM_MSc/IED/STEF/TEI"/>
        <includedIn rdf:resource="http://xworks.gr/ontologies/ccso#MSc_Informatics_&amp;_Multimedia/IM_MSc/IED/STEF/TEIC"/>
        <offeredBy rdf:resource="http://xworks.gr/ontologies/ccso#Department_of_Informatics_Engineering_of_TEI_of_Crete"/>
        <code rdf:datatype="http://www.w3.org/2001/XMLSchema#string">IM202/IM_MSc/IED/STEF/TEIC</code>
        <courseType rdf:datatype="http://www.w3.org/2001/XMLSchema#string">Elective</courseType>
        <csName rdf:datatype="http://www.w3.org/2001/XMLSchema#string">Wireless Networks</csName>
    </owl:NamedIndividual>
    


    <!-- http://xworks.gr/ontologies/ccso#IM202s1/IM_MSc/IED/STEF/TEI -->

    <owl:NamedIndividual rdf:about="http://xworks.gr/ontologies/ccso#IM202s1/IM_MSc/IED/STEF/TEI">
        <rdf:type rdf:resource="http://xworks.gr/ontologies/ccso#Syllabus"/>
        <affiliatedWith rdf:resource="http://xworks.gr/ontologies/ccso#Kondylakis_Haridimos"/>
        <affiliatedWith rdf:resource="http://xworks.gr/ontologies/ccso#Pallis_Evangelos"/>
        <affiliatedWith rdf:resource="http://xworks.gr/ontologies/ccso#Vidakis_Nikolaos"/>
        <hasCourseAssistant rdf:resource="http://xworks.gr/ontologies/ccso#Kondylakis_Haridimos"/>
        <hasInstructor rdf:resource="http://xworks.gr/ontologies/ccso#Pallis_Evangelos"/>
        <hasInstructor rdf:resource="http://xworks.gr/ontologies/ccso#Vidakis_Nikolaos"/>
        <hasSupervisor rdf:resource="http://xworks.gr/ontologies/ccso#Pallis_Evangelos"/>
        <syllabusOf rdf:resource="http://xworks.gr/ontologies/ccso#IM202/IM_MSc/IED/STEF/TEIC"/>
        <courseType rdf:datatype="http://www.w3.org/2001/XMLSchema#string">Elective</courseType>
        <creditsECTS rdf:datatype="http://www.w3.org/2001/XMLSchema#decimal">7.5</creditsECTS>
        <csName rdf:datatype="http://www.w3.org/2001/XMLSchema#string">Syllabus of course IM202 Wireless Networks</csName>
        <semesterinProgram rdf:datatype="http://www.w3.org/2001/XMLSchema#short">2</semesterinProgram>
    </owl:NamedIndividual>
    


    <!-- http://xworks.gr/ontologies/ccso#IM203/IM_MSc/IED/STEF/TEIC -->

    <owl:NamedIndividual rdf:about="http://xworks.gr/ontologies/ccso#IM203/IM_MSc/IED/STEF/TEIC">
        <rdf:type rdf:resource="http://xworks.gr/ontologies/ccso#Course"/>
        <affiliatedWith rdf:resource="http://xworks.gr/ontologies/ccso#Triantafillou_Irene"/>
        <affiliatedWith rdf:resource="http://xworks.gr/ontologies/ccso#Vassileiou_Tom"/>
        <coversKA rdf:resource="http://xworks.gr/ontologies/ccso#CS/NC_Networking_and_Communication"/>
        <hasAttender rdf:resource="http://xworks.gr/ontologies/ccso#Triantafillou_Irene"/>
        <hasAttender rdf:resource="http://xworks.gr/ontologies/ccso#Vassileiou_Tom"/>
        <hasSyllabus rdf:resource="http://xworks.gr/ontologies/ccso#IM203s1/IM_MSc/IED/STEF/TEI"/>
        <includedIn rdf:resource="http://xworks.gr/ontologies/ccso#MSc_Informatics_&amp;_Multimedia/IM_MSc/IED/STEF/TEIC"/>
        <offeredBy rdf:resource="http://xworks.gr/ontologies/ccso#Department_of_Informatics_Engineering_of_TEI_of_Crete"/>
        <code rdf:datatype="http://www.w3.org/2001/XMLSchema#string">IM203/IM_MSc/IED/STEF/TEIC</code>
        <courseType rdf:datatype="http://www.w3.org/2001/XMLSchema#string">Elective</courseType>
        <csName rdf:datatype="http://www.w3.org/2001/XMLSchema#string">Advanced Topics in Antennas and Wireless Propagation and Measurements</csName>
    </owl:NamedIndividual>
    


    <!-- http://xworks.gr/ontologies/ccso#IM203s1/IM_MSc/IED/STEF/TEI -->

    <owl:NamedIndividual rdf:about="http://xworks.gr/ontologies/ccso#IM203s1/IM_MSc/IED/STEF/TEI">
        <rdf:type rdf:resource="http://xworks.gr/ontologies/ccso#Syllabus"/>
        <affiliatedWith rdf:resource="http://xworks.gr/ontologies/ccso#Stratakis_Dimitrios"/>
        <hasInstructor rdf:resource="http://xworks.gr/ontologies/ccso#Stratakis_Dimitrios"/>
        <hasSupervisor rdf:resource="http://xworks.gr/ontologies/ccso#Stratakis_Dimitrios"/>
        <syllabusOf rdf:resource="http://xworks.gr/ontologies/ccso#IM203/IM_MSc/IED/STEF/TEIC"/>
        <courseType rdf:datatype="http://www.w3.org/2001/XMLSchema#string">Elective</courseType>
        <creditsECTS rdf:datatype="http://www.w3.org/2001/XMLSchema#decimal">7.5</creditsECTS>
        <csName rdf:datatype="http://www.w3.org/2001/XMLSchema#string">Syllabus of course IM203 Advanced Topics in Antennas and Wireless Propagation and Measurements</csName>
        <semesterinProgram rdf:datatype="http://www.w3.org/2001/XMLSchema#short">2</semesterinProgram>
    </owl:NamedIndividual>
    


    <!-- http://xworks.gr/ontologies/ccso#IM204/IM_MSc/IED/STEF/TEIC -->

    <owl:NamedIndividual rdf:about="http://xworks.gr/ontologies/ccso#IM204/IM_MSc/IED/STEF/TEIC">
        <rdf:type rdf:resource="http://xworks.gr/ontologies/ccso#Course"/>
        <affiliatedWith rdf:resource="http://xworks.gr/ontologies/ccso#Dallas_Nektarios"/>
        <coversKA rdf:resource="http://xworks.gr/ontologies/ccso#CS/NC_Networking_and_Communication"/>
        <coversKA rdf:resource="http://xworks.gr/ontologies/ccso#CS/PD_Parallel_and_Distributed_Computing"/>
        <hasAttender rdf:resource="http://xworks.gr/ontologies/ccso#Dallas_Nektarios"/>
        <hasSyllabus rdf:resource="http://xworks.gr/ontologies/ccso#IM204s1/IM_MSc/IED/STEF/TEI"/>
        <includedIn rdf:resource="http://xworks.gr/ontologies/ccso#MSc_Informatics_&amp;_Multimedia/IM_MSc/IED/STEF/TEIC"/>
        <offeredBy rdf:resource="http://xworks.gr/ontologies/ccso#Department_of_Informatics_Engineering_of_TEI_of_Crete"/>
        <code rdf:datatype="http://www.w3.org/2001/XMLSchema#string">IM204/IM_MSc/IED/STEF/TEIC</code>
        <courseType rdf:datatype="http://www.w3.org/2001/XMLSchema#string">Elective</courseType>
        <csName rdf:datatype="http://www.w3.org/2001/XMLSchema#string">Distributed Systems and Applications</csName>
    </owl:NamedIndividual>
    


    <!-- http://xworks.gr/ontologies/ccso#IM204s1/IM_MSc/IED/STEF/TEI -->

    <owl:NamedIndividual rdf:about="http://xworks.gr/ontologies/ccso#IM204s1/IM_MSc/IED/STEF/TEI">
        <rdf:type rdf:resource="http://xworks.gr/ontologies/ccso#Syllabus"/>
        <affiliatedWith rdf:resource="http://xworks.gr/ontologies/ccso#Fragopoulou_Paraskevi"/>
        <hasInstructor rdf:resource="http://xworks.gr/ontologies/ccso#Fragopoulou_Paraskevi"/>
        <hasSupervisor rdf:resource="http://xworks.gr/ontologies/ccso#Fragopoulou_Paraskevi"/>
        <syllabusOf rdf:resource="http://xworks.gr/ontologies/ccso#IM204/IM_MSc/IED/STEF/TEIC"/>
        <courseType rdf:datatype="http://www.w3.org/2001/XMLSchema#string">Elective</courseType>
        <creditsECTS rdf:datatype="http://www.w3.org/2001/XMLSchema#decimal">7.5</creditsECTS>
        <csName rdf:datatype="http://www.w3.org/2001/XMLSchema#string">Syllabus of course IM204 Distributed Systems and Applications</csName>
        <semesterinProgram rdf:datatype="http://www.w3.org/2001/XMLSchema#short">2</semesterinProgram>
    </owl:NamedIndividual>
    


    <!-- http://xworks.gr/ontologies/ccso#IM205/IM_MSc/IED/STEF/TEIC -->

    <owl:NamedIndividual rdf:about="http://xworks.gr/ontologies/ccso#IM205/IM_MSc/IED/STEF/TEIC">
        <rdf:type rdf:resource="http://xworks.gr/ontologies/ccso#Course"/>
        <affiliatedWith rdf:resource="http://xworks.gr/ontologies/ccso#Martelis_Stelios"/>
        <affiliatedWith rdf:resource="http://xworks.gr/ontologies/ccso#Starkeiou_Aria"/>
        <affiliatedWith rdf:resource="http://xworks.gr/ontologies/ccso#Triantafillou_Irene"/>
        <affiliatedWith rdf:resource="http://xworks.gr/ontologies/ccso#Vassileiou_Tom"/>
        <coversKA rdf:resource="http://xworks.gr/ontologies/ccso#CS/IS_Intelligent_Systems"/>
        <coversKA rdf:resource="http://xworks.gr/ontologies/ccso#CS/NC_Networking_and_Communication"/>
        <hasAttender rdf:resource="http://xworks.gr/ontologies/ccso#Martelis_Stelios"/>
        <hasAttender rdf:resource="http://xworks.gr/ontologies/ccso#Starkeiou_Aria"/>
        <hasAttender rdf:resource="http://xworks.gr/ontologies/ccso#Triantafillou_Irene"/>
        <hasAttender rdf:resource="http://xworks.gr/ontologies/ccso#Vassileiou_Tom"/>
        <hasSyllabus rdf:resource="http://xworks.gr/ontologies/ccso#IM205s1/IM_MSc/IED/STEF/TEI"/>
        <includedIn rdf:resource="http://xworks.gr/ontologies/ccso#MSc_Informatics_&amp;_Multimedia/IM_MSc/IED/STEF/TEIC"/>
        <offeredBy rdf:resource="http://xworks.gr/ontologies/ccso#Department_of_Informatics_Engineering_of_TEI_of_Crete"/>
        <code rdf:datatype="http://www.w3.org/2001/XMLSchema#string">IM205/IM_MSc/IED/STEF/TEIC</code>
        <courseType rdf:datatype="http://www.w3.org/2001/XMLSchema#string">Elective</courseType>
        <csName rdf:datatype="http://www.w3.org/2001/XMLSchema#string">Network Security</csName>
    </owl:NamedIndividual>
    


    <!-- http://xworks.gr/ontologies/ccso#IM205s1/IM_MSc/IED/STEF/TEI -->

    <owl:NamedIndividual rdf:about="http://xworks.gr/ontologies/ccso#IM205s1/IM_MSc/IED/STEF/TEI">
        <rdf:type rdf:resource="http://xworks.gr/ontologies/ccso#Syllabus"/>
        <affiliatedWith rdf:resource="http://xworks.gr/ontologies/ccso#Manifavas_Harry"/>
        <hasInstructor rdf:resource="http://xworks.gr/ontologies/ccso#Manifavas_Harry"/>
        <hasSupervisor rdf:resource="http://xworks.gr/ontologies/ccso#Manifavas_Harry"/>
        <syllabusOf rdf:resource="http://xworks.gr/ontologies/ccso#IM205/IM_MSc/IED/STEF/TEIC"/>
        <courseType rdf:datatype="http://www.w3.org/2001/XMLSchema#string">Elective</courseType>
        <creditsECTS rdf:datatype="http://www.w3.org/2001/XMLSchema#decimal">7.5</creditsECTS>
        <csName rdf:datatype="http://www.w3.org/2001/XMLSchema#string">Syllabus of course IM205 Network Security</csName>
        <semesterinProgram rdf:datatype="http://www.w3.org/2001/XMLSchema#short">2</semesterinProgram>
    </owl:NamedIndividual>
    


    <!-- http://xworks.gr/ontologies/ccso#IM206/IM_MSc/IED/STEF/TEIC -->

    <owl:NamedIndividual rdf:about="http://xworks.gr/ontologies/ccso#IM206/IM_MSc/IED/STEF/TEIC">
        <rdf:type rdf:resource="http://xworks.gr/ontologies/ccso#Course"/>
        <affiliatedWith rdf:resource="http://xworks.gr/ontologies/ccso#Agrimakis_Samson"/>
        <coversKA rdf:resource="http://xworks.gr/ontologies/ccso#CS/SW_Software_Engineering_Software_Systems_and_Applications"/>
        <hasAttender rdf:resource="http://xworks.gr/ontologies/ccso#Agrimakis_Samson"/>
        <hasSyllabus rdf:resource="http://xworks.gr/ontologies/ccso#IM206s1/IM_MSc/IED/STEF/TEI"/>
        <includedIn rdf:resource="http://xworks.gr/ontologies/ccso#MSc_Informatics_&amp;_Multimedia/IM_MSc/IED/STEF/TEIC"/>
        <offeredBy rdf:resource="http://xworks.gr/ontologies/ccso#Department_of_Informatics_Engineering_of_TEI_of_Crete"/>
        <code rdf:datatype="http://www.w3.org/2001/XMLSchema#string">IM206/IM_MSc/IED/STEF/TEIC</code>
        <courseType rdf:datatype="http://www.w3.org/2001/XMLSchema#string">Elective</courseType>
        <csName rdf:datatype="http://www.w3.org/2001/XMLSchema#string">Realisitic Multimedia and Animation</csName>
    </owl:NamedIndividual>
    


    <!-- http://xworks.gr/ontologies/ccso#IM206s1/IM_MSc/IED/STEF/TEI -->

    <owl:NamedIndividual rdf:about="http://xworks.gr/ontologies/ccso#IM206s1/IM_MSc/IED/STEF/TEI">
        <rdf:type rdf:resource="http://xworks.gr/ontologies/ccso#Syllabus"/>
        <affiliatedWith rdf:resource="http://xworks.gr/ontologies/ccso#Pachoulakis_Ioannis"/>
        <hasInstructor rdf:resource="http://xworks.gr/ontologies/ccso#Pachoulakis_Ioannis"/>
        <hasSupervisor rdf:resource="http://xworks.gr/ontologies/ccso#Pachoulakis_Ioannis"/>
        <syllabusOf rdf:resource="http://xworks.gr/ontologies/ccso#IM206/IM_MSc/IED/STEF/TEIC"/>
        <courseType rdf:datatype="http://www.w3.org/2001/XMLSchema#string">Elective</courseType>
        <creditsECTS rdf:datatype="http://www.w3.org/2001/XMLSchema#decimal">7.5</creditsECTS>
        <csName rdf:datatype="http://www.w3.org/2001/XMLSchema#string">Syllabus of course IM206 Realisitic Multimedia and Animation</csName>
        <semesterinProgram rdf:datatype="http://www.w3.org/2001/XMLSchema#short">2</semesterinProgram>
    </owl:NamedIndividual>
    


    <!-- http://xworks.gr/ontologies/ccso#IM207/IM_MSc/IED/STEF/TEIC -->

    <owl:NamedIndividual rdf:about="http://xworks.gr/ontologies/ccso#IM207/IM_MSc/IED/STEF/TEIC">
        <rdf:type rdf:resource="http://xworks.gr/ontologies/ccso#Course"/>
        <affiliatedWith rdf:resource="http://xworks.gr/ontologies/ccso#Hionis_John"/>
        <affiliatedWith rdf:resource="http://xworks.gr/ontologies/ccso#Kokkinos_Heraklis"/>
        <coversKA rdf:resource="http://xworks.gr/ontologies/ccso#CS/CVR_Computer_Vision_and_Robotics"/>
        <coversKA rdf:resource="http://xworks.gr/ontologies/ccso#CS/IS_Intelligent_Systems"/>
        <hasAttender rdf:resource="http://xworks.gr/ontologies/ccso#Hionis_John"/>
        <hasAttender rdf:resource="http://xworks.gr/ontologies/ccso#Kokkinos_Heraklis"/>
        <hasSyllabus rdf:resource="http://xworks.gr/ontologies/ccso#IM207s1/IM_MSc/IED/STEF/TEI"/>
        <includedIn rdf:resource="http://xworks.gr/ontologies/ccso#MSc_Informatics_&amp;_Multimedia/IM_MSc/IED/STEF/TEIC"/>
        <offeredBy rdf:resource="http://xworks.gr/ontologies/ccso#Department_of_Informatics_Engineering_of_TEI_of_Crete"/>
        <code rdf:datatype="http://www.w3.org/2001/XMLSchema#string">IM207/IM_MSc/IED/STEF/TEIC</code>
        <courseType rdf:datatype="http://www.w3.org/2001/XMLSchema#string">Elective</courseType>
        <csName rdf:datatype="http://www.w3.org/2001/XMLSchema#string">Advanced Topics in Artificial Intelligence</csName>
    </owl:NamedIndividual>
    


    <!-- http://xworks.gr/ontologies/ccso#IM207s1/IM_MSc/IED/STEF/TEI -->

    <owl:NamedIndividual rdf:about="http://xworks.gr/ontologies/ccso#IM207s1/IM_MSc/IED/STEF/TEI">
        <rdf:type rdf:resource="http://xworks.gr/ontologies/ccso#Syllabus"/>
        <affiliatedWith rdf:resource="http://xworks.gr/ontologies/ccso#Marakakis_Manolis"/>
        <hasInstructor rdf:resource="http://xworks.gr/ontologies/ccso#Marakakis_Manolis"/>
        <hasSupervisor rdf:resource="http://xworks.gr/ontologies/ccso#Marakakis_Manolis"/>
        <syllabusOf rdf:resource="http://xworks.gr/ontologies/ccso#IM207/IM_MSc/IED/STEF/TEIC"/>
        <courseType rdf:datatype="http://www.w3.org/2001/XMLSchema#string">Elective</courseType>
        <creditsECTS rdf:datatype="http://www.w3.org/2001/XMLSchema#decimal">7.5</creditsECTS>
        <csName rdf:datatype="http://www.w3.org/2001/XMLSchema#string">Syllabus of course IM207 Advanced Topics in Artificial Intelligence</csName>
        <semesterinProgram rdf:datatype="http://www.w3.org/2001/XMLSchema#short">2</semesterinProgram>
    </owl:NamedIndividual>
    


    <!-- http://xworks.gr/ontologies/ccso#IM208/IM_MSc/IED/STEF/TEIC -->

    <owl:NamedIndividual rdf:about="http://xworks.gr/ontologies/ccso#IM208/IM_MSc/IED/STEF/TEIC">
        <rdf:type rdf:resource="http://xworks.gr/ontologies/ccso#Course"/>
        <affiliatedWith rdf:resource="http://xworks.gr/ontologies/ccso#Hionis_John"/>
        <affiliatedWith rdf:resource="http://xworks.gr/ontologies/ccso#Vassileiou_Tom"/>
        <coversKA rdf:resource="http://xworks.gr/ontologies/ccso#CS/SW_Software_Engineering_Software_Systems_and_Applications"/>
        <hasAttender rdf:resource="http://xworks.gr/ontologies/ccso#Hionis_John"/>
        <hasAttender rdf:resource="http://xworks.gr/ontologies/ccso#Vassileiou_Tom"/>
        <hasSyllabus rdf:resource="http://xworks.gr/ontologies/ccso#IM208s1/IM_MSc/IED/STEF/TEI"/>
        <includedIn rdf:resource="http://xworks.gr/ontologies/ccso#MSc_Informatics_&amp;_Multimedia/IM_MSc/IED/STEF/TEIC"/>
        <offeredBy rdf:resource="http://xworks.gr/ontologies/ccso#Department_of_Informatics_Engineering_of_TEI_of_Crete"/>
        <code rdf:datatype="http://www.w3.org/2001/XMLSchema#string">IM208/IM_MSc/IED/STEF/TEIC</code>
        <courseType rdf:datatype="http://www.w3.org/2001/XMLSchema#string">Elective</courseType>
        <csName rdf:datatype="http://www.w3.org/2001/XMLSchema#string">Computer-Supported Collaboration</csName>
    </owl:NamedIndividual>
    


    <!-- http://xworks.gr/ontologies/ccso#IM208s1/IM_MSc/IED/STEF/TEI -->

    <owl:NamedIndividual rdf:about="http://xworks.gr/ontologies/ccso#IM208s1/IM_MSc/IED/STEF/TEI">
        <rdf:type rdf:resource="http://xworks.gr/ontologies/ccso#Syllabus"/>
        <affiliatedWith rdf:resource="http://xworks.gr/ontologies/ccso#Akoumianakis_Demosthenes"/>
        <hasInstructor rdf:resource="http://xworks.gr/ontologies/ccso#Akoumianakis_Demosthenes"/>
        <hasSupervisor rdf:resource="http://xworks.gr/ontologies/ccso#Akoumianakis_Demosthenes"/>
        <syllabusOf rdf:resource="http://xworks.gr/ontologies/ccso#IM208/IM_MSc/IED/STEF/TEIC"/>
        <courseType rdf:datatype="http://www.w3.org/2001/XMLSchema#string">Elective</courseType>
        <creditsECTS rdf:datatype="http://www.w3.org/2001/XMLSchema#decimal">7.5</creditsECTS>
        <csName rdf:datatype="http://www.w3.org/2001/XMLSchema#string">Syllabus of course IM208 Computer-Supported Collaboration</csName>
        <semesterinProgram rdf:datatype="http://www.w3.org/2001/XMLSchema#short">2</semesterinProgram>
    </owl:NamedIndividual>
    


    <!-- http://xworks.gr/ontologies/ccso#IM209/IM_MSc/IED/STEF/TEIC -->

    <owl:NamedIndividual rdf:about="http://xworks.gr/ontologies/ccso#IM209/IM_MSc/IED/STEF/TEIC">
        <rdf:type rdf:resource="http://xworks.gr/ontologies/ccso#Course"/>
        <affiliatedWith rdf:resource="http://xworks.gr/ontologies/ccso#Agrimakis_Samson"/>
        <affiliatedWith rdf:resource="http://xworks.gr/ontologies/ccso#Dallas_Nektarios"/>
        <affiliatedWith rdf:resource="http://xworks.gr/ontologies/ccso#Hionis_John"/>
        <affiliatedWith rdf:resource="http://xworks.gr/ontologies/ccso#Kokkinos_Heraklis"/>
        <affiliatedWith rdf:resource="http://xworks.gr/ontologies/ccso#Martelis_Stelios"/>
        <affiliatedWith rdf:resource="http://xworks.gr/ontologies/ccso#Starkeiou_Aria"/>
        <affiliatedWith rdf:resource="http://xworks.gr/ontologies/ccso#Vassileiou_Tom"/>
        <coversKA rdf:resource="http://xworks.gr/ontologies/ccso#CS/IM_Information_Management"/>
        <coversKA rdf:resource="http://xworks.gr/ontologies/ccso#CS/SW_Software_Engineering_Software_Systems_and_Applications"/>
        <hasAttender rdf:resource="http://xworks.gr/ontologies/ccso#Agrimakis_Samson"/>
        <hasAttender rdf:resource="http://xworks.gr/ontologies/ccso#Dallas_Nektarios"/>
        <hasAttender rdf:resource="http://xworks.gr/ontologies/ccso#Hionis_John"/>
        <hasAttender rdf:resource="http://xworks.gr/ontologies/ccso#Kokkinos_Heraklis"/>
        <hasAttender rdf:resource="http://xworks.gr/ontologies/ccso#Martelis_Stelios"/>
        <hasAttender rdf:resource="http://xworks.gr/ontologies/ccso#Starkeiou_Aria"/>
        <hasAttender rdf:resource="http://xworks.gr/ontologies/ccso#Vassileiou_Tom"/>
        <hasSyllabus rdf:resource="http://xworks.gr/ontologies/ccso#IM209s1/IM_MSc/IED/STEF/TEI"/>
        <includedIn rdf:resource="http://xworks.gr/ontologies/ccso#MSc_Informatics_&amp;_Multimedia/IM_MSc/IED/STEF/TEIC"/>
        <offeredBy rdf:resource="http://xworks.gr/ontologies/ccso#Department_of_Informatics_Engineering_of_TEI_of_Crete"/>
        <code rdf:datatype="http://www.w3.org/2001/XMLSchema#string">IM209/IM_MSc/IED/STEF/TEIC</code>
        <courseType rdf:datatype="http://www.w3.org/2001/XMLSchema#string">Elective</courseType>
        <csName rdf:datatype="http://www.w3.org/2001/XMLSchema#string">Information and Communication Technologies (ICT) and Education</csName>
    </owl:NamedIndividual>
    


    <!-- http://xworks.gr/ontologies/ccso#IM209s1/IM_MSc/IED/STEF/TEI -->

    <owl:NamedIndividual rdf:about="http://xworks.gr/ontologies/ccso#IM209s1/IM_MSc/IED/STEF/TEI">
        <rdf:type rdf:resource="http://xworks.gr/ontologies/ccso#Syllabus"/>
        <affiliatedWith rdf:resource="http://xworks.gr/ontologies/ccso#Kalogiannakis_Michail"/>
        <affiliatedWith rdf:resource="http://xworks.gr/ontologies/ccso#Katis_Evangelos"/>
        <affiliatedWith rdf:resource="http://xworks.gr/ontologies/ccso#Vassilakis_Kostas"/>
        <followsTEMethod rdf:resource="http://xworks.gr/ontologies/ccso#Discussion"/>
        <followsTEMethod rdf:resource="http://xworks.gr/ontologies/ccso#Project"/>
        <hasCourseAssistant rdf:resource="http://xworks.gr/ontologies/ccso#Katis_Evangelos"/>
        <hasInstructor rdf:resource="http://xworks.gr/ontologies/ccso#Kalogiannakis_Michail"/>
        <hasInstructor rdf:resource="http://xworks.gr/ontologies/ccso#Vassilakis_Kostas"/>
        <hasSupervisor rdf:resource="http://xworks.gr/ontologies/ccso#Vassilakis_Kostas"/>
        <syllabusOf rdf:resource="http://xworks.gr/ontologies/ccso#IM209/IM_MSc/IED/STEF/TEIC"/>
        <code rdf:datatype="http://www.w3.org/2001/XMLSchema#string">IM209s1/IM_MSc/IED/STEF/TEI</code>
        <courseType rdf:datatype="http://www.w3.org/2001/XMLSchema#string">Elective</courseType>
        <creditsECTS rdf:datatype="http://www.w3.org/2001/XMLSchema#decimal">7.5</creditsECTS>
        <csName rdf:datatype="http://www.w3.org/2001/XMLSchema#string">Syllabus of course IM209 Information and Communication Technologies (ICT) and Education</csName>
        <semesterinProgram rdf:datatype="http://www.w3.org/2001/XMLSchema#short">2</semesterinProgram>
        <weeklyHours rdf:datatype="http://www.w3.org/2001/XMLSchema#short">3</weeklyHours>
    </owl:NamedIndividual>
    


    <!-- http://xworks.gr/ontologies/ccso#IM210/IM_MSc/IED/STEF/TEIC -->

    <owl:NamedIndividual rdf:about="http://xworks.gr/ontologies/ccso#IM210/IM_MSc/IED/STEF/TEIC">
        <rdf:type rdf:resource="http://xworks.gr/ontologies/ccso#Course"/>
        <coversKA rdf:resource="http://xworks.gr/ontologies/ccso#CS/CVR_Computer_Vision_and_Robotics"/>
        <coversKA rdf:resource="http://xworks.gr/ontologies/ccso#CS/IS_Intelligent_Systems"/>
        <coversKA rdf:resource="http://xworks.gr/ontologies/ccso#CS/SW_Software_Engineering_Software_Systems_and_Applications"/>
        <hasSyllabus rdf:resource="http://xworks.gr/ontologies/ccso#IM210s1/IM_MSc/IED/STEF/TEI"/>
        <includedIn rdf:resource="http://xworks.gr/ontologies/ccso#MSc_Informatics_&amp;_Multimedia/IM_MSc/IED/STEF/TEIC"/>
        <offeredBy rdf:resource="http://xworks.gr/ontologies/ccso#Department_of_Informatics_Engineering_of_TEI_of_Crete"/>
        <code rdf:datatype="http://www.w3.org/2001/XMLSchema#string">IM210/IM_MSc/IED/STEF/TEIC</code>
        <courseType rdf:datatype="http://www.w3.org/2001/XMLSchema#string">Elective</courseType>
        <csName rdf:datatype="http://www.w3.org/2001/XMLSchema#string">Advances on Digital Imaging and Computer Vision</csName>
    </owl:NamedIndividual>
    


    <!-- http://xworks.gr/ontologies/ccso#IM210s1/IM_MSc/IED/STEF/TEI -->

    <owl:NamedIndividual rdf:about="http://xworks.gr/ontologies/ccso#IM210s1/IM_MSc/IED/STEF/TEI">
        <rdf:type rdf:resource="http://xworks.gr/ontologies/ccso#Syllabus"/>
        <affiliatedWith rdf:resource="http://xworks.gr/ontologies/ccso#Triantafyllidis_George"/>
        <hasInstructor rdf:resource="http://xworks.gr/ontologies/ccso#Triantafyllidis_George"/>
        <hasSupervisor rdf:resource="http://xworks.gr/ontologies/ccso#Triantafyllidis_George"/>
        <syllabusOf rdf:resource="http://xworks.gr/ontologies/ccso#IM210/IM_MSc/IED/STEF/TEIC"/>
        <courseType rdf:datatype="http://www.w3.org/2001/XMLSchema#string">Elective</courseType>
        <creditsECTS rdf:datatype="http://www.w3.org/2001/XMLSchema#decimal">7.5</creditsECTS>
        <csName rdf:datatype="http://www.w3.org/2001/XMLSchema#string">Syllabus of course IM210 Advances on Digital Imaging and Computer Vision</csName>
        <semesterinProgram rdf:datatype="http://www.w3.org/2001/XMLSchema#short">2</semesterinProgram>
    </owl:NamedIndividual>
    


    <!-- http://xworks.gr/ontologies/ccso#IM211/IM_MSc/IED/STEF/TEIC -->

    <owl:NamedIndividual rdf:about="http://xworks.gr/ontologies/ccso#IM211/IM_MSc/IED/STEF/TEIC">
        <rdf:type rdf:resource="http://xworks.gr/ontologies/ccso#Course"/>
        <coversKA rdf:resource="http://xworks.gr/ontologies/ccso#CS/IS_Intelligent_Systems"/>
        <coversKA rdf:resource="http://xworks.gr/ontologies/ccso#CS/PD_Parallel_and_Distributed_Computing"/>
        <hasSyllabus rdf:resource="http://xworks.gr/ontologies/ccso#IM211s1/IM_MSc/IED/STEF/TEI"/>
        <includedIn rdf:resource="http://xworks.gr/ontologies/ccso#MSc_Informatics_&amp;_Multimedia/IM_MSc/IED/STEF/TEIC"/>
        <offeredBy rdf:resource="http://xworks.gr/ontologies/ccso#Department_of_Informatics_Engineering_of_TEI_of_Crete"/>
        <code rdf:datatype="http://www.w3.org/2001/XMLSchema#string">IM211/IM_MSc/IED/STEF/TEIC</code>
        <courseType rdf:datatype="http://www.w3.org/2001/XMLSchema#string">Elective</courseType>
        <csName rdf:datatype="http://www.w3.org/2001/XMLSchema#string">Multicore Architectures</csName>
    </owl:NamedIndividual>
    


    <!-- http://xworks.gr/ontologies/ccso#IM211s1/IM_MSc/IED/STEF/TEI -->

    <owl:NamedIndividual rdf:about="http://xworks.gr/ontologies/ccso#IM211s1/IM_MSc/IED/STEF/TEI">
        <rdf:type rdf:resource="http://xworks.gr/ontologies/ccso#Syllabus"/>
        <affiliatedWith rdf:resource="http://xworks.gr/ontologies/ccso#Triantafyllidis_George"/>
        <hasInstructor rdf:resource="http://xworks.gr/ontologies/ccso#Triantafyllidis_George"/>
        <hasSupervisor rdf:resource="http://xworks.gr/ontologies/ccso#Triantafyllidis_George"/>
        <syllabusOf rdf:resource="http://xworks.gr/ontologies/ccso#IM211/IM_MSc/IED/STEF/TEIC"/>
        <courseType rdf:datatype="http://www.w3.org/2001/XMLSchema#string">Elective</courseType>
        <creditsECTS rdf:datatype="http://www.w3.org/2001/XMLSchema#decimal">7.5</creditsECTS>
        <csName rdf:datatype="http://www.w3.org/2001/XMLSchema#string">Syllabus of course IM211 Multicore Architectures</csName>
        <semesterinProgram rdf:datatype="http://www.w3.org/2001/XMLSchema#short">2</semesterinProgram>
    </owl:NamedIndividual>
    


    <!-- http://xworks.gr/ontologies/ccso#Kalogiannakis(2010)TrainingICT -->

    <owl:NamedIndividual rdf:about="http://xworks.gr/ontologies/ccso#Kalogiannakis(2010)TrainingICT">
        <rdf:type rdf:resource="http://xworks.gr/ontologies/ccso#Resource"/>
        <dc:creator rdf:resource="http://xworks.gr/ontologies/ccso#Kalogiannakis_Michail"/>
        <dc:date rdf:datatype="http://www.w3.org/2001/XMLSchema#date">2010</dc:date>
        <dc:date rdf:datatype="internal:anonymous-constants">2010</dc:date>
        <dc:title>Training with ICT for ICT from the trainer’s perspective. A Greek case study</dc:title>
        <dates rdf:datatype="internal:anonymous-constants">2010</dates>
        <rdfs:label xml:lang="en">Kalogiannakis (2010) Training with ICT for ICT from the trainer’s perspective. A Greek case study</rdfs:label>
    </owl:NamedIndividual>
    


    <!-- http://xworks.gr/ontologies/ccso#MSc_Computer_Science_and_Engineering/CSE_MSc/CSD/SSE/UoC -->

    <owl:NamedIndividual rdf:about="http://xworks.gr/ontologies/ccso#MSc_Computer_Science_and_Engineering/CSE_MSc/CSD/SSE/UoC">
        <rdf:type rdf:resource="http://xworks.gr/ontologies/ccso#Master"/>
        <rdf:type rdf:resource="http://xworks.gr/ontologies/ccso#ProgramofStudy"/>
        <affiliatedWith rdf:resource="http://xworks.gr/ontologies/ccso#Lionis_Joshua"/>
        <affiliatedWith rdf:resource="http://xworks.gr/ontologies/ccso#Vassilakis_Vassilis"/>
        <hasRegistered rdf:resource="http://xworks.gr/ontologies/ccso#Lionis_Joshua"/>
        <hasRegistered rdf:resource="http://xworks.gr/ontologies/ccso#Vassilakis_Vassilis"/>
        <includesCourse rdf:resource="http://xworks.gr/ontologies/ccso#CS539/CSE_MSc/CSD/SSE/UoC"/>
        <includesCourse rdf:resource="http://xworks.gr/ontologies/ccso#CS540/CSE_MSc/CSD/SSE/UoC"/>
        <providedBy rdf:resource="http://xworks.gr/ontologies/ccso#Computers_Sciences_Department_of_University_of_Crete"/>
        <requiresProgram rdf:resource="http://xworks.gr/ontologies/ccso#BSc_Computer_Science/CS_BSc/CSD/SSE/UoC"/>
        <requiresProgram rdf:resource="http://xworks.gr/ontologies/ccso#BSc_Informatics_Engineering/IE_BSc/IED/STEF/TEIC"/>
        <code rdf:datatype="http://www.w3.org/2001/XMLSchema#string">CSE_MSc/CSD/SSE/UoC</code>
        <creditsECTS rdf:datatype="http://www.w3.org/2001/XMLSchema#short">120</creditsECTS>
        <degreeTitle rdf:datatype="http://www.w3.org/2001/XMLSchema#string">Master of Science in Computer Science and Engineering of University of Crete</degreeTitle>
        <degreeType rdf:datatype="http://www.w3.org/2001/XMLSchema#string">MSc</degreeType>
        <degreeType rdf:datatype="http://www.w3.org/2001/XMLSchema#string">Master of Science</degreeType>
        <duration rdf:datatype="http://www.w3.org/2001/XMLSchema#duration">P2Y</duration>
        <duration rdf:datatype="internal:anonymous-constants">P2Y</duration>
        <psName rdf:datatype="http://www.w3.org/2001/XMLSchema#string">Master of Science (MSc) in Computer Science and Engineering 
of Computers Sciences Department (CSD) of University of Crete</psName>
        <rdfs:label xml:lang="en">Master of Science in Computer Science and Engineering of University of Crete</rdfs:label>
    </owl:NamedIndividual>
    


    <!-- http://xworks.gr/ontologies/ccso#MSc_Informatics_&amp;_Multimedia/IM_MSc/IED/STEF/TEIC -->

    <owl:NamedIndividual rdf:about="http://xworks.gr/ontologies/ccso#MSc_Informatics_&amp;_Multimedia/IM_MSc/IED/STEF/TEIC">
        <rdf:type rdf:resource="http://xworks.gr/ontologies/ccso#Master"/>
        <rdf:type rdf:resource="http://xworks.gr/ontologies/ccso#ProgramofStudy"/>
        <affiliatedWith rdf:resource="http://xworks.gr/ontologies/ccso#Agrimakis_Samson"/>
        <affiliatedWith rdf:resource="http://xworks.gr/ontologies/ccso#Dallas_Nektarios"/>
        <affiliatedWith rdf:resource="http://xworks.gr/ontologies/ccso#Hionis_John"/>
        <affiliatedWith rdf:resource="http://xworks.gr/ontologies/ccso#Kokkinos_Heraklis"/>
        <affiliatedWith rdf:resource="http://xworks.gr/ontologies/ccso#Martelis_Stelios"/>
        <affiliatedWith rdf:resource="http://xworks.gr/ontologies/ccso#Sandi_Elina"/>
        <affiliatedWith rdf:resource="http://xworks.gr/ontologies/ccso#Starkeiou_Alexandros"/>
        <affiliatedWith rdf:resource="http://xworks.gr/ontologies/ccso#Starkeiou_Aria"/>
        <affiliatedWith rdf:resource="http://xworks.gr/ontologies/ccso#Triantafillou_Irene"/>
        <affiliatedWith rdf:resource="http://xworks.gr/ontologies/ccso#Vassileiou_Tom"/>
        <hasRegistered rdf:resource="http://xworks.gr/ontologies/ccso#Agrimakis_Samson"/>
        <hasRegistered rdf:resource="http://xworks.gr/ontologies/ccso#Dallas_Nektarios"/>
        <hasRegistered rdf:resource="http://xworks.gr/ontologies/ccso#Hionis_John"/>
        <hasRegistered rdf:resource="http://xworks.gr/ontologies/ccso#Kokkinos_Heraklis"/>
        <hasRegistered rdf:resource="http://xworks.gr/ontologies/ccso#Martelis_Stelios"/>
        <hasRegistered rdf:resource="http://xworks.gr/ontologies/ccso#Sandi_Elina"/>
        <hasRegistered rdf:resource="http://xworks.gr/ontologies/ccso#Starkeiou_Alexandros"/>
        <hasRegistered rdf:resource="http://xworks.gr/ontologies/ccso#Starkeiou_Aria"/>
        <hasRegistered rdf:resource="http://xworks.gr/ontologies/ccso#Triantafillou_Irene"/>
        <hasRegistered rdf:resource="http://xworks.gr/ontologies/ccso#Vassileiou_Tom"/>
        <includesCourse rdf:resource="http://xworks.gr/ontologies/ccso#IM101/IM_MSc/IED/STEF/TEIC"/>
        <includesCourse rdf:resource="http://xworks.gr/ontologies/ccso#IM102/IM_MSc/IED/STEF/TEIC"/>
        <includesCourse rdf:resource="http://xworks.gr/ontologies/ccso#IM103/IM_MSc/IED/STEF/TEIC"/>
        <includesCourse rdf:resource="http://xworks.gr/ontologies/ccso#IM104/IM_MSc/IED/STEF/TEIC"/>
        <includesCourse rdf:resource="http://xworks.gr/ontologies/ccso#IM105/IM_MSc/IED/STEF/TEIC"/>
        <includesCourse rdf:resource="http://xworks.gr/ontologies/ccso#IM106/IM_MSc/IED/STEF/TEIC"/>
        <includesCourse rdf:resource="http://xworks.gr/ontologies/ccso#IM107/IM_MSc/IED/STEF/TEIC"/>
        <includesCourse rdf:resource="http://xworks.gr/ontologies/ccso#IM108/IM_MSc/IED/STEF/TEIC"/>
        <includesCourse rdf:resource="http://xworks.gr/ontologies/ccso#IM109/IM_MSc/IED/STEF/TEIC"/>
        <includesCourse rdf:resource="http://xworks.gr/ontologies/ccso#IM201/IM_MSc/IED/STEF/TEIC"/>
        <includesCourse rdf:resource="http://xworks.gr/ontologies/ccso#IM202/IM_MSc/IED/STEF/TEIC"/>
        <includesCourse rdf:resource="http://xworks.gr/ontologies/ccso#IM203/IM_MSc/IED/STEF/TEIC"/>
        <includesCourse rdf:resource="http://xworks.gr/ontologies/ccso#IM204/IM_MSc/IED/STEF/TEIC"/>
        <includesCourse rdf:resource="http://xworks.gr/ontologies/ccso#IM205/IM_MSc/IED/STEF/TEIC"/>
        <includesCourse rdf:resource="http://xworks.gr/ontologies/ccso#IM206/IM_MSc/IED/STEF/TEIC"/>
        <includesCourse rdf:resource="http://xworks.gr/ontologies/ccso#IM207/IM_MSc/IED/STEF/TEIC"/>
        <includesCourse rdf:resource="http://xworks.gr/ontologies/ccso#IM208/IM_MSc/IED/STEF/TEIC"/>
        <includesCourse rdf:resource="http://xworks.gr/ontologies/ccso#IM209/IM_MSc/IED/STEF/TEIC"/>
        <includesCourse rdf:resource="http://xworks.gr/ontologies/ccso#IM210/IM_MSc/IED/STEF/TEIC"/>
        <includesCourse rdf:resource="http://xworks.gr/ontologies/ccso#IM211/IM_MSc/IED/STEF/TEIC"/>
        <providedBy rdf:resource="http://xworks.gr/ontologies/ccso#Department_of_Informatics_Engineering_of_TEI_of_Crete"/>
        <requiresProgram rdf:resource="http://xworks.gr/ontologies/ccso#BSc_Computer_Science/CS_BSc/CSD/SSE/UoC"/>
        <requiresProgram rdf:resource="http://xworks.gr/ontologies/ccso#BSc_Informatics_Engineering/IE_BSc/IED/STEF/TEIC"/>
        <code rdf:datatype="http://www.w3.org/2001/XMLSchema#string">IM_MSc/IED/STEF/TEIC</code>
        <creditsECTS rdf:datatype="http://www.w3.org/2001/XMLSchema#short">120</creditsECTS>
        <degreeTitle rdf:datatype="http://www.w3.org/2001/XMLSchema#string">Master of Science in Informatics &amp; Multimedia</degreeTitle>
        <degreeType rdf:datatype="http://www.w3.org/2001/XMLSchema#string">MSc</degreeType>
        <degreeType rdf:datatype="http://www.w3.org/2001/XMLSchema#string">Master of Science</degreeType>
        <degreeURL rdf:datatype="http://www.w3.org/2001/XMLSchema#anyURI">https://www.teicrete.gr/mscie/</degreeURL>
        <psName rdf:datatype="http://www.w3.org/2001/XMLSchema#string">Master of Science in Informatics &amp; Multimedia of Department of Informatics Engineering (IED) of School of Engineering (STEF) of Technological Educational Institute (TEI) of Crete</psName>
        <webaddressURL rdf:datatype="http://www.w3.org/2001/XMLSchema#anyURI">https://www.teicrete.gr/mscie/</webaddressURL>
        <rdfs:label xml:lang="en">Master of Science in Informatics &amp; Multimedia of TEI of Crete</rdfs:label>
    </owl:NamedIndividual>
    


    <!-- http://xworks.gr/ontologies/ccso#MSc_School_Psychology/SP_MSc/PSY/SoC/UoC -->

    <owl:NamedIndividual rdf:about="http://xworks.gr/ontologies/ccso#MSc_School_Psychology/SP_MSc/PSY/SoC/UoC">
        <rdf:type rdf:resource="http://xworks.gr/ontologies/ccso#Master"/>
        <rdf:type rdf:resource="http://xworks.gr/ontologies/ccso#ProgramofStudy"/>
        <affiliatedWith rdf:resource="http://xworks.gr/ontologies/ccso#Assarioti_Mellisandri"/>
        <affiliatedWith rdf:resource="http://xworks.gr/ontologies/ccso#Assarioti_Tina"/>
        <affiliatedWith rdf:resource="http://xworks.gr/ontologies/ccso#Lioni_Catherine"/>
        <affiliatedWith rdf:resource="http://xworks.gr/ontologies/ccso#Mourati_Ginna"/>
        <affiliatedWith rdf:resource="http://xworks.gr/ontologies/ccso#Palaiologou_Ifigeneia"/>
        <hasRegistered rdf:resource="http://xworks.gr/ontologies/ccso#Assarioti_Mellisandri"/>
        <hasRegistered rdf:resource="http://xworks.gr/ontologies/ccso#Assarioti_Tina"/>
        <hasRegistered rdf:resource="http://xworks.gr/ontologies/ccso#Lioni_Catherine"/>
        <hasRegistered rdf:resource="http://xworks.gr/ontologies/ccso#Mourati_Ginna"/>
        <hasRegistered rdf:resource="http://xworks.gr/ontologies/ccso#Palaiologou_Ifigeneia"/>
        <providedBy rdf:resource="http://xworks.gr/ontologies/ccso#Psychology_Department_of_University_of_Crete"/>
        <requiresProgram rdf:resource="http://xworks.gr/ontologies/ccso#BSc_Psychology/PSY_BSc/SoC/UoC"/>
        <code rdf:datatype="http://www.w3.org/2001/XMLSchema#string">SP_MSc/PSY/SoC/UoC</code>
        <csName rdf:datatype="http://www.w3.org/2001/XMLSchema#string">Master of Science in School Psychology of Psychology Department of School of Social Sciences of University of Crete</csName>
        <degreeTitle rdf:datatype="http://www.w3.org/2001/XMLSchema#string">Master of Science in School Psychology</degreeTitle>
        <degreeType rdf:datatype="http://www.w3.org/2001/XMLSchema#string">MSc</degreeType>
        <degreeType rdf:datatype="http://www.w3.org/2001/XMLSchema#string">Master of Science</degreeType>
        <duration rdf:datatype="http://www.w3.org/2001/XMLSchema#duration">P4Y</duration>
        <duration rdf:datatype="internal:anonymous-constants">P4Y</duration>
        <rdfs:label xml:lang="en">Master of Science in School Psychology of University of Crete</rdfs:label>
    </owl:NamedIndividual>
    


    <!-- http://xworks.gr/ontologies/ccso#PSY/LO_Achieved_a_basic_understanding_of_how_programmes_for_the_promotion_of_health_are_implemented -->

    <owl:NamedIndividual rdf:about="http://xworks.gr/ontologies/ccso#PSY/LO_Achieved_a_basic_understanding_of_how_programmes_for_the_promotion_of_health_are_implemented">
        <rdf:type rdf:resource="http://xworks.gr/ontologies/ccso#LearningOutcome"/>
        <acquiredInCourse rdf:resource="http://xworks.gr/ontologies/ccso#PSY3601s1/PSY_BSc/SoC/Uoc"/>
        <label rdf:datatype="http://www.w3.org/2001/XMLSchema#string">Achieved a basic understanding of how programmes for the promotion of health are implemented</label>
        <levelofMastery rdf:datatype="http://www.w3.org/2001/XMLSchema#string">Usage</levelofMastery>
    </owl:NamedIndividual>
    


    <!-- http://xworks.gr/ontologies/ccso#PSY/LO_Acquire_basic_concepts_and_theories_in_Social_Psychology -->

    <owl:NamedIndividual rdf:about="http://xworks.gr/ontologies/ccso#PSY/LO_Acquire_basic_concepts_and_theories_in_Social_Psychology">
        <rdf:type rdf:resource="http://xworks.gr/ontologies/ccso#LearningOutcome"/>
        <acquiredInCourse rdf:resource="http://xworks.gr/ontologies/ccso#PSY1501s1/PSY_BSc/SoC/Uoc"/>
        <label rdf:datatype="http://www.w3.org/2001/XMLSchema#string">To acquire basic concepts and theories in Social Psychology</label>
        <levelofMastery rdf:datatype="http://www.w3.org/2001/XMLSchema#string">Familiarity</levelofMastery>
    </owl:NamedIndividual>
    


    <!-- http://xworks.gr/ontologies/ccso#PSY/LO_Be_aware_of_the_applications_and_implications_of_social_psychological_theory_for_the_explanation_of_real_life_phenomena -->

    <owl:NamedIndividual rdf:about="http://xworks.gr/ontologies/ccso#PSY/LO_Be_aware_of_the_applications_and_implications_of_social_psychological_theory_for_the_explanation_of_real_life_phenomena">
        <rdf:type rdf:resource="http://xworks.gr/ontologies/ccso#LearningOutcome"/>
        <acquiredInCourse rdf:resource="http://xworks.gr/ontologies/ccso#PSY1501s1/PSY_BSc/SoC/Uoc"/>
        <label rdf:datatype="http://www.w3.org/2001/XMLSchema#string">Familiarity</label>
        <label rdf:datatype="http://www.w3.org/2001/XMLSchema#string">To be aware of the applications and implications of social psychological theory for the explanation of real life phenomena</label>
    </owl:NamedIndividual>
    


    <!-- http://xworks.gr/ontologies/ccso#PSY/LO_Comprehended_the_psychological_factors_involved_in_the_experience_of_illness -->

    <owl:NamedIndividual rdf:about="http://xworks.gr/ontologies/ccso#PSY/LO_Comprehended_the_psychological_factors_involved_in_the_experience_of_illness">
        <rdf:type rdf:resource="http://xworks.gr/ontologies/ccso#LearningOutcome"/>
        <acquiredInCourse rdf:resource="http://xworks.gr/ontologies/ccso#PSY3601s1/PSY_BSc/SoC/Uoc"/>
        <label rdf:datatype="http://www.w3.org/2001/XMLSchema#string">Comprehended the psychological factors involved in the experience of illness</label>
        <levelofMastery rdf:datatype="http://www.w3.org/2001/XMLSchema#string">Familiarity</levelofMastery>
    </owl:NamedIndividual>
    


    <!-- http://xworks.gr/ontologies/ccso#PSY/LO_Demonstrate_a_critical_awareness_of_the_relationship_between_theoretical_perspectives_and_research_methodologies_in_social_psychology -->

    <owl:NamedIndividual rdf:about="http://xworks.gr/ontologies/ccso#PSY/LO_Demonstrate_a_critical_awareness_of_the_relationship_between_theoretical_perspectives_and_research_methodologies_in_social_psychology">
        <rdf:type rdf:resource="http://xworks.gr/ontologies/ccso#LearningOutcome"/>
        <acquiredInCourse rdf:resource="http://xworks.gr/ontologies/ccso#PSY1501s1/PSY_BSc/SoC/Uoc"/>
        <label rdf:datatype="http://www.w3.org/2001/XMLSchema#string">To demonstrate a critical awareness of the relationship between theoretical perspectives and research methodologies in social psychology</label>
        <levelofMastery rdf:datatype="http://www.w3.org/2001/XMLSchema#string">Usage</levelofMastery>
    </owl:NamedIndividual>
    


    <!-- http://xworks.gr/ontologies/ccso#PSY/LO_Evaluate_critically_the_major_theoretical_frameworks_in_which_social_psychologists_have_described_and_explained_human_behavior -->

    <owl:NamedIndividual rdf:about="http://xworks.gr/ontologies/ccso#PSY/LO_Evaluate_critically_the_major_theoretical_frameworks_in_which_social_psychologists_have_described_and_explained_human_behavior">
        <rdf:type rdf:resource="http://xworks.gr/ontologies/ccso#LearningOutcome"/>
        <acquiredInCourse rdf:resource="http://xworks.gr/ontologies/ccso#PSY1501s1/PSY_BSc/SoC/Uoc"/>
        <label rdf:datatype="http://www.w3.org/2001/XMLSchema#string">To be able to evaluate critically the major theoretical frameworks in which social psychologists have described and explained human behavior.</label>
        <levelofMastery rdf:datatype="http://www.w3.org/2001/XMLSchema#string">Assessment</levelofMastery>
    </owl:NamedIndividual>
    


    <!-- http://xworks.gr/ontologies/ccso#PSY/LO_Identify_and_evaluate_key_issues_and_controversies_within_social_psychology -->

    <owl:NamedIndividual rdf:about="http://xworks.gr/ontologies/ccso#PSY/LO_Identify_and_evaluate_key_issues_and_controversies_within_social_psychology">
        <rdf:type rdf:resource="http://xworks.gr/ontologies/ccso#LearningOutcome"/>
        <acquiredInCourse rdf:resource="http://xworks.gr/ontologies/ccso#PSY1501s1/PSY_BSc/SoC/Uoc"/>
        <label rdf:datatype="http://www.w3.org/2001/XMLSchema#string">To identify and evaluate key issues and controversies within social psychology.</label>
        <levelofMastery rdf:datatype="http://www.w3.org/2001/XMLSchema#string">Assessment</levelofMastery>
    </owl:NamedIndividual>
    


    <!-- http://xworks.gr/ontologies/ccso#PSY/LO_Realized_the_importance_of_the_link_between_theory_and_practice -->

    <owl:NamedIndividual rdf:about="http://xworks.gr/ontologies/ccso#PSY/LO_Realized_the_importance_of_the_link_between_theory_and_practice">
        <rdf:type rdf:resource="http://xworks.gr/ontologies/ccso#LearningOutcome"/>
        <acquiredInCourse rdf:resource="http://xworks.gr/ontologies/ccso#PSY3601s1/PSY_BSc/SoC/Uoc"/>
        <label rdf:datatype="http://www.w3.org/2001/XMLSchema#string">Realized the importance of the link between theory and practice</label>
        <levelofMastery rdf:datatype="http://www.w3.org/2001/XMLSchema#string">Familiarity</levelofMastery>
    </owl:NamedIndividual>
    


    <!-- http://xworks.gr/ontologies/ccso#PSY/LO_Seen_the_importance_of_multidisciplinary_collaboration_in_health_and_health_care_services -->

    <owl:NamedIndividual rdf:about="http://xworks.gr/ontologies/ccso#PSY/LO_Seen_the_importance_of_multidisciplinary_collaboration_in_health_and_health_care_services">
        <rdf:type rdf:resource="http://xworks.gr/ontologies/ccso#LearningOutcome"/>
        <acquiredInCourse rdf:resource="http://xworks.gr/ontologies/ccso#PSY3601s1/PSY_BSc/SoC/Uoc"/>
        <label rdf:datatype="http://www.w3.org/2001/XMLSchema#string">Seen the importance of multidisciplinary collaboration in health and health care services</label>
        <levelofMastery rdf:datatype="http://www.w3.org/2001/XMLSchema#string">Familiarity</levelofMastery>
    </owl:NamedIndividual>
    


    <!-- http://xworks.gr/ontologies/ccso#PSY/T_Intergroup_Behaviour -->

    <owl:NamedIndividual rdf:about="http://xworks.gr/ontologies/ccso#PSY/T_Intergroup_Behaviour">
        <rdf:type rdf:resource="http://xworks.gr/ontologies/ccso#Topic"/>
        <coveredInCourse rdf:resource="http://xworks.gr/ontologies/ccso#PSY1501s1/PSY_BSc/SoC/Uoc"/>
        <label rdf:datatype="http://www.w3.org/2001/XMLSchema#string">Intergroup Behaviour</label>
    </owl:NamedIndividual>
    


    <!-- http://xworks.gr/ontologies/ccso#PSY/T_Respect_for_difference_and_multiculturalism -->

    <owl:NamedIndividual rdf:about="http://xworks.gr/ontologies/ccso#PSY/T_Respect_for_difference_and_multiculturalism">
        <rdf:type rdf:resource="http://xworks.gr/ontologies/ccso#Topic"/>
        <coveredInCourse rdf:resource="http://xworks.gr/ontologies/ccso#PSY3601s1/PSY_BSc/SoC/Uoc"/>
        <label rdf:datatype="http://www.w3.org/2001/XMLSchema#string">Respect for difference and multiculturalism</label>
    </owl:NamedIndividual>
    


    <!-- http://xworks.gr/ontologies/ccso#PSY/T_Social_Psychology_and_Culture -->

    <owl:NamedIndividual rdf:about="http://xworks.gr/ontologies/ccso#PSY/T_Social_Psychology_and_Culture">
        <rdf:type rdf:resource="http://xworks.gr/ontologies/ccso#Topic"/>
        <coveredInCourse rdf:resource="http://xworks.gr/ontologies/ccso#PSY1501s1/PSY_BSc/SoC/Uoc"/>
        <label rdf:datatype="http://www.w3.org/2001/XMLSchema#string">Social Psychology and Culture</label>
    </owl:NamedIndividual>
    


    <!-- http://xworks.gr/ontologies/ccso#PSY/T_Stereotypes_and_Prejudice -->

    <owl:NamedIndividual rdf:about="http://xworks.gr/ontologies/ccso#PSY/T_Stereotypes_and_Prejudice">
        <rdf:type rdf:resource="http://xworks.gr/ontologies/ccso#Topic"/>
        <label rdf:datatype="http://www.w3.org/2001/XMLSchema#string">Stereotypes and Prejudice</label>
    </owl:NamedIndividual>
    


    <!-- http://xworks.gr/ontologies/ccso#PSY/T_The_Critical_thought_in_Social_Psychology -->

    <owl:NamedIndividual rdf:about="http://xworks.gr/ontologies/ccso#PSY/T_The_Critical_thought_in_Social_Psychology">
        <rdf:type rdf:resource="http://xworks.gr/ontologies/ccso#LearningOutcome"/>
        <rdf:type rdf:resource="http://xworks.gr/ontologies/ccso#Topic"/>
        <coveredInCourse rdf:resource="http://xworks.gr/ontologies/ccso#PSY1501s1/PSY_BSc/SoC/Uoc"/>
        <levelofMastery rdf:datatype="http://www.w3.org/2001/XMLSchema#string">Familiarity</levelofMastery>
    </owl:NamedIndividual>
    


    <!-- http://xworks.gr/ontologies/ccso#PSY/T_The_Self -->

    <owl:NamedIndividual rdf:about="http://xworks.gr/ontologies/ccso#PSY/T_The_Self">
        <rdf:type rdf:resource="http://xworks.gr/ontologies/ccso#Topic"/>
        <coveredInCourse rdf:resource="http://xworks.gr/ontologies/ccso#PSY1501s1/PSY_BSc/SoC/Uoc"/>
        <label rdf:datatype="http://www.w3.org/2001/XMLSchema#string">The Self</label>
    </owl:NamedIndividual>
    


    <!-- http://xworks.gr/ontologies/ccso#PSY/LO_Understood_the_interplay_between_biological,_psychological_and_social_determinants_of_health_and_illness -->

    <owl:NamedIndividual rdf:about="http://xworks.gr/ontologies/ccso#PSY/LO_Understood_the_interplay_between_biological,_psychological_and_social_determinants_of_health_and_illness">
        <rdf:type rdf:resource="http://xworks.gr/ontologies/ccso#LearningOutcome"/>
        <acquiredInCourse rdf:resource="http://xworks.gr/ontologies/ccso#PSY3601s1/PSY_BSc/SoC/Uoc"/>
        <label rdf:datatype="http://www.w3.org/2001/XMLSchema#string">Understood the interplay between biological, psychological and social determinants of health and illness,</label>
        <levelofMastery rdf:datatype="http://www.w3.org/2001/XMLSchema#string">Usage</levelofMastery>
    </owl:NamedIndividual>
    


    <!-- http://xworks.gr/ontologies/ccso#PSY/T_Attitudes:Personal_and_Social_approaches -->

    <owl:NamedIndividual rdf:about="http://xworks.gr/ontologies/ccso#PSY/T_Attitudes:Personal_and_Social_approaches">
        <rdf:type rdf:resource="http://xworks.gr/ontologies/ccso#Topic"/>
        <coveredInCourse rdf:resource="http://xworks.gr/ontologies/ccso#PSY1501s1/PSY_BSc/SoC/Uoc"/>
        <label rdf:datatype="http://www.w3.org/2001/XMLSchema#string">Attitudes: Personal and Social approaches</label>
    </owl:NamedIndividual>
    


    <!-- http://xworks.gr/ontologies/ccso#PSY/T_Identity_theory:A_multilevel_Perspective -->

    <owl:NamedIndividual rdf:about="http://xworks.gr/ontologies/ccso#PSY/T_Identity_theory:A_multilevel_Perspective">
        <rdf:type rdf:resource="http://xworks.gr/ontologies/ccso#Topic"/>
        <coveredInCourse rdf:resource="http://xworks.gr/ontologies/ccso#PSY1501s1/PSY_BSc/SoC/Uoc"/>
        <label rdf:datatype="http://www.w3.org/2001/XMLSchema#string">Identity theory: A multilevel perspective</label>
    </owl:NamedIndividual>
    


    <!-- http://xworks.gr/ontologies/ccso#PSY/T_Production_of_free,creative_and_inductive_thinking -->

    <owl:NamedIndividual rdf:about="http://xworks.gr/ontologies/ccso#PSY/T_Production_of_free,creative_and_inductive_thinking">
        <rdf:type rdf:resource="http://xworks.gr/ontologies/ccso#Topic"/>
        <coveredInCourse rdf:resource="http://xworks.gr/ontologies/ccso#PSY3601s1/PSY_BSc/SoC/Uoc"/>
        <label rdf:datatype="http://www.w3.org/2001/XMLSchema#string">Production of free, creative and inductive thinking</label>
    </owl:NamedIndividual>
    


    <!-- http://xworks.gr/ontologies/ccso#PSY/T_Search_for,Analysis_and_Synthesis_of_data_and_information,with_the_use_of_the_necessary_technology -->

    <owl:NamedIndividual rdf:about="http://xworks.gr/ontologies/ccso#PSY/T_Search_for,Analysis_and_Synthesis_of_data_and_information,with_the_use_of_the_necessary_technology">
        <rdf:type rdf:resource="http://xworks.gr/ontologies/ccso#Topic"/>
        <coveredInCourse rdf:resource="http://xworks.gr/ontologies/ccso#PSY3601s1/PSY_BSc/SoC/Uoc"/>
        <label rdf:datatype="http://www.w3.org/2001/XMLSchema#string">Search for, Analysis and Aynthesis of data and information, with the use of the necessary technology</label>
    </owl:NamedIndividual>
    


    <!-- http://xworks.gr/ontologies/ccso#PSY/T_Social_Influence:Conformity_and_obedience -->

    <owl:NamedIndividual rdf:about="http://xworks.gr/ontologies/ccso#PSY/T_Social_Influence:Conformity_and_obedience">
        <rdf:type rdf:resource="http://xworks.gr/ontologies/ccso#Topic"/>
        <label rdf:datatype="http://www.w3.org/2001/XMLSchema#string">Social Influence: Conformity and obedience</label>
    </owl:NamedIndividual>
    


    <!-- http://xworks.gr/ontologies/ccso#PSY/T_Social_Psychology:A_Historical_Perspective -->

    <owl:NamedIndividual rdf:about="http://xworks.gr/ontologies/ccso#PSY/T_Social_Psychology:A_Historical_Perspective">
        <rdf:type rdf:resource="http://xworks.gr/ontologies/ccso#Topic"/>
        <coveredInCourse rdf:resource="http://xworks.gr/ontologies/ccso#PSY1501s1/PSY_BSc/SoC/Uoc"/>
        <label rdf:datatype="http://www.w3.org/2001/XMLSchema#string">Social Psychology: An historical perspective</label>
    </owl:NamedIndividual>
    


    <!-- http://xworks.gr/ontologies/ccso#PSY131/CIA_MSc/Psy-Med/UoC -->

    <owl:NamedIndividual rdf:about="http://xworks.gr/ontologies/ccso#PSY131/CIA_MSc/Psy-Med/UoC">
        <rdf:type rdf:resource="http://xworks.gr/ontologies/ccso#Course"/>
        <offeredBy rdf:resource="http://xworks.gr/ontologies/ccso#Psychology_Department_of_University_of_Crete"/>
        <code rdf:datatype="http://www.w3.org/2001/XMLSchema#string">PSY131/CIA_MSc/Psy-Med/UoC</code>
        <csName rdf:datatype="http://www.w3.org/2001/XMLSchema#string">The Neurobiological and Psychopharmacological Basis of Drug Abuse and Addiction</csName>
    </owl:NamedIndividual>
    


    <!-- http://xworks.gr/ontologies/ccso#PSY132/CIA_MSc/Psy-Med/UoC -->

    <owl:NamedIndividual rdf:about="http://xworks.gr/ontologies/ccso#PSY132/CIA_MSc/Psy-Med/UoC">
        <rdf:type rdf:resource="http://xworks.gr/ontologies/ccso#Course"/>
        <rdf:type rdf:resource="http://xworks.gr/ontologies/ccso#Syllabus"/>
        <affiliatedWith rdf:resource="http://xworks.gr/ontologies/ccso#Sotiropoulou_Mikela"/>
        <hasAttender rdf:resource="http://xworks.gr/ontologies/ccso#Sotiropoulou_Mikela"/>
        <hasSyllabus rdf:resource="http://xworks.gr/ontologies/ccso#PSY132/CIA_MSc/Psy-Med/UoC"/>
        <offeredBy rdf:resource="http://xworks.gr/ontologies/ccso#Psychology_Department_of_University_of_Crete"/>
        <syllabusOf rdf:resource="http://xworks.gr/ontologies/ccso#PSY132/CIA_MSc/Psy-Med/UoC"/>
        <code rdf:datatype="http://www.w3.org/2001/XMLSchema#string">PSY132/CIA_MSc/Psy-Med/UoC</code>
        <csName rdf:datatype="http://www.w3.org/2001/XMLSchema#string">PSY132 Family Interventions in Substance Abuse and Addiction
Course in Clinical Interventions in Addictions Master of Science (MSc) of Psychology Department of School of Social Sciences of University of Crete</csName>
    </owl:NamedIndividual>
    


    <!-- http://xworks.gr/ontologies/ccso#PSY1501/PSY_BSc/SoC/Uoc -->

    <owl:NamedIndividual rdf:about="http://xworks.gr/ontologies/ccso#PSY1501/PSY_BSc/SoC/Uoc">
        <rdf:type rdf:resource="http://xworks.gr/ontologies/ccso#Course"/>
        <affiliatedWith rdf:resource="http://xworks.gr/ontologies/ccso#Kekili_Souzan"/>
        <affiliatedWith rdf:resource="http://xworks.gr/ontologies/ccso#Ralli_Mary"/>
        <affiliatedWith rdf:resource="http://xworks.gr/ontologies/ccso#Rallis_John"/>
        <hasAttender rdf:resource="http://xworks.gr/ontologies/ccso#Kekili_Souzan"/>
        <hasAttender rdf:resource="http://xworks.gr/ontologies/ccso#Ralli_Mary"/>
        <hasAttender rdf:resource="http://xworks.gr/ontologies/ccso#Rallis_John"/>
        <hasSyllabus rdf:resource="http://xworks.gr/ontologies/ccso#PSY1501s1/PSY_BSc/SoC/Uoc"/>
        <includedIn rdf:resource="http://xworks.gr/ontologies/ccso#BSc_Psychology/PSY_BSc/SoC/UoC"/>
        <offeredBy rdf:resource="http://xworks.gr/ontologies/ccso#Psychology_Department_of_University_of_Crete"/>
        <code rdf:datatype="http://www.w3.org/2001/XMLSchema#string">PSY1501/PSY_BSc/SoC/Uoc</code>
        <csName rdf:datatype="http://www.w3.org/2001/XMLSchema#string">Social Psychology I : Introduction to Social Psychology</csName>
    </owl:NamedIndividual>
    


    <!-- http://xworks.gr/ontologies/ccso#PSY1501_s2017-18-L01/PSY_BSc/SoC/Uoc -->

    <owl:NamedIndividual rdf:about="http://xworks.gr/ontologies/ccso#PSY1501_s2017-18-L01/PSY_BSc/SoC/Uoc">
        <rdf:type rdf:resource="http://xworks.gr/ontologies/ccso#Event"/>
        <rdf:type rdf:resource="http://xworks.gr/ontologies/ccso#Syllabus"/>
        <rdf:type rdf:resource="http://xworks.gr/ontologies/ccso#TeachingEvent"/>
        <affiliatedWith rdf:resource="http://xworks.gr/ontologies/ccso#Kafetsios_Konstantinos"/>
        <affiliatedWith rdf:resource="http://xworks.gr/ontologies/ccso#Tsaeri_Elena"/>
        <expectsLO rdf:resource="http://xworks.gr/ontologies/ccso#PSY/LO_Acquire_basic_concepts_and_theories_in_Social_Psychology"/>
        <followsTEMethod rdf:resource="http://xworks.gr/ontologies/ccso#Lecture"/>
        <hasTeacher rdf:resource="http://xworks.gr/ontologies/ccso#Kafetsios_Konstantinos"/>
        <hasTeacher rdf:resource="http://xworks.gr/ontologies/ccso#Tsaeri_Elena"/>
        <hasTopic rdf:resource="http://xworks.gr/ontologies/ccso#PSY/T_Social_Psychology:A_Historical_Perspective"/>
        <dates rdf:datatype="http://www.w3.org/2001/XMLSchema#dateTime">2017-10-14T12:00:00</dates>
        <duration rdf:datatype="http://www.w3.org/2001/XMLSchema#duration">PT2H</duration>
        <duration rdf:datatype="internal:anonymous-constants">PT2H</duration>
        <eventClassroom rdf:datatype="http://www.w3.org/2001/XMLSchema#duration">15</eventClassroom>
        <eventClassroom rdf:datatype="internal:anonymous-constants">15</eventClassroom>
        <eventDateTime rdf:datatype="http://www.w3.org/2001/XMLSchema#dateTime">2017-10-14T12:00:00</eventDateTime>
        <eventWeekNo rdf:datatype="http://www.w3.org/2001/XMLSchema#short">01</eventWeekNo>
        <label rdf:datatype="http://www.w3.org/2001/XMLSchema#string">Lesson 01
PSY1501 Social Psychology SC1/Psy/BSc/SoC/Uoc
Social Psychology: An historical perspective</label>
        <language rdf:datatype="http://www.w3.org/2001/XMLSchema#duration">Greek</language>
        <language rdf:datatype="internal:anonymous-constants">Greek</language>
        <weeklyWorkload rdf:datatype="http://www.w3.org/2001/XMLSchema#duration">PT45M</weeklyWorkload>
        <weeklyWorkload rdf:datatype="internal:anonymous-constants">PT45M</weeklyWorkload>
    </owl:NamedIndividual>
    


    <!-- http://xworks.gr/ontologies/ccso#PSY1501s1/PSY_BSc/SoC/Uoc -->

    <owl:NamedIndividual rdf:about="http://xworks.gr/ontologies/ccso#PSY1501s1/PSY_BSc/SoC/Uoc">
        <rdf:type rdf:resource="http://xworks.gr/ontologies/ccso#Syllabus"/>
        <affiliatedWith rdf:resource="http://xworks.gr/ontologies/ccso#Kafetsios_Konstantinos"/>
        <affiliatedWith rdf:resource="http://xworks.gr/ontologies/ccso#Tsaeri_Elena"/>
        <aimsToLO rdf:resource="http://xworks.gr/ontologies/ccso#PSY/LO_Acquire_basic_concepts_and_theories_in_Social_Psychology"/>
        <aimsToLO rdf:resource="http://xworks.gr/ontologies/ccso#PSY/LO_Be_aware_of_the_applications_and_implications_of_social_psychological_theory_for_the_explanation_of_real_life_phenomena"/>
        <aimsToLO rdf:resource="http://xworks.gr/ontologies/ccso#PSY/LO_Demonstrate_a_critical_awareness_of_the_relationship_between_theoretical_perspectives_and_research_methodologies_in_social_psychology"/>
        <aimsToLO rdf:resource="http://xworks.gr/ontologies/ccso#PSY/LO_Evaluate_critically_the_major_theoretical_frameworks_in_which_social_psychologists_have_described_and_explained_human_behavior"/>
        <aimsToLO rdf:resource="http://xworks.gr/ontologies/ccso#PSY/LO_Identify_and_evaluate_key_issues_and_controversies_within_social_psychology"/>
        <coversTopic rdf:resource="http://xworks.gr/ontologies/ccso#PSY/T_Intergroup_Behaviour"/>
        <coversTopic rdf:resource="http://xworks.gr/ontologies/ccso#PSY/T_Social_Psychology_and_Culture"/>
        <coversTopic rdf:resource="http://xworks.gr/ontologies/ccso#PSY/T_The_Critical_thought_in_Social_Psychology"/>
        <coversTopic rdf:resource="http://xworks.gr/ontologies/ccso#PSY/T_The_Self"/>
        <coversTopic rdf:resource="http://xworks.gr/ontologies/ccso#PSY/T_Attitudes:Personal_and_Social_approaches"/>
        <coversTopic rdf:resource="http://xworks.gr/ontologies/ccso#PSY/T_Identity_theory:A_multilevel_Perspective"/>
        <coversTopic rdf:resource="http://xworks.gr/ontologies/ccso#PSY/T_Social_Psychology:A_Historical_Perspective"/>
        <followsTEMethod rdf:resource="http://xworks.gr/ontologies/ccso#Demonstration"/>
        <followsTEMethod rdf:resource="http://xworks.gr/ontologies/ccso#Lecture"/>
        <followsTEMethod rdf:resource="http://xworks.gr/ontologies/ccso#Project"/>
        <followsTEMethod rdf:resource="http://xworks.gr/ontologies/ccso#WrittenExam"/>
        <hasEvent rdf:resource="http://xworks.gr/ontologies/ccso#PSY1501_s2017-18-L01/PSY_BSc/SoC/Uoc"/>
        <hasInstructor rdf:resource="http://xworks.gr/ontologies/ccso#Kafetsios_Konstantinos"/>
        <hasInstructor rdf:resource="http://xworks.gr/ontologies/ccso#Tsaeri_Elena"/>
        <hasLM rdf:resource="http://xworks.gr/ontologies/ccso#Hogg2010SocialPsychology"/>
        <hasLM rdf:resource="http://xworks.gr/ontologies/ccso#Papastamou2008EpistimologikoiProvlimatismoi"/>
        <hasLM rdf:resource="http://xworks.gr/ontologies/ccso#Sapsford2006TheorySocialPsychology"/>
        <hasSupervisor rdf:resource="http://xworks.gr/ontologies/ccso#Kafetsios_Konstantinos"/>
        <syllabusOf rdf:resource="http://xworks.gr/ontologies/ccso#PSY1501/PSY_BSc/SoC/Uoc"/>
        <academicYear rdf:datatype="http://www.w3.org/2001/XMLSchema#string">Spring</academicYear>
        <code rdf:datatype="http://www.w3.org/2001/XMLSchema#string">PSY1501s1/PSY_BSc/SoC/Uoc</code>
        <courseType rdf:datatype="http://www.w3.org/2001/XMLSchema#string">Compulsory</courseType>
        <creditsECTS rdf:datatype="http://www.w3.org/2001/XMLSchema#short">4</creditsECTS>
        <csName rdf:datatype="http://www.w3.org/2001/XMLSchema#string">Syllabus of course PSY1501 Social Psychology I : Introduction to Social Psychology</csName>
        <dates rdf:datatype="internal:anonymous-constants">2017-10-01</dates>
        <dates rdf:datatype="internal:anonymous-constants">2018-01-29</dates>
        <description rdf:datatype="http://www.w3.org/2001/XMLSchema#string">Course contents:
•  Social Psychology: An historical perspective
•  Attitudes: Personal and social approaches
•  Stereotypes and Prejudice
•  Social influence: Conformity and obedience
•  Intergroup behavior
•  The Self
•  Identity theory: A multilevel perspective
•  Social Psychology and culture
•  The Critical thought in Social Psychology</description>
        <description rdf:datatype="http://www.w3.org/2001/XMLSchema#string">Objectives of the course (preferably expressed in terms of learning outcomes and competences):
1. To acquire basic concepts and theories in social psychology
2. To be able to evaluate critically the major theoretical frameworks in which social psychologists have described and explained human behavior.
3. To demonstrate a critical awareness of the relationship between theoretical perspectives and research methodologies in social psychology
4. To identify and evaluate key issues and controversies within social psychology.
5. To be aware of the applications and implications of social psychological theory for the explanation of real life phenomena</description>
        <duration rdf:datatype="http://www.w3.org/2001/XMLSchema#duration">P4M</duration>
        <duration rdf:datatype="internal:anonymous-constants">P4M</duration>
        <endDate rdf:datatype="http://www.w3.org/2001/XMLSchema#date">2018-01-29</endDate>
        <endDate rdf:datatype="internal:anonymous-constants">2018-01-29</endDate>
        <language rdf:datatype="http://www.w3.org/2001/XMLSchema#string">Greek</language>
        <semesterinProgram rdf:datatype="http://www.w3.org/2001/XMLSchema#short">1</semesterinProgram>
        <startDate rdf:datatype="http://www.w3.org/2001/XMLSchema#date">2017-10-01</startDate>
        <startDate rdf:datatype="internal:anonymous-constants">2017-10-01</startDate>
    </owl:NamedIndividual>
    


    <!-- http://xworks.gr/ontologies/ccso#PSY2401/PSY_BSc/SoC/Uoc -->

    <owl:NamedIndividual rdf:about="http://xworks.gr/ontologies/ccso#PSY2401/PSY_BSc/SoC/Uoc">
        <rdf:type rdf:resource="http://xworks.gr/ontologies/ccso#Course"/>
        <rdf:type rdf:resource="http://xworks.gr/ontologies/ccso#Syllabus"/>
        <hasSyllabus rdf:resource="http://xworks.gr/ontologies/ccso#PSY2401/PSY_BSc/SoC/Uoc"/>
        <includedIn rdf:resource="http://xworks.gr/ontologies/ccso#BSc_Psychology/PSY_BSc/SoC/UoC"/>
        <offeredBy rdf:resource="http://xworks.gr/ontologies/ccso#Psychology_Department_of_University_of_Crete"/>
        <syllabusOf rdf:resource="http://xworks.gr/ontologies/ccso#PSY2401/PSY_BSc/SoC/Uoc"/>
        <code rdf:datatype="http://www.w3.org/2001/XMLSchema#string">PSY2401/PSY_BSc/SoC/Uoc</code>
        <csName rdf:datatype="http://www.w3.org/2001/XMLSchema#string">Physiological Psychology I</csName>
    </owl:NamedIndividual>
    


    <!-- http://xworks.gr/ontologies/ccso#PSY3601/PSY_BSc/SoC/Uoc -->

    <owl:NamedIndividual rdf:about="http://xworks.gr/ontologies/ccso#PSY3601/PSY_BSc/SoC/Uoc">
        <rdf:type rdf:resource="http://xworks.gr/ontologies/ccso#Course"/>
        <hasPrerequisite rdf:resource="http://xworks.gr/ontologies/ccso#PSY2401/PSY_BSc/SoC/Uoc"/>
        <hasSyllabus rdf:resource="http://xworks.gr/ontologies/ccso#PSY3601s1/PSY_BSc/SoC/Uoc"/>
        <includedIn rdf:resource="http://xworks.gr/ontologies/ccso#BSc_Psychology/PSY_BSc/SoC/UoC"/>
        <offeredBy rdf:resource="http://xworks.gr/ontologies/ccso#Psychology_Department_of_University_of_Crete"/>
        <code rdf:datatype="http://www.w3.org/2001/XMLSchema#string">PSY3601/PSY_BSc/SoC/Uoc</code>
        <csName rdf:datatype="http://www.w3.org/2001/XMLSchema#string">Health Psychology</csName>
    </owl:NamedIndividual>
    


    <!-- http://xworks.gr/ontologies/ccso#PSY3601s1/PSY_BSc/SoC/Uoc -->

    <owl:NamedIndividual rdf:about="http://xworks.gr/ontologies/ccso#PSY3601s1/PSY_BSc/SoC/Uoc">
        <rdf:type rdf:resource="http://xworks.gr/ontologies/ccso#Syllabus"/>
        <affiliatedWith rdf:resource="http://xworks.gr/ontologies/ccso#Kafetsios_Konstantinos"/>
        <aimsToLO rdf:resource="http://xworks.gr/ontologies/ccso#PSY/LO_Achieved_a_basic_understanding_of_how_programmes_for_the_promotion_of_health_are_implemented"/>
        <aimsToLO rdf:resource="http://xworks.gr/ontologies/ccso#PSY/LO_Comprehended_the_psychological_factors_involved_in_the_experience_of_illness"/>
        <aimsToLO rdf:resource="http://xworks.gr/ontologies/ccso#PSY/LO_Realized_the_importance_of_the_link_between_theory_and_practice"/>
        <aimsToLO rdf:resource="http://xworks.gr/ontologies/ccso#PSY/LO_Seen_the_importance_of_multidisciplinary_collaboration_in_health_and_health_care_services"/>
        <aimsToLO rdf:resource="http://xworks.gr/ontologies/ccso#PSY/LO_Understood_the_interplay_between_biological,_psychological_and_social_determinants_of_health_and_illness"/>
        <coversTopic rdf:resource="http://xworks.gr/ontologies/ccso#PSY/T_Respect_for_difference_and_multiculturalism"/>
        <coversTopic rdf:resource="http://xworks.gr/ontologies/ccso#PSY/T_Production_of_free,creative_and_inductive_thinking"/>
        <coversTopic rdf:resource="http://xworks.gr/ontologies/ccso#PSY/T_Search_for,Analysis_and_Synthesis_of_data_and_information,with_the_use_of_the_necessary_technology"/>
        <followsTEMethod rdf:resource="http://xworks.gr/ontologies/ccso#Demonstration"/>
        <followsTEMethod rdf:resource="http://xworks.gr/ontologies/ccso#Lecture"/>
        <hasInstructor rdf:resource="http://xworks.gr/ontologies/ccso#Kafetsios_Konstantinos"/>
        <hasLM rdf:resource="http://xworks.gr/ontologies/ccso#Friedman2011OxfordHandbook"/>
        <syllabusOf rdf:resource="http://xworks.gr/ontologies/ccso#PSY3601/PSY_BSc/SoC/Uoc"/>
        <code rdf:datatype="http://www.w3.org/2001/XMLSchema#string">PSY3601s1/PSY_BSc/SoC/Uoc</code>
        <courseType rdf:datatype="http://www.w3.org/2001/XMLSchema#string">Compulsory</courseType>
        <courseURL rdf:datatype="http://www.w3.org/2001/XMLSchema#anyURI">https://elearn.uoc.gr/course/view.php?id=110</courseURL>
        <creditsECTS rdf:datatype="http://www.w3.org/2001/XMLSchema#short">5</creditsECTS>
        <csName rdf:datatype="http://www.w3.org/2001/XMLSchema#string">Syllabus of course PSY3601 Health Psychology</csName>
        <description rdf:datatype="http://www.w3.org/2001/XMLSchema#string">This course aims to introduce students in the field of health psychology, which refers to the study of the biopsychosocial mechanisms and processes that determine health, illness and health care.
Specifically, the course focuses on important aspects of health and illness, including the definitions of these two concepts, the psychosocial factors and the interactions that determine health and illness, health behaviour prediction and change, the experience of illness and its determinants. The overall aim of this course is to help students achieve a general understanding of the above concepts and of their relation to other fields in psychology as well as to clinical practice.</description>
        <evaluationInfo rdf:datatype="http://www.w3.org/2001/XMLSchema#string">Erasmus Students: Individualized reading material assessed with two extended written reports (in English).

Final exams (70% of the final grade), including:
• multiple choice questions,
• open-ended questions.
Mid-term exam (30% of the final grade), including open-ended questions.
Evaluation criteria are accessible to students via the web-site of course on the UoC e-learn platform.</evaluationInfo>
        <language rdf:datatype="http://www.w3.org/2001/XMLSchema#string">Greek</language>
        <offeredtoErasmus rdf:datatype="http://www.w3.org/2001/XMLSchema#boolean">true</offeredtoErasmus>
        <semesterinProgram rdf:datatype="http://www.w3.org/2001/XMLSchema#short">5</semesterinProgram>
        <webaddressURL rdf:datatype="http://www.w3.org/2001/XMLSchema#anyURI">https://elearn.uoc.gr/course/view.php?id=110</webaddressURL>
        <weeklyHours rdf:datatype="http://www.w3.org/2001/XMLSchema#duration">PT3H</weeklyHours>
        <weeklyHours rdf:datatype="internal:anonymous-constants">PT3H</weeklyHours>
        <weeklyWorkload rdf:datatype="http://www.w3.org/2001/XMLSchema#duration">PT12H</weeklyWorkload>
        <weeklyWorkload rdf:datatype="internal:anonymous-constants">PT12H</weeklyWorkload>
    </owl:NamedIndividual>
    


    <!-- http://xworks.gr/ontologies/ccso#PSY642/CP_PhD/Psy/SoC/UoC -->

    <owl:NamedIndividual rdf:about="http://xworks.gr/ontologies/ccso#PSY642/CP_PhD/Psy/SoC/UoC">
        <rdf:type rdf:resource="http://xworks.gr/ontologies/ccso#Course"/>
        <includedIn rdf:resource="http://xworks.gr/ontologies/ccso#PhD_Clinical_Psychology/CP_PhD/Psy/SoC/UoC"/>
        <offeredBy rdf:resource="http://xworks.gr/ontologies/ccso#Psychology_Department_of_University_of_Crete"/>
        <code rdf:datatype="http://www.w3.org/2001/XMLSchema#string">PSY642/CP_PhD/Psy/SoC/UoC</code>
        <csName rdf:datatype="http://www.w3.org/2001/XMLSchema#string">Child and Adolescent Psychopathology</csName>
    </owl:NamedIndividual>
    


    <!-- http://xworks.gr/ontologies/ccso#PhD_Clinical_Psychology/CP_PhD/Psy/SoC/UoC -->

    <owl:NamedIndividual rdf:about="http://xworks.gr/ontologies/ccso#PhD_Clinical_Psychology/CP_PhD/Psy/SoC/UoC">
        <rdf:type rdf:resource="http://xworks.gr/ontologies/ccso#Doctorate"/>
        <rdf:type rdf:resource="http://xworks.gr/ontologies/ccso#ProgramofStudy"/>
        <affiliatedWith rdf:resource="http://xworks.gr/ontologies/ccso#Tarla_Elena"/>
        <hasRegistered rdf:resource="http://xworks.gr/ontologies/ccso#Tarla_Elena"/>
        <includesCourse rdf:resource="http://xworks.gr/ontologies/ccso#PSY642/CP_PhD/Psy/SoC/UoC"/>
        <providedBy rdf:resource="http://xworks.gr/ontologies/ccso#Psychology_Department_of_University_of_Crete"/>
        <code rdf:datatype="http://www.w3.org/2001/XMLSchema#string">CP_PhD/Psy/SoC/UoC</code>
        <creditsECTS rdf:datatype="http://www.w3.org/2001/XMLSchema#short">320</creditsECTS>
        <degreeTitle rdf:datatype="http://www.w3.org/2001/XMLSchema#string">Doctor of Philosophy in Clinical Psychology</degreeTitle>
        <degreeType rdf:datatype="http://www.w3.org/2001/XMLSchema#string">Doctor of Philosophy</degreeType>
        <degreeType rdf:datatype="http://www.w3.org/2001/XMLSchema#string">PhD</degreeType>
        <psName rdf:datatype="http://www.w3.org/2001/XMLSchema#string">PhD in Clinical Psychology of Computers Sciences Department (CSD) of University of Crete</psName>
        <rdfs:label xml:lang="en">PhD in Clinical Psychology of University of Crete</rdfs:label>
    </owl:NamedIndividual>
    


    <!-- http://xworks.gr/ontologies/ccso#PhD_Computer_Science_and_Engineering/CSE_PhD/CSD/SSE/UoC -->

    <owl:NamedIndividual rdf:about="http://xworks.gr/ontologies/ccso#PhD_Computer_Science_and_Engineering/CSE_PhD/CSD/SSE/UoC">
        <rdf:type rdf:resource="http://xworks.gr/ontologies/ccso#Doctorate"/>
        <rdf:type rdf:resource="http://xworks.gr/ontologies/ccso#ProgramofStudy"/>
        <affiliatedWith rdf:resource="http://xworks.gr/ontologies/ccso#Starkeiou_Michael"/>
        <hasRegistered rdf:resource="http://xworks.gr/ontologies/ccso#Starkeiou_Michael"/>
        <includesCourse rdf:resource="http://xworks.gr/ontologies/ccso#CS672/CSE_PhD/CSD/SSE/UoC"/>
        <providedBy rdf:resource="http://xworks.gr/ontologies/ccso#Computers_Sciences_Department_of_University_of_Crete"/>
        <code rdf:datatype="http://www.w3.org/2001/XMLSchema#string">CSE_PhD/CSD/SSE/UoC</code>
        <creditsECTS rdf:datatype="http://www.w3.org/2001/XMLSchema#short">320</creditsECTS>
        <degreeTitle rdf:datatype="http://www.w3.org/2001/XMLSchema#string">Doctor of Philosophy in Computer Science and Engineering of</degreeTitle>
        <degreeType rdf:datatype="http://www.w3.org/2001/XMLSchema#string">Doctor of Philosophy</degreeType>
        <degreeType rdf:datatype="http://www.w3.org/2001/XMLSchema#string">PhD</degreeType>
        <psName rdf:datatype="http://www.w3.org/2001/XMLSchema#string">PhD in Computer Science and Engineering of Computers Sciences Department (CSD) of University of Crete</psName>
        <rdfs:label xml:lang="en">PhD in Computer Science and Engineering of University of Crete</rdfs:label>
    </owl:NamedIndividual>
    


    <!-- http://xworks.gr/ontologies/ccso#TP10K1/IE_BSc/IED/STEF/TEIC -->

    <owl:NamedIndividual rdf:about="http://xworks.gr/ontologies/ccso#TP10K1/IE_BSc/IED/STEF/TEIC">
        <rdf:type rdf:resource="http://xworks.gr/ontologies/ccso#Course"/>
        <hasSyllabus rdf:resource="http://xworks.gr/ontologies/ccso#TP10K1s2015-16/IE_BSc/IED/STEF/TEIC"/>
        <hasSyllabus rdf:resource="http://xworks.gr/ontologies/ccso#TP10K1s2016-17/IE_BSc/IED/STEF/TEIC"/>
        <hasSyllabus rdf:resource="http://xworks.gr/ontologies/ccso#TP10K1s2017-18/IE_BSc/IED/STEF/TEIC"/>
        <includedIn rdf:resource="http://xworks.gr/ontologies/ccso#BSc_Informatics_Engineering/IE_BSc/IED/STEF/TEIC"/>
        <offeredBy rdf:resource="http://xworks.gr/ontologies/ccso#Department_of_Informatics_Engineering_of_TEI_of_Crete"/>
        <courseType rdf:datatype="http://www.w3.org/2001/XMLSchema#string">Core</courseType>
        <csName rdf:datatype="http://www.w3.org/2001/XMLSchema#string">Physics</csName>
    </owl:NamedIndividual>
    


    <!-- http://xworks.gr/ontologies/ccso#TP10K1s2015-16/IE_BSc/IED/STEF/TEIC -->

    <owl:NamedIndividual rdf:about="http://xworks.gr/ontologies/ccso#TP10K1s2015-16/IE_BSc/IED/STEF/TEIC">
        <rdf:type rdf:resource="http://xworks.gr/ontologies/ccso#Syllabus"/>
        <affiliatedWith rdf:resource="http://xworks.gr/ontologies/ccso#Pachoulakis_Ioannis"/>
        <hasInstructor rdf:resource="http://xworks.gr/ontologies/ccso#Pachoulakis_Ioannis"/>
        <hasSupervisor rdf:resource="http://xworks.gr/ontologies/ccso#Pachoulakis_Ioannis"/>
        <syllabusOf rdf:resource="http://xworks.gr/ontologies/ccso#TP10K1/IE_BSc/IED/STEF/TEIC"/>
        <academicYear rdf:datatype="http://www.w3.org/2001/XMLSchema#string">2015-16</academicYear>
        <code rdf:datatype="http://www.w3.org/2001/XMLSchema#string">TP10K1s2015-16/IE_BSc/IED/STEF/TEIC</code>
        <courseType rdf:datatype="http://www.w3.org/2001/XMLSchema#string">Core</courseType>
        <creditsECTS rdf:datatype="http://www.w3.org/2001/XMLSchema#short">2</creditsECTS>
        <csName rdf:datatype="http://www.w3.org/2001/XMLSchema#string">Syllabus of course TP10K1 Physics</csName>
        <semesterinProgram rdf:datatype="http://www.w3.org/2001/XMLSchema#short">1</semesterinProgram>
    </owl:NamedIndividual>
    


    <!-- http://xworks.gr/ontologies/ccso#TP10K1s2016-17/IE_BSc/IED/STEF/TEIC -->

    <owl:NamedIndividual rdf:about="http://xworks.gr/ontologies/ccso#TP10K1s2016-17/IE_BSc/IED/STEF/TEIC">
        <rdf:type rdf:resource="http://xworks.gr/ontologies/ccso#Syllabus"/>
        <affiliatedWith rdf:resource="http://xworks.gr/ontologies/ccso#Pachoulakis_Ioannis"/>
        <hasInstructor rdf:resource="http://xworks.gr/ontologies/ccso#Pachoulakis_Ioannis"/>
        <hasSupervisor rdf:resource="http://xworks.gr/ontologies/ccso#Pachoulakis_Ioannis"/>
        <syllabusOf rdf:resource="http://xworks.gr/ontologies/ccso#TP10K1/IE_BSc/IED/STEF/TEIC"/>
        <academicYear rdf:datatype="http://www.w3.org/2001/XMLSchema#string">2016-17</academicYear>
        <code rdf:datatype="http://www.w3.org/2001/XMLSchema#string">TP10K1s2016-17/IE_BSc/IED/STEF/TEIC</code>
        <csName rdf:datatype="http://www.w3.org/2001/XMLSchema#string">Syllabus of course TP10K1 Physics</csName>
    </owl:NamedIndividual>
    


    <!-- http://xworks.gr/ontologies/ccso#TP10K1s2017-18/IE_BSc/IED/STEF/TEIC -->

    <owl:NamedIndividual rdf:about="http://xworks.gr/ontologies/ccso#TP10K1s2017-18/IE_BSc/IED/STEF/TEIC">
        <rdf:type rdf:resource="http://xworks.gr/ontologies/ccso#Syllabus"/>
        <affiliatedWith rdf:resource="http://xworks.gr/ontologies/ccso#Pachoulakis_Ioannis"/>
        <affiliatedWith rdf:resource="http://xworks.gr/ontologies/ccso#Papadourakis_George"/>
        <hasInstructor rdf:resource="http://xworks.gr/ontologies/ccso#Papadourakis_George"/>
        <hasSupervisor rdf:resource="http://xworks.gr/ontologies/ccso#Pachoulakis_Ioannis"/>
        <syllabusOf rdf:resource="http://xworks.gr/ontologies/ccso#TP10K1/IE_BSc/IED/STEF/TEIC"/>
        <academicYear rdf:datatype="http://www.w3.org/2001/XMLSchema#string">2017-18</academicYear>
        <code rdf:datatype="http://www.w3.org/2001/XMLSchema#string">TP10K1s2017-18/IE_BSc/IED/STEF/TEIC</code>
        <csName rdf:datatype="http://www.w3.org/2001/XMLSchema#string">Syllabus of course TP10K1 Physics</csName>
    </owl:NamedIndividual>
    


    <!-- http://xworks.gr/ontologies/ccso#TP10K2/IE_BSc/IED/STEF/TEIC -->

    <owl:NamedIndividual rdf:about="http://xworks.gr/ontologies/ccso#TP10K2/IE_BSc/IED/STEF/TEIC">
        <rdf:type rdf:resource="http://xworks.gr/ontologies/ccso#Course"/>
        <hasSyllabus rdf:resource="http://xworks.gr/ontologies/ccso#TP10K2s1/IE_BSc/IED/STEF/TEIC"/>
        <includedIn rdf:resource="http://xworks.gr/ontologies/ccso#BSc_Informatics_Engineering/IE_BSc/IED/STEF/TEIC"/>
        <offeredBy rdf:resource="http://xworks.gr/ontologies/ccso#Department_of_Informatics_Engineering_of_TEI_of_Crete"/>
        <code rdf:datatype="http://www.w3.org/2001/XMLSchema#string">TP10K2/IE_BSc/IED/STEF/TEIC</code>
        <courseType rdf:datatype="http://www.w3.org/2001/XMLSchema#string">Core</courseType>
        <csName rdf:datatype="http://www.w3.org/2001/XMLSchema#string">Modern Topics in Informatic</csName>
    </owl:NamedIndividual>
    


    <!-- http://xworks.gr/ontologies/ccso#TP10K2s1/IE_BSc/IED/STEF/TEIC -->

    <owl:NamedIndividual rdf:about="http://xworks.gr/ontologies/ccso#TP10K2s1/IE_BSc/IED/STEF/TEIC">
        <rdf:type rdf:resource="http://xworks.gr/ontologies/ccso#Syllabus"/>
        <affiliatedWith rdf:resource="http://xworks.gr/ontologies/ccso#Papadakis_Nikos"/>
        <hasInstructor rdf:resource="http://xworks.gr/ontologies/ccso#Papadakis_Nikos"/>
        <hasSupervisor rdf:resource="http://xworks.gr/ontologies/ccso#Papadakis_Nikos"/>
        <syllabusOf rdf:resource="http://xworks.gr/ontologies/ccso#TP10K2/IE_BSc/IED/STEF/TEIC"/>
        <code rdf:datatype="http://www.w3.org/2001/XMLSchema#string">TP10K2s1/IE_BSc/IED/STEF/TEIC</code>
        <courseType rdf:datatype="http://www.w3.org/2001/XMLSchema#string">Core</courseType>
        <creditsECTS rdf:datatype="http://www.w3.org/2001/XMLSchema#short">6</creditsECTS>
        <csName rdf:datatype="http://www.w3.org/2001/XMLSchema#string">Syllabus of course TP10K2 Modern Topics in Informatics</csName>
        <semesterinProgram rdf:datatype="http://www.w3.org/2001/XMLSchema#short">1</semesterinProgram>
        <weeklyHours rdf:datatype="http://www.w3.org/2001/XMLSchema#short">4</weeklyHours>
        <weeklyWorkload rdf:datatype="http://www.w3.org/2001/XMLSchema#short">6</weeklyWorkload>
    </owl:NamedIndividual>
    


    <!-- http://xworks.gr/ontologies/ccso#TP10K3/IE_BSc/IED/STEF/TEIC -->

    <owl:NamedIndividual rdf:about="http://xworks.gr/ontologies/ccso#TP10K3/IE_BSc/IED/STEF/TEIC">
        <rdf:type rdf:resource="http://xworks.gr/ontologies/ccso#Course"/>
        <hasSyllabus rdf:resource="http://xworks.gr/ontologies/ccso#TP10K3s1/IE_BSc/IED/STEF/TEIC"/>
        <includedIn rdf:resource="http://xworks.gr/ontologies/ccso#BSc_Informatics_Engineering/IE_BSc/IED/STEF/TEIC"/>
        <offeredBy rdf:resource="http://xworks.gr/ontologies/ccso#Department_of_Informatics_Engineering_of_TEI_of_Crete"/>
        <courseType rdf:datatype="http://www.w3.org/2001/XMLSchema#string">Core</courseType>
        <csName rdf:datatype="http://www.w3.org/2001/XMLSchema#string">Digital Design</csName>
    </owl:NamedIndividual>
    


    <!-- http://xworks.gr/ontologies/ccso#TP10K3s1/IE_BSc/IED/STEF/TEIC -->

    <owl:NamedIndividual rdf:about="http://xworks.gr/ontologies/ccso#TP10K3s1/IE_BSc/IED/STEF/TEIC">
        <rdf:type rdf:resource="http://xworks.gr/ontologies/ccso#Syllabus"/>
        <affiliatedWith rdf:resource="http://xworks.gr/ontologies/ccso#Kornaros_George"/>
        <hasInstructor rdf:resource="http://xworks.gr/ontologies/ccso#Kornaros_George"/>
        <hasSupervisor rdf:resource="http://xworks.gr/ontologies/ccso#Kornaros_George"/>
        <syllabusOf rdf:resource="http://xworks.gr/ontologies/ccso#TP10K3/IE_BSc/IED/STEF/TEIC"/>
        <courseType rdf:datatype="http://www.w3.org/2001/XMLSchema#string">Core</courseType>
        <creditsECTS rdf:datatype="http://www.w3.org/2001/XMLSchema#short">8</creditsECTS>
        <csName rdf:datatype="http://www.w3.org/2001/XMLSchema#string">Syllabus of course TP10K3 Digital Design</csName>
        <semesterinProgram rdf:datatype="http://www.w3.org/2001/XMLSchema#short">1</semesterinProgram>
    </owl:NamedIndividual>
    


    <!-- http://xworks.gr/ontologies/ccso#TP10K4/IE_BSc/IED/STEF/TEIC -->

    <owl:NamedIndividual rdf:about="http://xworks.gr/ontologies/ccso#TP10K4/IE_BSc/IED/STEF/TEIC">
        <rdf:type rdf:resource="http://xworks.gr/ontologies/ccso#Course"/>
        <affiliatedWith rdf:resource="http://xworks.gr/ontologies/ccso#Vassileiou_Joshua"/>
        <coversKA rdf:resource="http://xworks.gr/ontologies/ccso#CS/PL_Programming_Languages"/>
        <hasAttender rdf:resource="http://xworks.gr/ontologies/ccso#Vassileiou_Joshua"/>
        <hasSyllabus rdf:resource="http://xworks.gr/ontologies/ccso#TP10K4s1/IE_BSc/IED/STEF/TEIC"/>
        <includedIn rdf:resource="http://xworks.gr/ontologies/ccso#BSc_Informatics_Engineering/IE_BSc/IED/STEF/TEIC"/>
        <offeredBy rdf:resource="http://xworks.gr/ontologies/ccso#Department_of_Informatics_Engineering_of_TEI_of_Crete"/>
        <code rdf:datatype="http://www.w3.org/2001/XMLSchema#string">TP10K4/IE_BSc/IED/STEF/TEIC</code>
        <courseType rdf:datatype="http://www.w3.org/2001/XMLSchema#string">Core</courseType>
        <csName rdf:datatype="http://www.w3.org/2001/XMLSchema#string">Programming</csName>
    </owl:NamedIndividual>
    


    <!-- http://xworks.gr/ontologies/ccso#TP10K4s1/IE_BSc/IED/STEF/TEIC -->

    <owl:NamedIndividual rdf:about="http://xworks.gr/ontologies/ccso#TP10K4s1/IE_BSc/IED/STEF/TEIC">
        <rdf:type rdf:resource="http://xworks.gr/ontologies/ccso#Syllabus"/>
        <affiliatedWith rdf:resource="http://xworks.gr/ontologies/ccso#Vassilakis_Kostas"/>
        <aimsToLO rdf:resource="http://xworks.gr/ontologies/ccso#CS/PL/LO_Use_subclassing_to_design_simple_class_hierarchies_that_allow_code_to_be_reused_for_distinct_subclasses"/>
        <aimsToLO rdf:resource="http://xworks.gr/ontologies/ccso#CS/PL/LO_Compare_and_contrast_the_procedural/functional_approach_and_the_object-oriented_approach"/>
        <coversTopic rdf:resource="http://xworks.gr/ontologies/ccso#CS/PL/T_Definition_of_classes:fields,methods,and_constructors"/>
        <coversTopic rdf:resource="http://xworks.gr/ontologies/ccso#CS/PL/T_Object-Oriented_Design,Class-Hierarchy_design_for_modeling"/>
        <coversTopic rdf:resource="http://xworks.gr/ontologies/ccso#CS/PL/T_Object-Oriented_Design,_Decomposition_into_objects_carrying_state_and_having_behavior"/>
        <hasInstructor rdf:resource="http://xworks.gr/ontologies/ccso#Vassilakis_Kostas"/>
        <hasSupervisor rdf:resource="http://xworks.gr/ontologies/ccso#Vassilakis_Kostas"/>
        <syllabusOf rdf:resource="http://xworks.gr/ontologies/ccso#TP10K4/IE_BSc/IED/STEF/TEIC"/>
        <syllabusOf rdf:resource="http://xworks.gr/ontologies/ccso#TP40K4/IE_BSc/IED/STEF/TEIC"/>
        <code rdf:datatype="http://www.w3.org/2001/XMLSchema#string">TP10K4s1/IE_BSc/IED/STEF/TEIC</code>
        <courseType rdf:datatype="http://www.w3.org/2001/XMLSchema#string">Core</courseType>
        <creditsECTS rdf:datatype="http://www.w3.org/2001/XMLSchema#short">8</creditsECTS>
        <csName rdf:datatype="http://www.w3.org/2001/XMLSchema#string">Syllabus of course TP10K4 Programming</csName>
        <semesterinProgram rdf:datatype="http://www.w3.org/2001/XMLSchema#short">1</semesterinProgram>
        <weeklyHours rdf:datatype="http://www.w3.org/2001/XMLSchema#short">6</weeklyHours>
        <weeklyWorkload rdf:datatype="http://www.w3.org/2001/XMLSchema#short">14</weeklyWorkload>
    </owl:NamedIndividual>
    


    <!-- http://xworks.gr/ontologies/ccso#TP10K5/IE_BSc/IED/STEF/TEIC -->

    <owl:NamedIndividual rdf:about="http://xworks.gr/ontologies/ccso#TP10K5/IE_BSc/IED/STEF/TEIC">
        <rdf:type rdf:resource="http://xworks.gr/ontologies/ccso#Course"/>
        <affiliatedWith rdf:resource="http://xworks.gr/ontologies/ccso#Tarlis_Kostas"/>
        <hasAttender rdf:resource="http://xworks.gr/ontologies/ccso#Tarlis_Kostas"/>
        <hasSyllabus rdf:resource="http://xworks.gr/ontologies/ccso#TP10K5s1/IE_BSc/IED/STEF/TEIC"/>
        <includedIn rdf:resource="http://xworks.gr/ontologies/ccso#BSc_Informatics_Engineering/IE_BSc/IED/STEF/TEIC"/>
        <offeredBy rdf:resource="http://xworks.gr/ontologies/ccso#Department_of_Informatics_Engineering_of_TEI_of_Crete"/>
        <code rdf:datatype="http://www.w3.org/2001/XMLSchema#string">TP10K5/IE_BSc/IED/STEF/TEIC</code>
        <courseType rdf:datatype="http://www.w3.org/2001/XMLSchema#string">Core</courseType>
        <csName rdf:datatype="http://www.w3.org/2001/XMLSchema#string">Calculus</csName>
    </owl:NamedIndividual>
    


    <!-- http://xworks.gr/ontologies/ccso#TP10K5s1/IE_BSc/IED/STEF/TEIC -->

    <owl:NamedIndividual rdf:about="http://xworks.gr/ontologies/ccso#TP10K5s1/IE_BSc/IED/STEF/TEIC">
        <rdf:type rdf:resource="http://xworks.gr/ontologies/ccso#Syllabus"/>
        <affiliatedWith rdf:resource="http://xworks.gr/ontologies/ccso#Kalogiannakis_Michail"/>
        <hasInstructor rdf:resource="http://xworks.gr/ontologies/ccso#Kalogiannakis_Michail"/>
        <hasSupervisor rdf:resource="http://xworks.gr/ontologies/ccso#Kalogiannakis_Michail"/>
        <syllabusOf rdf:resource="http://xworks.gr/ontologies/ccso#TP10K5/IE_BSc/IED/STEF/TEIC"/>
        <code rdf:datatype="http://www.w3.org/2001/XMLSchema#string">TP10K5s1/IE_BSc/IED/STEF/TEIC</code>
        <courseType rdf:datatype="http://www.w3.org/2001/XMLSchema#string">Core</courseType>
        <creditsECTS rdf:datatype="http://www.w3.org/2001/XMLSchema#short">4</creditsECTS>
        <csName rdf:datatype="http://www.w3.org/2001/XMLSchema#string">Syllabus of course TP10K5 Calculus</csName>
        <semesterinProgram rdf:datatype="http://www.w3.org/2001/XMLSchema#short">1</semesterinProgram>
        <weeklyHours rdf:datatype="http://www.w3.org/2001/XMLSchema#short">4</weeklyHours>
        <weeklyWorkload rdf:datatype="http://www.w3.org/2001/XMLSchema#short">8</weeklyWorkload>
    </owl:NamedIndividual>
    


    <!-- http://xworks.gr/ontologies/ccso#TP10K6/IE_BSc/IED/STEF/TEIC -->

    <owl:NamedIndividual rdf:about="http://xworks.gr/ontologies/ccso#TP10K6/IE_BSc/IED/STEF/TEIC">
        <rdf:type rdf:resource="http://xworks.gr/ontologies/ccso#Course"/>
        <coversKA rdf:resource="http://xworks.gr/ontologies/ccso#CS/SIP_Social_Issues_and_Professional_Practice"/>
        <hasSyllabus rdf:resource="http://xworks.gr/ontologies/ccso#TP10K6s1/IE_BSc/IED/STEF/TEIC"/>
        <includedIn rdf:resource="http://xworks.gr/ontologies/ccso#BSc_Informatics_Engineering/IE_BSc/IED/STEF/TEIC"/>
        <offeredBy rdf:resource="http://xworks.gr/ontologies/ccso#Department_of_Informatics_Engineering_of_TEI_of_Crete"/>
        <courseType rdf:datatype="http://www.w3.org/2001/XMLSchema#string">Core</courseType>
        <csName rdf:datatype="http://www.w3.org/2001/XMLSchema#string">Education</csName>
    </owl:NamedIndividual>
    


    <!-- http://xworks.gr/ontologies/ccso#TP10K6s1/IE_BSc/IED/STEF/TEIC -->

    <owl:NamedIndividual rdf:about="http://xworks.gr/ontologies/ccso#TP10K6s1/IE_BSc/IED/STEF/TEIC">
        <rdf:type rdf:resource="http://xworks.gr/ontologies/ccso#Syllabus"/>
        <affiliatedWith rdf:resource="http://xworks.gr/ontologies/ccso#Xezonakis_Ioannis"/>
        <hasInstructor rdf:resource="http://xworks.gr/ontologies/ccso#Xezonakis_Ioannis"/>
        <hasSupervisor rdf:resource="http://xworks.gr/ontologies/ccso#Xezonakis_Ioannis"/>
        <syllabusOf rdf:resource="http://xworks.gr/ontologies/ccso#TP10K6/IE_BSc/IED/STEF/TEIC"/>
        <courseType rdf:datatype="http://www.w3.org/2001/XMLSchema#string">Core</courseType>
        <creditsECTS rdf:datatype="http://www.w3.org/2001/XMLSchema#short">2</creditsECTS>
        <csName rdf:datatype="http://www.w3.org/2001/XMLSchema#string">Syllabus of course TP10K6 Education</csName>
        <semesterinProgram rdf:datatype="http://www.w3.org/2001/XMLSchema#short">1</semesterinProgram>
    </owl:NamedIndividual>
    


    <!-- http://xworks.gr/ontologies/ccso#TP20K1/IE_BSc/IED/STEF/TEIC -->

    <owl:NamedIndividual rdf:about="http://xworks.gr/ontologies/ccso#TP20K1/IE_BSc/IED/STEF/TEIC">
        <rdf:type rdf:resource="http://xworks.gr/ontologies/ccso#Course"/>
        <hasSyllabus rdf:resource="http://xworks.gr/ontologies/ccso#TP20K1s1/IE_BSc/IED/STEF/TEIC"/>
        <includedIn rdf:resource="http://xworks.gr/ontologies/ccso#BSc_Informatics_Engineering/IE_BSc/IED/STEF/TEIC"/>
        <offeredBy rdf:resource="http://xworks.gr/ontologies/ccso#Department_of_Informatics_Engineering_of_TEI_of_Crete"/>
        <courseType rdf:datatype="http://www.w3.org/2001/XMLSchema#string">Core</courseType>
        <csName rdf:datatype="http://www.w3.org/2001/XMLSchema#string">Microelectronics</csName>
    </owl:NamedIndividual>
    


    <!-- http://xworks.gr/ontologies/ccso#TP20K1s1/IE_BSc/IED/STEF/TEIC -->

    <owl:NamedIndividual rdf:about="http://xworks.gr/ontologies/ccso#TP20K1s1/IE_BSc/IED/STEF/TEIC">
        <rdf:type rdf:resource="http://xworks.gr/ontologies/ccso#Syllabus"/>
        <affiliatedWith rdf:resource="http://xworks.gr/ontologies/ccso#Panagiotakis_Spyros"/>
        <hasInstructor rdf:resource="http://xworks.gr/ontologies/ccso#Panagiotakis_Spyros"/>
        <hasSupervisor rdf:resource="http://xworks.gr/ontologies/ccso#Panagiotakis_Spyros"/>
        <syllabusOf rdf:resource="http://xworks.gr/ontologies/ccso#TP20K1/IE_BSc/IED/STEF/TEIC"/>
        <courseType rdf:datatype="http://www.w3.org/2001/XMLSchema#string">Core</courseType>
        <creditsECTS rdf:datatype="http://www.w3.org/2001/XMLSchema#short">6</creditsECTS>
        <csName rdf:datatype="http://www.w3.org/2001/XMLSchema#string">Syllabus of course TP20K1 Microelectronics</csName>
        <semesterinProgram rdf:datatype="http://www.w3.org/2001/XMLSchema#short">2</semesterinProgram>
    </owl:NamedIndividual>
    


    <!-- http://xworks.gr/ontologies/ccso#TP20K2/IE_BSc/IED/STEF/TEIC -->

    <owl:NamedIndividual rdf:about="http://xworks.gr/ontologies/ccso#TP20K2/IE_BSc/IED/STEF/TEIC">
        <rdf:type rdf:resource="http://xworks.gr/ontologies/ccso#Course"/>
        <hasSyllabus rdf:resource="http://xworks.gr/ontologies/ccso#TP20K2s1/IE_BSc/IED/STEF/TEIC"/>
        <includedIn rdf:resource="http://xworks.gr/ontologies/ccso#BSc_Informatics_Engineering/IE_BSc/IED/STEF/TEIC"/>
        <offeredBy rdf:resource="http://xworks.gr/ontologies/ccso#Department_of_Informatics_Engineering_of_TEI_of_Crete"/>
        <courseType rdf:datatype="http://www.w3.org/2001/XMLSchema#string">Core</courseType>
        <csName rdf:datatype="http://www.w3.org/2001/XMLSchema#string">Computer Architecture</csName>
    </owl:NamedIndividual>
    


    <!-- http://xworks.gr/ontologies/ccso#TP20K2s1/IE_BSc/IED/STEF/TEIC -->

    <owl:NamedIndividual rdf:about="http://xworks.gr/ontologies/ccso#TP20K2s1/IE_BSc/IED/STEF/TEIC">
        <rdf:type rdf:resource="http://xworks.gr/ontologies/ccso#Syllabus"/>
        <affiliatedWith rdf:resource="http://xworks.gr/ontologies/ccso#Kornaros_George"/>
        <hasInstructor rdf:resource="http://xworks.gr/ontologies/ccso#Kornaros_George"/>
        <hasSupervisor rdf:resource="http://xworks.gr/ontologies/ccso#Kornaros_George"/>
        <syllabusOf rdf:resource="http://xworks.gr/ontologies/ccso#TP20K2/IE_BSc/IED/STEF/TEIC"/>
        <courseType rdf:datatype="http://www.w3.org/2001/XMLSchema#string">Core</courseType>
        <creditsECTS rdf:datatype="http://www.w3.org/2001/XMLSchema#short">6</creditsECTS>
        <csName rdf:datatype="http://www.w3.org/2001/XMLSchema#string">Syllabus of course TP20K2 Computer Architecture</csName>
        <semesterinProgram rdf:datatype="http://www.w3.org/2001/XMLSchema#short">2</semesterinProgram>
    </owl:NamedIndividual>
    


    <!-- http://xworks.gr/ontologies/ccso#TP20K3/IE_BSc/IED/STEF/TEIC -->

    <owl:NamedIndividual rdf:about="http://xworks.gr/ontologies/ccso#TP20K3/IE_BSc/IED/STEF/TEIC">
        <rdf:type rdf:resource="http://xworks.gr/ontologies/ccso#Course"/>
        <hasSyllabus rdf:resource="http://xworks.gr/ontologies/ccso#TP20K3s1/IE_BSc/IED/STEF/TEIC"/>
        <includedIn rdf:resource="http://xworks.gr/ontologies/ccso#BSc_Informatics_Engineering/IE_BSc/IED/STEF/TEIC"/>
        <offeredBy rdf:resource="http://xworks.gr/ontologies/ccso#Department_of_Informatics_Engineering_of_TEI_of_Crete"/>
        <courseType rdf:datatype="http://www.w3.org/2001/XMLSchema#string">Core</courseType>
        <csName rdf:datatype="http://www.w3.org/2001/XMLSchema#string">Introduction to Telecommunications</csName>
    </owl:NamedIndividual>
    


    <!-- http://xworks.gr/ontologies/ccso#TP20K3s1/IE_BSc/IED/STEF/TEIC -->

    <owl:NamedIndividual rdf:about="http://xworks.gr/ontologies/ccso#TP20K3s1/IE_BSc/IED/STEF/TEIC">
        <rdf:type rdf:resource="http://xworks.gr/ontologies/ccso#Syllabus"/>
        <affiliatedWith rdf:resource="http://xworks.gr/ontologies/ccso#Stratakis_Dimitrios"/>
        <hasInstructor rdf:resource="http://xworks.gr/ontologies/ccso#Stratakis_Dimitrios"/>
        <hasSupervisor rdf:resource="http://xworks.gr/ontologies/ccso#Stratakis_Dimitrios"/>
        <syllabusOf rdf:resource="http://xworks.gr/ontologies/ccso#TP20K3/IE_BSc/IED/STEF/TEIC"/>
        <courseType rdf:datatype="http://www.w3.org/2001/XMLSchema#string">Core</courseType>
        <creditsECTS rdf:datatype="http://www.w3.org/2001/XMLSchema#short">6</creditsECTS>
        <csName rdf:datatype="http://www.w3.org/2001/XMLSchema#string">Syllabus of course TP20K3 Introduction to Telecommunications</csName>
        <semesterinProgram rdf:datatype="http://www.w3.org/2001/XMLSchema#short">2</semesterinProgram>
    </owl:NamedIndividual>
    


    <!-- http://xworks.gr/ontologies/ccso#TP20K4/IE_BSc/IED/STEF/TEIC -->

    <owl:NamedIndividual rdf:about="http://xworks.gr/ontologies/ccso#TP20K4/IE_BSc/IED/STEF/TEIC">
        <rdf:type rdf:resource="http://xworks.gr/ontologies/ccso#Course"/>
        <hasPrerequisite rdf:resource="http://xworks.gr/ontologies/ccso#TP10K4/IE_BSc/IED/STEF/TEIC"/>
        <hasSyllabus rdf:resource="http://xworks.gr/ontologies/ccso#TP20K4s1/IE_BSc/IED/STEF/TEIC"/>
        <includedIn rdf:resource="http://xworks.gr/ontologies/ccso#BSc_Informatics_Engineering/IE_BSc/IED/STEF/TEIC"/>
        <offeredBy rdf:resource="http://xworks.gr/ontologies/ccso#Department_of_Informatics_Engineering_of_TEI_of_Crete"/>
        <code rdf:datatype="http://www.w3.org/2001/XMLSchema#string">TP20K4/IE_BSc/IED/STEF/TEIC</code>
        <courseType rdf:datatype="http://www.w3.org/2001/XMLSchema#string">Core</courseType>
        <csName rdf:datatype="http://www.w3.org/2001/XMLSchema#string">Data Structures</csName>
    </owl:NamedIndividual>
    


    <!-- http://xworks.gr/ontologies/ccso#TP20K4s1/IE_BSc/IED/STEF/TEIC -->

    <owl:NamedIndividual rdf:about="http://xworks.gr/ontologies/ccso#TP20K4s1/IE_BSc/IED/STEF/TEIC">
        <rdf:type rdf:resource="http://xworks.gr/ontologies/ccso#Syllabus"/>
        <affiliatedWith rdf:resource="http://xworks.gr/ontologies/ccso#Vassilakis_Kostas"/>
        <aimsToLO rdf:resource="http://xworks.gr/ontologies/ccso#CS/PL/LO_Compare_and_contrast_the_procedural/functional_approach_and_the_object-oriented_approach"/>
        <coversTopic rdf:resource="http://xworks.gr/ontologies/ccso#CS/PL/T_Definition_of_classes:fields,methods,and_constructors"/>
        <coversTopic rdf:resource="http://xworks.gr/ontologies/ccso#CS/PL/T_Dynamic_dispatch:Definition_of_Method-Call"/>
        <coversTopic rdf:resource="http://xworks.gr/ontologies/ccso#CS/PL/T_Subclasses,Inheritance,and_Method_Overriding"/>
        <hasInstructor rdf:resource="http://xworks.gr/ontologies/ccso#Vassilakis_Kostas"/>
        <hasSupervisor rdf:resource="http://xworks.gr/ontologies/ccso#Vassilakis_Kostas"/>
        <syllabusOf rdf:resource="http://xworks.gr/ontologies/ccso#TP20K4/IE_BSc/IED/STEF/TEIC"/>
        <code rdf:datatype="http://www.w3.org/2001/XMLSchema#string">TP20K4s1/IE_BSc/IED/STEF/TEIC</code>
        <courseType rdf:datatype="http://www.w3.org/2001/XMLSchema#string">Core</courseType>
        <creditsECTS rdf:datatype="http://www.w3.org/2001/XMLSchema#short">6</creditsECTS>
        <csName rdf:datatype="http://www.w3.org/2001/XMLSchema#string">Syllabus of course TP20K4 Data Structures</csName>
        <semesterinProgram rdf:datatype="http://www.w3.org/2001/XMLSchema#short">2</semesterinProgram>
        <weeklyHours rdf:datatype="http://www.w3.org/2001/XMLSchema#short">5</weeklyHours>
        <weeklyWorkload rdf:datatype="http://www.w3.org/2001/XMLSchema#short">11</weeklyWorkload>
    </owl:NamedIndividual>
    


    <!-- http://xworks.gr/ontologies/ccso#TP20K6/IE_BSc/IED/STEF/TEIC -->

    <owl:NamedIndividual rdf:about="http://xworks.gr/ontologies/ccso#TP20K6/IE_BSc/IED/STEF/TEIC">
        <rdf:type rdf:resource="http://xworks.gr/ontologies/ccso#Course"/>
        <hasSyllabus rdf:resource="http://xworks.gr/ontologies/ccso#TP20K6s1/IE_BSc/IED/STEF/TEIC"/>
        <includedIn rdf:resource="http://xworks.gr/ontologies/ccso#BSc_Informatics_Engineering/IE_BSc/IED/STEF/TEIC"/>
        <offeredBy rdf:resource="http://xworks.gr/ontologies/ccso#Department_of_Informatics_Engineering_of_TEI_of_Crete"/>
        <courseType rdf:datatype="http://www.w3.org/2001/XMLSchema#string">Core</courseType>
        <csName rdf:datatype="http://www.w3.org/2001/XMLSchema#string">Innovation, the Internet and Entrepreneurship</csName>
    </owl:NamedIndividual>
    


    <!-- http://xworks.gr/ontologies/ccso#TP20K6s1/IE_BSc/IED/STEF/TEIC -->

    <owl:NamedIndividual rdf:about="http://xworks.gr/ontologies/ccso#TP20K6s1/IE_BSc/IED/STEF/TEIC">
        <rdf:type rdf:resource="http://xworks.gr/ontologies/ccso#Syllabus"/>
        <affiliatedWith rdf:resource="http://xworks.gr/ontologies/ccso#Tsiknakis_Manolis"/>
        <hasInstructor rdf:resource="http://xworks.gr/ontologies/ccso#Tsiknakis_Manolis"/>
        <hasSupervisor rdf:resource="http://xworks.gr/ontologies/ccso#Tsiknakis_Manolis"/>
        <syllabusOf rdf:resource="http://xworks.gr/ontologies/ccso#TP20K6/IE_BSc/IED/STEF/TEIC"/>
        <courseType rdf:datatype="http://www.w3.org/2001/XMLSchema#string">Core</courseType>
        <creditsECTS rdf:datatype="http://www.w3.org/2001/XMLSchema#short">2</creditsECTS>
        <csName rdf:datatype="http://www.w3.org/2001/XMLSchema#string">Syllabus of course TP20K6 Innovation, the Internet and Entrepreneurship</csName>
        <semesterinProgram rdf:datatype="http://www.w3.org/2001/XMLSchema#short">2</semesterinProgram>
    </owl:NamedIndividual>
    


    <!-- http://xworks.gr/ontologies/ccso#TP20K7/IE_BSc/IED/STEF/TEIC -->

    <owl:NamedIndividual rdf:about="http://xworks.gr/ontologies/ccso#TP20K7/IE_BSc/IED/STEF/TEIC">
        <rdf:type rdf:resource="http://xworks.gr/ontologies/ccso#Course"/>
        <hasPrerequisite rdf:resource="http://xworks.gr/ontologies/ccso#TP10K5/IE_BSc/IED/STEF/TEIC"/>
        <hasSyllabus rdf:resource="http://xworks.gr/ontologies/ccso#TP20K7s1/IE_BSc/IED/STEF/TEIC"/>
        <includedIn rdf:resource="http://xworks.gr/ontologies/ccso#BSc_Informatics_Engineering/IE_BSc/IED/STEF/TEIC"/>
        <offeredBy rdf:resource="http://xworks.gr/ontologies/ccso#Department_of_Informatics_Engineering_of_TEI_of_Crete"/>
        <code rdf:datatype="http://www.w3.org/2001/XMLSchema#string">TP20K7/IE_BSc/IED/STEF/TEIC</code>
        <courseType rdf:datatype="http://www.w3.org/2001/XMLSchema#string">Core</courseType>
        <csName rdf:datatype="http://www.w3.org/2001/XMLSchema#string">Discrete Mathematics</csName>
    </owl:NamedIndividual>
    


    <!-- http://xworks.gr/ontologies/ccso#TP20K7s1/IE_BSc/IED/STEF/TEIC -->

    <owl:NamedIndividual rdf:about="http://xworks.gr/ontologies/ccso#TP20K7s1/IE_BSc/IED/STEF/TEIC">
        <rdf:type rdf:resource="http://xworks.gr/ontologies/ccso#Syllabus"/>
        <affiliatedWith rdf:resource="http://xworks.gr/ontologies/ccso#Kalogiannakis_Michail"/>
        <hasInstructor rdf:resource="http://xworks.gr/ontologies/ccso#Kalogiannakis_Michail"/>
        <hasSupervisor rdf:resource="http://xworks.gr/ontologies/ccso#Kalogiannakis_Michail"/>
        <syllabusOf rdf:resource="http://xworks.gr/ontologies/ccso#TP20K7/IE_BSc/IED/STEF/TEIC"/>
        <code rdf:datatype="http://www.w3.org/2001/XMLSchema#string">TP20K7s1/IE_BSc/IED/STEF/TEIC</code>
        <courseType rdf:datatype="http://www.w3.org/2001/XMLSchema#string">Core</courseType>
        <creditsECTS rdf:datatype="http://www.w3.org/2001/XMLSchema#short">4</creditsECTS>
        <csName rdf:datatype="http://www.w3.org/2001/XMLSchema#string">Syllabus of course TP20K7 Discrete Mathematics</csName>
        <semesterinProgram rdf:datatype="http://www.w3.org/2001/XMLSchema#short">2</semesterinProgram>
        <weeklyHours rdf:datatype="http://www.w3.org/2001/XMLSchema#short">3</weeklyHours>
        <weeklyWorkload rdf:datatype="http://www.w3.org/2001/XMLSchema#short">8</weeklyWorkload>
    </owl:NamedIndividual>
    


    <!-- http://xworks.gr/ontologies/ccso#TP30K1/IE_BSc/IED/STEF/TEIC -->

    <owl:NamedIndividual rdf:about="http://xworks.gr/ontologies/ccso#TP30K1/IE_BSc/IED/STEF/TEIC">
        <rdf:type rdf:resource="http://xworks.gr/ontologies/ccso#Course"/>
        <affiliatedWith rdf:resource="http://xworks.gr/ontologies/ccso#Vassileiou_Marcela"/>
        <hasAttender rdf:resource="http://xworks.gr/ontologies/ccso#Vassileiou_Marcela"/>
        <hasSyllabus rdf:resource="http://xworks.gr/ontologies/ccso#TP30K1s1/IE_BSc/IED/STEF/TEIC"/>
        <includedIn rdf:resource="http://xworks.gr/ontologies/ccso#BSc_Informatics_Engineering/IE_BSc/IED/STEF/TEIC"/>
        <offeredBy rdf:resource="http://xworks.gr/ontologies/ccso#Department_of_Informatics_Engineering_of_TEI_of_Crete"/>
        <courseType rdf:datatype="http://www.w3.org/2001/XMLSchema#string">Core</courseType>
        <csName rdf:datatype="http://www.w3.org/2001/XMLSchema#string">Operating Systems</csName>
    </owl:NamedIndividual>
    


    <!-- http://xworks.gr/ontologies/ccso#TP30K1s1/IE_BSc/IED/STEF/TEIC -->

    <owl:NamedIndividual rdf:about="http://xworks.gr/ontologies/ccso#TP30K1s1/IE_BSc/IED/STEF/TEIC">
        <rdf:type rdf:resource="http://xworks.gr/ontologies/ccso#Syllabus"/>
        <affiliatedWith rdf:resource="http://xworks.gr/ontologies/ccso#Grammatikakis_Miltiadis"/>
        <hasInstructor rdf:resource="http://xworks.gr/ontologies/ccso#Grammatikakis_Miltiadis"/>
        <hasSupervisor rdf:resource="http://xworks.gr/ontologies/ccso#Grammatikakis_Miltiadis"/>
        <syllabusOf rdf:resource="http://xworks.gr/ontologies/ccso#TP30K1/IE_BSc/IED/STEF/TEIC"/>
        <courseType rdf:datatype="http://www.w3.org/2001/XMLSchema#string">Core</courseType>
        <creditsECTS rdf:datatype="http://www.w3.org/2001/XMLSchema#short">6</creditsECTS>
        <csName rdf:datatype="http://www.w3.org/2001/XMLSchema#string">Syllabus of course TP30K1 Operating Systems</csName>
        <semesterinProgram rdf:datatype="http://www.w3.org/2001/XMLSchema#short">3</semesterinProgram>
    </owl:NamedIndividual>
    


    <!-- http://xworks.gr/ontologies/ccso#TP30K2/IE_BSc/IED/STEF/TEIC -->

    <owl:NamedIndividual rdf:about="http://xworks.gr/ontologies/ccso#TP30K2/IE_BSc/IED/STEF/TEIC">
        <rdf:type rdf:resource="http://xworks.gr/ontologies/ccso#Course"/>
        <affiliatedWith rdf:resource="http://xworks.gr/ontologies/ccso#Vassileiou_Marcela"/>
        <hasAttender rdf:resource="http://xworks.gr/ontologies/ccso#Vassileiou_Marcela"/>
        <hasSyllabus rdf:resource="http://xworks.gr/ontologies/ccso#TP30K2s1/IE_BSc/IED/STEF/TEIC"/>
        <includedIn rdf:resource="http://xworks.gr/ontologies/ccso#BSc_Informatics_Engineering/IE_BSc/IED/STEF/TEIC"/>
        <offeredBy rdf:resource="http://xworks.gr/ontologies/ccso#Department_of_Informatics_Engineering_of_TEI_of_Crete"/>
        <courseType rdf:datatype="http://www.w3.org/2001/XMLSchema#string">Core</courseType>
        <csName rdf:datatype="http://www.w3.org/2001/XMLSchema#string">Databases</csName>
    </owl:NamedIndividual>
    


    <!-- http://xworks.gr/ontologies/ccso#TP30K2s1/IE_BSc/IED/STEF/TEIC -->

    <owl:NamedIndividual rdf:about="http://xworks.gr/ontologies/ccso#TP30K2s1/IE_BSc/IED/STEF/TEIC">
        <rdf:type rdf:resource="http://xworks.gr/ontologies/ccso#Syllabus"/>
        <affiliatedWith rdf:resource="http://xworks.gr/ontologies/ccso#Akoumianakis_Demosthenes"/>
        <hasInstructor rdf:resource="http://xworks.gr/ontologies/ccso#Akoumianakis_Demosthenes"/>
        <hasSupervisor rdf:resource="http://xworks.gr/ontologies/ccso#Akoumianakis_Demosthenes"/>
        <syllabusOf rdf:resource="http://xworks.gr/ontologies/ccso#TP30K2/IE_BSc/IED/STEF/TEIC"/>
        <courseType rdf:datatype="http://www.w3.org/2001/XMLSchema#string">Core</courseType>
        <creditsECTS rdf:datatype="http://www.w3.org/2001/XMLSchema#short">6</creditsECTS>
        <csName rdf:datatype="http://www.w3.org/2001/XMLSchema#string">Syllabus of course TP30K2 Databases</csName>
        <semesterinProgram rdf:datatype="http://www.w3.org/2001/XMLSchema#short">3</semesterinProgram>
    </owl:NamedIndividual>
    


    <!-- http://xworks.gr/ontologies/ccso#TP30K4/IE_BSc/IED/STEF/TEIC -->

    <owl:NamedIndividual rdf:about="http://xworks.gr/ontologies/ccso#TP30K4/IE_BSc/IED/STEF/TEIC">
        <rdf:type rdf:resource="http://xworks.gr/ontologies/ccso#Course"/>
        <affiliatedWith rdf:resource="http://xworks.gr/ontologies/ccso#Vassileiou_Marcela"/>
        <coversKA rdf:resource="http://xworks.gr/ontologies/ccso#CS/PL_Programming_Languages"/>
        <hasAttender rdf:resource="http://xworks.gr/ontologies/ccso#Vassileiou_Marcela"/>
        <hasSyllabus rdf:resource="http://xworks.gr/ontologies/ccso#TP30K4s1/IE_BSc/IED/STEF/TEIC"/>
        <includedIn rdf:resource="http://xworks.gr/ontologies/ccso#BSc_Informatics_Engineering/IE_BSc/IED/STEF/TEIC"/>
        <offeredBy rdf:resource="http://xworks.gr/ontologies/ccso#Department_of_Informatics_Engineering_of_TEI_of_Crete"/>
        <courseType rdf:datatype="http://www.w3.org/2001/XMLSchema#string">Core</courseType>
        <csName rdf:datatype="http://www.w3.org/2001/XMLSchema#string">Algorithms</csName>
    </owl:NamedIndividual>
    


    <!-- http://xworks.gr/ontologies/ccso#TP30K4s1/IE_BSc/IED/STEF/TEIC -->

    <owl:NamedIndividual rdf:about="http://xworks.gr/ontologies/ccso#TP30K4s1/IE_BSc/IED/STEF/TEIC">
        <rdf:type rdf:resource="http://xworks.gr/ontologies/ccso#Syllabus"/>
        <affiliatedWith rdf:resource="http://xworks.gr/ontologies/ccso#Fragopoulou_Paraskevi"/>
        <hasInstructor rdf:resource="http://xworks.gr/ontologies/ccso#Fragopoulou_Paraskevi"/>
        <hasSupervisor rdf:resource="http://xworks.gr/ontologies/ccso#Fragopoulou_Paraskevi"/>
        <syllabusOf rdf:resource="http://xworks.gr/ontologies/ccso#TP30K4/IE_BSc/IED/STEF/TEIC"/>
        <courseType rdf:datatype="http://www.w3.org/2001/XMLSchema#string">Core</courseType>
        <creditsECTS rdf:datatype="http://www.w3.org/2001/XMLSchema#short">6</creditsECTS>
        <csName rdf:datatype="http://www.w3.org/2001/XMLSchema#string">Syllabus of course TP30K4 Algorithms</csName>
        <semesterinProgram rdf:datatype="http://www.w3.org/2001/XMLSchema#short">3</semesterinProgram>
    </owl:NamedIndividual>
    


    <!-- http://xworks.gr/ontologies/ccso#TP30K5/IE_BSc/IED/STEF/TEIC -->

    <owl:NamedIndividual rdf:about="http://xworks.gr/ontologies/ccso#TP30K5/IE_BSc/IED/STEF/TEIC">
        <rdf:type rdf:resource="http://xworks.gr/ontologies/ccso#Course"/>
        <affiliatedWith rdf:resource="http://xworks.gr/ontologies/ccso#Vassileiou_Marcela"/>
        <hasAttender rdf:resource="http://xworks.gr/ontologies/ccso#Vassileiou_Marcela"/>
        <hasPrerequisite rdf:resource="http://xworks.gr/ontologies/ccso#TP10K5/IE_BSc/IED/STEF/TEIC"/>
        <hasSyllabus rdf:resource="http://xworks.gr/ontologies/ccso#TP30K5s1/IE_BSc/IED/STEF/TEIC"/>
        <includedIn rdf:resource="http://xworks.gr/ontologies/ccso#BSc_Informatics_Engineering/IE_BSc/IED/STEF/TEIC"/>
        <offeredBy rdf:resource="http://xworks.gr/ontologies/ccso#Department_of_Informatics_Engineering_of_TEI_of_Crete"/>
        <courseType rdf:datatype="http://www.w3.org/2001/XMLSchema#string">Core</courseType>
        <csName rdf:datatype="http://www.w3.org/2001/XMLSchema#string">Applied Mathematics</csName>
    </owl:NamedIndividual>
    


    <!-- http://xworks.gr/ontologies/ccso#TP30K5s1/IE_BSc/IED/STEF/TEIC -->

    <owl:NamedIndividual rdf:about="http://xworks.gr/ontologies/ccso#TP30K5s1/IE_BSc/IED/STEF/TEIC">
        <rdf:type rdf:resource="http://xworks.gr/ontologies/ccso#Syllabus"/>
        <affiliatedWith rdf:resource="http://xworks.gr/ontologies/ccso#Karagiannakis_Dimitrios"/>
        <hasInstructor rdf:resource="http://xworks.gr/ontologies/ccso#Karagiannakis_Dimitrios"/>
        <hasSupervisor rdf:resource="http://xworks.gr/ontologies/ccso#Karagiannakis_Dimitrios"/>
        <syllabusOf rdf:resource="http://xworks.gr/ontologies/ccso#TP30K5/IE_BSc/IED/STEF/TEIC"/>
        <courseType rdf:datatype="http://www.w3.org/2001/XMLSchema#string">Core</courseType>
        <creditsECTS rdf:datatype="http://www.w3.org/2001/XMLSchema#short">4</creditsECTS>
        <csName rdf:datatype="http://www.w3.org/2001/XMLSchema#string">Syllabus of course TP30K5 Applied Mathematics</csName>
        <semesterinProgram rdf:datatype="http://www.w3.org/2001/XMLSchema#short">3</semesterinProgram>
    </owl:NamedIndividual>
    


    <!-- http://xworks.gr/ontologies/ccso#TP30K6/IE_BSc/IED/STEF/TEIC -->

    <owl:NamedIndividual rdf:about="http://xworks.gr/ontologies/ccso#TP30K6/IE_BSc/IED/STEF/TEIC">
        <rdf:type rdf:resource="http://xworks.gr/ontologies/ccso#Course"/>
        <affiliatedWith rdf:resource="http://xworks.gr/ontologies/ccso#Vassileiou_Marcela"/>
        <hasAttender rdf:resource="http://xworks.gr/ontologies/ccso#Vassileiou_Marcela"/>
        <hasSyllabus rdf:resource="http://xworks.gr/ontologies/ccso#TP30K6s1/IE_BSc/IED/STEF/TEIC"/>
        <includedIn rdf:resource="http://xworks.gr/ontologies/ccso#BSc_Informatics_Engineering/IE_BSc/IED/STEF/TEIC"/>
        <offeredBy rdf:resource="http://xworks.gr/ontologies/ccso#Department_of_Informatics_Engineering_of_TEI_of_Crete"/>
        <courseType rdf:datatype="http://www.w3.org/2001/XMLSchema#string">Core</courseType>
        <csName rdf:datatype="http://www.w3.org/2001/XMLSchema#string">Terminology and Technical Writing</csName>
    </owl:NamedIndividual>
    


    <!-- http://xworks.gr/ontologies/ccso#TP30K6s1/IE_BSc/IED/STEF/TEIC -->

    <owl:NamedIndividual rdf:about="http://xworks.gr/ontologies/ccso#TP30K6s1/IE_BSc/IED/STEF/TEIC">
        <rdf:type rdf:resource="http://xworks.gr/ontologies/ccso#Syllabus"/>
        <affiliatedWith rdf:resource="http://xworks.gr/ontologies/ccso#Tsiknakis_Manolis"/>
        <hasInstructor rdf:resource="http://xworks.gr/ontologies/ccso#Tsiknakis_Manolis"/>
        <hasSupervisor rdf:resource="http://xworks.gr/ontologies/ccso#Tsiknakis_Manolis"/>
        <syllabusOf rdf:resource="http://xworks.gr/ontologies/ccso#TP30K6/IE_BSc/IED/STEF/TEIC"/>
        <courseType rdf:datatype="http://www.w3.org/2001/XMLSchema#string">Core</courseType>
        <creditsECTS rdf:datatype="http://www.w3.org/2001/XMLSchema#short">2</creditsECTS>
        <csName rdf:datatype="http://www.w3.org/2001/XMLSchema#string">Syllabus of course TP30K6 Terminology and Technical Writing</csName>
        <semesterinProgram rdf:datatype="http://www.w3.org/2001/XMLSchema#short">3</semesterinProgram>
    </owl:NamedIndividual>
    


    <!-- http://xworks.gr/ontologies/ccso#TP30K7/IE_BSc/IED/STEF/TEIC -->

    <owl:NamedIndividual rdf:about="http://xworks.gr/ontologies/ccso#TP30K7/IE_BSc/IED/STEF/TEIC">
        <rdf:type rdf:resource="http://xworks.gr/ontologies/ccso#Course"/>
        <hasSyllabus rdf:resource="http://xworks.gr/ontologies/ccso#TP30K7s1/IE_BSc/IED/STEF/TEIC"/>
        <includedIn rdf:resource="http://xworks.gr/ontologies/ccso#BSc_Informatics_Engineering/IE_BSc/IED/STEF/TEIC"/>
        <offeredBy rdf:resource="http://xworks.gr/ontologies/ccso#Department_of_Informatics_Engineering_of_TEI_of_Crete"/>
        <courseType rdf:datatype="http://www.w3.org/2001/XMLSchema#string">Core</courseType>
        <csName rdf:datatype="http://www.w3.org/2001/XMLSchema#string">Multimedia Technology</csName>
    </owl:NamedIndividual>
    


    <!-- http://xworks.gr/ontologies/ccso#TP30K7s1/IE_BSc/IED/STEF/TEIC -->

    <owl:NamedIndividual rdf:about="http://xworks.gr/ontologies/ccso#TP30K7s1/IE_BSc/IED/STEF/TEIC">
        <rdf:type rdf:resource="http://xworks.gr/ontologies/ccso#Syllabus"/>
        <affiliatedWith rdf:resource="http://xworks.gr/ontologies/ccso#Pachoulakis_Ioannis"/>
        <hasInstructor rdf:resource="http://xworks.gr/ontologies/ccso#Pachoulakis_Ioannis"/>
        <hasSupervisor rdf:resource="http://xworks.gr/ontologies/ccso#Pachoulakis_Ioannis"/>
        <syllabusOf rdf:resource="http://xworks.gr/ontologies/ccso#TP30K7/IE_BSc/IED/STEF/TEIC"/>
        <courseType rdf:datatype="http://www.w3.org/2001/XMLSchema#string">Core</courseType>
        <creditsECTS rdf:datatype="http://www.w3.org/2001/XMLSchema#short">6</creditsECTS>
        <csName rdf:datatype="http://www.w3.org/2001/XMLSchema#string">Syllabus of course TP30K7 Multimedia Technology</csName>
        <semesterinProgram rdf:datatype="http://www.w3.org/2001/XMLSchema#short">3</semesterinProgram>
    </owl:NamedIndividual>
    


    <!-- http://xworks.gr/ontologies/ccso#TP40K1/IE_BSc/IED/STEF/TEIC -->

    <owl:NamedIndividual rdf:about="http://xworks.gr/ontologies/ccso#TP40K1/IE_BSc/IED/STEF/TEIC">
        <rdf:type rdf:resource="http://xworks.gr/ontologies/ccso#Course"/>
        <affiliatedWith rdf:resource="http://xworks.gr/ontologies/ccso#Tarlis_Kostas"/>
        <hasAttender rdf:resource="http://xworks.gr/ontologies/ccso#Tarlis_Kostas"/>
        <hasSyllabus rdf:resource="http://xworks.gr/ontologies/ccso#TP40K1s1/IE_BSc/IED/STEF/TEIC"/>
        <includedIn rdf:resource="http://xworks.gr/ontologies/ccso#BSc_Informatics_Engineering/IE_BSc/IED/STEF/TEIC"/>
        <offeredBy rdf:resource="http://xworks.gr/ontologies/ccso#Department_of_Informatics_Engineering_of_TEI_of_Crete"/>
        <courseType rdf:datatype="http://www.w3.org/2001/XMLSchema#string">Core</courseType>
        <csName rdf:datatype="http://www.w3.org/2001/XMLSchema#string">Digital Signal Processing</csName>
    </owl:NamedIndividual>
    


    <!-- http://xworks.gr/ontologies/ccso#TP40K1s1/IE_BSc/IED/STEF/TEIC -->

    <owl:NamedIndividual rdf:about="http://xworks.gr/ontologies/ccso#TP40K1s1/IE_BSc/IED/STEF/TEIC">
        <rdf:type rdf:resource="http://xworks.gr/ontologies/ccso#Syllabus"/>
        <affiliatedWith rdf:resource="http://xworks.gr/ontologies/ccso#Papadourakis_George"/>
        <hasInstructor rdf:resource="http://xworks.gr/ontologies/ccso#Papadourakis_George"/>
        <hasSupervisor rdf:resource="http://xworks.gr/ontologies/ccso#Papadourakis_George"/>
        <syllabusOf rdf:resource="http://xworks.gr/ontologies/ccso#TP40K1/IE_BSc/IED/STEF/TEIC"/>
        <courseType rdf:datatype="http://www.w3.org/2001/XMLSchema#string">Core</courseType>
        <creditsECTS rdf:datatype="http://www.w3.org/2001/XMLSchema#short">6</creditsECTS>
        <csName rdf:datatype="http://www.w3.org/2001/XMLSchema#string">Syllabus of course TP40K1 Digital Signal Processing</csName>
        <semesterinProgram rdf:datatype="http://www.w3.org/2001/XMLSchema#short">4</semesterinProgram>
    </owl:NamedIndividual>
    


    <!-- http://xworks.gr/ontologies/ccso#TP40K2/IE_BSc/IED/STEF/TEIC -->

    <owl:NamedIndividual rdf:about="http://xworks.gr/ontologies/ccso#TP40K2/IE_BSc/IED/STEF/TEIC">
        <rdf:type rdf:resource="http://xworks.gr/ontologies/ccso#Course"/>
        <affiliatedWith rdf:resource="http://xworks.gr/ontologies/ccso#Tarlis_Kostas"/>
        <hasAttender rdf:resource="http://xworks.gr/ontologies/ccso#Tarlis_Kostas"/>
        <hasSyllabus rdf:resource="http://xworks.gr/ontologies/ccso#TP40K2s1/IE_BSc/IED/STEF/TEIC"/>
        <includedIn rdf:resource="http://xworks.gr/ontologies/ccso#BSc_Informatics_Engineering/IE_BSc/IED/STEF/TEIC"/>
        <offeredBy rdf:resource="http://xworks.gr/ontologies/ccso#Department_of_Informatics_Engineering_of_TEI_of_Crete"/>
        <code rdf:datatype="http://www.w3.org/2001/XMLSchema#string">TP40K2/IE_BSc/IED/STEF/TEIC</code>
        <courseType rdf:datatype="http://www.w3.org/2001/XMLSchema#string">Core</courseType>
        <csName rdf:datatype="http://www.w3.org/2001/XMLSchema#string">Computer Networks</csName>
    </owl:NamedIndividual>
    


    <!-- http://xworks.gr/ontologies/ccso#TP40K2s1/IE_BSc/IED/STEF/TEIC -->

    <owl:NamedIndividual rdf:about="http://xworks.gr/ontologies/ccso#TP40K2s1/IE_BSc/IED/STEF/TEIC">
        <rdf:type rdf:resource="http://xworks.gr/ontologies/ccso#Syllabus"/>
        <affiliatedWith rdf:resource="http://xworks.gr/ontologies/ccso#Panagiotakis_Spyros"/>
        <aimsToLO rdf:resource="http://xworks.gr/ontologies/ccso#CS/NC/LAN/LO_Describe_how_frames_are_forwarded_in_an_Ethernet_network"/>
        <aimsToLO rdf:resource="http://xworks.gr/ontologies/ccso#CS/NC/LAN/LO_Describe_the_steps_used_in_one_common_approach_to_the_multiple_access_problem"/>
        <aimsToLO rdf:resource="http://xworks.gr/ontologies/ccso#CS/NC/LAN/LO_Identify_the_differences_between_IP_and_Ethernet"/>
        <coversTopic rdf:resource="http://xworks.gr/ontologies/ccso#CS/NC/LAN/T_Ethernet"/>
        <coversTopic rdf:resource="http://xworks.gr/ontologies/ccso#CS/NC/LAN/T_Multiple_Access_Problem"/>
        <coversTopic rdf:resource="http://xworks.gr/ontologies/ccso#CS/NC/LAN/T_Switching"/>
        <hasInstructor rdf:resource="http://xworks.gr/ontologies/ccso#Panagiotakis_Spyros"/>
        <hasSupervisor rdf:resource="http://xworks.gr/ontologies/ccso#Panagiotakis_Spyros"/>
        <syllabusOf rdf:resource="http://xworks.gr/ontologies/ccso#TP40K2/IE_BSc/IED/STEF/TEIC"/>
        <courseType rdf:datatype="http://www.w3.org/2001/XMLSchema#string">Core</courseType>
        <creditsECTS rdf:datatype="http://www.w3.org/2001/XMLSchema#short">6</creditsECTS>
        <csName rdf:datatype="http://www.w3.org/2001/XMLSchema#string">Syllabus of course TP40K2 Computer Networks</csName>
        <semesterinProgram rdf:datatype="http://www.w3.org/2001/XMLSchema#short">4</semesterinProgram>
    </owl:NamedIndividual>
    


    <!-- http://xworks.gr/ontologies/ccso#TP40K3/IE_BSc/IED/STEF/TEIC -->

    <owl:NamedIndividual rdf:about="http://xworks.gr/ontologies/ccso#TP40K3/IE_BSc/IED/STEF/TEIC">
        <rdf:type rdf:resource="http://xworks.gr/ontologies/ccso#Course"/>
        <affiliatedWith rdf:resource="http://xworks.gr/ontologies/ccso#Tarlis_Kostas"/>
        <coversKA rdf:resource="http://xworks.gr/ontologies/ccso#CS/PL_Programming_Languages"/>
        <hasAttender rdf:resource="http://xworks.gr/ontologies/ccso#Tarlis_Kostas"/>
        <hasSyllabus rdf:resource="http://xworks.gr/ontologies/ccso#TP40K3s1/IE_BSc/IED/STEF/TEIC"/>
        <includedIn rdf:resource="http://xworks.gr/ontologies/ccso#BSc_Informatics_Engineering/IE_BSc/IED/STEF/TEIC"/>
        <offeredBy rdf:resource="http://xworks.gr/ontologies/ccso#Department_of_Informatics_Engineering_of_TEI_of_Crete"/>
        <courseType rdf:datatype="http://www.w3.org/2001/XMLSchema#string">Core</courseType>
        <csName rdf:datatype="http://www.w3.org/2001/XMLSchema#string">Internet Programming</csName>
    </owl:NamedIndividual>
    


    <!-- http://xworks.gr/ontologies/ccso#TP40K3s1/IE_BSc/IED/STEF/TEIC -->

    <owl:NamedIndividual rdf:about="http://xworks.gr/ontologies/ccso#TP40K3s1/IE_BSc/IED/STEF/TEIC">
        <rdf:type rdf:resource="http://xworks.gr/ontologies/ccso#Syllabus"/>
        <affiliatedWith rdf:resource="http://xworks.gr/ontologies/ccso#Malamos_Athanasios"/>
        <hasInstructor rdf:resource="http://xworks.gr/ontologies/ccso#Malamos_Athanasios"/>
        <hasSupervisor rdf:resource="http://xworks.gr/ontologies/ccso#Malamos_Athanasios"/>
        <syllabusOf rdf:resource="http://xworks.gr/ontologies/ccso#TP40K3/IE_BSc/IED/STEF/TEIC"/>
        <courseType rdf:datatype="http://www.w3.org/2001/XMLSchema#string">Core</courseType>
        <creditsECTS rdf:datatype="http://www.w3.org/2001/XMLSchema#short">6</creditsECTS>
        <csName rdf:datatype="http://www.w3.org/2001/XMLSchema#string">Syllabus of course TP40K3 Internet Programming</csName>
        <semesterinProgram rdf:datatype="http://www.w3.org/2001/XMLSchema#short">4</semesterinProgram>
    </owl:NamedIndividual>
    


    <!-- http://xworks.gr/ontologies/ccso#TP40K4/IE_BSc/IED/STEF/TEIC -->

    <owl:NamedIndividual rdf:about="http://xworks.gr/ontologies/ccso#TP40K4/IE_BSc/IED/STEF/TEIC">
        <rdf:type rdf:resource="http://xworks.gr/ontologies/ccso#Course"/>
        <affiliatedWith rdf:resource="http://xworks.gr/ontologies/ccso#Tarlis_Kostas"/>
        <hasAttender rdf:resource="http://xworks.gr/ontologies/ccso#Tarlis_Kostas"/>
        <hasPrerequisite rdf:resource="http://xworks.gr/ontologies/ccso#TP10K4/IE_BSc/IED/STEF/TEIC"/>
        <hasSyllabus rdf:resource="http://xworks.gr/ontologies/ccso#TP10K4s1/IE_BSc/IED/STEF/TEIC"/>
        <includedIn rdf:resource="http://xworks.gr/ontologies/ccso#BSc_Informatics_Engineering/IE_BSc/IED/STEF/TEIC"/>
        <offeredBy rdf:resource="http://xworks.gr/ontologies/ccso#Department_of_Informatics_Engineering_of_TEI_of_Crete"/>
        <courseType rdf:datatype="http://www.w3.org/2001/XMLSchema#string">Core</courseType>
        <csName rdf:datatype="http://www.w3.org/2001/XMLSchema#string">Principles of Software Engineering</csName>
    </owl:NamedIndividual>
    


    <!-- http://xworks.gr/ontologies/ccso#TP40K4s1/IE_BSc/IED/STEF/TEIC -->

    <owl:NamedIndividual rdf:about="http://xworks.gr/ontologies/ccso#TP40K4s1/IE_BSc/IED/STEF/TEIC">
        <rdf:type rdf:resource="http://xworks.gr/ontologies/ccso#Syllabus"/>
        <affiliatedWith rdf:resource="http://xworks.gr/ontologies/ccso#Vidakis_Nikolaos"/>
        <hasInstructor rdf:resource="http://xworks.gr/ontologies/ccso#Vidakis_Nikolaos"/>
        <hasSupervisor rdf:resource="http://xworks.gr/ontologies/ccso#Vidakis_Nikolaos"/>
        <courseType rdf:datatype="http://www.w3.org/2001/XMLSchema#string">Core</courseType>
        <creditsECTS rdf:datatype="http://www.w3.org/2001/XMLSchema#short">6</creditsECTS>
        <csName rdf:datatype="http://www.w3.org/2001/XMLSchema#string">Syllabus of course TP40K4 Principles of Software Engineering</csName>
        <semesterinProgram rdf:datatype="http://www.w3.org/2001/XMLSchema#short">4</semesterinProgram>
    </owl:NamedIndividual>
    


    <!-- http://xworks.gr/ontologies/ccso#TP40K5/IE_BSc/IED/STEF/TEIC -->

    <owl:NamedIndividual rdf:about="http://xworks.gr/ontologies/ccso#TP40K5/IE_BSc/IED/STEF/TEIC">
        <rdf:type rdf:resource="http://xworks.gr/ontologies/ccso#Course"/>
        <hasPrerequisite rdf:resource="http://xworks.gr/ontologies/ccso#TP30K5/IE_BSc/IED/STEF/TEIC"/>
        <hasSyllabus rdf:resource="http://xworks.gr/ontologies/ccso#TP40K5s1/IE_BSc/IED/STEF/TEIC"/>
        <includedIn rdf:resource="http://xworks.gr/ontologies/ccso#BSc_Informatics_Engineering/IE_BSc/IED/STEF/TEIC"/>
        <offeredBy rdf:resource="http://xworks.gr/ontologies/ccso#Department_of_Informatics_Engineering_of_TEI_of_Crete"/>
        <courseType rdf:datatype="http://www.w3.org/2001/XMLSchema#string">Core</courseType>
        <csName rdf:datatype="http://www.w3.org/2001/XMLSchema#string">Linear Algebra</csName>
    </owl:NamedIndividual>
    


    <!-- http://xworks.gr/ontologies/ccso#TP40K5s1/IE_BSc/IED/STEF/TEIC -->

    <owl:NamedIndividual rdf:about="http://xworks.gr/ontologies/ccso#TP40K5s1/IE_BSc/IED/STEF/TEIC">
        <rdf:type rdf:resource="http://xworks.gr/ontologies/ccso#Syllabus"/>
        <affiliatedWith rdf:resource="http://xworks.gr/ontologies/ccso#Karagiannakis_Dimitrios"/>
        <hasInstructor rdf:resource="http://xworks.gr/ontologies/ccso#Karagiannakis_Dimitrios"/>
        <hasSupervisor rdf:resource="http://xworks.gr/ontologies/ccso#Karagiannakis_Dimitrios"/>
        <syllabusOf rdf:resource="http://xworks.gr/ontologies/ccso#TP40K5/IE_BSc/IED/STEF/TEIC"/>
        <courseType rdf:datatype="http://www.w3.org/2001/XMLSchema#string">Core</courseType>
        <creditsECTS rdf:datatype="http://www.w3.org/2001/XMLSchema#short">4</creditsECTS>
        <csName rdf:datatype="http://www.w3.org/2001/XMLSchema#string">Syllabus of course TP40K5 Linear Algebra</csName>
        <semesterinProgram rdf:datatype="http://www.w3.org/2001/XMLSchema#short">4</semesterinProgram>
    </owl:NamedIndividual>
    


    <!-- http://xworks.gr/ontologies/ccso#TP40K6/IE_BSc/IED/STEF/TEIC -->

    <owl:NamedIndividual rdf:about="http://xworks.gr/ontologies/ccso#TP40K6/IE_BSc/IED/STEF/TEIC">
        <rdf:type rdf:resource="http://xworks.gr/ontologies/ccso#Course"/>
        <affiliatedWith rdf:resource="http://xworks.gr/ontologies/ccso#Tarlis_Kostas"/>
        <hasAttender rdf:resource="http://xworks.gr/ontologies/ccso#Tarlis_Kostas"/>
        <hasSyllabus rdf:resource="http://xworks.gr/ontologies/ccso#TP40K6s1/IE_BSc/IED/STEF/TEIC"/>
        <includedIn rdf:resource="http://xworks.gr/ontologies/ccso#BSc_Informatics_Engineering/IE_BSc/IED/STEF/TEIC"/>
        <offeredBy rdf:resource="http://xworks.gr/ontologies/ccso#Department_of_Informatics_Engineering_of_TEI_of_Crete"/>
        <courseType rdf:datatype="http://www.w3.org/2001/XMLSchema#string">Core</courseType>
        <csName rdf:datatype="http://www.w3.org/2001/XMLSchema#string">Teaching Informatics</csName>
    </owl:NamedIndividual>
    


    <!-- http://xworks.gr/ontologies/ccso#TP40K6s1/IE_BSc/IED/STEF/TEIC -->

    <owl:NamedIndividual rdf:about="http://xworks.gr/ontologies/ccso#TP40K6s1/IE_BSc/IED/STEF/TEIC">
        <rdf:type rdf:resource="http://xworks.gr/ontologies/ccso#Syllabus"/>
        <affiliatedWith rdf:resource="http://xworks.gr/ontologies/ccso#Xezonakis_Ioannis"/>
        <hasInstructor rdf:resource="http://xworks.gr/ontologies/ccso#Xezonakis_Ioannis"/>
        <hasSupervisor rdf:resource="http://xworks.gr/ontologies/ccso#Xezonakis_Ioannis"/>
        <syllabusOf rdf:resource="http://xworks.gr/ontologies/ccso#TP40K6/IE_BSc/IED/STEF/TEIC"/>
        <courseType rdf:datatype="http://www.w3.org/2001/XMLSchema#string">Core</courseType>
        <creditsECTS rdf:datatype="http://www.w3.org/2001/XMLSchema#short">2</creditsECTS>
        <csName rdf:datatype="http://www.w3.org/2001/XMLSchema#string">Syllabus of course TP40K6 Teaching Informatics</csName>
        <semesterinProgram rdf:datatype="http://www.w3.org/2001/XMLSchema#short">4</semesterinProgram>
    </owl:NamedIndividual>
    


    <!-- http://xworks.gr/ontologies/ccso#TP50D2/IE_BSc/IED/STEF/TEIC -->

    <owl:NamedIndividual rdf:about="http://xworks.gr/ontologies/ccso#TP50D2/IE_BSc/IED/STEF/TEIC">
        <rdf:type rdf:resource="http://xworks.gr/ontologies/ccso#Course"/>
        <coversKA rdf:resource="http://xworks.gr/ontologies/ccso#CS/NC_Networking_and_Communication"/>
        <hasSyllabus rdf:resource="http://xworks.gr/ontologies/ccso#TP50D2s1/IE_BSc/IED/STEF/TEIC"/>
        <includedIn rdf:resource="http://xworks.gr/ontologies/ccso#BSc_Informatics_Engineering/IE_BSc/IED/STEF/TEIC"/>
        <offeredBy rdf:resource="http://xworks.gr/ontologies/ccso#Department_of_Informatics_Engineering_of_TEI_of_Crete"/>
        <courseType rdf:datatype="http://www.w3.org/2001/XMLSchema#string">Core</courseType>
        <csName rdf:datatype="http://www.w3.org/2001/XMLSchema#string">Wireless Communication Transmission
Structures</csName>
    </owl:NamedIndividual>
    


    <!-- http://xworks.gr/ontologies/ccso#TP50D2s1/IE_BSc/IED/STEF/TEIC -->

    <owl:NamedIndividual rdf:about="http://xworks.gr/ontologies/ccso#TP50D2s1/IE_BSc/IED/STEF/TEIC">
        <rdf:type rdf:resource="http://xworks.gr/ontologies/ccso#Syllabus"/>
        <affiliatedWith rdf:resource="http://xworks.gr/ontologies/ccso#Stratakis_Dimitrios"/>
        <aimsToLO rdf:resource="http://xworks.gr/ontologies/ccso#CS/NC/LAN/LO_Describe_how_frames_are_forwarded_in_an_Ethernet_network"/>
        <aimsToLO rdf:resource="http://xworks.gr/ontologies/ccso#CS/NC/LAN/LO_Describe_the_interrelations_between_IP_and_Ethernet"/>
        <aimsToLO rdf:resource="http://xworks.gr/ontologies/ccso#CS/NC/LAN/LO_Identify_the_differences_between_IP_and_Ethernet"/>
        <coversTopic rdf:resource="http://xworks.gr/ontologies/ccso#CS/NC/LAN/T_Common_approaches_to_multiple_access"/>
        <coversTopic rdf:resource="http://xworks.gr/ontologies/ccso#CS/NC/LAN/T_Multiple_Access_Problem"/>
        <hasInstructor rdf:resource="http://xworks.gr/ontologies/ccso#Stratakis_Dimitrios"/>
        <hasSupervisor rdf:resource="http://xworks.gr/ontologies/ccso#Stratakis_Dimitrios"/>
        <syllabusOf rdf:resource="http://xworks.gr/ontologies/ccso#TP50D2/IE_BSc/IED/STEF/TEIC"/>
        <courseType rdf:datatype="http://www.w3.org/2001/XMLSchema#string">Core</courseType>
        <creditsECTS rdf:datatype="http://www.w3.org/2001/XMLSchema#short">6</creditsECTS>
        <csName rdf:datatype="http://www.w3.org/2001/XMLSchema#string">Syllabus of course TP50D2 Wireless Communication Transmission
Structures</csName>
        <semesterinProgram rdf:datatype="http://www.w3.org/2001/XMLSchema#short">5</semesterinProgram>
    </owl:NamedIndividual>
    


    <!-- http://xworks.gr/ontologies/ccso#TP50D4/IE_BSc/IED/STEF/TEIC -->

    <owl:NamedIndividual rdf:about="http://xworks.gr/ontologies/ccso#TP50D4/IE_BSc/IED/STEF/TEIC">
        <rdf:type rdf:resource="http://xworks.gr/ontologies/ccso#Course"/>
        <coversKA rdf:resource="http://xworks.gr/ontologies/ccso#CS/NC_Networking_and_Communication"/>
        <hasSyllabus rdf:resource="http://xworks.gr/ontologies/ccso#TP50D4s1/IE_BSc/IED/STEF/TEIC"/>
        <includedIn rdf:resource="http://xworks.gr/ontologies/ccso#BSc_Informatics_Engineering/IE_BSc/IED/STEF/TEIC"/>
        <offeredBy rdf:resource="http://xworks.gr/ontologies/ccso#Department_of_Informatics_Engineering_of_TEI_of_Crete"/>
        <courseType rdf:datatype="http://www.w3.org/2001/XMLSchema#string">Elective</courseType>
        <csName rdf:datatype="http://www.w3.org/2001/XMLSchema#string">Satellite Communication Systems</csName>
    </owl:NamedIndividual>
    


    <!-- http://xworks.gr/ontologies/ccso#TP50D4s1/IE_BSc/IED/STEF/TEIC -->

    <owl:NamedIndividual rdf:about="http://xworks.gr/ontologies/ccso#TP50D4s1/IE_BSc/IED/STEF/TEIC">
        <rdf:type rdf:resource="http://xworks.gr/ontologies/ccso#Syllabus"/>
        <affiliatedWith rdf:resource="http://xworks.gr/ontologies/ccso#Panagiotakis_Spyros"/>
        <hasInstructor rdf:resource="http://xworks.gr/ontologies/ccso#Panagiotakis_Spyros"/>
        <hasSupervisor rdf:resource="http://xworks.gr/ontologies/ccso#Panagiotakis_Spyros"/>
        <syllabusOf rdf:resource="http://xworks.gr/ontologies/ccso#TP50D4/IE_BSc/IED/STEF/TEIC"/>
        <courseType rdf:datatype="http://www.w3.org/2001/XMLSchema#string">Elective</courseType>
        <creditsECTS rdf:datatype="http://www.w3.org/2001/XMLSchema#short">6</creditsECTS>
        <csName rdf:datatype="http://www.w3.org/2001/XMLSchema#string">Syllabus of course TP50D4 Satellite Communication Systems</csName>
        <semesterinProgram rdf:datatype="http://www.w3.org/2001/XMLSchema#short">5</semesterinProgram>
    </owl:NamedIndividual>
    


    <!-- http://xworks.gr/ontologies/ccso#TP50D5/IE_BSc/IED/STEF/TEIC -->

    <owl:NamedIndividual rdf:about="http://xworks.gr/ontologies/ccso#TP50D5/IE_BSc/IED/STEF/TEIC">
        <rdf:type rdf:resource="http://xworks.gr/ontologies/ccso#Course"/>
        <coversKA rdf:resource="http://xworks.gr/ontologies/ccso#CS/NC_Networking_and_Communication"/>
        <hasSyllabus rdf:resource="http://xworks.gr/ontologies/ccso#TP50D5s1/IE_BSc/IED/STEF/TEIC"/>
        <includedIn rdf:resource="http://xworks.gr/ontologies/ccso#BSc_Informatics_Engineering/IE_BSc/IED/STEF/TEIC"/>
        <offeredBy rdf:resource="http://xworks.gr/ontologies/ccso#Department_of_Informatics_Engineering_of_TEI_of_Crete"/>
        <courseType rdf:datatype="http://www.w3.org/2001/XMLSchema#string">Elective</courseType>
        <csName rdf:datatype="http://www.w3.org/2001/XMLSchema#string">Digital Television Principles</csName>
    </owl:NamedIndividual>
    


    <!-- http://xworks.gr/ontologies/ccso#TP50D5s1/IE_BSc/IED/STEF/TEIC -->

    <owl:NamedIndividual rdf:about="http://xworks.gr/ontologies/ccso#TP50D5s1/IE_BSc/IED/STEF/TEIC">
        <rdf:type rdf:resource="http://xworks.gr/ontologies/ccso#Syllabus"/>
        <affiliatedWith rdf:resource="http://xworks.gr/ontologies/ccso#Pallis_Evangelos"/>
        <hasInstructor rdf:resource="http://xworks.gr/ontologies/ccso#Pallis_Evangelos"/>
        <hasSupervisor rdf:resource="http://xworks.gr/ontologies/ccso#Pallis_Evangelos"/>
        <syllabusOf rdf:resource="http://xworks.gr/ontologies/ccso#TP50D5/IE_BSc/IED/STEF/TEIC"/>
        <courseType rdf:datatype="http://www.w3.org/2001/XMLSchema#string">Elective</courseType>
        <creditsECTS rdf:datatype="http://www.w3.org/2001/XMLSchema#short">6</creditsECTS>
        <csName rdf:datatype="http://www.w3.org/2001/XMLSchema#string">Syllabus of course TP50D5 Digital Television Principles</csName>
        <semesterinProgram rdf:datatype="http://www.w3.org/2001/XMLSchema#short">5</semesterinProgram>
    </owl:NamedIndividual>
    


    <!-- http://xworks.gr/ontologies/ccso#TP50D6/IE_BSc/IED/STEF/TEIC -->

    <owl:NamedIndividual rdf:about="http://xworks.gr/ontologies/ccso#TP50D6/IE_BSc/IED/STEF/TEIC">
        <rdf:type rdf:resource="http://xworks.gr/ontologies/ccso#Course"/>
        <coversKA rdf:resource="http://xworks.gr/ontologies/ccso#CS/NC_Networking_and_Communication"/>
        <hasSyllabus rdf:resource="http://xworks.gr/ontologies/ccso#TP50D6s1/IE_BSc/IED/STEF/TEIC"/>
        <includedIn rdf:resource="http://xworks.gr/ontologies/ccso#BSc_Informatics_Engineering/IE_BSc/IED/STEF/TEIC"/>
        <offeredBy rdf:resource="http://xworks.gr/ontologies/ccso#Department_of_Informatics_Engineering_of_TEI_of_Crete"/>
        <courseType rdf:datatype="http://www.w3.org/2001/XMLSchema#string">Core</courseType>
        <csName rdf:datatype="http://www.w3.org/2001/XMLSchema#string">Digital Communications</csName>
    </owl:NamedIndividual>
    


    <!-- http://xworks.gr/ontologies/ccso#TP50D6s1/IE_BSc/IED/STEF/TEIC -->

    <owl:NamedIndividual rdf:about="http://xworks.gr/ontologies/ccso#TP50D6s1/IE_BSc/IED/STEF/TEIC">
        <rdf:type rdf:resource="http://xworks.gr/ontologies/ccso#Syllabus"/>
        <affiliatedWith rdf:resource="http://xworks.gr/ontologies/ccso#Stratakis_Dimitrios"/>
        <hasInstructor rdf:resource="http://xworks.gr/ontologies/ccso#Stratakis_Dimitrios"/>
        <hasSupervisor rdf:resource="http://xworks.gr/ontologies/ccso#Stratakis_Dimitrios"/>
        <syllabusOf rdf:resource="http://xworks.gr/ontologies/ccso#TP50D6/IE_BSc/IED/STEF/TEIC"/>
        <courseType rdf:datatype="http://www.w3.org/2001/XMLSchema#string">Core</courseType>
        <creditsECTS rdf:datatype="http://www.w3.org/2001/XMLSchema#short">6</creditsECTS>
        <csName rdf:datatype="http://www.w3.org/2001/XMLSchema#string">Syllabus of course TP50D6 Digital Communications</csName>
        <semesterinProgram rdf:datatype="http://www.w3.org/2001/XMLSchema#short">5</semesterinProgram>
    </owl:NamedIndividual>
    


    <!-- http://xworks.gr/ontologies/ccso#TP50L1/IE_BSc/IED/STEF/TEIC -->

    <owl:NamedIndividual rdf:about="http://xworks.gr/ontologies/ccso#TP50L1/IE_BSc/IED/STEF/TEIC">
        <rdf:type rdf:resource="http://xworks.gr/ontologies/ccso#Course"/>
        <coversKA rdf:resource="http://xworks.gr/ontologies/ccso#CS/NC_Networking_and_Communication"/>
        <coversKA rdf:resource="http://xworks.gr/ontologies/ccso#CS/SW_Software_Engineering_Software_Systems_and_Applications"/>
        <hasSyllabus rdf:resource="http://xworks.gr/ontologies/ccso#TP50L1s1/IE_BSc/IED/STEF/TEIC"/>
        <includedIn rdf:resource="http://xworks.gr/ontologies/ccso#BSc_Informatics_Engineering/IE_BSc/IED/STEF/TEIC"/>
        <offeredBy rdf:resource="http://xworks.gr/ontologies/ccso#Department_of_Informatics_Engineering_of_TEI_of_Crete"/>
        <courseType rdf:datatype="http://www.w3.org/2001/XMLSchema#string">Elective</courseType>
        <csName rdf:datatype="http://www.w3.org/2001/XMLSchema#string">Multimedia eHealth Services</csName>
    </owl:NamedIndividual>
    


    <!-- http://xworks.gr/ontologies/ccso#TP50L1s1/IE_BSc/IED/STEF/TEIC -->

    <owl:NamedIndividual rdf:about="http://xworks.gr/ontologies/ccso#TP50L1s1/IE_BSc/IED/STEF/TEIC">
        <rdf:type rdf:resource="http://xworks.gr/ontologies/ccso#Syllabus"/>
        <affiliatedWith rdf:resource="http://xworks.gr/ontologies/ccso#Tsiknakis_Manolis"/>
        <hasInstructor rdf:resource="http://xworks.gr/ontologies/ccso#Tsiknakis_Manolis"/>
        <hasSupervisor rdf:resource="http://xworks.gr/ontologies/ccso#Tsiknakis_Manolis"/>
        <syllabusOf rdf:resource="http://xworks.gr/ontologies/ccso#TP50L1/IE_BSc/IED/STEF/TEIC"/>
        <courseType rdf:datatype="http://www.w3.org/2001/XMLSchema#string">Core</courseType>
        <creditsECTS rdf:datatype="http://www.w3.org/2001/XMLSchema#short">6</creditsECTS>
        <csName rdf:datatype="http://www.w3.org/2001/XMLSchema#string">Syllabus of course TP50L1 Multimedia eHealth Services</csName>
        <semesterinProgram rdf:datatype="http://www.w3.org/2001/XMLSchema#short">5</semesterinProgram>
    </owl:NamedIndividual>
    


    <!-- http://xworks.gr/ontologies/ccso#TP50L2/IE_BSc/IED/STEF/TEIC -->

    <owl:NamedIndividual rdf:about="http://xworks.gr/ontologies/ccso#TP50L2/IE_BSc/IED/STEF/TEIC">
        <rdf:type rdf:resource="http://xworks.gr/ontologies/ccso#Course"/>
        <coversKA rdf:resource="http://xworks.gr/ontologies/ccso#CS/SW_Software_Engineering_Software_Systems_and_Applications"/>
        <hasPrerequisite rdf:resource="http://xworks.gr/ontologies/ccso#TP10K4/IE_BSc/IED/STEF/TEIC"/>
        <hasSyllabus rdf:resource="http://xworks.gr/ontologies/ccso#TP50L2s1/IE_BSc/IED/STEF/TEIC"/>
        <includedIn rdf:resource="http://xworks.gr/ontologies/ccso#BSc_Informatics_Engineering/IE_BSc/IED/STEF/TEIC"/>
        <offeredBy rdf:resource="http://xworks.gr/ontologies/ccso#Department_of_Informatics_Engineering_of_TEI_of_Crete"/>
        <courseType rdf:datatype="http://www.w3.org/2001/XMLSchema#string">Core</courseType>
        <csName rdf:datatype="http://www.w3.org/2001/XMLSchema#string">Plan-Driven and Agile Programming</csName>
    </owl:NamedIndividual>
    


    <!-- http://xworks.gr/ontologies/ccso#TP50L2s1/IE_BSc/IED/STEF/TEIC -->

    <owl:NamedIndividual rdf:about="http://xworks.gr/ontologies/ccso#TP50L2s1/IE_BSc/IED/STEF/TEIC">
        <rdf:type rdf:resource="http://xworks.gr/ontologies/ccso#Syllabus"/>
        <affiliatedWith rdf:resource="http://xworks.gr/ontologies/ccso#Vidakis_Nikolaos"/>
        <hasInstructor rdf:resource="http://xworks.gr/ontologies/ccso#Vidakis_Nikolaos"/>
        <hasSupervisor rdf:resource="http://xworks.gr/ontologies/ccso#Vidakis_Nikolaos"/>
        <syllabusOf rdf:resource="http://xworks.gr/ontologies/ccso#TP50L2/IE_BSc/IED/STEF/TEIC"/>
        <courseType rdf:datatype="http://www.w3.org/2001/XMLSchema#string">Core</courseType>
        <creditsECTS rdf:datatype="http://www.w3.org/2001/XMLSchema#short">6</creditsECTS>
        <csName rdf:datatype="http://www.w3.org/2001/XMLSchema#string">Syllabus of course TP50L2 Plan-Driven and Agile Programming</csName>
        <semesterinProgram rdf:datatype="http://www.w3.org/2001/XMLSchema#short">5</semesterinProgram>
    </owl:NamedIndividual>
    


    <!-- http://xworks.gr/ontologies/ccso#TP50L3/IE_BSc/IED/STEF/TEIC -->

    <owl:NamedIndividual rdf:about="http://xworks.gr/ontologies/ccso#TP50L3/IE_BSc/IED/STEF/TEIC">
        <rdf:type rdf:resource="http://xworks.gr/ontologies/ccso#Course"/>
        <coversKA rdf:resource="http://xworks.gr/ontologies/ccso#CS/SW_Software_Engineering_Software_Systems_and_Applications"/>
        <hasSyllabus rdf:resource="http://xworks.gr/ontologies/ccso#TP50L3s1/IE_BSc/IED/STEF/TEIC"/>
        <includedIn rdf:resource="http://xworks.gr/ontologies/ccso#BSc_Informatics_Engineering/IE_BSc/IED/STEF/TEIC"/>
        <offeredBy rdf:resource="http://xworks.gr/ontologies/ccso#Department_of_Informatics_Engineering_of_TEI_of_Crete"/>
        <courseType rdf:datatype="http://www.w3.org/2001/XMLSchema#string">Core</courseType>
        <csName rdf:datatype="http://www.w3.org/2001/XMLSchema#string">Logic Programming</csName>
    </owl:NamedIndividual>
    


    <!-- http://xworks.gr/ontologies/ccso#TP50L3s1/IE_BSc/IED/STEF/TEIC -->

    <owl:NamedIndividual rdf:about="http://xworks.gr/ontologies/ccso#TP50L3s1/IE_BSc/IED/STEF/TEIC">
        <rdf:type rdf:resource="http://xworks.gr/ontologies/ccso#Syllabus"/>
        <affiliatedWith rdf:resource="http://xworks.gr/ontologies/ccso#Marakakis_Manolis"/>
        <coversTopic rdf:resource="http://xworks.gr/ontologies/ccso#CS/PL/T_Object-Oriented_Design,_Decomposition_into_objects_carrying_state_and_having_behavior"/>
        <coversTopic rdf:resource="http://xworks.gr/ontologies/ccso#CS/PL/T_Subclasses,Inheritance,and_Method_Overriding"/>
        <hasInstructor rdf:resource="http://xworks.gr/ontologies/ccso#Marakakis_Manolis"/>
        <hasSupervisor rdf:resource="http://xworks.gr/ontologies/ccso#Marakakis_Manolis"/>
        <syllabusOf rdf:resource="http://xworks.gr/ontologies/ccso#TP50L3/IE_BSc/IED/STEF/TEIC"/>
        <courseType rdf:datatype="http://www.w3.org/2001/XMLSchema#string">Core</courseType>
        <creditsECTS rdf:datatype="http://www.w3.org/2001/XMLSchema#short">6</creditsECTS>
        <csName rdf:datatype="http://www.w3.org/2001/XMLSchema#string">Syllabus of course TP50L3 Logic Programming</csName>
        <semesterinProgram rdf:datatype="http://www.w3.org/2001/XMLSchema#short">5</semesterinProgram>
    </owl:NamedIndividual>
    


    <!-- http://xworks.gr/ontologies/ccso#TP50L4/IE_BSc/IED/STEF/TEIC -->

    <owl:NamedIndividual rdf:about="http://xworks.gr/ontologies/ccso#TP50L4/IE_BSc/IED/STEF/TEIC">
        <rdf:type rdf:resource="http://xworks.gr/ontologies/ccso#Course"/>
        <coversKA rdf:resource="http://xworks.gr/ontologies/ccso#CS/SW_Software_Engineering_Software_Systems_and_Applications"/>
        <hasSyllabus rdf:resource="http://xworks.gr/ontologies/ccso#TP50L4s1/IE_BSc/IED/STEF/TEIC"/>
        <includedIn rdf:resource="http://xworks.gr/ontologies/ccso#BSc_Informatics_Engineering/IE_BSc/IED/STEF/TEIC"/>
        <offeredBy rdf:resource="http://xworks.gr/ontologies/ccso#Department_of_Informatics_Engineering_of_TEI_of_Crete"/>
        <courseType rdf:datatype="http://www.w3.org/2001/XMLSchema#string">Elective</courseType>
        <csName rdf:datatype="http://www.w3.org/2001/XMLSchema#string">Data/Information Visualization</csName>
    </owl:NamedIndividual>
    


    <!-- http://xworks.gr/ontologies/ccso#TP50L4s1/IE_BSc/IED/STEF/TEIC -->

    <owl:NamedIndividual rdf:about="http://xworks.gr/ontologies/ccso#TP50L4s1/IE_BSc/IED/STEF/TEIC">
        <rdf:type rdf:resource="http://xworks.gr/ontologies/ccso#Syllabus"/>
        <affiliatedWith rdf:resource="http://xworks.gr/ontologies/ccso#Aivalis_Costas"/>
        <hasInstructor rdf:resource="http://xworks.gr/ontologies/ccso#Aivalis_Costas"/>
        <hasSupervisor rdf:resource="http://xworks.gr/ontologies/ccso#Aivalis_Costas"/>
        <syllabusOf rdf:resource="http://xworks.gr/ontologies/ccso#TP50L4/IE_BSc/IED/STEF/TEIC"/>
        <courseType rdf:datatype="http://www.w3.org/2001/XMLSchema#string">Elective</courseType>
        <creditsECTS rdf:datatype="http://www.w3.org/2001/XMLSchema#short">6</creditsECTS>
        <csName rdf:datatype="http://www.w3.org/2001/XMLSchema#string">Syllabus of course TP50L4 Data/Information Visualization</csName>
        <semesterinProgram rdf:datatype="http://www.w3.org/2001/XMLSchema#short">5</semesterinProgram>
    </owl:NamedIndividual>
    


    <!-- http://xworks.gr/ontologies/ccso#TP50L5/IE_BSc/IED/STEF/TEIC -->

    <owl:NamedIndividual rdf:about="http://xworks.gr/ontologies/ccso#TP50L5/IE_BSc/IED/STEF/TEIC">
        <rdf:type rdf:resource="http://xworks.gr/ontologies/ccso#Course"/>
        <coversKA rdf:resource="http://xworks.gr/ontologies/ccso#CS/SW_Software_Engineering_Software_Systems_and_Applications"/>
        <hasSyllabus rdf:resource="http://xworks.gr/ontologies/ccso#TP50L5s1/IE_BSc/IED/STEF/TEIC"/>
        <includedIn rdf:resource="http://xworks.gr/ontologies/ccso#BSc_Informatics_Engineering/IE_BSc/IED/STEF/TEIC"/>
        <offeredBy rdf:resource="http://xworks.gr/ontologies/ccso#Department_of_Informatics_Engineering_of_TEI_of_Crete"/>
        <courseType rdf:datatype="http://www.w3.org/2001/XMLSchema#string">Elective</courseType>
        <csName rdf:datatype="http://www.w3.org/2001/XMLSchema#string">Programming Languages</csName>
    </owl:NamedIndividual>
    


    <!-- http://xworks.gr/ontologies/ccso#TP50L5s1/IE_BSc/IED/STEF/TEIC -->

    <owl:NamedIndividual rdf:about="http://xworks.gr/ontologies/ccso#TP50L5s1/IE_BSc/IED/STEF/TEIC">
        <rdf:type rdf:resource="http://xworks.gr/ontologies/ccso#Syllabus"/>
        <affiliatedWith rdf:resource="http://xworks.gr/ontologies/ccso#Papadakis_Nikos"/>
        <coversTopic rdf:resource="http://xworks.gr/ontologies/ccso#CS/PL/T_Definition_of_classes:fields,methods,and_constructors"/>
        <coversTopic rdf:resource="http://xworks.gr/ontologies/ccso#CS/PL/T_Dynamic_dispatch:Definition_of_Method-Call"/>
        <coversTopic rdf:resource="http://xworks.gr/ontologies/ccso#CS/PL/T_Object-Oriented_Design,Class-Hierarchy_design_for_modeling"/>
        <coversTopic rdf:resource="http://xworks.gr/ontologies/ccso#CS/PL/T_Object-Oriented_Design,_Decomposition_into_objects_carrying_state_and_having_behavior"/>
        <coversTopic rdf:resource="http://xworks.gr/ontologies/ccso#CS/PL/T_Subclasses,Inheritance,and_Method_Overriding"/>
        <hasInstructor rdf:resource="http://xworks.gr/ontologies/ccso#Papadakis_Nikos"/>
        <hasSupervisor rdf:resource="http://xworks.gr/ontologies/ccso#Papadakis_Nikos"/>
        <syllabusOf rdf:resource="http://xworks.gr/ontologies/ccso#TP50L5/IE_BSc/IED/STEF/TEIC"/>
        <courseType rdf:datatype="http://www.w3.org/2001/XMLSchema#string">Elective</courseType>
        <creditsECTS rdf:datatype="http://www.w3.org/2001/XMLSchema#short">6</creditsECTS>
        <csName rdf:datatype="http://www.w3.org/2001/XMLSchema#string">Syllabus of course TP50L5 Programming Languages</csName>
        <semesterinProgram rdf:datatype="http://www.w3.org/2001/XMLSchema#short">5</semesterinProgram>
    </owl:NamedIndividual>
    


    <!-- http://xworks.gr/ontologies/ccso#TP50Y1/IE_BSc/IED/STEF/TEIC -->

    <owl:NamedIndividual rdf:about="http://xworks.gr/ontologies/ccso#TP50Y1/IE_BSc/IED/STEF/TEIC">
        <rdf:type rdf:resource="http://xworks.gr/ontologies/ccso#Course"/>
        <coversKA rdf:resource="http://xworks.gr/ontologies/ccso#CS/HW_Hardware_and_Computer_Systems"/>
        <hasSyllabus rdf:resource="http://xworks.gr/ontologies/ccso#TP50Y1s1/IE_BSc/IED/STEF/TEIC"/>
        <includedIn rdf:resource="http://xworks.gr/ontologies/ccso#BSc_Informatics_Engineering/IE_BSc/IED/STEF/TEIC"/>
        <offeredBy rdf:resource="http://xworks.gr/ontologies/ccso#Department_of_Informatics_Engineering_of_TEI_of_Crete"/>
        <courseType rdf:datatype="http://www.w3.org/2001/XMLSchema#string">Core</courseType>
        <csName rdf:datatype="http://www.w3.org/2001/XMLSchema#string">Graphics</csName>
    </owl:NamedIndividual>
    


    <!-- http://xworks.gr/ontologies/ccso#TP50Y1s1/IE_BSc/IED/STEF/TEIC -->

    <owl:NamedIndividual rdf:about="http://xworks.gr/ontologies/ccso#TP50Y1s1/IE_BSc/IED/STEF/TEIC">
        <rdf:type rdf:resource="http://xworks.gr/ontologies/ccso#Syllabus"/>
        <affiliatedWith rdf:resource="http://xworks.gr/ontologies/ccso#Malamos_Athanasios"/>
        <hasInstructor rdf:resource="http://xworks.gr/ontologies/ccso#Malamos_Athanasios"/>
        <hasSupervisor rdf:resource="http://xworks.gr/ontologies/ccso#Malamos_Athanasios"/>
        <syllabusOf rdf:resource="http://xworks.gr/ontologies/ccso#TP50Y1/IE_BSc/IED/STEF/TEIC"/>
        <courseType rdf:datatype="http://www.w3.org/2001/XMLSchema#string">Core</courseType>
        <creditsECTS rdf:datatype="http://www.w3.org/2001/XMLSchema#short">6</creditsECTS>
        <csName rdf:datatype="http://www.w3.org/2001/XMLSchema#string">Syllabus of course TP50Y1 Graphics</csName>
        <semesterinProgram rdf:datatype="http://www.w3.org/2001/XMLSchema#short">5</semesterinProgram>
    </owl:NamedIndividual>
    


    <!-- http://xworks.gr/ontologies/ccso#TP50Y2/IE_BSc/IED/STEF/TEIC -->

    <owl:NamedIndividual rdf:about="http://xworks.gr/ontologies/ccso#TP50Y2/IE_BSc/IED/STEF/TEIC">
        <rdf:type rdf:resource="http://xworks.gr/ontologies/ccso#Course"/>
        <coversKA rdf:resource="http://xworks.gr/ontologies/ccso#CS/HW_Hardware_and_Computer_Systems"/>
        <hasSyllabus rdf:resource="http://xworks.gr/ontologies/ccso#TP50Y2s1/IE_BSc/IED/STEF/TEIC"/>
        <includedIn rdf:resource="http://xworks.gr/ontologies/ccso#BSc_Informatics_Engineering/IE_BSc/IED/STEF/TEIC"/>
        <offeredBy rdf:resource="http://xworks.gr/ontologies/ccso#Department_of_Informatics_Engineering_of_TEI_of_Crete"/>
        <courseType rdf:datatype="http://www.w3.org/2001/XMLSchema#string">Core</courseType>
        <csName rdf:datatype="http://www.w3.org/2001/XMLSchema#string">Digital Image Processing</csName>
    </owl:NamedIndividual>
    


    <!-- http://xworks.gr/ontologies/ccso#TP50Y2s1/IE_BSc/IED/STEF/TEIC -->

    <owl:NamedIndividual rdf:about="http://xworks.gr/ontologies/ccso#TP50Y2s1/IE_BSc/IED/STEF/TEIC">
        <rdf:type rdf:resource="http://xworks.gr/ontologies/ccso#Syllabus"/>
        <affiliatedWith rdf:resource="http://xworks.gr/ontologies/ccso#Marias_Kostas"/>
        <hasInstructor rdf:resource="http://xworks.gr/ontologies/ccso#Marias_Kostas"/>
        <hasSupervisor rdf:resource="http://xworks.gr/ontologies/ccso#Marias_Kostas"/>
        <syllabusOf rdf:resource="http://xworks.gr/ontologies/ccso#TP50Y2/IE_BSc/IED/STEF/TEIC"/>
        <courseType rdf:datatype="http://www.w3.org/2001/XMLSchema#string">Core</courseType>
        <creditsECTS rdf:datatype="http://www.w3.org/2001/XMLSchema#short">6</creditsECTS>
        <csName rdf:datatype="http://www.w3.org/2001/XMLSchema#string">Syllabus of course TP50Y2 Digital Image Processing</csName>
        <semesterinProgram rdf:datatype="http://www.w3.org/2001/XMLSchema#short">5</semesterinProgram>
    </owl:NamedIndividual>
    


    <!-- http://xworks.gr/ontologies/ccso#TP50Y3/IE_BSc/IED/STEF/TEIC -->

    <owl:NamedIndividual rdf:about="http://xworks.gr/ontologies/ccso#TP50Y3/IE_BSc/IED/STEF/TEIC">
        <rdf:type rdf:resource="http://xworks.gr/ontologies/ccso#Course"/>
        <coversKA rdf:resource="http://xworks.gr/ontologies/ccso#CS/HW_Hardware_and_Computer_Systems"/>
        <hasSyllabus rdf:resource="http://xworks.gr/ontologies/ccso#TP50Y3s1/IE_BSc/IED/STEF/TEIC"/>
        <includedIn rdf:resource="http://xworks.gr/ontologies/ccso#BSc_Informatics_Engineering/IE_BSc/IED/STEF/TEIC"/>
        <offeredBy rdf:resource="http://xworks.gr/ontologies/ccso#Department_of_Informatics_Engineering_of_TEI_of_Crete"/>
        <courseType rdf:datatype="http://www.w3.org/2001/XMLSchema#string">Core</courseType>
        <csName rdf:datatype="http://www.w3.org/2001/XMLSchema#string">Pattern Recognition</csName>
    </owl:NamedIndividual>
    


    <!-- http://xworks.gr/ontologies/ccso#TP50Y3s1/IE_BSc/IED/STEF/TEIC -->

    <owl:NamedIndividual rdf:about="http://xworks.gr/ontologies/ccso#TP50Y3s1/IE_BSc/IED/STEF/TEIC">
        <rdf:type rdf:resource="http://xworks.gr/ontologies/ccso#Syllabus"/>
        <affiliatedWith rdf:resource="http://xworks.gr/ontologies/ccso#Papadourakis_George"/>
        <hasInstructor rdf:resource="http://xworks.gr/ontologies/ccso#Papadourakis_George"/>
        <hasSupervisor rdf:resource="http://xworks.gr/ontologies/ccso#Papadourakis_George"/>
        <syllabusOf rdf:resource="http://xworks.gr/ontologies/ccso#TP50Y3/IE_BSc/IED/STEF/TEIC"/>
        <courseType rdf:datatype="http://www.w3.org/2001/XMLSchema#string">Core</courseType>
        <creditsECTS rdf:datatype="http://www.w3.org/2001/XMLSchema#short">6</creditsECTS>
        <csName rdf:datatype="http://www.w3.org/2001/XMLSchema#string">Syllabus of course TP50Y3 Pattern Recognition</csName>
        <semesterinProgram rdf:datatype="http://www.w3.org/2001/XMLSchema#short">5</semesterinProgram>
    </owl:NamedIndividual>
    


    <!-- http://xworks.gr/ontologies/ccso#TP50Y4/IE_BSc/IED/STEF/TEIC -->

    <owl:NamedIndividual rdf:about="http://xworks.gr/ontologies/ccso#TP50Y4/IE_BSc/IED/STEF/TEIC">
        <rdf:type rdf:resource="http://xworks.gr/ontologies/ccso#Course"/>
        <coversKA rdf:resource="http://xworks.gr/ontologies/ccso#CS/HW_Hardware_and_Computer_Systems"/>
        <hasSyllabus rdf:resource="http://xworks.gr/ontologies/ccso#TP50Y4s1/IE_BSc/IED/STEF/TEIC"/>
        <includedIn rdf:resource="http://xworks.gr/ontologies/ccso#BSc_Informatics_Engineering/IE_BSc/IED/STEF/TEIC"/>
        <offeredBy rdf:resource="http://xworks.gr/ontologies/ccso#Department_of_Informatics_Engineering_of_TEI_of_Crete"/>
        <courseType rdf:datatype="http://www.w3.org/2001/XMLSchema#string">Elective</courseType>
        <csName rdf:datatype="http://www.w3.org/2001/XMLSchema#string">Introduction to Robotics</csName>
    </owl:NamedIndividual>
    


    <!-- http://xworks.gr/ontologies/ccso#TP50Y4s1/IE_BSc/IED/STEF/TEIC -->

    <owl:NamedIndividual rdf:about="http://xworks.gr/ontologies/ccso#TP50Y4s1/IE_BSc/IED/STEF/TEIC">
        <rdf:type rdf:resource="http://xworks.gr/ontologies/ccso#Syllabus"/>
        <affiliatedWith rdf:resource="http://xworks.gr/ontologies/ccso#Papadourakis_George"/>
        <hasInstructor rdf:resource="http://xworks.gr/ontologies/ccso#Papadourakis_George"/>
        <hasSupervisor rdf:resource="http://xworks.gr/ontologies/ccso#Papadourakis_George"/>
        <syllabusOf rdf:resource="http://xworks.gr/ontologies/ccso#TP50Y4/IE_BSc/IED/STEF/TEIC"/>
        <courseType rdf:datatype="http://www.w3.org/2001/XMLSchema#string">Elective</courseType>
        <creditsECTS rdf:datatype="http://www.w3.org/2001/XMLSchema#short">6</creditsECTS>
        <csName rdf:datatype="http://www.w3.org/2001/XMLSchema#string">Syllabus of course TP50Y4 Introduction to Robotics</csName>
        <semesterinProgram rdf:datatype="http://www.w3.org/2001/XMLSchema#short">5</semesterinProgram>
    </owl:NamedIndividual>
    


    <!-- http://xworks.gr/ontologies/ccso#TP50Y5/IE_BSc/IED/STEF/TEIC -->

    <owl:NamedIndividual rdf:about="http://xworks.gr/ontologies/ccso#TP50Y5/IE_BSc/IED/STEF/TEIC">
        <rdf:type rdf:resource="http://xworks.gr/ontologies/ccso#Course"/>
        <coversKA rdf:resource="http://xworks.gr/ontologies/ccso#CS/HW_Hardware_and_Computer_Systems"/>
        <hasSyllabus rdf:resource="http://xworks.gr/ontologies/ccso#TP50Y5s1/IE_BSc/IED/STEF/TEIC"/>
        <includedIn rdf:resource="http://xworks.gr/ontologies/ccso#BSc_Informatics_Engineering/IE_BSc/IED/STEF/TEIC"/>
        <offeredBy rdf:resource="http://xworks.gr/ontologies/ccso#Department_of_Informatics_Engineering_of_TEI_of_Crete"/>
        <courseType rdf:datatype="http://www.w3.org/2001/XMLSchema#string">Elective</courseType>
        <csName rdf:datatype="http://www.w3.org/2001/XMLSchema#string">Machine Learning and Data Mining</csName>
    </owl:NamedIndividual>
    


    <!-- http://xworks.gr/ontologies/ccso#TP50Y5s1/IE_BSc/IED/STEF/TEIC -->

    <owl:NamedIndividual rdf:about="http://xworks.gr/ontologies/ccso#TP50Y5s1/IE_BSc/IED/STEF/TEIC">
        <rdf:type rdf:resource="http://xworks.gr/ontologies/ccso#Syllabus"/>
        <affiliatedWith rdf:resource="http://xworks.gr/ontologies/ccso#Papadakis_Nikos"/>
        <hasInstructor rdf:resource="http://xworks.gr/ontologies/ccso#Papadakis_Nikos"/>
        <hasSupervisor rdf:resource="http://xworks.gr/ontologies/ccso#Papadakis_Nikos"/>
        <syllabusOf rdf:resource="http://xworks.gr/ontologies/ccso#TP50Y5/IE_BSc/IED/STEF/TEIC"/>
        <courseType rdf:datatype="http://www.w3.org/2001/XMLSchema#string">Elective</courseType>
        <creditsECTS rdf:datatype="http://www.w3.org/2001/XMLSchema#short">6</creditsECTS>
        <csName rdf:datatype="http://www.w3.org/2001/XMLSchema#string">Syllabus of course TP50Y5 Machine Learning and Data Mining</csName>
        <semesterinProgram rdf:datatype="http://www.w3.org/2001/XMLSchema#short">5</semesterinProgram>
    </owl:NamedIndividual>
    


    <!-- http://xworks.gr/ontologies/ccso#TP60D1/IE_BSc/IED/STEF/TEIC -->

    <owl:NamedIndividual rdf:about="http://xworks.gr/ontologies/ccso#TP60D1/IE_BSc/IED/STEF/TEIC">
        <rdf:type rdf:resource="http://xworks.gr/ontologies/ccso#Course"/>
        <coversKA rdf:resource="http://xworks.gr/ontologies/ccso#CS/NC_Networking_and_Communication"/>
        <hasPrerequisite rdf:resource="http://xworks.gr/ontologies/ccso#TP40K2/IE_BSc/IED/STEF/TEIC"/>
        <hasSyllabus rdf:resource="http://xworks.gr/ontologies/ccso#TP60D1s1/IE_BSc/IED/STEF/TEIC"/>
        <includedIn rdf:resource="http://xworks.gr/ontologies/ccso#BSc_Informatics_Engineering/IE_BSc/IED/STEF/TEIC"/>
        <offeredBy rdf:resource="http://xworks.gr/ontologies/ccso#Department_of_Informatics_Engineering_of_TEI_of_Crete"/>
        <code rdf:datatype="http://www.w3.org/2001/XMLSchema#string">TP60D1/IE_BSc/IED/STEF/TEIC</code>
        <courseType rdf:datatype="http://www.w3.org/2001/XMLSchema#string">Core</courseType>
        <csName rdf:datatype="http://www.w3.org/2001/XMLSchema#string">Computer Networks II</csName>
    </owl:NamedIndividual>
    


    <!-- http://xworks.gr/ontologies/ccso#TP60D1s1/IE_BSc/IED/STEF/TEIC -->

    <owl:NamedIndividual rdf:about="http://xworks.gr/ontologies/ccso#TP60D1s1/IE_BSc/IED/STEF/TEIC">
        <rdf:type rdf:resource="http://xworks.gr/ontologies/ccso#Syllabus"/>
        <affiliatedWith rdf:resource="http://xworks.gr/ontologies/ccso#Fragopoulou_Paraskevi"/>
        <hasInstructor rdf:resource="http://xworks.gr/ontologies/ccso#Fragopoulou_Paraskevi"/>
        <hasSupervisor rdf:resource="http://xworks.gr/ontologies/ccso#Fragopoulou_Paraskevi"/>
        <syllabusOf rdf:resource="http://xworks.gr/ontologies/ccso#TP60D1/IE_BSc/IED/STEF/TEIC"/>
        <courseType rdf:datatype="http://www.w3.org/2001/XMLSchema#string">Core</courseType>
        <creditsECTS rdf:datatype="http://www.w3.org/2001/XMLSchema#short">6</creditsECTS>
        <csName rdf:datatype="http://www.w3.org/2001/XMLSchema#string">Syllabus of course TP60D1 Computer Networks II</csName>
        <semesterinProgram rdf:datatype="http://www.w3.org/2001/XMLSchema#short">6</semesterinProgram>
    </owl:NamedIndividual>
    


    <!-- http://xworks.gr/ontologies/ccso#TP60D2/IE_BSc/IED/STEF/TEIC -->

    <owl:NamedIndividual rdf:about="http://xworks.gr/ontologies/ccso#TP60D2/IE_BSc/IED/STEF/TEIC">
        <rdf:type rdf:resource="http://xworks.gr/ontologies/ccso#Course"/>
        <coversKA rdf:resource="http://xworks.gr/ontologies/ccso#CS/NC_Networking_and_Communication"/>
        <hasSyllabus rdf:resource="http://xworks.gr/ontologies/ccso#TP60D2s1/IE_BSc/IED/STEF/TEIC"/>
        <includedIn rdf:resource="http://xworks.gr/ontologies/ccso#BSc_Informatics_Engineering/IE_BSc/IED/STEF/TEIC"/>
        <offeredBy rdf:resource="http://xworks.gr/ontologies/ccso#Department_of_Informatics_Engineering_of_TEI_of_Crete"/>
        <courseType rdf:datatype="http://www.w3.org/2001/XMLSchema#string">Core</courseType>
        <csName rdf:datatype="http://www.w3.org/2001/XMLSchema#string">Wireless Networks</csName>
    </owl:NamedIndividual>
    


    <!-- http://xworks.gr/ontologies/ccso#TP60D2s1/IE_BSc/IED/STEF/TEIC -->

    <owl:NamedIndividual rdf:about="http://xworks.gr/ontologies/ccso#TP60D2s1/IE_BSc/IED/STEF/TEIC">
        <rdf:type rdf:resource="http://xworks.gr/ontologies/ccso#Syllabus"/>
        <affiliatedWith rdf:resource="http://xworks.gr/ontologies/ccso#Pallis_Evangelos"/>
        <hasInstructor rdf:resource="http://xworks.gr/ontologies/ccso#Pallis_Evangelos"/>
        <hasSupervisor rdf:resource="http://xworks.gr/ontologies/ccso#Pallis_Evangelos"/>
        <syllabusOf rdf:resource="http://xworks.gr/ontologies/ccso#TP60D2/IE_BSc/IED/STEF/TEIC"/>
        <courseType rdf:datatype="http://www.w3.org/2001/XMLSchema#string">Core</courseType>
        <creditsECTS rdf:datatype="http://www.w3.org/2001/XMLSchema#short">6</creditsECTS>
        <csName rdf:datatype="http://www.w3.org/2001/XMLSchema#string">Syllabus of course TP60D2 Wireless Networks</csName>
        <semesterinProgram rdf:datatype="http://www.w3.org/2001/XMLSchema#short">6</semesterinProgram>
    </owl:NamedIndividual>
    


    <!-- http://xworks.gr/ontologies/ccso#TP60D3/IE_BSc/IED/STEF/TEIC -->

    <owl:NamedIndividual rdf:about="http://xworks.gr/ontologies/ccso#TP60D3/IE_BSc/IED/STEF/TEIC">
        <rdf:type rdf:resource="http://xworks.gr/ontologies/ccso#Course"/>
        <coversKA rdf:resource="http://xworks.gr/ontologies/ccso#CS/NC_Networking_and_Communication"/>
        <hasPrerequisite rdf:resource="http://xworks.gr/ontologies/ccso#TP40K3/IE_BSc/IED/STEF/TEIC"/>
        <hasSyllabus rdf:resource="http://xworks.gr/ontologies/ccso#TP60D3s1/IE_BSc/IED/STEF/TEIC"/>
        <includedIn rdf:resource="http://xworks.gr/ontologies/ccso#BSc_Informatics_Engineering/IE_BSc/IED/STEF/TEIC"/>
        <offeredBy rdf:resource="http://xworks.gr/ontologies/ccso#Department_of_Informatics_Engineering_of_TEI_of_Crete"/>
        <courseType rdf:datatype="http://www.w3.org/2001/XMLSchema#string">Core</courseType>
        <csName rdf:datatype="http://www.w3.org/2001/XMLSchema#string">Multimedia Application Development</csName>
    </owl:NamedIndividual>
    


    <!-- http://xworks.gr/ontologies/ccso#TP60D3s1/IE_BSc/IED/STEF/TEIC -->

    <owl:NamedIndividual rdf:about="http://xworks.gr/ontologies/ccso#TP60D3s1/IE_BSc/IED/STEF/TEIC">
        <rdf:type rdf:resource="http://xworks.gr/ontologies/ccso#Syllabus"/>
        <affiliatedWith rdf:resource="http://xworks.gr/ontologies/ccso#Malamos_Athanasios"/>
        <hasInstructor rdf:resource="http://xworks.gr/ontologies/ccso#Malamos_Athanasios"/>
        <hasSupervisor rdf:resource="http://xworks.gr/ontologies/ccso#Malamos_Athanasios"/>
        <syllabusOf rdf:resource="http://xworks.gr/ontologies/ccso#TP60D3/IE_BSc/IED/STEF/TEIC"/>
        <courseType rdf:datatype="http://www.w3.org/2001/XMLSchema#string">Core</courseType>
        <creditsECTS rdf:datatype="http://www.w3.org/2001/XMLSchema#short">6</creditsECTS>
        <csName rdf:datatype="http://www.w3.org/2001/XMLSchema#string">Syllabus of course TP60D3 Multimedia Application Development</csName>
        <semesterinProgram rdf:datatype="http://www.w3.org/2001/XMLSchema#short">6</semesterinProgram>
    </owl:NamedIndividual>
    


    <!-- http://xworks.gr/ontologies/ccso#TP60D4/IE_BSc/IED/STEF/TEIC -->

    <owl:NamedIndividual rdf:about="http://xworks.gr/ontologies/ccso#TP60D4/IE_BSc/IED/STEF/TEIC">
        <rdf:type rdf:resource="http://xworks.gr/ontologies/ccso#Course"/>
        <coversKA rdf:resource="http://xworks.gr/ontologies/ccso#CS/HW_Hardware_and_Computer_Systems"/>
        <coversKA rdf:resource="http://xworks.gr/ontologies/ccso#CS/NC_Networking_and_Communication"/>
        <hasSyllabus rdf:resource="http://xworks.gr/ontologies/ccso#TP60D4s1/IE_BSc/IED/STEF/TEIC"/>
        <includedIn rdf:resource="http://xworks.gr/ontologies/ccso#BSc_Informatics_Engineering/IE_BSc/IED/STEF/TEIC"/>
        <offeredBy rdf:resource="http://xworks.gr/ontologies/ccso#Department_of_Informatics_Engineering_of_TEI_of_Crete"/>
        <courseType rdf:datatype="http://www.w3.org/2001/XMLSchema#string">Elective</courseType>
        <csName rdf:datatype="http://www.w3.org/2001/XMLSchema#string">Game Technologies</csName>
    </owl:NamedIndividual>
    


    <!-- http://xworks.gr/ontologies/ccso#TP60D4s1/IE_BSc/IED/STEF/TEIC -->

    <owl:NamedIndividual rdf:about="http://xworks.gr/ontologies/ccso#TP60D4s1/IE_BSc/IED/STEF/TEIC">
        <rdf:type rdf:resource="http://xworks.gr/ontologies/ccso#Syllabus"/>
        <affiliatedWith rdf:resource="http://xworks.gr/ontologies/ccso#Pachoulakis_Ioannis"/>
        <hasInstructor rdf:resource="http://xworks.gr/ontologies/ccso#Pachoulakis_Ioannis"/>
        <hasSupervisor rdf:resource="http://xworks.gr/ontologies/ccso#Pachoulakis_Ioannis"/>
        <syllabusOf rdf:resource="http://xworks.gr/ontologies/ccso#TP60D4/IE_BSc/IED/STEF/TEIC"/>
        <courseType rdf:datatype="http://www.w3.org/2001/XMLSchema#string">Elective</courseType>
        <creditsECTS rdf:datatype="http://www.w3.org/2001/XMLSchema#short">6</creditsECTS>
        <csName rdf:datatype="http://www.w3.org/2001/XMLSchema#string">Syllabus of course TP60D4 Game Technologies</csName>
        <semesterinProgram rdf:datatype="http://www.w3.org/2001/XMLSchema#short">6</semesterinProgram>
    </owl:NamedIndividual>
    


    <!-- http://xworks.gr/ontologies/ccso#TP60D5/IE_BSc/IED/STEF/TEIC -->

    <owl:NamedIndividual rdf:about="http://xworks.gr/ontologies/ccso#TP60D5/IE_BSc/IED/STEF/TEIC">
        <rdf:type rdf:resource="http://xworks.gr/ontologies/ccso#Course"/>
        <coversKA rdf:resource="http://xworks.gr/ontologies/ccso#CS/HW_Hardware_and_Computer_Systems"/>
        <coversKA rdf:resource="http://xworks.gr/ontologies/ccso#CS/NC_Networking_and_Communication"/>
        <hasSyllabus rdf:resource="http://xworks.gr/ontologies/ccso#TP60D5s1/IE_BSc/IED/STEF/TEIC"/>
        <includedIn rdf:resource="http://xworks.gr/ontologies/ccso#BSc_Informatics_Engineering/IE_BSc/IED/STEF/TEIC"/>
        <offeredBy rdf:resource="http://xworks.gr/ontologies/ccso#Department_of_Informatics_Engineering_of_TEI_of_Crete"/>
        <courseType rdf:datatype="http://www.w3.org/2001/XMLSchema#string">Elective</courseType>
        <csName rdf:datatype="http://www.w3.org/2001/XMLSchema#string">Parallel Processing and Systems</csName>
    </owl:NamedIndividual>
    


    <!-- http://xworks.gr/ontologies/ccso#TP60D5s1/IE_BSc/IED/STEF/TEIC -->

    <owl:NamedIndividual rdf:about="http://xworks.gr/ontologies/ccso#TP60D5s1/IE_BSc/IED/STEF/TEIC">
        <rdf:type rdf:resource="http://xworks.gr/ontologies/ccso#Syllabus"/>
        <affiliatedWith rdf:resource="http://xworks.gr/ontologies/ccso#Fragopoulou_Paraskevi"/>
        <coversTopic rdf:resource="http://xworks.gr/ontologies/ccso#CS/PL/T_Dynamic_dispatch:Definition_of_Method-Call"/>
        <coversTopic rdf:resource="http://xworks.gr/ontologies/ccso#CS/PL/T_Subclasses,Inheritance,and_Method_Overriding"/>
        <hasInstructor rdf:resource="http://xworks.gr/ontologies/ccso#Fragopoulou_Paraskevi"/>
        <hasSupervisor rdf:resource="http://xworks.gr/ontologies/ccso#Fragopoulou_Paraskevi"/>
        <syllabusOf rdf:resource="http://xworks.gr/ontologies/ccso#TP60D5/IE_BSc/IED/STEF/TEIC"/>
        <courseType rdf:datatype="http://www.w3.org/2001/XMLSchema#string">Elective</courseType>
        <creditsECTS rdf:datatype="http://www.w3.org/2001/XMLSchema#short">6</creditsECTS>
        <csName rdf:datatype="http://www.w3.org/2001/XMLSchema#string">Syllabus of course TP60D5 Parallel Processing and Systems</csName>
        <semesterinProgram rdf:datatype="http://www.w3.org/2001/XMLSchema#short">6</semesterinProgram>
    </owl:NamedIndividual>
    


    <!-- http://xworks.gr/ontologies/ccso#TP60L1/IE_BSc/IED/STEF/TEIC -->

    <owl:NamedIndividual rdf:about="http://xworks.gr/ontologies/ccso#TP60L1/IE_BSc/IED/STEF/TEIC">
        <rdf:type rdf:resource="http://xworks.gr/ontologies/ccso#Course"/>
        <coversKA rdf:resource="http://xworks.gr/ontologies/ccso#CS/SW_Software_Engineering_Software_Systems_and_Applications"/>
        <hasPrerequisite rdf:resource="http://xworks.gr/ontologies/ccso#TP30K2/IE_BSc/IED/STEF/TEIC"/>
        <hasSyllabus rdf:resource="http://xworks.gr/ontologies/ccso#TP60L1s1/IE_BSc/IED/STEF/TEIC"/>
        <includedIn rdf:resource="http://xworks.gr/ontologies/ccso#BSc_Informatics_Engineering/IE_BSc/IED/STEF/TEIC"/>
        <offeredBy rdf:resource="http://xworks.gr/ontologies/ccso#Department_of_Informatics_Engineering_of_TEI_of_Crete"/>
        <courseType rdf:datatype="http://www.w3.org/2001/XMLSchema#string">Core</courseType>
        <csName rdf:datatype="http://www.w3.org/2001/XMLSchema#string">Advanced Topics in Databases</csName>
    </owl:NamedIndividual>
    


    <!-- http://xworks.gr/ontologies/ccso#TP60L1s1/IE_BSc/IED/STEF/TEIC -->

    <owl:NamedIndividual rdf:about="http://xworks.gr/ontologies/ccso#TP60L1s1/IE_BSc/IED/STEF/TEIC">
        <rdf:type rdf:resource="http://xworks.gr/ontologies/ccso#Syllabus"/>
        <affiliatedWith rdf:resource="http://xworks.gr/ontologies/ccso#Akoumianakis_Demosthenes"/>
        <hasInstructor rdf:resource="http://xworks.gr/ontologies/ccso#Akoumianakis_Demosthenes"/>
        <hasSupervisor rdf:resource="http://xworks.gr/ontologies/ccso#Akoumianakis_Demosthenes"/>
        <syllabusOf rdf:resource="http://xworks.gr/ontologies/ccso#TP60L1/IE_BSc/IED/STEF/TEIC"/>
        <courseType rdf:datatype="http://www.w3.org/2001/XMLSchema#string">Core</courseType>
        <creditsECTS rdf:datatype="http://www.w3.org/2001/XMLSchema#short">6</creditsECTS>
        <csName rdf:datatype="http://www.w3.org/2001/XMLSchema#string">Syllabus of course TP60L1 Advanced Topics in Databases</csName>
        <semesterinProgram rdf:datatype="http://www.w3.org/2001/XMLSchema#short">6</semesterinProgram>
    </owl:NamedIndividual>
    


    <!-- http://xworks.gr/ontologies/ccso#TP60L2/IE_BSc/IED/STEF/TEIC -->

    <owl:NamedIndividual rdf:about="http://xworks.gr/ontologies/ccso#TP60L2/IE_BSc/IED/STEF/TEIC">
        <rdf:type rdf:resource="http://xworks.gr/ontologies/ccso#Course"/>
        <coversKA rdf:resource="http://xworks.gr/ontologies/ccso#CS/SW_Software_Engineering_Software_Systems_and_Applications"/>
        <hasPrerequisite rdf:resource="http://xworks.gr/ontologies/ccso#TP50L3/IE_BSc/IED/STEF/TEIC"/>
        <hasSyllabus rdf:resource="http://xworks.gr/ontologies/ccso#TP60L2s1/IE_BSc/IED/STEF/TEIC"/>
        <includedIn rdf:resource="http://xworks.gr/ontologies/ccso#BSc_Informatics_Engineering/IE_BSc/IED/STEF/TEIC"/>
        <offeredBy rdf:resource="http://xworks.gr/ontologies/ccso#Department_of_Informatics_Engineering_of_TEI_of_Crete"/>
        <courseType rdf:datatype="http://www.w3.org/2001/XMLSchema#string">Core</courseType>
        <csName rdf:datatype="http://www.w3.org/2001/XMLSchema#string">Artificial Intelligence</csName>
    </owl:NamedIndividual>
    


    <!-- http://xworks.gr/ontologies/ccso#TP60L2s1/IE_BSc/IED/STEF/TEIC -->

    <owl:NamedIndividual rdf:about="http://xworks.gr/ontologies/ccso#TP60L2s1/IE_BSc/IED/STEF/TEIC">
        <rdf:type rdf:resource="http://xworks.gr/ontologies/ccso#Syllabus"/>
        <affiliatedWith rdf:resource="http://xworks.gr/ontologies/ccso#Marakakis_Manolis"/>
        <hasInstructor rdf:resource="http://xworks.gr/ontologies/ccso#Marakakis_Manolis"/>
        <hasSupervisor rdf:resource="http://xworks.gr/ontologies/ccso#Marakakis_Manolis"/>
        <syllabusOf rdf:resource="http://xworks.gr/ontologies/ccso#TP60L2/IE_BSc/IED/STEF/TEIC"/>
        <courseType rdf:datatype="http://www.w3.org/2001/XMLSchema#string">Core</courseType>
        <creditsECTS rdf:datatype="http://www.w3.org/2001/XMLSchema#short">6</creditsECTS>
        <csName rdf:datatype="http://www.w3.org/2001/XMLSchema#string">Syllabus of course TP60L2 Artificial Intelligence</csName>
        <semesterinProgram rdf:datatype="http://www.w3.org/2001/XMLSchema#short">6</semesterinProgram>
    </owl:NamedIndividual>
    


    <!-- http://xworks.gr/ontologies/ccso#TP60L3/IE_BSc/IED/STEF/TEIC -->

    <owl:NamedIndividual rdf:about="http://xworks.gr/ontologies/ccso#TP60L3/IE_BSc/IED/STEF/TEIC">
        <rdf:type rdf:resource="http://xworks.gr/ontologies/ccso#Course"/>
        <coversKA rdf:resource="http://xworks.gr/ontologies/ccso#CS/SW_Software_Engineering_Software_Systems_and_Applications"/>
        <hasSyllabus rdf:resource="http://xworks.gr/ontologies/ccso#TP60L3s1/IE_BSc/IED/STEF/TEIC"/>
        <includedIn rdf:resource="http://xworks.gr/ontologies/ccso#BSc_Informatics_Engineering/IE_BSc/IED/STEF/TEIC"/>
        <offeredBy rdf:resource="http://xworks.gr/ontologies/ccso#Department_of_Informatics_Engineering_of_TEI_of_Crete"/>
        <courseType rdf:datatype="http://www.w3.org/2001/XMLSchema#string">Core</courseType>
        <csName rdf:datatype="http://www.w3.org/2001/XMLSchema#string">Management of ICT Projects</csName>
    </owl:NamedIndividual>
    


    <!-- http://xworks.gr/ontologies/ccso#TP60L3s1/IE_BSc/IED/STEF/TEIC -->

    <owl:NamedIndividual rdf:about="http://xworks.gr/ontologies/ccso#TP60L3s1/IE_BSc/IED/STEF/TEIC">
        <rdf:type rdf:resource="http://xworks.gr/ontologies/ccso#Syllabus"/>
        <affiliatedWith rdf:resource="http://xworks.gr/ontologies/ccso#Tsiknakis_Manolis"/>
        <hasInstructor rdf:resource="http://xworks.gr/ontologies/ccso#Tsiknakis_Manolis"/>
        <hasSupervisor rdf:resource="http://xworks.gr/ontologies/ccso#Tsiknakis_Manolis"/>
        <syllabusOf rdf:resource="http://xworks.gr/ontologies/ccso#TP60L3/IE_BSc/IED/STEF/TEIC"/>
        <courseType rdf:datatype="http://www.w3.org/2001/XMLSchema#string">Core</courseType>
        <creditsECTS rdf:datatype="http://www.w3.org/2001/XMLSchema#short">6</creditsECTS>
        <csName rdf:datatype="http://www.w3.org/2001/XMLSchema#string">Syllabus of course TP60L3 Management of ICT Projects</csName>
        <semesterinProgram rdf:datatype="http://www.w3.org/2001/XMLSchema#short">6</semesterinProgram>
    </owl:NamedIndividual>
    


    <!-- http://xworks.gr/ontologies/ccso#TP60L4/IE_BSc/IED/STEF/TEIC -->

    <owl:NamedIndividual rdf:about="http://xworks.gr/ontologies/ccso#TP60L4/IE_BSc/IED/STEF/TEIC">
        <rdf:type rdf:resource="http://xworks.gr/ontologies/ccso#Course"/>
        <coversKA rdf:resource="http://xworks.gr/ontologies/ccso#CS/SW_Software_Engineering_Software_Systems_and_Applications"/>
        <hasSyllabus rdf:resource="http://xworks.gr/ontologies/ccso#TP60L4s1/IE_BSc/IED/STEF/TEIC"/>
        <includedIn rdf:resource="http://xworks.gr/ontologies/ccso#BSc_Informatics_Engineering/IE_BSc/IED/STEF/TEIC"/>
        <offeredBy rdf:resource="http://xworks.gr/ontologies/ccso#Department_of_Informatics_Engineering_of_TEI_of_Crete"/>
        <courseType rdf:datatype="http://www.w3.org/2001/XMLSchema#string">Elective</courseType>
        <csName rdf:datatype="http://www.w3.org/2001/XMLSchema#string">Bioinformatics and Simulation of Physiological Systems</csName>
    </owl:NamedIndividual>
    


    <!-- http://xworks.gr/ontologies/ccso#TP60L4s1/IE_BSc/IED/STEF/TEIC -->

    <owl:NamedIndividual rdf:about="http://xworks.gr/ontologies/ccso#TP60L4s1/IE_BSc/IED/STEF/TEIC">
        <rdf:type rdf:resource="http://xworks.gr/ontologies/ccso#Syllabus"/>
        <affiliatedWith rdf:resource="http://xworks.gr/ontologies/ccso#Tsiknakis_Manolis"/>
        <hasInstructor rdf:resource="http://xworks.gr/ontologies/ccso#Tsiknakis_Manolis"/>
        <hasSupervisor rdf:resource="http://xworks.gr/ontologies/ccso#Tsiknakis_Manolis"/>
        <syllabusOf rdf:resource="http://xworks.gr/ontologies/ccso#TP60L4/IE_BSc/IED/STEF/TEIC"/>
        <courseType rdf:datatype="http://www.w3.org/2001/XMLSchema#string">Elective</courseType>
        <creditsECTS rdf:datatype="http://www.w3.org/2001/XMLSchema#short">6</creditsECTS>
        <csName rdf:datatype="http://www.w3.org/2001/XMLSchema#string">Syllabus of course TP60L4 Bioinformatics and Simulation of Physiological Systems</csName>
        <semesterinProgram rdf:datatype="http://www.w3.org/2001/XMLSchema#short">6</semesterinProgram>
    </owl:NamedIndividual>
    


    <!-- http://xworks.gr/ontologies/ccso#TP60L5/IE_BSc/IED/STEF/TEIC -->

    <owl:NamedIndividual rdf:about="http://xworks.gr/ontologies/ccso#TP60L5/IE_BSc/IED/STEF/TEIC">
        <rdf:type rdf:resource="http://xworks.gr/ontologies/ccso#Course"/>
        <coversKA rdf:resource="http://xworks.gr/ontologies/ccso#CS/SW_Software_Engineering_Software_Systems_and_Applications"/>
        <hasSyllabus rdf:resource="http://xworks.gr/ontologies/ccso#TP60L5s1/IE_BSc/IED/STEF/TEIC"/>
        <includedIn rdf:resource="http://xworks.gr/ontologies/ccso#BSc_Informatics_Engineering/IE_BSc/IED/STEF/TEIC"/>
        <offeredBy rdf:resource="http://xworks.gr/ontologies/ccso#Department_of_Informatics_Engineering_of_TEI_of_Crete"/>
        <courseType rdf:datatype="http://www.w3.org/2001/XMLSchema#string">Elective</courseType>
        <csName rdf:datatype="http://www.w3.org/2001/XMLSchema#string">Web Application Evaluation Systems</csName>
    </owl:NamedIndividual>
    


    <!-- http://xworks.gr/ontologies/ccso#TP60L5s1/IE_BSc/IED/STEF/TEIC -->

    <owl:NamedIndividual rdf:about="http://xworks.gr/ontologies/ccso#TP60L5s1/IE_BSc/IED/STEF/TEIC">
        <rdf:type rdf:resource="http://xworks.gr/ontologies/ccso#Syllabus"/>
        <affiliatedWith rdf:resource="http://xworks.gr/ontologies/ccso#Aivalis_Costas"/>
        <hasInstructor rdf:resource="http://xworks.gr/ontologies/ccso#Aivalis_Costas"/>
        <hasSupervisor rdf:resource="http://xworks.gr/ontologies/ccso#Aivalis_Costas"/>
        <syllabusOf rdf:resource="http://xworks.gr/ontologies/ccso#TP60L5/IE_BSc/IED/STEF/TEIC"/>
        <courseType rdf:datatype="http://www.w3.org/2001/XMLSchema#string">Elective</courseType>
        <creditsECTS rdf:datatype="http://www.w3.org/2001/XMLSchema#short">6</creditsECTS>
        <csName rdf:datatype="http://www.w3.org/2001/XMLSchema#string">Syllabus of course TP60L5 Web Application Evaluation Systems</csName>
        <semesterinProgram rdf:datatype="http://www.w3.org/2001/XMLSchema#short">6</semesterinProgram>
    </owl:NamedIndividual>
    


    <!-- http://xworks.gr/ontologies/ccso#TP60Y1/IE_BSc/IED/STEF/TEIC -->

    <owl:NamedIndividual rdf:about="http://xworks.gr/ontologies/ccso#TP60Y1/IE_BSc/IED/STEF/TEIC">
        <rdf:type rdf:resource="http://xworks.gr/ontologies/ccso#Course"/>
        <coversKA rdf:resource="http://xworks.gr/ontologies/ccso#CS/HW_Hardware_and_Computer_Systems"/>
        <hasSyllabus rdf:resource="http://xworks.gr/ontologies/ccso#TP60Y1s1/IE_BSc/IED/STEF/TEIC"/>
        <includedIn rdf:resource="http://xworks.gr/ontologies/ccso#BSc_Informatics_Engineering/IE_BSc/IED/STEF/TEIC"/>
        <offeredBy rdf:resource="http://xworks.gr/ontologies/ccso#Department_of_Informatics_Engineering_of_TEI_of_Crete"/>
        <courseType rdf:datatype="http://www.w3.org/2001/XMLSchema#string">Core</courseType>
        <csName rdf:datatype="http://www.w3.org/2001/XMLSchema#string">Neural Nets</csName>
    </owl:NamedIndividual>
    


    <!-- http://xworks.gr/ontologies/ccso#TP60Y1s1/IE_BSc/IED/STEF/TEIC -->

    <owl:NamedIndividual rdf:about="http://xworks.gr/ontologies/ccso#TP60Y1s1/IE_BSc/IED/STEF/TEIC">
        <rdf:type rdf:resource="http://xworks.gr/ontologies/ccso#Syllabus"/>
        <affiliatedWith rdf:resource="http://xworks.gr/ontologies/ccso#Papadourakis_George"/>
        <hasInstructor rdf:resource="http://xworks.gr/ontologies/ccso#Papadourakis_George"/>
        <hasSupervisor rdf:resource="http://xworks.gr/ontologies/ccso#Papadourakis_George"/>
        <syllabusOf rdf:resource="http://xworks.gr/ontologies/ccso#TP60Y1/IE_BSc/IED/STEF/TEIC"/>
        <courseType rdf:datatype="http://www.w3.org/2001/XMLSchema#string">Core</courseType>
        <creditsECTS rdf:datatype="http://www.w3.org/2001/XMLSchema#short">6</creditsECTS>
        <csName rdf:datatype="http://www.w3.org/2001/XMLSchema#string">Syllabus of course TP60Y1 Neural Nets</csName>
        <semesterinProgram rdf:datatype="http://www.w3.org/2001/XMLSchema#short">6</semesterinProgram>
    </owl:NamedIndividual>
    


    <!-- http://xworks.gr/ontologies/ccso#TP60Y2/IE_BSc/IED/STEF/TEIC -->

    <owl:NamedIndividual rdf:about="http://xworks.gr/ontologies/ccso#TP60Y2/IE_BSc/IED/STEF/TEIC">
        <rdf:type rdf:resource="http://xworks.gr/ontologies/ccso#Course"/>
        <coversKA rdf:resource="http://xworks.gr/ontologies/ccso#CS/HW_Hardware_and_Computer_Systems"/>
        <hasSyllabus rdf:resource="http://xworks.gr/ontologies/ccso#TP60Y2s1/IE_BSc/IED/STEF/TEIC"/>
        <includedIn rdf:resource="http://xworks.gr/ontologies/ccso#BSc_Informatics_Engineering/IE_BSc/IED/STEF/TEIC"/>
        <offeredBy rdf:resource="http://xworks.gr/ontologies/ccso#Department_of_Informatics_Engineering_of_TEI_of_Crete"/>
        <courseType rdf:datatype="http://www.w3.org/2001/XMLSchema#string">Core</courseType>
        <csName rdf:datatype="http://www.w3.org/2001/XMLSchema#string">Design and Architecture on FPGAs</csName>
    </owl:NamedIndividual>
    


    <!-- http://xworks.gr/ontologies/ccso#TP60Y2s1/IE_BSc/IED/STEF/TEIC -->

    <owl:NamedIndividual rdf:about="http://xworks.gr/ontologies/ccso#TP60Y2s1/IE_BSc/IED/STEF/TEIC">
        <rdf:type rdf:resource="http://xworks.gr/ontologies/ccso#Syllabus"/>
        <affiliatedWith rdf:resource="http://xworks.gr/ontologies/ccso#Kornaros_George"/>
        <hasInstructor rdf:resource="http://xworks.gr/ontologies/ccso#Kornaros_George"/>
        <hasSupervisor rdf:resource="http://xworks.gr/ontologies/ccso#Kornaros_George"/>
        <syllabusOf rdf:resource="http://xworks.gr/ontologies/ccso#TP60Y2/IE_BSc/IED/STEF/TEIC"/>
        <courseType rdf:datatype="http://www.w3.org/2001/XMLSchema#string">Core</courseType>
        <creditsECTS rdf:datatype="http://www.w3.org/2001/XMLSchema#short">6</creditsECTS>
        <csName rdf:datatype="http://www.w3.org/2001/XMLSchema#string">Syllabus of course TP60Y2 Design and Architecture on FPGAs</csName>
        <semesterinProgram rdf:datatype="http://www.w3.org/2001/XMLSchema#short">6</semesterinProgram>
    </owl:NamedIndividual>
    


    <!-- http://xworks.gr/ontologies/ccso#TP60Y6/IE_BSc/IED/STEF/TEIC -->

    <owl:NamedIndividual rdf:about="http://xworks.gr/ontologies/ccso#TP60Y6/IE_BSc/IED/STEF/TEIC">
        <rdf:type rdf:resource="http://xworks.gr/ontologies/ccso#Course"/>
        <coversKA rdf:resource="http://xworks.gr/ontologies/ccso#CS/HW_Hardware_and_Computer_Systems"/>
        <hasSyllabus rdf:resource="http://xworks.gr/ontologies/ccso#TP60Y6s1/IE_BSc/IED/STEF/TEIC"/>
        <includedIn rdf:resource="http://xworks.gr/ontologies/ccso#BSc_Informatics_Engineering/IE_BSc/IED/STEF/TEIC"/>
        <offeredBy rdf:resource="http://xworks.gr/ontologies/ccso#Department_of_Informatics_Engineering_of_TEI_of_Crete"/>
        <courseType rdf:datatype="http://www.w3.org/2001/XMLSchema#string">Core</courseType>
        <csName rdf:datatype="http://www.w3.org/2001/XMLSchema#string">Systems Programming</csName>
    </owl:NamedIndividual>
    


    <!-- http://xworks.gr/ontologies/ccso#TP60Y6s1/IE_BSc/IED/STEF/TEIC -->

    <owl:NamedIndividual rdf:about="http://xworks.gr/ontologies/ccso#TP60Y6s1/IE_BSc/IED/STEF/TEIC">
        <rdf:type rdf:resource="http://xworks.gr/ontologies/ccso#Syllabus"/>
        <affiliatedWith rdf:resource="http://xworks.gr/ontologies/ccso#Grammatikakis_Miltiadis"/>
        <hasInstructor rdf:resource="http://xworks.gr/ontologies/ccso#Grammatikakis_Miltiadis"/>
        <hasSupervisor rdf:resource="http://xworks.gr/ontologies/ccso#Grammatikakis_Miltiadis"/>
        <syllabusOf rdf:resource="http://xworks.gr/ontologies/ccso#TP60Y6/IE_BSc/IED/STEF/TEIC"/>
        <courseType rdf:datatype="http://www.w3.org/2001/XMLSchema#string">Core</courseType>
        <creditsECTS rdf:datatype="http://www.w3.org/2001/XMLSchema#short">6</creditsECTS>
        <csName rdf:datatype="http://www.w3.org/2001/XMLSchema#string">Syllabus of course TP60Y6 Systems Programming</csName>
        <semesterinProgram rdf:datatype="http://www.w3.org/2001/XMLSchema#short">6</semesterinProgram>
    </owl:NamedIndividual>
    


    <!-- http://xworks.gr/ontologies/ccso#TP70D1/IE_BSc/IED/STEF/TEIC -->

    <owl:NamedIndividual rdf:about="http://xworks.gr/ontologies/ccso#TP70D1/IE_BSc/IED/STEF/TEIC">
        <rdf:type rdf:resource="http://xworks.gr/ontologies/ccso#Course"/>
        <coversKA rdf:resource="http://xworks.gr/ontologies/ccso#CS/NC_Networking_and_Communication"/>
        <hasSyllabus rdf:resource="http://xworks.gr/ontologies/ccso#TP70D1s1/IE_BSc/IED/STEF/TEIC"/>
        <includedIn rdf:resource="http://xworks.gr/ontologies/ccso#BSc_Informatics_Engineering/IE_BSc/IED/STEF/TEIC"/>
        <offeredBy rdf:resource="http://xworks.gr/ontologies/ccso#Department_of_Informatics_Engineering_of_TEI_of_Crete"/>
        <courseType rdf:datatype="http://www.w3.org/2001/XMLSchema#string">Core</courseType>
        <csName rdf:datatype="http://www.w3.org/2001/XMLSchema#string">Mobile and Personal Communication Networks</csName>
    </owl:NamedIndividual>
    


    <!-- http://xworks.gr/ontologies/ccso#TP70D1s1/IE_BSc/IED/STEF/TEIC -->

    <owl:NamedIndividual rdf:about="http://xworks.gr/ontologies/ccso#TP70D1s1/IE_BSc/IED/STEF/TEIC">
        <rdf:type rdf:resource="http://xworks.gr/ontologies/ccso#Syllabus"/>
        <affiliatedWith rdf:resource="http://xworks.gr/ontologies/ccso#Stratakis_Dimitrios"/>
        <hasInstructor rdf:resource="http://xworks.gr/ontologies/ccso#Stratakis_Dimitrios"/>
        <hasSupervisor rdf:resource="http://xworks.gr/ontologies/ccso#Stratakis_Dimitrios"/>
        <syllabusOf rdf:resource="http://xworks.gr/ontologies/ccso#TP70D1/IE_BSc/IED/STEF/TEIC"/>
        <courseType rdf:datatype="http://www.w3.org/2001/XMLSchema#string">Core</courseType>
        <creditsECTS rdf:datatype="http://www.w3.org/2001/XMLSchema#short">6</creditsECTS>
        <csName rdf:datatype="http://www.w3.org/2001/XMLSchema#string">Syllabus of course TP70D1 Mobile and Personal Communication Networks</csName>
        <semesterinProgram rdf:datatype="http://www.w3.org/2001/XMLSchema#short">7</semesterinProgram>
    </owl:NamedIndividual>
    


    <!-- http://xworks.gr/ontologies/ccso#TP70D2/IE_BSc/IED/STEF/TEIC -->

    <owl:NamedIndividual rdf:about="http://xworks.gr/ontologies/ccso#TP70D2/IE_BSc/IED/STEF/TEIC">
        <rdf:type rdf:resource="http://xworks.gr/ontologies/ccso#Course"/>
        <coversKA rdf:resource="http://xworks.gr/ontologies/ccso#CS/NC_Networking_and_Communication"/>
        <hasSyllabus rdf:resource="http://xworks.gr/ontologies/ccso#TP70D2s1/IE_BSc/IED/STEF/TEIC"/>
        <includedIn rdf:resource="http://xworks.gr/ontologies/ccso#BSc_Informatics_Engineering/IE_BSc/IED/STEF/TEIC"/>
        <offeredBy rdf:resource="http://xworks.gr/ontologies/ccso#Department_of_Informatics_Engineering_of_TEI_of_Crete"/>
        <courseType rdf:datatype="http://www.w3.org/2001/XMLSchema#string">Core</courseType>
        <csName rdf:datatype="http://www.w3.org/2001/XMLSchema#string">Networks Security</csName>
    </owl:NamedIndividual>
    


    <!-- http://xworks.gr/ontologies/ccso#TP70D2s1/IE_BSc/IED/STEF/TEIC -->

    <owl:NamedIndividual rdf:about="http://xworks.gr/ontologies/ccso#TP70D2s1/IE_BSc/IED/STEF/TEIC">
        <rdf:type rdf:resource="http://xworks.gr/ontologies/ccso#Syllabus"/>
        <affiliatedWith rdf:resource="http://xworks.gr/ontologies/ccso#Panagiotakis_Spyros"/>
        <hasInstructor rdf:resource="http://xworks.gr/ontologies/ccso#Panagiotakis_Spyros"/>
        <hasSupervisor rdf:resource="http://xworks.gr/ontologies/ccso#Panagiotakis_Spyros"/>
        <syllabusOf rdf:resource="http://xworks.gr/ontologies/ccso#TP70D2/IE_BSc/IED/STEF/TEIC"/>
        <courseType rdf:datatype="http://www.w3.org/2001/XMLSchema#string">Core</courseType>
        <creditsECTS rdf:datatype="http://www.w3.org/2001/XMLSchema#short">6</creditsECTS>
        <csName rdf:datatype="http://www.w3.org/2001/XMLSchema#string">Syllabus of course TP70D2 Networks Security</csName>
        <semesterinProgram rdf:datatype="http://www.w3.org/2001/XMLSchema#short">7</semesterinProgram>
    </owl:NamedIndividual>
    


    <!-- http://xworks.gr/ontologies/ccso#TP70D3/IE_BSc/IED/STEF/TEIC -->

    <owl:NamedIndividual rdf:about="http://xworks.gr/ontologies/ccso#TP70D3/IE_BSc/IED/STEF/TEIC">
        <rdf:type rdf:resource="http://xworks.gr/ontologies/ccso#Course"/>
        <coversKA rdf:resource="http://xworks.gr/ontologies/ccso#CS/NC_Networking_and_Communication"/>
        <hasSyllabus rdf:resource="http://xworks.gr/ontologies/ccso#TP70D3s1/IE_BSc/IED/STEF/TEIC"/>
        <includedIn rdf:resource="http://xworks.gr/ontologies/ccso#BSc_Informatics_Engineering/IE_BSc/IED/STEF/TEIC"/>
        <offeredBy rdf:resource="http://xworks.gr/ontologies/ccso#Department_of_Informatics_Engineering_of_TEI_of_Crete"/>
        <courseType rdf:datatype="http://www.w3.org/2001/XMLSchema#string">Core</courseType>
        <csName rdf:datatype="http://www.w3.org/2001/XMLSchema#string">Distributed Systems and Cloud Computing</csName>
    </owl:NamedIndividual>
    


    <!-- http://xworks.gr/ontologies/ccso#TP70D3s1/IE_BSc/IED/STEF/TEIC -->

    <owl:NamedIndividual rdf:about="http://xworks.gr/ontologies/ccso#TP70D3s1/IE_BSc/IED/STEF/TEIC">
        <rdf:type rdf:resource="http://xworks.gr/ontologies/ccso#Syllabus"/>
        <affiliatedWith rdf:resource="http://xworks.gr/ontologies/ccso#Fragopoulou_Paraskevi"/>
        <hasInstructor rdf:resource="http://xworks.gr/ontologies/ccso#Fragopoulou_Paraskevi"/>
        <hasSupervisor rdf:resource="http://xworks.gr/ontologies/ccso#Fragopoulou_Paraskevi"/>
        <syllabusOf rdf:resource="http://xworks.gr/ontologies/ccso#TP70D3/IE_BSc/IED/STEF/TEIC"/>
        <courseType rdf:datatype="http://www.w3.org/2001/XMLSchema#string">Core</courseType>
        <creditsECTS rdf:datatype="http://www.w3.org/2001/XMLSchema#short">6</creditsECTS>
        <csName rdf:datatype="http://www.w3.org/2001/XMLSchema#string">Syllabus of course TP70D3 Distributed Systems and Cloud Computing</csName>
        <semesterinProgram rdf:datatype="http://www.w3.org/2001/XMLSchema#short">7</semesterinProgram>
    </owl:NamedIndividual>
    


    <!-- http://xworks.gr/ontologies/ccso#TP70D5/IE_BSc/IED/STEF/TEIC -->

    <owl:NamedIndividual rdf:about="http://xworks.gr/ontologies/ccso#TP70D5/IE_BSc/IED/STEF/TEIC">
        <rdf:type rdf:resource="http://xworks.gr/ontologies/ccso#Course"/>
        <coversKA rdf:resource="http://xworks.gr/ontologies/ccso#CS/HW_Hardware_and_Computer_Systems"/>
        <coversKA rdf:resource="http://xworks.gr/ontologies/ccso#CS/NC_Networking_and_Communication"/>
        <hasSyllabus rdf:resource="http://xworks.gr/ontologies/ccso#TP70D5s1/IE_BSc/IED/STEF/TEIC"/>
        <includedIn rdf:resource="http://xworks.gr/ontologies/ccso#BSc_Informatics_Engineering/IE_BSc/IED/STEF/TEIC"/>
        <offeredBy rdf:resource="http://xworks.gr/ontologies/ccso#Department_of_Informatics_Engineering_of_TEI_of_Crete"/>
        <courseType rdf:datatype="http://www.w3.org/2001/XMLSchema#string">Elective</courseType>
        <csName rdf:datatype="http://www.w3.org/2001/XMLSchema#string">Internet Multimedia and Graphics</csName>
    </owl:NamedIndividual>
    


    <!-- http://xworks.gr/ontologies/ccso#TP70D5s1/IE_BSc/IED/STEF/TEIC -->

    <owl:NamedIndividual rdf:about="http://xworks.gr/ontologies/ccso#TP70D5s1/IE_BSc/IED/STEF/TEIC">
        <rdf:type rdf:resource="http://xworks.gr/ontologies/ccso#Syllabus"/>
        <affiliatedWith rdf:resource="http://xworks.gr/ontologies/ccso#Malamos_Athanasios"/>
        <hasInstructor rdf:resource="http://xworks.gr/ontologies/ccso#Malamos_Athanasios"/>
        <hasSupervisor rdf:resource="http://xworks.gr/ontologies/ccso#Malamos_Athanasios"/>
        <syllabusOf rdf:resource="http://xworks.gr/ontologies/ccso#TP70D5/IE_BSc/IED/STEF/TEIC"/>
        <courseType rdf:datatype="http://www.w3.org/2001/XMLSchema#string">Core</courseType>
        <creditsECTS rdf:datatype="http://www.w3.org/2001/XMLSchema#short">6</creditsECTS>
        <csName rdf:datatype="http://www.w3.org/2001/XMLSchema#string">Syllabus of course TP70D5 Internet Multimedia and Graphics</csName>
        <semesterinProgram rdf:datatype="http://www.w3.org/2001/XMLSchema#short">7</semesterinProgram>
    </owl:NamedIndividual>
    


    <!-- http://xworks.gr/ontologies/ccso#TP70L1/IE_BSc/IED/STEF/TEIC -->

    <owl:NamedIndividual rdf:about="http://xworks.gr/ontologies/ccso#TP70L1/IE_BSc/IED/STEF/TEIC">
        <rdf:type rdf:resource="http://xworks.gr/ontologies/ccso#Course"/>
        <coversKA rdf:resource="http://xworks.gr/ontologies/ccso#CS/SW_Software_Engineering_Software_Systems_and_Applications"/>
        <hasPrerequisite rdf:resource="http://xworks.gr/ontologies/ccso#TP60L2/IE_BSc/IED/STEF/TEIC"/>
        <hasSyllabus rdf:resource="http://xworks.gr/ontologies/ccso#TP70L1s1/IE_BSc/IED/STEF/TEIC"/>
        <includedIn rdf:resource="http://xworks.gr/ontologies/ccso#BSc_Informatics_Engineering/IE_BSc/IED/STEF/TEIC"/>
        <offeredBy rdf:resource="http://xworks.gr/ontologies/ccso#Department_of_Informatics_Engineering_of_TEI_of_Crete"/>
        <courseType rdf:datatype="http://www.w3.org/2001/XMLSchema#string">Core</courseType>
        <csName rdf:datatype="http://www.w3.org/2001/XMLSchema#string">Knowledge Systems</csName>
    </owl:NamedIndividual>
    


    <!-- http://xworks.gr/ontologies/ccso#TP70L1s1/IE_BSc/IED/STEF/TEIC -->

    <owl:NamedIndividual rdf:about="http://xworks.gr/ontologies/ccso#TP70L1s1/IE_BSc/IED/STEF/TEIC">
        <rdf:type rdf:resource="http://xworks.gr/ontologies/ccso#Syllabus"/>
        <affiliatedWith rdf:resource="http://xworks.gr/ontologies/ccso#Marakakis_Manolis"/>
        <hasInstructor rdf:resource="http://xworks.gr/ontologies/ccso#Marakakis_Manolis"/>
        <hasSupervisor rdf:resource="http://xworks.gr/ontologies/ccso#Marakakis_Manolis"/>
        <syllabusOf rdf:resource="http://xworks.gr/ontologies/ccso#TP70L1/IE_BSc/IED/STEF/TEIC"/>
        <courseType rdf:datatype="http://www.w3.org/2001/XMLSchema#string">Core</courseType>
        <creditsECTS rdf:datatype="http://www.w3.org/2001/XMLSchema#short">6</creditsECTS>
        <csName rdf:datatype="http://www.w3.org/2001/XMLSchema#string">Syllabus of course TP70L1 Knowledge Systems</csName>
        <semesterinProgram rdf:datatype="http://www.w3.org/2001/XMLSchema#short">7</semesterinProgram>
    </owl:NamedIndividual>
    


    <!-- http://xworks.gr/ontologies/ccso#TP70L2/IE_BSc/IED/STEF/TEIC -->

    <owl:NamedIndividual rdf:about="http://xworks.gr/ontologies/ccso#TP70L2/IE_BSc/IED/STEF/TEIC">
        <rdf:type rdf:resource="http://xworks.gr/ontologies/ccso#Course"/>
        <coversKA rdf:resource="http://xworks.gr/ontologies/ccso#CS/SW_Software_Engineering_Software_Systems_and_Applications"/>
        <hasSyllabus rdf:resource="http://xworks.gr/ontologies/ccso#TP70L2s1/IE_BSc/IED/STEF/TEIC"/>
        <includedIn rdf:resource="http://xworks.gr/ontologies/ccso#BSc_Informatics_Engineering/IE_BSc/IED/STEF/TEIC"/>
        <offeredBy rdf:resource="http://xworks.gr/ontologies/ccso#Department_of_Informatics_Engineering_of_TEI_of_Crete"/>
        <courseType rdf:datatype="http://www.w3.org/2001/XMLSchema#string">Core</courseType>
        <csName rdf:datatype="http://www.w3.org/2001/XMLSchema#string">Designing the User Interface</csName>
    </owl:NamedIndividual>
    


    <!-- http://xworks.gr/ontologies/ccso#TP70L2s1/IE_BSc/IED/STEF/TEIC -->

    <owl:NamedIndividual rdf:about="http://xworks.gr/ontologies/ccso#TP70L2s1/IE_BSc/IED/STEF/TEIC">
        <rdf:type rdf:resource="http://xworks.gr/ontologies/ccso#Syllabus"/>
        <affiliatedWith rdf:resource="http://xworks.gr/ontologies/ccso#Akoumianakis_Demosthenes"/>
        <hasInstructor rdf:resource="http://xworks.gr/ontologies/ccso#Akoumianakis_Demosthenes"/>
        <hasSupervisor rdf:resource="http://xworks.gr/ontologies/ccso#Akoumianakis_Demosthenes"/>
        <syllabusOf rdf:resource="http://xworks.gr/ontologies/ccso#TP70L2/IE_BSc/IED/STEF/TEIC"/>
        <courseType rdf:datatype="http://www.w3.org/2001/XMLSchema#string">Elective</courseType>
        <creditsECTS rdf:datatype="http://www.w3.org/2001/XMLSchema#short">6</creditsECTS>
        <csName rdf:datatype="http://www.w3.org/2001/XMLSchema#string">Syllabus of course TP70L2 Designing the User Interface</csName>
        <semesterinProgram rdf:datatype="http://www.w3.org/2001/XMLSchema#short">7</semesterinProgram>
    </owl:NamedIndividual>
    


    <!-- http://xworks.gr/ontologies/ccso#TP70L3/IE_BSc/IED/STEF/TEIC -->

    <owl:NamedIndividual rdf:about="http://xworks.gr/ontologies/ccso#TP70L3/IE_BSc/IED/STEF/TEIC">
        <rdf:type rdf:resource="http://xworks.gr/ontologies/ccso#Course"/>
        <coversKA rdf:resource="http://xworks.gr/ontologies/ccso#CS/SW_Software_Engineering_Software_Systems_and_Applications"/>
        <hasSyllabus rdf:resource="http://xworks.gr/ontologies/ccso#TP70L3s1/IE_BSc/IED/STEF/TEIC"/>
        <includedIn rdf:resource="http://xworks.gr/ontologies/ccso#BSc_Informatics_Engineering/IE_BSc/IED/STEF/TEIC"/>
        <offeredBy rdf:resource="http://xworks.gr/ontologies/ccso#Department_of_Informatics_Engineering_of_TEI_of_Crete"/>
        <courseType rdf:datatype="http://www.w3.org/2001/XMLSchema#string">Elective</courseType>
        <csName rdf:datatype="http://www.w3.org/2001/XMLSchema#string">Information Systems Security</csName>
    </owl:NamedIndividual>
    


    <!-- http://xworks.gr/ontologies/ccso#TP70L3s1/IE_BSc/IED/STEF/TEIC -->

    <owl:NamedIndividual rdf:about="http://xworks.gr/ontologies/ccso#TP70L3s1/IE_BSc/IED/STEF/TEIC">
        <rdf:type rdf:resource="http://xworks.gr/ontologies/ccso#Syllabus"/>
        <affiliatedWith rdf:resource="http://xworks.gr/ontologies/ccso#Grammatikakis_Miltiadis"/>
        <hasInstructor rdf:resource="http://xworks.gr/ontologies/ccso#Grammatikakis_Miltiadis"/>
        <hasSupervisor rdf:resource="http://xworks.gr/ontologies/ccso#Grammatikakis_Miltiadis"/>
        <syllabusOf rdf:resource="http://xworks.gr/ontologies/ccso#TP70L3/IE_BSc/IED/STEF/TEIC"/>
        <courseType rdf:datatype="http://www.w3.org/2001/XMLSchema#string">Core</courseType>
        <creditsECTS rdf:datatype="http://www.w3.org/2001/XMLSchema#short">6</creditsECTS>
        <csName rdf:datatype="http://www.w3.org/2001/XMLSchema#string">Syllabus of course TP70L3 Information Systems Security</csName>
        <semesterinProgram rdf:datatype="http://www.w3.org/2001/XMLSchema#short">7</semesterinProgram>
    </owl:NamedIndividual>
    


    <!-- http://xworks.gr/ontologies/ccso#TP70L4/IE_BSc/IED/STEF/TEIC -->

    <owl:NamedIndividual rdf:about="http://xworks.gr/ontologies/ccso#TP70L4/IE_BSc/IED/STEF/TEIC">
        <rdf:type rdf:resource="http://xworks.gr/ontologies/ccso#Course"/>
        <coversKA rdf:resource="http://xworks.gr/ontologies/ccso#CS/SW_Software_Engineering_Software_Systems_and_Applications"/>
        <hasSyllabus rdf:resource="http://xworks.gr/ontologies/ccso#TP70L4s1/IE_BSc/IED/STEF/TEIC"/>
        <includedIn rdf:resource="http://xworks.gr/ontologies/ccso#BSc_Informatics_Engineering/IE_BSc/IED/STEF/TEIC"/>
        <offeredBy rdf:resource="http://xworks.gr/ontologies/ccso#Department_of_Informatics_Engineering_of_TEI_of_Crete"/>
        <courseType rdf:datatype="http://www.w3.org/2001/XMLSchema#string">Elective</courseType>
        <csName rdf:datatype="http://www.w3.org/2001/XMLSchema#string">Digital Technology and Applications in Engineering</csName>
    </owl:NamedIndividual>
    


    <!-- http://xworks.gr/ontologies/ccso#TP70L4s1/IE_BSc/IED/STEF/TEIC -->

    <owl:NamedIndividual rdf:about="http://xworks.gr/ontologies/ccso#TP70L4s1/IE_BSc/IED/STEF/TEIC">
        <rdf:type rdf:resource="http://xworks.gr/ontologies/ccso#Syllabus"/>
        <affiliatedWith rdf:resource="http://xworks.gr/ontologies/ccso#Akoumianakis_Demosthenes"/>
        <hasInstructor rdf:resource="http://xworks.gr/ontologies/ccso#Akoumianakis_Demosthenes"/>
        <hasSupervisor rdf:resource="http://xworks.gr/ontologies/ccso#Akoumianakis_Demosthenes"/>
        <syllabusOf rdf:resource="http://xworks.gr/ontologies/ccso#TP70L4/IE_BSc/IED/STEF/TEIC"/>
        <courseType rdf:datatype="http://www.w3.org/2001/XMLSchema#string">Elective</courseType>
        <creditsECTS rdf:datatype="http://www.w3.org/2001/XMLSchema#short">6</creditsECTS>
        <csName rdf:datatype="http://www.w3.org/2001/XMLSchema#string">Syllabus of course TP70L4 Digital Technology and Applications in Engineering</csName>
        <semesterinProgram rdf:datatype="http://www.w3.org/2001/XMLSchema#short">7</semesterinProgram>
    </owl:NamedIndividual>
    


    <!-- http://xworks.gr/ontologies/ccso#TP70L5/IE_BSc/IED/STEF/TEIC -->

    <owl:NamedIndividual rdf:about="http://xworks.gr/ontologies/ccso#TP70L5/IE_BSc/IED/STEF/TEIC">
        <rdf:type rdf:resource="http://xworks.gr/ontologies/ccso#Course"/>
        <coversKA rdf:resource="http://xworks.gr/ontologies/ccso#CS/SW_Software_Engineering_Software_Systems_and_Applications"/>
        <hasSyllabus rdf:resource="http://xworks.gr/ontologies/ccso#TP70L5s1/IE_BSc/IED/STEF/TEIC"/>
        <includedIn rdf:resource="http://xworks.gr/ontologies/ccso#BSc_Informatics_Engineering/IE_BSc/IED/STEF/TEIC"/>
        <offeredBy rdf:resource="http://xworks.gr/ontologies/ccso#Department_of_Informatics_Engineering_of_TEI_of_Crete"/>
        <courseType rdf:datatype="http://www.w3.org/2001/XMLSchema#string">Elective</courseType>
        <csName rdf:datatype="http://www.w3.org/2001/XMLSchema#string">Business Process Management
Information Systems and Workflows</csName>
    </owl:NamedIndividual>
    


    <!-- http://xworks.gr/ontologies/ccso#TP70L5s1/IE_BSc/IED/STEF/TEIC -->

    <owl:NamedIndividual rdf:about="http://xworks.gr/ontologies/ccso#TP70L5s1/IE_BSc/IED/STEF/TEIC">
        <rdf:type rdf:resource="http://xworks.gr/ontologies/ccso#Syllabus"/>
        <affiliatedWith rdf:resource="http://xworks.gr/ontologies/ccso#Papadakis_Nikos"/>
        <hasInstructor rdf:resource="http://xworks.gr/ontologies/ccso#Papadakis_Nikos"/>
        <hasSupervisor rdf:resource="http://xworks.gr/ontologies/ccso#Papadakis_Nikos"/>
        <syllabusOf rdf:resource="http://xworks.gr/ontologies/ccso#TP70L5/IE_BSc/IED/STEF/TEIC"/>
        <courseType rdf:datatype="http://www.w3.org/2001/XMLSchema#string">Elective</courseType>
        <creditsECTS rdf:datatype="http://www.w3.org/2001/XMLSchema#short">6</creditsECTS>
        <csName rdf:datatype="http://www.w3.org/2001/XMLSchema#string">Syllabus of course TP70L5 Business Process Management
Information Systems and Workflows</csName>
        <semesterinProgram rdf:datatype="http://www.w3.org/2001/XMLSchema#short">7</semesterinProgram>
    </owl:NamedIndividual>
    


    <!-- http://xworks.gr/ontologies/ccso#TP70Y1/IE_BSc/IED/STEF/TEIC -->

    <owl:NamedIndividual rdf:about="http://xworks.gr/ontologies/ccso#TP70Y1/IE_BSc/IED/STEF/TEIC">
        <rdf:type rdf:resource="http://xworks.gr/ontologies/ccso#Course"/>
        <coversKA rdf:resource="http://xworks.gr/ontologies/ccso#CS/HW_Hardware_and_Computer_Systems"/>
        <hasSyllabus rdf:resource="http://xworks.gr/ontologies/ccso#TP70Y1s1/IE_BSc/IED/STEF/TEIC"/>
        <includedIn rdf:resource="http://xworks.gr/ontologies/ccso#BSc_Informatics_Engineering/IE_BSc/IED/STEF/TEIC"/>
        <offeredBy rdf:resource="http://xworks.gr/ontologies/ccso#Department_of_Informatics_Engineering_of_TEI_of_Crete"/>
        <courseType rdf:datatype="http://www.w3.org/2001/XMLSchema#string">Core</courseType>
        <csName rdf:datatype="http://www.w3.org/2001/XMLSchema#string">Embedded Systems</csName>
    </owl:NamedIndividual>
    


    <!-- http://xworks.gr/ontologies/ccso#TP70Y1s1/IE_BSc/IED/STEF/TEIC -->

    <owl:NamedIndividual rdf:about="http://xworks.gr/ontologies/ccso#TP70Y1s1/IE_BSc/IED/STEF/TEIC">
        <rdf:type rdf:resource="http://xworks.gr/ontologies/ccso#Syllabus"/>
        <affiliatedWith rdf:resource="http://xworks.gr/ontologies/ccso#Kornaros_George"/>
        <hasInstructor rdf:resource="http://xworks.gr/ontologies/ccso#Kornaros_George"/>
        <hasSupervisor rdf:resource="http://xworks.gr/ontologies/ccso#Kornaros_George"/>
        <syllabusOf rdf:resource="http://xworks.gr/ontologies/ccso#TP70Y1/IE_BSc/IED/STEF/TEIC"/>
        <courseType rdf:datatype="http://www.w3.org/2001/XMLSchema#string">Elective</courseType>
        <creditsECTS rdf:datatype="http://www.w3.org/2001/XMLSchema#short">6</creditsECTS>
        <csName rdf:datatype="http://www.w3.org/2001/XMLSchema#string">Syllabus of course TP70Y1 Embedded Systems</csName>
        <semesterinProgram rdf:datatype="http://www.w3.org/2001/XMLSchema#short">7</semesterinProgram>
    </owl:NamedIndividual>
    


    <!-- http://xworks.gr/ontologies/ccso#TP70Y2/IE_BSc/IED/STEF/TEIC -->

    <owl:NamedIndividual rdf:about="http://xworks.gr/ontologies/ccso#TP70Y2/IE_BSc/IED/STEF/TEIC">
        <rdf:type rdf:resource="http://xworks.gr/ontologies/ccso#Course"/>
        <coversKA rdf:resource="http://xworks.gr/ontologies/ccso#CS/CVR_Computer_Vision_and_Robotics"/>
        <coversKA rdf:resource="http://xworks.gr/ontologies/ccso#CS/HW_Hardware_and_Computer_Systems"/>
        <hasSyllabus rdf:resource="http://xworks.gr/ontologies/ccso#TP70Y2s1/IE_BSc/IED/STEF/TEIC"/>
        <includedIn rdf:resource="http://xworks.gr/ontologies/ccso#BSc_Informatics_Engineering/IE_BSc/IED/STEF/TEIC"/>
        <offeredBy rdf:resource="http://xworks.gr/ontologies/ccso#Department_of_Informatics_Engineering_of_TEI_of_Crete"/>
        <courseType rdf:datatype="http://www.w3.org/2001/XMLSchema#string">Core</courseType>
        <csName rdf:datatype="http://www.w3.org/2001/XMLSchema#string">Computer Vision</csName>
    </owl:NamedIndividual>
    


    <!-- http://xworks.gr/ontologies/ccso#TP70Y2s1/IE_BSc/IED/STEF/TEIC -->

    <owl:NamedIndividual rdf:about="http://xworks.gr/ontologies/ccso#TP70Y2s1/IE_BSc/IED/STEF/TEIC">
        <rdf:type rdf:resource="http://xworks.gr/ontologies/ccso#Syllabus"/>
        <affiliatedWith rdf:resource="http://xworks.gr/ontologies/ccso#Kornaros_George"/>
        <affiliatedWith rdf:resource="http://xworks.gr/ontologies/ccso#Marias_Kostas"/>
        <hasInstructor rdf:resource="http://xworks.gr/ontologies/ccso#Kornaros_George"/>
        <hasSupervisor rdf:resource="http://xworks.gr/ontologies/ccso#Marias_Kostas"/>
        <syllabusOf rdf:resource="http://xworks.gr/ontologies/ccso#TP70Y2/IE_BSc/IED/STEF/TEIC"/>
        <courseType rdf:datatype="http://www.w3.org/2001/XMLSchema#string">Elective</courseType>
        <creditsECTS rdf:datatype="http://www.w3.org/2001/XMLSchema#short">6</creditsECTS>
        <csName rdf:datatype="http://www.w3.org/2001/XMLSchema#string">Syllabus of course TP70Y2 Computer Vision</csName>
        <semesterinProgram rdf:datatype="http://www.w3.org/2001/XMLSchema#short">7</semesterinProgram>
    </owl:NamedIndividual>
    


    <!-- http://xworks.gr/ontologies/ccso#TP70Y3/IE_BSc/IED/STEF/TEIC -->

    <owl:NamedIndividual rdf:about="http://xworks.gr/ontologies/ccso#TP70Y3/IE_BSc/IED/STEF/TEIC">
        <rdf:type rdf:resource="http://xworks.gr/ontologies/ccso#Course"/>
        <courseType rdf:datatype="http://www.w3.org/2001/XMLSchema#string">Core</courseType>
    </owl:NamedIndividual>
    


    <!-- http://xworks.gr/ontologies/ccso#TP70Y6/IE_BSc/IED/STEF/TEIC -->

    <owl:NamedIndividual rdf:about="http://xworks.gr/ontologies/ccso#TP70Y6/IE_BSc/IED/STEF/TEIC">
        <rdf:type rdf:resource="http://xworks.gr/ontologies/ccso#Course"/>
        <coversKA rdf:resource="http://xworks.gr/ontologies/ccso#CS/HW_Hardware_and_Computer_Systems"/>
        <coversKA rdf:resource="http://xworks.gr/ontologies/ccso#CS/NC_Networking_and_Communication"/>
        <hasSyllabus rdf:resource="http://xworks.gr/ontologies/ccso#TP70Y6s1/IE_BSc/IED/STEF/TEIC"/>
        <includedIn rdf:resource="http://xworks.gr/ontologies/ccso#BSc_Informatics_Engineering/IE_BSc/IED/STEF/TEIC"/>
        <offeredBy rdf:resource="http://xworks.gr/ontologies/ccso#Department_of_Informatics_Engineering_of_TEI_of_Crete"/>
        <courseType rdf:datatype="http://www.w3.org/2001/XMLSchema#string">Elective</courseType>
        <csName rdf:datatype="http://www.w3.org/2001/XMLSchema#string">Internet of Things and Automation</csName>
    </owl:NamedIndividual>
    


    <!-- http://xworks.gr/ontologies/ccso#TP70Y6s1/IE_BSc/IED/STEF/TEIC -->

    <owl:NamedIndividual rdf:about="http://xworks.gr/ontologies/ccso#TP70Y6s1/IE_BSc/IED/STEF/TEIC">
        <rdf:type rdf:resource="http://xworks.gr/ontologies/ccso#Syllabus"/>
        <affiliatedWith rdf:resource="http://xworks.gr/ontologies/ccso#Panagiotakis_Spyros"/>
        <hasInstructor rdf:resource="http://xworks.gr/ontologies/ccso#Panagiotakis_Spyros"/>
        <hasSupervisor rdf:resource="http://xworks.gr/ontologies/ccso#Panagiotakis_Spyros"/>
        <syllabusOf rdf:resource="http://xworks.gr/ontologies/ccso#TP70Y6/IE_BSc/IED/STEF/TEIC"/>
        <courseType rdf:datatype="http://www.w3.org/2001/XMLSchema#string">Elective</courseType>
        <creditsECTS rdf:datatype="http://www.w3.org/2001/XMLSchema#short">6</creditsECTS>
        <csName rdf:datatype="http://www.w3.org/2001/XMLSchema#string">Syllabus of course TP70Y6 Internet of Things and Automation</csName>
        <semesterinProgram rdf:datatype="http://www.w3.org/2001/XMLSchema#short">7</semesterinProgram>
    </owl:NamedIndividual>
    


    <!-- http://xworks.gr/ontologies/ccso#TP80/IE_BSc/IED/STEF/TEIC -->

    <owl:NamedIndividual rdf:about="http://xworks.gr/ontologies/ccso#TP80/IE_BSc/IED/STEF/TEIC">
        <rdf:type rdf:resource="http://xworks.gr/ontologies/ccso#Course"/>
        <includedIn rdf:resource="http://xworks.gr/ontologies/ccso#BSc_Informatics_Engineering/IE_BSc/IED/STEF/TEIC"/>
        <offeredBy rdf:resource="http://xworks.gr/ontologies/ccso#Department_of_Informatics_Engineering_of_TEI_of_Crete"/>
        <courseType rdf:datatype="http://www.w3.org/2001/XMLSchema#string">Core</courseType>
        <csName rdf:datatype="http://www.w3.org/2001/XMLSchema#string">Bachelor Thesis</csName>
    </owl:NamedIndividual>
    


    <!-- 
    ///////////////////////////////////////////////////////////////////////////////////////
    //
    // Annotations
    //
    ///////////////////////////////////////////////////////////////////////////////////////
     -->

    <rdf:Description rdf:about="http://xworks.gr/ontologies/ccso#Papadakis_Nikolaos">
        <rdfs:label xml:lang="en">Papadakis Nikos</rdfs:label>
    </rdf:Description>
    


    <!-- 
    ///////////////////////////////////////////////////////////////////////////////////////
    //
    // Rules
    //
    ///////////////////////////////////////////////////////////////////////////////////////
     -->

    <rdf:Description rdf:about="urn:swrl#AST">
        <rdf:type rdf:resource="http://www.w3.org/2003/11/swrl#Variable"/>
    </rdf:Description>
    <rdf:Description rdf:about="urn:swrl#SL">
        <rdf:type rdf:resource="http://www.w3.org/2003/11/swrl#Variable"/>
    </rdf:Description>
    <rdf:Description rdf:about="urn:swrl#CS">
        <rdf:type rdf:resource="http://www.w3.org/2003/11/swrl#Variable"/>
    </rdf:Description>
    <rdf:Description rdf:about="urn:swrl#PS">
        <rdf:type rdf:resource="http://www.w3.org/2003/11/swrl#Variable"/>
    </rdf:Description>
    <rdf:Description rdf:about="urn:swrl#DPT">
        <rdf:type rdf:resource="http://www.w3.org/2003/11/swrl#Variable"/>
    </rdf:Description>
    <rdf:Description rdf:about="urn:swrl#SYL">
        <rdf:type rdf:resource="http://www.w3.org/2003/11/swrl#Variable"/>
    </rdf:Description>
    <rdf:Description rdf:about="urn:swrl#EV">
        <rdf:type rdf:resource="http://www.w3.org/2003/11/swrl#Variable"/>
    </rdf:Description>
    <rdf:Description rdf:about="urn:swrl#LO">
        <rdf:type rdf:resource="http://www.w3.org/2003/11/swrl#Variable"/>
    </rdf:Description>
    <rdf:Description rdf:about="urn:swrl#PER">
        <rdf:type rdf:resource="http://www.w3.org/2003/11/swrl#Variable"/>
    </rdf:Description>
    <rdf:Description rdf:about="urn:swrl#PF">
        <rdf:type rdf:resource="http://www.w3.org/2003/11/swrl#Variable"/>
    </rdf:Description>
    <rdf:Description rdf:about="urn:swrl#TP">
        <rdf:type rdf:resource="http://www.w3.org/2003/11/swrl#Variable"/>
    </rdf:Description>
    <rdf:Description>
        <rdfs:comment xml:lang="en">An Assistant (AST) that is instructor in a course (CS) which is included in a program of study (PS) which is provided by a Department (DPT) 
THEN
the Department (DPT) has employee the Professor (PF)</rdfs:comment>
        <rdf:type rdf:resource="http://www.w3.org/2003/11/swrl#Imp"/>
        <swrl:body>
            <rdf:Description>
                <rdf:type rdf:resource="http://www.w3.org/2003/11/swrl#AtomList"/>
                <rdf:first>
                    <rdf:Description>
                        <rdf:type rdf:resource="http://www.w3.org/2003/11/swrl#IndividualPropertyAtom"/>
                        <swrl:propertyPredicate rdf:resource="http://xworks.gr/ontologies/ccso#assistsInCourse"/>
                        <swrl:argument1 rdf:resource="urn:swrl#AST"/>
                        <swrl:argument2 rdf:resource="urn:swrl#SL"/>
                    </rdf:Description>
                </rdf:first>
                <rdf:rest>
                    <rdf:Description>
                        <rdf:type rdf:resource="http://www.w3.org/2003/11/swrl#AtomList"/>
                        <rdf:first>
                            <rdf:Description>
                                <rdf:type rdf:resource="http://www.w3.org/2003/11/swrl#IndividualPropertyAtom"/>
                                <swrl:propertyPredicate rdf:resource="http://xworks.gr/ontologies/ccso#hasSyllabus"/>
                                <swrl:argument1 rdf:resource="urn:swrl#CS"/>
                                <swrl:argument2 rdf:resource="urn:swrl#SL"/>
                            </rdf:Description>
                        </rdf:first>
                        <rdf:rest>
                            <rdf:Description>
                                <rdf:type rdf:resource="http://www.w3.org/2003/11/swrl#AtomList"/>
                                <rdf:first>
                                    <rdf:Description>
                                        <rdf:type rdf:resource="http://www.w3.org/2003/11/swrl#IndividualPropertyAtom"/>
                                        <swrl:propertyPredicate rdf:resource="http://xworks.gr/ontologies/ccso#includesCourse"/>
                                        <swrl:argument1 rdf:resource="urn:swrl#PS"/>
                                        <swrl:argument2 rdf:resource="urn:swrl#CS"/>
                                    </rdf:Description>
                                </rdf:first>
                                <rdf:rest>
                                    <rdf:Description>
                                        <rdf:type rdf:resource="http://www.w3.org/2003/11/swrl#AtomList"/>
                                        <rdf:first>
                                            <rdf:Description>
                                                <rdf:type rdf:resource="http://www.w3.org/2003/11/swrl#IndividualPropertyAtom"/>
                                                <swrl:propertyPredicate rdf:resource="http://xworks.gr/ontologies/ccso#providesProgram"/>
                                                <swrl:argument1 rdf:resource="urn:swrl#DPT"/>
                                                <swrl:argument2 rdf:resource="urn:swrl#PS"/>
                                            </rdf:Description>
                                        </rdf:first>
                                        <rdf:rest rdf:resource="http://www.w3.org/1999/02/22-rdf-syntax-ns#nil"/>
                                    </rdf:Description>
                                </rdf:rest>
                            </rdf:Description>
                        </rdf:rest>
                    </rdf:Description>
                </rdf:rest>
            </rdf:Description>
        </swrl:body>
        <swrl:head>
            <rdf:Description>
                <rdf:type rdf:resource="http://www.w3.org/2003/11/swrl#AtomList"/>
                <rdf:first>
                    <rdf:Description>
                        <rdf:type rdf:resource="http://www.w3.org/2003/11/swrl#IndividualPropertyAtom"/>
                        <swrl:propertyPredicate rdf:resource="http://xworks.gr/ontologies/ccso#hasEmployee"/>
                        <swrl:argument1 rdf:resource="urn:swrl#DPT"/>
                        <swrl:argument2 rdf:resource="urn:swrl#AST"/>
                    </rdf:Description>
                </rdf:first>
                <rdf:rest rdf:resource="http://www.w3.org/1999/02/22-rdf-syntax-ns#nil"/>
            </rdf:Description>
        </swrl:head>
    </rdf:Description>
    <rdf:Description>
        <rdfs:comment xml:lang="en">When a Syllabus (Course)(SYL) has an Event (EV) that expects a LearningOutcome (LO)
THEN the Syllabus (Course)(SYL) aims to that LearningOutcome (LO)</rdfs:comment>
        <rdf:type rdf:resource="http://www.w3.org/2003/11/swrl#Imp"/>
        <swrl:body>
            <rdf:Description>
                <rdf:type rdf:resource="http://www.w3.org/2003/11/swrl#AtomList"/>
                <rdf:first>
                    <rdf:Description>
                        <rdf:type rdf:resource="http://www.w3.org/2003/11/swrl#IndividualPropertyAtom"/>
                        <swrl:propertyPredicate rdf:resource="http://xworks.gr/ontologies/ccso#hasEvent"/>
                        <swrl:argument1 rdf:resource="urn:swrl#SYL"/>
                        <swrl:argument2 rdf:resource="urn:swrl#EV"/>
                    </rdf:Description>
                </rdf:first>
                <rdf:rest>
                    <rdf:Description>
                        <rdf:type rdf:resource="http://www.w3.org/2003/11/swrl#AtomList"/>
                        <rdf:first>
                            <rdf:Description>
                                <rdf:type rdf:resource="http://www.w3.org/2003/11/swrl#IndividualPropertyAtom"/>
                                <swrl:propertyPredicate rdf:resource="http://xworks.gr/ontologies/ccso#expectsLO"/>
                                <swrl:argument1 rdf:resource="urn:swrl#EV"/>
                                <swrl:argument2 rdf:resource="urn:swrl#LO"/>
                            </rdf:Description>
                        </rdf:first>
                        <rdf:rest rdf:resource="http://www.w3.org/1999/02/22-rdf-syntax-ns#nil"/>
                    </rdf:Description>
                </rdf:rest>
            </rdf:Description>
        </swrl:body>
        <swrl:head>
            <rdf:Description>
                <rdf:type rdf:resource="http://www.w3.org/2003/11/swrl#AtomList"/>
                <rdf:first>
                    <rdf:Description>
                        <rdf:type rdf:resource="http://www.w3.org/2003/11/swrl#IndividualPropertyAtom"/>
                        <swrl:propertyPredicate rdf:resource="http://xworks.gr/ontologies/ccso#aimsToLO"/>
                        <swrl:argument1 rdf:resource="urn:swrl#SYL"/>
                        <swrl:argument2 rdf:resource="urn:swrl#LO"/>
                    </rdf:Description>
                </rdf:first>
                <rdf:rest rdf:resource="http://www.w3.org/1999/02/22-rdf-syntax-ns#nil"/>
            </rdf:Description>
        </swrl:head>
    </rdf:Description>
    <rdf:Description>
        <rdfs:comment xml:lang="en">A Person (PER), who has Degree (PS) that provided by a Department (DPT) 
IS Alumnus of that Department (DPT)</rdfs:comment>
        <rdf:type rdf:resource="http://www.w3.org/2003/11/swrl#Imp"/>
        <swrl:body>
            <rdf:Description>
                <rdf:type rdf:resource="http://www.w3.org/2003/11/swrl#AtomList"/>
                <rdf:first>
                    <rdf:Description>
                        <rdf:type rdf:resource="http://www.w3.org/2003/11/swrl#IndividualPropertyAtom"/>
                        <swrl:propertyPredicate rdf:resource="http://xworks.gr/ontologies/ccso#hasDegree"/>
                        <swrl:argument1 rdf:resource="urn:swrl#PER"/>
                        <swrl:argument2 rdf:resource="urn:swrl#PS"/>
                    </rdf:Description>
                </rdf:first>
                <rdf:rest>
                    <rdf:Description>
                        <rdf:type rdf:resource="http://www.w3.org/2003/11/swrl#AtomList"/>
                        <rdf:first>
                            <rdf:Description>
                                <rdf:type rdf:resource="http://www.w3.org/2003/11/swrl#IndividualPropertyAtom"/>
                                <swrl:propertyPredicate rdf:resource="http://xworks.gr/ontologies/ccso#providedBy"/>
                                <swrl:argument1 rdf:resource="urn:swrl#PS"/>
                                <swrl:argument2 rdf:resource="urn:swrl#DPT"/>
                            </rdf:Description>
                        </rdf:first>
                        <rdf:rest rdf:resource="http://www.w3.org/1999/02/22-rdf-syntax-ns#nil"/>
                    </rdf:Description>
                </rdf:rest>
            </rdf:Description>
        </swrl:body>
        <swrl:head>
            <rdf:Description>
                <rdf:type rdf:resource="http://www.w3.org/2003/11/swrl#AtomList"/>
                <rdf:first>
                    <rdf:Description>
                        <rdf:type rdf:resource="http://www.w3.org/2003/11/swrl#IndividualPropertyAtom"/>
                        <swrl:propertyPredicate rdf:resource="http://xworks.gr/ontologies/ccso#alumnusOf"/>
                        <swrl:argument1 rdf:resource="urn:swrl#PER"/>
                        <swrl:argument2 rdf:resource="urn:swrl#DPT"/>
                    </rdf:Description>
                </rdf:first>
                <rdf:rest rdf:resource="http://www.w3.org/1999/02/22-rdf-syntax-ns#nil"/>
            </rdf:Description>
        </swrl:head>
    </rdf:Description>
    <rdf:Description>
        <rdfs:comment xml:lang="en">A Professor (PF) that teaches in an Event (EV) for a course (CS) which is included in a program of study (PS) which is provided by a Department (DPT) 
THEN
the Department (DPT) has Academic Staff that Professor (PF)</rdfs:comment>
        <rdf:type rdf:resource="http://www.w3.org/2003/11/swrl#Imp"/>
        <swrl:body>
            <rdf:Description>
                <rdf:type rdf:resource="http://www.w3.org/2003/11/swrl#AtomList"/>
                <rdf:first>
                    <rdf:Description>
                        <rdf:type rdf:resource="http://www.w3.org/2003/11/swrl#IndividualPropertyAtom"/>
                        <swrl:propertyPredicate rdf:resource="http://xworks.gr/ontologies/ccso#teachesIn"/>
                        <swrl:argument1 rdf:resource="urn:swrl#PF"/>
                        <swrl:argument2 rdf:resource="urn:swrl#EV"/>
                    </rdf:Description>
                </rdf:first>
                <rdf:rest>
                    <rdf:Description>
                        <rdf:type rdf:resource="http://www.w3.org/2003/11/swrl#AtomList"/>
                        <rdf:first>
                            <rdf:Description>
                                <rdf:type rdf:resource="http://www.w3.org/2003/11/swrl#IndividualPropertyAtom"/>
                                <swrl:propertyPredicate rdf:resource="http://xworks.gr/ontologies/ccso#hasEvent"/>
                                <swrl:argument1 rdf:resource="urn:swrl#SL"/>
                                <swrl:argument2 rdf:resource="urn:swrl#EV"/>
                            </rdf:Description>
                        </rdf:first>
                        <rdf:rest rdf:resource="http://www.w3.org/1999/02/22-rdf-syntax-ns#nil"/>
                    </rdf:Description>
                </rdf:rest>
            </rdf:Description>
        </swrl:body>
        <swrl:head>
            <rdf:Description>
                <rdf:type rdf:resource="http://www.w3.org/2003/11/swrl#AtomList"/>
                <rdf:first>
                    <rdf:Description>
                        <rdf:type rdf:resource="http://www.w3.org/2003/11/swrl#IndividualPropertyAtom"/>
                        <swrl:propertyPredicate rdf:resource="http://xworks.gr/ontologies/ccso#hasInstructor"/>
                        <swrl:argument1 rdf:resource="urn:swrl#SL"/>
                        <swrl:argument2 rdf:resource="urn:swrl#PF"/>
                    </rdf:Description>
                </rdf:first>
                <rdf:rest rdf:resource="http://www.w3.org/1999/02/22-rdf-syntax-ns#nil"/>
            </rdf:Description>
        </swrl:head>
    </rdf:Description>
    <rdf:Description>
        <rdfs:comment xml:lang="en">When a Syllabus (Course)(SYL) has an Event (EV) that covers a Topic (TP)
THEN the Syllabus (Course)(SYL) covers that Topic (TP)</rdfs:comment>
        <rdf:type rdf:resource="http://www.w3.org/2003/11/swrl#Imp"/>
        <swrl:body>
            <rdf:Description>
                <rdf:type rdf:resource="http://www.w3.org/2003/11/swrl#AtomList"/>
                <rdf:first>
                    <rdf:Description>
                        <rdf:type rdf:resource="http://www.w3.org/2003/11/swrl#IndividualPropertyAtom"/>
                        <swrl:propertyPredicate rdf:resource="http://xworks.gr/ontologies/ccso#hasEvent"/>
                        <swrl:argument1 rdf:resource="urn:swrl#SYL"/>
                        <swrl:argument2 rdf:resource="urn:swrl#EV"/>
                    </rdf:Description>
                </rdf:first>
                <rdf:rest>
                    <rdf:Description>
                        <rdf:type rdf:resource="http://www.w3.org/2003/11/swrl#AtomList"/>
                        <rdf:first>
                            <rdf:Description>
                                <rdf:type rdf:resource="http://www.w3.org/2003/11/swrl#IndividualPropertyAtom"/>
                                <swrl:propertyPredicate rdf:resource="http://xworks.gr/ontologies/ccso#hasTopic"/>
                                <swrl:argument1 rdf:resource="urn:swrl#EV"/>
                                <swrl:argument2 rdf:resource="urn:swrl#TP"/>
                            </rdf:Description>
                        </rdf:first>
                        <rdf:rest rdf:resource="http://www.w3.org/1999/02/22-rdf-syntax-ns#nil"/>
                    </rdf:Description>
                </rdf:rest>
            </rdf:Description>
        </swrl:body>
        <swrl:head>
            <rdf:Description>
                <rdf:type rdf:resource="http://www.w3.org/2003/11/swrl#AtomList"/>
                <rdf:first>
                    <rdf:Description>
                        <rdf:type rdf:resource="http://www.w3.org/2003/11/swrl#IndividualPropertyAtom"/>
                        <swrl:propertyPredicate rdf:resource="http://xworks.gr/ontologies/ccso#coversTopic"/>
                        <swrl:argument1 rdf:resource="urn:swrl#SYL"/>
                        <swrl:argument2 rdf:resource="urn:swrl#TP"/>
                    </rdf:Description>
                </rdf:first>
                <rdf:rest rdf:resource="http://www.w3.org/1999/02/22-rdf-syntax-ns#nil"/>
            </rdf:Description>
        </swrl:head>
    </rdf:Description>
    <rdf:Description>
        <rdfs:comment xml:lang="en">A Professor (PF) that is instructor in a course (CS) which is included in a program of study (PS) which is provided by a Department (DPT) 
THEN
that Professor (PF) is member of the Academic Staff of the Department (DPT)</rdfs:comment>
        <rdf:type rdf:resource="http://www.w3.org/2003/11/swrl#Imp"/>
        <swrl:body>
            <rdf:Description>
                <rdf:type rdf:resource="http://www.w3.org/2003/11/swrl#AtomList"/>
                <rdf:first>
                    <rdf:Description>
                        <rdf:type rdf:resource="http://www.w3.org/2003/11/swrl#IndividualPropertyAtom"/>
                        <swrl:propertyPredicate rdf:resource="http://xworks.gr/ontologies/ccso#instructorOf"/>
                        <swrl:argument1 rdf:resource="urn:swrl#PF"/>
                        <swrl:argument2 rdf:resource="urn:swrl#SL"/>
                    </rdf:Description>
                </rdf:first>
                <rdf:rest>
                    <rdf:Description>
                        <rdf:type rdf:resource="http://www.w3.org/2003/11/swrl#AtomList"/>
                        <rdf:first>
                            <rdf:Description>
                                <rdf:type rdf:resource="http://www.w3.org/2003/11/swrl#IndividualPropertyAtom"/>
                                <swrl:propertyPredicate rdf:resource="http://xworks.gr/ontologies/ccso#hasSyllabus"/>
                                <swrl:argument1 rdf:resource="urn:swrl#CS"/>
                                <swrl:argument2 rdf:resource="urn:swrl#SL"/>
                            </rdf:Description>
                        </rdf:first>
                        <rdf:rest>
                            <rdf:Description>
                                <rdf:type rdf:resource="http://www.w3.org/2003/11/swrl#AtomList"/>
                                <rdf:first>
                                    <rdf:Description>
                                        <rdf:type rdf:resource="http://www.w3.org/2003/11/swrl#IndividualPropertyAtom"/>
                                        <swrl:propertyPredicate rdf:resource="http://xworks.gr/ontologies/ccso#includesCourse"/>
                                        <swrl:argument1 rdf:resource="urn:swrl#PS"/>
                                        <swrl:argument2 rdf:resource="urn:swrl#CS"/>
                                    </rdf:Description>
                                </rdf:first>
                                <rdf:rest>
                                    <rdf:Description>
                                        <rdf:type rdf:resource="http://www.w3.org/2003/11/swrl#AtomList"/>
                                        <rdf:first>
                                            <rdf:Description>
                                                <rdf:type rdf:resource="http://www.w3.org/2003/11/swrl#IndividualPropertyAtom"/>
                                                <swrl:propertyPredicate rdf:resource="http://xworks.gr/ontologies/ccso#providesProgram"/>
                                                <swrl:argument1 rdf:resource="urn:swrl#DPT"/>
                                                <swrl:argument2 rdf:resource="urn:swrl#PS"/>
                                            </rdf:Description>
                                        </rdf:first>
                                        <rdf:rest rdf:resource="http://www.w3.org/1999/02/22-rdf-syntax-ns#nil"/>
                                    </rdf:Description>
                                </rdf:rest>
                            </rdf:Description>
                        </rdf:rest>
                    </rdf:Description>
                </rdf:rest>
            </rdf:Description>
        </swrl:body>
        <swrl:head>
            <rdf:Description>
                <rdf:type rdf:resource="http://www.w3.org/2003/11/swrl#AtomList"/>
                <rdf:first>
                    <rdf:Description>
                        <rdf:type rdf:resource="http://www.w3.org/2003/11/swrl#IndividualPropertyAtom"/>
                        <swrl:propertyPredicate rdf:resource="http://xworks.gr/ontologies/ccso#hasAcademicStaff"/>
                        <swrl:argument1 rdf:resource="urn:swrl#DPT"/>
                        <swrl:argument2 rdf:resource="urn:swrl#PF"/>
                    </rdf:Description>
                </rdf:first>
                <rdf:rest rdf:resource="http://www.w3.org/1999/02/22-rdf-syntax-ns#nil"/>
            </rdf:Description>
        </swrl:head>
    </rdf:Description>
    <rdf:Description>
        <rdfs:comment xml:lang="en">A Professor (PF) that is instructor in a course (CS) which is included in a program of study (PS) which is provided by a Department (DPT) 
THEN
the Department (DPT) has employee the Professor (PF)</rdfs:comment>
        <rdf:type rdf:resource="http://www.w3.org/2003/11/swrl#Imp"/>
        <swrl:body>
            <rdf:Description>
                <rdf:type rdf:resource="http://www.w3.org/2003/11/swrl#AtomList"/>
                <rdf:first>
                    <rdf:Description>
                        <rdf:type rdf:resource="http://www.w3.org/2003/11/swrl#IndividualPropertyAtom"/>
                        <swrl:propertyPredicate rdf:resource="http://xworks.gr/ontologies/ccso#instructorOf"/>
                        <swrl:argument1 rdf:resource="urn:swrl#PF"/>
                        <swrl:argument2 rdf:resource="urn:swrl#SL"/>
                    </rdf:Description>
                </rdf:first>
                <rdf:rest>
                    <rdf:Description>
                        <rdf:type rdf:resource="http://www.w3.org/2003/11/swrl#AtomList"/>
                        <rdf:first>
                            <rdf:Description>
                                <rdf:type rdf:resource="http://www.w3.org/2003/11/swrl#IndividualPropertyAtom"/>
                                <swrl:propertyPredicate rdf:resource="http://xworks.gr/ontologies/ccso#hasSyllabus"/>
                                <swrl:argument1 rdf:resource="urn:swrl#CS"/>
                                <swrl:argument2 rdf:resource="urn:swrl#SL"/>
                            </rdf:Description>
                        </rdf:first>
                        <rdf:rest>
                            <rdf:Description>
                                <rdf:type rdf:resource="http://www.w3.org/2003/11/swrl#AtomList"/>
                                <rdf:first>
                                    <rdf:Description>
                                        <rdf:type rdf:resource="http://www.w3.org/2003/11/swrl#IndividualPropertyAtom"/>
                                        <swrl:propertyPredicate rdf:resource="http://xworks.gr/ontologies/ccso#includesCourse"/>
                                        <swrl:argument1 rdf:resource="urn:swrl#PS"/>
                                        <swrl:argument2 rdf:resource="urn:swrl#CS"/>
                                    </rdf:Description>
                                </rdf:first>
                                <rdf:rest>
                                    <rdf:Description>
                                        <rdf:type rdf:resource="http://www.w3.org/2003/11/swrl#AtomList"/>
                                        <rdf:first>
                                            <rdf:Description>
                                                <rdf:type rdf:resource="http://www.w3.org/2003/11/swrl#IndividualPropertyAtom"/>
                                                <swrl:propertyPredicate rdf:resource="http://xworks.gr/ontologies/ccso#providesProgram"/>
                                                <swrl:argument1 rdf:resource="urn:swrl#DPT"/>
                                                <swrl:argument2 rdf:resource="urn:swrl#PS"/>
                                            </rdf:Description>
                                        </rdf:first>
                                        <rdf:rest rdf:resource="http://www.w3.org/1999/02/22-rdf-syntax-ns#nil"/>
                                    </rdf:Description>
                                </rdf:rest>
                            </rdf:Description>
                        </rdf:rest>
                    </rdf:Description>
                </rdf:rest>
            </rdf:Description>
        </swrl:body>
        <swrl:head>
            <rdf:Description>
                <rdf:type rdf:resource="http://www.w3.org/2003/11/swrl#AtomList"/>
                <rdf:first>
                    <rdf:Description>
                        <rdf:type rdf:resource="http://www.w3.org/2003/11/swrl#IndividualPropertyAtom"/>
                        <swrl:propertyPredicate rdf:resource="http://xworks.gr/ontologies/ccso#hasEmployee"/>
                        <swrl:argument1 rdf:resource="urn:swrl#DPT"/>
                        <swrl:argument2 rdf:resource="urn:swrl#PF"/>
                    </rdf:Description>
                </rdf:first>
                <rdf:rest rdf:resource="http://www.w3.org/1999/02/22-rdf-syntax-ns#nil"/>
            </rdf:Description>
        </swrl:head>
    </rdf:Description>
    <rdf:Description>
        <rdfs:comment xml:lang="en">A Course (CS) that is included in a ProgramofStudy (PS) which is provided by a Department (DPT) 
IS offered by that Department (DPT)</rdfs:comment>
        <rdf:type rdf:resource="http://www.w3.org/2003/11/swrl#Imp"/>
        <swrl:body>
            <rdf:Description>
                <rdf:type rdf:resource="http://www.w3.org/2003/11/swrl#AtomList"/>
                <rdf:first>
                    <rdf:Description>
                        <rdf:type rdf:resource="http://www.w3.org/2003/11/swrl#IndividualPropertyAtom"/>
                        <swrl:propertyPredicate rdf:resource="http://xworks.gr/ontologies/ccso#includedIn"/>
                        <swrl:argument1 rdf:resource="urn:swrl#CS"/>
                        <swrl:argument2 rdf:resource="urn:swrl#PS"/>
                    </rdf:Description>
                </rdf:first>
                <rdf:rest>
                    <rdf:Description>
                        <rdf:type rdf:resource="http://www.w3.org/2003/11/swrl#AtomList"/>
                        <rdf:first>
                            <rdf:Description>
                                <rdf:type rdf:resource="http://www.w3.org/2003/11/swrl#IndividualPropertyAtom"/>
                                <swrl:propertyPredicate rdf:resource="http://xworks.gr/ontologies/ccso#providedBy"/>
                                <swrl:argument1 rdf:resource="urn:swrl#PS"/>
                                <swrl:argument2 rdf:resource="urn:swrl#DPT"/>
                            </rdf:Description>
                        </rdf:first>
                        <rdf:rest rdf:resource="http://www.w3.org/1999/02/22-rdf-syntax-ns#nil"/>
                    </rdf:Description>
                </rdf:rest>
            </rdf:Description>
        </swrl:body>
        <swrl:head>
            <rdf:Description>
                <rdf:type rdf:resource="http://www.w3.org/2003/11/swrl#AtomList"/>
                <rdf:first>
                    <rdf:Description>
                        <rdf:type rdf:resource="http://www.w3.org/2003/11/swrl#IndividualPropertyAtom"/>
                        <swrl:propertyPredicate rdf:resource="http://xworks.gr/ontologies/ccso#offeredBy"/>
                        <swrl:argument1 rdf:resource="urn:swrl#CS"/>
                        <swrl:argument2 rdf:resource="urn:swrl#DPT"/>
                    </rdf:Description>
                </rdf:first>
                <rdf:rest rdf:resource="http://www.w3.org/1999/02/22-rdf-syntax-ns#nil"/>
            </rdf:Description>
        </swrl:head>
    </rdf:Description>
</rdf:RDF>



<!-- Generated by the OWL API (version 4.2.8.20170104-2310) https://github.com/owlcs/owlapi -->

